@prefix d3f:        <http://d3fend.mitre.org/ontologies/d3fend.owl#> .
@prefix dcterms:    <http://purl.org/dc/terms/> .
@prefix fun:        <http://w3id.org/sparql-generate/fn/> .
@prefix iter:       <http://w3id.org/sparql-generate/iter/> .
@prefix jsonschema: <https://www.w3.org/2019/wot/json-schema#> .
@prefix ocsf:       <https://schema.ocsf.io/1.3.0/ontology/> .
@prefix owl:        <http://www.w3.org/2002/07/owl#> .
@prefix rdf:        <http://www.w3.org/1999/02/22-rdf-syntax-ns#> .
@prefix rdfs:       <http://www.w3.org/2000/01/rdf-schema#> .
@prefix skos:       <http://www.w3.org/2004/02/skos/core#> .
@prefix xsd:        <http://www.w3.org/2001/XMLSchema#> .

ocsf:port  rdf:type          owl:DatatypeProperty;
        rdfs:label           "Port";
        rdfs:range           ocsf:port_t;
        dcterms:description  "The TCP/UDP port number associated with a connection. See specific usage." .

ocsf:entity  rdf:type        owl:ObjectProperty;
        rdfs:label           "Entity";
        rdfs:range           ocsf:ManagedEntity;
        dcterms:description  "The managed entity that is being acted upon." .

ocsf:mac_t  rdf:type         rdfs:Datatype;
        rdfs:label           "MAC Address";
        rdfs:subClassOf      xsd:string;
        dcterms:description  "Media Access Control (MAC) address. For example: <code>18:36:F3:98:4F:9A</code>.";
        xsd:pattern          "^([0-9A-Fa-f]{2}[:-]){5}([0-9A-Fa-f]{2})$" .

ocsf:module  rdf:type        owl:ObjectProperty;
        rdfs:label           "Module";
        rdfs:range           ocsf:Module;
        dcterms:description  "The module that pertains to the event." .

ocsf:supporting_data  rdf:type  owl:DatatypeProperty;
        rdfs:label           "Supporting Data";
        rdfs:range           ocsf:json_t;
        dcterms:description  "Additional data supporting a finding as provided by security tool" .

ocsf:ticket  rdf:type        owl:ObjectProperty;
        rdfs:label           "Ticket";
        rdfs:range           ocsf:Ticket;
        dcterms:description  "The linked ticket in the ticketing system." .

ocsf:algorithm_id  rdf:type  owl:DatatypeProperty;
        rdfs:label           "Algorithm ID";
        rdfs:range           ocsf:integer_t;
        dcterms:description  "The normalized identifier of the algorithm. See specific usage.";
        jsonschema:enum      "Other" , "Unknown" .

ocsf:client_ciphers  rdf:type  owl:DatatypeProperty;
        rdfs:label           "Client Cipher Suites";
        rdfs:range           ocsf:string_t;
        dcterms:description  "The client cipher suites that were exchanged during the TLS handshake negotiation." .

ocsf:name_servers  rdf:type  owl:DatatypeProperty;
        rdfs:label           "Name Servers";
        rdfs:range           ocsf:string_t;
        dcterms:description  "A collection of name servers related to a domain registration or other record." .

ocsf:remote_display  rdf:type  owl:ObjectProperty;
        rdfs:label           "Remote Display";
        rdfs:range           ocsf:Display;
        dcterms:description  "The remote display affiliated with the event" .

ocsf:intermediate_ips
        rdf:type             owl:DatatypeProperty;
        rdfs:label           "Intermediate IP Addresses";
        rdfs:range           ocsf:ip_t;
        dcterms:description  "The intermediate IP Addresses. For example, the IP addresses in the HTTP X-Forwarded-For header." .

ocsf:policy  rdf:type        owl:ObjectProperty;
        rdfs:label           "Policy";
        rdfs:range           ocsf:Policy;
        dcterms:description  "Describes details of a policy. See specific usage." .

ocsf:delay  rdf:type         owl:DatatypeProperty;
        rdfs:label           "Root Delay";
        rdfs:range           ocsf:integer_t;
        dcterms:description  "The total round-trip delay to the reference clock in milliseconds." .

ocsf:last_run_time  rdf:type  owl:DatatypeProperty;
        rdfs:label           "Last Run";
        rdfs:range           ocsf:timestamp_t;
        dcterms:description  "The last run time of application or service. See specific usage." .

ocsf:security_questions
        rdf:type             owl:DatatypeProperty;
        rdfs:label           "Security Questions";
        rdfs:range           ocsf:string_t;
        dcterms:description  "The question(s) provided to user for a question-based authentication factor." .

ocsf:zone  rdf:type          owl:DatatypeProperty;
        rdfs:label           "Network Zone";
        rdfs:range           ocsf:string_t;
        dcterms:description  "The network zone or LAN segment." .

ocsf:category_id  rdf:type   owl:DatatypeProperty;
        rdfs:label           "Category ID";
        rdfs:range           ocsf:integer_t;
        dcterms:description  "The normalized identifier of the object category. See specific usage." .

ocsf:phones  rdf:type        owl:DatatypeProperty;
        rdfs:label           "Phones";
        rdfs:range           ocsf:string_t;
        dcterms:description  "The phone numbers associated with the user" .

ocsf:match_location  rdf:type  owl:DatatypeProperty;
        rdfs:label           "Match Location";
        rdfs:range           ocsf:string_t;
        dcterms:description  "The location of the matched data in the source which resulted in the triggered firewall rule. For example: HEADER." .

ocsf:risk_details  rdf:type  owl:DatatypeProperty;
        rdfs:label           "Risk Details";
        rdfs:range           ocsf:string_t;
        dcterms:description  "Describes the risk associated with the finding." .

ocsf:authorizations  rdf:type  owl:ObjectProperty;
        rdfs:label           "Authorization Information";
        rdfs:range           ocsf:AuthorizationResult;
        dcterms:description  "Provides details about an authorization, such as authorization outcome, and any associated policies related to the activity/event." .

ocsf:boundary  rdf:type      owl:DatatypeProperty;
        rdfs:label           "Boundary";
        rdfs:range           ocsf:string_t;
        dcterms:description  "The boundary of the connection, normalized to the caption of 'boundary_id'. In the case of 'Other', it is defined by the event source. <p> For cloud connections, this translates to the traffic-boundary(same VPC, through IGW, etc.). For traditional networks, this is described as Local, Internal, or External.</p>" .

ocsf:phase_id  rdf:type      owl:DatatypeProperty;
        rdfs:label           "Kill Chain Phase ID";
        rdfs:range           ocsf:integer_t;
        dcterms:description  "The cyber kill chain phase identifier.";
        jsonschema:enum      "Unknown" , "Exploitation" , "Delivery" , "Command & Control" , "Reconnaissance" , "Installation" , "Actions on Objectives" , "Weaponization" , "Other" .

ocsf:duration_mins  rdf:type  owl:DatatypeProperty;
        rdfs:label           "Duration Minutes";
        rdfs:range           ocsf:integer_t;
        dcterms:description  "Represents the duration of the activity in minutes. See specific usage." .

ocsf:physical_width  rdf:type  owl:DatatypeProperty;
        rdfs:label           "Physical Width";
        rdfs:range           ocsf:integer_t;
        dcterms:description  "The numeric physical width of display." .

ocsf:category_name  rdf:type  owl:DatatypeProperty;
        rdfs:label           "Category";
        rdfs:range           ocsf:string_t;
        dcterms:description  "The event category name, as defined by category_uid value." .

ocsf:policies  rdf:type      owl:ObjectProperty;
        rdfs:label           "Policies";
        rdfs:range           ocsf:Policy;
        dcterms:description  "An array of <code>Policy</code> objects." .

ocsf:parent_folder  rdf:type  owl:DatatypeProperty;
        rdfs:label           "Parent Folder";
        rdfs:range           ocsf:string_t;
        dcterms:description  "The parent folder in which the file resides. For example: <code>c:\\windows\\system32</code>" .

ocsf:hostname_t  rdf:type    rdfs:Datatype;
        rdfs:label           "Hostname";
        rdfs:subClassOf      xsd:string;
        dcterms:description  "Unique name assigned to a device connected to a computer network. A domain name in general is an Internet address that can be resolved through the Domain Name System (DNS). For example: <code>r2-d2.example.com</code>.";
        xsd:pattern          "^(([a-zA-Z0-9]|[a-zA-Z0-9][a-zA-Z0-9\\-]*[a-zA-Z0-9])\\.)*([A-Za-z0-9]|[A-Za-z0-9][A-Za-z0-9\\-]*[A-Za-z0-9])$" .

ocsf:activity_id  rdf:type   owl:DatatypeProperty;
        rdfs:label           "Activity ID";
        rdfs:range           ocsf:integer_t;
        dcterms:description  "The normalized identifier of the activity that triggered the event.";
        jsonschema:enum      "Other" , "Unknown" .

ocsf:analytic  rdf:type      owl:ObjectProperty;
        rdfs:label           "Analytic";
        rdfs:range           ocsf:Analytic;
        dcterms:description  "The analytic technique used to analyze and derive insights from the data or information that led to the finding or conclusion." .

ocsf:email_uid  rdf:type     owl:DatatypeProperty;
        rdfs:label           "Email UID";
        rdfs:range           ocsf:string_t;
        dcterms:description  "The unique identifier of the email, used to correlate related email alert and activity events." .

ocsf:phase  rdf:type         owl:DatatypeProperty;
        rdfs:label           "Kill Chain Phase";
        rdfs:range           ocsf:string_t;
        dcterms:description  "The cyber kill chain phase." .

ocsf:is_self_signed  rdf:type  owl:DatatypeProperty;
        rdfs:label           "Certificate Self-Signed";
        rdfs:range           ocsf:boolean_t;
        dcterms:description  "Denotes whether a digital certificate is self-signed or signed by a known certificate authority (CA)." .

ocsf:criticality  rdf:type   owl:DatatypeProperty;
        rdfs:label           "Criticality";
        rdfs:range           ocsf:string_t;
        dcterms:description  "Criticality of a resource/object in question" .

ocsf:is_mfa  rdf:type        owl:DatatypeProperty;
        rdfs:label           "Multi Factor Authentication";
        rdfs:range           ocsf:boolean_t;
        dcterms:description  "Indicates whether Multi Factor Authentication was used during authentication." .

ocsf:bios_ver  rdf:type      owl:DatatypeProperty;
        rdfs:label           "BIOS Version";
        rdfs:range           ocsf:string_t;
        dcterms:description  "The BIOS version. For example: <code>LENOVO G5ETA2WW (2.62)</code>." .

ocsf:subnet  rdf:type        owl:DatatypeProperty;
        rdfs:label           "Subnet";
        rdfs:range           ocsf:subnet_t;
        dcterms:description  "The subnet mask." .

ocsf:impact_score  rdf:type  owl:DatatypeProperty;
        rdfs:label           "Impact";
        rdfs:range           ocsf:integer_t;
        dcterms:description  "The impact of the finding, valid range 0-100." .

ocsf:start_line  rdf:type    owl:DatatypeProperty;
        rdfs:label           "Start Line";
        rdfs:range           ocsf:integer_t;
        dcterms:description  "The line number of the first line of code block identified as vulnerable." .

ocsf:subject  rdf:type       owl:DatatypeProperty;
        rdfs:label           "Subject Details";
        rdfs:range           ocsf:string_t;
        dcterms:description  "The identifier of the subject. See specific usage." .

ocsf:path  rdf:type          owl:DatatypeProperty;
        rdfs:label           "Path";
        rdfs:range           ocsf:string_t;
        dcterms:description  "The path that pertains to the event or object. See specific usage." .

ocsf:confidence_score
        rdf:type             owl:DatatypeProperty;
        rdfs:label           "Confidence Score";
        rdfs:range           ocsf:integer_t;
        dcterms:description  "The confidence score as reported by the event source." .

ocsf:file_name_t  rdf:type   rdfs:Datatype;
        rdfs:label           "File Name";
        rdfs:subClassOf      xsd:string;
        dcterms:description  "File name. For example: <code>text-file.txt</code>." .

ocsf:number  rdf:type        owl:DatatypeProperty;
        rdfs:label           "Number";
        rdfs:range           ocsf:integer_t;
        dcterms:description  "The number of the entity. See specific usage." .

ocsf:keyboard_info  rdf:type  owl:ObjectProperty;
        rdfs:label           "Keyboard Information";
        rdfs:range           ocsf:KeyboardInformation;
        dcterms:description  "The keyboard detailed information." .

ocsf:smtp_from  rdf:type     owl:DatatypeProperty;
        rdfs:label           "SMTP From";
        rdfs:range           ocsf:email_t;
        dcterms:description  "The value of the SMTP MAIL FROM command." .

ocsf:is_system  rdf:type     owl:DatatypeProperty;
        rdfs:label           "System";
        rdfs:range           ocsf:boolean_t;
        dcterms:description  "The indication of whether the object is part of the operating system." .

ocsf:terminated_time  rdf:type  owl:DatatypeProperty;
        rdfs:label           "Terminated Time";
        rdfs:range           ocsf:timestamp_t;
        dcterms:description  "The time when the entity was terminated. See specific usage." .

ocsf:xattributes  rdf:type   owl:ObjectProperty;
        rdfs:label           "Extended Attributes";
        rdfs:range           ocsf:Object;
        dcterms:description  "An unordered collection of zero or more name/value pairs where each pair represents a file or folder extended attribute.</p>For example: Windows alternate data stream attributes (ADS stream name, ADS size, etc.), user-defined or application-defined attributes, ACL, owner, primary group, etc. Examples from DCS: </p><ul><li><strong>ads_name</strong></li><li><strong>ads_size</strong></li><li><strong>dacl</strong></li><li><strong>owner</strong></li><li><strong>primary_group</strong></li><li><strong>link_name</strong> - name of the link associated to the file.</li><li><strong>hard_link_count</strong> - the number of links that are associated to the file.</li></ul>" .

ocsf:ja3s_hash  rdf:type     owl:ObjectProperty;
        rdfs:label           "JA3S Hash";
        rdfs:range           ocsf:Fingerprint;
        dcterms:description  "The MD5 hash of a JA3S string." .

ocsf:verdict  rdf:type       owl:DatatypeProperty;
        rdfs:label           "Verdict";
        rdfs:range           ocsf:string_t;
        dcterms:description  "The verdict assigned to an Incident finding." .

ocsf:condition  rdf:type     owl:DatatypeProperty;
        rdfs:label           "Condition";
        rdfs:range           ocsf:string_t;
        dcterms:description  "The rule trigger condition for the rule. For example: SQL_INJECTION." .

ocsf:modifier  rdf:type      owl:ObjectProperty;
        rdfs:label           "Modifier";
        rdfs:range           ocsf:User;
        dcterms:description  "The user that last modified the object associated with the event. See specific usage." .

ocsf:invoked_by  rdf:type    owl:DatatypeProperty;
        rdfs:label           "Invoked by";
        rdfs:range           ocsf:string_t;
        dcterms:description  "The name of the service that invoked the activity as described in the event." .

ocsf:log_type  rdf:type      owl:DatatypeProperty;
        rdfs:label           "Log Type";
        rdfs:range           ocsf:string_t;
        dcterms:description  "The log type, normalized to the caption of the <code>log_type_id</code> value. In the case of 'Other', it is defined by the event source." .

ocsf:sensitivity  rdf:type   owl:DatatypeProperty;
        rdfs:label           "Sensitivity";
        rdfs:range           ocsf:string_t;
        dcterms:description  "The sensitivity of the firewall rule in the matched event. For example: HIGH." .

ocsf:package_manager  rdf:type  owl:DatatypeProperty;
        rdfs:label           "Package Manager";
        rdfs:range           ocsf:string_t;
        dcterms:description  "The software packager manager utilized to manage a package on a system, e.g. npm, yum, dpkg etc." .

ocsf:labels  rdf:type        owl:DatatypeProperty;
        rdfs:label           "Labels";
        rdfs:range           ocsf:string_t;
        dcterms:description  "The list of labels attached to an event, object, or attribute." .

ocsf:data  rdf:type          owl:DatatypeProperty;
        rdfs:label           "Data";
        rdfs:range           ocsf:json_t;
        dcterms:description  "The additional data that is associated with the event or object. See specific usage." .

ocsf:username_t  rdf:type    rdfs:Datatype;
        rdfs:label           "User Name";
        rdfs:subClassOf      xsd:string;
        dcterms:description  "User name. For example: <code>john_doe</code>." .

ocsf:args  rdf:type          owl:DatatypeProperty;
        rdfs:label           "HTTP Arguments";
        rdfs:range           ocsf:string_t;
        dcterms:description  "The arguments sent along with the HTTP request." .

ocsf:type  rdf:type          owl:DatatypeProperty;
        rdfs:label           "Type";
        rdfs:range           ocsf:string_t;
        dcterms:description  "The type of an object or value, normalized to the caption of the type_id value. In the case of 'Other', it is defined by the event source. See specific usage." .

ocsf:table  rdf:type         owl:ObjectProperty;
        rdfs:label           "Table";
        rdfs:range           ocsf:Table;
        dcterms:description  "The table object represents a table within a structured relational database or datastore, which contains columns and rows of data that are able to be create, updated, deleted and queried." .

ocsf:cvss  rdf:type          owl:ObjectProperty;
        rdfs:label           "CVSS Score";
        rdfs:range           ocsf:CVSSScore;
        dcterms:description  "The CVSS object details Common Vulnerability Scoring System (<a target='_blank' href='https://www.first.org/cvss/'>CVSS</a>) scores from the advisory that are related to the vulnerability." .

ocsf:lat  rdf:type           owl:DatatypeProperty;
        rdfs:label           "Latitude";
        rdfs:range           ocsf:float_t;
        dcterms:description  "The geographical Latitude coordinate represented in Decimal Degrees (DD). For example: <code>42.361145</code>." .

ocsf:devices  rdf:type       owl:ObjectProperty;
        rdfs:label           "Devices";
        dcterms:description  "The object describes details related to the list of devices." .

ocsf:image  rdf:type         owl:ObjectProperty;
        rdfs:label           "Image";
        rdfs:range           ocsf:Image;
        dcterms:description  "The image used as a template to run a container or virtual machine." .

ocsf:share  rdf:type         owl:DatatypeProperty;
        rdfs:label           "Share";
        rdfs:range           ocsf:string_t;
        dcterms:description  "The share name. See specific usage." .

ocsf:timezone_offset  rdf:type  owl:DatatypeProperty;
        rdfs:label           "Timezone Offset";
        rdfs:range           ocsf:integer_t;
        dcterms:description  "The number of minutes that the reported event <code>time</code> is ahead or behind UTC, in the range -1,080 to +1,080." .

ocsf:technique  rdf:type     owl:ObjectProperty;
        rdfs:label           "Technique";
        rdfs:range           ocsf:MITREATTCKTechnique;
        dcterms:description  "The Technique object describes the technique ID and/or name associated to an attack, as defined by <a target='_blank' href='https://attack.mitre.org/wiki/ATT&CK_Matrix'>ATT&CK® Matrix</a>." .

ocsf:uuid_t  rdf:type        rdfs:Datatype;
        rdfs:label           "UUID";
        rdfs:subClassOf      xsd:string;
        dcterms:description  "128-bit universal unique identifier. For example: <code>123e4567-e89b-12d3-a456-42661417400</code>.";
        xsd:pattern          "[0-9a-fA-F]{8}-[0-9a-fA-F]{4}-[0-9a-fA-F]{4}-[0-9a-fA-F]{4}-[0-9a-fA-F]{12}" .

ocsf:command  rdf:type       owl:DatatypeProperty;
        rdfs:label           "Command";
        rdfs:range           ocsf:string_t;
        dcterms:description  "The command name." .

ocsf:purl  rdf:type          owl:DatatypeProperty;
        rdfs:label           "Package URL";
        rdfs:range           ocsf:string_t;
        dcterms:description  "A purl is a URL string used to identify and locate a software package in a mostly universal and uniform way across programming languages, package managers, packaging conventions, tools, APIs and databases." .

ocsf:class_uid  rdf:type     owl:DatatypeProperty;
        rdfs:label           "Class ID";
        rdfs:range           ocsf:integer_t;
        dcterms:description  "The unique identifier of a class. A class describes the attributes available in an event." .

ocsf:ja3_hash  rdf:type      owl:ObjectProperty;
        rdfs:label           "JA3 Hash";
        rdfs:range           ocsf:Fingerprint;
        dcterms:description  "The MD5 hash of a JA3 string." .

ocsf:created_time  rdf:type  owl:DatatypeProperty;
        rdfs:label           "Created Time";
        rdfs:range           ocsf:timestamp_t;
        dcterms:description  "The time when the object was created. See specific usage." .

ocsf:raw_data  rdf:type      owl:DatatypeProperty;
        rdfs:label           "Raw Data";
        rdfs:range           ocsf:string_t;
        dcterms:description  "The raw event/finding data as received from the source." .

ocsf:message_uid  rdf:type   owl:DatatypeProperty;
        rdfs:label           "Message UID";
        rdfs:range           ocsf:string_t;
        dcterms:description  "The email header Message-Id value, as defined by RFC 5322." .

ocsf:impact  rdf:type        owl:DatatypeProperty;
        rdfs:label           "Impact";
        rdfs:range           ocsf:string_t;
        dcterms:description  "The impact , normalized to the caption of the impact_id value. In the case of 'Other', it is defined by the event source." .

ocsf:is_new_logon  rdf:type  owl:DatatypeProperty;
        rdfs:label           "New Logon";
        rdfs:range           ocsf:boolean_t;
        dcterms:description  "Indicates logon is from a device not seen before or a first time account logon." .

ocsf:countermeasures  rdf:type  owl:ObjectProperty;
        rdfs:label           "Countermeasures";
        rdfs:range           ocsf:MITRED3FEND;
        dcterms:description  "The MITRE DEFEND™ Matrix Countermeasures associated with a remediation." .

ocsf:correlation_uid  rdf:type  owl:DatatypeProperty;
        rdfs:label           "Correlation UID";
        rdfs:range           ocsf:string_t;
        dcterms:description  "The unique identifier used to correlate events." .

ocsf:full_name  rdf:type     owl:DatatypeProperty;
        rdfs:label           "Full Name";
        rdfs:range           ocsf:string_t;
        dcterms:description  "The full name of the person, as per the LDAP Common Name attribute (cn)." .

ocsf:flags  rdf:type         owl:DatatypeProperty;
        rdfs:label           "Flags";
        rdfs:range           ocsf:string_t;
        dcterms:description  "The list of communication flags, normalized to the captions of the flag_ids values. In the case of 'Other', they are defined by the event source." .

ocsf:cve  rdf:type           owl:ObjectProperty;
        rdfs:label           "CVE";
        rdfs:range           ocsf:CVE;
        dcterms:description  "The Common Vulnerabilities and Exposures (<a target='_blank' href='https://cve.mitre.org/'>CVE</a>)." .

ocsf:attacks  rdf:type       owl:ObjectProperty;
        rdfs:label           "MITRE ATT&CK® Details";
        rdfs:range           ocsf:MITREATTCK;
        dcterms:description  "An array of <a target='_blank' href='https://attack.mitre.org'>MITRE ATT&CK®</a> objects describing the tactics, techniques & sub-techniques identified by a security control or finding." .

ocsf:related_vulnerabilities
        rdf:type             owl:DatatypeProperty;
        rdfs:label           "Related Vulnerabilities";
        rdfs:range           ocsf:string_t;
        dcterms:description  "List of vulnerabilities that are related to this vulnerability." .

ocsf:depth  rdf:type         owl:DatatypeProperty;
        rdfs:label           "CVSS Depth";
        rdfs:range           ocsf:string_t;
        dcterms:description  "The CVSS depth represents a depth of the equation used to calculate CVSS score.";
        jsonschema:enum      "Temporal" , "Environmental" , "Base" .

ocsf:cost_center  rdf:type   owl:DatatypeProperty;
        rdfs:label           "Cost Center";
        rdfs:range           ocsf:string_t;
        dcterms:description  "The cost center associated with the user." .

ocsf:proxy_traffic  rdf:type  owl:ObjectProperty;
        rdfs:label           "Proxy Traffic";
        rdfs:range           ocsf:NetworkTraffic;
        dcterms:description  "The network traffic refers to the amount of data moving across a network, from proxy to remote server at a given point of time." .

ocsf:security_level  rdf:type  owl:DatatypeProperty;
        rdfs:label           "Security Level";
        rdfs:range           ocsf:string_t;
        dcterms:description  "The current security level of the entity" .

ocsf:cis_benchmark  rdf:type  owl:ObjectProperty;
        rdfs:label           "CIS Benchmark";
        rdfs:range           ocsf:CISBenchmark;
        dcterms:description  "The CIS Benchmark describes best practices for securely configuring IT systems, software, networks, and cloud infrastructure as defined by the Center for Internet Security (<a target='_blank' href='https://www.cisecurity.org/cis-benchmarks/'>CIS</a>)." .

ocsf:chunks_out  rdf:type    owl:DatatypeProperty;
        rdfs:label           "Chunks Out";
        rdfs:range           ocsf:long_t;
        dcterms:description  "A unit of information within an SCTP packet, consisting of a chunk header and chunk-specific content. See RFC 4960. This field can be used for the chunks sent from the source to the destination." .

ocsf:access_mask  rdf:type   owl:DatatypeProperty;
        rdfs:label           "Access Mask";
        rdfs:range           ocsf:integer_t;
        dcterms:description  "The access mask in a platform-native format." .

ocsf:ou_name  rdf:type       owl:DatatypeProperty;
        rdfs:label           "Org Unit Name";
        rdfs:range           ocsf:string_t;
        dcterms:description  "The name of the organizational unit, within an organization.  For example, Finance, IT, R&D" .

ocsf:float_t  rdf:type       rdfs:Datatype;
        rdfs:label           "Float";
        rdfs:subClassOf      xsd:decimal;
        dcterms:description  "Real floating-point value. For example: <code>3.14</code>." .

ocsf:request  rdf:type       owl:ObjectProperty;
        rdfs:label           "API Request Details";
        rdfs:range           ocsf:RequestElements;
        dcterms:description  "General Purpose API Request Object. See specific usage" .

ocsf:phone_number  rdf:type  owl:DatatypeProperty;
        rdfs:label           "Phone Number";
        rdfs:range           ocsf:string_t;
        dcterms:description  "The number associated with the phone." .

ocsf:country  rdf:type       owl:DatatypeProperty;
        rdfs:label           "Country";
        rdfs:range           ocsf:string_t;
        dcterms:description  "The ISO 3166-1 Alpha-2 country code. For the complete list of country codes see <a target='_blank' href='https://www.iso.org/obp/ui/#iso:pub:PUB500001:en' >ISO 3166-1 alpha-2 codes</a>.<p><b>Note:</b> The two letter country code should be capitalized. For example: <code>US</code> or <code>CA</code>.</p>" .

ocsf:long  rdf:type          owl:DatatypeProperty;
        rdfs:label           "Longitude";
        rdfs:range           ocsf:float_t;
        dcterms:description  "The geographical Longitude coordinate represented in Decimal Degrees (DD). For example: <code>-71.057083</code>." .

ocsf:delivered_to  rdf:type  owl:DatatypeProperty;
        rdfs:label           "Delivered To";
        rdfs:range           ocsf:email_t;
        dcterms:description  "The <strong>Delivered-To</strong> email header field." .

ocsf:is_default  rdf:type    owl:DatatypeProperty;
        rdfs:label           "Default Value";
        rdfs:range           ocsf:boolean_t;
        dcterms:description  "The indication of whether the value is from a default value name. For example, the value name could be missing." .

ocsf:injection_type_id
        rdf:type             owl:DatatypeProperty;
        rdfs:label           "Injection Type ID";
        rdfs:range           ocsf:integer_t;
        dcterms:description  "The normalized identifier of the process injection method.";
        jsonschema:enum      "Other" , "Queue APC" , "Load Library" , "Remote Thread" , "Unknown" .

ocsf:num_skipped_items
        rdf:type             owl:DatatypeProperty;
        rdfs:label           "Skipped";
        rdfs:range           ocsf:integer_t;
        dcterms:description  "The number of skipped items." .

ocsf:peripheral_device
        rdf:type             owl:ObjectProperty;
        rdfs:label           "Peripheral Device";
        rdfs:range           ocsf:PeripheralDevice;
        dcterms:description  "The peripheral device that triggered the event." .

ocsf:project_uid  rdf:type   owl:DatatypeProperty;
        rdfs:label           "Project ID";
        rdfs:range           ocsf:string_t;
        dcterms:description  "The unique identifier of a Cloud project." .

ocsf:app  rdf:type           owl:ObjectProperty;
        rdfs:label           "Application";
        rdfs:range           ocsf:Product;
        dcterms:description  "The application that reported the event." .

ocsf:ttl  rdf:type           owl:DatatypeProperty;
        rdfs:label           "TTL";
        rdfs:range           ocsf:integer_t;
        dcterms:description  "The time interval that the resource record may be cached. Zero value means that the resource record can only be used for the transaction in progress, and should not be cached." .

ocsf:is_compliant  rdf:type  owl:DatatypeProperty;
        rdfs:label           "Compliant Device";
        rdfs:range           ocsf:boolean_t;
        dcterms:description  "The event occurred on a compliant device." .

ocsf:d3f_technique  rdf:type  owl:ObjectProperty;
        rdfs:label           "MITRE DEFEND™ Technique";
        rdfs:range           ocsf:MITREDEFENDTechnique;
        dcterms:description  "The D3FEND Technique object describes the defensive technique ID and/or name associated with a countermeasure, as defined by <a target='_blank' href='https://d3fend.mitre.org'>D3FEND<sup>TM</sup> Matrix</a>." .

ocsf:remediation  rdf:type   owl:ObjectProperty;
        rdfs:label           "Remediation Guidance";
        rdfs:range           ocsf:Remediation;
        dcterms:description  "Describes the recommended remediation steps to address identified issue(s)." .

ocsf:logon_type_id  rdf:type  owl:DatatypeProperty;
        rdfs:label           "Logon Type ID";
        rdfs:range           ocsf:integer_t;
        dcterms:description  "The normalized logon type identifier.";
        jsonschema:enum      "New Credentials" , "Cached Remote Interactive" , "Network" , "Unknown" , "Network Cleartext" , "OS Service" , "Unlock" , "Cached Unlock" , "Remote Interactive" , "Batch" , "Other" , "System" , "Interactive" , "Cached Interactive" .

ocsf:ja4_fingerprint_list
        rdf:type             owl:ObjectProperty;
        rdfs:label           "JA4+ Fingerprints";
        rdfs:range           ocsf:JA4Fingerprint;
        dcterms:description  "A list of the JA4+ network fingerprints." .

ocsf:company_name  rdf:type  owl:DatatypeProperty;
        rdfs:label           "Company Name";
        rdfs:range           ocsf:string_t;
        dcterms:description  "The name of the company that published the file. For example: <code>Microsoft Corporation</code>." .

ocsf:tenant_uid  rdf:type    owl:DatatypeProperty;
        rdfs:label           "Tenant UID";
        rdfs:range           ocsf:string_t;
        dcterms:description  "The unique tenant identifier." .

ocsf:src_endpoint  rdf:type  owl:ObjectProperty;
        rdfs:label           "Source Endpoint";
        dcterms:description  "The network source endpoint." .

ocsf:query_info  rdf:type    owl:ObjectProperty;
        rdfs:label           "Query Info";
        dcterms:description  "The query info object holds information related to data access within a datastore. To access, manipulate, delete, or retrieve data from a datastore, a database query must be written using a specific syntax." .

ocsf:log_version  rdf:type   owl:DatatypeProperty;
        rdfs:label           "Log Version";
        rdfs:range           ocsf:string_t;
        dcterms:description  "The event log schema version that specifies the format of the original event. For example syslog version or Cisco Log Schema Version." .

ocsf:sp_name  rdf:type       owl:DatatypeProperty;
        rdfs:label           "OS Service Pack";
        rdfs:range           ocsf:string_t;
        dcterms:description  "The name of the latest Service Pack." .

ocsf:databucket  rdf:type    owl:ObjectProperty;
        rdfs:label           "Databucket";
        rdfs:range           ocsf:Databucket;
        dcterms:description  "The data bucket object is a basic container that holds data, typically organized through the use of data partitions." .

ocsf:operation  rdf:type     owl:DatatypeProperty;
        rdfs:label           "Operation";
        rdfs:range           ocsf:string_t;
        dcterms:description  "Verb/Operation associated with the request" .

ocsf:orchestrator  rdf:type  owl:DatatypeProperty;
        rdfs:label           "Orchestrator";
        rdfs:range           ocsf:string_t;
        dcterms:description  "The orchestrator managing the container, such as ECS, EKS, K8s, or OpenShift." .

ocsf:direction  rdf:type     owl:DatatypeProperty;
        rdfs:label           "Direction";
        rdfs:range           ocsf:string_t;
        dcterms:description  "The direction of the initiated connection, traffic, or email, normalized to the caption of the direction_id value. In the case of 'Other', it is defined by the event source." .

ocsf:user_result  rdf:type   owl:ObjectProperty;
        rdfs:label           "User Result";
        rdfs:range           ocsf:User;
        dcterms:description  "The result of the user account change. It should contain the new values of the changed attributes." .

ocsf:latency  rdf:type       owl:DatatypeProperty;
        rdfs:label           "Latency";
        rdfs:range           ocsf:integer_t;
        dcterms:description  "The HTTP response latency measured in milliseconds." .

ocsf:metrics  rdf:type       owl:ObjectProperty;
        rdfs:label           "Metrics";
        rdfs:range           ocsf:Metric;
        dcterms:description  "The general purpose metrics associated with the event. See specific usage." .

ocsf:packets_in  rdf:type    owl:DatatypeProperty;
        rdfs:label           "Packets In";
        rdfs:range           ocsf:long_t;
        dcterms:description  "The number of packets sent from the destination to the source." .

ocsf:compliance  rdf:type    owl:ObjectProperty;
        rdfs:label           "Compliance";
        rdfs:range           ocsf:Compliance;
        dcterms:description  "The compliance object provides context to compliance findings (e.g., a check against a specific regulatory or best practice framework such as CIS, NIST etc.) and contains compliance related details." .

ocsf:to  rdf:type            owl:DatatypeProperty;
        rdfs:label           "To";
        rdfs:range           ocsf:email_t;
        dcterms:description  "The email header To values, as defined by RFC 5322." .

ocsf:share_type_id  rdf:type  owl:DatatypeProperty;
        rdfs:label           "Share Type Id";
        rdfs:range           ocsf:integer_t;
        dcterms:description  "The normalized identifier of the share type.";
        jsonschema:enum      "Other" , "Print" , "Pipe" , "File" , "Unknown" .

ocsf:section_c  rdf:type     owl:DatatypeProperty;
        rdfs:label           "JA4 Section C";
        rdfs:range           ocsf:string_t;
        dcterms:description  "The 'c' section of the JA4 fingerprint." .

ocsf:os  rdf:type            owl:ObjectProperty;
        rdfs:label           "OS";
        rdfs:range           ocsf:OperatingSystemOS;
        dcterms:description  "The endpoint operating system." .

ocsf:fix_available  rdf:type  owl:DatatypeProperty;
        rdfs:label           "Fix Availability";
        rdfs:range           ocsf:boolean_t;
        dcterms:description  "Indicates if a fix is available for the reported vulnerability." .

ocsf:http_response  rdf:type  owl:ObjectProperty;
        rdfs:label           "HTTP Response";
        rdfs:range           ocsf:HTTPResponse;
        dcterms:description  "The HTTP Response from a web server to a requester." .

ocsf:is_fix_available
        rdf:type             owl:DatatypeProperty;
        rdfs:label           "Fix Availability";
        rdfs:range           ocsf:boolean_t;
        dcterms:description  "Indicates if a fix is available for the reported vulnerability." .

ocsf:url_string  rdf:type    owl:DatatypeProperty;
        rdfs:label           "URL String";
        rdfs:range           ocsf:url_t;
        dcterms:description  "The URL string. See RFC 1738. For example: <code>http://www.example.com/download/trouble.exe</code>." .

ocsf:job_title  rdf:type     owl:DatatypeProperty;
        rdfs:label           "Job Title";
        rdfs:range           ocsf:string_t;
        dcterms:description  "The user's job title." .

ocsf:original_time  rdf:type  owl:DatatypeProperty;
        rdfs:label           "Original Time";
        rdfs:range           ocsf:string_t;
        dcterms:description  "The original event time as reported by the event source. For example, the time in the original format from system event log such as Syslog on Unix/Linux and the System event file on Windows. Omit if event is generated instead of collected via logs." .

ocsf:tls  rdf:type           owl:ObjectProperty;
        rdfs:label           "TLS";
        rdfs:range           ocsf:TransportLayerSecurityTLS;
        dcterms:description  "The Transport Layer Security (TLS) attributes." .

ocsf:architecture  rdf:type  owl:DatatypeProperty;
        rdfs:label           "Architecture";
        rdfs:range           ocsf:string_t;
        dcterms:description  "Architecture is a shorthand name describing the type of computer hardware the packaged software is meant to run on." .

ocsf:metadata  rdf:type      owl:ObjectProperty;
        rdfs:label           "Metadata";
        rdfs:range           ocsf:Metadata;
        dcterms:description  "The metadata associated with the event or a finding." .

ocsf:spf  rdf:type           owl:DatatypeProperty;
        rdfs:label           "SPF Status";
        rdfs:range           ocsf:string_t;
        dcterms:description  "The Sender Policy Framework (SPF) status of the email." .

ocsf:risk_score  rdf:type    owl:DatatypeProperty;
        rdfs:label           "Risk Score";
        rdfs:range           ocsf:integer_t;
        dcterms:description  "The risk score as reported by the event source." .

ocsf:cis_csc  rdf:type       owl:ObjectProperty;
        rdfs:label           "CIS CSC";
        rdfs:range           ocsf:CISCSC;
        dcterms:description  "The CIS Critical Security Controls is a list of top 20 actions and practices an organization’s security team can take on such that cyber attacks or malware, are minimized and prevented." .

ocsf:folder  rdf:type        owl:ObjectProperty;
        rdfs:label           "Folder";
        rdfs:range           ocsf:File;
        dcterms:description  "The folder that pertains to the event." .

ocsf:fingerprints  rdf:type  owl:ObjectProperty;
        rdfs:label           "Fingerprints";
        rdfs:range           ocsf:Fingerprint;
        dcterms:description  "An array of digital fingerprint objects." .

ocsf:caption  rdf:type       owl:DatatypeProperty;
        rdfs:label           "Caption";
        rdfs:range           ocsf:string_t;
        dcterms:description  "A short description or caption of the device. For example: <code>Scanner 1</code> or <code>Database Manager</code>." .

ocsf:function_name  rdf:type  owl:DatatypeProperty;
        rdfs:label           "Function Name";
        rdfs:range           ocsf:string_t;
        dcterms:description  "The entry-point function of the module. The system calls the entry-point function whenever a process or thread loads or unloads the module." .

ocsf:client_dialects  rdf:type  owl:DatatypeProperty;
        rdfs:label           "Client Dialects";
        rdfs:range           ocsf:string_t;
        dcterms:description  "The list of SMB dialects that the client speaks." .

ocsf:dmarc  rdf:type         owl:DatatypeProperty;
        rdfs:label           "DMARC Status";
        rdfs:range           ocsf:string_t;
        dcterms:description  "The Domain-based Message Authentication, Reporting and Conformance (DMARC) status of the email." .

ocsf:server_hassh  rdf:type  owl:ObjectProperty;
        rdfs:label           "Server HASSH";
        rdfs:range           ocsf:HASSH;
        dcterms:description  "The Server HASSH fingerprinting object." .

ocsf:tcp_flags  rdf:type     owl:DatatypeProperty;
        rdfs:label           "TCP Flags";
        rdfs:range           ocsf:integer_t;
        dcterms:description  "The network connection TCP header flags (i.e., control bits)." .

ocsf:tree_uid  rdf:type      owl:DatatypeProperty;
        rdfs:label           "Tree UID";
        rdfs:range           ocsf:string_t;
        dcterms:description  "The tree id is a unique SMB identifier which represents an open connection to a share." .

ocsf:algorithm  rdf:type     owl:DatatypeProperty;
        rdfs:label           "Algorithm";
        rdfs:range           ocsf:string_t;
        dcterms:description  "The applicable algorithm, normalized to the caption of 'algorithm_id'. See specific usage." .

ocsf:status  rdf:type        owl:DatatypeProperty;
        rdfs:label           "Status";
        rdfs:range           ocsf:string_t;
        dcterms:description  "The event status, normalized to the caption of the status_id value. In the case of 'Other', it is defined by the event source." .

ocsf:tunnel_type_id  rdf:type  owl:DatatypeProperty;
        rdfs:label           "Type";
        rdfs:range           ocsf:integer_t;
        dcterms:description  "The normalized tunnel type ID." .

ocsf:protocol_ver  rdf:type  owl:DatatypeProperty;
        rdfs:label           "Protocol Version";
        rdfs:range           ocsf:string_t;
        dcterms:description  "The Protocol version, normalized to the caption of the protocol_ver_id value. In the case of 'Other', it is defined by the event source." .

ocsf:lang  rdf:type          owl:DatatypeProperty;
        rdfs:label           "Language";
        rdfs:range           ocsf:string_t;
        dcterms:description  "The two letter lower case language codes, as defined by <a target='_blank' href='https://en.wikipedia.org/wiki/ISO_639-1'>ISO 639-1</a>. For example: <code>en</code> (English), <code>de</code> (German), or <code>fr</code> (French)." .

ocsf:answers  rdf:type       owl:ObjectProperty;
        rdfs:label           "DNS Answer";
        rdfs:range           ocsf:DNSAnswer;
        dcterms:description  "The Domain Name System (DNS) answers." .

ocsf:edition  rdf:type       owl:DatatypeProperty;
        rdfs:label           "OS Edition";
        rdfs:range           ocsf:string_t;
        dcterms:description  "The operating system edition. For example: <code>Professional</code>." .

ocsf:content_type  rdf:type  owl:DatatypeProperty;
        rdfs:label           "HTTP Content Type";
        rdfs:range           ocsf:string_t;
        dcterms:description  "The request header that identifies the original <a target='_blank' href='https://www.iana.org/assignments/media-types/media-types.xhtml'>media type </a> of the resource (prior to any content encoding applied for sending)." .

ocsf:is_on_premises  rdf:type  owl:DatatypeProperty;
        rdfs:label           "On Premises";
        rdfs:range           ocsf:boolean_t;
        dcterms:description  "The indication of whether the location is on premises." .

ocsf:uid_alt  rdf:type       owl:DatatypeProperty;
        rdfs:label           "Alternate ID";
        rdfs:range           ocsf:string_t;
        dcterms:description  "The alternate unique identifier. See specific usage." .

ocsf:hash  rdf:type          owl:ObjectProperty;
        rdfs:label           "Hash";
        rdfs:range           ocsf:Fingerprint;
        dcterms:description  "The hash attribute is the value of a digital fingerprint including information about its algorithm." .

ocsf:email_addrs  rdf:type   owl:DatatypeProperty;
        rdfs:label           "Email Addresses";
        rdfs:range           ocsf:email_t;
        dcterms:description  "A list of additional email addresses for the user." .

ocsf:confidence_id  rdf:type  owl:DatatypeProperty;
        rdfs:label           "Confidence Id";
        rdfs:range           ocsf:integer_t;
        dcterms:description  "The normalized confidence refers to the accuracy of the rule that created the finding. A rule with a low confidence means that the finding scope is wide and may create finding reports that may not be malicious in nature.";
        jsonschema:enum      "Other" , "High" , "Medium" , "Low" , "Unknown" .

ocsf:count  rdf:type         owl:DatatypeProperty;
        rdfs:label           "Count";
        rdfs:range           ocsf:integer_t;
        dcterms:description  "The number of times that events in the same logical group occurred during the event <strong>Start Time</strong> to <strong>End Time</strong> period." .

ocsf:dst_endpoint  rdf:type  owl:ObjectProperty;
        rdfs:label           "Destination Endpoint";
        dcterms:description  "The network destination endpoint." .

ocsf:data_classification
        rdf:type             owl:ObjectProperty;
        rdfs:label           "Data Classification";
        dcterms:description  "The Data Classification object includes information about data classification levels and data category types." .

ocsf:file_hash_t  rdf:type   rdfs:Datatype;
        rdfs:label           "Hash";
        rdfs:subClassOf      xsd:string;
        dcterms:description  "Hash. A unique value that corresponds to the content of the file, image, ja3_hash or hassh found in the schema. For example MD5: <code>3172ac7e2b55cbb81f04a6e65855a628</code>." .

ocsf:url  rdf:type           owl:ObjectProperty;
        rdfs:label           "URL";
        rdfs:range           ocsf:UniformResourceLocator;
        dcterms:description  "The URL object that pertains to the event or object. See specific usage." .

ocsf:cwe_url  rdf:type       owl:DatatypeProperty;
        rdfs:label           "CWE URL";
        rdfs:range           ocsf:url_t;
        dcterms:description  "Common Weakness Enumeration (CWE) definition URL. For example: <code>https://cwe.mitre.org/data/definitions/787.html</code>." .

ocsf:tag  rdf:type           owl:DatatypeProperty;
        rdfs:label           "Image Tag";
        rdfs:range           ocsf:string_t;
        dcterms:description  "The image tag. For example: <code>1.11-alpine</code>." .

ocsf:error  rdf:type         owl:DatatypeProperty;
        rdfs:label           "Error Code";
        rdfs:range           ocsf:string_t;
        dcterms:description  "Error Code" .

ocsf:instance_uid  rdf:type  owl:DatatypeProperty;
        rdfs:label           "Instance ID";
        rdfs:range           ocsf:string_t;
        dcterms:description  "The unique identifier of a VM instance." .

ocsf:command_uid  rdf:type   owl:DatatypeProperty;
        rdfs:label           "Command UID";
        rdfs:range           ocsf:string_t;
        dcterms:description  "The unique command identifier." .

ocsf:auth_type  rdf:type     owl:DatatypeProperty;
        rdfs:label           "Authentication Type";
        rdfs:range           ocsf:string_t;
        dcterms:description  "The agreed upon authentication type, normalized to the caption of 'auth_type_id'. In the case of 'Other', it is defined by the event source." .

ocsf:client_hassh  rdf:type  owl:ObjectProperty;
        rdfs:label           "Client HASSH";
        rdfs:range           ocsf:HASSH;
        dcterms:description  "The Client HASSH fingerprinting object." .

ocsf:log_name  rdf:type      owl:DatatypeProperty;
        rdfs:label           "Log Name";
        rdfs:range           ocsf:string_t;
        dcterms:description  "The event log name. For example, syslog file name or Windows logging subsystem: Security." .

ocsf:requirements  rdf:type  owl:DatatypeProperty;
        rdfs:label           "Compliance Requirements";
        rdfs:range           ocsf:string_t;
        dcterms:description  "A list of requirements associated to a specific control in an industry or regulatory framework. e.g. <code> NIST.800-53.r5 AU-10 </code>" .

ocsf:api  rdf:type           owl:ObjectProperty;
        rdfs:label           "API Details";
        rdfs:range           ocsf:API;
        dcterms:description  "Describes details about a typical API (Application Programming Interface) call." .

ocsf:resource_uid_t  rdf:type  rdfs:Datatype;
        rdfs:label           "Resource UID";
        rdfs:subClassOf      xsd:string;
        dcterms:description  "Resource unique identifier. For example, S3 Bucket name or EC2 Instance ID." .

ocsf:hire_time  rdf:type     owl:DatatypeProperty;
        rdfs:label           "Hire Time";
        rdfs:range           ocsf:timestamp_t;
        dcterms:description  "The timestamp when the user was or will be hired by the organization." .

ocsf:is_suspected_breach
        rdf:type             owl:DatatypeProperty;
        rdfs:label           "Suspected Breach";
        rdfs:range           ocsf:boolean_t;
        dcterms:description  "A determination based on analytics as to whether a potential breach was found." .

ocsf:tunnel_type  rdf:type   owl:DatatypeProperty;
        rdfs:label           "Type";
        rdfs:range           ocsf:string_t;
        dcterms:description  "The tunnel type. See specific usage." .

ocsf:num_folders  rdf:type   owl:DatatypeProperty;
        rdfs:label           "Scanned Folders";
        rdfs:range           ocsf:integer_t;
        dcterms:description  "The number of folders scanned." .

ocsf:timestamp_t  rdf:type   rdfs:Datatype;
        rdfs:label           "Timestamp";
        rdfs:subClassOf      xsd:long;
        dcterms:description  "The timestamp format is the number of milliseconds since the Epoch 01/01/1970 00:00:00 UTC. For example <code>1618524549901</code>." .

ocsf:ram_size  rdf:type      owl:DatatypeProperty;
        rdfs:label           "RAM Size";
        rdfs:range           ocsf:integer_t;
        dcterms:description  "The total amount of installed RAM, in Megabytes. For example: <code>2048</code>." .

ocsf:agent  rdf:type         owl:ObjectProperty;
        rdfs:label           "Agent";
        dcterms:description  "An Agent (also known as a Sensor) is typically installed on an Operating System (OS) and serves as a specialized software component that can be designed to monitor, detect, collect, archive, or take action. These activities and possible actions are defined by the upstream system controlling the Agent and its intended purpose. For instance, an Agent can include Endpoint Detection & Response (EDR) agents, backup/disaster recovery sensors, Application Performance Monitoring or profiling sensors, and similar software." .

ocsf:http_status  rdf:type   owl:DatatypeProperty;
        rdfs:label           "HTTP Status";
        rdfs:range           ocsf:integer_t;
        dcterms:description  "The Hypertext Transfer Protocol (HTTP) <a target='_blank' href='https://www.iana.org/assignments/http-status-codes/http-status-codes.xhtml'>status code</a> returned to the client." .

ocsf:email  rdf:type         owl:ObjectProperty;
        rdfs:label           "Email";
        rdfs:range           ocsf:Email;
        dcterms:description  "The email object." .

ocsf:status_id  rdf:type     owl:DatatypeProperty;
        rdfs:label           "Status ID";
        rdfs:range           ocsf:integer_t;
        dcterms:description  "The normalized identifier of the event status.";
        jsonschema:enum      "Other" , "Failure" , "Success" , "Unknown" .

ocsf:security_level_id
        rdf:type             owl:DatatypeProperty;
        rdfs:label           "Security Level ID";
        rdfs:range           ocsf:integer_t;
        dcterms:description  "The current security level of the entity";
        jsonschema:enum      "Other" , "Compromised" , "At Risk" , "Secure" , "Unknown" .

ocsf:packets_out  rdf:type   owl:DatatypeProperty;
        rdfs:label           "Packets Out";
        rdfs:range           ocsf:long_t;
        dcterms:description  "The number of packets sent from the source to the destination." .

ocsf:finding_info_list
        rdf:type             owl:ObjectProperty;
        rdfs:label           "Finding Information List";
        rdfs:range           ocsf:FindingInformation;
        dcterms:description  "A list of <code>finding_info</code> objects associated to an incident." .

ocsf:sans  rdf:type          owl:ObjectProperty;
        rdfs:label           "Subject Alternative Names";
        rdfs:range           ocsf:SubjectAlternativeName;
        dcterms:description  "The list of subject alternative names that are secured by a specific certificate." .

ocsf:activity_name  rdf:type  owl:DatatypeProperty;
        rdfs:label           "Activity";
        rdfs:range           ocsf:string_t;
        dcterms:description  "The event activity name, as defined by the activity_id." .

ocsf:expiration_reason
        rdf:type             owl:DatatypeProperty;
        rdfs:label           "Expiration Reason";
        rdfs:range           ocsf:string_t;
        dcterms:description  "The expiration reason. See specific usage." .

ocsf:employee_uid  rdf:type  owl:DatatypeProperty;
        rdfs:label           "Employee ID";
        rdfs:range           ocsf:string_t;
        dcterms:description  "The employee identifier assigned to the user by the organization." .

ocsf:evidence  rdf:type      owl:DatatypeProperty;
        rdfs:label           "Evidence";
        rdfs:range           ocsf:json_t;
        dcterms:description  "The data the finding exposes to the analyst." .

ocsf:protocol_num  rdf:type  owl:DatatypeProperty;
        rdfs:label           "Protocol Number";
        rdfs:range           ocsf:integer_t;
        dcterms:description  "The TCP/IP protocol number, as defined by the Internet Assigned Numbers Authority (IANA). Use -1 if the protocol is not defined by IANA. See <a target='_blank' href='https://www.iana.org/assignments/protocol-numbers/protocol-numbers.xhtml'>Protocol Numbers</a>. For example: <code>6</code> for TCP and <code>17</code> for UDP." .

ocsf:physical_orientation
        rdf:type             owl:DatatypeProperty;
        rdfs:label           "Physical Orientation";
        rdfs:range           ocsf:integer_t;
        dcterms:description  "The numeric physical orientation of display." .

ocsf:component  rdf:type     owl:DatatypeProperty;
        rdfs:label           "Component";
        rdfs:range           ocsf:string_t;
        dcterms:description  "The component of a data object. See specific usage." .

ocsf:log_type_id  rdf:type   owl:DatatypeProperty;
        rdfs:label           "Log Type ID";
        rdfs:range           ocsf:integer_t;
        dcterms:description  "The normalized log type identifier.";
        jsonschema:enum      "Other" , "Application" , "OS" , "Unknown" .

ocsf:title  rdf:type         owl:DatatypeProperty;
        rdfs:label           "Title";
        rdfs:range           ocsf:string_t;
        dcterms:description  "The title of an entity. See specific usage." .

ocsf:port_t  rdf:type        rdfs:Datatype;
        rdfs:label           "Port";
        rdfs:subClassOf      xsd:integer;
        dcterms:description  "The TCP/UDP port number. For example: <code>80</code> or <code>22</code>.";
        xsd:maxInclusive     65535;
        xsd:minInclusive     0 .

ocsf:hw_info  rdf:type       owl:ObjectProperty;
        rdfs:label           "Hardware Info";
        rdfs:range           ocsf:DeviceHardwareInfo;
        dcterms:description  "The endpoint hardware information." .

ocsf:package  rdf:type       owl:ObjectProperty;
        rdfs:label           "Software Package";
        rdfs:range           ocsf:SoftwarePackage;
        dcterms:description  "The Software Package object describes details about a software package. Defined by D3FEND <a target='_blank' href='https://d3fend.mitre.org/dao/artifact/d3f:SoftwarePackage/'>d3f:SoftwarePackage</a>." .

ocsf:vector_string  rdf:type  owl:DatatypeProperty;
        rdfs:label           "Vector String";
        rdfs:range           ocsf:string_t;
        dcterms:description  "The CVSS vector string is a text representation of a set of CVSS metrics. It is commonly used to record or transfer CVSS metric information in a concise form. For example: <code>3.1/AV:L/AC:L/PR:L/UI:N/S:U/C:H/I:N/A:H</code>." .

ocsf:permission  rdf:type    owl:DatatypeProperty;
        rdfs:label           "Permission";
        rdfs:range           ocsf:string_t;
        dcterms:description  "The IAM permission related to an event" .

ocsf:osint  rdf:type         owl:ObjectProperty;
        rdfs:label           "OSINT";
        rdfs:range           ocsf:OSINT;
        dcterms:description  "The OSINT (Open Source Intelligence) object contains details related to an indicator such as the indicator itself, related indicators, geolocation, registrar information, subdomains, analyst commentary, and other contextual information. This information can be used to further enrich a detection or finding by providing decisioning support to other analysts and engineers." .

ocsf:requested_permissions
        rdf:type             owl:DatatypeProperty;
        rdfs:label           "Requested Permissions";
        rdfs:range           ocsf:integer_t;
        dcterms:description  "The permissions mask that were requested by the process." .

ocsf:digest  rdf:type        owl:ObjectProperty;
        rdfs:label           "Message Digest";
        rdfs:range           ocsf:Fingerprint;
        dcterms:description  "The message digest attribute contains the fixed length message hash representation and the corresponding hashing algorithm information." .

ocsf:processed_time  rdf:type  owl:DatatypeProperty;
        rdfs:label           "Processed Time";
        rdfs:range           ocsf:timestamp_t;
        dcterms:description  "The event processed time, such as an ETL operation." .

ocsf:expiration_time  rdf:type  owl:DatatypeProperty;
        rdfs:label           "Expiration Time";
        rdfs:range           ocsf:timestamp_t;
        dcterms:description  "The expiration time. See specific usage." .

ocsf:ack_reason  rdf:type    owl:DatatypeProperty;
        rdfs:label           "Acknowledgement Reason";
        rdfs:range           ocsf:integer_t;
        dcterms:description  "An integer that provides a reason code or additional information about the acknowledgment result." .

ocsf:verdict_id  rdf:type    owl:DatatypeProperty;
        rdfs:label           "Verdict ID";
        rdfs:range           ocsf:integer_t;
        dcterms:description  "The normalized verdict of an Incident.";
        jsonschema:enum      "False Positive" , "Duplicate" , "Suspicious" , "Unknown" , "Test" , "True Positive" , "Insufficient Data" , "Managed Externally" , "Benign" , "Security Risk" , "Other" , "Disregard" .

ocsf:tactic  rdf:type        owl:ObjectProperty;
        rdfs:label           "Tactic";
        rdfs:range           ocsf:MITREATTCKTactic;
        dcterms:description  "The Tactic object describes the tactic ID and/or name that is associated to an attack, as defined by <a target='_blank' href='https://attack.mitre.org/wiki/ATT&CK_Matrix'>ATT&CK® Matrix</a>." .

ocsf:proxy_http_request
        rdf:type             owl:ObjectProperty;
        rdfs:label           "Proxy HTTP Request";
        rdfs:range           ocsf:HTTPRequest;
        dcterms:description  "The HTTP Request from the proxy server to the remote server." .

ocsf:rcode  rdf:type         owl:DatatypeProperty;
        rdfs:label           "Response Code";
        rdfs:range           ocsf:string_t;
        dcterms:description  "The server response code, normalized to the caption of the rcode_id value. In the case of 'Other', it is defined by the event source." .

ocsf:run_state  rdf:type     owl:DatatypeProperty;
        rdfs:label           "Run State";
        rdfs:range           ocsf:string_t;
        dcterms:description  "The state of the job or service, normalized to the caption of the run_state_id value. In the case of 'Other', it is defined by the event source. See specific usage." .

ocsf:model  rdf:type         owl:DatatypeProperty;
        rdfs:label           "Model";
        rdfs:range           ocsf:string_t;
        dcterms:description  "The peripheral device model." .

ocsf:percentile  rdf:type    owl:DatatypeProperty;
        rdfs:label           "EPSS Percentile";
        rdfs:range           ocsf:float_t;
        dcterms:description  "The EPSS score's percentile representing relative importance and ranking of the score in the larger EPSS dataset." .

ocsf:open_type  rdf:type     owl:DatatypeProperty;
        rdfs:label           "Open Type";
        rdfs:range           ocsf:string_t;
        dcterms:description  "The file open type." .

ocsf:section_a  rdf:type     owl:DatatypeProperty;
        rdfs:label           "JA4 Section A";
        rdfs:range           ocsf:string_t;
        dcterms:description  "The 'a' section of the JA4 fingerprint." .

ocsf:data_lifecycle_state
        rdf:type             owl:DatatypeProperty;
        rdfs:label           "Data Lifecycle State";
        rdfs:range           ocsf:string_t;
        dcterms:description  "The name of the stage or state that the data was in. E.g., Data-at-Rest, Data-in-Transit, etc." .

ocsf:sandbox  rdf:type       owl:DatatypeProperty;
        rdfs:label           "Sandbox";
        rdfs:range           ocsf:string_t;
        dcterms:description  "The name of the containment jail (i.e., sandbox). For example, hardened_ps, high_security_ps, oracle_ps, netsvcs_ps, or default_ps." .

ocsf:base_score  rdf:type    owl:DatatypeProperty;
        rdfs:label           "Base Score";
        rdfs:range           ocsf:float_t;
        dcterms:description  "The base score as reported by the event source. See specific usage." .

ocsf:unmapped  rdf:type      owl:ObjectProperty;
        rdfs:label           "Unmapped Data";
        rdfs:range           ocsf:Object;
        dcterms:description  "The attributes that are not mapped to the event schema. The names and values of those attributes are specific to the event source." .

ocsf:assignee_group  rdf:type  owl:ObjectProperty;
        rdfs:label           "Assignee Group";
        rdfs:range           ocsf:Group;
        dcterms:description  "The details of the group assigned to an Incident." .

ocsf:sub_technique  rdf:type  owl:ObjectProperty;
        rdfs:label           "Sub Technique";
        rdfs:range           ocsf:MITREATTCKSubTechnique;
        dcterms:description  "The Sub Technique object describes the sub technique ID and/or name associated to an attack, as defined by <a target='_blank' href='https://attack.mitre.org/wiki/ATT&CK_Matrix'>ATT&CK® Matrix</a>." .

ocsf:proxy_connection_info
        rdf:type             owl:ObjectProperty;
        rdfs:label           "Proxy Connection Info";
        rdfs:range           ocsf:NetworkConnectionInformation;
        dcterms:description  "The connection information from the proxy server to the remote server." .

ocsf:accessor  rdf:type      owl:ObjectProperty;
        rdfs:label           "Accessor";
        rdfs:range           ocsf:User;
        dcterms:description  "The name of the user who last accessed the object." .

ocsf:query_string  rdf:type  owl:DatatypeProperty;
        rdfs:label           "HTTP Query String";
        rdfs:range           ocsf:string_t;
        dcterms:description  "The query portion of the URL. For example: the query portion of the URL <code>http://www.example.com/search?q=bad&sort=date</code> is <code>q=bad&sort=date</code>." .

ocsf:state_id  rdf:type      owl:DatatypeProperty;
        rdfs:label           "State ID";
        rdfs:range           ocsf:integer_t;
        dcterms:description  "The normalized state ID of the event or object. See specific usage.";
        jsonschema:enum      "Other" , "Unknown" .

ocsf:is_personal  rdf:type   owl:DatatypeProperty;
        rdfs:label           "Personal Device";
        rdfs:range           ocsf:boolean_t;
        dcterms:description  "The event occurred on a personal device." .

ocsf:cis_benchmark_result
        rdf:type             owl:ObjectProperty;
        rdfs:label           "CIS Benchmark Result";
        rdfs:range           ocsf:CISBenchmarkResult;
        dcterms:description  "The CIS benchmark result." .

ocsf:start_time  rdf:type    owl:DatatypeProperty;
        rdfs:label           "Start Time";
        rdfs:range           ocsf:timestamp_t;
        dcterms:description  "The start time of a time period. See specific usage." .

ocsf:prev_security_level_id
        rdf:type             owl:DatatypeProperty;
        rdfs:label           "Previous Security Level ID";
        rdfs:range           ocsf:integer_t;
        dcterms:description  "The previous security level of the entity";
        jsonschema:enum      "Other" , "Compromised" , "At Risk" , "Secure" , "Unknown" .

ocsf:first_seen_time  rdf:type  owl:DatatypeProperty;
        rdfs:label           "First Seen";
        rdfs:range           ocsf:timestamp_t;
        dcterms:description  "The initial detection time of the activity or object. See specific usage" .

ocsf:hostname  rdf:type      owl:DatatypeProperty;
        rdfs:label           "Hostname";
        rdfs:range           ocsf:hostname_t;
        dcterms:description  "The hostname of an endpoint or a device." .

ocsf:owner  rdf:type         owl:ObjectProperty;
        rdfs:label           "Owner";
        rdfs:range           ocsf:User;
        dcterms:description  "The user that owns the file/object." .

ocsf:identifier_cookie
        rdf:type             owl:DatatypeProperty;
        rdfs:label           "Identifier Cookie";
        rdfs:range           ocsf:string_t;
        dcterms:description  "The client identifier cookie during client/server exchange." .

ocsf:proxy_tls  rdf:type     owl:ObjectProperty;
        rdfs:label           "Proxy TLS";
        rdfs:range           ocsf:TransportLayerSecurityTLS;
        dcterms:description  "The TLS protocol negotiated between the proxy server and the remote server." .

ocsf:is_renewal  rdf:type    owl:DatatypeProperty;
        rdfs:label           "Renewal";
        rdfs:range           ocsf:boolean_t;
        dcterms:description  "The indication of whether this is a lease/session renewal event." .

ocsf:duration_secs  rdf:type  owl:DatatypeProperty;
        rdfs:label           "Duration Seconds";
        rdfs:range           ocsf:integer_t;
        dcterms:description  "Represents the duration of the activity in seconds. See specific usage." .

ocsf:fixed_in_version
        rdf:type             owl:DatatypeProperty;
        rdfs:label           "Fixed In Version";
        rdfs:range           ocsf:string_t;
        dcterms:description  "The software package version in which a reported vulnerability was patched/fixed." .

ocsf:standards  rdf:type     owl:DatatypeProperty;
        rdfs:label           "Security Standards";
        rdfs:range           ocsf:string_t;
        dcterms:description  "Security standards are a set of criteria organizations can follow to protect sensitive and confidential information. e.g. <code>NIST SP 800-53, CIS AWS Foundations Benchmark v1.4.0, ISO/IEC 27001</code>" .

ocsf:auth_protocol  rdf:type  owl:DatatypeProperty;
        rdfs:label           "Auth Protocol";
        rdfs:range           ocsf:string_t;
        dcterms:description  "The authentication protocol as defined by the caption of 'auth_protocol_id'. In the case of 'Other', it is defined by the event source." .

ocsf:subdomains  rdf:type    owl:DatatypeProperty;
        rdfs:label           "Subdomains";
        rdfs:range           ocsf:string_t;
        dcterms:description  "An array of subdomain strings. Can be used to collect several subdomains such as those from Domain Generation Algorithms (DGAs)." .

ocsf:system_call  rdf:type   owl:DatatypeProperty;
        rdfs:label           "System Call";
        rdfs:range           ocsf:string_t;
        dcterms:description  "The system call that was invoked." .

ocsf:chunks  rdf:type        owl:DatatypeProperty;
        rdfs:label           "Chunks";
        rdfs:range           ocsf:long_t;
        dcterms:description  "A unit of information within an SCTP packet, consisting of a chunk header and chunk-specific content. See RFC 4960. This field can be used for the total number of chunks (in and out)." .

ocsf:is_applied  rdf:type    owl:DatatypeProperty;
        rdfs:label           "Applied";
        rdfs:range           ocsf:boolean_t;
        dcterms:description  "A determination if a policy, rule, or enforcement action was applied." .

ocsf:install_state  rdf:type  owl:DatatypeProperty;
        rdfs:label           "Install State";
        rdfs:range           ocsf:string_t;
        dcterms:description  "The install state, normalized to the caption of install_state_id. In the case of 'Other', it is defined by the event source." .

ocsf:office_location  rdf:type  owl:DatatypeProperty;
        rdfs:label           "Office Location";
        rdfs:range           ocsf:string_t;
        dcterms:description  "The primary office location associated with the user. This could be any string and isn't a specific address. For example, <code>South East Virtual</code>." .

ocsf:src_url  rdf:type       owl:DatatypeProperty;
        rdfs:label           "Source URL";
        rdfs:range           ocsf:url_t;
        dcterms:description  "The URL pointing towards the source of an entity. See specific usage." .

ocsf:loggers  rdf:type       owl:ObjectProperty;
        rdfs:label           "Loggers";
        rdfs:range           ocsf:Logger;
        dcterms:description  "An array of Logger objects that describe the devices and logging products between the event source and its eventual destination. Note, this attribute can be used when there is a complex end-to-end path of event flow." .

ocsf:confidentiality  rdf:type  owl:DatatypeProperty;
        rdfs:label           "Confidentiality";
        rdfs:range           ocsf:string_t;
        dcterms:description  "The file content confidentiality, normalized to the confidentiality_id value. In the case of 'Other', it is defined by the event source." .

ocsf:transaction_uid  rdf:type  owl:DatatypeProperty;
        rdfs:label           "Transaction UID";
        rdfs:range           ocsf:string_t;
        dcterms:description  "The unique identifier of the transaction." .

ocsf:response  rdf:type      owl:ObjectProperty;
        rdfs:label           "API Response Details";
        rdfs:range           ocsf:ResponseElements;
        dcterms:description  "General Purpose API Response Object. See specific usage." .

ocsf:desc  rdf:type          owl:DatatypeProperty;
        rdfs:label           "Description";
        rdfs:range           ocsf:string_t;
        dcterms:description  "The description that pertains to the object or event. See specific usage." .

ocsf:uid  rdf:type           owl:DatatypeProperty;
        rdfs:label           "Unique ID";
        rdfs:range           ocsf:string_t;
        dcterms:description  "The unique identifier. See specific usage." .

ocsf:raw_header  rdf:type    owl:DatatypeProperty;
        rdfs:label           "Raw Header";
        rdfs:range           ocsf:string_t;
        dcterms:description  "The email authentication header." .

ocsf:file  rdf:type          owl:ObjectProperty;
        rdfs:label           "File";
        rdfs:range           ocsf:File;
        dcterms:description  "The file that pertains to the event or object. See specific usage." .

ocsf:disposition_id  rdf:type  owl:DatatypeProperty;
        rdfs:label           "Disposition ID";
        rdfs:range           ocsf:integer_t;
        dcterms:description  "Describes the outcome or action taken by a security control, such as access control checks, malware detections or various types of policy violations.";
        jsonschema:enum      "Logged" , "Custom Action" , "Alert" , "Unauthorized" , "Unknown" , "Count" , "Challenge" , "Partially Corrected" , "Restored" , "Rejected" , "Access Revoked" , "Deleted" , "Blocked" , "Dropped" , "Error" , "Tagged" , "Detected" , "Corrected" , "Isolated" , "Approved" , "Allowed" , "Other" , "Quarantined" , "Captcha" , "Exonerated" , "Delayed" , "Uncorrected" , "Reset" , "No Action" .

ocsf:ldap_dn  rdf:type       owl:DatatypeProperty;
        rdfs:label           "LDAP Distinguished Name";
        rdfs:range           ocsf:string_t;
        dcterms:description  "The X.500 Distinguished Name (DN) is a structured string that uniquely identifies an entry, such as a user, in an X.500 directory service For example, <code>cn=John Doe,ou=People,dc=example,dc=com</code>." .

ocsf:cwe_uid  rdf:type       owl:DatatypeProperty;
        rdfs:label           "CWE UID";
        rdfs:range           ocsf:string_t;
        dcterms:description  "The <a target='_blank' href='https://cwe.mitre.org/'>Common Weakness Enumeration (CWE)</a> unique identifier. For example: <code>CWE-787</code>." .

ocsf:proxy_endpoint  rdf:type  owl:ObjectProperty;
        rdfs:label           "Proxy Endpoint";
        dcterms:description  "The proxy (server) in a network connection." .

ocsf:referrer  rdf:type      owl:DatatypeProperty;
        rdfs:label           "HTTP Referrer";
        rdfs:range           ocsf:string_t;
        dcterms:description  "The request header that identifies the address of the previous web page, which is linked to the current web page or resource being requested." .

ocsf:types  rdf:type         owl:DatatypeProperty;
        rdfs:label           "Types";
        rdfs:range           ocsf:string_t;
        dcterms:description  "The type/s of an entity. See specific usage." .

ocsf:function_keys  rdf:type  owl:DatatypeProperty;
        rdfs:label           "Function Keys";
        rdfs:range           ocsf:integer_t;
        dcterms:description  "The number of function keys on client keyboard." .

ocsf:desktop_display  rdf:type  owl:ObjectProperty;
        rdfs:label           "Desktop Display";
        rdfs:range           ocsf:Display;
        dcterms:description  "The desktop display affiliated with the event" .

ocsf:num_files  rdf:type     owl:DatatypeProperty;
        rdfs:label           "Scanned Files";
        rdfs:range           ocsf:integer_t;
        dcterms:description  "The number of files scanned." .

ocsf:tactics  rdf:type       owl:ObjectProperty;
        rdfs:label           "Tactics";
        rdfs:range           ocsf:MITREATTCKTactic;
        dcterms:description  "The Tactic object describes the tactic ID and/or tactic name that are associated with the attack technique, as defined by <a target='_blank' href='https://attack.mitre.org/wiki/ATT&CK_Matrix'>ATT&CK® Matrix</a>." .

ocsf:feature  rdf:type       owl:ObjectProperty;
        rdfs:label           "Feature";
        rdfs:range           ocsf:Feature;
        dcterms:description  "The feature that reported the event." .

ocsf:manager  rdf:type       owl:ObjectProperty;
        rdfs:label           "Manager";
        rdfs:range           ocsf:User;
        dcterms:description  "The user's manager. This helps in understanding an org hierarchy. This should only ever be populated once in an event. I.e. there should not be a manager's manager in an event." .

ocsf:key_length  rdf:type    owl:DatatypeProperty;
        rdfs:label           "Key Length";
        rdfs:range           ocsf:integer_t;
        dcterms:description  "The length of the encryption key." .

ocsf:dmarc_policy  rdf:type  owl:DatatypeProperty;
        rdfs:label           "DMARC Policy";
        rdfs:range           ocsf:string_t;
        dcterms:description  "The Domain-based Message Authentication, Reporting and Conformance (DMARC) policy status." .

ocsf:privileges  rdf:type    owl:DatatypeProperty;
        rdfs:label           "Privileges";
        rdfs:range           ocsf:string_t;
        dcterms:description  "The user or group privileges." .

ocsf:integer_t  rdf:type     rdfs:Datatype;
        rdfs:label           "Integer";
        rdfs:subClassOf      xsd:integer;
        dcterms:description  "Signed integer value." .

ocsf:vulnerability  rdf:type  owl:ObjectProperty;
        rdfs:label           "Vulnerability";
        rdfs:range           ocsf:VulnerabilityDetails;
        dcterms:description  "The vulnerability object describes details related to the observed vulnerability" .

ocsf:packages  rdf:type      owl:ObjectProperty;
        rdfs:label           "Software Packages";
        rdfs:range           ocsf:SoftwarePackage;
        dcterms:description  "List of vulnerable packages as identified by the security product" .

ocsf:cmd_line  rdf:type      owl:DatatypeProperty;
        rdfs:label           "Command Line";
        rdfs:range           ocsf:string_t;
        dcterms:description  "The full command line used to launch an application, service, process, or job. For example: <code>ssh user@10.0.0.10</code>. If the command line is unavailable or missing, the empty string <code>''</code> is to be used." .

ocsf:protocol_name  rdf:type  owl:DatatypeProperty;
        rdfs:label           "Protocol Name";
        rdfs:range           ocsf:string_t;
        dcterms:description  "The TCP/IP protocol name in lowercase, as defined by the Internet Assigned Numbers Authority (IANA). See <a target='_blank' href='https://www.iana.org/assignments/protocol-numbers/protocol-numbers.xhtml'>Protocol Numbers</a>. For example: <code>tcp</code> or <code>udp</code>." .

ocsf:rcode_id  rdf:type      owl:DatatypeProperty;
        rdfs:label           "Response Code ID";
        rdfs:range           ocsf:integer_t;
        dcterms:description  "The normalized identifier of the server response code. See specific usage.";
        jsonschema:enum      "Other" , "Unknown" .

ocsf:process  rdf:type       owl:ObjectProperty;
        rdfs:label           "Process";
        rdfs:range           ocsf:Process;
        dcterms:description  "The process object." .

ocsf:scheme  rdf:type        owl:DatatypeProperty;
        rdfs:label           "Scheme";
        rdfs:range           ocsf:string_t;
        dcterms:description  "The scheme portion of the URL. For example: <code>http</code>, <code>https</code>, <code>ftp</code>, or <code>sftp</code>." .

ocsf:severity_id  rdf:type   owl:DatatypeProperty;
        rdfs:label           "Severity ID";
        rdfs:range           ocsf:integer_t;
        dcterms:description  "<p>The normalized identifier of the event/finding severity.</p>The normalized severity is a measurement the effort and expense required to manage and resolve an event or incident. Smaller numerical values represent lower impact events, and larger numerical values represent higher impact events.";
        jsonschema:enum      "High" , "Unknown" , "Fatal" , "Critical" , "Other" , "Informational" , "Medium" , "Low" .

ocsf:entity_result  rdf:type  owl:ObjectProperty;
        rdfs:label           "Entity Result";
        rdfs:range           ocsf:ManagedEntity;
        dcterms:description  "The updated managed entity." .

ocsf:code  rdf:type          owl:DatatypeProperty;
        rdfs:label           "Response Code";
        rdfs:range           ocsf:integer_t;
        dcterms:description  "The numeric response sent to a request." .

ocsf:bytes  rdf:type         owl:DatatypeProperty;
        rdfs:label           "Total Bytes";
        rdfs:range           ocsf:long_t;
        dcterms:description  "The total number of bytes (in and out)." .

ocsf:proxy  rdf:type         owl:ObjectProperty;
        rdfs:label           "Proxy";
        dcterms:description  "The proxy (server) in a network connection." .

ocsf:score_id  rdf:type      owl:DatatypeProperty;
        rdfs:label           "Reputation Score ID";
        rdfs:range           ocsf:integer_t;
        dcterms:description  "The normalized reputation score identifier.";
        jsonschema:enum      "Safe" , "Malicious" , "Unknown" , "Other" , "May not be Safe" , "Suspicious/Risky" , "Probably Malicious" , "Probably Safe" , "Exercise Caution" , "Leans Safe" , "Possibly Malicious" , "Very Safe" .

ocsf:fingerprint  rdf:type   owl:ObjectProperty;
        rdfs:label           "Fingerprint";
        rdfs:range           ocsf:Fingerprint;
        dcterms:description  "The digital fingerprint associated with an object." .

ocsf:ack_result  rdf:type    owl:DatatypeProperty;
        rdfs:label           "Acknowledgement Result";
        rdfs:range           ocsf:integer_t;
        dcterms:description  "An integer that denotes the acknowledgment result of the DCE/RPC call." .

ocsf:num_resolutions  rdf:type  owl:DatatypeProperty;
        rdfs:label           "Resolutions";
        rdfs:range           ocsf:integer_t;
        dcterms:description  "The number of items that were resolved." .

ocsf:datetime_t  rdf:type    rdfs:Datatype;
        rdfs:label           "Datetime";
        rdfs:subClassOf      xsd:string;
        dcterms:description  "The Internet Date/Time format as defined in <a target='_blank' href='https://www.rfc-editor.org/rfc/rfc3339.html'>RFC-3339</a>. For example <code>1985-04-12T23:20:50.52Z</code>.";
        xsd:pattern          "^\\d{4}-\\d{2}-\\d{2}T\\d{2}:\\d{2}:\\d{2}(?:\\.\\d+)?(Z|[\\+-]\\d{2}:\\d{2})?$" .

ocsf:x_forwarded_for  rdf:type  owl:DatatypeProperty;
        rdfs:label           "X-Forwarded-For";
        rdfs:range           ocsf:ip_t;
        dcterms:description  "The X-Forwarded-For header identifying the originating IP address(es) of a client connecting to a web server through an HTTP proxy or a load balancer." .

ocsf:finding_info  rdf:type  owl:ObjectProperty;
        rdfs:label           "Finding Information";
        rdfs:range           ocsf:FindingInformation;
        dcterms:description  "Describes the supporting information about a generated finding." .

ocsf:kernel  rdf:type        owl:ObjectProperty;
        rdfs:label           "Kernel";
        rdfs:range           ocsf:KernelResource;
        dcterms:description  "The kernel resource object that pertains to the event." .

ocsf:certificate  rdf:type   owl:ObjectProperty;
        rdfs:label           "Certificate";
        rdfs:range           ocsf:DigitalCertificate;
        dcterms:description  "The certificate object containing information about the digital certificate." .

ocsf:container  rdf:type     owl:ObjectProperty;
        rdfs:label           "Container";
        rdfs:range           ocsf:Container;
        dcterms:description  "The information describing an instance of a container. A container is a prepackaged, portable system image that runs isolated on an existing system using a container runtime like containerd." .

ocsf:color_depth  rdf:type   owl:DatatypeProperty;
        rdfs:label           "Color Depth";
        rdfs:range           ocsf:integer_t;
        dcterms:description  "The numeric color depth." .

ocsf:enrichments  rdf:type   owl:ObjectProperty;
        rdfs:label           "Enrichments";
        rdfs:range           ocsf:Enrichment;
        dcterms:description  "The additional information from an external data source, which is associated with the event or a finding. For example add location information for the IP address in the DNS answers:</p><code>[{\"name\": \"answers.ip\", \"value\": \"92.24.47.250\", \"type\": \"location\", \"data\": {\"city\": \"Socotra\", \"continent\": \"Asia\", \"coordinates\": [-25.4153, 17.0743], \"country\": \"YE\", \"desc\": \"Yemen\"}}]</code>" .

ocsf:file_diff  rdf:type     owl:DatatypeProperty;
        rdfs:label           "File Diff";
        rdfs:range           ocsf:string_t;
        dcterms:description  "File content differences used for change detection. For example, a common use case is to identify itemized changes within INI or configuration/property setting values." .

ocsf:handshake_dur  rdf:type  owl:DatatypeProperty;
        rdfs:label           "Handshake Duration";
        rdfs:range           ocsf:integer_t;
        dcterms:description  "The amount of total time for the TLS handshake to complete after the TCP connection is established, including client-side delays, in milliseconds." .

ocsf:assignee  rdf:type      owl:ObjectProperty;
        rdfs:label           "Assignee";
        rdfs:range           ocsf:User;
        dcterms:description  "The details of the user assigned to an Incident." .

ocsf:extension_list  rdf:type  owl:ObjectProperty;
        rdfs:label           "Extension List";
        rdfs:range           ocsf:TLSExtension;
        dcterms:description  "The list of TLS extensions." .

ocsf:prev_security_states
        rdf:type             owl:ObjectProperty;
        rdfs:label           "Previous Security States";
        dcterms:description  "The previous security states. See specific usage." .

ocsf:product_uid  rdf:type   owl:DatatypeProperty;
        rdfs:label           "Product Identifier";
        rdfs:range           ocsf:string_t;
        dcterms:description  "Unique Identifier of a product." .

ocsf:cpu_bits  rdf:type      owl:DatatypeProperty;
        rdfs:label           "CPU Bits";
        rdfs:range           ocsf:integer_t;
        dcterms:description  "The cpu architecture, the number of bits used for addressing in memory. For example: <code>32</code> or <code>64</code>." .

ocsf:rate_limit  rdf:type    owl:DatatypeProperty;
        rdfs:label           "Rate Limit";
        rdfs:range           ocsf:integer_t;
        dcterms:description  "The rate limit for a rate-based rule." .

ocsf:domain_contact  rdf:type  owl:ObjectProperty;
        rdfs:label           "Domain Contact";
        rdfs:range           ocsf:DomainContact;
        dcterms:description  "The contact information related to a domain registration, e.g., registrant, administrator, abuse, billing, or technical contact." .

ocsf:is_exploit_available
        rdf:type             owl:DatatypeProperty;
        rdfs:label           "Exploit Availability";
        rdfs:range           ocsf:boolean_t;
        dcterms:description  "Indicates if an exploit or a PoC (proof-of-concept) is available for the reported vulnerability." .

ocsf:detection_pattern
        rdf:type             owl:DatatypeProperty;
        rdfs:label           "Detection Pattern";
        rdfs:range           ocsf:string_t;
        dcterms:description  "Specific pattern, algorithm, fingerpint, or model used for detection." .

ocsf:security_states  rdf:type  owl:ObjectProperty;
        rdfs:label           "Security States";
        dcterms:description  "The current security states. See specific usage." .

ocsf:priority  rdf:type      owl:DatatypeProperty;
        rdfs:label           "Priority";
        rdfs:range           ocsf:string_t;
        dcterms:description  "The priority, normalized to the caption of the priority_id value. In the case of 'Other', it is defined by the event source." .

ocsf:http_headers  rdf:type  owl:ObjectProperty;
        rdfs:label           "HTTP Headers";
        rdfs:range           ocsf:HTTPHeader;
        dcterms:description  "Additional HTTP headers of an HTTP request or response." .

ocsf:firewall_rule  rdf:type  owl:ObjectProperty;
        rdfs:label           "Firewall Rule";
        dcterms:description  "The firewall rule that triggered the event." .

ocsf:app_uid  rdf:type       owl:DatatypeProperty;
        rdfs:label           "Application ID";
        rdfs:range           ocsf:string_t;
        dcterms:description  "The unique ID of the application associated with the event or object." .

ocsf:groups  rdf:type        owl:ObjectProperty;
        rdfs:label           "Groups";
        rdfs:range           ocsf:Group;
        dcterms:description  "The groups to which an entity belongs. See specific usage." .

ocsf:query_time  rdf:type    owl:DatatypeProperty;
        rdfs:label           "Query Time";
        rdfs:range           ocsf:timestamp_t;
        dcterms:description  "The Domain Name System (DNS) query time." .

ocsf:dkim_signature  rdf:type  owl:DatatypeProperty;
        rdfs:label           "DKIM Signature";
        rdfs:range           ocsf:string_t;
        dcterms:description  "The DomainKeys Identified Mail (DKIM) signature used by the sending/receiving system." .

ocsf:chunks_in  rdf:type     owl:DatatypeProperty;
        rdfs:label           "Chunks In";
        rdfs:range           ocsf:long_t;
        dcterms:description  "A unit of information within an SCTP packet, consisting of a chunk header and chunk-specific content. See RFC 4960. This field can be used for the chunks sent from the destination to the source." .

ocsf:auth_type_id  rdf:type  owl:DatatypeProperty;
        rdfs:label           "Authentication Type ID";
        rdfs:range           ocsf:integer_t;
        dcterms:description  "The normalized identifier of the agreed upon authentication type. See specific usage.";
        jsonschema:enum      "Other" , "Unknown" .

ocsf:network_interfaces
        rdf:type             owl:ObjectProperty;
        rdfs:label           "Network Interfaces";
        rdfs:range           ocsf:NetworkInterface;
        dcterms:description  "The network interfaces that are associated with the device, one for each unique MAC address/IP address/hostname/name combination.<p><b>Note:</b> The first element of the array is the network information that pertains to the event.</p>" .

ocsf:risk_level_id  rdf:type  owl:DatatypeProperty;
        rdfs:label           "Risk Level ID";
        rdfs:range           ocsf:integer_t;
        dcterms:description  "The normalized risk level id.";
        jsonschema:enum      "Info" , "High" , "Other" , "Medium" , "Low" , "Critical" .

ocsf:server_ciphers  rdf:type  owl:DatatypeProperty;
        rdfs:label           "Server Cipher Suites";
        rdfs:range           ocsf:string_t;
        dcterms:description  "The server cipher suites that were exchanged during the TLS handshake negotiation." .

ocsf:reputation  rdf:type    owl:ObjectProperty;
        rdfs:label           "Reputation Scores";
        rdfs:range           ocsf:Reputation;
        dcterms:description  "Contains the original and normalized reputation scores." .

ocsf:bios_manufacturer
        rdf:type             owl:DatatypeProperty;
        rdfs:label           "BIOS Manufacturer";
        rdfs:range           ocsf:string_t;
        dcterms:description  "The BIOS manufacturer. For example: <code>LENOVO</code>." .

ocsf:match_details  rdf:type  owl:DatatypeProperty;
        rdfs:label           "Match Details";
        rdfs:range           ocsf:string_t;
        dcterms:description  "The data in a request that rule matched. For example: '[\"10\",\"and\",\"1\"]'." .

ocsf:data_lifecycle_state_id
        rdf:type             owl:DatatypeProperty;
        rdfs:label           "Data Lifecycle State ID";
        rdfs:range           ocsf:integer_t;
        dcterms:description  "The stage or state that the data was in when it was assessed or scanned by a data security tool.";
        jsonschema:enum      "Other" , "Data in-Use" , "Data in-Transit" , "Data at-Rest" , "Unknown" .

ocsf:chassis  rdf:type       owl:DatatypeProperty;
        rdfs:label           "Chassis";
        rdfs:range           ocsf:string_t;
        dcterms:description  "The chassis type describes the system enclosure or physical form factor. Such as the following examples for Windows <a target='_blank' href='https://docs.microsoft.com/en-us/windows/win32/cimwin32prov/win32-systemenclosure'>Windows Chassis Types</a>" .

ocsf:user  rdf:type          owl:ObjectProperty;
        rdfs:label           "User";
        rdfs:range           ocsf:User;
        dcterms:description  "The user that pertains to the event or object." .

ocsf:logged_time  rdf:type   owl:DatatypeProperty;
        rdfs:label           "Logged Time";
        rdfs:range           ocsf:timestamp_t;
        dcterms:description  "<p>The time when the logging system collected and logged the event.</p>This attribute is distinct from the event time in that event time typically contain the time extracted from the original event. Most of the time, these two times will be different." .

ocsf:impact_id  rdf:type     owl:DatatypeProperty;
        rdfs:label           "Impact ID";
        rdfs:range           ocsf:integer_t;
        dcterms:description  "The normalized impact of the finding.";
        jsonschema:enum      "Other" , "Low" , "Critical" , "Unknown" , "Medium" , "High" .

ocsf:signatures  rdf:type    owl:ObjectProperty;
        rdfs:label           "Digital Signatures";
        rdfs:range           ocsf:DigitalSignature;
        dcterms:description  "A collection of <code>Digital Signature</code> objects." .

ocsf:base_address  rdf:type  owl:DatatypeProperty;
        rdfs:label           "Base Address";
        rdfs:range           ocsf:string_t;
        dcterms:description  "The memory address where the module was loaded." .

ocsf:category  rdf:type      owl:DatatypeProperty;
        rdfs:label           "Category";
        rdfs:range           ocsf:string_t;
        dcterms:description  "The object category, normalized to the caption of <code>category_id</code>. See specific usage." .

ocsf:cpu_count  rdf:type     owl:DatatypeProperty;
        rdfs:label           "CPU Count";
        rdfs:range           ocsf:integer_t;
        dcterms:description  "The number of physical processors on a system. For example: <code>1</code>." .

ocsf:resources_result
        rdf:type             owl:ObjectProperty;
        rdfs:label           "Resource Results Array";
        dcterms:description  "Updated resources after an activity/event." .

ocsf:event_code  rdf:type    owl:DatatypeProperty;
        rdfs:label           "Event Code";
        rdfs:range           ocsf:string_t;
        dcterms:description  "The Event ID or Code that the product uses to describe the event." .

ocsf:version  rdf:type       owl:DatatypeProperty;
        rdfs:label           "Version";
        rdfs:range           ocsf:string_t;
        dcterms:description  "The version that pertains to the event or object. See specific usage." .

ocsf:compliance_references
        rdf:type             owl:ObjectProperty;
        rdfs:label           "Complaince References Articles";
        rdfs:range           ocsf:KBArticle;
        dcterms:description  "A list of sources of information or tools that help organizations understand, interpret, and implement compliance standards. They provide guidance, best practices, and examples." .

ocsf:query_result_id  rdf:type  owl:DatatypeProperty;
        rdfs:label           "Query Result ID";
        rdfs:range           ocsf:integer_t;
        dcterms:description  "The normalized identifier of the query result.";
        jsonschema:enum      "Exists" , "Error" , "Unsupported" , "Unknown" , "Other" , "Partial" , "Does not exist" .

ocsf:extensions  rdf:type    owl:ObjectProperty;
        rdfs:label           "Schema Extensions";
        rdfs:range           ocsf:SchemaExtension;
        dcterms:description  "The schema extensions used to create the event." .

ocsf:log_level  rdf:type     owl:DatatypeProperty;
        rdfs:label           "Log Level";
        rdfs:range           ocsf:string_t;
        dcterms:description  "The audit level at which an event was generated." .

ocsf:factor_type  rdf:type   owl:DatatypeProperty;
        rdfs:label           "Factor Type";
        rdfs:range           ocsf:string_t;
        dcterms:description  "The type of authentication factor used in an authentication attempt." .

ocsf:driver  rdf:type        owl:ObjectProperty;
        rdfs:label           "Kernel Driver";
        rdfs:range           ocsf:KernelExtension;
        dcterms:description  "The driver that was loaded/unloaded into the kernel" .

ocsf:users  rdf:type         owl:ObjectProperty;
        rdfs:label           "Users";
        rdfs:range           ocsf:User;
        dcterms:description  "The users that pertain to the event or object." .

ocsf:scale_factor  rdf:type  owl:DatatypeProperty;
        rdfs:label           "Scale Factor";
        rdfs:range           ocsf:integer_t;
        dcterms:description  "The numeric scale factor of display." .

ocsf:value  rdf:type         owl:DatatypeProperty;
        rdfs:label           "Value";
        rdfs:range           ocsf:string_t;
        dcterms:description  "The value that pertains to the object. See specific usage." .

ocsf:app_name  rdf:type      owl:DatatypeProperty;
        rdfs:label           "Application Name";
        rdfs:range           ocsf:string_t;
        dcterms:description  "The name of the application associated with the event or object." .

ocsf:network_endpoint
        rdf:type             owl:ObjectProperty;
        rdfs:label           "Network Endpoint";
        dcterms:description  "The Network Endpoint object describes characteristics of a network endpoint. See specific usage." .

ocsf:keyboard_layout  rdf:type  owl:DatatypeProperty;
        rdfs:label           "Keyboard Layout";
        rdfs:range           ocsf:string_t;
        dcterms:description  "The keyboard locale identifier name (e.g., en-US)." .

ocsf:auth_protocol_id
        rdf:type             owl:DatatypeProperty;
        rdfs:label           "Auth Protocol ID";
        rdfs:range           ocsf:integer_t;
        dcterms:description  "The normalized identifier of the authentication protocol used to create the user session.";
        jsonschema:enum      "OpenID" , "PAP" , "NTLM" , "Unknown" , "SAML" , "Digest" , "EAP" , "CHAP" , "Other" , "Kerberos" , "OAUTH 2.0" , "RADIUS" .

ocsf:action_id  rdf:type     owl:DatatypeProperty;
        rdfs:label           "Action ID";
        rdfs:range           ocsf:integer_t;
        dcterms:description  "The normalized action taken by a control or other policy-based system leading to an outcome or disposition.";
        jsonschema:enum      "Other" , "Denied" , "Allowed" , "Unknown" .

ocsf:decision  rdf:type      owl:DatatypeProperty;
        rdfs:label           "Authorization Decision/Outcome";
        rdfs:range           ocsf:string_t;
        dcterms:description  "Decision/outcome of the authorization mechanism (e.g. Approved, Denied)" .

ocsf:command_responses
        rdf:type             owl:DatatypeProperty;
        rdfs:label           "Command Responses";
        rdfs:range           ocsf:string_t;
        dcterms:description  "The responses to the command." .

ocsf:issuer  rdf:type        owl:DatatypeProperty;
        rdfs:label           "Issuer Details";
        rdfs:range           ocsf:string_t;
        dcterms:description  "The identifier of the issuer. See specific usage." .

ocsf:attributes  rdf:type    owl:DatatypeProperty;
        rdfs:label           "Attributes";
        rdfs:range           ocsf:integer_t;
        dcterms:description  "The bitmask value that represents the file attributes." .

ocsf:last_login_time  rdf:type  owl:DatatypeProperty;
        rdfs:label           "Last Login";
        rdfs:range           ocsf:timestamp_t;
        dcterms:description  "The last time when the user logged in." .

ocsf:bytestring_t  rdf:type  rdfs:Datatype;
        rdfs:label           "Byte String";
        rdfs:subClassOf      xsd:string;
        dcterms:description  "Base64 encoded immutable byte sequence." .

ocsf:stratum  rdf:type       owl:DatatypeProperty;
        rdfs:label           "Stratum";
        rdfs:range           ocsf:string_t;
        dcterms:description  "The stratum level of the NTP server's time source, normalized to the caption of the stratum_id value." .

ocsf:boolean_t  rdf:type     rdfs:Datatype;
        rdfs:label           "Boolean";
        rdfs:subClassOf      xsd:boolean;
        dcterms:description  "Boolean value. One of <code>true</code> or <code>false</code>." .

ocsf:class_name  rdf:type    owl:DatatypeProperty;
        rdfs:label           "Class";
        rdfs:range           ocsf:string_t;
        dcterms:description  "The event class name, as defined by class_uid value." .

ocsf:kb_articles  rdf:type   owl:DatatypeProperty;
        rdfs:label           "Knowledgebase Articles";
        rdfs:range           ocsf:string_t;
        dcterms:description  "The KB article/s related to the entity. A KB Article contains metadata that describes the patch or an update." .

ocsf:build  rdf:type         owl:DatatypeProperty;
        rdfs:label           "OS Build";
        rdfs:range           ocsf:string_t;
        dcterms:description  "The operating system build number." .

ocsf:certificate_chain
        rdf:type             owl:DatatypeProperty;
        rdfs:label           "Certificate Chain";
        rdfs:range           ocsf:string_t;
        dcterms:description  "The Chain of Certificate Serial Numbers field provides a chain of Certificate Issuer Serial Numbers leading to the Root Certificate Issuer." .

ocsf:is_secure  rdf:type     owl:DatatypeProperty;
        rdfs:label           "Secure";
        rdfs:range           ocsf:boolean_t;
        dcterms:description  "The cookie attribute indicates that cookies are sent to the server only when the request is encrypted using the HTTPS protocol." .

ocsf:severity  rdf:type      owl:DatatypeProperty;
        rdfs:label           "Severity";
        rdfs:range           ocsf:string_t;
        dcterms:description  "The event/finding severity, normalized to the caption of the severity_id value. In the case of 'Other', it is defined by the source." .

ocsf:url_t  rdf:type         rdfs:Datatype;
        rdfs:label           "URL String";
        rdfs:subClassOf      xsd:string;
        dcterms:description  "Uniform Resource Locator (URL) string. For example: <code>http://www.example.com/download/trouble.exe</code>." .

ocsf:continent  rdf:type     owl:DatatypeProperty;
        rdfs:label           "Continent";
        rdfs:range           ocsf:string_t;
        dcterms:description  "The name of the continent." .

ocsf:email_addr  rdf:type    owl:DatatypeProperty;
        rdfs:label           "Email Address";
        rdfs:range           ocsf:email_t;
        dcterms:description  "The user's primary email address." .

ocsf:profiles  rdf:type      owl:DatatypeProperty;
        rdfs:label           "Profiles";
        rdfs:range           ocsf:string_t;
        dcterms:description  "The list of profiles used to create the event.  Profiles should be referenced by their <code>name</code> attribute for core profiles, or <code>extension/name</code> for profiles from extensions." .

ocsf:ip  rdf:type            owl:DatatypeProperty;
        rdfs:label           "IP Address";
        rdfs:range           ocsf:ip_t;
        dcterms:description  "The IP address, in either IPv4 or IPv6 format." .

ocsf:last_seen_time  rdf:type  owl:DatatypeProperty;
        rdfs:label           "Last Seen";
        rdfs:range           ocsf:timestamp_t;
        dcterms:description  "The most recent detection time of the activity or object. See specific usage." .

ocsf:bytes_out  rdf:type     owl:DatatypeProperty;
        rdfs:label           "Bytes Out";
        rdfs:range           ocsf:long_t;
        dcterms:description  "The number of bytes sent from the source to the destination." .

ocsf:stratum_id  rdf:type    owl:DatatypeProperty;
        rdfs:label           "Stratum ID";
        rdfs:range           ocsf:integer_t;
        dcterms:description  "The normalized identifier of the stratum level, as defined in <a target='_blank' href='https://www.rfc-editor.org/rfc/rfc5905.html'>RFC-5905</a>.";
        jsonschema:enum      "Unknown" , "Other" , "Primary Server" , "Unsynchronized" , "Reserved" , "Secondary Server" .

ocsf:section_d  rdf:type     owl:DatatypeProperty;
        rdfs:label           "JA4 Section D";
        rdfs:range           ocsf:string_t;
        dcterms:description  "The 'd' section of the JA4 fingerprint." .

ocsf:pid  rdf:type           owl:DatatypeProperty;
        rdfs:label           "Process ID";
        rdfs:range           ocsf:integer_t;
        dcterms:description  "The process identifier, as reported by the operating system. Process ID (PID) is a number used by the operating system to uniquely identify an active process." .

ocsf:vpc_uid  rdf:type       owl:DatatypeProperty;
        rdfs:label           "VPC UID";
        rdfs:range           ocsf:string_t;
        dcterms:description  "The unique identifier of the Virtual Private Cloud (VPC)." .

ocsf:log_provider  rdf:type  owl:DatatypeProperty;
        rdfs:label           "Log Provider";
        rdfs:range           ocsf:string_t;
        dcterms:description  "The logging provider or logging service that logged the event. For example, Microsoft-Windows-Security-Auditing." .

ocsf:ip_t  rdf:type          rdfs:Datatype;
        rdfs:label           "IP Address";
        rdfs:subClassOf      xsd:string;
        dcterms:description  "Internet Protocol address (IP address), in either IPv4 or IPv6 format. For example, <code>192.168.200.24</code> or <code>2001:0db8:85a3:0000:0000:8a2e:0370:7334</code>.";
        xsd:pattern          "((^\\s*((([0-9]|[1-9][0-9]|1[0-9]{2}|2[0-4][0-9]|25[0-5]).){3}([0-9]|[1-9][0-9]|1[0-9]{2}|2[0-4][0-9]|25[0-5]))\\s*$)|(^\\s*((([0-9A-Fa-f]{1,4}:){7}([0-9A-Fa-f]{1,4}|:))|(([0-9A-Fa-f]{1,4}:){6}(:[0-9A-Fa-f]{1,4}|((25[0-5]|2[0-4]\\d|1\\d\\d|[1-9]?\\d)(.(25[0-5]|2[0-4]\\d|1\\d\\d|[1-9]?\\d)){3})|:))|(([0-9A-Fa-f]{1,4}:){5}(((:[0-9A-Fa-f]{1,4}){1,2})|:((25[0-5]|2[0-4]\\d|1\\d\\d|[1-9]?\\d)(.(25[0-5]|2[0-4]\\d|1\\d\\d|[1-9]?\\d)){3})|:))|(([0-9A-Fa-f]{1,4}:){4}(((:[0-9A-Fa-f]{1,4}){1,3})|((:[0-9A-Fa-f]{1,4})?:((25[0-5]|2[0-4]\\d|1\\d\\d|[1-9]?\\d)(.(25[0-5]|2[0-4]\\d|1\\d\\d|[1-9]?\\d)){3}))|:))|(([0-9A-Fa-f]{1,4}:){3}(((:[0-9A-Fa-f]{1,4}){1,4})|((:[0-9A-Fa-f]{1,4}){0,2}:((25[0-5]|2[0-4]\\d|1\\d\\d|[1-9]?\\d)(.(25[0-5]|2[0-4]\\d|1\\d\\d|[1-9]?\\d)){3}))|:))|(([0-9A-Fa-f]{1,4}:){2}(((:[0-9A-Fa-f]{1,4}){1,5})|((:[0-9A-Fa-f]{1,4}){0,3}:((25[0-5]|2[0-4]\\d|1\\d\\d|[1-9]?\\d)(.(25[0-5]|2[0-4]\\d|1\\d\\d|[1-9]?\\d)){3}))|:))|(([0-9A-Fa-f]{1,4}:){1}(((:[0-9A-Fa-f]{1,4}){1,6})|((:[0-9A-Fa-f]{1,4}){0,4}:((25[0-5]|2[0-4]\\d|1\\d\\d|[1-9]?\\d)(.(25[0-5]|2[0-4]\\d|1\\d\\d|[1-9]?\\d)){3}))|:))|(:(((:[0-9A-Fa-f]{1,4}){1,7})|((:[0-9A-Fa-f]{1,4}){0,5}:((25[0-5]|2[0-4]\\d|1\\d\\d|[1-9]?\\d)(.(25[0-5]|2[0-4]\\d|1\\d\\d|[1-9]?\\d)){3}))|:)))(%.+)?\\s*$))" .

ocsf:vlan_uid  rdf:type      owl:DatatypeProperty;
        rdfs:label           "VLAN";
        rdfs:range           ocsf:string_t;
        dcterms:description  "The Virtual LAN identifier." .

ocsf:lineage  rdf:type       owl:DatatypeProperty;
        rdfs:label           "Lineage";
        rdfs:range           ocsf:string_t;
        dcterms:description  "The lineage of the process, represented by a list of paths for each ancestor process. For example: <code>['/usr/sbin/sshd', '/usr/bin/bash', '/usr/bin/whoami']</code>." .

ocsf:is_hotp  rdf:type       owl:DatatypeProperty;
        rdfs:label           "HMAC-based One-time Password (HOTP)";
        rdfs:range           ocsf:boolean_t;
        dcterms:description  "Whether the authentication factor is an HMAC-based One-time Password (HOTP)." .

ocsf:provider  rdf:type      owl:DatatypeProperty;
        rdfs:label           "Provider";
        rdfs:range           ocsf:string_t;
        dcterms:description  "The origin of information associated with the event. See specific usage." .

ocsf:category_ids  rdf:type  owl:DatatypeProperty;
        rdfs:label           "Website Categorization IDs";
        rdfs:range           ocsf:integer_t;
        dcterms:description  "The Website categorization identifiers.";
        jsonschema:enum      "Malicious Sources/Malnets" , "Personals/Dating" , "Malicious Outbound Data/Botnets" , "Humor/Jokes" , "Hacking" , "E-Card/Invitations" , "Vehicles" , "Other" , "Uncategorized" , "Restaurants/Dining/Food" , "Potentially Unwanted Software" , "Abortion" , "News/Media" , "Online Meetings" , "Financial Services" , "Audio/Video Clips" , "Spam" , "Remote Access Tools" , "Translation" , "Business/Economy" , "Health" , "Sex Education" , "Phishing" , "Job Search/Careers" , "TV/Video Streams" , "Extreme" , "Dynamic DNS Host" , "Marijuana" , "Reference" , "Nudity" , "Child Pornography" , "Content Servers" , "Education" , "Real Estate" , "Informational" , "Alcohol" , "Shopping" , "Suspicious" , "File Storage/Sharing" , "Games" , "Piracy/Copyright Concerns" , "Unknown" , "Intimate Apparel/Swimsuit" , "Chat (IM)/SMS" , "Entertainment" , "Peer-to-Peer (P2P)" , "Alternative Spirituality/Belief" , "Gambling" , "Web Ads/Analytics" , "Government/Legal" , "Computer/Information Security" , "Adult/Mature Content" , "Controlled Substances" , "Art/Culture" , "Scam/Questionable/Illegal" , "Search Engines/Portals" , "Charitable Organizations" , "Sports/Recreation" , "Travel" , "Media Sharing" , "Internet Telephony" , "Radio/Audio Streams" , "Newsgroups/Forums" , "Society/Daily Living" , "Auctions" , "Pornography" , "Sexual Expression" , "For Kids" , "Email" , "Software Downloads" , "Non-Viewable/Infrastructure" , "Internet Connected Devices" , "Social Networking" , "Military" , "Placeholders" , "Technology/Internet" , "Personal Sites" , "Violence/Hate/Racism" , "Political/Social Advocacy" , "Brokerage/Trading" , "Weapons" , "Proxy Avoidance" , "Web Hosting" , "Tobacco" , "Office/Business Applications" , "Mixed Content/Potentially Adult" , "Religion" .

ocsf:cpu_type  rdf:type      owl:DatatypeProperty;
        rdfs:label           "Processor Type";
        rdfs:range           ocsf:string_t;
        dcterms:description  "The processor type. For example: <code>x86 Family 6 Model 37 Stepping 5</code>." .

ocsf:keyboard_type  rdf:type  owl:DatatypeProperty;
        rdfs:label           "Keyboard Type";
        rdfs:range           ocsf:string_t;
        dcterms:description  "The keyboard type (e.g., xt, ico)." .

ocsf:dnssec_status  rdf:type  owl:DatatypeProperty;
        rdfs:label           "DNSSEC Status";
        rdfs:range           ocsf:string_t;
        dcterms:description  "The normalized value of dnssec_status_id." .

ocsf:access_result  rdf:type  owl:DatatypeProperty;
        rdfs:label           "Access Check Result";
        rdfs:range           ocsf:json_t;
        dcterms:description  "The list of access check results." .

ocsf:num_detections  rdf:type  owl:DatatypeProperty;
        rdfs:label           "Detections";
        rdfs:range           ocsf:integer_t;
        dcterms:description  "The number of detections." .

ocsf:ldap_person  rdf:type   owl:ObjectProperty;
        rdfs:label           "LDAP Person";
        rdfs:range           ocsf:LDAPPerson;
        dcterms:description  "The additional LDAP attributes that describe a person." .

ocsf:cipher  rdf:type        owl:DatatypeProperty;
        rdfs:label           "Cipher Suite";
        rdfs:range           ocsf:string_t;
        dcterms:description  "The negotiated cipher suite." .

ocsf:finding  rdf:type       owl:ObjectProperty;
        rdfs:label           "Finding";
        rdfs:range           ocsf:Finding;
        dcterms:description  "The Finding object provides details about a finding/detection generated by a security tool." .

ocsf:data_security  rdf:type  owl:ObjectProperty;
        rdfs:label           "Data Security";
        dcterms:description  "The Data Security object describes the characteristics, techniques and content of a Data Loss Prevention (DLP), Data Loss Detection (DLD), Data Classification, or similar tools' finding, alert, or detection mechanism(s)." .

ocsf:hypervisor  rdf:type    owl:DatatypeProperty;
        rdfs:label           "Hypervisor";
        rdfs:range           ocsf:string_t;
        dcterms:description  "The name of the hypervisor running on the device. For example, <code>Xen</code>, <code>VMware</code>, <code>Hyper-V</code>, <code>VirtualBox</code>, etc." .

ocsf:traffic  rdf:type       owl:ObjectProperty;
        rdfs:label           "Traffic";
        rdfs:range           ocsf:NetworkTraffic;
        dcterms:description  "The network traffic refers to the amount of data moving across a network at a given point of time. Intended to be used alongside Network Connection." .

ocsf:actor  rdf:type         owl:ObjectProperty;
        rdfs:label           "Actor";
        rdfs:range           ocsf:Actor;
        dcterms:description  "The actor object describes details about the user/role/process that was the source of the activity." .

ocsf:dkim  rdf:type          owl:DatatypeProperty;
        rdfs:label           "DKIM Status";
        rdfs:range           ocsf:string_t;
        dcterms:description  "The DomainKeys Identified Mail (DKIM) status of the email." .

ocsf:affected_code  rdf:type  owl:ObjectProperty;
        rdfs:label           "Affected Code";
        rdfs:range           ocsf:AffectedCode;
        dcterms:description  "List of Affected Code objects that describe details about code blocks identified as vulnerable." .

ocsf:details  rdf:type       owl:DatatypeProperty;
        rdfs:label           "Details";
        rdfs:range           ocsf:string_t;
        dcterms:description  "Details of an entity. See specific usage" .

ocsf:short_desc  rdf:type    owl:DatatypeProperty;
        rdfs:label           "Short Description";
        rdfs:range           ocsf:string_t;
        dcterms:description  "The short description that pertains to the object or event. See specific usage." .

ocsf:next_run_time  rdf:type  owl:DatatypeProperty;
        rdfs:label           "Next Run";
        rdfs:range           ocsf:timestamp_t;
        dcterms:description  "The next run time. See specific usage." .

ocsf:duration_years  rdf:type  owl:DatatypeProperty;
        rdfs:label           "Duration Years";
        rdfs:range           ocsf:integer_t;
        dcterms:description  "Represents the duration of the activity in years. See specific usage." .

ocsf:subnet_uid  rdf:type    owl:DatatypeProperty;
        rdfs:label           "Subnet UID";
        rdfs:range           ocsf:string_t;
        dcterms:description  "The unique identifier of a virtual subnet." .

ocsf:account  rdf:type       owl:ObjectProperty;
        rdfs:label           "Account";
        rdfs:range           ocsf:Account;
        dcterms:description  "The account object describes details about the account that was the source or target of the activity." .

ocsf:extension  rdf:type     owl:ObjectProperty;
        rdfs:label           "Schema Extension";
        rdfs:range           ocsf:SchemaExtension;
        dcterms:description  "The schema extension used to create the event." .

ocsf:endpoint_connections
        rdf:type             owl:ObjectProperty;
        rdfs:label           "Endpoint Connections";
        dcterms:description  "Contains information about network connection attempts. See specific usage." .

ocsf:loaded_modules  rdf:type  owl:DatatypeProperty;
        rdfs:label           "Loaded Modules";
        rdfs:range           ocsf:string_t;
        dcterms:description  "The list of loaded module names." .

ocsf:state  rdf:type         owl:DatatypeProperty;
        rdfs:label           "State";
        rdfs:range           ocsf:string_t;
        dcterms:description  "The state of the event or object, normalized to the caption of the state_id value. In the case of 'Other', it is defined by the event source. See specific usage." .

ocsf:mime_type  rdf:type     owl:DatatypeProperty;
        rdfs:label           "MIME type";
        rdfs:range           ocsf:string_t;
        dcterms:description  "The Multipurpose Internet Mail Extensions (MIME) type of the file, if applicable." .

ocsf:transmit_time  rdf:type  owl:DatatypeProperty;
        rdfs:label           "Transmission Time";
        rdfs:range           ocsf:timestamp_t;
        dcterms:description  "The event transmission time from one device to another.  See specific usage." .

ocsf:class  rdf:type         owl:DatatypeProperty;
        rdfs:label           "Class";
        rdfs:range           ocsf:string_t;
        dcterms:description  "The class name of the object. See specific usage." .

ocsf:deleted_time  rdf:type  owl:DatatypeProperty;
        rdfs:label           "Deleted Time";
        rdfs:range           ocsf:timestamp_t;
        dcterms:description  "The timestamp when the user was deleted. In Active Directory (AD), when a user is deleted they are moved to a temporary container and then removed after 30 days. So, this field can be populated even after a user is deleted for the next 30 days." .

ocsf:terminal  rdf:type      owl:DatatypeProperty;
        rdfs:label           "Terminal";
        rdfs:range           ocsf:string_t;
        dcterms:description  "The Pseudo Terminal. Ex: the tty or pts value." .

ocsf:tunnel_interface
        rdf:type             owl:ObjectProperty;
        rdfs:label           "Interface";
        rdfs:range           ocsf:NetworkInterface;
        dcterms:description  "The information about the tunnel interface. See specific usage." .

ocsf:schedule_uid  rdf:type  owl:DatatypeProperty;
        rdfs:label           "Schedule UID";
        rdfs:range           ocsf:string_t;
        dcterms:description  "The unique identifier of the schedule associated with a scan job." .

ocsf:rpc_interface  rdf:type  owl:ObjectProperty;
        rdfs:label           "Remote Procedure Call Interface";
        rdfs:range           ocsf:RPCInterface;
        dcterms:description  "The RPC Interface object describes the details pertaining to the remote procedure call interface." .

ocsf:region  rdf:type        owl:DatatypeProperty;
        rdfs:label           "Region";
        rdfs:range           ocsf:string_t;
        dcterms:description  "The name or the code of a region. See specific usage." .

ocsf:boot_time  rdf:type     owl:DatatypeProperty;
        rdfs:label           "Boot Time";
        rdfs:range           ocsf:timestamp_t;
        dcterms:description  "The time when the system was booted." .

ocsf:security_descriptor
        rdf:type             owl:DatatypeProperty;
        rdfs:label           "Security Descriptor";
        rdfs:range           ocsf:string_t;
        dcterms:description  "The object security descriptor." .

ocsf:is_managed  rdf:type    owl:DatatypeProperty;
        rdfs:label           "Managed Device";
        rdfs:range           ocsf:boolean_t;
        dcterms:description  "The event occurred on a managed device." .

ocsf:mac  rdf:type           owl:DatatypeProperty;
        rdfs:label           "MAC Address";
        rdfs:range           ocsf:mac_t;
        dcterms:description  "The Media Access Control (MAC) address that is associated with the network interface." .

ocsf:malware  rdf:type       owl:ObjectProperty;
        rdfs:label           "Malware";
        rdfs:range           ocsf:Malware;
        dcterms:description  "A list of Malware objects, describing details about the identified malware." .

ocsf:categories  rdf:type    owl:DatatypeProperty;
        rdfs:label           "Website Categorization";
        rdfs:range           ocsf:string_t;
        dcterms:description  "The Website categorization names, as defined by <code>category_ids</code> enum values." .

ocsf:is_http_only  rdf:type  owl:DatatypeProperty;
        rdfs:label           "HTTP Only";
        rdfs:range           ocsf:boolean_t;
        dcterms:description  "This attribute prevents the cookie from being accessed via JavaScript." .

ocsf:samesite  rdf:type      owl:DatatypeProperty;
        rdfs:label           "SameSite";
        rdfs:range           ocsf:string_t;
        dcterms:description  "The cookie attribute that lets servers specify whether/when cookies are sent with cross-site requests. Values are: Strict, Lax or None" .

ocsf:http_method  rdf:type   owl:DatatypeProperty;
        rdfs:label           "HTTP Method";
        rdfs:range           ocsf:string_t;
        dcterms:description  "The HTTP request method indicates the desired action to be performed for a given resource. Expected values: <ul> <li>TRACE</li> <li>CONNECT</li> <li>OPTIONS</li> <li>HEAD</li> <li>DELETE</li> <li>POST</li> <li>PUT</li> <li>GET</li></ul>" .

ocsf:autonomous_system
        rdf:type             owl:ObjectProperty;
        rdfs:label           "Autonomous System";
        rdfs:range           ocsf:AutonomousSystem;
        dcterms:description  "The Autonomous System details associated with an IP address." .

ocsf:start_address  rdf:type  owl:DatatypeProperty;
        rdfs:label           "Start Address";
        rdfs:range           ocsf:string_t;
        dcterms:description  "The start address of the execution." .

ocsf:runtime  rdf:type       owl:DatatypeProperty;
        rdfs:label           "Runtime";
        rdfs:range           ocsf:string_t;
        dcterms:description  "The backend running the container, such as containerd or cri-o." .

ocsf:serial_number  rdf:type  owl:DatatypeProperty;
        rdfs:label           "Serial Number";
        rdfs:range           ocsf:string_t;
        dcterms:description  "The serial number that pertains to the object. See specific usage." .

ocsf:service  rdf:type       owl:ObjectProperty;
        rdfs:label           "Service";
        rdfs:range           ocsf:Service;
        dcterms:description  "The service that pertains to the event." .

ocsf:coordinates  rdf:type   owl:DatatypeProperty;
        rdfs:label           "Coordinates";
        rdfs:range           ocsf:float_t;
        dcterms:description  "A two-element array, containing a longitude/latitude pair. The format conforms with <a target='_blank' href='https://geojson.org'>GeoJSON</a>. For example: <code>[-73.983, 40.719]</code>." .

ocsf:signature  rdf:type     owl:ObjectProperty;
        rdfs:label           "Digital Signature";
        rdfs:range           ocsf:DigitalSignature;
        dcterms:description  "The digital signature of the file." .

ocsf:actual_permissions
        rdf:type             owl:DatatypeProperty;
        rdfs:label           "Actual Permissions";
        rdfs:range           ocsf:integer_t;
        dcterms:description  "The permissions that were granted to the in a platform-native format." .

ocsf:type_id  rdf:type       owl:DatatypeProperty;
        rdfs:label           "Type ID";
        rdfs:range           ocsf:integer_t;
        dcterms:description  "The normalized type identifier of an object. See specific usage.";
        jsonschema:enum      "Other" , "Unknown" .

ocsf:disposition  rdf:type   owl:DatatypeProperty;
        rdfs:label           "Disposition";
        rdfs:range           ocsf:string_t;
        dcterms:description  "The disposition name, normalized to the caption of the disposition_id value. In the case of 'Other', it is defined by the event source." .

ocsf:opcode_id  rdf:type     owl:DatatypeProperty;
        rdfs:label           "DNS Opcode ID";
        rdfs:range           ocsf:integer_t;
        dcterms:description  "The DNS opcode ID specifies the normalized query message type as defined in <a target='_blank' href='https://www.rfc-editor.org/rfc/rfc5395.html'>RFC-5395</a>.";
        jsonschema:enum      "Inverse Query" , "Other" , "Query" , "Update" , "Reserved" , "DSO Message" , "Notify" , "Status" .

ocsf:boundary_id  rdf:type   owl:DatatypeProperty;
        rdfs:label           "Boundary ID";
        rdfs:range           ocsf:integer_t;
        dcterms:description  "<p>The normalized identifier of the boundary of the connection. </p><p> For cloud connections, this translates to the traffic-boundary (same VPC, through IGW, etc.). For traditional networks, this is described as Local, Internal, or External.</p>";
        jsonschema:enum      "Same VPC" , "External" , "Internet Gateway" , "Other" , "Localhost" , "Virtual Private Gateway" , "Inter-region VPC" , "Gateway VPC" , "Intra-region VPC" , "Internal" , "Internet/VPC Gateway" , "Local Gateway" , "Unknown" .

ocsf:codes  rdf:type         owl:DatatypeProperty;
        rdfs:label           "Response Codes";
        rdfs:range           ocsf:integer_t;
        dcterms:description  "The list of numeric responses sent to a request." .

ocsf:direction_id  rdf:type  owl:DatatypeProperty;
        rdfs:label           "Direction ID";
        rdfs:range           ocsf:integer_t;
        dcterms:description  "The normalized identifier of the direction of the initiated connection, traffic, or email.";
        jsonschema:enum      "Other" , "Lateral" , "Outbound" , "Inbound" , "Unknown" .

ocsf:relay  rdf:type         owl:ObjectProperty;
        rdfs:label           "Relay";
        rdfs:range           ocsf:NetworkInterface;
        dcterms:description  "The network relay that is associated with the event." .

ocsf:ldap_cn  rdf:type       owl:DatatypeProperty;
        rdfs:label           "LDAP Common Name";
        rdfs:range           ocsf:string_t;
        dcterms:description  "The LDAP and X.500 <code>commonName</code> attribute, typically the full name of the person. For example, <code>John Doe</code>." .

ocsf:lease_dur  rdf:type     owl:DatatypeProperty;
        rdfs:label           "Lease Duration";
        rdfs:range           ocsf:integer_t;
        dcterms:description  "This represents the length of the DHCP lease in seconds. This is present in DHCP Ack events." .

ocsf:network_driver  rdf:type  owl:DatatypeProperty;
        rdfs:label           "Network Driver";
        rdfs:range           ocsf:string_t;
        dcterms:description  "The network driver used by the container. For example, bridge, overlay, host, none, etc." .

ocsf:num_trusted_items
        rdf:type             owl:DatatypeProperty;
        rdfs:label           "Trusted";
        rdfs:range           ocsf:integer_t;
        dcterms:description  "The number of trusted items." .

ocsf:name  rdf:type          owl:DatatypeProperty;
        rdfs:label           "Name";
        rdfs:range           ocsf:string_t;
        dcterms:description  "The name of the entity. See specific usage." .

ocsf:is_trusted  rdf:type    owl:DatatypeProperty;
        rdfs:label           "Trusted Device";
        rdfs:range           ocsf:boolean_t;
        dcterms:description  "The event occurred on a trusted device." .

ocsf:is_totp  rdf:type       owl:DatatypeProperty;
        rdfs:label           "Time-based One-time Password (TOTP)";
        rdfs:range           ocsf:boolean_t;
        dcterms:description  "Whether the authentication factor is a Time-based One-time Password (TOTP)." .

ocsf:interface_name  rdf:type  owl:DatatypeProperty;
        rdfs:label           "Network Interface Name";
        rdfs:range           ocsf:string_t;
        dcterms:description  "The name of the network interface (e.g. eth2)." .

ocsf:pod_uuid  rdf:type      owl:DatatypeProperty;
        rdfs:label           "Pod UUID";
        rdfs:range           ocsf:uuid_t;
        dcterms:description  "The unique identifier of the pod (or equivalent) that the container is executing on." .

ocsf:detection_system_id
        rdf:type             owl:DatatypeProperty;
        rdfs:label           "Detection System ID";
        rdfs:range           ocsf:integer_t;
        dcterms:description  "The type of data security tool or system that the finding, detection, or alert originated from.";
        jsonschema:enum      "Secure Web Gateway" , "Mobile Device Management" , "Unknown" , "Other" , "Data Security Posture Management" , "Cloud Access Security Broker" , "Application-Level DLP" , "Digital Rights Management" , "DLP Gateway" , "Developer Security" , "Endpoint" , "Database Activity Monitoring" , "Secure Email Gateway" , "Data Discovery & Classification" .

ocsf:overall_score  rdf:type  owl:DatatypeProperty;
        rdfs:label           "Overall Score";
        rdfs:range           ocsf:float_t;
        dcterms:description  "The overall score as reported by the event source. See specific usage." .

ocsf:status_detail  rdf:type  owl:DatatypeProperty;
        rdfs:label           "Status Detail";
        rdfs:range           ocsf:string_t;
        dcterms:description  "The status detail contains additional information about the event/finding outcome." .

ocsf:interface_uid  rdf:type  owl:DatatypeProperty;
        rdfs:label           "Network Interface ID";
        rdfs:range           ocsf:string_t;
        dcterms:description  "The unique identifier of the network interface." .

ocsf:epss  rdf:type          owl:ObjectProperty;
        rdfs:label           "EPSS";
        rdfs:range           ocsf:EPSS;
        dcterms:description  "The Exploit Prediction Scoring System (EPSS) object describes the estimated probability a vulnerability will be exploited. EPSS is a community-driven effort to combine descriptive information about vulnerabilities (CVEs) with evidence of actual exploitation in-the-wild. (<a target='_blank' href='https://www.first.org/epss/'>EPSS</a>)." .

ocsf:end_time  rdf:type      owl:DatatypeProperty;
        rdfs:label           "End Time";
        rdfs:range           ocsf:timestamp_t;
        dcterms:description  "The end time of a time period. See specific usage." .

ocsf:related_events  rdf:type  owl:ObjectProperty;
        rdfs:label           "Related Events";
        rdfs:range           ocsf:RelatedEvent;
        dcterms:description  "Describes events and/or other findings related to the finding as identified by the security product." .

ocsf:epoch  rdf:type         owl:DatatypeProperty;
        rdfs:label           "Epoch";
        rdfs:range           ocsf:integer_t;
        dcterms:description  "The software package epoch. Epoch is a way to define weighted dependencies based on version numbers." .

ocsf:dialect  rdf:type       owl:DatatypeProperty;
        rdfs:label           "Dialect";
        rdfs:range           ocsf:string_t;
        dcterms:description  "The negotiated protocol dialect." .

ocsf:injection_type  rdf:type  owl:DatatypeProperty;
        rdfs:label           "Injection Type";
        rdfs:range           ocsf:string_t;
        dcterms:description  "The process injection method, normalized to the caption of the injection_type_id value. In the case of 'Other', it is defined by the event source." .

ocsf:observables  rdf:type   owl:ObjectProperty;
        rdfs:label           "Observables";
        rdfs:range           ocsf:Observable;
        dcterms:description  "The observables associated with the event or a finding." .

ocsf:cpe_name  rdf:type      owl:DatatypeProperty;
        rdfs:label           "The product CPE identifier";
        rdfs:range           ocsf:string_t;
        dcterms:description  "The Common Platform Enumeration (CPE) name as described by (<a target='_blank' href='https://nvd.nist.gov/products/cpe'>NIST</a>) For example: <code>cpe:/a:apple:safari:16.2</code>." .

ocsf:email_auth  rdf:type    owl:ObjectProperty;
        rdfs:label           "Email Authentication";
        rdfs:range           ocsf:EmailAuthentication;
        dcterms:description  "The SPF, DKIM and DMARC attributes of an email." .

ocsf:opcode  rdf:type        owl:DatatypeProperty;
        rdfs:label           "DNS Opcode";
        rdfs:range           ocsf:string_t;
        dcterms:description  "The DNS opcode specifies the type of the query message." .

ocsf:load_type_id  rdf:type  owl:DatatypeProperty;
        rdfs:label           "Load Type ID";
        rdfs:range           ocsf:integer_t;
        dcterms:description  "The normalized identifier of the load type. See specific uasge.";
        jsonschema:enum      "Other" , "Unknown" .

ocsf:integrity_id  rdf:type  owl:DatatypeProperty;
        rdfs:label           "Integrity Level";
        rdfs:range           ocsf:integer_t;
        dcterms:description  "The normalized identifier of the process integrity level (Windows only).";
        jsonschema:enum      "Protected" , "System" , "Untrusted" , "Other" , "Medium" , "High" , "Low" , "Unknown" .

ocsf:sp_ver  rdf:type        owl:DatatypeProperty;
        rdfs:label           "OS Service Pack Version";
        rdfs:range           ocsf:integer_t;
        dcterms:description  "The version number of the latest Service Pack." .

ocsf:length  rdf:type        owl:DatatypeProperty;
        rdfs:label           "Response Length";
        rdfs:range           ocsf:integer_t;
        dcterms:description  "The HTTP response length, in number of bytes." .

ocsf:duration_hours  rdf:type  owl:DatatypeProperty;
        rdfs:label           "Duration Hours";
        rdfs:range           ocsf:integer_t;
        dcterms:description  "Represents the duration of the activity in hours. See specific usage." .

ocsf:resource  rdf:type      owl:ObjectProperty;
        rdfs:label           "Resource";
        dcterms:description  "The target resource." .

ocsf:geohash  rdf:type       owl:DatatypeProperty;
        rdfs:label           "Geohash";
        rdfs:range           ocsf:string_t;
        dcterms:description  "<p>Geohash of the geo-coordinates (latitude and longitude).</p><a target='_blank' href='https://en.wikipedia.org/wiki/Geohash'>Geohashing</a> is a geocoding system used to encode geographic coordinates in decimal degrees, to a single string." .

ocsf:is_vpn  rdf:type        owl:DatatypeProperty;
        rdfs:label           "VPN Session";
        rdfs:range           ocsf:boolean_t;
        dcterms:description  "The indication of whether the session is a VPN session." .

ocsf:detection_uid  rdf:type  owl:DatatypeProperty;
        rdfs:label           "Detection UID";
        rdfs:range           ocsf:string_t;
        dcterms:description  "The associated unique detection event identifier. For example: detection response events include the <b>Detection ID</b> of the original event." .

ocsf:physical_height  rdf:type  owl:DatatypeProperty;
        rdfs:label           "Physical Height";
        rdfs:range           ocsf:integer_t;
        dcterms:description  "The numeric physical height of display." .

ocsf:vulnerabilities  rdf:type  owl:ObjectProperty;
        rdfs:label           "Vulnerabilities";
        rdfs:range           ocsf:VulnerabilityDetails;
        dcterms:description  "This object describes vulnerabilities reported in a security finding." .

ocsf:modified_time  rdf:type  owl:DatatypeProperty;
        rdfs:label           "Modified Time";
        rdfs:range           ocsf:timestamp_t;
        dcterms:description  "The time when the object was last modified. See specific usage." .

ocsf:alert  rdf:type         owl:DatatypeProperty;
        rdfs:label           "Client TLS Alert";
        rdfs:range           ocsf:integer_t;
        dcterms:description  "The integer value of TLS alert if present. The alerts are defined in the TLS specification in <a target='_blank' href='https://datatracker.ietf.org/doc/html/rfc2246'>RFC-2246</a>." .

ocsf:subnet_t  rdf:type      rdfs:Datatype;
        rdfs:label           "Subnet";
        rdfs:subClassOf      xsd:string;
        dcterms:description  "The subnet represented in a CIDR notation, using the format network_address/prefix_length. The network_address can be in either IPv4 or IPv6 format. The prefix length indicates the number of bits used for the network portion, and the remaining bits are available for host addresses within that subnet. <div>For example:<ul><li>192.168.1.0/24</li><li>2001:0db8:85a3:0000::/64</li></ul></div>" .

ocsf:nist  rdf:type          owl:DatatypeProperty;
        rdfs:label           "NIST List";
        rdfs:range           ocsf:string_t;
        dcterms:description  "The NIST Cybersecurity Framework recommendations for managing the cybersecurity risk." .

ocsf:share_type  rdf:type    owl:DatatypeProperty;
        rdfs:label           "Share Type";
        rdfs:range           ocsf:string_t;
        dcterms:description  "The share type, normalized to the caption of the share_type_id value. In the case of 'Other', it is defined by the event source." .

ocsf:packet_uid  rdf:type    owl:DatatypeProperty;
        rdfs:label           "Packet UID";
        rdfs:range           ocsf:integer_t;
        dcterms:description  "The packet identifier assigned by the protocol." .

ocsf:postal_code  rdf:type   owl:DatatypeProperty;
        rdfs:label           "Postal Code";
        rdfs:range           ocsf:string_t;
        dcterms:description  "The postal code of the location." .

ocsf:whois  rdf:type         owl:ObjectProperty;
        rdfs:label           "WHOIS";
        rdfs:range           ocsf:WHOIS;
        dcterms:description  "The resources of a WHOIS record for a given domain. This can include domain names, IP address blocks, autonomous system information, and/or contact and registration information for a domain." .

ocsf:job  rdf:type           owl:ObjectProperty;
        rdfs:label           "Job";
        rdfs:range           ocsf:Job;
        dcterms:description  "The job object that pertains to the event." .

ocsf:file_result  rdf:type   owl:ObjectProperty;
        rdfs:label           "File Result";
        rdfs:range           ocsf:File;
        dcterms:description  "The result of the file change. It should contain the new values of the changed attributes." .

ocsf:imei  rdf:type          owl:DatatypeProperty;
        rdfs:label           "IMEI";
        rdfs:range           ocsf:string_t;
        dcterms:description  "The International Mobile Station Equipment Identifier that is associated with the device." .

ocsf:related_analytics
        rdf:type             owl:ObjectProperty;
        rdfs:label           "Related Analytics";
        rdfs:range           ocsf:Analytic;
        dcterms:description  "Describes analytics related to the analytic of a finding or detection as identified by the security product." .

ocsf:connection_info  rdf:type  owl:ObjectProperty;
        rdfs:label           "Connection Info";
        rdfs:range           ocsf:NetworkConnectionInformation;
        dcterms:description  "The network connection information." .

ocsf:banner  rdf:type        owl:DatatypeProperty;
        rdfs:label           "SMTP Banner";
        rdfs:range           ocsf:string_t;
        dcterms:description  "The initial SMTP connection response that a messaging server receives after it connects to a email server." .

ocsf:is_remote  rdf:type     owl:DatatypeProperty;
        rdfs:label           "Remote";
        rdfs:range           ocsf:boolean_t;
        dcterms:description  "The indication of whether the session is remote." .

ocsf:product  rdf:type       owl:ObjectProperty;
        rdfs:label           "Product";
        rdfs:range           ocsf:Product;
        dcterms:description  "The product that reported the event." .

ocsf:tls_extension_list
        rdf:type             owl:ObjectProperty;
        rdfs:label           "TLS Extension List";
        rdfs:range           ocsf:TLSExtension;
        dcterms:description  "The list of TLS extensions." .

ocsf:num_violations  rdf:type  owl:DatatypeProperty;
        rdfs:label           "Violations";
        rdfs:range           ocsf:integer_t;
        dcterms:description  "The number of times the policy or rule was violated." .

ocsf:duration_months  rdf:type  owl:DatatypeProperty;
        rdfs:label           "Duration Months";
        rdfs:range           ocsf:integer_t;
        dcterms:description  "Represents the duration of the activity in months. See specific usage." .

ocsf:registrar  rdf:type     owl:DatatypeProperty;
        rdfs:label           "Domain Registrar";
        rdfs:range           ocsf:string_t;
        dcterms:description  "The domain registrar." .

ocsf:dispersion  rdf:type    owl:DatatypeProperty;
        rdfs:label           "Root Dispersion";
        rdfs:range           ocsf:integer_t;
        dcterms:description  "The dispersion in the NTP protocol is the estimated time error or uncertainty relative to the reference clock in milliseconds." .

ocsf:section_b  rdf:type     owl:DatatypeProperty;
        rdfs:label           "JA4 Section B";
        rdfs:range           ocsf:string_t;
        dcterms:description  "The 'b' section of the JA4 fingerprint." .

ocsf:domain_contacts  rdf:type  owl:ObjectProperty;
        rdfs:label           "Domain Contacts";
        rdfs:range           ocsf:DomainContact;
        dcterms:description  "An array of <code>Domain Contact</code> objects." .

ocsf:num_network_items
        rdf:type             owl:DatatypeProperty;
        rdfs:label           "Scanned Network Items";
        rdfs:range           ocsf:integer_t;
        dcterms:description  "The number of network items scanned." .

ocsf:domain  rdf:type        owl:DatatypeProperty;
        rdfs:label           "Domain";
        rdfs:range           ocsf:string_t;
        dcterms:description  "The name of the domain." .

ocsf:smtp_to  rdf:type       owl:DatatypeProperty;
        rdfs:label           "SMTP To";
        rdfs:range           ocsf:email_t;
        dcterms:description  "The value of the SMTP envelope RCPT TO command." .

ocsf:install_state_id
        rdf:type             owl:DatatypeProperty;
        rdfs:label           "Install State ID";
        rdfs:range           ocsf:integer_t;
        dcterms:description  "The normalized state of the install.";
        jsonschema:enum      "Other" , "Installed Pending Reboot" , "Not Installed" , "Installed" , "Unknown" .

ocsf:control  rdf:type       owl:DatatypeProperty;
        rdfs:label           "Security Control";
        rdfs:range           ocsf:string_t;
        dcterms:description  "A Control is prescriptive, prioritized, and simplified set of best practices that one can use to strengthen their cybersecurity posture. e.g. AWS SecurityHub Controls, CIS Controls." .

ocsf:ou_uid  rdf:type        owl:DatatypeProperty;
        rdfs:label           "Org Unit ID";
        rdfs:range           ocsf:string_t;
        dcterms:description  "The alternate identifier for an entity's unique identifier. For example, its Active Directory OU DN or AWS OU ID." .

ocsf:namespace  rdf:type     owl:DatatypeProperty;
        rdfs:label           "Namespace";
        rdfs:range           ocsf:string_t;
        dcterms:description  "The namespace is useful in merger or acquisition situations. For example, when similar entities exist that you need to keep separate." .

ocsf:license  rdf:type       owl:DatatypeProperty;
        rdfs:label           "Software License";
        rdfs:range           ocsf:string_t;
        dcterms:description  "The name or identifier of the license applied on package or software. See <a target='_blank' href='https://spdx.org/licenses/'>SPDX License List</a>." .

ocsf:capabilities  rdf:type  owl:DatatypeProperty;
        rdfs:label           "Capabilities";
        rdfs:range           ocsf:string_t;
        dcterms:description  "A list of RDP capabilities." .

ocsf:packets  rdf:type       owl:DatatypeProperty;
        rdfs:label           "Total Packets";
        rdfs:range           ocsf:long_t;
        dcterms:description  "The total number of packets (in and out)." .

ocsf:end_line  rdf:type      owl:DatatypeProperty;
        rdfs:label           "End Line";
        rdfs:range           ocsf:integer_t;
        dcterms:description  "The line number of the last line of code block identified as vulnerable." .

ocsf:web_resources_result
        rdf:type             owl:ObjectProperty;
        rdfs:label           "Web Resources Result";
        dcterms:description  "The results of the activity on web resources. It should contain the new values of the changed attributes of the web resources." .

ocsf:containers  rdf:type    owl:ObjectProperty;
        rdfs:label           "Containers";
        rdfs:range           ocsf:Container;
        dcterms:description  "When working with containerized applications, the set of containers which write to the standard the output of a particular logging driver. For example, this may be the set of containers involved in handling api requests and responses for a containerized application." .

ocsf:svc_name  rdf:type      owl:DatatypeProperty;
        rdfs:label           "Service Name";
        rdfs:range           ocsf:string_t;
        dcterms:description  "The service name in service-to-service connections. For example, AWS VPC logs the pkt-src-aws-service and pkt-dst-aws-service fields identify the connection is coming from or going to an AWS service." .

ocsf:user_agent  rdf:type    owl:DatatypeProperty;
        rdfs:label           "HTTP User-Agent";
        rdfs:range           ocsf:string_t;
        dcterms:description  "The request header that identifies the operating system and web browser." .

ocsf:size  rdf:type          owl:DatatypeProperty;
        rdfs:label           "Size";
        rdfs:range           ocsf:long_t;
        dcterms:description  "The size of data, in bytes." .

ocsf:keyboard_subtype
        rdf:type             owl:DatatypeProperty;
        rdfs:label           "Keyboard Subtype";
        rdfs:range           ocsf:integer_t;
        dcterms:description  "The keyboard numeric code." .

ocsf:resources  rdf:type     owl:ObjectProperty;
        rdfs:label           "Resources Array";
        dcterms:description  "Describes details about resources that were affected by the activity/event." .

ocsf:database  rdf:type      owl:ObjectProperty;
        rdfs:label           "Database";
        rdfs:range           ocsf:Database;
        dcterms:description  "The database object is used for databases which are typically datastore services that contain an organized collection of structured and unstructured data or a types of data." .

ocsf:affected_packages
        rdf:type             owl:ObjectProperty;
        rdfs:label           "Affected Software Packages";
        rdfs:range           ocsf:AffectedSoftwarePackage;
        dcterms:description  "List of software packages identified as affected by a vulnerability/vulnerabilities." .

ocsf:bulletin  rdf:type      owl:DatatypeProperty;
        rdfs:label           "Patch Bulletin";
        rdfs:range           ocsf:string_t;
        dcterms:description  "The vendor bulletin identifier." .

ocsf:total  rdf:type         owl:DatatypeProperty;
        rdfs:label           "Total";
        rdfs:range           ocsf:integer_t;
        dcterms:description  "The total number of items. See specific usage." .

ocsf:vendor_name  rdf:type   owl:DatatypeProperty;
        rdfs:label           "Vendor Name";
        rdfs:range           ocsf:string_t;
        dcterms:description  "The name of the vendor. See specific usage." .

ocsf:org  rdf:type           owl:ObjectProperty;
        rdfs:label           "Organization";
        rdfs:range           ocsf:Organization;
        dcterms:description  "Organization and org unit relevant to the event or object." .

ocsf:uuid  rdf:type          owl:DatatypeProperty;
        rdfs:label           "UUID";
        rdfs:range           ocsf:uuid_t;
        dcterms:description  "The universally unique identifier. See specific usage." .

ocsf:response_time  rdf:type  owl:DatatypeProperty;
        rdfs:label           "Response Time";
        rdfs:range           ocsf:timestamp_t;
        dcterms:description  "The Domain Name System (DNS) response time." .

ocsf:type_name  rdf:type     owl:DatatypeProperty;
        rdfs:label           "Type Name";
        rdfs:range           ocsf:string_t;
        dcterms:description  "The event/finding type name, as defined by the type_uid." .

ocsf:location  rdf:type      owl:ObjectProperty;
        rdfs:label           "Geo Location";
        rdfs:range           ocsf:GeoLocation;
        dcterms:description  "The detailed geographical location usually associated with an IP address." .

ocsf:group_name  rdf:type    owl:DatatypeProperty;
        rdfs:label           "Group Name";
        rdfs:range           ocsf:string_t;
        dcterms:description  "The name of the group that the resource belongs to." .

ocsf:is_superseded  rdf:type  owl:DatatypeProperty;
        rdfs:label           "The patch is superseded.";
        rdfs:range           ocsf:boolean_t;
        dcterms:description  "The vendor patch has been replaced by another." .

ocsf:d3f_tactic  rdf:type    owl:ObjectProperty;
        rdfs:label           "MITRE DEFEND™ Tactic";
        rdfs:range           ocsf:MITRED3FENDTactic;
        dcterms:description  "The D3FEND Tactic object describes the defensive tactic name associated with a countermeasure, as defined by <a target='_blank' href='https://d3fend.mitre.org'>D3FEND<sup>TM</sup> Matrix</a>." .

ocsf:process_name_t  rdf:type  rdfs:Datatype;
        rdfs:label           "Process Name";
        rdfs:subClassOf      xsd:string;
        dcterms:description  "Process name. For example: <code>Notepad</code>." .

ocsf:prev_security_level
        rdf:type             owl:DatatypeProperty;
        rdfs:label           "Previous Security Level";
        rdfs:range           ocsf:string_t;
        dcterms:description  "The previous security level of the entity" .

ocsf:accessed_time  rdf:type  owl:DatatypeProperty;
        rdfs:label           "Accessed Time";
        rdfs:range           ocsf:timestamp_t;
        dcterms:description  "The time when the file was last accessed." .

ocsf:cpu_speed  rdf:type     owl:DatatypeProperty;
        rdfs:label           "Processor Speed";
        rdfs:range           ocsf:integer_t;
        dcterms:description  "The speed of the processor in Mhz. For Example: <code>4200</code>." .

ocsf:autoscale_uid  rdf:type  owl:DatatypeProperty;
        rdfs:label           "Autoscale UID";
        rdfs:range           ocsf:string_t;
        dcterms:description  "The unique identifier of the cloud autoscale configuration." .

ocsf:dmarc_override  rdf:type  owl:DatatypeProperty;
        rdfs:label           "DMARC Override";
        rdfs:range           ocsf:string_t;
        dcterms:description  "The Domain-based Message Authentication, Reporting and Conformance (DMARC) override action." .

ocsf:http_only  rdf:type     owl:DatatypeProperty;
        rdfs:label           "HTTP Only";
        rdfs:range           ocsf:boolean_t;
        dcterms:description  "A cookie attribute to make it inaccessible via JavaScript" .

ocsf:developer_uid  rdf:type  owl:DatatypeProperty;
        rdfs:label           "Developer UID";
        rdfs:range           ocsf:string_t;
        dcterms:description  "The developer ID on the certificate that signed the file." .

ocsf:risk_level  rdf:type    owl:DatatypeProperty;
        rdfs:label           "Risk Level";
        rdfs:range           ocsf:string_t;
        dcterms:description  "The risk level, normalized to the caption of the risk_level_id value." .

ocsf:reply_to  rdf:type      owl:DatatypeProperty;
        rdfs:label           "Reply To";
        rdfs:range           ocsf:email_t;
        dcterms:description  "The email header Reply-To values, as defined by RFC 5322." .

ocsf:access_list  rdf:type   owl:DatatypeProperty;
        rdfs:label           "Access List";
        rdfs:range           ocsf:string_t;
        dcterms:description  "The list of requested access rights." .

ocsf:leave_time  rdf:type    owl:DatatypeProperty;
        rdfs:label           "Leave Time";
        rdfs:range           ocsf:timestamp_t;
        dcterms:description  "The timestamp when the user left or will be leaving the organization." .

ocsf:http_cookies  rdf:type  owl:ObjectProperty;
        rdfs:label           "HTTP Cookies";
        rdfs:range           ocsf:HTTPCookie;
        dcterms:description  "The cookies object describes details about HTTP cookies" .

ocsf:factor_type_id  rdf:type  owl:DatatypeProperty;
        rdfs:label           "Factor Type ID";
        rdfs:range           ocsf:integer_t;
        dcterms:description  "The normalized identifier for the authentication factor.";
        jsonschema:enum      "Other" , "WebAuthn" , "Security Question" , "U2F" , "Hardware Token" , "Biometric" , "Phone Call" , "Password" , "Unknown" , "Email" , "SMS" , "Push Notification" , "OTP" .

ocsf:num_registry_items
        rdf:type             owl:DatatypeProperty;
        rdfs:label           "Scanned Registry Items";
        rdfs:range           ocsf:integer_t;
        dcterms:description  "The number of registry items scanned." .

ocsf:run_state_id  rdf:type  owl:DatatypeProperty;
        rdfs:label           "Run State ID";
        rdfs:range           ocsf:integer_t;
        dcterms:description  "The normalized identifier of the state of the job or service. See specific usage.";
        jsonschema:enum      "Other" , "Unknown" .

ocsf:opnum  rdf:type         owl:DatatypeProperty;
        rdfs:label           "Opnum";
        rdfs:range           ocsf:integer_t;
        dcterms:description  "An operation number used to identify a specific remote procedure call (RPC) method or a method in an interface." .

ocsf:load_balancer  rdf:type  owl:ObjectProperty;
        rdfs:label           "Load Balancer";
        rdfs:range           ocsf:LoadBalancer;
        dcterms:description  "The Load Balancer object contains information related to the device that is distributing incoming traffic to specified destinations." .

ocsf:create_mask  rdf:type   owl:DatatypeProperty;
        rdfs:label           "Create Mask";
        rdfs:range           ocsf:string_t;
        dcterms:description  "The original Windows mask that is required to create the object." .

ocsf:isp  rdf:type           owl:DatatypeProperty;
        rdfs:label           "ISP";
        rdfs:range           ocsf:string_t;
        dcterms:description  "The name of the Internet Service Provider (ISP)." .

ocsf:time  rdf:type          owl:DatatypeProperty;
        rdfs:label           "Event Time";
        rdfs:range           ocsf:timestamp_t;
        dcterms:description  "The normalized event occurrence time or the finding creation time." .

ocsf:cwe  rdf:type           owl:ObjectProperty;
        rdfs:label           "CWE";
        rdfs:range           ocsf:CWE;
        dcterms:description  "The CWE object represents a weakness in a software system that can be exploited by a threat actor to perform an attack. The CWE object is based on the <a target='_blank' href='https://cwe.mitre.org/'>Common Weakness Enumeration (CWE)</a> catalog." .

ocsf:tid  rdf:type           owl:DatatypeProperty;
        rdfs:label           "Thread ID";
        rdfs:range           ocsf:integer_t;
        dcterms:description  "The Identifier of the thread associated with the event, as returned by the operating system." .

ocsf:device  rdf:type        owl:ObjectProperty;
        rdfs:label           "Device";
        dcterms:description  "An addressable device, computer system or host." .

ocsf:credential_uid  rdf:type  owl:DatatypeProperty;
        rdfs:label           "User Credential ID";
        rdfs:range           ocsf:string_t;
        dcterms:description  "The unique identifier of the user's credential. For example, AWS Access Key ID." .

ocsf:error_message  rdf:type  owl:DatatypeProperty;
        rdfs:label           "Error Message";
        rdfs:range           ocsf:string_t;
        dcterms:description  "Error Message" .

ocsf:references  rdf:type    owl:DatatypeProperty;
        rdfs:label           "References";
        rdfs:range           ocsf:string_t;
        dcterms:description  "A list of reference URLs supporting the finding/detection." .

ocsf:dnssec_status_id
        rdf:type             owl:DatatypeProperty;
        rdfs:label           "DNSSEC Status ID";
        rdfs:range           ocsf:integer_t;
        dcterms:description  "Describes the normalized status of DNS Security Extensions (DNSSEC) for a domain.";
        jsonschema:enum      "Other" , "Unsigned" , "Signed" , "Unknown" .

ocsf:kb_article_list  rdf:type  owl:ObjectProperty;
        rdfs:label           "Knowledgebase Articles";
        rdfs:range           ocsf:KBArticle;
        dcterms:description  "A list of KB articles or patches related to an endpoint. A KB Article contains metadata that describes the patch or an update." .

ocsf:attempt  rdf:type       owl:DatatypeProperty;
        rdfs:label           "Attempt";
        rdfs:range           ocsf:integer_t;
        dcterms:description  "The delivery attempt." .

ocsf:x_originating_ip
        rdf:type             owl:DatatypeProperty;
        rdfs:label           "X-Originating-IP";
        rdfs:range           ocsf:ip_t;
        dcterms:description  "The X-Originating-IP header identifying the emails originating IP address(es)." .

ocsf:secure  rdf:type        owl:DatatypeProperty;
        rdfs:label           "Secure";
        rdfs:range           ocsf:boolean_t;
        dcterms:description  "The cookie attribute to only send cookies to the server with an encrypted request over the HTTPS protocol." .

ocsf:cloud  rdf:type         owl:ObjectProperty;
        rdfs:label           "Cloud";
        rdfs:range           ocsf:Cloud;
        dcterms:description  "Describes details about the Cloud environment where the event was originally created or logged." .

ocsf:detection_system
        rdf:type             owl:DatatypeProperty;
        rdfs:label           "Detection System";
        rdfs:range           ocsf:string_t;
        dcterms:description  "The name of the type of data security tool or system that the finding, detection, or alert originated from. E.g., Endpoint, Secure Email Gateway, etc." .

ocsf:hashes  rdf:type        owl:ObjectProperty;
        rdfs:label           "Hashes";
        rdfs:range           ocsf:Fingerprint;
        dcterms:description  "An array of hash attributes." .

ocsf:confidentiality_id
        rdf:type             owl:DatatypeProperty;
        rdfs:label           "Confidentiality ID";
        rdfs:range           ocsf:integer_t;
        dcterms:description  "The normalized identifier of the file content confidentiality indicator.";
        jsonschema:enum      "Top Secret" , "Other" , "Secret" , "Private" , "Not Confidential" , "Restricted" , "Unknown" , "Confidential" .

ocsf:category_uid  rdf:type  owl:DatatypeProperty;
        rdfs:label           "Category ID";
        rdfs:range           ocsf:integer_t;
        dcterms:description  "The category unique identifier of the event." .

ocsf:ext  rdf:type           owl:DatatypeProperty;
        rdfs:label           "Extension";
        rdfs:range           ocsf:string_t;
        dcterms:description  "The extension. See specific usage." .

ocsf:cpu_cores  rdf:type     owl:DatatypeProperty;
        rdfs:label           "CPU Cores";
        rdfs:range           ocsf:integer_t;
        dcterms:description  "The number of processor cores in all installed processors. For Example: <code>42</code>." .

ocsf:data_sources  rdf:type  owl:DatatypeProperty;
        rdfs:label           "Data Sources";
        rdfs:range           ocsf:string_t;
        dcterms:description  "A list of data sources utilized in generation of the finding." .

ocsf:score  rdf:type         owl:DatatypeProperty;
        rdfs:label           "Reputation Score";
        rdfs:range           ocsf:string_t;
        dcterms:description  "The reputation score, normalized to the caption of the score_id value. In the case of 'Other', it is defined by the event source." .

ocsf:smtp_hello  rdf:type    owl:DatatypeProperty;
        rdfs:label           "SMTP Hello";
        rdfs:range           ocsf:string_t;
        dcterms:description  "The value of the SMTP HELO or EHLO command." .

ocsf:avg_timespan  rdf:type  owl:ObjectProperty;
        rdfs:label           "Average Timespan";
        rdfs:range           ocsf:TimeSpan;
        dcterms:description  "The average time span of an activity." .

ocsf:auth_factors  rdf:type  owl:ObjectProperty;
        rdfs:label           "Authentication Factors";
        dcterms:description  "Describes a category of methods used for identity verification in an authentication attempt." .

ocsf:cc  rdf:type            owl:DatatypeProperty;
        rdfs:label           "Cc";
        rdfs:range           ocsf:email_t;
        dcterms:description  "The email header Cc values, as defined by RFC 5322." .

ocsf:rule  rdf:type          owl:ObjectProperty;
        rdfs:label           "Rule";
        rdfs:range           ocsf:Rule;
        dcterms:description  "The rules that reported the events." .

ocsf:classification  rdf:type  owl:DatatypeProperty;
        rdfs:label           "Classification";
        rdfs:range           ocsf:string_t;
        dcterms:description  "The classification as defined by the vendor." .

ocsf:namespace_pid  rdf:type  owl:DatatypeProperty;
        rdfs:label           "Namespace PID";
        rdfs:range           ocsf:integer_t;
        dcterms:description  "If running under a process namespace (such as in a container), the process identifier within that process namespace." .

ocsf:surname  rdf:type       owl:DatatypeProperty;
        rdfs:label           "Surname";
        rdfs:range           ocsf:string_t;
        dcterms:description  "The last or family name for the user." .

ocsf:is_cleartext  rdf:type  owl:DatatypeProperty;
        rdfs:label           "Cleartext Credentials";
        rdfs:range           ocsf:boolean_t;
        dcterms:description  "Indicates whether the credentials were passed in clear text.<p><b>Note:</b> True if the credentials were passed in a clear text protocol such as FTP or TELNET, or if Windows detected that a user's logon password was passed to the authentication package in clear text.</p>" .

ocsf:integrity  rdf:type     owl:DatatypeProperty;
        rdfs:label           "Integrity";
        rdfs:range           ocsf:string_t;
        dcterms:description  "The process integrity level, normalized to the caption of the integrity_id value. In the case of 'Other', it is defined by the event source (Windows only)." .

ocsf:cves  rdf:type          owl:ObjectProperty;
        rdfs:label           "CVE List";
        rdfs:range           ocsf:CVE;
        dcterms:description  "List of Common Vulnerabilities and Exposures (<a target='_blank' href='https://cve.mitre.org/'>CVE</a>)." .

ocsf:open_mask  rdf:type     owl:DatatypeProperty;
        rdfs:label           "Open Mask";
        rdfs:range           ocsf:integer_t;
        dcterms:description  "The Windows options needed to open a registry key." .

ocsf:type_uid  rdf:type      owl:DatatypeProperty;
        rdfs:label           "Type ID";
        rdfs:range           ocsf:long_t;
        dcterms:description  "The event/finding type ID. It identifies the event's semantics and structure. The value is calculated by the logging system as: <code>class_uid * 100 + activity_id</code>." .

ocsf:flag_ids  rdf:type      owl:DatatypeProperty;
        rdfs:label           "Communication Flag IDs";
        rdfs:range           ocsf:integer_t;
        dcterms:description  "The list of normalized identifiers of the communication flag IDs. See specific usage.";
        jsonschema:enum      "Other" , "Unknown" .

ocsf:status_code  rdf:type   owl:DatatypeProperty;
        rdfs:label           "Status Code";
        rdfs:range           ocsf:string_t;
        dcterms:description  "The event status code, as reported by the event source.<br /><br />For example, in a Windows Failed Authentication event, this would be the value of 'Failure Code', e.g. 0x18." .

ocsf:command_response
        rdf:type             owl:DatatypeProperty;
        rdfs:label           "Command Response";
        rdfs:range           ocsf:string_t;
        dcterms:description  "The response to the command." .

ocsf:evidences  rdf:type     owl:ObjectProperty;
        rdfs:label           "Evidence Artifacts";
        rdfs:range           ocsf:EvidenceArtifacts;
        dcterms:description  "Describes various evidence artifacts associated to the activity/activities that triggered a security detection." .

ocsf:query  rdf:type         owl:ObjectProperty;
        rdfs:label           "DNS Query";
        rdfs:range           ocsf:DNSQuery;
        dcterms:description  "The Domain Name System (DNS) query." .

ocsf:bios_date  rdf:type     owl:DatatypeProperty;
        rdfs:label           "BIOS Date";
        rdfs:range           ocsf:string_t;
        dcterms:description  "The BIOS date. For example: <code>03/31/16</code>." .

ocsf:proxy_http_response
        rdf:type             owl:ObjectProperty;
        rdfs:label           "Proxy HTTP Response";
        rdfs:range           ocsf:HTTPResponse;
        dcterms:description  "The HTTP Response from the remote server to the proxy server." .

ocsf:email_t  rdf:type       rdfs:Datatype;
        rdfs:label           "Email Address";
        rdfs:subClassOf      xsd:string;
        dcterms:description  "Email address. For example: <code>john_doe@example.com</code>.";
        xsd:pattern          "^[a-zA-Z0-9!#$%&'*+-/=?^_`{|}~.]+@[a-zA-Z0-9-]+\\.[a-zA-Z0-9-.]+$" .

ocsf:http_request  rdf:type  owl:ObjectProperty;
        rdfs:label           "HTTP Request";
        rdfs:range           ocsf:HTTPRequest;
        dcterms:description  "The HTTP Request Object documents attributes of a request made to a web server." .

ocsf:kill_chain  rdf:type    owl:ObjectProperty;
        rdfs:label           "Kill Chain";
        rdfs:range           ocsf:KillChainPhase;
        dcterms:description  "The <a target='_blank' href='https://www.lockheedmartin.com/en-us/capabilities/cyber/cyber-kill-chain.html'>Cyber Kill Chain®</a> provides a detailed description of each phase and its associated activities within the broader context of a cyber attack." .

ocsf:scan  rdf:type          owl:ObjectProperty;
        rdfs:label           "Scan";
        rdfs:range           ocsf:Scan;
        dcterms:description  "The Scan object describes characteristics of a scan.  See specific usage." .

ocsf:long_t  rdf:type        rdfs:Datatype;
        rdfs:label           "Long";
        rdfs:subClassOf      xsd:long;
        dcterms:description  "8-byte long, signed integer value." .

ocsf:load_type  rdf:type     owl:DatatypeProperty;
        rdfs:label           "Load Type";
        rdfs:range           ocsf:string_t;
        dcterms:description  "The load type, normalized to the caption of the load_type_id value. In the case of 'Other', it is defined by the event source." .

ocsf:idp  rdf:type           owl:ObjectProperty;
        rdfs:label           "Identity Provider";
        rdfs:range           ocsf:IdentityProvider;
        dcterms:description  "This object describes details about the Identity Provider used." .

ocsf:protocol_ver_id  rdf:type  owl:DatatypeProperty;
        rdfs:label           "Protocol Version ID";
        rdfs:range           ocsf:integer_t;
        dcterms:description  "The normalized identifier of the Protocol version. See specific usage.";
        jsonschema:enum      "Other" , "Unknown" .

ocsf:session  rdf:type       owl:ObjectProperty;
        rdfs:label           "Session";
        rdfs:range           ocsf:Session;
        dcterms:description  "The authenticated user or service session." .

ocsf:comment  rdf:type       owl:DatatypeProperty;
        rdfs:label           "Comment";
        rdfs:range           ocsf:string_t;
        dcterms:description  "The user-provided comment." .

ocsf:dkim_domain  rdf:type   owl:DatatypeProperty;
        rdfs:label           "DKIM Domain";
        rdfs:range           ocsf:string_t;
        dcterms:description  "The DomainKeys Identified Mail (DKIM) signing domain of the email." .

ocsf:city  rdf:type          owl:DatatypeProperty;
        rdfs:label           "City";
        rdfs:range           ocsf:string_t;
        dcterms:description  "The name of the city." .

ocsf:logon_process  rdf:type  owl:ObjectProperty;
        rdfs:label           "Logon Process";
        rdfs:range           ocsf:Process;
        dcterms:description  "The trusted process that validated the authentication credentials." .

ocsf:confidence  rdf:type    owl:DatatypeProperty;
        rdfs:label           "Confidence";
        rdfs:range           ocsf:string_t;
        dcterms:description  "The confidence, normalized to the caption of the confidence_id value. In the case of 'Other', it is defined by the event source." .

ocsf:given_name  rdf:type    owl:DatatypeProperty;
        rdfs:label           "Given Name";
        rdfs:range           ocsf:string_t;
        dcterms:description  "The given or first name of the user." .

ocsf:action  rdf:type        owl:DatatypeProperty;
        rdfs:label           "Action";
        rdfs:range           ocsf:string_t;
        dcterms:description  "The normalized caption of 'action_id' or the source specific action." .

ocsf:precision  rdf:type     owl:DatatypeProperty;
        rdfs:label           "Precision";
        rdfs:range           ocsf:integer_t;
        dcterms:description  "The numeric precision. See specific usage." .

ocsf:resource_type  rdf:type  owl:DatatypeProperty;
        rdfs:label           "Resource Type";
        rdfs:range           ocsf:string_t;
        dcterms:description  "The resource type as defined by the event source." .

ocsf:classification_ids
        rdf:type             owl:DatatypeProperty;
        rdfs:label           "Classification IDs";
        rdfs:range           ocsf:integer_t;
        dcterms:description  "The list of normalized classification identifiers. See specific usage.";
        jsonschema:enum      "Other" , "Unknown" .

ocsf:duration  rdf:type      owl:DatatypeProperty;
        rdfs:label           "Duration Milliseconds";
        rdfs:range           ocsf:long_t;
        dcterms:description  "This represents the duration of the activity in milliseconds. See specific usage." .

ocsf:duration_days  rdf:type  owl:DatatypeProperty;
        rdfs:label           "Duration Days";
        rdfs:range           ocsf:integer_t;
        dcterms:description  "Represents the duration of the activity in days. See specific usage." .

ocsf:release  rdf:type       owl:DatatypeProperty;
        rdfs:label           "Software Release Details";
        rdfs:range           ocsf:string_t;
        dcterms:description  "Release is the number of times a version of the software has been packaged." .

ocsf:cloud_partition  rdf:type  owl:DatatypeProperty;
        rdfs:label           "Cloud Partition";
        rdfs:range           ocsf:string_t;
        dcterms:description  "The canonical cloud partition name to which the region is assigned (e.g. AWS Partitions: aws, aws-cn, aws-us-gov)." .

ocsf:dce_rpc  rdf:type       owl:ObjectProperty;
        rdfs:label           "Distributed Computing Environment/Remote Procedure Call (DCE/RPC)";
        rdfs:range           ocsf:DCERPC;
        dcterms:description  "The DCE/RPC object describes the remote procedure call system for distributed computing environments." .

ocsf:web_resources  rdf:type  owl:ObjectProperty;
        rdfs:label           "Web Resources";
        dcterms:description  "Describes details about web resources that were affected by an activity/event." .

ocsf:rdata  rdf:type         owl:DatatypeProperty;
        rdfs:label           "DNS RData";
        rdfs:range           ocsf:string_t;
        dcterms:description  "The data describing the DNS resource. The meaning of this data depends on the type and class of the resource record." .

ocsf:num_processes  rdf:type  owl:DatatypeProperty;
        rdfs:label           "Scanned Processes";
        rdfs:range           ocsf:integer_t;
        dcterms:description  "The number of processes scanned." .

ocsf:string_t  rdf:type      rdfs:Datatype;
        rdfs:label           "String";
        rdfs:subClassOf      xsd:string;
        dcterms:description  "UTF-8 encoded byte sequence." .

ocsf:subnet_prefix  rdf:type  owl:DatatypeProperty;
        rdfs:label           "Subnet Prefix Length";
        rdfs:range           ocsf:integer_t;
        dcterms:description  "The subnet prefix length determines the number of bits used to represent the network part of the IP address. The remaining bits are reserved for identifying individual hosts within that subnet." .

ocsf:classifications  rdf:type  owl:DatatypeProperty;
        rdfs:label           "Classifications";
        rdfs:range           ocsf:string_t;
        dcterms:description  "The list of malware classifications, normalized to the captions of the classification_id values. In the case of 'Other', they are defined by the event source." .

ocsf:duration_weeks  rdf:type  owl:DatatypeProperty;
        rdfs:label           "Duration Weeks";
        rdfs:range           ocsf:integer_t;
        dcterms:description  "Represents the duration of the activity in weeks. See specific usage." .

ocsf:customer_uid  rdf:type  owl:DatatypeProperty;
        rdfs:label           "Customer UID";
        rdfs:range           ocsf:string_t;
        dcterms:description  "The unique customer identifier." .

ocsf:pattern_match  rdf:type  owl:DatatypeProperty;
        rdfs:label           "Pattern Match";
        rdfs:range           ocsf:string_t;
        dcterms:description  "A text, binary, file name, or datastore that matched against a detection rule." .

ocsf:parent_process  rdf:type  owl:ObjectProperty;
        rdfs:label           "Parent Process";
        rdfs:range           ocsf:Process;
        dcterms:description  "The parent process of this process object. It is recommended to only populate this field for the first process object, to prevent deep nesting." .

ocsf:ime  rdf:type           owl:DatatypeProperty;
        rdfs:label           "IME";
        rdfs:range           ocsf:string_t;
        dcterms:description  "The Input Method Editor (IME) file name." .

ocsf:cis_controls  rdf:type  owl:ObjectProperty;
        rdfs:label           "CIS Controls";
        rdfs:range           ocsf:CISControl;
        dcterms:description  "The CIS Critical Security Controls is a prioritized set of actions to protect your organization and data from cyber-attack vectors." .

ocsf:tlp  rdf:type           owl:DatatypeProperty;
        rdfs:label           "Traffic Light Protocol";
        rdfs:range           ocsf:string_t;
        dcterms:description  "The <a target='_blank' href='https://www.first.org/tlp/'>Traffic Light Protocol</a> was created to facilitate greater sharing of potentially sensitive information and more effective collaboration. TLP provides a simple and intuitive schema for indicating with whom potentially sensitive information can be shared." .

ocsf:subdomain  rdf:type     owl:DatatypeProperty;
        rdfs:label           "Subdomain";
        rdfs:range           ocsf:string_t;
        dcterms:description  "The subdomain portion of the URL. For example: <code>sub</code> in <code>https://sub.example.com</code> or <code>sub2.sub1</code> in <code>https://sub2.sub1.example.com</code>." .

ocsf:priority_id  rdf:type   owl:DatatypeProperty;
        rdfs:label           "Priority ID";
        rdfs:range           ocsf:integer_t;
        dcterms:description  "The normalized priority. Priority identifies the relative importance of the finding. It is a measurement of urgency.";
        jsonschema:enum      "High" , "Medium" , "Critical" , "Low" , "Other" , "Unknown" .

ocsf:bytes_in  rdf:type      owl:DatatypeProperty;
        rdfs:label           "Bytes In";
        rdfs:range           ocsf:long_t;
        dcterms:description  "The number of bytes sent from the destination to the source." .

ocsf:group  rdf:type         owl:ObjectProperty;
        rdfs:label           "Group";
        rdfs:range           ocsf:Group;
        dcterms:description  "The group object associated with an entity such as user, policy, or rule." .

ocsf:from  rdf:type          owl:DatatypeProperty;
        rdfs:label           "From";
        rdfs:range           ocsf:email_t;
        dcterms:description  "The email header From values, as defined by RFC 5322." .

ocsf:sni  rdf:type           owl:DatatypeProperty;
        rdfs:label           "Server Name Indication";
        rdfs:range           ocsf:string_t;
        dcterms:description  " The Server Name Indication (SNI) extension sent by the client." .

ocsf:connection_uid  rdf:type  owl:DatatypeProperty;
        rdfs:label           "Connection Identifier";
        rdfs:range           ocsf:string_t;
        dcterms:description  "The network connection identifier." .

ocsf:query_result  rdf:type  owl:DatatypeProperty;
        rdfs:label           "Query Result";
        rdfs:range           ocsf:string_t;
        dcterms:description  "The result of the query." .

ocsf:message  rdf:type       owl:DatatypeProperty;
        rdfs:label           "Message";
        rdfs:range           ocsf:string_t;
        dcterms:description  "The description of the event/finding, as defined by the source." .

ocsf:exit_code  rdf:type     owl:DatatypeProperty;
        rdfs:label           "Exit Code";
        rdfs:range           ocsf:integer_t;
        dcterms:description  "The exit code reported by a process when it terminates. The convention is that zero indicates success and any non-zero exit code indicates that some error occurred." .

ocsf:compliance_standards
        rdf:type             owl:ObjectProperty;
        rdfs:label           "Compliance Standards Articles";
        rdfs:range           ocsf:KBArticle;
        dcterms:description  "A list of established guidelines or criteria that define specific requirements an organization must follow." .

ocsf:agent_list  rdf:type    owl:ObjectProperty;
        rdfs:label           "Agent List";
        dcterms:description  "A list of <code>agent</code> objects associated with a device, endpoint, or resource." .

ocsf:logon_type  rdf:type    owl:DatatypeProperty;
        rdfs:label           "Logon Type";
        rdfs:range           ocsf:string_t;
        dcterms:description  "The logon type, normalized to the caption of the logon_type_id value. In the case of 'Other', it is defined by the event source." .

ocsf:json_t  rdf:type        rdfs:Datatype;
        rdfs:label           "JSON";
        rdfs:subClassOf      rdf:JSON;
        dcterms:description  "Embedded JSON value. A value can be a string, or a number, or true or false or null, or an object or an array. These structures can be nested. See <a target='_blank' href='https://www.json.org'>www.json.org</a>." .

ocsf:sequence  rdf:type      owl:DatatypeProperty;
        rdfs:label           "Sequence Number";
        rdfs:range           ocsf:integer_t;
        dcterms:description  "Sequence number of the event. The sequence number is a value available in some events, to make the exact ordering of events unambiguous, regardless of the event time precision." .

ocsf:creator  rdf:type       owl:ObjectProperty;
        rdfs:label           "Creator";
        rdfs:range           ocsf:User;
        dcterms:description  "The user that created the object associated with event. See specific usage." .
