@prefix d3f:        <http://d3fend.mitre.org/ontologies/d3fend.owl#> .
@prefix dcterms:    <http://purl.org/dc/terms/> .
@prefix fun:        <http://w3id.org/sparql-generate/fn/> .
@prefix iter:       <http://w3id.org/sparql-generate/iter/> .
@prefix jsonschema: <https://www.w3.org/2019/wot/json-schema#> .
@prefix ocsf:       <https://schema.ocsf.io/1.1.0-dev/ontology/> .
@prefix owl:        <http://www.w3.org/2002/07/owl#> .
@prefix rdf:        <http://www.w3.org/1999/02/22-rdf-syntax-ns#> .
@prefix rdfs:       <http://www.w3.org/2000/01/rdf-schema#> .
@prefix skos:       <http://www.w3.org/2004/02/skos/core#> .
@prefix xsd:        <http://www.w3.org/2001/XMLSchema#> .

ocsf:http_only  rdf:type     owl:DatatypeProperty;
        rdfs:label           "HTTP Only";
        rdfs:range           ocsf:boolean_t;
        dcterms:description  "A cookie attribute to make it inaccessible via JavaScript" .

ocsf:bios_manufacturer
        rdf:type             owl:DatatypeProperty;
        rdfs:label           "BIOS Manufacturer";
        rdfs:range           ocsf:string_t;
        dcterms:description  "The BIOS manufacturer. For example: <code>LENOVO</code>." .

ocsf:file_result  rdf:type   owl:ObjectProperty;
        rdfs:label           "File Result";
        rdfs:range           ocsf:File;
        dcterms:description  "The result of the file change. It should contain the new values of the changed attributes." .

ocsf:percentile  rdf:type    owl:DatatypeProperty;
        rdfs:label           "EPSS Percentile";
        rdfs:range           ocsf:float_t;
        dcterms:description  "The EPSS score's percentile representing relative importance and ranking of the score in the larger EPSS dataset." .

ocsf:cis_benchmark_result
        rdf:type             owl:ObjectProperty;
        rdfs:label           "CIS Benchmark Result";
        rdfs:range           ocsf:CISBenchmarkResult;
        dcterms:description  "The CIS benchmark result." .

ocsf:isp  rdf:type           owl:DatatypeProperty;
        rdfs:label           "ISP";
        rdfs:range           ocsf:string_t;
        dcterms:description  "The name of the Internet Service Provider (ISP)." .

ocsf:dispersion  rdf:type    owl:DatatypeProperty;
        rdfs:label           "Root Dispersion";
        rdfs:range           ocsf:integer_t;
        dcterms:description  "The dispersion in the NTP protocol is the estimated time error or uncertainty relative to the reference clock in milliseconds." .

ocsf:Logger  rdf:type        owl:Class;
        rdfs:label           "Logger";
        rdfs:subClassOf      ocsf:Entity;
        rdfs:subClassOf      [ rdf:type            owl:Restriction;
                               owl:onProperty      ocsf:product;
                               owl:someValuesFrom  ocsf:Product
                             ];
        rdfs:subClassOf      [ rdf:type            owl:Restriction;
                               owl:onProperty      ocsf:device;
                               owl:someValuesFrom  ocsf:Device
                             ];
        dcterms:description  "The Logger object represents the device and product where events are stored with times for receipt and transmission.  This may be at the source device where the event occurred, a remote scanning device, intermediate hops, or the ultimate destination.";
        ocsf:name            "logger" .

ocsf:decision  rdf:type      owl:DatatypeProperty;
        rdfs:label           "Authorization Decision/Outcome";
        rdfs:range           ocsf:string_t;
        dcterms:description  "Decision/outcome of the authorization mechanism (e.g. Approved, Denied)" .

ocsf:integrity  rdf:type     owl:DatatypeProperty;
        rdfs:label           "Integrity";
        rdfs:range           ocsf:string_t;
        dcterms:description  "The process integrity level, normalized to the caption of the direction_id value. In the case of 'Other', it is defined by the event source (Windows only)." .

ocsf:autoscale_uid  rdf:type  owl:DatatypeProperty;
        rdfs:label           "Autoscale UID";
        rdfs:range           ocsf:string_t;
        dcterms:description  "The unique identifier of the cloud autoscale configuration." .

ocsf:loaded_modules  rdf:type  owl:DatatypeProperty;
        rdfs:label           "Loaded Modules";
        rdfs:range           ocsf:string_t;
        dcterms:description  "The list of loaded module names." .

ocsf:traffic  rdf:type       owl:ObjectProperty;
        rdfs:label           "Traffic";
        rdfs:range           ocsf:NetworkTraffic;
        dcterms:description  "The network traffic refers to the amount of data moving across a network at a given point of time. Intended to be used alongside Network Connection." .

ocsf:response  rdf:type      owl:ObjectProperty;
        rdfs:label           "API Response Details";
        rdfs:range           ocsf:ResponseElements;
        dcterms:description  "General Purpose API Response Object. See specific usage." .

ocsf:cpu_type  rdf:type      owl:DatatypeProperty;
        rdfs:label           "Processor Type";
        rdfs:range           ocsf:string_t;
        dcterms:description  "The processor type. For example: <code>x86 Family 6 Model 37 Stepping 5</code>." .

ocsf:caption  rdf:type       owl:DatatypeProperty;
        rdfs:label           "Caption";
        rdfs:range           ocsf:string_t;
        dcterms:description  "A short description or caption of the device. For example: <code>Scanner 1</code> or <code>Database Manager</code>." .

ocsf:match_location  rdf:type  owl:DatatypeProperty;
        rdfs:label           "Match Location";
        rdfs:range           ocsf:string_t;
        dcterms:description  "The location of the matched data in the source which resulted in the triggered firewall rule. For example: HEADER." .

ocsf:modifier  rdf:type      owl:ObjectProperty;
        rdfs:label           "Modifier";
        rdfs:range           ocsf:User;
        dcterms:description  "The user that last modified the object associated with the event. See specific usage." .

ocsf:leave_time  rdf:type    owl:DatatypeProperty;
        rdfs:label           "Leave Time";
        rdfs:range           ocsf:timestamp_t;
        dcterms:description  "The timestamp when the user left or will be leaving the organization." .

ocsf:http_headers  rdf:type  owl:ObjectProperty;
        rdfs:label           "HTTP Headers";
        rdfs:range           ocsf:HTTPHeader;
        dcterms:description  "Additional HTTP headers of an HTTP request or response." .

ocsf:actor  rdf:type         owl:ObjectProperty;
        rdfs:label           "Actor";
        rdfs:range           ocsf:Actor;
        dcterms:description  "The actor object describes details about the user/role/process that was the source of the activity." .

ocsf:classifications  rdf:type  owl:DatatypeProperty;
        rdfs:label           "Classifications";
        rdfs:range           ocsf:string_t;
        dcterms:description  "The list of malware classifications, normalized to the captions of the classification_id values. In the case of 'Other', they are defined by the event source." .

ocsf:KernelResource  rdf:type  owl:Class;
        rdfs:label           "Kernel Resource";
        rdfs:subClassOf      ocsf:Object;
        dcterms:description  "The Kernel Resource object provides information about a specific kernel resource, including its name and type. It describes essential attributes associated with a resource managed by the kernel of an operating system. Defined by D3FEND <a target='_blank' href='https://d3fend.mitre.org/dao/artifact/d3f:Kernel/'>d3f:Kernel</a>.";
        ocsf:name            "kernel" .

ocsf:title  rdf:type         owl:DatatypeProperty;
        rdfs:label           "Title";
        rdfs:range           ocsf:string_t;
        dcterms:description  "The title of an entity. See specific usage." .

ocsf:access_list  rdf:type   owl:DatatypeProperty;
        rdfs:label           "Access List";
        rdfs:range           ocsf:string_t;
        dcterms:description  "The list of requested access rights." .

ocsf:log_name  rdf:type      owl:DatatypeProperty;
        rdfs:label           "Log Name";
        rdfs:range           ocsf:string_t;
        dcterms:description  "The event log name. For example, syslog file name or Windows logging subsystem: Security." .

ocsf:impact_id  rdf:type     owl:DatatypeProperty;
        rdfs:label           "Impact ID";
        rdfs:range           ocsf:integer_t;
        dcterms:description  "The normalized impact of the finding.";
        jsonschema:enum      "Critical" , "Low" , "Unknown" , "High" , "Medium" , "Other" .

ocsf:Tactic  rdf:type        owl:Class;
        rdfs:label           "Tactic";
        rdfs:subClassOf      ocsf:Entity;
        dcterms:description  "The Tactic object describes the tactic ID and/or name that is associated to an attack, as defined by <a target='_blank' href='https://attack.mitre.org/wiki/ATT&CK_Matrix'>ATT&CK Matrix<sup>TM</sup></a>.";
        ocsf:name            "tactic" .

ocsf:cc  rdf:type            owl:DatatypeProperty;
        rdfs:label           "Cc";
        rdfs:range           ocsf:email_t;
        dcterms:description  "The email header Cc values, as defined by RFC 5322." .

ocsf:subject  rdf:type       owl:DatatypeProperty;
        rdfs:label           "Subject Details";
        rdfs:range           ocsf:string_t;
        dcterms:description  "The identifier of the subject. See specific usage." .

ocsf:json_t  rdf:type        rdfs:Datatype;
        rdfs:label           "JSON";
        rdfs:subClassOf      rdf:JSON;
        dcterms:description  "Embedded JSON value. A value can be a string, or a number, or true or false or null, or an object or an array. These structures can be nested. See <a target='_blank' href='https://www.json.org'>www.json.org</a>." .

ocsf:Process  rdf:type       owl:Class;
        rdfs:label           "Process";
        rdfs:subClassOf      ocsf:Entity;
        rdfs:subClassOf      [ rdf:type            owl:Restriction;
                               owl:onProperty      ocsf:session;
                               owl:someValuesFrom  ocsf:Session
                             ];
        rdfs:subClassOf      [ rdf:type            owl:Restriction;
                               owl:onProperty      ocsf:xattributes;
                               owl:someValuesFrom  ocsf:Object
                             ];
        rdfs:subClassOf      [ rdf:type            owl:Restriction;
                               owl:onProperty      ocsf:user;
                               owl:someValuesFrom  ocsf:User
                             ];
        rdfs:subClassOf      [ rdf:type            owl:Restriction;
                               owl:onProperty      ocsf:parent_process;
                               owl:someValuesFrom  ocsf:Process
                             ];
        rdfs:subClassOf      [ rdf:type            owl:Restriction;
                               owl:onProperty      ocsf:file;
                               owl:someValuesFrom  ocsf:File
                             ];
        dcterms:description  "The Process object describes a running instance of a launched program. Defined by D3FEND <a target='_blank' href='https://d3fend.mitre.org/dao/artifact/d3f:Process/'>d3f:Process</a>.";
        ocsf:constraints     "{\"at_least_one\":[\"pid\",\"uid\"]}";
        ocsf:name            "process";
        ocsf:observable      25;
        ocsf:profiles        "[\"container\"]" .

ocsf:dialect  rdf:type       owl:DatatypeProperty;
        rdfs:label           "Dialect";
        rdfs:range           ocsf:string_t;
        dcterms:description  "The negotiated protocol dialect." .

ocsf:Remediation  rdf:type   owl:Class;
        rdfs:label           "Remediation";
        rdfs:subClassOf      ocsf:Object;
        rdfs:subClassOf      [ rdf:type            owl:Restriction;
                               owl:onProperty      ocsf:kb_articles;
                               owl:someValuesFrom  ocsf:KBArticle
                             ];
        dcterms:description  "The Remediation object describes the recommended remediation steps to address identified issue(s).";
        ocsf:name            "remediation" .

ocsf:server_ciphers  rdf:type  owl:DatatypeProperty;
        rdfs:label           "Server Cipher Suites";
        rdfs:range           ocsf:string_t;
        dcterms:description  "The server cipher suites that were exchanged during the TLS handshake negotiation." .

ocsf:EmailActivityEvent
        rdf:type             owl:Class;
        rdfs:label           "Email Activity";
        rdfs:subClassOf      d3f:DigitalEvent;
        rdfs:subClassOf      [ rdf:type         owl:Restriction;
                               owl:cardinality  1;
                               owl:onProperty   ocsf:email
                             ];
        rdfs:subClassOf      [ rdf:type            owl:Restriction;
                               owl:onProperty      ocsf:email_auth;
                               owl:someValuesFrom  ocsf:EmailAuthentication
                             ];
        rdfs:subClassOf      [ rdf:type            owl:Restriction;
                               owl:onProperty      ocsf:dst_endpoint;
                               owl:someValuesFrom  ocsf:NetworkEndpoint
                             ];
        rdfs:subClassOf      [ rdf:type            owl:Restriction;
                               owl:onProperty      ocsf:src_endpoint;
                               owl:someValuesFrom  ocsf:NetworkEndpoint
                             ];
        dcterms:description  "Email events report activities of emails.";
        ocsf:category        "network";
        ocsf:name            "email_activity";
        ocsf:profiles        "[\"host\",\"security_control\"]";
        ocsf:uid             9 .

ocsf:ResourceDetails  rdf:type  owl:Class;
        rdfs:label           "Resource Details";
        rdfs:subClassOf      ocsf:Resource;
        rdfs:subClassOf      [ rdf:type            owl:Restriction;
                               owl:onProperty      ocsf:owner;
                               owl:someValuesFrom  ocsf:User
                             ];
        rdfs:subClassOf      [ rdf:type            owl:Restriction;
                               owl:onProperty      ocsf:group;
                               owl:someValuesFrom  ocsf:Group
                             ];
        dcterms:description  "The Resource Details object describes details about resources that were affected by the activity/event.";
        ocsf:name            "resource_details" .

ocsf:full_name  rdf:type     owl:DatatypeProperty;
        rdfs:label           "Full Name";
        rdfs:range           ocsf:string_t;
        dcterms:description  "The full name of the person, as per the LDAP Common Name attribute (cn)." .

ocsf:security_descriptor
        rdf:type             owl:DatatypeProperty;
        rdfs:label           "Security Descriptor";
        rdfs:range           ocsf:string_t;
        dcterms:description  "The object security descriptor." .

ocsf:injection_type_id
        rdf:type             owl:DatatypeProperty;
        rdfs:label           "Injection Type ID";
        rdfs:range           ocsf:integer_t;
        dcterms:description  "The normalized identifier of the process injection method.";
        jsonschema:enum      "Load Library" , "Remote Thread" , "Unknown" , "Other" .

ocsf:AffectedCode  rdf:type  owl:Class;
        rdfs:label           "Affected Code";
        rdfs:subClassOf      ocsf:Object;
        rdfs:subClassOf      [ rdf:type            owl:Restriction;
                               owl:onProperty      ocsf:remediation;
                               owl:someValuesFrom  ocsf:Remediation
                             ];
        rdfs:subClassOf      [ rdf:type            owl:Restriction;
                               owl:onProperty      ocsf:owner;
                               owl:someValuesFrom  ocsf:User
                             ];
        rdfs:subClassOf      [ rdf:type         owl:Restriction;
                               owl:cardinality  1;
                               owl:onProperty   ocsf:file
                             ];
        dcterms:description  "The Affected Code object describes details about a code block identified as vulnerable.";
        ocsf:name            "affected_code" .

ocsf:TLSExtension  rdf:type  owl:Class;
        rdfs:label           "TLS Extension";
        rdfs:subClassOf      ocsf:Object;
        dcterms:description  "The TLS Extension object describes additional attributes that extend the base Transport Layer Security (TLS) object.";
        ocsf:name            "tls_extension" .

ocsf:dmarc_override  rdf:type  owl:DatatypeProperty;
        rdfs:label           "DMARC Override";
        rdfs:range           ocsf:string_t;
        dcterms:description  "The Domain-based Message Authentication, Reporting and Conformance (DMARC) override action." .

ocsf:package  rdf:type       owl:ObjectProperty;
        rdfs:label           "Software Package";
        rdfs:range           ocsf:SoftwarePackage;
        dcterms:description  "The Software Package object describes details about a software package. Defined by D3FEND <a target='_blank' href='https://d3fend.mitre.org/dao/artifact/d3f:SoftwarePackage/'>d3f:SoftwarePackage</a>." .

ocsf:PeripheralDevice
        rdf:type             owl:Class;
        rdfs:label           "Peripheral Device";
        rdfs:subClassOf      ocsf:Entity;
        dcterms:description  "The peripheral device object describes the identity, vendor and model of a peripheral device.";
        ocsf:name            "peripheral_device" .

ocsf:system_call  rdf:type   owl:DatatypeProperty;
        rdfs:label           "System Call";
        rdfs:range           ocsf:string_t;
        dcterms:description  "The system call that was invoked." .

ocsf:query_info  rdf:type    owl:ObjectProperty;
        rdfs:label           "Query Info";
        dcterms:description  "The query info object holds information related to data access within a datastore. To access, manipulate, delete, or retrieve data from a datastore, a database query must be written using a specific syntax." .

ocsf:release  rdf:type       owl:DatatypeProperty;
        rdfs:label           "Software Release Details";
        rdfs:range           ocsf:string_t;
        dcterms:description  "Release is the number of times a version of the software has been packaged." .

ocsf:ProcessActivityEvent
        rdf:type             owl:Class;
        rdfs:label           "Process Activity";
        rdfs:subClassOf      d3f:DigitalEvent;
        rdfs:subClassOf      [ rdf:type         owl:Restriction;
                               owl:cardinality  1;
                               owl:onProperty   ocsf:process
                             ];
        rdfs:subClassOf      [ rdf:type            owl:Restriction;
                               owl:onProperty      ocsf:module;
                               owl:someValuesFrom  ocsf:Module
                             ];
        rdfs:subClassOf      [ rdf:type            owl:Restriction;
                               owl:onProperty      ocsf:actor;
                               owl:someValuesFrom  ocsf:Actor
                             ];
        dcterms:description  "Process Activity events report when a process launches, injects, opens or terminates another process, successful or otherwise.";
        ocsf:name            "process_activity";
        ocsf:uid             7 .

ocsf:score_id  rdf:type      owl:DatatypeProperty;
        rdfs:label           "Reputation Score ID";
        rdfs:range           ocsf:integer_t;
        dcterms:description  "The normalized reputation score identifier.";
        jsonschema:enum      "Possibly Malicious" , "Probably Safe" , "Suspicious/Risky" , "Leans Safe" , "Probably Malicious" , "Malicious" , "Exercise Caution" , "Safe" , "Unknown" , "Very Safe" , "May not be Safe" , "Other" .

ocsf:start_line  rdf:type    owl:DatatypeProperty;
        rdfs:label           "Start Line";
        rdfs:range           ocsf:integer_t;
        dcterms:description  "The line number of the first line of code block identified as vulnerable." .

ocsf:databucket  rdf:type    owl:ObjectProperty;
        rdfs:label           "Databucket";
        dcterms:description  "The data bucket object is a basic container that holds data, typically organized through the use of data partitions." .

ocsf:UserInventoryInfoEvent
        rdf:type             owl:Class;
        rdfs:label           "User Inventory Info";
        rdfs:subClassOf      d3f:DigitalEvent;
        rdfs:subClassOf      [ rdf:type         owl:Restriction;
                               owl:cardinality  1;
                               owl:onProperty   ocsf:user
                             ];
        rdfs:subClassOf      [ rdf:type            owl:Restriction;
                               owl:onProperty      ocsf:actor;
                               owl:someValuesFrom  ocsf:Actor
                             ];
        dcterms:description  "For example, this can be utilized to collect user information by gathering Active Directory data.";
        ocsf:name            "user_inventory";
        ocsf:uid             3 .

ocsf:message  rdf:type       owl:DatatypeProperty;
        rdfs:label           "Message";
        rdfs:range           ocsf:string_t;
        dcterms:description  "The description of the event/finding, as defined by the source." .

ocsf:domain  rdf:type        owl:DatatypeProperty;
        rdfs:label           "Domain";
        rdfs:range           ocsf:string_t;
        dcterms:description  "The name of the domain." .

ocsf:share_type  rdf:type    owl:DatatypeProperty;
        rdfs:label           "Share Type";
        rdfs:range           ocsf:string_t;
        dcterms:description  "The SMB share type, normalized to the caption of the share_type_id value. In the case of 'Other', it is defined by the event source." .

ocsf:severity  rdf:type      owl:DatatypeProperty;
        rdfs:label           "Severity";
        rdfs:range           ocsf:string_t;
        dcterms:description  "The event/finding severity, normalized to the caption of the severity_id value. In the case of 'Other', it is defined by the source." .

ocsf:privileges  rdf:type    owl:DatatypeProperty;
        rdfs:label           "Privileges";
        rdfs:range           ocsf:string_t;
        dcterms:description  "The user or group privileges." .

ocsf:deleted_time  rdf:type  owl:DatatypeProperty;
        rdfs:label           "Deleted Time";
        rdfs:range           ocsf:timestamp_t;
        dcterms:description  "The timestamp when the user was deleted. In Active Directory (AD), when a user is deleted they are moved to a temporary container and then removed after 30 days. So, this field can be populated even after a user is deleted for the next 30 days." .

ocsf:surname  rdf:type       owl:DatatypeProperty;
        rdfs:label           "Surname";
        rdfs:range           ocsf:string_t;
        dcterms:description  "The last or family name for the user." .

ocsf:Actor  rdf:type         owl:Class;
        rdfs:label           "Actor";
        rdfs:subClassOf      ocsf:Object;
        rdfs:subClassOf      [ rdf:type            owl:Restriction;
                               owl:onProperty      ocsf:idp;
                               owl:someValuesFrom  ocsf:IdentityProvider
                             ];
        rdfs:subClassOf      [ rdf:type            owl:Restriction;
                               owl:onProperty      ocsf:process;
                               owl:someValuesFrom  ocsf:Process
                             ];
        rdfs:subClassOf      [ rdf:type            owl:Restriction;
                               owl:onProperty      ocsf:user;
                               owl:someValuesFrom  ocsf:User
                             ];
        rdfs:subClassOf      [ rdf:type            owl:Restriction;
                               owl:onProperty      ocsf:authorizations;
                               owl:someValuesFrom  ocsf:AuthorizationResult
                             ];
        rdfs:subClassOf      [ rdf:type            owl:Restriction;
                               owl:onProperty      ocsf:session;
                               owl:someValuesFrom  ocsf:Session
                             ];
        dcterms:description  "The Actor object contains details about the user, role, or process that initiated or performed a specific activity.";
        ocsf:constraints     "{\"at_least_one\":[\"process\",\"user\",\"invoked_by\",\"session\"]}";
        ocsf:name            "actor" .

ocsf:FirewallRule  rdf:type  owl:Class;
        rdfs:label           "Firewall Rule";
        rdfs:subClassOf      ocsf:Rule;
        dcterms:description  "The Firewall Rule object represents a specific rule within a firewall policy or event. It contains information about a rule's configuration, properties, and associated actions that define how network traffic is handled by the firewall.";
        ocsf:name            "firewall_rule" .

ocsf:DHCPActivityEvent
        rdf:type             owl:Class;
        rdfs:label           "DHCP Activity";
        rdfs:subClassOf      d3f:DigitalEvent;
        rdfs:subClassOf      [ rdf:type            owl:Restriction;
                               owl:onProperty      ocsf:src_endpoint;
                               owl:someValuesFrom  ocsf:NetworkEndpoint
                             ];
        rdfs:subClassOf      [ rdf:type            owl:Restriction;
                               owl:onProperty      ocsf:dst_endpoint;
                               owl:someValuesFrom  ocsf:NetworkEndpoint
                             ];
        rdfs:subClassOf      [ rdf:type            owl:Restriction;
                               owl:onProperty      ocsf:relay;
                               owl:someValuesFrom  ocsf:NetworkInterface
                             ];
        dcterms:description  "DHCP Activity events report MAC to IP assignment via DHCP from a client or server.";
        ocsf:category        "network";
        ocsf:name            "dhcp_activity";
        ocsf:profiles        "[\"host\"]";
        ocsf:uid             4 .

ocsf:peripheral_device
        rdf:type             owl:ObjectProperty;
        rdfs:label           "Peripheral Device";
        rdfs:range           ocsf:PeripheralDevice;
        dcterms:description  "The peripheral device that triggered the event." .

ocsf:NetworkEndpoint  rdf:type  owl:Class;
        rdfs:label           "Network Endpoint";
        rdfs:subClassOf      ocsf:Endpoint;
        dcterms:description  "The Network Endpoint object describes characteristics of a network endpoint. These can be a source or destination of a network connection.";
        ocsf:constraints     "{\"at_least_one\":[\"ip\",\"uid\",\"name\",\"hostname\",\"svc_name\",\"instance_uid\",\"interface_uid\",\"interface_name\"]}";
        ocsf:name            "network_endpoint" .

ocsf:end_time  rdf:type      owl:DatatypeProperty;
        rdfs:label           "End Time";
        rdfs:range           ocsf:timestamp_t;
        dcterms:description  "The end time of a time period. See specific usage." .

ocsf:loggers  rdf:type       owl:ObjectProperty;
        rdfs:label           "Loggers";
        rdfs:range           ocsf:Logger;
        dcterms:description  "An array of Logger objects that describe the devices and logging products between the event source and its eventual destination. Note, this attribute can be used when there is a complex end-to-end path of event flow." .

ocsf:server_hassh  rdf:type  owl:ObjectProperty;
        rdfs:label           "Server HASSH";
        rdfs:range           ocsf:HASSH;
        dcterms:description  "The Server HASSH fingerprinting object." .

ocsf:provider  rdf:type      owl:DatatypeProperty;
        rdfs:label           "Provider";
        rdfs:range           ocsf:string_t;
        dcterms:description  "The origin of information associated with the event. See specific usage." .

ocsf:opcode  rdf:type        owl:DatatypeProperty;
        rdfs:label           "DNS Opcode";
        rdfs:range           ocsf:string_t;
        dcterms:description  "The DNS opcode specifies the type of the query message." .

ocsf:http_cookies  rdf:type  owl:ObjectProperty;
        rdfs:label           "HTTP Cookies";
        rdfs:range           ocsf:HTTPCookie;
        dcterms:description  "The cookies object describes details about HTTP cookies" .

ocsf:APIActivityEvent
        rdf:type             owl:Class;
        rdfs:label           "API Activity";
        rdfs:subClassOf      d3f:DigitalEvent;
        rdfs:subClassOf      [ rdf:type            owl:Restriction;
                               owl:onProperty      ocsf:resources;
                               owl:someValuesFrom  ocsf:ResourceDetails
                             ];
        rdfs:subClassOf      [ rdf:type         owl:Restriction;
                               owl:cardinality  1;
                               owl:onProperty   ocsf:api
                             ];
        rdfs:subClassOf      [ rdf:type         owl:Restriction;
                               owl:cardinality  1;
                               owl:onProperty   ocsf:actor
                             ];
        rdfs:subClassOf      [ rdf:type         owl:Restriction;
                               owl:cardinality  1;
                               owl:onProperty   ocsf:src_endpoint
                             ];
        rdfs:subClassOf      [ rdf:type            owl:Restriction;
                               owl:onProperty      ocsf:http_request;
                               owl:someValuesFrom  ocsf:HTTPRequest
                             ];
        rdfs:subClassOf      [ rdf:type            owl:Restriction;
                               owl:onProperty      ocsf:dst_endpoint;
                               owl:someValuesFrom  ocsf:NetworkEndpoint
                             ];
        dcterms:description  "API events describe general CRUD (Create, Read, Update, Delete) API activities, e.g. (AWS Cloudtrail)";
        ocsf:name            "api_activity";
        ocsf:uid             3 .

ocsf:hire_time  rdf:type     owl:DatatypeProperty;
        rdfs:label           "Hire Time";
        rdfs:range           ocsf:timestamp_t;
        dcterms:description  "The timestamp when the user was or will be hired by the organization." .

ocsf:groups  rdf:type        owl:ObjectProperty;
        rdfs:label           "Groups";
        rdfs:range           ocsf:Group;
        dcterms:description  "The groups to which an entity belongs. See specific usage." .

ocsf:PeripheralDeviceInfoEvent
        rdf:type             owl:Class;
        rdfs:label           "Peripheral Device Info";
        rdfs:subClassOf      d3f:DigitalEvent;
        rdfs:subClassOf      [ rdf:type         owl:Restriction;
                               owl:cardinality  1;
                               owl:onProperty   ocsf:peripheral_device
                             ];
        dcterms:description  "Peripheral Device Info events report information about peripheral devices.";
        ocsf:name            "peripheral_device_info";
        ocsf:uid             14 .

ocsf:log_provider  rdf:type  owl:DatatypeProperty;
        rdfs:label           "Log Provider";
        rdfs:range           ocsf:string_t;
        dcterms:description  "The logging provider or logging service that logged the event. For example, Microsoft-Windows-Security-Auditing." .

ocsf:dce_rpc  rdf:type       owl:ObjectProperty;
        rdfs:label           "Distributed Computing Environment/Remote Procedure Call (DCE/RPC)";
        rdfs:range           ocsf:DCERPC;
        dcterms:description  "The DCE/RPC object describes the remote procedure call system for distributed computing environments." .

ocsf:vendor_name  rdf:type   owl:DatatypeProperty;
        rdfs:label           "Vendor Name";
        rdfs:range           ocsf:string_t;
        dcterms:description  "The name of the vendor. See specific usage." .

ocsf:hashes  rdf:type        owl:ObjectProperty;
        rdfs:label           "Hashes";
        rdfs:range           ocsf:Fingerprint;
        dcterms:description  "An array of hash attributes." .

ocsf:HTTPActivityEvent
        rdf:type             owl:Class;
        rdfs:label           "HTTP Activity";
        rdfs:subClassOf      d3f:DigitalEvent;
        rdfs:subClassOf      [ rdf:type         owl:Restriction;
                               owl:cardinality  1;
                               owl:onProperty   ocsf:http_request
                             ];
        rdfs:subClassOf      [ rdf:type            owl:Restriction;
                               owl:onProperty      ocsf:http_cookies;
                               owl:someValuesFrom  ocsf:HTTPCookie
                             ];
        rdfs:subClassOf      [ rdf:type         owl:Restriction;
                               owl:cardinality  1;
                               owl:onProperty   ocsf:http_response
                             ];
        dcterms:description  "HTTP Activity events report HTTP connection and traffic information.";
        ocsf:category        "network";
        ocsf:name            "http_activity";
        ocsf:uid             2 .

ocsf:phase  rdf:type         owl:DatatypeProperty;
        rdfs:label           "Kill Chain Phase";
        rdfs:range           ocsf:string_t;
        dcterms:description  "The cyber kill chain phase." .

ocsf:proxy_http_response
        rdf:type             owl:ObjectProperty;
        rdfs:label           "Proxy HTTP Response";
        rdfs:range           ocsf:HTTPResponse;
        dcterms:description  "The HTTP Response from the remote server to the proxy server." .

ocsf:EmailAuthentication
        rdf:type             owl:Class;
        rdfs:label           "Email Authentication";
        rdfs:subClassOf      ocsf:Object;
        dcterms:description  "The Email Authentication object describes the Sender Policy Framework (SPF), DomainKeys Identified Mail (DKIM) and Domain-based Message Authentication, Reporting and Conformance (DMARC) attributes of an email.";
        ocsf:name            "email_auth" .

ocsf:Module  rdf:type        owl:Class;
        rdfs:label           "Module";
        rdfs:subClassOf      ocsf:Object;
        rdfs:subClassOf      [ rdf:type            owl:Restriction;
                               owl:onProperty      ocsf:file;
                               owl:someValuesFrom  ocsf:File
                             ];
        dcterms:description  "The Module object describes the load attributes of a module.";
        ocsf:name            "module" .

ocsf:categories  rdf:type    owl:DatatypeProperty;
        rdfs:label           "Website Categorization";
        rdfs:range           ocsf:string_t;
        dcterms:description  "The Website categorization names, as defined by <code>category_ids</code> enum values." .

ocsf:dmarc  rdf:type         owl:DatatypeProperty;
        rdfs:label           "DMARC Status";
        rdfs:range           ocsf:string_t;
        dcterms:description  "The Domain-based Message Authentication, Reporting and Conformance (DMARC) status of the email." .

ocsf:location  rdf:type      owl:ObjectProperty;
        rdfs:label           "Geo Location";
        rdfs:range           ocsf:GeoLocation;
        dcterms:description  "The detailed geographical location usually associated with an IP address." .

ocsf:correlation_uid  rdf:type  owl:DatatypeProperty;
        rdfs:label           "Correlation UID";
        rdfs:range           ocsf:string_t;
        dcterms:description  "The unique identifier used to correlate events." .

ocsf:vulnerabilities  rdf:type  owl:ObjectProperty;
        rdfs:label           "Vulnerabilities";
        rdfs:range           ocsf:VulnerabilityDetails;
        dcterms:description  "This object describes vulnerabilities reported in a security finding." .

ocsf:type_name  rdf:type     owl:DatatypeProperty;
        rdfs:label           "Type Name";
        rdfs:range           ocsf:string_t;
        dcterms:description  "The event/finding type name, as defined by the type_uid." .

ocsf:KernelExtensionActivityEvent
        rdf:type             owl:Class;
        rdfs:label           "Kernel Extension Activity";
        rdfs:subClassOf      d3f:DigitalEvent;
        rdfs:subClassOf      [ rdf:type         owl:Restriction;
                               owl:cardinality  1;
                               owl:onProperty   ocsf:driver
                             ];
        rdfs:subClassOf      [ rdf:type         owl:Restriction;
                               owl:cardinality  1;
                               owl:onProperty   ocsf:actor
                             ];
        dcterms:description  "Kernel Extension events report when a driver/extension is loaded or unloaded into the kernel";
        ocsf:name            "kernel_extension";
        ocsf:uid             2 .

ocsf:AuthorizationResult
        rdf:type             owl:Class;
        rdfs:label           "Authorization Result";
        rdfs:subClassOf      ocsf:Object;
        rdfs:subClassOf      [ rdf:type            owl:Restriction;
                               owl:onProperty      ocsf:policy;
                               owl:someValuesFrom  ocsf:Policy
                             ];
        dcterms:description  "The Authorization Result object provides details about the authorization outcome and associated policies related to activity.";
        ocsf:name            "authorization" .

ocsf:overall_score  rdf:type  owl:DatatypeProperty;
        rdfs:label           "Overall Score";
        rdfs:range           ocsf:float_t;
        dcterms:description  "The overall score as reported by the event source. See specific usage." .

ocsf:ldap_cn  rdf:type       owl:DatatypeProperty;
        rdfs:label           "LDAP Common Name";
        rdfs:range           ocsf:string_t;
        dcterms:description  "The LDAP and X.500 <code>commonName</code> attribute, typically the full name of the person. For example, <code>John Doe</code>." .

ocsf:sni  rdf:type           owl:DatatypeProperty;
        rdfs:label           "Server Name Indication";
        rdfs:range           ocsf:string_t;
        dcterms:description  " The Server Name Indication (SNI) extension sent by the client." .

ocsf:category_uid  rdf:type  owl:DatatypeProperty;
        rdfs:label           "Category ID";
        rdfs:range           ocsf:integer_t;
        dcterms:description  "The category unique identifier of the event." .

ocsf:feature  rdf:type       owl:ObjectProperty;
        rdfs:label           "Feature";
        rdfs:range           ocsf:Feature;
        dcterms:description  "The feature that reported the event." .

ocsf:TransportLayerSecurityTLS
        rdf:type             owl:Class;
        rdfs:label           "Transport Layer Security (TLS)";
        rdfs:subClassOf      ocsf:Object;
        rdfs:subClassOf      [ rdf:type            owl:Restriction;
                               owl:onProperty      ocsf:extension_list;
                               owl:someValuesFrom  ocsf:TLSExtension
                             ];
        rdfs:subClassOf      [ rdf:type            owl:Restriction;
                               owl:onProperty      ocsf:ja3_hash;
                               owl:someValuesFrom  ocsf:Fingerprint
                             ];
        rdfs:subClassOf      [ rdf:type            owl:Restriction;
                               owl:onProperty      ocsf:certificate;
                               owl:someValuesFrom  ocsf:DigitalCertificate
                             ];
        rdfs:subClassOf      [ rdf:type            owl:Restriction;
                               owl:onProperty      ocsf:ja3s_hash;
                               owl:someValuesFrom  ocsf:Fingerprint
                             ];
        rdfs:subClassOf      [ rdf:type            owl:Restriction;
                               owl:onProperty      ocsf:sans;
                               owl:someValuesFrom  ocsf:SubjectAlternativeName
                             ];
        dcterms:description  "The Transport Layer Security (TLS) object describes the negotiated TLS protocol used for secure communications over an establish network connection.";
        ocsf:name            "tls" .

ocsf:confidentiality_id
        rdf:type             owl:DatatypeProperty;
        rdfs:label           "Confidentiality ID";
        rdfs:range           ocsf:integer_t;
        dcterms:description  "The normalized identifier of the file content confidentiality indicator.";
        jsonschema:enum      "Unknown" , "Other" , "Not Confidential" , "Confidential" , "Top Secret" , "Secret" .

ocsf:is_fix_available
        rdf:type             owl:DatatypeProperty;
        rdfs:label           "Fix Availability";
        rdfs:range           ocsf:boolean_t;
        dcterms:description  "Indicates if a fix is available for the reported vulnerability." .

ocsf:kb_articles  rdf:type   owl:DatatypeProperty;
        rdfs:label           "Knowledgebase Articles";
        rdfs:range           ocsf:string_t;
        dcterms:description  "The KB article/s related to the entity. A KB Article contains metadata that describes the patch or an update." .

ocsf:rate_limit  rdf:type    owl:DatatypeProperty;
        rdfs:label           "Rate Limit";
        rdfs:range           ocsf:integer_t;
        dcterms:description  "The rate limit for a rate-based rule." .

ocsf:AuthenticationEvent
        rdf:type             owl:Class;
        rdfs:label           "Authentication";
        rdfs:subClassOf      d3f:DigitalEvent;
        rdfs:subClassOf      [ rdf:type            owl:Restriction;
                               owl:onProperty      ocsf:certificate;
                               owl:someValuesFrom  ocsf:DigitalCertificate
                             ];
        rdfs:subClassOf      [ rdf:type            owl:Restriction;
                               owl:onProperty      ocsf:http_request;
                               owl:someValuesFrom  ocsf:HTTPRequest
                             ];
        rdfs:subClassOf      [ rdf:type            owl:Restriction;
                               owl:onProperty      ocsf:session;
                               owl:someValuesFrom  ocsf:Session
                             ];
        rdfs:subClassOf      [ rdf:type            owl:Restriction;
                               owl:onProperty      ocsf:src_endpoint;
                               owl:someValuesFrom  ocsf:NetworkEndpoint
                             ];
        rdfs:subClassOf      [ rdf:type            owl:Restriction;
                               owl:onProperty      ocsf:dst_endpoint;
                               owl:someValuesFrom  ocsf:NetworkEndpoint
                             ];
        rdfs:subClassOf      [ rdf:type            owl:Restriction;
                               owl:onProperty      ocsf:logon_process;
                               owl:someValuesFrom  ocsf:Process
                             ];
        rdfs:subClassOf      [ rdf:type            owl:Restriction;
                               owl:onProperty      ocsf:actor;
                               owl:someValuesFrom  ocsf:Actor
                             ];
        rdfs:subClassOf      [ rdf:type            owl:Restriction;
                               owl:onProperty      ocsf:service;
                               owl:someValuesFrom  ocsf:Service
                             ];
        rdfs:subClassOf      [ rdf:type         owl:Restriction;
                               owl:cardinality  1;
                               owl:onProperty   ocsf:user
                             ];
        dcterms:description  "Authentication events report authentication session activities such as user attempts a logon or logoff, successfully or otherwise.";
        ocsf:associations    "{\"actor.user\":[\"src_endpoint\"],\"dst_endpoint\":[\"user\"],\"src_endpoint\":[\"actor.user\"],\"user\":[\"dst_endpoint\"]}";
        ocsf:constraints     "{\"at_least_one\":[\"service\",\"dst_endpoint\"]}";
        ocsf:name            "authentication";
        ocsf:uid             2 .

ocsf:command_response
        rdf:type             owl:DatatypeProperty;
        rdfs:label           "Command Response";
        rdfs:range           ocsf:string_t;
        dcterms:description  "The response to the command." .

ocsf:SystemActivityEvent
        rdf:type             owl:Class;
        rdfs:label           "System Activity";
        rdfs:subClassOf      d3f:DigitalEvent;
        rdfs:subClassOf      [ rdf:type         owl:Restriction;
                               owl:cardinality  1;
                               owl:onProperty   ocsf:actor
                             ];
        rdfs:subClassOf      [ rdf:type         owl:Restriction;
                               owl:cardinality  1;
                               owl:onProperty   ocsf:device
                             ];
        dcterms:description  "The System Activity event is a generic event that defines a set of attributes available in the system activity events. As a generic event, it could be used to log events that are not otherwise defined by the System Activity category.";
        ocsf:associations    "{\"device\":[\"actor.user\"],\"actor.user\":[\"device\"]}";
        ocsf:category        "system";
        ocsf:name            "system";
        ocsf:profiles        "[\"host\",\"security_control\"]" .

ocsf:packets_in  rdf:type    owl:DatatypeProperty;
        rdfs:label           "Packets In";
        rdfs:range           ocsf:long_t;
        dcterms:description  "The number of packets sent from the destination to the source." .

ocsf:CISCSC  rdf:type        owl:Class;
        rdfs:label           "CIS CSC";
        rdfs:subClassOf      ocsf:Object;
        dcterms:description  "The CIS Critical Security Control (CSC) contains information as defined by the Center for Internet Security Critical Security Control <a target='_blank' href='https://www.cisecurity.org/controls'>(CIS CSC)</a>. Prioritized set of actions to protect your organization and data from cyber-attack vectors.";
        ocsf:name            "cis_csc" .

ocsf:web_resources  rdf:type  owl:ObjectProperty;
        rdfs:label           "Web Resources";
        rdfs:range           ocsf:WebResource;
        dcterms:description  "Describes details about web resources that were affected by an activity/event." .

ocsf:latency  rdf:type       owl:DatatypeProperty;
        rdfs:label           "Latency";
        rdfs:range           ocsf:integer_t;
        dcterms:description  "The HTTP response latency measured in milliseconds." .

ocsf:src_endpoint  rdf:type  owl:ObjectProperty;
        rdfs:label           "Source Endpoint";
        rdfs:range           ocsf:NetworkEndpoint;
        dcterms:description  "The network source endpoint." .

ocsf:compliance  rdf:type    owl:ObjectProperty;
        rdfs:label           "Compliance";
        rdfs:range           ocsf:Compliance;
        dcterms:description  "The compliance object provides context to compliance findings (e.g., a check against a specific regulatory or best practice framework such as CIS, NIST etc.) and contains compliance related details." .

ocsf:subnet_prefix  rdf:type  owl:DatatypeProperty;
        rdfs:label           "Subnet Prefix Length";
        rdfs:range           ocsf:integer_t;
        dcterms:description  "The subnet prefix length determines the number of bits used to represent the network part of the IP address. The remaining bits are reserved for identifying individual hosts within that subnet." .

ocsf:http_method  rdf:type   owl:DatatypeProperty;
        rdfs:label           "HTTP Method";
        rdfs:range           ocsf:string_t;
        dcterms:description  "The HTTP request method indicates the desired action to be performed for a given resource. Expected values: <ul> <li>TRACE</li> <li>CONNECT</li> <li>OPTIONS</li> <li>HEAD</li> <li>DELETE</li> <li>POST</li> <li>PUT</li> <li>GET</li></ul>" .

ocsf:response_time  rdf:type  owl:DatatypeProperty;
        rdfs:label           "Response Time";
        rdfs:range           ocsf:timestamp_t;
        dcterms:description  "The Domain Name System (DNS) response time." .

ocsf:auth_type  rdf:type     owl:DatatypeProperty;
        rdfs:label           "Authentication Type";
        rdfs:range           ocsf:string_t;
        dcterms:description  "The agreed upon authentication type, normalized to the caption of 'auth_type_id'. In the case of 'Other', it is defined by the event source." .

ocsf:remote_display  rdf:type  owl:ObjectProperty;
        rdfs:label           "Remote Display";
        rdfs:range           ocsf:Display;
        dcterms:description  "The remote display affiliated with the event" .

ocsf:office_location  rdf:type  owl:DatatypeProperty;
        rdfs:label           "Office Location";
        rdfs:range           ocsf:string_t;
        dcterms:description  "The primary office location associated with the user. This could be any string and isn't a specific address. For example, <code>South East Virtual</code>." .

ocsf:secure  rdf:type        owl:DatatypeProperty;
        rdfs:label           "Secure";
        rdfs:range           ocsf:boolean_t;
        dcterms:description  "The cookie attribute to only send cookies to the server with an encrypted request over the HTTPS protocol." .

ocsf:client_dialects  rdf:type  owl:DatatypeProperty;
        rdfs:label           "Client Dialects";
        rdfs:range           ocsf:string_t;
        dcterms:description  "The list of SMB dialects that the client speaks." .

ocsf:model  rdf:type         owl:DatatypeProperty;
        rdfs:label           "Model";
        rdfs:range           ocsf:string_t;
        dcterms:description  "The peripheral device model." .

ocsf:src_url  rdf:type       owl:DatatypeProperty;
        rdfs:label           "Source URL";
        rdfs:range           ocsf:url_t;
        dcterms:description  "The URL pointing towards the source of an entity. See specific usage." .

ocsf:package_manager  rdf:type  owl:DatatypeProperty;
        rdfs:label           "Package Manager";
        rdfs:range           ocsf:string_t;
        dcterms:description  "The software packager manager utilized to manage a package on a system, e.g. npm, yum, dpkg etc." .

ocsf:app_name  rdf:type      owl:DatatypeProperty;
        rdfs:label           "Application Name";
        rdfs:range           ocsf:string_t;
        dcterms:description  "The name of the application that is associated with the event or object." .

ocsf:user_agent  rdf:type    owl:DatatypeProperty;
        rdfs:label           "HTTP User-Agent";
        rdfs:range           ocsf:string_t;
        dcterms:description  "The request header that identifies the operating system and web browser." .

ocsf:bytes  rdf:type         owl:DatatypeProperty;
        rdfs:label           "Total Bytes";
        rdfs:range           ocsf:long_t;
        dcterms:description  "The total number of bytes (in and out)." .

ocsf:size  rdf:type          owl:DatatypeProperty;
        rdfs:label           "Size";
        rdfs:range           ocsf:long_t;
        dcterms:description  "The size of data, in bytes." .

ocsf:cis_controls  rdf:type  owl:ObjectProperty;
        rdfs:label           "CIS Controls";
        rdfs:range           ocsf:CISControl;
        dcterms:description  "The CIS Critical Security Controls is a prioritized set of actions to protect your organization and data from cyber-attack vectors." .

ocsf:criticality  rdf:type   owl:DatatypeProperty;
        rdfs:label           "Criticality";
        rdfs:range           ocsf:string_t;
        dcterms:description  "Criticality of a resource/object in question" .

ocsf:operation  rdf:type     owl:DatatypeProperty;
        rdfs:label           "Operation";
        rdfs:range           ocsf:string_t;
        dcterms:description  "Verb/Operation associated with the request" .

ocsf:SubjectAlternativeName
        rdf:type             owl:Class;
        rdfs:label           "Subject Alternative Name";
        rdfs:subClassOf      ocsf:Object;
        dcterms:description  "The Subject Alternative name (SAN) object describes a SAN secured by a digital certificate";
        ocsf:name            "san" .

ocsf:tactic  rdf:type        owl:ObjectProperty;
        rdfs:label           "Tactic";
        rdfs:range           ocsf:Tactic;
        dcterms:description  "The Tactic object describes the tactic ID and/or name that is associated to an attack, as defined by <a target='_blank' href='https://attack.mitre.org/wiki/ATT&CK_Matrix'>ATT&CK Matrix<sup>TM</sup></a>." .

ocsf:tls  rdf:type           owl:ObjectProperty;
        rdfs:label           "TLS";
        rdfs:range           ocsf:TransportLayerSecurityTLS;
        dcterms:description  "The Transport Layer Security (TLS) attributes." .

ocsf:length  rdf:type        owl:DatatypeProperty;
        rdfs:label           "Response Length";
        rdfs:range           ocsf:integer_t;
        dcterms:description  "The HTTP response length, in number of bytes." .

ocsf:product_uid  rdf:type   owl:DatatypeProperty;
        rdfs:label           "Product Identifier";
        rdfs:range           ocsf:string_t;
        dcterms:description  "Unique Identifier of a product." .

ocsf:vpc_uid  rdf:type       owl:DatatypeProperty;
        rdfs:label           "VPC UID";
        rdfs:range           ocsf:string_t;
        dcterms:description  "The unique identifier of the Virtual Private Cloud (VPC)." .

ocsf:resources  rdf:type     owl:ObjectProperty;
        rdfs:label           "Resources Array";
        rdfs:range           ocsf:ResourceDetails;
        dcterms:description  "Describes details about resources that were affected by the activity/event." .

ocsf:dkim  rdf:type          owl:DatatypeProperty;
        rdfs:label           "DKIM Status";
        rdfs:range           ocsf:string_t;
        dcterms:description  "The DomainKeys Identified Mail (DKIM) status of the email." .

ocsf:EmailURLActivityEvent
        rdf:type             owl:Class;
        rdfs:label           "Email URL Activity";
        rdfs:subClassOf      d3f:DigitalEvent;
        rdfs:subClassOf      [ rdf:type         owl:Restriction;
                               owl:cardinality  1;
                               owl:onProperty   ocsf:url
                             ];
        dcterms:description  "Email URL Activity events report URLs within an email.";
        ocsf:category        "network";
        ocsf:name            "email_url_activity";
        ocsf:profiles        "[\"host\",\"security_control\"]";
        ocsf:uid             12 .

ocsf:http_request  rdf:type  owl:ObjectProperty;
        rdfs:label           "HTTP Request";
        rdfs:range           ocsf:HTTPRequest;
        dcterms:description  "The HTTP Request Object documents attributes of a request made to a web server." .

ocsf:web_resources_result
        rdf:type             owl:ObjectProperty;
        rdfs:label           "Web Resources Result";
        rdfs:range           ocsf:WebResource;
        dcterms:description  "The results of the activity on web resources. It should contain the new values of the changed attributes of the web resources." .

ocsf:Rule  rdf:type          owl:Class;
        rdfs:label           "Rule";
        rdfs:subClassOf      ocsf:Entity;
        dcterms:description  "The Rule object describes characteristics of a rule associated with a policy or an event.";
        ocsf:name            "rule" .

ocsf:VulnerabilityDetails
        rdf:type             owl:Class;
        rdfs:label           "Vulnerability Details";
        rdfs:subClassOf      ocsf:Object;
        rdfs:subClassOf      [ rdf:type            owl:Restriction;
                               owl:onProperty      ocsf:kb_articles;
                               owl:someValuesFrom  ocsf:KBArticle
                             ];
        rdfs:subClassOf      [ rdf:type            owl:Restriction;
                               owl:onProperty      ocsf:cve;
                               owl:someValuesFrom  ocsf:CVE
                             ];
        rdfs:subClassOf      [ rdf:type            owl:Restriction;
                               owl:onProperty      ocsf:cwe;
                               owl:someValuesFrom  ocsf:CWE
                             ];
        rdfs:subClassOf      [ rdf:type            owl:Restriction;
                               owl:onProperty      ocsf:affected_code;
                               owl:someValuesFrom  ocsf:AffectedCode
                             ];
        rdfs:subClassOf      [ rdf:type            owl:Restriction;
                               owl:onProperty      ocsf:packages;
                               owl:someValuesFrom  ocsf:SoftwarePackage
                             ];
        rdfs:subClassOf      [ rdf:type            owl:Restriction;
                               owl:onProperty      ocsf:remediation;
                               owl:someValuesFrom  ocsf:Remediation
                             ];
        rdfs:subClassOf      [ rdf:type            owl:Restriction;
                               owl:onProperty      ocsf:affected_packages;
                               owl:someValuesFrom  ocsf:AffectedSoftwarePackage
                             ];
        dcterms:description  "The vulnerability is an unintended characteristic of a computing component or system configuration that multiplies the risk of an adverse event or a loss occurring either due to accidental exposure, deliberate attack, or conflict with new system components.";
        ocsf:constraints     "{\"at_least_one\":[\"cve\",\"cwe\"]}";
        ocsf:name            "vulnerability" .

ocsf:interface_uid  rdf:type  owl:DatatypeProperty;
        rdfs:label           "Network Interface ID";
        rdfs:range           ocsf:string_t;
        dcterms:description  "The unique identifier of the network interface." .

ocsf:EvidenceArtifacts
        rdf:type             owl:Class;
        rdfs:label           "Evidence Artifacts";
        rdfs:subClassOf      ocsf:Object;
        rdfs:subClassOf      [ rdf:type            owl:Restriction;
                               owl:onProperty      ocsf:src_endpoint;
                               owl:someValuesFrom  ocsf:NetworkEndpoint
                             ];
        rdfs:subClassOf      [ rdf:type            owl:Restriction;
                               owl:onProperty      ocsf:query;
                               owl:someValuesFrom  ocsf:DNSQuery
                             ];
        rdfs:subClassOf      [ rdf:type            owl:Restriction;
                               owl:onProperty      ocsf:process;
                               owl:someValuesFrom  ocsf:Process
                             ];
        rdfs:subClassOf      [ rdf:type            owl:Restriction;
                               owl:onProperty      ocsf:file;
                               owl:someValuesFrom  ocsf:File
                             ];
        rdfs:subClassOf      [ rdf:type            owl:Restriction;
                               owl:onProperty      ocsf:connection_info;
                               owl:someValuesFrom  ocsf:NetworkConnectionInformation
                             ];
        rdfs:subClassOf      [ rdf:type            owl:Restriction;
                               owl:onProperty      ocsf:api;
                               owl:someValuesFrom  ocsf:API
                             ];
        rdfs:subClassOf      [ rdf:type            owl:Restriction;
                               owl:onProperty      ocsf:actor;
                               owl:someValuesFrom  ocsf:Actor
                             ];
        rdfs:subClassOf      [ rdf:type            owl:Restriction;
                               owl:onProperty      ocsf:dst_endpoint;
                               owl:someValuesFrom  ocsf:NetworkEndpoint
                             ];
        dcterms:description  "A collection of evidence artifacts associated to the activity/activities that triggered a security detection.";
        ocsf:constraints     "{\"at_least_one\":[\"actor\",\"api\",\"connection_info\",\"data\",\"dst_endpoint\",\"file\",\"process\",\"query\",\"src_endpoint\"]}";
        ocsf:name            "evidences" .

ocsf:mac_t  rdf:type         rdfs:Datatype;
        rdfs:label           "MAC Address";
        rdfs:subClassOf      xsd:string;
        dcterms:description  "Media Access Control (MAC) address. For example: <code>18:36:F3:98:4F:9A</code>.";
        xsd:pattern          "^([0-9A-Fa-f]{2}[:-]){5}([0-9A-Fa-f]{2})$" .

ocsf:sensitivity  rdf:type   owl:DatatypeProperty;
        rdfs:label           "Sensitivity";
        rdfs:range           ocsf:string_t;
        dcterms:description  "The sensitivity of the firewall rule in the matched event. For example: HIGH." .

ocsf:nist  rdf:type          owl:DatatypeProperty;
        rdfs:label           "NIST List";
        rdfs:range           ocsf:string_t;
        dcterms:description  "The NIST Cybersecurity Framework recommendations for managing the cybersecurity risk." .

ocsf:run_state_id  rdf:type  owl:DatatypeProperty;
        rdfs:label           "Run State ID";
        rdfs:range           ocsf:integer_t;
        dcterms:description  "The normalized identifier of the state of the job or service. See specific usage." .

ocsf:WebResource  rdf:type   owl:Class;
        rdfs:label           "Web Resource";
        rdfs:subClassOf      ocsf:Resource;
        dcterms:description  "The Web Resource object describes characteristics of a web resource that was affected by the activity/event.";
        ocsf:name            "web_resource" .

ocsf:bios_ver  rdf:type      owl:DatatypeProperty;
        rdfs:label           "BIOS Version";
        rdfs:range           ocsf:string_t;
        dcterms:description  "The BIOS version. For example: <code>LENOVO G5ETA2WW (2.62)</code>." .

ocsf:capabilities  rdf:type  owl:DatatypeProperty;
        rdfs:label           "Capabilities";
        rdfs:range           ocsf:string_t;
        dcterms:description  "A list of RDP capabilities." .

ocsf:Product  rdf:type       owl:Class;
        rdfs:label           "Product";
        rdfs:subClassOf      ocsf:Entity;
        rdfs:subClassOf      [ rdf:type            owl:Restriction;
                               owl:onProperty      ocsf:feature;
                               owl:someValuesFrom  ocsf:Feature
                             ];
        dcterms:description  "The Product object describes characteristics of a software product.";
        ocsf:name            "product" .

ocsf:fixed_in_version
        rdf:type             owl:DatatypeProperty;
        rdfs:label           "Fixed In Version";
        rdfs:range           ocsf:string_t;
        dcterms:description  "The software package version in which a reported vulnerability was patched/fixed." .

ocsf:Reputation  rdf:type    owl:Class;
        rdfs:label           "Reputation";
        rdfs:subClassOf      ocsf:Object;
        dcterms:description  "The Reputation object describes the reputation/risk score of an entity (e.g. device, user, domain).";
        ocsf:name            "reputation" .

ocsf:category  rdf:type      owl:DatatypeProperty;
        rdfs:label           "Category";
        rdfs:range           ocsf:string_t;
        dcterms:description  "The object category. See specific usage." .

ocsf:packages  rdf:type      owl:ObjectProperty;
        rdfs:label           "Software Packages";
        rdfs:range           ocsf:SoftwarePackage;
        dcterms:description  "List of vulnerable packages as identified by the security product" .

ocsf:metadata  rdf:type      owl:ObjectProperty;
        rdfs:label           "Metadata";
        rdfs:range           ocsf:Metadata;
        dcterms:description  "The metadata associated with the event or a finding." .

ocsf:build  rdf:type         owl:DatatypeProperty;
        rdfs:label           "OS Build";
        rdfs:range           ocsf:string_t;
        dcterms:description  "The operating system build number." .

ocsf:bulletin  rdf:type      owl:DatatypeProperty;
        rdfs:label           "Patch Bulletin";
        rdfs:range           ocsf:string_t;
        dcterms:description  "The vendor bulletin identfier." .

ocsf:last_login_time  rdf:type  owl:DatatypeProperty;
        rdfs:label           "Last Login";
        rdfs:range           ocsf:timestamp_t;
        dcterms:description  "The last time when the user logged in." .

ocsf:NTPActivityEvent
        rdf:type             owl:Class;
        rdfs:label           "NTP Activity";
        rdfs:subClassOf      d3f:DigitalEvent;
        dcterms:description  "The Network Time Protocol (NTP) Activity events report instances of remote clients synchronizing their clocks with an NTP server, as observed on the network.";
        ocsf:name            "ntp_activity";
        ocsf:uid             13 .

ocsf:email_addr  rdf:type    owl:DatatypeProperty;
        rdfs:label           "Email Address";
        rdfs:range           ocsf:email_t;
        dcterms:description  "The user's primary email address." .

ocsf:integer_t  rdf:type     rdfs:Datatype;
        rdfs:label           "Integer";
        rdfs:subClassOf      xsd:integer;
        dcterms:description  "Signed integer value." .

ocsf:impact  rdf:type        owl:DatatypeProperty;
        rdfs:label           "Impact";
        rdfs:range           ocsf:string_t;
        dcterms:description  "The impact , normalized to the caption of the impact_id value. In the case of 'Other', it is defined by the event source." .

ocsf:HTTPHeader  rdf:type    owl:Class;
        rdfs:label           "HTTP Header";
        rdfs:subClassOf      ocsf:Object;
        dcterms:description  "TThe HTTP Header object represents the headers sent in an HTTP request or response. HTTP headers are key-value pairs that convey additional information about the HTTP message, including details about the content, caching, authentication, encoding, and other aspects of the communication.";
        ocsf:name            "http_header" .

ocsf:BaseEvent  rdf:type     owl:Class;
        rdfs:label           "Base Event";
        rdfs:subClassOf      ocsf:SchemaExtension , ocsf:AuthorizationResult , ocsf:PeripheralDevice , ocsf:Observable , ocsf:KeyboardInformation , ocsf:Analytic , ocsf:IdentityProvider , ocsf:NetworkInterface , ocsf:Finding , ocsf:Endpoint , ocsf:Metadata , ocsf:Policy , ocsf:EPSS , ocsf:DCERPC , ocsf:VulnerabilityDetails , ocsf:Email , ocsf:DigitalCertificate , ocsf:SubjectAlternativeName , ocsf:Remediation , ocsf:EmailAuthentication , ocsf:Object , ocsf:NetworkTraffic , ocsf:KBArticle , ocsf:Organization , ocsf:Group , ocsf:Logger , ocsf:GeoLocation , ocsf:FirewallRule , ocsf:ResourceDetails , ocsf:Account , ocsf:Tactic , ocsf:File , ocsf:LDAPPerson , ocsf:Feature , ocsf:Image , ocsf:WebResource , ocsf:DNSAnswer , ocsf:Job , ocsf:TLSExtension , ocsf:NetworkEndpoint , ocsf:HTTPCookie , ocsf:ResponseElements , ocsf:Malware , ocsf:Session , ocsf:User , ocsf:AffectedCode , d3f:DigitalEvent , ocsf:CISBenchmark , ocsf:HTTPHeader , ocsf:Resource , ocsf:CVE , ocsf:Service , ocsf:Entity , ocsf:ManagedEntity , ocsf:DNSQuery , ocsf:NetworkProxyEndpoint , ocsf:CVSSScore , ocsf:DNS , ocsf:Cloud , ocsf:Process , ocsf:Technique , ocsf:HTTPRequest , ocsf:CISBenchmarkResult , ocsf:SoftwarePackage , ocsf:OperatingSystemOS , ocsf:AffectedSoftwarePackage , ocsf:TransportLayerSecurityTLS , ocsf:Metric , ocsf:Fingerprint , ocsf:Module , ocsf:Container , ocsf:FindingInformation , ocsf:DeviceHardwareInfo , ocsf:Reputation , ocsf:RequestElements , ocsf:Rule , ocsf:KillChainPhase , ocsf:Actor , ocsf:CISCSC , ocsf:Enrichment , ocsf:SubTechnique , ocsf:Device , ocsf:Product , ocsf:RelatedEvent , ocsf:EvidenceArtifacts , ocsf:CISControl , ocsf:HTTPResponse , ocsf:KernelResource , ocsf:CWE , ocsf:KernelExtension , ocsf:DigitalSignature , ocsf:HASSH , ocsf:NetworkConnectionInformation , ocsf:RPCInterface , ocsf:API , ocsf:Display , ocsf:Compliance , ocsf:UniformResourceLocator , ocsf:MITREATTCK;
        rdfs:subClassOf      [ rdf:type         owl:Restriction;
                               owl:cardinality  1;
                               owl:onProperty   ocsf:metadata
                             ];
        rdfs:subClassOf      [ rdf:type         owl:Restriction;
                               owl:cardinality  1;
                               owl:onProperty   ocsf:metadata
                             ];
        rdfs:subClassOf      [ rdf:type         owl:Restriction;
                               owl:cardinality  1;
                               owl:onProperty   ocsf:metadata
                             ];
        rdfs:subClassOf      [ rdf:type            owl:Restriction;
                               owl:onProperty      ocsf:observables;
                               owl:someValuesFrom  ocsf:Observable
                             ];
        rdfs:subClassOf      [ rdf:type            owl:Restriction;
                               owl:onProperty      ocsf:unmapped;
                               owl:someValuesFrom  ocsf:Object
                             ];
        rdfs:subClassOf      [ rdf:type            owl:Restriction;
                               owl:onProperty      ocsf:enrichments;
                               owl:someValuesFrom  ocsf:Enrichment
                             ];
        rdfs:subClassOf      [ rdf:type            owl:Restriction;
                               owl:onProperty      ocsf:observables;
                               owl:someValuesFrom  ocsf:Observable
                             ];
        rdfs:subClassOf      [ rdf:type            owl:Restriction;
                               owl:onProperty      ocsf:enrichments;
                               owl:someValuesFrom  ocsf:Enrichment
                             ];
        rdfs:subClassOf      [ rdf:type         owl:Restriction;
                               owl:cardinality  1;
                               owl:onProperty   ocsf:metadata
                             ];
        rdfs:subClassOf      [ rdf:type         owl:Restriction;
                               owl:cardinality  1;
                               owl:onProperty   ocsf:metadata
                             ];
        rdfs:subClassOf      [ rdf:type            owl:Restriction;
                               owl:onProperty      ocsf:enrichments;
                               owl:someValuesFrom  ocsf:Enrichment
                             ];
        rdfs:subClassOf      [ rdf:type            owl:Restriction;
                               owl:onProperty      ocsf:unmapped;
                               owl:someValuesFrom  ocsf:Object
                             ];
        rdfs:subClassOf      [ rdf:type            owl:Restriction;
                               owl:onProperty      ocsf:unmapped;
                               owl:someValuesFrom  ocsf:Object
                             ];
        rdfs:subClassOf      [ rdf:type            owl:Restriction;
                               owl:onProperty      ocsf:unmapped;
                               owl:someValuesFrom  ocsf:Object
                             ];
        rdfs:subClassOf      [ rdf:type            owl:Restriction;
                               owl:onProperty      ocsf:unmapped;
                               owl:someValuesFrom  ocsf:Object
                             ];
        rdfs:subClassOf      [ rdf:type         owl:Restriction;
                               owl:cardinality  1;
                               owl:onProperty   ocsf:metadata
                             ];
        rdfs:subClassOf      [ rdf:type            owl:Restriction;
                               owl:onProperty      ocsf:observables;
                               owl:someValuesFrom  ocsf:Observable
                             ];
        rdfs:subClassOf      [ rdf:type            owl:Restriction;
                               owl:onProperty      ocsf:observables;
                               owl:someValuesFrom  ocsf:Observable
                             ];
        rdfs:subClassOf      [ rdf:type            owl:Restriction;
                               owl:onProperty      ocsf:enrichments;
                               owl:someValuesFrom  ocsf:Enrichment
                             ];
        rdfs:subClassOf      [ rdf:type            owl:Restriction;
                               owl:onProperty      ocsf:observables;
                               owl:someValuesFrom  ocsf:Observable
                             ];
        rdfs:subClassOf      [ rdf:type         owl:Restriction;
                               owl:cardinality  1;
                               owl:onProperty   ocsf:metadata
                             ];
        rdfs:subClassOf      [ rdf:type            owl:Restriction;
                               owl:onProperty      ocsf:unmapped;
                               owl:someValuesFrom  ocsf:Object
                             ];
        rdfs:subClassOf      [ rdf:type            owl:Restriction;
                               owl:onProperty      ocsf:unmapped;
                               owl:someValuesFrom  ocsf:Object
                             ];
        rdfs:subClassOf      [ rdf:type         owl:Restriction;
                               owl:cardinality  1;
                               owl:onProperty   ocsf:metadata
                             ];
        rdfs:subClassOf      [ rdf:type            owl:Restriction;
                               owl:onProperty      ocsf:enrichments;
                               owl:someValuesFrom  ocsf:Enrichment
                             ];
        rdfs:subClassOf      [ rdf:type            owl:Restriction;
                               owl:onProperty      ocsf:enrichments;
                               owl:someValuesFrom  ocsf:Enrichment
                             ];
        rdfs:subClassOf      [ rdf:type            owl:Restriction;
                               owl:onProperty      ocsf:enrichments;
                               owl:someValuesFrom  ocsf:Enrichment
                             ];
        rdfs:subClassOf      [ rdf:type         owl:Restriction;
                               owl:cardinality  1;
                               owl:onProperty   ocsf:metadata
                             ];
        rdfs:subClassOf      [ rdf:type            owl:Restriction;
                               owl:onProperty      ocsf:observables;
                               owl:someValuesFrom  ocsf:Observable
                             ];
        rdfs:subClassOf      [ rdf:type            owl:Restriction;
                               owl:onProperty      ocsf:enrichments;
                               owl:someValuesFrom  ocsf:Enrichment
                             ];
        rdfs:subClassOf      [ rdf:type            owl:Restriction;
                               owl:onProperty      ocsf:unmapped;
                               owl:someValuesFrom  ocsf:Object
                             ];
        rdfs:subClassOf      [ rdf:type            owl:Restriction;
                               owl:onProperty      ocsf:observables;
                               owl:someValuesFrom  ocsf:Observable
                             ];
        rdfs:subClassOf      [ rdf:type         owl:Restriction;
                               owl:cardinality  1;
                               owl:onProperty   ocsf:metadata
                             ];
        rdfs:subClassOf      [ rdf:type            owl:Restriction;
                               owl:onProperty      ocsf:observables;
                               owl:someValuesFrom  ocsf:Observable
                             ];
        rdfs:subClassOf      [ rdf:type            owl:Restriction;
                               owl:onProperty      ocsf:unmapped;
                               owl:someValuesFrom  ocsf:Object
                             ];
        rdfs:subClassOf      [ rdf:type            owl:Restriction;
                               owl:onProperty      ocsf:enrichments;
                               owl:someValuesFrom  ocsf:Enrichment
                             ];
        rdfs:subClassOf      [ rdf:type            owl:Restriction;
                               owl:onProperty      ocsf:unmapped;
                               owl:someValuesFrom  ocsf:Object
                             ];
        rdfs:subClassOf      [ rdf:type         owl:Restriction;
                               owl:cardinality  1;
                               owl:onProperty   ocsf:metadata
                             ];
        rdfs:subClassOf      [ rdf:type         owl:Restriction;
                               owl:cardinality  1;
                               owl:onProperty   ocsf:metadata
                             ];
        rdfs:subClassOf      [ rdf:type            owl:Restriction;
                               owl:onProperty      ocsf:observables;
                               owl:someValuesFrom  ocsf:Observable
                             ];
        rdfs:subClassOf      [ rdf:type            owl:Restriction;
                               owl:onProperty      ocsf:unmapped;
                               owl:someValuesFrom  ocsf:Object
                             ];
        rdfs:subClassOf      [ rdf:type         owl:Restriction;
                               owl:cardinality  1;
                               owl:onProperty   ocsf:metadata
                             ];
        rdfs:subClassOf      [ rdf:type            owl:Restriction;
                               owl:onProperty      ocsf:unmapped;
                               owl:someValuesFrom  ocsf:Object
                             ];
        rdfs:subClassOf      [ rdf:type         owl:Restriction;
                               owl:cardinality  1;
                               owl:onProperty   ocsf:metadata
                             ];
        rdfs:subClassOf      [ rdf:type         owl:Restriction;
                               owl:cardinality  1;
                               owl:onProperty   ocsf:metadata
                             ];
        rdfs:subClassOf      [ rdf:type         owl:Restriction;
                               owl:cardinality  1;
                               owl:onProperty   ocsf:metadata
                             ];
        rdfs:subClassOf      [ rdf:type            owl:Restriction;
                               owl:onProperty      ocsf:enrichments;
                               owl:someValuesFrom  ocsf:Enrichment
                             ];
        rdfs:subClassOf      [ rdf:type            owl:Restriction;
                               owl:onProperty      ocsf:unmapped;
                               owl:someValuesFrom  ocsf:Object
                             ];
        rdfs:subClassOf      [ rdf:type         owl:Restriction;
                               owl:cardinality  1;
                               owl:onProperty   ocsf:metadata
                             ];
        rdfs:subClassOf      [ rdf:type            owl:Restriction;
                               owl:onProperty      ocsf:unmapped;
                               owl:someValuesFrom  ocsf:Object
                             ];
        rdfs:subClassOf      [ rdf:type            owl:Restriction;
                               owl:onProperty      ocsf:unmapped;
                               owl:someValuesFrom  ocsf:Object
                             ];
        rdfs:subClassOf      [ rdf:type         owl:Restriction;
                               owl:cardinality  1;
                               owl:onProperty   ocsf:metadata
                             ];
        rdfs:subClassOf      [ rdf:type            owl:Restriction;
                               owl:onProperty      ocsf:enrichments;
                               owl:someValuesFrom  ocsf:Enrichment
                             ];
        rdfs:subClassOf      [ rdf:type         owl:Restriction;
                               owl:cardinality  1;
                               owl:onProperty   ocsf:metadata
                             ];
        rdfs:subClassOf      [ rdf:type            owl:Restriction;
                               owl:onProperty      ocsf:observables;
                               owl:someValuesFrom  ocsf:Observable
                             ];
        rdfs:subClassOf      [ rdf:type            owl:Restriction;
                               owl:onProperty      ocsf:unmapped;
                               owl:someValuesFrom  ocsf:Object
                             ];
        rdfs:subClassOf      [ rdf:type            owl:Restriction;
                               owl:onProperty      ocsf:unmapped;
                               owl:someValuesFrom  ocsf:Object
                             ];
        rdfs:subClassOf      [ rdf:type            owl:Restriction;
                               owl:onProperty      ocsf:enrichments;
                               owl:someValuesFrom  ocsf:Enrichment
                             ];
        rdfs:subClassOf      [ rdf:type         owl:Restriction;
                               owl:cardinality  1;
                               owl:onProperty   ocsf:metadata
                             ];
        rdfs:subClassOf      [ rdf:type            owl:Restriction;
                               owl:onProperty      ocsf:enrichments;
                               owl:someValuesFrom  ocsf:Enrichment
                             ];
        rdfs:subClassOf      [ rdf:type         owl:Restriction;
                               owl:cardinality  1;
                               owl:onProperty   ocsf:metadata
                             ];
        rdfs:subClassOf      [ rdf:type         owl:Restriction;
                               owl:cardinality  1;
                               owl:onProperty   ocsf:metadata
                             ];
        rdfs:subClassOf      [ rdf:type         owl:Restriction;
                               owl:cardinality  1;
                               owl:onProperty   ocsf:metadata
                             ];
        rdfs:subClassOf      [ rdf:type            owl:Restriction;
                               owl:onProperty      ocsf:unmapped;
                               owl:someValuesFrom  ocsf:Object
                             ];
        rdfs:subClassOf      [ rdf:type         owl:Restriction;
                               owl:cardinality  1;
                               owl:onProperty   ocsf:metadata
                             ];
        rdfs:subClassOf      [ rdf:type            owl:Restriction;
                               owl:onProperty      ocsf:observables;
                               owl:someValuesFrom  ocsf:Observable
                             ];
        rdfs:subClassOf      [ rdf:type            owl:Restriction;
                               owl:onProperty      ocsf:observables;
                               owl:someValuesFrom  ocsf:Observable
                             ];
        rdfs:subClassOf      [ rdf:type            owl:Restriction;
                               owl:onProperty      ocsf:unmapped;
                               owl:someValuesFrom  ocsf:Object
                             ];
        rdfs:subClassOf      [ rdf:type            owl:Restriction;
                               owl:onProperty      ocsf:enrichments;
                               owl:someValuesFrom  ocsf:Enrichment
                             ];
        rdfs:subClassOf      [ rdf:type         owl:Restriction;
                               owl:cardinality  1;
                               owl:onProperty   ocsf:metadata
                             ];
        rdfs:subClassOf      [ rdf:type            owl:Restriction;
                               owl:onProperty      ocsf:observables;
                               owl:someValuesFrom  ocsf:Observable
                             ];
        rdfs:subClassOf      [ rdf:type         owl:Restriction;
                               owl:cardinality  1;
                               owl:onProperty   ocsf:metadata
                             ];
        rdfs:subClassOf      [ rdf:type            owl:Restriction;
                               owl:onProperty      ocsf:enrichments;
                               owl:someValuesFrom  ocsf:Enrichment
                             ];
        rdfs:subClassOf      [ rdf:type            owl:Restriction;
                               owl:onProperty      ocsf:observables;
                               owl:someValuesFrom  ocsf:Observable
                             ];
        rdfs:subClassOf      [ rdf:type         owl:Restriction;
                               owl:cardinality  1;
                               owl:onProperty   ocsf:metadata
                             ];
        rdfs:subClassOf      [ rdf:type            owl:Restriction;
                               owl:onProperty      ocsf:observables;
                               owl:someValuesFrom  ocsf:Observable
                             ];
        rdfs:subClassOf      [ rdf:type            owl:Restriction;
                               owl:onProperty      ocsf:unmapped;
                               owl:someValuesFrom  ocsf:Object
                             ];
        rdfs:subClassOf      [ rdf:type            owl:Restriction;
                               owl:onProperty      ocsf:enrichments;
                               owl:someValuesFrom  ocsf:Enrichment
                             ];
        rdfs:subClassOf      [ rdf:type         owl:Restriction;
                               owl:cardinality  1;
                               owl:onProperty   ocsf:metadata
                             ];
        rdfs:subClassOf      [ rdf:type         owl:Restriction;
                               owl:cardinality  1;
                               owl:onProperty   ocsf:metadata
                             ];
        rdfs:subClassOf      [ rdf:type            owl:Restriction;
                               owl:onProperty      ocsf:enrichments;
                               owl:someValuesFrom  ocsf:Enrichment
                             ];
        rdfs:subClassOf      [ rdf:type            owl:Restriction;
                               owl:onProperty      ocsf:observables;
                               owl:someValuesFrom  ocsf:Observable
                             ];
        rdfs:subClassOf      [ rdf:type         owl:Restriction;
                               owl:cardinality  1;
                               owl:onProperty   ocsf:metadata
                             ];
        rdfs:subClassOf      [ rdf:type         owl:Restriction;
                               owl:cardinality  1;
                               owl:onProperty   ocsf:metadata
                             ];
        rdfs:subClassOf      [ rdf:type            owl:Restriction;
                               owl:onProperty      ocsf:unmapped;
                               owl:someValuesFrom  ocsf:Object
                             ];
        rdfs:subClassOf      [ rdf:type         owl:Restriction;
                               owl:cardinality  1;
                               owl:onProperty   ocsf:metadata
                             ];
        rdfs:subClassOf      [ rdf:type         owl:Restriction;
                               owl:cardinality  1;
                               owl:onProperty   ocsf:metadata
                             ];
        rdfs:subClassOf      [ rdf:type            owl:Restriction;
                               owl:onProperty      ocsf:observables;
                               owl:someValuesFrom  ocsf:Observable
                             ];
        rdfs:subClassOf      [ rdf:type            owl:Restriction;
                               owl:onProperty      ocsf:unmapped;
                               owl:someValuesFrom  ocsf:Object
                             ];
        rdfs:subClassOf      [ rdf:type         owl:Restriction;
                               owl:cardinality  1;
                               owl:onProperty   ocsf:metadata
                             ];
        rdfs:subClassOf      [ rdf:type            owl:Restriction;
                               owl:onProperty      ocsf:enrichments;
                               owl:someValuesFrom  ocsf:Enrichment
                             ];
        rdfs:subClassOf      [ rdf:type            owl:Restriction;
                               owl:onProperty      ocsf:enrichments;
                               owl:someValuesFrom  ocsf:Enrichment
                             ];
        rdfs:subClassOf      [ rdf:type            owl:Restriction;
                               owl:onProperty      ocsf:enrichments;
                               owl:someValuesFrom  ocsf:Enrichment
                             ];
        rdfs:subClassOf      [ rdf:type            owl:Restriction;
                               owl:onProperty      ocsf:enrichments;
                               owl:someValuesFrom  ocsf:Enrichment
                             ];
        rdfs:subClassOf      [ rdf:type         owl:Restriction;
                               owl:cardinality  1;
                               owl:onProperty   ocsf:metadata
                             ];
        rdfs:subClassOf      [ rdf:type            owl:Restriction;
                               owl:onProperty      ocsf:observables;
                               owl:someValuesFrom  ocsf:Observable
                             ];
        rdfs:subClassOf      [ rdf:type            owl:Restriction;
                               owl:onProperty      ocsf:unmapped;
                               owl:someValuesFrom  ocsf:Object
                             ];
        rdfs:subClassOf      [ rdf:type            owl:Restriction;
                               owl:onProperty      ocsf:observables;
                               owl:someValuesFrom  ocsf:Observable
                             ];
        rdfs:subClassOf      [ rdf:type            owl:Restriction;
                               owl:onProperty      ocsf:unmapped;
                               owl:someValuesFrom  ocsf:Object
                             ];
        rdfs:subClassOf      [ rdf:type         owl:Restriction;
                               owl:cardinality  1;
                               owl:onProperty   ocsf:metadata
                             ];
        rdfs:subClassOf      [ rdf:type            owl:Restriction;
                               owl:onProperty      ocsf:enrichments;
                               owl:someValuesFrom  ocsf:Enrichment
                             ];
        rdfs:subClassOf      [ rdf:type         owl:Restriction;
                               owl:cardinality  1;
                               owl:onProperty   ocsf:metadata
                             ];
        rdfs:subClassOf      [ rdf:type            owl:Restriction;
                               owl:onProperty      ocsf:enrichments;
                               owl:someValuesFrom  ocsf:Enrichment
                             ];
        rdfs:subClassOf      [ rdf:type         owl:Restriction;
                               owl:cardinality  1;
                               owl:onProperty   ocsf:metadata
                             ];
        rdfs:subClassOf      [ rdf:type            owl:Restriction;
                               owl:onProperty      ocsf:observables;
                               owl:someValuesFrom  ocsf:Observable
                             ];
        rdfs:subClassOf      [ rdf:type            owl:Restriction;
                               owl:onProperty      ocsf:enrichments;
                               owl:someValuesFrom  ocsf:Enrichment
                             ];
        rdfs:subClassOf      [ rdf:type            owl:Restriction;
                               owl:onProperty      ocsf:observables;
                               owl:someValuesFrom  ocsf:Observable
                             ];
        rdfs:subClassOf      [ rdf:type            owl:Restriction;
                               owl:onProperty      ocsf:enrichments;
                               owl:someValuesFrom  ocsf:Enrichment
                             ];
        rdfs:subClassOf      [ rdf:type            owl:Restriction;
                               owl:onProperty      ocsf:unmapped;
                               owl:someValuesFrom  ocsf:Object
                             ];
        rdfs:subClassOf      [ rdf:type         owl:Restriction;
                               owl:cardinality  1;
                               owl:onProperty   ocsf:metadata
                             ];
        rdfs:subClassOf      [ rdf:type            owl:Restriction;
                               owl:onProperty      ocsf:observables;
                               owl:someValuesFrom  ocsf:Observable
                             ];
        rdfs:subClassOf      [ rdf:type            owl:Restriction;
                               owl:onProperty      ocsf:observables;
                               owl:someValuesFrom  ocsf:Observable
                             ];
        rdfs:subClassOf      [ rdf:type         owl:Restriction;
                               owl:cardinality  1;
                               owl:onProperty   ocsf:metadata
                             ];
        rdfs:subClassOf      [ rdf:type            owl:Restriction;
                               owl:onProperty      ocsf:unmapped;
                               owl:someValuesFrom  ocsf:Object
                             ];
        rdfs:subClassOf      [ rdf:type            owl:Restriction;
                               owl:onProperty      ocsf:unmapped;
                               owl:someValuesFrom  ocsf:Object
                             ];
        rdfs:subClassOf      [ rdf:type            owl:Restriction;
                               owl:onProperty      ocsf:observables;
                               owl:someValuesFrom  ocsf:Observable
                             ];
        rdfs:subClassOf      [ rdf:type            owl:Restriction;
                               owl:onProperty      ocsf:observables;
                               owl:someValuesFrom  ocsf:Observable
                             ];
        rdfs:subClassOf      [ rdf:type            owl:Restriction;
                               owl:onProperty      ocsf:observables;
                               owl:someValuesFrom  ocsf:Observable
                             ];
        rdfs:subClassOf      [ rdf:type         owl:Restriction;
                               owl:cardinality  1;
                               owl:onProperty   ocsf:metadata
                             ];
        rdfs:subClassOf      [ rdf:type            owl:Restriction;
                               owl:onProperty      ocsf:enrichments;
                               owl:someValuesFrom  ocsf:Enrichment
                             ];
        rdfs:subClassOf      [ rdf:type            owl:Restriction;
                               owl:onProperty      ocsf:enrichments;
                               owl:someValuesFrom  ocsf:Enrichment
                             ];
        rdfs:subClassOf      [ rdf:type            owl:Restriction;
                               owl:onProperty      ocsf:observables;
                               owl:someValuesFrom  ocsf:Observable
                             ];
        rdfs:subClassOf      [ rdf:type            owl:Restriction;
                               owl:onProperty      ocsf:enrichments;
                               owl:someValuesFrom  ocsf:Enrichment
                             ];
        rdfs:subClassOf      [ rdf:type            owl:Restriction;
                               owl:onProperty      ocsf:unmapped;
                               owl:someValuesFrom  ocsf:Object
                             ];
        rdfs:subClassOf      [ rdf:type            owl:Restriction;
                               owl:onProperty      ocsf:unmapped;
                               owl:someValuesFrom  ocsf:Object
                             ];
        rdfs:subClassOf      [ rdf:type            owl:Restriction;
                               owl:onProperty      ocsf:enrichments;
                               owl:someValuesFrom  ocsf:Enrichment
                             ];
        rdfs:subClassOf      [ rdf:type            owl:Restriction;
                               owl:onProperty      ocsf:unmapped;
                               owl:someValuesFrom  ocsf:Object
                             ];
        rdfs:subClassOf      [ rdf:type            owl:Restriction;
                               owl:onProperty      ocsf:unmapped;
                               owl:someValuesFrom  ocsf:Object
                             ];
        rdfs:subClassOf      [ rdf:type            owl:Restriction;
                               owl:onProperty      ocsf:observables;
                               owl:someValuesFrom  ocsf:Observable
                             ];
        rdfs:subClassOf      [ rdf:type            owl:Restriction;
                               owl:onProperty      ocsf:enrichments;
                               owl:someValuesFrom  ocsf:Enrichment
                             ];
        rdfs:subClassOf      [ rdf:type            owl:Restriction;
                               owl:onProperty      ocsf:observables;
                               owl:someValuesFrom  ocsf:Observable
                             ];
        rdfs:subClassOf      [ rdf:type         owl:Restriction;
                               owl:cardinality  1;
                               owl:onProperty   ocsf:metadata
                             ];
        rdfs:subClassOf      [ rdf:type         owl:Restriction;
                               owl:cardinality  1;
                               owl:onProperty   ocsf:metadata
                             ];
        rdfs:subClassOf      [ rdf:type         owl:Restriction;
                               owl:cardinality  1;
                               owl:onProperty   ocsf:metadata
                             ];
        rdfs:subClassOf      [ rdf:type            owl:Restriction;
                               owl:onProperty      ocsf:unmapped;
                               owl:someValuesFrom  ocsf:Object
                             ];
        rdfs:subClassOf      [ rdf:type            owl:Restriction;
                               owl:onProperty      ocsf:unmapped;
                               owl:someValuesFrom  ocsf:Object
                             ];
        rdfs:subClassOf      [ rdf:type            owl:Restriction;
                               owl:onProperty      ocsf:enrichments;
                               owl:someValuesFrom  ocsf:Enrichment
                             ];
        rdfs:subClassOf      [ rdf:type            owl:Restriction;
                               owl:onProperty      ocsf:unmapped;
                               owl:someValuesFrom  ocsf:Object
                             ];
        rdfs:subClassOf      [ rdf:type         owl:Restriction;
                               owl:cardinality  1;
                               owl:onProperty   ocsf:metadata
                             ];
        rdfs:subClassOf      [ rdf:type         owl:Restriction;
                               owl:cardinality  1;
                               owl:onProperty   ocsf:metadata
                             ];
        rdfs:subClassOf      [ rdf:type            owl:Restriction;
                               owl:onProperty      ocsf:unmapped;
                               owl:someValuesFrom  ocsf:Object
                             ];
        rdfs:subClassOf      [ rdf:type            owl:Restriction;
                               owl:onProperty      ocsf:unmapped;
                               owl:someValuesFrom  ocsf:Object
                             ];
        rdfs:subClassOf      [ rdf:type            owl:Restriction;
                               owl:onProperty      ocsf:enrichments;
                               owl:someValuesFrom  ocsf:Enrichment
                             ];
        rdfs:subClassOf      [ rdf:type            owl:Restriction;
                               owl:onProperty      ocsf:enrichments;
                               owl:someValuesFrom  ocsf:Enrichment
                             ];
        rdfs:subClassOf      [ rdf:type            owl:Restriction;
                               owl:onProperty      ocsf:unmapped;
                               owl:someValuesFrom  ocsf:Object
                             ];
        rdfs:subClassOf      [ rdf:type            owl:Restriction;
                               owl:onProperty      ocsf:observables;
                               owl:someValuesFrom  ocsf:Observable
                             ];
        rdfs:subClassOf      [ rdf:type            owl:Restriction;
                               owl:onProperty      ocsf:observables;
                               owl:someValuesFrom  ocsf:Observable
                             ];
        rdfs:subClassOf      [ rdf:type            owl:Restriction;
                               owl:onProperty      ocsf:unmapped;
                               owl:someValuesFrom  ocsf:Object
                             ];
        rdfs:subClassOf      [ rdf:type            owl:Restriction;
                               owl:onProperty      ocsf:observables;
                               owl:someValuesFrom  ocsf:Observable
                             ];
        rdfs:subClassOf      [ rdf:type         owl:Restriction;
                               owl:cardinality  1;
                               owl:onProperty   ocsf:metadata
                             ];
        rdfs:subClassOf      [ rdf:type            owl:Restriction;
                               owl:onProperty      ocsf:unmapped;
                               owl:someValuesFrom  ocsf:Object
                             ];
        rdfs:subClassOf      [ rdf:type            owl:Restriction;
                               owl:onProperty      ocsf:unmapped;
                               owl:someValuesFrom  ocsf:Object
                             ];
        rdfs:subClassOf      [ rdf:type            owl:Restriction;
                               owl:onProperty      ocsf:enrichments;
                               owl:someValuesFrom  ocsf:Enrichment
                             ];
        rdfs:subClassOf      [ rdf:type            owl:Restriction;
                               owl:onProperty      ocsf:enrichments;
                               owl:someValuesFrom  ocsf:Enrichment
                             ];
        rdfs:subClassOf      [ rdf:type            owl:Restriction;
                               owl:onProperty      ocsf:observables;
                               owl:someValuesFrom  ocsf:Observable
                             ];
        rdfs:subClassOf      [ rdf:type         owl:Restriction;
                               owl:cardinality  1;
                               owl:onProperty   ocsf:metadata
                             ];
        rdfs:subClassOf      [ rdf:type            owl:Restriction;
                               owl:onProperty      ocsf:unmapped;
                               owl:someValuesFrom  ocsf:Object
                             ];
        rdfs:subClassOf      [ rdf:type            owl:Restriction;
                               owl:onProperty      ocsf:observables;
                               owl:someValuesFrom  ocsf:Observable
                             ];
        rdfs:subClassOf      [ rdf:type         owl:Restriction;
                               owl:cardinality  1;
                               owl:onProperty   ocsf:metadata
                             ];
        rdfs:subClassOf      [ rdf:type            owl:Restriction;
                               owl:onProperty      ocsf:enrichments;
                               owl:someValuesFrom  ocsf:Enrichment
                             ];
        rdfs:subClassOf      [ rdf:type         owl:Restriction;
                               owl:cardinality  1;
                               owl:onProperty   ocsf:metadata
                             ];
        rdfs:subClassOf      [ rdf:type            owl:Restriction;
                               owl:onProperty      ocsf:unmapped;
                               owl:someValuesFrom  ocsf:Object
                             ];
        rdfs:subClassOf      [ rdf:type            owl:Restriction;
                               owl:onProperty      ocsf:observables;
                               owl:someValuesFrom  ocsf:Observable
                             ];
        rdfs:subClassOf      [ rdf:type            owl:Restriction;
                               owl:onProperty      ocsf:enrichments;
                               owl:someValuesFrom  ocsf:Enrichment
                             ];
        rdfs:subClassOf      [ rdf:type            owl:Restriction;
                               owl:onProperty      ocsf:observables;
                               owl:someValuesFrom  ocsf:Observable
                             ];
        rdfs:subClassOf      [ rdf:type            owl:Restriction;
                               owl:onProperty      ocsf:observables;
                               owl:someValuesFrom  ocsf:Observable
                             ];
        rdfs:subClassOf      [ rdf:type            owl:Restriction;
                               owl:onProperty      ocsf:unmapped;
                               owl:someValuesFrom  ocsf:Object
                             ];
        rdfs:subClassOf      [ rdf:type         owl:Restriction;
                               owl:cardinality  1;
                               owl:onProperty   ocsf:metadata
                             ];
        rdfs:subClassOf      [ rdf:type            owl:Restriction;
                               owl:onProperty      ocsf:unmapped;
                               owl:someValuesFrom  ocsf:Object
                             ];
        rdfs:subClassOf      [ rdf:type            owl:Restriction;
                               owl:onProperty      ocsf:enrichments;
                               owl:someValuesFrom  ocsf:Enrichment
                             ];
        rdfs:subClassOf      [ rdf:type            owl:Restriction;
                               owl:onProperty      ocsf:observables;
                               owl:someValuesFrom  ocsf:Observable
                             ];
        rdfs:subClassOf      [ rdf:type            owl:Restriction;
                               owl:onProperty      ocsf:unmapped;
                               owl:someValuesFrom  ocsf:Object
                             ];
        rdfs:subClassOf      [ rdf:type         owl:Restriction;
                               owl:cardinality  1;
                               owl:onProperty   ocsf:metadata
                             ];
        rdfs:subClassOf      [ rdf:type            owl:Restriction;
                               owl:onProperty      ocsf:enrichments;
                               owl:someValuesFrom  ocsf:Enrichment
                             ];
        rdfs:subClassOf      [ rdf:type         owl:Restriction;
                               owl:cardinality  1;
                               owl:onProperty   ocsf:metadata
                             ];
        rdfs:subClassOf      [ rdf:type            owl:Restriction;
                               owl:onProperty      ocsf:observables;
                               owl:someValuesFrom  ocsf:Observable
                             ];
        rdfs:subClassOf      [ rdf:type            owl:Restriction;
                               owl:onProperty      ocsf:enrichments;
                               owl:someValuesFrom  ocsf:Enrichment
                             ];
        rdfs:subClassOf      [ rdf:type            owl:Restriction;
                               owl:onProperty      ocsf:enrichments;
                               owl:someValuesFrom  ocsf:Enrichment
                             ];
        rdfs:subClassOf      [ rdf:type            owl:Restriction;
                               owl:onProperty      ocsf:enrichments;
                               owl:someValuesFrom  ocsf:Enrichment
                             ];
        rdfs:subClassOf      [ rdf:type         owl:Restriction;
                               owl:cardinality  1;
                               owl:onProperty   ocsf:metadata
                             ];
        rdfs:subClassOf      [ rdf:type         owl:Restriction;
                               owl:cardinality  1;
                               owl:onProperty   ocsf:metadata
                             ];
        rdfs:subClassOf      [ rdf:type            owl:Restriction;
                               owl:onProperty      ocsf:enrichments;
                               owl:someValuesFrom  ocsf:Enrichment
                             ];
        rdfs:subClassOf      [ rdf:type            owl:Restriction;
                               owl:onProperty      ocsf:enrichments;
                               owl:someValuesFrom  ocsf:Enrichment
                             ];
        rdfs:subClassOf      [ rdf:type            owl:Restriction;
                               owl:onProperty      ocsf:unmapped;
                               owl:someValuesFrom  ocsf:Object
                             ];
        rdfs:subClassOf      [ rdf:type            owl:Restriction;
                               owl:onProperty      ocsf:observables;
                               owl:someValuesFrom  ocsf:Observable
                             ];
        rdfs:subClassOf      [ rdf:type            owl:Restriction;
                               owl:onProperty      ocsf:enrichments;
                               owl:someValuesFrom  ocsf:Enrichment
                             ];
        rdfs:subClassOf      [ rdf:type         owl:Restriction;
                               owl:cardinality  1;
                               owl:onProperty   ocsf:metadata
                             ];
        rdfs:subClassOf      [ rdf:type            owl:Restriction;
                               owl:onProperty      ocsf:observables;
                               owl:someValuesFrom  ocsf:Observable
                             ];
        rdfs:subClassOf      [ rdf:type            owl:Restriction;
                               owl:onProperty      ocsf:enrichments;
                               owl:someValuesFrom  ocsf:Enrichment
                             ];
        rdfs:subClassOf      [ rdf:type            owl:Restriction;
                               owl:onProperty      ocsf:observables;
                               owl:someValuesFrom  ocsf:Observable
                             ];
        rdfs:subClassOf      [ rdf:type            owl:Restriction;
                               owl:onProperty      ocsf:unmapped;
                               owl:someValuesFrom  ocsf:Object
                             ];
        rdfs:subClassOf      [ rdf:type         owl:Restriction;
                               owl:cardinality  1;
                               owl:onProperty   ocsf:metadata
                             ];
        rdfs:subClassOf      [ rdf:type            owl:Restriction;
                               owl:onProperty      ocsf:observables;
                               owl:someValuesFrom  ocsf:Observable
                             ];
        rdfs:subClassOf      [ rdf:type            owl:Restriction;
                               owl:onProperty      ocsf:observables;
                               owl:someValuesFrom  ocsf:Observable
                             ];
        rdfs:subClassOf      [ rdf:type            owl:Restriction;
                               owl:onProperty      ocsf:enrichments;
                               owl:someValuesFrom  ocsf:Enrichment
                             ];
        rdfs:subClassOf      [ rdf:type            owl:Restriction;
                               owl:onProperty      ocsf:enrichments;
                               owl:someValuesFrom  ocsf:Enrichment
                             ];
        rdfs:subClassOf      [ rdf:type            owl:Restriction;
                               owl:onProperty      ocsf:unmapped;
                               owl:someValuesFrom  ocsf:Object
                             ];
        rdfs:subClassOf      [ rdf:type            owl:Restriction;
                               owl:onProperty      ocsf:unmapped;
                               owl:someValuesFrom  ocsf:Object
                             ];
        rdfs:subClassOf      [ rdf:type            owl:Restriction;
                               owl:onProperty      ocsf:unmapped;
                               owl:someValuesFrom  ocsf:Object
                             ];
        rdfs:subClassOf      [ rdf:type         owl:Restriction;
                               owl:cardinality  1;
                               owl:onProperty   ocsf:metadata
                             ];
        rdfs:subClassOf      [ rdf:type         owl:Restriction;
                               owl:cardinality  1;
                               owl:onProperty   ocsf:metadata
                             ];
        rdfs:subClassOf      [ rdf:type         owl:Restriction;
                               owl:cardinality  1;
                               owl:onProperty   ocsf:metadata
                             ];
        rdfs:subClassOf      [ rdf:type            owl:Restriction;
                               owl:onProperty      ocsf:unmapped;
                               owl:someValuesFrom  ocsf:Object
                             ];
        rdfs:subClassOf      [ rdf:type         owl:Restriction;
                               owl:cardinality  1;
                               owl:onProperty   ocsf:metadata
                             ];
        rdfs:subClassOf      [ rdf:type            owl:Restriction;
                               owl:onProperty      ocsf:observables;
                               owl:someValuesFrom  ocsf:Observable
                             ];
        rdfs:subClassOf      [ rdf:type            owl:Restriction;
                               owl:onProperty      ocsf:observables;
                               owl:someValuesFrom  ocsf:Observable
                             ];
        rdfs:subClassOf      [ rdf:type         owl:Restriction;
                               owl:cardinality  1;
                               owl:onProperty   ocsf:metadata
                             ];
        rdfs:subClassOf      [ rdf:type         owl:Restriction;
                               owl:cardinality  1;
                               owl:onProperty   ocsf:metadata
                             ];
        rdfs:subClassOf      [ rdf:type            owl:Restriction;
                               owl:onProperty      ocsf:observables;
                               owl:someValuesFrom  ocsf:Observable
                             ];
        rdfs:subClassOf      [ rdf:type            owl:Restriction;
                               owl:onProperty      ocsf:unmapped;
                               owl:someValuesFrom  ocsf:Object
                             ];
        rdfs:subClassOf      [ rdf:type         owl:Restriction;
                               owl:cardinality  1;
                               owl:onProperty   ocsf:metadata
                             ];
        rdfs:subClassOf      [ rdf:type            owl:Restriction;
                               owl:onProperty      ocsf:enrichments;
                               owl:someValuesFrom  ocsf:Enrichment
                             ];
        rdfs:subClassOf      [ rdf:type            owl:Restriction;
                               owl:onProperty      ocsf:observables;
                               owl:someValuesFrom  ocsf:Observable
                             ];
        rdfs:subClassOf      [ rdf:type         owl:Restriction;
                               owl:cardinality  1;
                               owl:onProperty   ocsf:metadata
                             ];
        rdfs:subClassOf      [ rdf:type            owl:Restriction;
                               owl:onProperty      ocsf:unmapped;
                               owl:someValuesFrom  ocsf:Object
                             ];
        rdfs:subClassOf      [ rdf:type            owl:Restriction;
                               owl:onProperty      ocsf:enrichments;
                               owl:someValuesFrom  ocsf:Enrichment
                             ];
        rdfs:subClassOf      [ rdf:type         owl:Restriction;
                               owl:cardinality  1;
                               owl:onProperty   ocsf:metadata
                             ];
        rdfs:subClassOf      [ rdf:type            owl:Restriction;
                               owl:onProperty      ocsf:unmapped;
                               owl:someValuesFrom  ocsf:Object
                             ];
        rdfs:subClassOf      [ rdf:type            owl:Restriction;
                               owl:onProperty      ocsf:observables;
                               owl:someValuesFrom  ocsf:Observable
                             ];
        rdfs:subClassOf      [ rdf:type            owl:Restriction;
                               owl:onProperty      ocsf:observables;
                               owl:someValuesFrom  ocsf:Observable
                             ];
        rdfs:subClassOf      [ rdf:type            owl:Restriction;
                               owl:onProperty      ocsf:observables;
                               owl:someValuesFrom  ocsf:Observable
                             ];
        rdfs:subClassOf      [ rdf:type            owl:Restriction;
                               owl:onProperty      ocsf:enrichments;
                               owl:someValuesFrom  ocsf:Enrichment
                             ];
        rdfs:subClassOf      [ rdf:type            owl:Restriction;
                               owl:onProperty      ocsf:observables;
                               owl:someValuesFrom  ocsf:Observable
                             ];
        rdfs:subClassOf      [ rdf:type            owl:Restriction;
                               owl:onProperty      ocsf:enrichments;
                               owl:someValuesFrom  ocsf:Enrichment
                             ];
        rdfs:subClassOf      [ rdf:type         owl:Restriction;
                               owl:cardinality  1;
                               owl:onProperty   ocsf:metadata
                             ];
        rdfs:subClassOf      [ rdf:type            owl:Restriction;
                               owl:onProperty      ocsf:enrichments;
                               owl:someValuesFrom  ocsf:Enrichment
                             ];
        rdfs:subClassOf      [ rdf:type         owl:Restriction;
                               owl:cardinality  1;
                               owl:onProperty   ocsf:metadata
                             ];
        rdfs:subClassOf      [ rdf:type            owl:Restriction;
                               owl:onProperty      ocsf:unmapped;
                               owl:someValuesFrom  ocsf:Object
                             ];
        rdfs:subClassOf      [ rdf:type         owl:Restriction;
                               owl:cardinality  1;
                               owl:onProperty   ocsf:metadata
                             ];
        rdfs:subClassOf      [ rdf:type            owl:Restriction;
                               owl:onProperty      ocsf:unmapped;
                               owl:someValuesFrom  ocsf:Object
                             ];
        rdfs:subClassOf      [ rdf:type            owl:Restriction;
                               owl:onProperty      ocsf:enrichments;
                               owl:someValuesFrom  ocsf:Enrichment
                             ];
        rdfs:subClassOf      [ rdf:type            owl:Restriction;
                               owl:onProperty      ocsf:observables;
                               owl:someValuesFrom  ocsf:Observable
                             ];
        rdfs:subClassOf      [ rdf:type            owl:Restriction;
                               owl:onProperty      ocsf:observables;
                               owl:someValuesFrom  ocsf:Observable
                             ];
        rdfs:subClassOf      [ rdf:type            owl:Restriction;
                               owl:onProperty      ocsf:observables;
                               owl:someValuesFrom  ocsf:Observable
                             ];
        rdfs:subClassOf      [ rdf:type            owl:Restriction;
                               owl:onProperty      ocsf:enrichments;
                               owl:someValuesFrom  ocsf:Enrichment
                             ];
        rdfs:subClassOf      [ rdf:type         owl:Restriction;
                               owl:cardinality  1;
                               owl:onProperty   ocsf:metadata
                             ];
        rdfs:subClassOf      [ rdf:type            owl:Restriction;
                               owl:onProperty      ocsf:unmapped;
                               owl:someValuesFrom  ocsf:Object
                             ];
        rdfs:subClassOf      [ rdf:type            owl:Restriction;
                               owl:onProperty      ocsf:enrichments;
                               owl:someValuesFrom  ocsf:Enrichment
                             ];
        rdfs:subClassOf      [ rdf:type            owl:Restriction;
                               owl:onProperty      ocsf:unmapped;
                               owl:someValuesFrom  ocsf:Object
                             ];
        rdfs:subClassOf      [ rdf:type            owl:Restriction;
                               owl:onProperty      ocsf:enrichments;
                               owl:someValuesFrom  ocsf:Enrichment
                             ];
        rdfs:subClassOf      [ rdf:type            owl:Restriction;
                               owl:onProperty      ocsf:unmapped;
                               owl:someValuesFrom  ocsf:Object
                             ];
        rdfs:subClassOf      [ rdf:type            owl:Restriction;
                               owl:onProperty      ocsf:enrichments;
                               owl:someValuesFrom  ocsf:Enrichment
                             ];
        rdfs:subClassOf      [ rdf:type            owl:Restriction;
                               owl:onProperty      ocsf:observables;
                               owl:someValuesFrom  ocsf:Observable
                             ];
        rdfs:subClassOf      [ rdf:type            owl:Restriction;
                               owl:onProperty      ocsf:unmapped;
                               owl:someValuesFrom  ocsf:Object
                             ];
        rdfs:subClassOf      [ rdf:type            owl:Restriction;
                               owl:onProperty      ocsf:observables;
                               owl:someValuesFrom  ocsf:Observable
                             ];
        rdfs:subClassOf      [ rdf:type            owl:Restriction;
                               owl:onProperty      ocsf:observables;
                               owl:someValuesFrom  ocsf:Observable
                             ];
        rdfs:subClassOf      [ rdf:type            owl:Restriction;
                               owl:onProperty      ocsf:unmapped;
                               owl:someValuesFrom  ocsf:Object
                             ];
        rdfs:subClassOf      [ rdf:type            owl:Restriction;
                               owl:onProperty      ocsf:observables;
                               owl:someValuesFrom  ocsf:Observable
                             ];
        rdfs:subClassOf      [ rdf:type            owl:Restriction;
                               owl:onProperty      ocsf:observables;
                               owl:someValuesFrom  ocsf:Observable
                             ];
        rdfs:subClassOf      [ rdf:type            owl:Restriction;
                               owl:onProperty      ocsf:unmapped;
                               owl:someValuesFrom  ocsf:Object
                             ];
        rdfs:subClassOf      [ rdf:type            owl:Restriction;
                               owl:onProperty      ocsf:unmapped;
                               owl:someValuesFrom  ocsf:Object
                             ];
        rdfs:subClassOf      [ rdf:type            owl:Restriction;
                               owl:onProperty      ocsf:unmapped;
                               owl:someValuesFrom  ocsf:Object
                             ];
        rdfs:subClassOf      [ rdf:type         owl:Restriction;
                               owl:cardinality  1;
                               owl:onProperty   ocsf:metadata
                             ];
        rdfs:subClassOf      [ rdf:type         owl:Restriction;
                               owl:cardinality  1;
                               owl:onProperty   ocsf:metadata
                             ];
        rdfs:subClassOf      [ rdf:type            owl:Restriction;
                               owl:onProperty      ocsf:unmapped;
                               owl:someValuesFrom  ocsf:Object
                             ];
        rdfs:subClassOf      [ rdf:type            owl:Restriction;
                               owl:onProperty      ocsf:unmapped;
                               owl:someValuesFrom  ocsf:Object
                             ];
        rdfs:subClassOf      [ rdf:type            owl:Restriction;
                               owl:onProperty      ocsf:observables;
                               owl:someValuesFrom  ocsf:Observable
                             ];
        rdfs:subClassOf      [ rdf:type            owl:Restriction;
                               owl:onProperty      ocsf:unmapped;
                               owl:someValuesFrom  ocsf:Object
                             ];
        rdfs:subClassOf      [ rdf:type            owl:Restriction;
                               owl:onProperty      ocsf:unmapped;
                               owl:someValuesFrom  ocsf:Object
                             ];
        rdfs:subClassOf      [ rdf:type            owl:Restriction;
                               owl:onProperty      ocsf:observables;
                               owl:someValuesFrom  ocsf:Observable
                             ];
        rdfs:subClassOf      [ rdf:type            owl:Restriction;
                               owl:onProperty      ocsf:unmapped;
                               owl:someValuesFrom  ocsf:Object
                             ];
        rdfs:subClassOf      [ rdf:type            owl:Restriction;
                               owl:onProperty      ocsf:observables;
                               owl:someValuesFrom  ocsf:Observable
                             ];
        rdfs:subClassOf      [ rdf:type            owl:Restriction;
                               owl:onProperty      ocsf:observables;
                               owl:someValuesFrom  ocsf:Observable
                             ];
        rdfs:subClassOf      [ rdf:type            owl:Restriction;
                               owl:onProperty      ocsf:enrichments;
                               owl:someValuesFrom  ocsf:Enrichment
                             ];
        rdfs:subClassOf      [ rdf:type            owl:Restriction;
                               owl:onProperty      ocsf:unmapped;
                               owl:someValuesFrom  ocsf:Object
                             ];
        rdfs:subClassOf      [ rdf:type            owl:Restriction;
                               owl:onProperty      ocsf:enrichments;
                               owl:someValuesFrom  ocsf:Enrichment
                             ];
        rdfs:subClassOf      [ rdf:type            owl:Restriction;
                               owl:onProperty      ocsf:observables;
                               owl:someValuesFrom  ocsf:Observable
                             ];
        rdfs:subClassOf      [ rdf:type            owl:Restriction;
                               owl:onProperty      ocsf:enrichments;
                               owl:someValuesFrom  ocsf:Enrichment
                             ];
        rdfs:subClassOf      [ rdf:type         owl:Restriction;
                               owl:cardinality  1;
                               owl:onProperty   ocsf:metadata
                             ];
        rdfs:subClassOf      [ rdf:type            owl:Restriction;
                               owl:onProperty      ocsf:enrichments;
                               owl:someValuesFrom  ocsf:Enrichment
                             ];
        rdfs:subClassOf      [ rdf:type            owl:Restriction;
                               owl:onProperty      ocsf:unmapped;
                               owl:someValuesFrom  ocsf:Object
                             ];
        rdfs:subClassOf      [ rdf:type            owl:Restriction;
                               owl:onProperty      ocsf:observables;
                               owl:someValuesFrom  ocsf:Observable
                             ];
        rdfs:subClassOf      [ rdf:type            owl:Restriction;
                               owl:onProperty      ocsf:observables;
                               owl:someValuesFrom  ocsf:Observable
                             ];
        rdfs:subClassOf      [ rdf:type            owl:Restriction;
                               owl:onProperty      ocsf:observables;
                               owl:someValuesFrom  ocsf:Observable
                             ];
        rdfs:subClassOf      [ rdf:type            owl:Restriction;
                               owl:onProperty      ocsf:enrichments;
                               owl:someValuesFrom  ocsf:Enrichment
                             ];
        rdfs:subClassOf      [ rdf:type            owl:Restriction;
                               owl:onProperty      ocsf:unmapped;
                               owl:someValuesFrom  ocsf:Object
                             ];
        rdfs:subClassOf      [ rdf:type            owl:Restriction;
                               owl:onProperty      ocsf:observables;
                               owl:someValuesFrom  ocsf:Observable
                             ];
        rdfs:subClassOf      [ rdf:type            owl:Restriction;
                               owl:onProperty      ocsf:unmapped;
                               owl:someValuesFrom  ocsf:Object
                             ];
        rdfs:subClassOf      [ rdf:type            owl:Restriction;
                               owl:onProperty      ocsf:unmapped;
                               owl:someValuesFrom  ocsf:Object
                             ];
        rdfs:subClassOf      [ rdf:type         owl:Restriction;
                               owl:cardinality  1;
                               owl:onProperty   ocsf:metadata
                             ];
        rdfs:subClassOf      [ rdf:type            owl:Restriction;
                               owl:onProperty      ocsf:unmapped;
                               owl:someValuesFrom  ocsf:Object
                             ];
        rdfs:subClassOf      [ rdf:type         owl:Restriction;
                               owl:cardinality  1;
                               owl:onProperty   ocsf:metadata
                             ];
        rdfs:subClassOf      [ rdf:type            owl:Restriction;
                               owl:onProperty      ocsf:enrichments;
                               owl:someValuesFrom  ocsf:Enrichment
                             ];
        rdfs:subClassOf      [ rdf:type            owl:Restriction;
                               owl:onProperty      ocsf:observables;
                               owl:someValuesFrom  ocsf:Observable
                             ];
        rdfs:subClassOf      [ rdf:type            owl:Restriction;
                               owl:onProperty      ocsf:observables;
                               owl:someValuesFrom  ocsf:Observable
                             ];
        rdfs:subClassOf      [ rdf:type            owl:Restriction;
                               owl:onProperty      ocsf:enrichments;
                               owl:someValuesFrom  ocsf:Enrichment
                             ];
        rdfs:subClassOf      [ rdf:type         owl:Restriction;
                               owl:cardinality  1;
                               owl:onProperty   ocsf:metadata
                             ];
        rdfs:subClassOf      [ rdf:type            owl:Restriction;
                               owl:onProperty      ocsf:unmapped;
                               owl:someValuesFrom  ocsf:Object
                             ];
        rdfs:subClassOf      [ rdf:type         owl:Restriction;
                               owl:cardinality  1;
                               owl:onProperty   ocsf:metadata
                             ];
        rdfs:subClassOf      [ rdf:type         owl:Restriction;
                               owl:cardinality  1;
                               owl:onProperty   ocsf:metadata
                             ];
        rdfs:subClassOf      [ rdf:type            owl:Restriction;
                               owl:onProperty      ocsf:observables;
                               owl:someValuesFrom  ocsf:Observable
                             ];
        rdfs:subClassOf      [ rdf:type            owl:Restriction;
                               owl:onProperty      ocsf:enrichments;
                               owl:someValuesFrom  ocsf:Enrichment
                             ];
        rdfs:subClassOf      [ rdf:type         owl:Restriction;
                               owl:cardinality  1;
                               owl:onProperty   ocsf:metadata
                             ];
        rdfs:subClassOf      [ rdf:type         owl:Restriction;
                               owl:cardinality  1;
                               owl:onProperty   ocsf:metadata
                             ];
        rdfs:subClassOf      [ rdf:type            owl:Restriction;
                               owl:onProperty      ocsf:unmapped;
                               owl:someValuesFrom  ocsf:Object
                             ];
        rdfs:subClassOf      [ rdf:type            owl:Restriction;
                               owl:onProperty      ocsf:enrichments;
                               owl:someValuesFrom  ocsf:Enrichment
                             ];
        rdfs:subClassOf      [ rdf:type            owl:Restriction;
                               owl:onProperty      ocsf:observables;
                               owl:someValuesFrom  ocsf:Observable
                             ];
        rdfs:subClassOf      [ rdf:type            owl:Restriction;
                               owl:onProperty      ocsf:observables;
                               owl:someValuesFrom  ocsf:Observable
                             ];
        rdfs:subClassOf      [ rdf:type            owl:Restriction;
                               owl:onProperty      ocsf:enrichments;
                               owl:someValuesFrom  ocsf:Enrichment
                             ];
        rdfs:subClassOf      [ rdf:type         owl:Restriction;
                               owl:cardinality  1;
                               owl:onProperty   ocsf:metadata
                             ];
        rdfs:subClassOf      [ rdf:type            owl:Restriction;
                               owl:onProperty      ocsf:unmapped;
                               owl:someValuesFrom  ocsf:Object
                             ];
        rdfs:subClassOf      [ rdf:type            owl:Restriction;
                               owl:onProperty      ocsf:enrichments;
                               owl:someValuesFrom  ocsf:Enrichment
                             ];
        rdfs:subClassOf      [ rdf:type            owl:Restriction;
                               owl:onProperty      ocsf:unmapped;
                               owl:someValuesFrom  ocsf:Object
                             ];
        rdfs:subClassOf      [ rdf:type         owl:Restriction;
                               owl:cardinality  1;
                               owl:onProperty   ocsf:metadata
                             ];
        rdfs:subClassOf      [ rdf:type            owl:Restriction;
                               owl:onProperty      ocsf:enrichments;
                               owl:someValuesFrom  ocsf:Enrichment
                             ];
        rdfs:subClassOf      [ rdf:type            owl:Restriction;
                               owl:onProperty      ocsf:enrichments;
                               owl:someValuesFrom  ocsf:Enrichment
                             ];
        rdfs:subClassOf      [ rdf:type         owl:Restriction;
                               owl:cardinality  1;
                               owl:onProperty   ocsf:metadata
                             ];
        rdfs:subClassOf      [ rdf:type            owl:Restriction;
                               owl:onProperty      ocsf:unmapped;
                               owl:someValuesFrom  ocsf:Object
                             ];
        rdfs:subClassOf      [ rdf:type            owl:Restriction;
                               owl:onProperty      ocsf:observables;
                               owl:someValuesFrom  ocsf:Observable
                             ];
        rdfs:subClassOf      [ rdf:type            owl:Restriction;
                               owl:onProperty      ocsf:enrichments;
                               owl:someValuesFrom  ocsf:Enrichment
                             ];
        rdfs:subClassOf      [ rdf:type         owl:Restriction;
                               owl:cardinality  1;
                               owl:onProperty   ocsf:metadata
                             ];
        rdfs:subClassOf      [ rdf:type         owl:Restriction;
                               owl:cardinality  1;
                               owl:onProperty   ocsf:metadata
                             ];
        rdfs:subClassOf      [ rdf:type            owl:Restriction;
                               owl:onProperty      ocsf:enrichments;
                               owl:someValuesFrom  ocsf:Enrichment
                             ];
        rdfs:subClassOf      [ rdf:type            owl:Restriction;
                               owl:onProperty      ocsf:enrichments;
                               owl:someValuesFrom  ocsf:Enrichment
                             ];
        rdfs:subClassOf      [ rdf:type         owl:Restriction;
                               owl:cardinality  1;
                               owl:onProperty   ocsf:metadata
                             ];
        rdfs:subClassOf      [ rdf:type            owl:Restriction;
                               owl:onProperty      ocsf:observables;
                               owl:someValuesFrom  ocsf:Observable
                             ];
        rdfs:subClassOf      [ rdf:type            owl:Restriction;
                               owl:onProperty      ocsf:observables;
                               owl:someValuesFrom  ocsf:Observable
                             ];
        rdfs:subClassOf      [ rdf:type            owl:Restriction;
                               owl:onProperty      ocsf:observables;
                               owl:someValuesFrom  ocsf:Observable
                             ];
        rdfs:subClassOf      [ rdf:type            owl:Restriction;
                               owl:onProperty      ocsf:observables;
                               owl:someValuesFrom  ocsf:Observable
                             ];
        rdfs:subClassOf      [ rdf:type            owl:Restriction;
                               owl:onProperty      ocsf:unmapped;
                               owl:someValuesFrom  ocsf:Object
                             ];
        rdfs:subClassOf      [ rdf:type            owl:Restriction;
                               owl:onProperty      ocsf:observables;
                               owl:someValuesFrom  ocsf:Observable
                             ];
        rdfs:subClassOf      [ rdf:type            owl:Restriction;
                               owl:onProperty      ocsf:enrichments;
                               owl:someValuesFrom  ocsf:Enrichment
                             ];
        rdfs:subClassOf      [ rdf:type            owl:Restriction;
                               owl:onProperty      ocsf:observables;
                               owl:someValuesFrom  ocsf:Observable
                             ];
        rdfs:subClassOf      [ rdf:type            owl:Restriction;
                               owl:onProperty      ocsf:enrichments;
                               owl:someValuesFrom  ocsf:Enrichment
                             ];
        rdfs:subClassOf      [ rdf:type            owl:Restriction;
                               owl:onProperty      ocsf:enrichments;
                               owl:someValuesFrom  ocsf:Enrichment
                             ];
        rdfs:subClassOf      [ rdf:type            owl:Restriction;
                               owl:onProperty      ocsf:observables;
                               owl:someValuesFrom  ocsf:Observable
                             ];
        rdfs:subClassOf      [ rdf:type         owl:Restriction;
                               owl:cardinality  1;
                               owl:onProperty   ocsf:metadata
                             ];
        rdfs:subClassOf      [ rdf:type         owl:Restriction;
                               owl:cardinality  1;
                               owl:onProperty   ocsf:metadata
                             ];
        rdfs:subClassOf      [ rdf:type            owl:Restriction;
                               owl:onProperty      ocsf:observables;
                               owl:someValuesFrom  ocsf:Observable
                             ];
        rdfs:subClassOf      [ rdf:type            owl:Restriction;
                               owl:onProperty      ocsf:enrichments;
                               owl:someValuesFrom  ocsf:Enrichment
                             ];
        rdfs:subClassOf      [ rdf:type            owl:Restriction;
                               owl:onProperty      ocsf:enrichments;
                               owl:someValuesFrom  ocsf:Enrichment
                             ];
        rdfs:subClassOf      [ rdf:type            owl:Restriction;
                               owl:onProperty      ocsf:observables;
                               owl:someValuesFrom  ocsf:Observable
                             ];
        rdfs:subClassOf      [ rdf:type         owl:Restriction;
                               owl:cardinality  1;
                               owl:onProperty   ocsf:metadata
                             ];
        rdfs:subClassOf      [ rdf:type            owl:Restriction;
                               owl:onProperty      ocsf:enrichments;
                               owl:someValuesFrom  ocsf:Enrichment
                             ];
        rdfs:subClassOf      [ rdf:type         owl:Restriction;
                               owl:cardinality  1;
                               owl:onProperty   ocsf:metadata
                             ];
        rdfs:subClassOf      [ rdf:type            owl:Restriction;
                               owl:onProperty      ocsf:enrichments;
                               owl:someValuesFrom  ocsf:Enrichment
                             ];
        rdfs:subClassOf      [ rdf:type            owl:Restriction;
                               owl:onProperty      ocsf:unmapped;
                               owl:someValuesFrom  ocsf:Object
                             ];
        rdfs:subClassOf      [ rdf:type            owl:Restriction;
                               owl:onProperty      ocsf:observables;
                               owl:someValuesFrom  ocsf:Observable
                             ];
        rdfs:subClassOf      [ rdf:type            owl:Restriction;
                               owl:onProperty      ocsf:enrichments;
                               owl:someValuesFrom  ocsf:Enrichment
                             ];
        rdfs:subClassOf      [ rdf:type            owl:Restriction;
                               owl:onProperty      ocsf:unmapped;
                               owl:someValuesFrom  ocsf:Object
                             ];
        rdfs:subClassOf      [ rdf:type            owl:Restriction;
                               owl:onProperty      ocsf:unmapped;
                               owl:someValuesFrom  ocsf:Object
                             ];
        rdfs:subClassOf      [ rdf:type            owl:Restriction;
                               owl:onProperty      ocsf:unmapped;
                               owl:someValuesFrom  ocsf:Object
                             ];
        rdfs:subClassOf      [ rdf:type            owl:Restriction;
                               owl:onProperty      ocsf:enrichments;
                               owl:someValuesFrom  ocsf:Enrichment
                             ];
        rdfs:subClassOf      [ rdf:type            owl:Restriction;
                               owl:onProperty      ocsf:unmapped;
                               owl:someValuesFrom  ocsf:Object
                             ];
        rdfs:subClassOf      [ rdf:type         owl:Restriction;
                               owl:cardinality  1;
                               owl:onProperty   ocsf:metadata
                             ];
        rdfs:subClassOf      [ rdf:type            owl:Restriction;
                               owl:onProperty      ocsf:unmapped;
                               owl:someValuesFrom  ocsf:Object
                             ];
        rdfs:subClassOf      [ rdf:type            owl:Restriction;
                               owl:onProperty      ocsf:enrichments;
                               owl:someValuesFrom  ocsf:Enrichment
                             ];
        rdfs:subClassOf      [ rdf:type            owl:Restriction;
                               owl:onProperty      ocsf:enrichments;
                               owl:someValuesFrom  ocsf:Enrichment
                             ];
        rdfs:subClassOf      [ rdf:type            owl:Restriction;
                               owl:onProperty      ocsf:observables;
                               owl:someValuesFrom  ocsf:Observable
                             ];
        rdfs:subClassOf      [ rdf:type            owl:Restriction;
                               owl:onProperty      ocsf:unmapped;
                               owl:someValuesFrom  ocsf:Object
                             ];
        rdfs:subClassOf      [ rdf:type            owl:Restriction;
                               owl:onProperty      ocsf:enrichments;
                               owl:someValuesFrom  ocsf:Enrichment
                             ];
        rdfs:subClassOf      [ rdf:type            owl:Restriction;
                               owl:onProperty      ocsf:enrichments;
                               owl:someValuesFrom  ocsf:Enrichment
                             ];
        rdfs:subClassOf      [ rdf:type         owl:Restriction;
                               owl:cardinality  1;
                               owl:onProperty   ocsf:metadata
                             ];
        rdfs:subClassOf      [ rdf:type            owl:Restriction;
                               owl:onProperty      ocsf:enrichments;
                               owl:someValuesFrom  ocsf:Enrichment
                             ];
        rdfs:subClassOf      [ rdf:type            owl:Restriction;
                               owl:onProperty      ocsf:enrichments;
                               owl:someValuesFrom  ocsf:Enrichment
                             ];
        rdfs:subClassOf      [ rdf:type            owl:Restriction;
                               owl:onProperty      ocsf:enrichments;
                               owl:someValuesFrom  ocsf:Enrichment
                             ];
        rdfs:subClassOf      [ rdf:type            owl:Restriction;
                               owl:onProperty      ocsf:unmapped;
                               owl:someValuesFrom  ocsf:Object
                             ];
        rdfs:subClassOf      [ rdf:type         owl:Restriction;
                               owl:cardinality  1;
                               owl:onProperty   ocsf:metadata
                             ];
        rdfs:subClassOf      [ rdf:type         owl:Restriction;
                               owl:cardinality  1;
                               owl:onProperty   ocsf:metadata
                             ];
        rdfs:subClassOf      [ rdf:type            owl:Restriction;
                               owl:onProperty      ocsf:unmapped;
                               owl:someValuesFrom  ocsf:Object
                             ];
        rdfs:subClassOf      [ rdf:type            owl:Restriction;
                               owl:onProperty      ocsf:unmapped;
                               owl:someValuesFrom  ocsf:Object
                             ];
        rdfs:subClassOf      [ rdf:type         owl:Restriction;
                               owl:cardinality  1;
                               owl:onProperty   ocsf:metadata
                             ];
        rdfs:subClassOf      [ rdf:type            owl:Restriction;
                               owl:onProperty      ocsf:unmapped;
                               owl:someValuesFrom  ocsf:Object
                             ];
        rdfs:subClassOf      [ rdf:type            owl:Restriction;
                               owl:onProperty      ocsf:unmapped;
                               owl:someValuesFrom  ocsf:Object
                             ];
        rdfs:subClassOf      [ rdf:type            owl:Restriction;
                               owl:onProperty      ocsf:enrichments;
                               owl:someValuesFrom  ocsf:Enrichment
                             ];
        rdfs:subClassOf      [ rdf:type            owl:Restriction;
                               owl:onProperty      ocsf:enrichments;
                               owl:someValuesFrom  ocsf:Enrichment
                             ];
        rdfs:subClassOf      [ rdf:type            owl:Restriction;
                               owl:onProperty      ocsf:observables;
                               owl:someValuesFrom  ocsf:Observable
                             ];
        rdfs:subClassOf      [ rdf:type            owl:Restriction;
                               owl:onProperty      ocsf:enrichments;
                               owl:someValuesFrom  ocsf:Enrichment
                             ];
        rdfs:subClassOf      [ rdf:type            owl:Restriction;
                               owl:onProperty      ocsf:observables;
                               owl:someValuesFrom  ocsf:Observable
                             ];
        rdfs:subClassOf      [ rdf:type            owl:Restriction;
                               owl:onProperty      ocsf:observables;
                               owl:someValuesFrom  ocsf:Observable
                             ];
        rdfs:subClassOf      [ rdf:type            owl:Restriction;
                               owl:onProperty      ocsf:observables;
                               owl:someValuesFrom  ocsf:Observable
                             ];
        rdfs:subClassOf      [ rdf:type            owl:Restriction;
                               owl:onProperty      ocsf:unmapped;
                               owl:someValuesFrom  ocsf:Object
                             ];
        rdfs:subClassOf      [ rdf:type            owl:Restriction;
                               owl:onProperty      ocsf:observables;
                               owl:someValuesFrom  ocsf:Observable
                             ];
        rdfs:subClassOf      [ rdf:type            owl:Restriction;
                               owl:onProperty      ocsf:enrichments;
                               owl:someValuesFrom  ocsf:Enrichment
                             ];
        rdfs:subClassOf      [ rdf:type            owl:Restriction;
                               owl:onProperty      ocsf:observables;
                               owl:someValuesFrom  ocsf:Observable
                             ];
        rdfs:subClassOf      [ rdf:type            owl:Restriction;
                               owl:onProperty      ocsf:unmapped;
                               owl:someValuesFrom  ocsf:Object
                             ];
        rdfs:subClassOf      [ rdf:type            owl:Restriction;
                               owl:onProperty      ocsf:unmapped;
                               owl:someValuesFrom  ocsf:Object
                             ];
        rdfs:subClassOf      [ rdf:type            owl:Restriction;
                               owl:onProperty      ocsf:enrichments;
                               owl:someValuesFrom  ocsf:Enrichment
                             ];
        rdfs:subClassOf      [ rdf:type            owl:Restriction;
                               owl:onProperty      ocsf:observables;
                               owl:someValuesFrom  ocsf:Observable
                             ];
        rdfs:subClassOf      [ rdf:type         owl:Restriction;
                               owl:cardinality  1;
                               owl:onProperty   ocsf:metadata
                             ];
        rdfs:subClassOf      [ rdf:type            owl:Restriction;
                               owl:onProperty      ocsf:observables;
                               owl:someValuesFrom  ocsf:Observable
                             ];
        rdfs:subClassOf      [ rdf:type            owl:Restriction;
                               owl:onProperty      ocsf:enrichments;
                               owl:someValuesFrom  ocsf:Enrichment
                             ];
        rdfs:subClassOf      [ rdf:type            owl:Restriction;
                               owl:onProperty      ocsf:observables;
                               owl:someValuesFrom  ocsf:Observable
                             ];
        rdfs:subClassOf      [ rdf:type            owl:Restriction;
                               owl:onProperty      ocsf:unmapped;
                               owl:someValuesFrom  ocsf:Object
                             ];
        rdfs:subClassOf      [ rdf:type            owl:Restriction;
                               owl:onProperty      ocsf:observables;
                               owl:someValuesFrom  ocsf:Observable
                             ];
        rdfs:subClassOf      [ rdf:type            owl:Restriction;
                               owl:onProperty      ocsf:observables;
                               owl:someValuesFrom  ocsf:Observable
                             ];
        rdfs:subClassOf      [ rdf:type            owl:Restriction;
                               owl:onProperty      ocsf:enrichments;
                               owl:someValuesFrom  ocsf:Enrichment
                             ];
        rdfs:subClassOf      [ rdf:type         owl:Restriction;
                               owl:cardinality  1;
                               owl:onProperty   ocsf:metadata
                             ];
        rdfs:subClassOf      [ rdf:type            owl:Restriction;
                               owl:onProperty      ocsf:enrichments;
                               owl:someValuesFrom  ocsf:Enrichment
                             ];
        rdfs:subClassOf      [ rdf:type            owl:Restriction;
                               owl:onProperty      ocsf:observables;
                               owl:someValuesFrom  ocsf:Observable
                             ];
        rdfs:subClassOf      [ rdf:type         owl:Restriction;
                               owl:cardinality  1;
                               owl:onProperty   ocsf:metadata
                             ];
        rdfs:subClassOf      [ rdf:type            owl:Restriction;
                               owl:onProperty      ocsf:unmapped;
                               owl:someValuesFrom  ocsf:Object
                             ];
        dcterms:description  "The base event is a generic and concrete event. It also defines a set of attributes available in most event classes. As a generic event that does not belong to any event category, it could be used to log events that are not otherwise defined by the schema.";
        ocsf:category        "other";
        ocsf:name            "base_event";
        ocsf:profiles        "[\"cloud\",\"datetime\"]" .

ocsf:Resource  rdf:type      owl:Class;
        rdfs:label           "Resource";
        rdfs:subClassOf      ocsf:Entity;
        dcterms:description  "The Resource object contains attributes that provide information about a particular resource. It serves as a base object, offering attributes that help identify and classify the resource effectively.";
        ocsf:name            "_resource" .

ocsf:transmit_time  rdf:type  owl:DatatypeProperty;
        rdfs:label           "Transmission Time";
        rdfs:range           ocsf:timestamp_t;
        dcterms:description  "The event transmission time from one device to another.  See specific usage" .

ocsf:OperatingSystemOS
        rdf:type             owl:Class;
        rdfs:label           "Operating System (OS)";
        rdfs:subClassOf      ocsf:Object;
        dcterms:description  "The Operating System (OS) object describes characteristics of an OS, such as Linux or Windows. Defined by D3FEND <a target='_blank' href='https://d3fend.mitre.org/dao/artifact/d3f:OperatingSystem/'>d3f:OperatingSystem</a>.";
        ocsf:name            "os" .

ocsf:NetworkTraffic  rdf:type  owl:Class;
        rdfs:label           "Network Traffic";
        rdfs:subClassOf      ocsf:Object;
        dcterms:description  "The Network Traffic object describes characteristics of network traffic. Network traffic refers to data moving across a network at a given point of time. Defined by D3FEND <a target='_blank' href='https://d3fend.mitre.org/dao/artifact/d3f:NetworkTraffic/'>d3f:NetworkTraffic</a>.";
        ocsf:name            "network_traffic" .

ocsf:datetime_t  rdf:type    rdfs:Datatype;
        rdfs:label           "Datetime";
        rdfs:subClassOf      xsd:string;
        dcterms:description  "The Internet Date/Time format as defined in <a target='_blank' href='https://www.rfc-editor.org/rfc/rfc3339.html'>RFC-3339</a>. For example <code>1985-04-12T23:20:50.52Z</code>.";
        xsd:pattern          "^\\d{4}-\\d{2}-\\d{2}T\\d{2}:\\d{2}:\\d{2}(?:\\.\\d+)?(Z|[\\+-]\\d{2}:\\d{2})?$" .

ocsf:evidences  rdf:type     owl:ObjectProperty;
        rdfs:label           "Evidence Artifacts";
        rdfs:range           ocsf:EvidenceArtifacts;
        dcterms:description  "Describes various evidence artifacts associated to the activity/activities that triggered a security detection." .

ocsf:is_compliant  rdf:type  owl:DatatypeProperty;
        rdfs:label           "Compliant Device";
        rdfs:range           ocsf:boolean_t;
        dcterms:description  "The event occurred on a compliant device." .

ocsf:base_address  rdf:type  owl:DatatypeProperty;
        rdfs:label           "Base Address";
        rdfs:range           ocsf:string_t;
        dcterms:description  "The memory address where the module was loaded." .

ocsf:city  rdf:type          owl:DatatypeProperty;
        rdfs:label           "City";
        rdfs:range           ocsf:string_t;
        dcterms:description  "The name of the city." .

ocsf:RequestElements  rdf:type  owl:Class;
        rdfs:label           "Request Elements";
        rdfs:subClassOf      ocsf:Object;
        rdfs:subClassOf      [ rdf:type            owl:Restriction;
                               owl:onProperty      ocsf:containers;
                               owl:someValuesFrom  ocsf:Container
                             ];
        dcterms:description  "The Request Elements object describes characteristics of an API request.";
        ocsf:name            "request" .

ocsf:attributes  rdf:type    owl:DatatypeProperty;
        rdfs:label           "Attributes";
        rdfs:range           ocsf:integer_t;
        dcterms:description  "The bitmask value that represents the file attributes." .

ocsf:query_string  rdf:type  owl:DatatypeProperty;
        rdfs:label           "HTTP Query String";
        rdfs:range           ocsf:string_t;
        dcterms:description  "The query portion of the URL. For example: the query portion of the URL <code>http://www.example.com/search?q=bad&sort=date</code> is <code>q=bad&sort=date</code>." .

ocsf:job_title  rdf:type     owl:DatatypeProperty;
        rdfs:label           "Job Title";
        rdfs:range           ocsf:string_t;
        dcterms:description  "The user's job title." .

ocsf:state_id  rdf:type      owl:DatatypeProperty;
        rdfs:label           "State ID";
        rdfs:range           ocsf:integer_t;
        dcterms:description  "The normalized state ID of the event or object. See specific usage.";
        jsonschema:enum      "Unknown" , "Other" .

ocsf:confidence  rdf:type    owl:DatatypeProperty;
        rdfs:label           "Confidence";
        rdfs:range           ocsf:string_t;
        dcterms:description  "The confidence, normalized to the caption of the confidence_id value. In the case of 'Other', it is defined by the event source." .

ocsf:org  rdf:type           owl:ObjectProperty;
        rdfs:label           "Organization";
        rdfs:range           ocsf:Organization;
        dcterms:description  "Organization and org unit relevant to the event or object." .

ocsf:class  rdf:type         owl:DatatypeProperty;
        rdfs:label           "Class";
        rdfs:range           ocsf:string_t;
        dcterms:description  "The class name of the object. See specific usage." .

ocsf:UniformResourceLocator
        rdf:type             owl:Class;
        rdfs:label           "Uniform Resource Locator";
        rdfs:subClassOf      ocsf:Object;
        dcterms:description  "The Uniform Resource Locator(URL) object describes the characteristics of a URL. Defined in <a target='_blank' href='https://datatracker.ietf.org/doc/html/rfc1738'>RFC 1738</a> and by D3FEND <a target='_blank' href='https://d3fend.mitre.org/dao/artifact/d3f:URL/'>d3f:URL</a>.";
        ocsf:constraints     "{\"at_least_one\":[\"url_string\",\"path\"]}";
        ocsf:name            "url";
        ocsf:observable      23 .

ocsf:Organization  rdf:type  owl:Class;
        rdfs:label           "Organization";
        rdfs:subClassOf      ocsf:Entity;
        dcterms:description  "The Organization object describes characteristics of an orgnization or company and its division if any.";
        ocsf:name            "organization" .

ocsf:command  rdf:type       owl:DatatypeProperty;
        rdfs:label           "Command";
        rdfs:range           ocsf:string_t;
        dcterms:description  "The command name." .

ocsf:purl  rdf:type          owl:DatatypeProperty;
        rdfs:label           "Package URL";
        rdfs:range           ocsf:string_t;
        dcterms:description  "A purl is a URL string used to identify and locate a software package in a mostly universal and uniform way across programing languages, package managers, packaging conventions, tools, APIs and databases." .

ocsf:request  rdf:type       owl:ObjectProperty;
        rdfs:label           "API Request Details";
        rdfs:range           ocsf:RequestElements;
        dcterms:description  "General Purpose API Request Object. See specific usage" .

ocsf:CWE  rdf:type           owl:Class;
        rdfs:label           "CWE";
        rdfs:subClassOf      ocsf:Object;
        dcterms:description  "The CWE object represents a weakness in a software system that can be exploited by a threat actor to perform an attack. The CWE object is based on the <a target='_blank' href='https://cwe.mitre.org/'>Common Weakness Enumeration (CWE)</a> catalog.";
        ocsf:name            "cwe" .

ocsf:CISControl  rdf:type    owl:Class;
        rdfs:label           "CIS Control";
        rdfs:subClassOf      ocsf:Object;
        dcterms:description  "The CIS Control (aka Critical Security Control) object describes a prioritized set of actions to protect your organization and data from cyber-attack vectors. The <a target='_blank' href='https://www.cisecurity.org/controls'>CIS Controls</a> are defined by the Center for Internet Security.";
        ocsf:name            "cis_control" .

ocsf:auth_protocol  rdf:type  owl:DatatypeProperty;
        rdfs:label           "Auth Protocol";
        rdfs:range           ocsf:string_t;
        dcterms:description  "The authentication protocol as defined by the caption of 'auth_protocol_id'. In the case of 'Other', it is defined by the event source." .

ocsf:spf  rdf:type           owl:DatatypeProperty;
        rdfs:label           "SPF Status";
        rdfs:range           ocsf:string_t;
        dcterms:description  "The Sender Policy Framework (SPF) status of the email." .

ocsf:event_code  rdf:type    owl:DatatypeProperty;
        rdfs:label           "Event Code";
        rdfs:range           ocsf:string_t;
        dcterms:description  "The Event ID or Code that the product uses to describe the event." .

ocsf:NetworkFileActivityEvent
        rdf:type             owl:Class;
        rdfs:label           "Network File Activity";
        rdfs:subClassOf      d3f:DigitalEvent;
        rdfs:subClassOf      [ rdf:type         owl:Restriction;
                               owl:cardinality  1;
                               owl:onProperty   ocsf:src_endpoint
                             ];
        rdfs:subClassOf      [ rdf:type         owl:Restriction;
                               owl:cardinality  1;
                               owl:onProperty   ocsf:file
                             ];
        rdfs:subClassOf      [ rdf:type         owl:Restriction;
                               owl:cardinality  1;
                               owl:onProperty   ocsf:actor
                             ];
        rdfs:subClassOf      [ rdf:type            owl:Restriction;
                               owl:onProperty      ocsf:dst_endpoint;
                               owl:someValuesFrom  ocsf:NetworkEndpoint
                             ];
        rdfs:subClassOf      [ rdf:type            owl:Restriction;
                               owl:onProperty      ocsf:connection_info;
                               owl:someValuesFrom  ocsf:NetworkConnectionInformation
                             ];
        dcterms:description  "Network File Activity events report file activities traversing the network, including file storage services such as Box, MS OneDrive, or Google Drive.";
        ocsf:category        "network";
        ocsf:name            "network_file_activity";
        ocsf:uid             10 .

ocsf:SecurityFindingEvent
        rdf:type             owl:Class;
        rdfs:label           "Security Finding";
        rdfs:subClassOf      d3f:DigitalEvent;
        rdfs:subClassOf      [ rdf:type            owl:Restriction;
                               owl:onProperty      ocsf:malware;
                               owl:someValuesFrom  ocsf:Malware
                             ];
        rdfs:subClassOf      [ rdf:type            owl:Restriction;
                               owl:onProperty      ocsf:cis_csc;
                               owl:someValuesFrom  ocsf:CISCSC
                             ];
        rdfs:subClassOf      [ rdf:type            owl:Restriction;
                               owl:onProperty      ocsf:resources;
                               owl:someValuesFrom  ocsf:ResourceDetails
                             ];
        rdfs:subClassOf      [ rdf:type         owl:Restriction;
                               owl:cardinality  1;
                               owl:onProperty   ocsf:finding
                             ];
        rdfs:subClassOf      [ rdf:type            owl:Restriction;
                               owl:onProperty      ocsf:kill_chain;
                               owl:someValuesFrom  ocsf:KillChainPhase
                             ];
        rdfs:subClassOf      [ rdf:type            owl:Restriction;
                               owl:onProperty      ocsf:process;
                               owl:someValuesFrom  ocsf:Process
                             ];
        rdfs:subClassOf      [ rdf:type            owl:Restriction;
                               owl:onProperty      ocsf:analytic;
                               owl:someValuesFrom  ocsf:Analytic
                             ];
        rdfs:subClassOf      [ rdf:type            owl:Restriction;
                               owl:onProperty      ocsf:compliance;
                               owl:someValuesFrom  ocsf:Compliance
                             ];
        rdfs:subClassOf      [ rdf:type            owl:Restriction;
                               owl:onProperty      ocsf:attacks;
                               owl:someValuesFrom  ocsf:MITREATTCK
                             ];
        rdfs:subClassOf      [ rdf:type            owl:Restriction;
                               owl:onProperty      ocsf:vulnerabilities;
                               owl:someValuesFrom  ocsf:VulnerabilityDetails
                             ];
        dcterms:description  "Security Finding events describe findings, detections, anomalies, alerts and/or actions performed by security products";
        ocsf:category        "findings";
        ocsf:name            "security_finding";
        ocsf:uid             1 .

ocsf:manager  rdf:type       owl:ObjectProperty;
        rdfs:label           "Manager";
        rdfs:range           ocsf:User;
        dcterms:description  "The user's manager. This helps in understanding an org hierarchy. This should only ever be populated once in an event. I.e. there should not be a manager's manager in an event." .

ocsf:exit_code  rdf:type     owl:DatatypeProperty;
        rdfs:label           "Exit Code";
        rdfs:range           ocsf:integer_t;
        dcterms:description  "The exit code reported by a process when it terminates. The convention is that zero indicates success and any non-zero exit code indicates that some error occurred." .

ocsf:action_id  rdf:type     owl:DatatypeProperty;
        rdfs:label           "Action ID";
        rdfs:range           ocsf:integer_t;
        dcterms:description  "The normalized action taken by a control or other policy-based system leading to an outcome or disposition.";
        jsonschema:enum      "Denied" , "Allowed" , "Unknown" , "Other" .

ocsf:ack_reason  rdf:type    owl:DatatypeProperty;
        rdfs:label           "Acknowledgement Reason";
        rdfs:range           ocsf:integer_t;
        dcterms:description  "An integer that provides a reason code or additional information about the acknowledgment result." .

ocsf:activity_name  rdf:type  owl:DatatypeProperty;
        rdfs:label           "Activity";
        rdfs:range           ocsf:string_t;
        dcterms:description  "The event activity name, as defined by the activity_id." .

ocsf:finding  rdf:type       owl:ObjectProperty;
        rdfs:label           "Finding";
        rdfs:range           ocsf:Finding;
        dcterms:description  "The Finding object provides details about a finding/detection generated by a security tool." .

ocsf:http_status  rdf:type   owl:DatatypeProperty;
        rdfs:label           "HTTP Status";
        rdfs:range           ocsf:integer_t;
        dcterms:description  "The Hypertext Transfer Protocol (HTTP) <a target='_blank' href='https://www.iana.org/assignments/http-status-codes/http-status-codes.xhtml'>status code</a> returned to the client." .

ocsf:delay  rdf:type         owl:DatatypeProperty;
        rdfs:label           "Root Delay";
        rdfs:range           ocsf:integer_t;
        dcterms:description  "The total round-trip delay to the reference clock in milliseconds." .

ocsf:ou_uid  rdf:type        owl:DatatypeProperty;
        rdfs:label           "Org Unit ID";
        rdfs:range           ocsf:string_t;
        dcterms:description  "The alternate identifier for an entity's unique identifier. For example, its Active Directory OU DN or AWS OU ID." .

ocsf:profiles  rdf:type      owl:DatatypeProperty;
        rdfs:label           "Profiles";
        rdfs:range           ocsf:string_t;
        dcterms:description  "The list of profiles used to create the event." .

ocsf:is_secure  rdf:type     owl:DatatypeProperty;
        rdfs:label           "Secure";
        rdfs:range           ocsf:boolean_t;
        dcterms:description  "The cookie attribute indicates that cookies are sent to the server only when the request is encrypted using the HTTPS protocol." .

ocsf:value  rdf:type         owl:DatatypeProperty;
        rdfs:label           "Value";
        rdfs:range           ocsf:string_t;
        dcterms:description  "The value that pertains to the object. See specific usage." .

ocsf:last_seen_time  rdf:type  owl:DatatypeProperty;
        rdfs:label           "Last Seen";
        rdfs:range           ocsf:timestamp_t;
        dcterms:description  "The most recent detection time of the activity or object. See specific usage." .

ocsf:uuid_t  rdf:type        rdfs:Datatype;
        rdfs:label           "UUID";
        rdfs:subClassOf      xsd:string;
        dcterms:description  "128-bit universal unique identifier. For example: <code>123e4567-e89b-12d3-a456-42661417400</code>.";
        xsd:pattern          "[0-9a-fA-F]{8}-[0-9a-fA-F]{4}-[0-9a-fA-F]{4}-[0-9a-fA-F]{4}-[0-9a-fA-F]{12}" .

ocsf:query_time  rdf:type    owl:DatatypeProperty;
        rdfs:label           "Query Time";
        rdfs:range           ocsf:timestamp_t;
        dcterms:description  "The Domain Name System (DNS) query time." .

ocsf:supporting_data  rdf:type  owl:DatatypeProperty;
        rdfs:label           "Supporting Data";
        rdfs:range           ocsf:json_t;
        dcterms:description  "Additional data supporting a finding as provided by security tool" .

ocsf:type_id  rdf:type       owl:DatatypeProperty;
        rdfs:label           "Type ID";
        rdfs:range           ocsf:integer_t;
        dcterms:description  "The normalized type identifier of an object. See specific usage.";
        jsonschema:enum      "Unknown" , "Other" .

ocsf:scheme  rdf:type        owl:DatatypeProperty;
        rdfs:label           "Scheme";
        rdfs:range           ocsf:string_t;
        dcterms:description  "The scheme portion of the URL. For example: <code>http</code>, <code>https</code>, <code>ftp</code>, or <code>sftp</code>." .

ocsf:path  rdf:type          owl:DatatypeProperty;
        rdfs:label           "Path";
        rdfs:range           ocsf:string_t;
        dcterms:description  "The path that pertains to the event or object. See specific usage." .

ocsf:users  rdf:type         owl:ObjectProperty;
        rdfs:label           "Users";
        rdfs:range           ocsf:User;
        dcterms:description  "The users that pertain to the event or object." .

ocsf:detection_uid  rdf:type  owl:DatatypeProperty;
        rdfs:label           "Detection UID";
        rdfs:range           ocsf:string_t;
        dcterms:description  "The associated unique detection event identifier. For example: detection response events include the <b>Detection ID</b> of the original event." .

ocsf:cvss  rdf:type          owl:ObjectProperty;
        rdfs:label           "CVSS Score";
        rdfs:range           ocsf:CVSSScore;
        dcterms:description  "The CVSS object details Common Vulnerability Scoring System (<a target='_blank' href='https://www.first.org/cvss/'>CVSS</a>) scores from the advisory that are related to the vulnerability." .

ocsf:Display  rdf:type       owl:Class;
        rdfs:label           "Display";
        rdfs:subClassOf      ocsf:Object;
        dcterms:description  "The Display object contains information about the physical or virtual display connected to a computer system.";
        ocsf:name            "display" .

ocsf:handshake_dur  rdf:type  owl:DatatypeProperty;
        rdfs:label           "Handshake Duration";
        rdfs:range           ocsf:integer_t;
        dcterms:description  "The amount of total time for the TLS handshake to complete after the TCP connection is established, including client-side delays, in milliseconds." .

ocsf:AffectedSoftwarePackage
        rdf:type             owl:Class;
        rdfs:label           "Affected Software Package";
        rdfs:subClassOf      ocsf:SoftwarePackage;
        rdfs:subClassOf      [ rdf:type            owl:Restriction;
                               owl:onProperty      ocsf:remediation;
                               owl:someValuesFrom  ocsf:Remediation
                             ];
        dcterms:description  "The Affected Package object describes details about a software package identified as affected by a vulnerability/vulnerabilities.";
        ocsf:name            "affected_package" .

ocsf:dmarc_policy  rdf:type  owl:DatatypeProperty;
        rdfs:label           "DMARC Policy";
        rdfs:range           ocsf:string_t;
        dcterms:description  "The Domain-based Message Authentication, Reporting and Conformance (DMARC) policy status." .

ocsf:FileInfoEvent  rdf:type  owl:Class;
        rdfs:label           "File Info";
        rdfs:subClassOf      d3f:DigitalEvent;
        rdfs:subClassOf      [ rdf:type         owl:Restriction;
                               owl:cardinality  1;
                               owl:onProperty   ocsf:file
                             ];
        dcterms:description  "File Info events report information about files that are present on the system.";
        ocsf:name            "file_info";
        ocsf:uid             7 .

ocsf:url_string  rdf:type    owl:DatatypeProperty;
        rdfs:label           "URL String";
        rdfs:range           ocsf:url_t;
        dcterms:description  "The URL string. See RFC 1738. For example: <code>http://www.example.com/download/trouble.exe</code>." .

ocsf:sequence  rdf:type      owl:DatatypeProperty;
        rdfs:label           "Sequence Number";
        rdfs:range           ocsf:integer_t;
        dcterms:description  "Sequence number of the event. The sequence number is a value available in some events, to make the exact ordering of events unambiguous, regardless of the event time precision." .

ocsf:cis_csc  rdf:type       owl:ObjectProperty;
        rdfs:label           "CIS CSC";
        rdfs:range           ocsf:CISCSC;
        dcterms:description  "The CIS Critical Security Controls is a list of top 20 actions and practices an organization’s security team can take on such that cyber attacks or malware, are minimized and prevented." .

ocsf:classification  rdf:type  owl:DatatypeProperty;
        rdfs:label           "Classification";
        rdfs:range           ocsf:string_t;
        dcterms:description  "The classification as defined by the vendor." .

ocsf:DetectionFindingEvent
        rdf:type             owl:Class;
        rdfs:label           "Detection Finding";
        rdfs:subClassOf      ocsf:Finding , d3f:DigitalEvent;
        rdfs:subClassOf      [ rdf:type            owl:Restriction;
                               owl:onProperty      ocsf:evidences;
                               owl:someValuesFrom  ocsf:EvidenceArtifacts
                             ];
        rdfs:subClassOf      [ rdf:type            owl:Restriction;
                               owl:onProperty      ocsf:vulnerabilities;
                               owl:someValuesFrom  ocsf:VulnerabilityDetails
                             ];
        rdfs:subClassOf      [ rdf:type            owl:Restriction;
                               owl:onProperty      ocsf:resources;
                               owl:someValuesFrom  ocsf:ResourceDetails
                             ];
        rdfs:subClassOf      [ rdf:type            owl:Restriction;
                               owl:onProperty      ocsf:remediation;
                               owl:someValuesFrom  ocsf:Remediation
                             ];
        dcterms:description  "A Detection Finding describes detections or alerts generated by security products using correlation engines, detection engines or other methodologies. Note: if the product is a security control, the <code>security_control</code> profile should be applied and its <code>attacks</code> information should be duplicated into the <code>finding_info</code> object.";
        ocsf:category        "findings";
        ocsf:name            "detection_finding";
        ocsf:profiles        "[\"security_control\"]";
        ocsf:uid             4 .

ocsf:SubTechnique  rdf:type  owl:Class;
        rdfs:label           "Sub Technique";
        rdfs:subClassOf      ocsf:Entity;
        dcterms:description  "The Sub Technique object describes the sub technique ID and/or name associated to an attack, as defined by <a target='_blank' href='https://attack.mitre.org/wiki/ATT&CK_Matrix'>ATT&CK Matrix<sup>TM</sup></a>.";
        ocsf:name            "sub_technique" .

ocsf:action  rdf:type        owl:DatatypeProperty;
        rdfs:label           "Action";
        rdfs:range           ocsf:string_t;
        dcterms:description  "The normalized caption of 'action_id' or the source specific action." .

ocsf:raw_data  rdf:type      owl:DatatypeProperty;
        rdfs:label           "Raw Data";
        rdfs:range           ocsf:string_t;
        dcterms:description  "The raw event/finding data as received from the source." .

ocsf:NetworksInfoEvent
        rdf:type             owl:Class;
        rdfs:label           "Networks Info";
        rdfs:subClassOf      d3f:DigitalEvent;
        rdfs:subClassOf      [ rdf:type         owl:Restriction;
                               owl:cardinality  1;
                               owl:onProperty   ocsf:network_interfaces
                             ];
        dcterms:description  "Networks Info events report information about network adapters.";
        ocsf:name            "networks_info";
        ocsf:uid             13 .

ocsf:endpoint_connections
        rdf:type             owl:ObjectProperty;
        rdfs:label           "Endpoint Connections";
        dcterms:description  "Contains information about network connection attempts. See specific usage." .

ocsf:access_mask  rdf:type   owl:DatatypeProperty;
        rdfs:label           "Access Mask";
        rdfs:range           ocsf:integer_t;
        dcterms:description  "The access mask in a platform-native format." .

ocsf:CVSSScore  rdf:type     owl:Class;
        rdfs:label           "CVSS Score";
        rdfs:subClassOf      ocsf:Object;
        rdfs:subClassOf      [ rdf:type            owl:Restriction;
                               owl:onProperty      ocsf:metrics;
                               owl:someValuesFrom  ocsf:Metric
                             ];
        dcterms:description  "The Common Vulnerability Scoring System (<a target='_blank' href='https://www.first.org/cvss/'>CVSS</a>) object provides a way to capture the principal characteristics of a vulnerability and produce a numerical score reflecting its severity.";
        ocsf:name            "cvss" .

ocsf:details  rdf:type       owl:DatatypeProperty;
        rdfs:label           "Details";
        rdfs:range           ocsf:string_t;
        dcterms:description  "Details of an entity. See specific usage" .

ocsf:time  rdf:type          owl:DatatypeProperty;
        rdfs:label           "Event Time";
        rdfs:range           ocsf:timestamp_t;
        dcterms:description  "The normalized event occurrence time or the finding creation time." .

ocsf:SoftwarePackage  rdf:type  owl:Class;
        rdfs:label           "Software Package";
        rdfs:subClassOf      ocsf:Object;
        dcterms:description  "The Software Package object describes details about a software package. Defined by D3FEND <a target='_blank' href='https://d3fend.mitre.org/dao/artifact/d3f:SoftwarePackage/'>d3f:SoftwarePackage</a>.";
        ocsf:name            "package" .

ocsf:process_name_t  rdf:type  rdfs:Datatype;
        rdfs:label           "Process Name";
        rdfs:subClassOf      xsd:string;
        dcterms:description  "Process name. For example: <code>Notepad</code>." .

ocsf:algorithm  rdf:type     owl:DatatypeProperty;
        rdfs:label           "Algorithm";
        rdfs:range           ocsf:string_t;
        dcterms:description  "The applicable algorithm, normalized to the caption of 'algorithm_id'. See specific usage." .

ocsf:tenant_uid  rdf:type    owl:DatatypeProperty;
        rdfs:label           "Tenant UID";
        rdfs:range           ocsf:string_t;
        dcterms:description  "The unique tenant identifier." .

ocsf:idp  rdf:type           owl:ObjectProperty;
        rdfs:label           "Identity Provider";
        rdfs:range           ocsf:IdentityProvider;
        dcterms:description  "This object describes details about the Identity Provider used." .

ocsf:resource_uid_t  rdf:type  rdfs:Datatype;
        rdfs:label           "Resource UID";
        rdfs:subClassOf      xsd:string;
        dcterms:description  "Resource unique identifier. For example, S3 Bucket name or EC2 Instance ID." .

ocsf:direction_id  rdf:type  owl:DatatypeProperty;
        rdfs:label           "Direction ID";
        rdfs:range           ocsf:integer_t;
        dcterms:description  "The normalized identifier of the direction of the initiated connection, traffic, or email.";
        jsonschema:enum      "Other" , "Lateral" , "Outbound" , "Inbound" , "Unknown" .

ocsf:start_address  rdf:type  owl:DatatypeProperty;
        rdfs:label           "Start Address";
        rdfs:range           ocsf:string_t;
        dcterms:description  "The start address of the execution." .

ocsf:AccountChangeEvent
        rdf:type             owl:Class;
        rdfs:label           "Account Change";
        rdfs:subClassOf      d3f:DigitalEvent;
        rdfs:subClassOf      [ rdf:type            owl:Restriction;
                               owl:onProperty      ocsf:actor;
                               owl:someValuesFrom  ocsf:Actor
                             ];
        rdfs:subClassOf      [ rdf:type         owl:Restriction;
                               owl:cardinality  1;
                               owl:onProperty   ocsf:user
                             ];
        rdfs:subClassOf      [ rdf:type            owl:Restriction;
                               owl:onProperty      ocsf:src_endpoint;
                               owl:someValuesFrom  ocsf:NetworkEndpoint
                             ];
        rdfs:subClassOf      [ rdf:type            owl:Restriction;
                               owl:onProperty      ocsf:user_result;
                               owl:someValuesFrom  ocsf:User
                             ];
        rdfs:subClassOf      [ rdf:type            owl:Restriction;
                               owl:onProperty      ocsf:policy;
                               owl:someValuesFrom  ocsf:Policy
                             ];
        rdfs:subClassOf      [ rdf:type            owl:Restriction;
                               owl:onProperty      ocsf:http_request;
                               owl:someValuesFrom  ocsf:HTTPRequest
                             ];
        dcterms:description  "Account Change events report when specific user account management tasks are performed, such as a user/role being created, changed, deleted, renamed, disabled, enabled, locked out or unlocked.";
        ocsf:name            "account_change";
        ocsf:uid             1 .

ocsf:string_t  rdf:type      rdfs:Datatype;
        rdfs:label           "String";
        rdfs:subClassOf      xsd:string;
        dcterms:description  "UTF-8 encoded byte sequence." .

ocsf:file  rdf:type          owl:ObjectProperty;
        rdfs:label           "File";
        rdfs:range           ocsf:File;
        dcterms:description  "The file that pertains to the event or object. See specific usage." .

ocsf:injection_type  rdf:type  owl:DatatypeProperty;
        rdfs:label           "Injection Type";
        rdfs:range           ocsf:string_t;
        dcterms:description  "The process injection method, normalized to the caption of the injection_type_id value. In the case of 'Other', it is defined by the event source." .

ocsf:IdentityAccessManagementEvent
        rdf:type             owl:Class;
        rdfs:label           "Identity & Access Management";
        rdfs:subClassOf      d3f:DigitalEvent;
        dcterms:description  "The Identity & Access Management event is a generic event that defines a set of attributes available in the access control events. As a generic event, it could be used to log events that are not otherwise defined by the IAM category.";
        ocsf:category        "iam";
        ocsf:name            "iam";
        ocsf:profiles        "[\"host\"]" .

ocsf:bytestring_t  rdf:type  rdfs:Datatype;
        rdfs:label           "Byte String";
        rdfs:subClassOf      xsd:string;
        dcterms:description  "Base64 encoded immutable byte sequence." .

ocsf:ApplicationLifecycleEvent
        rdf:type             owl:Class;
        rdfs:label           "Application Lifecycle";
        rdfs:subClassOf      d3f:DigitalEvent;
        rdfs:subClassOf      [ rdf:type         owl:Restriction;
                               owl:cardinality  1;
                               owl:onProperty   ocsf:app
                             ];
        dcterms:description  "Application Lifecycle events report installation, removal, start, stop of an application or service.";
        ocsf:name            "application_lifecycle";
        ocsf:profiles        "[\"host\"]";
        ocsf:uid             2 .

ocsf:load_type_id  rdf:type  owl:DatatypeProperty;
        rdfs:label           "Load Type ID";
        rdfs:range           ocsf:integer_t;
        dcterms:description  "The normalized identifier of the load type. It identifies how the module was loaded in memory." .

ocsf:invoked_by  rdf:type    owl:DatatypeProperty;
        rdfs:label           "Invoked by";
        rdfs:range           ocsf:string_t;
        dcterms:description  "The name of the service that invoked the activity as described in the event." .

ocsf:firewall_rule  rdf:type  owl:ObjectProperty;
        rdfs:label           "Firewall Rule";
        rdfs:range           ocsf:FirewallRule;
        dcterms:description  "The firewall rule that triggered the event." .

ocsf:cloud  rdf:type         owl:ObjectProperty;
        rdfs:label           "Cloud";
        rdfs:range           ocsf:Cloud;
        dcterms:description  "Describes details about the Cloud environment where the event was originally created or logged." .

ocsf:permission  rdf:type    owl:DatatypeProperty;
        rdfs:label           "Permission";
        rdfs:range           ocsf:string_t;
        dcterms:description  "The IAM permission related to an event" .

ocsf:query  rdf:type         owl:ObjectProperty;
        rdfs:label           "DNS Query";
        rdfs:range           ocsf:DNSQuery;
        dcterms:description  "The Domain Name System (DNS) query." .

ocsf:accessor  rdf:type      owl:ObjectProperty;
        rdfs:label           "Accessor";
        rdfs:range           ocsf:User;
        dcterms:description  "The name of the user who last accessed the object." .

ocsf:disposition_id  rdf:type  owl:DatatypeProperty;
        rdfs:label           "Disposition ID";
        rdfs:range           ocsf:integer_t;
        dcterms:description  "Describes the outcome or action taken by a security control, such as access control checks, malware detections or various types of policy violations.";
        jsonschema:enum      "Unknown" , "Other" .

ocsf:type_uid  rdf:type      owl:DatatypeProperty;
        rdfs:label           "Type ID";
        rdfs:range           ocsf:integer_t;
        dcterms:description  "The event/finding type ID. It identifies the event's semantics and structure. The value is calculated by the logging system as: <code>class_uid * 100 + activity_id</code>." .

ocsf:postal_code  rdf:type   owl:DatatypeProperty;
        rdfs:label           "Postal Code";
        rdfs:range           ocsf:string_t;
        dcterms:description  "The postal code of the location." .

ocsf:kernel  rdf:type        owl:ObjectProperty;
        rdfs:label           "Kernel";
        rdfs:range           ocsf:KernelResource;
        dcterms:description  "The kernel resource object that pertains to the event." .

ocsf:architecture  rdf:type  owl:DatatypeProperty;
        rdfs:label           "Architecture";
        rdfs:range           ocsf:string_t;
        dcterms:description  "Architecture is a shorthand name describing the type of computer hardware the packaged software is meant to run on." .

ocsf:sub_technique  rdf:type  owl:ObjectProperty;
        rdfs:label           "Sub Technique";
        rdfs:range           ocsf:SubTechnique;
        dcterms:description  "The Sub Technique object describes the sub technique ID and/or name associated to an attack, as defined by <a target='_blank' href='https://attack.mitre.org/wiki/ATT&CK_Matrix'>ATT&CK Matrix<sup>TM</sup></a>." .

ocsf:AdminGroupInfoEvent
        rdf:type             owl:Class;
        rdfs:label           "Admin Group Info";
        rdfs:subClassOf      d3f:DigitalEvent;
        rdfs:subClassOf      [ rdf:type            owl:Restriction;
                               owl:onProperty      ocsf:users;
                               owl:someValuesFrom  ocsf:User
                             ];
        rdfs:subClassOf      [ rdf:type         owl:Restriction;
                               owl:cardinality  1;
                               owl:onProperty   ocsf:group
                             ];
        dcterms:description  "Group Info events report information about administrative groups.";
        ocsf:name            "admin_group_info";
        ocsf:uid             9 .

ocsf:DigitalCertificate
        rdf:type             owl:Class;
        rdfs:label           "Digital Certificate";
        rdfs:subClassOf      ocsf:Object;
        rdfs:subClassOf      [ rdf:type         owl:Restriction;
                               owl:cardinality  1;
                               owl:onProperty   ocsf:fingerprints
                             ];
        dcterms:description  "The Digital Certificate, also known as a Public Key Certificate, object contains information about the ownership and usage of a public key. It serves as a means to establish trust in the authenticity and integrity of the public key and the associated entity. Defined by D3FEND <a target='_blank' href='https://d3fend.mitre.org/dao/artifact/d3f:Certificate/'>d3f:Certificate</a>.";
        ocsf:name            "certificate" .

ocsf:is_on_premises  rdf:type  owl:DatatypeProperty;
        rdfs:label           "On Premises";
        rdfs:range           ocsf:boolean_t;
        dcterms:description  "The indication of whether the location is on premises." .

ocsf:KernelActivityEvent
        rdf:type             owl:Class;
        rdfs:label           "Kernel Activity";
        rdfs:subClassOf      d3f:DigitalEvent;
        rdfs:subClassOf      [ rdf:type         owl:Restriction;
                               owl:cardinality  1;
                               owl:onProperty   ocsf:kernel
                             ];
        dcterms:description  "Kernel Activity events report when an process creates, reads, or deletes a kernel resource.";
        ocsf:name            "kernel_activity";
        ocsf:uid             3 .

ocsf:Service  rdf:type       owl:Class;
        rdfs:label           "Service";
        rdfs:subClassOf      ocsf:Entity;
        dcterms:description  "The Service object describes characteristics of a service, <code> e.g. AWS EC2. </code>";
        ocsf:name            "service" .

ocsf:references  rdf:type    owl:DatatypeProperty;
        rdfs:label           "References";
        rdfs:range           ocsf:string_t;
        dcterms:description  "A list of reference URLs supporting the finding/detection." .

ocsf:job  rdf:type           owl:ObjectProperty;
        rdfs:label           "Job";
        rdfs:range           ocsf:Job;
        dcterms:description  "The job object that pertains to the event." .

ocsf:packet_uid  rdf:type    owl:DatatypeProperty;
        rdfs:label           "Packet UID";
        rdfs:range           ocsf:integer_t;
        dcterms:description  "The packet identifier assigned by the protocol." .

ocsf:stratum_id  rdf:type    owl:DatatypeProperty;
        rdfs:label           "Stratum ID";
        rdfs:range           ocsf:integer_t;
        dcterms:description  "The normalized identifier of the stratum level, as defined in <a target='_blank' href='https://www.rfc-editor.org/rfc/rfc5905.html'>RFC-5905</a>.";
        jsonschema:enum      "Primary Server" , "Secondary Server" , "Unknown" , "Reserved" , "Other" , "Unsynchronized" .

ocsf:vector_string  rdf:type  owl:DatatypeProperty;
        rdfs:label           "Vector String";
        rdfs:range           ocsf:string_t;
        dcterms:description  "The CVSS vector string is a text representation of a set of CVSS metrics. It is commonly used to record or transfer CVSS metric information in a concise form. For example: <code>3.1/AV:L/AC:L/PR:L/UI:N/S:U/C:H/I:N/A:H</code>." .

ocsf:fingerprint  rdf:type   owl:ObjectProperty;
        rdfs:label           "Fingerprint";
        rdfs:range           ocsf:Fingerprint;
        dcterms:description  "The digital fingerprint associated with an object." .

ocsf:Endpoint  rdf:type      owl:Class;
        rdfs:label           "Endpoint";
        rdfs:subClassOf      ocsf:Entity;
        rdfs:subClassOf      [ rdf:type            owl:Restriction;
                               owl:onProperty      ocsf:location;
                               owl:someValuesFrom  ocsf:GeoLocation
                             ];
        dcterms:description  "The Endpoint object describes a physical or virtual device that connects to and exchanges information with a computer network. Some examples of endpoints are mobile devices, desktop computers, virtual machines, embedded devices, and servers. Internet-of-Things devices—like cameras, lighting, refrigerators, security systems, smart speakers, and thermostats—are also endpoints.";
        ocsf:constraints     "{\"at_least_one\":[\"ip\",\"uid\",\"name\",\"hostname\",\"instance_uid\",\"interface_uid\",\"interface_name\"]}";
        ocsf:name            "endpoint";
        ocsf:observable      20 .

ocsf:network_endpoint
        rdf:type             owl:ObjectProperty;
        rdfs:label           "Network Endpoint";
        rdfs:range           ocsf:NetworkEndpoint;
        dcterms:description  "The Network Endpoint object describes characteristics of a network endpoint. See specific usage." .

ocsf:evidence  rdf:type      owl:DatatypeProperty;
        rdfs:label           "Evidence";
        rdfs:range           ocsf:json_t;
        dcterms:description  "The data the finding exposes to the analyst." .

ocsf:proxy  rdf:type         owl:ObjectProperty;
        rdfs:label           "Proxy";
        rdfs:range           ocsf:NetworkProxyEndpoint;
        dcterms:description  "The proxy (server) in a network connection." .

ocsf:type  rdf:type          owl:DatatypeProperty;
        rdfs:label           "Type";
        rdfs:range           ocsf:string_t;
        dcterms:description  "The type of an object or value, normalized to the caption of the type_id value. In the case of 'Other', it is defined by the event source. See specific usage." .

ocsf:intermediate_ips
        rdf:type             owl:DatatypeProperty;
        rdfs:label           "Intermediate IP Addresses";
        rdfs:range           ocsf:ip_t;
        dcterms:description  "The intermediate IP Addresses. For example, the IP addresses in the HTTP X-Forwarded-For header." .

ocsf:HTTPResponse  rdf:type  owl:Class;
        rdfs:label           "HTTP Response";
        rdfs:subClassOf      ocsf:Object;
        rdfs:subClassOf      [ rdf:type            owl:Restriction;
                               owl:onProperty      ocsf:http_headers;
                               owl:someValuesFrom  ocsf:HTTPHeader
                             ];
        dcterms:description  "The HTTP Response object contains detailed information about the response sent from a web server to the requester. It encompasses attributes and metadata that describe the response status, headers, body content, and other relevant information.";
        ocsf:name            "http_response" .

ocsf:NetworkConnectionInfoEvent
        rdf:type             owl:Class;
        rdfs:label           "Network Connection Info";
        rdfs:subClassOf      d3f:DigitalEvent;
        rdfs:subClassOf      [ rdf:type         owl:Restriction;
                               owl:cardinality  1;
                               owl:onProperty   ocsf:process
                             ];
        rdfs:subClassOf      [ rdf:type         owl:Restriction;
                               owl:cardinality  1;
                               owl:onProperty   ocsf:connection_info
                             ];
        dcterms:description  "Network Connection Info events report information about active network connections.";
        ocsf:name            "network_connection_info";
        ocsf:uid             12 .

ocsf:load_balancer  rdf:type  owl:ObjectProperty;
        rdfs:label           "Load Balancer";
        dcterms:description  "The Load Balancer object contains information related to the device that is distributing incoming traffic to specified destinations." .

ocsf:dst_endpoint  rdf:type  owl:ObjectProperty;
        rdfs:label           "Destination Endpoint";
        rdfs:range           ocsf:NetworkEndpoint;
        dcterms:description  "The network destination endpoint." .

ocsf:ProcessInfoEvent
        rdf:type             owl:Class;
        rdfs:label           "Process Info";
        rdfs:subClassOf      d3f:DigitalEvent;
        rdfs:subClassOf      [ rdf:type         owl:Restriction;
                               owl:cardinality  1;
                               owl:onProperty   ocsf:process
                             ];
        dcterms:description  "Process Info events report information about running processes.";
        ocsf:name            "process_info";
        ocsf:uid             15 .

ocsf:terminated_time  rdf:type  owl:DatatypeProperty;
        rdfs:label           "Terminated Time";
        rdfs:range           ocsf:timestamp_t;
        dcterms:description  "The time when the entity was terminated. See specific usage." .

ocsf:keyboard_subtype
        rdf:type             owl:DatatypeProperty;
        rdfs:label           "Keyboard Subtype";
        rdfs:range           ocsf:integer_t;
        dcterms:description  "The keyboard numeric code." .

ocsf:enrichments  rdf:type   owl:ObjectProperty;
        rdfs:label           "Enrichments";
        rdfs:range           ocsf:Enrichment;
        dcterms:description  "The additional information from an external data source, which is associated with the event or a finding. For example add location information for the IP address in the DNS answers:</p><code>[{\"name\": \"answers.ip\", \"value\": \"92.24.47.250\", \"type\": \"location\", \"data\": {\"city\": \"Socotra\", \"continent\": \"Asia\", \"coordinates\": [-25.4153, 17.0743], \"country\": \"YE\", \"desc\": \"Yemen\"}}]</code>" .

ocsf:category_ids  rdf:type  owl:DatatypeProperty;
        rdfs:label           "Website Categorization IDs";
        rdfs:range           ocsf:integer_t;
        dcterms:description  "The Website categorization identifies.";
        jsonschema:enum      "Translation" , "Piracy/Copyright Concerns" , "Peer-to-Peer (P2P)" , "Violence/Hate/Racism" , "Health" , "Sex Education" , "Computer/Information Security" , "Search Engines/Portals" , "Placeholders" , "Travel" , "Web Ads/Analytics" , "News/Media" , "For Kids" , "Software Downloads" , "Brokerage/Trading" , "Entertainment" , "Art/Culture" , "Job Search/Careers" , "Social Networking" , "Gambling" , "Military" , "Real Estate" , "Society/Daily Living" , "Government/Legal" , "Nudity" , "Marijuana" , "Informational" , "Education" , "Intimate Apparel/Swimsuit" , "Potentially Unwanted Software" , "Personals/Dating" , "Radio/Audio Streams" , "Non-Viewable/Infrastructure" , "Humor/Jokes" , "Suspicious" , "Games" , "Auctions" , "Charitable Organizations" , "Reference" , "Dynamic DNS Host" , "Online Meetings" , "Content Servers" , "Malicious Sources/Malnets" , "Scam/Questionable/Illegal" , "Malicious Outbound Data/Botnets" , "Newsgroups/Forums" , "Alternative Spirituality/Belief" , "Shopping" , "E-Card/Invitations" , "Unknown" , "Abortion" , "Alcohol" , "Financial Services" , "Web Hosting" , "Audio/Video Clips" , "Political/Social Advocacy" , "Hacking" , "Phishing" , "Extreme" , "Sports/Recreation" , "Business/Economy" , "Spam" , "Proxy Avoidance" , "Controlled Substances" , "Other" , "Tobacco" , "Internet Telephony" , "Weapons" , "Pornography" , "Personal Sites" , "Technology/Internet" , "Remote Access Tools" , "Email" , "Office/Business Applications" , "Media Sharing" , "Religion" , "Uncategorized" , "Adult/Mature Content" , "Vehicles" , "TV/Video Streams" , "Child Pornography" , "File Storage/Sharing" , "Restaurants/Dining/Food" , "Mixed Content/Potentially Adult" , "Internet Connected Devices" , "Chat (IM)/SMS" , "Sexual Expression" .

ocsf:state  rdf:type         owl:DatatypeProperty;
        rdfs:label           "State";
        rdfs:range           ocsf:string_t;
        dcterms:description  "The state of the event or object, normalized to the caption of the state_id value. In the case of 'Other', it is defined by the event source. See specific usage." .

ocsf:bytes_in  rdf:type      owl:DatatypeProperty;
        rdfs:label           "Bytes In";
        rdfs:range           ocsf:long_t;
        dcterms:description  "The number of bytes sent from the destination to the source." .

ocsf:identifier_cookie
        rdf:type             owl:DatatypeProperty;
        rdfs:label           "Identifier Cookie";
        rdfs:range           ocsf:string_t;
        dcterms:description  "The client identifier cookie during client/server exchange." .

ocsf:parent_folder  rdf:type  owl:DatatypeProperty;
        rdfs:label           "Parent Folder";
        rdfs:range           ocsf:string_t;
        dcterms:description  "The parent folder in which the file resides. For example: <code>c:\\windows\\system32</code>" .

ocsf:dkim_signature  rdf:type  owl:DatatypeProperty;
        rdfs:label           "DKIM Signature";
        rdfs:range           ocsf:string_t;
        dcterms:description  "The DomainKeys Identified Mail (DKIM) signature used by the sending/receiving system." .

ocsf:owner  rdf:type         owl:ObjectProperty;
        rdfs:label           "Owner";
        rdfs:range           ocsf:User;
        dcterms:description  "The user that owns the file/object." .

ocsf:Cloud  rdf:type         owl:Class;
        rdfs:label           "Cloud";
        rdfs:subClassOf      ocsf:Object;
        rdfs:subClassOf      [ rdf:type            owl:Restriction;
                               owl:onProperty      ocsf:org;
                               owl:someValuesFrom  ocsf:Organization
                             ];
        rdfs:subClassOf      [ rdf:type            owl:Restriction;
                               owl:onProperty      ocsf:account;
                               owl:someValuesFrom  ocsf:Account
                             ];
        dcterms:description  "The Cloud object contains information about a cloud account such as AWS Account ID, regions, etc.";
        ocsf:name            "cloud" .

ocsf:analytic  rdf:type      owl:ObjectProperty;
        rdfs:label           "Analytic";
        rdfs:range           ocsf:Analytic;
        dcterms:description  "The analytic technique used to analyze and derive insights from the data or information that led to the finding or conclusion." .

ocsf:coordinates  rdf:type   owl:DatatypeProperty;
        rdfs:label           "Coordinates";
        rdfs:range           ocsf:float_t;
        dcterms:description  "A two-element array, containing a longitude/latitude pair. The format conforms with <a target='_blank' href='https://geojson.org'>GeoJSON</a>. For example: <code>[-73.983, 40.719]</code>." .

ocsf:WebResourceAccessActivityEvent
        rdf:type             owl:Class;
        rdfs:label           "Web Resource Access Activity";
        rdfs:subClassOf      d3f:DigitalEvent;
        rdfs:subClassOf      [ rdf:type            owl:Restriction;
                               owl:onProperty      ocsf:tls;
                               owl:someValuesFrom  ocsf:TransportLayerSecurityTLS
                             ];
        rdfs:subClassOf      [ rdf:type            owl:Restriction;
                               owl:onProperty      ocsf:http_response;
                               owl:someValuesFrom  ocsf:HTTPResponse
                             ];
        rdfs:subClassOf      [ rdf:type         owl:Restriction;
                               owl:cardinality  1;
                               owl:onProperty   ocsf:web_resources
                             ];
        rdfs:subClassOf      [ rdf:type         owl:Restriction;
                               owl:cardinality  1;
                               owl:onProperty   ocsf:http_request
                             ];
        rdfs:subClassOf      [ rdf:type            owl:Restriction;
                               owl:onProperty      ocsf:proxy;
                               owl:someValuesFrom  ocsf:NetworkProxyEndpoint
                             ];
        rdfs:subClassOf      [ rdf:type            owl:Restriction;
                               owl:onProperty      ocsf:src_endpoint;
                               owl:someValuesFrom  ocsf:NetworkEndpoint
                             ];
        dcterms:description  "Web Resource Access Activity events describe successful/failed attempts to access a web resource over HTTP.";
        ocsf:category        "application";
        ocsf:name            "web_resource_access_activity";
        ocsf:profiles        "[\"host\",\"network_proxy\"]";
        ocsf:uid             4 .

ocsf:Observable  rdf:type    owl:Class;
        rdfs:label           "Observable";
        rdfs:subClassOf      ocsf:Object;
        rdfs:subClassOf      [ rdf:type            owl:Restriction;
                               owl:onProperty      ocsf:reputation;
                               owl:someValuesFrom  ocsf:Reputation
                             ];
        dcterms:description  "The observable object is a pivot element that contains related information found in many places in the event.";
        ocsf:name            "observable" .

ocsf:http_response  rdf:type  owl:ObjectProperty;
        rdfs:label           "HTTP Response";
        rdfs:range           ocsf:HTTPResponse;
        dcterms:description  "The HTTP Response from a web server to a requester." .

ocsf:risk_level  rdf:type    owl:DatatypeProperty;
        rdfs:label           "Risk Level";
        rdfs:range           ocsf:string_t;
        dcterms:description  "The risk level, normalized to the caption of the risk_level_id value. In the case of 'Other', it is defined by the event source." .

ocsf:NetworkEvent  rdf:type  owl:Class;
        rdfs:label           "Network";
        rdfs:subClassOf      d3f:DigitalEvent;
        rdfs:subClassOf      [ rdf:type            owl:Restriction;
                               owl:onProperty      ocsf:traffic;
                               owl:someValuesFrom  ocsf:NetworkTraffic
                             ];
        rdfs:subClassOf      [ rdf:type            owl:Restriction;
                               owl:onProperty      ocsf:tls;
                               owl:someValuesFrom  ocsf:TransportLayerSecurityTLS
                             ];
        rdfs:subClassOf      [ rdf:type         owl:Restriction;
                               owl:cardinality  1;
                               owl:onProperty   ocsf:src_endpoint
                             ];
        rdfs:subClassOf      [ rdf:type            owl:Restriction;
                               owl:onProperty      ocsf:connection_info;
                               owl:someValuesFrom  ocsf:NetworkConnectionInformation
                             ];
        rdfs:subClassOf      [ rdf:type            owl:Restriction;
                               owl:onProperty      ocsf:proxy;
                               owl:someValuesFrom  ocsf:NetworkProxyEndpoint
                             ];
        rdfs:subClassOf      [ rdf:type         owl:Restriction;
                               owl:cardinality  1;
                               owl:onProperty   ocsf:dst_endpoint
                             ];
        dcterms:description  "Network event is a generic event that defines a set of attributes available in the Network category.";
        ocsf:category        "network";
        ocsf:name            "network";
        ocsf:profiles        "[\"host\",\"network_proxy\",\"security_control\",\"load_balancer\"]" .

ocsf:extension  rdf:type     owl:ObjectProperty;
        rdfs:label           "Schema Extension";
        rdfs:range           ocsf:SchemaExtension;
        dcterms:description  "The schema extension used to create the event." .

ocsf:is_default  rdf:type    owl:DatatypeProperty;
        rdfs:label           "Default Value";
        rdfs:range           ocsf:boolean_t;
        dcterms:description  "The indication of whether the value is from a default value name. For example, the value name could be missing." .

ocsf:CISBenchmarkResult
        rdf:type             owl:Class;
        rdfs:label           "CIS Benchmark Result";
        rdfs:subClassOf      ocsf:Object;
        rdfs:subClassOf      [ rdf:type            owl:Restriction;
                               owl:onProperty      ocsf:rule;
                               owl:someValuesFrom  ocsf:Rule
                             ];
        rdfs:subClassOf      [ rdf:type            owl:Restriction;
                               owl:onProperty      ocsf:remediation;
                               owl:someValuesFrom  ocsf:Remediation
                             ];
        dcterms:description  "The CIS Benchmark Result object contains information as defined by the Center for Internet Security (<a target='_blank' href='https://www.cisecurity.org/cis-benchmarks/'>CIS</a>) benchmark result. CIS Benchmarks are a collection of best practices for securely configuring IT systems, software, networks, and cloud infrastructure.";
        ocsf:name            "cis_benchmark_result" .

ocsf:file_diff  rdf:type     owl:DatatypeProperty;
        rdfs:label           "File Diff";
        rdfs:range           ocsf:string_t;
        dcterms:description  "File content differences used for change detection. For example, a common use case is to identify itemized changes within INI or configuration/property setting values." .

ocsf:cve  rdf:type           owl:ObjectProperty;
        rdfs:label           "CVE";
        rdfs:range           ocsf:CVE;
        dcterms:description  "The Common Vulnerabilities and Exposures (<a target='_blank' href='https://cve.mitre.org/'>CVE</a>)." .

ocsf:rpc_interface  rdf:type  owl:ObjectProperty;
        rdfs:label           "Remote Procedure Call Interface";
        rdfs:range           ocsf:RPCInterface;
        dcterms:description  "The RPC Interface object describes the details pertaining to the remote procedure call interface." .

ocsf:keyboard_info  rdf:type  owl:ObjectProperty;
        rdfs:label           "Keyboard Information";
        rdfs:range           ocsf:KeyboardInformation;
        dcterms:description  "The keyboard detailed information." .

ocsf:malware  rdf:type       owl:ObjectProperty;
        rdfs:label           "Malware";
        rdfs:range           ocsf:Malware;
        dcterms:description  "A list of Malware objects, decribing details about the identified malware." .

ocsf:NetworkActivityEvent
        rdf:type             owl:Class;
        rdfs:label           "Network Activity";
        rdfs:subClassOf      d3f:DigitalEvent;
        rdfs:subClassOf      [ rdf:type            owl:Restriction;
                               owl:onProperty      ocsf:url;
                               owl:someValuesFrom  ocsf:UniformResourceLocator
                             ];
        dcterms:description  "Network Activity events report network connection and traffic activity.";
        ocsf:category        "network";
        ocsf:name            "network_activity";
        ocsf:uid             1 .

ocsf:signature  rdf:type     owl:ObjectProperty;
        rdfs:label           "Digital Signature";
        rdfs:range           ocsf:DigitalSignature;
        dcterms:description  "The digital signature of the file." .

ocsf:class_name  rdf:type    owl:DatatypeProperty;
        rdfs:label           "Class";
        rdfs:range           ocsf:string_t;
        dcterms:description  "The event class name, as defined by class_uid value." .

ocsf:integrity_id  rdf:type  owl:DatatypeProperty;
        rdfs:label           "Integrity Level";
        rdfs:range           ocsf:integer_t;
        dcterms:description  "The normalized identifier of the process integrity level (Windows only)." .

ocsf:CISBenchmark  rdf:type  owl:Class;
        rdfs:label           "CIS Benchmark";
        rdfs:subClassOf      ocsf:Object;
        rdfs:subClassOf      [ rdf:type            owl:Restriction;
                               owl:onProperty      ocsf:cis_controls;
                               owl:someValuesFrom  ocsf:CISControl
                             ];
        dcterms:description  "The CIS Benchmark object describes best practices for securely configuring IT systems, software, networks, and cloud infrastructure as defined by the <a target='_blank' href='https://www.cisecurity.org/cis-benchmarks/'>Center for Internet Security</a>. See also <a target='_blank' href='https://www.cisecurity.org/insights/blog/getting-to-know-the-cis-benchmarks'>Getting to Know the CIS Benchmarks</a>.";
        ocsf:name            "cis_benchmark" .

ocsf:confidentiality  rdf:type  owl:DatatypeProperty;
        rdfs:label           "Confidentiality";
        rdfs:range           ocsf:string_t;
        dcterms:description  "The file content confidentiality, normalized to the confidentiality_id value. In the case of 'Other', it is defined by the event source." .

ocsf:related_analytics
        rdf:type             owl:ObjectProperty;
        rdfs:label           "Related Analytics";
        rdfs:range           ocsf:Analytic;
        dcterms:description  "Describes analytics related to the analytic of a finding or detection as identified by the security product." .

ocsf:data  rdf:type          owl:DatatypeProperty;
        rdfs:label           "Data";
        rdfs:range           ocsf:json_t;
        dcterms:description  "The additional data that is associated with the event or object. See specific usage." .

ocsf:account  rdf:type       owl:ObjectProperty;
        rdfs:label           "Account";
        rdfs:range           ocsf:Account;
        dcterms:description  "The account object describes details about the account that was the source or target of the activity." .

ocsf:run_state  rdf:type     owl:DatatypeProperty;
        rdfs:label           "Run State";
        rdfs:range           ocsf:string_t;
        dcterms:description  "The state of the job or service, normalized to the caption of the run_state_id value. In the case of 'Other', it is defined by the event source. See specific usage." .

ocsf:codes  rdf:type         owl:DatatypeProperty;
        rdfs:label           "Response Codes";
        rdfs:range           ocsf:integer_t;
        dcterms:description  "The list of numeric responses sent to a request." .

ocsf:logon_type_id  rdf:type  owl:DatatypeProperty;
        rdfs:label           "Logon Type ID";
        rdfs:range           ocsf:integer_t;
        dcterms:description  "The normalized logon type identifier.";
        jsonschema:enum      "New Credentials" , "Unlock" , "Interactive" , "Remote Interactive" , "Cached Unlock" , "Other" , "Cached Remote Interactive" , "Cached Interactive" , "Network" , "Batch" , "System" , "OS Service" , "Network Cleartext" .

ocsf:accessed_time  rdf:type  owl:DatatypeProperty;
        rdfs:label           "Accessed Time";
        rdfs:range           ocsf:timestamp_t;
        dcterms:description  "The time when the file was last accessed." .

ocsf:is_managed  rdf:type    owl:DatatypeProperty;
        rdfs:label           "Managed Device";
        rdfs:range           ocsf:boolean_t;
        dcterms:description  "The event occurred on a managed device." .

ocsf:bytes_out  rdf:type     owl:DatatypeProperty;
        rdfs:label           "Bytes Out";
        rdfs:range           ocsf:long_t;
        dcterms:description  "The number of bytes sent from the source to the destination." .

ocsf:file_name_t  rdf:type   rdfs:Datatype;
        rdfs:label           "File Name";
        rdfs:subClassOf      xsd:string;
        dcterms:description  "File name. For example: <code>text-file.txt</code>." .

ocsf:authorizations  rdf:type  owl:ObjectProperty;
        rdfs:label           "Authorization Information";
        rdfs:range           ocsf:AuthorizationResult;
        dcterms:description  "Provides details about an authorization, such as authorization outcome, and any associated policies related to the activity/event." .

ocsf:remediation  rdf:type   owl:ObjectProperty;
        rdfs:label           "Remediation Guidance";
        rdfs:range           ocsf:Remediation;
        dcterms:description  "Describes the recommended remediation steps to address identified issue(s)." .

ocsf:desc  rdf:type          owl:DatatypeProperty;
        rdfs:label           "Description";
        rdfs:range           ocsf:string_t;
        dcterms:description  "The description that pertains to the object or event. See specific usage." .

ocsf:port  rdf:type          owl:DatatypeProperty;
        rdfs:label           "Port";
        rdfs:range           ocsf:port_t;
        dcterms:description  "The TCP/UDP port number associated with a connection. See specific usage." .

ocsf:license  rdf:type       owl:DatatypeProperty;
        rdfs:label           "Software License";
        rdfs:range           ocsf:string_t;
        dcterms:description  "The name or identifier of the license applied on package or software. See <a target='_blank' href='https://spdx.org/licenses/'>SPDX License List</a>." .

ocsf:url_t  rdf:type         rdfs:Datatype;
        rdfs:label           "URL String";
        rdfs:subClassOf      xsd:string;
        dcterms:description  "Uniform Resource Locator (URL) string. For example: <code>http://www.example.com/download/trouble.exe</code>." .

ocsf:Container  rdf:type     owl:Class;
        rdfs:label           "Container";
        rdfs:subClassOf      ocsf:Object;
        rdfs:subClassOf      [ rdf:type            owl:Restriction;
                               owl:onProperty      ocsf:hash;
                               owl:someValuesFrom  ocsf:Fingerprint
                             ];
        rdfs:subClassOf      [ rdf:type            owl:Restriction;
                               owl:onProperty      ocsf:image;
                               owl:someValuesFrom  ocsf:Image
                             ];
        dcterms:description  "The Container object describes an instance of a specific container. A container is a prepackaged, portable system image that runs isolated on an existing system using a container runtime like containerd.";
        ocsf:constraints     "{\"at_least_one\":[\"uid\",\"name\"]}";
        ocsf:name            "container";
        ocsf:observable      27 .

ocsf:attempt  rdf:type       owl:DatatypeProperty;
        rdfs:label           "Attempt";
        rdfs:range           ocsf:integer_t;
        dcterms:description  "The delivery attempt." .

ocsf:logon_type  rdf:type    owl:DatatypeProperty;
        rdfs:label           "Logon Type";
        rdfs:range           ocsf:string_t;
        dcterms:description  "The logon type, normalized to the caption of the logon_type_id value. In the case of 'Other', it is defined by the event source." .

ocsf:runtime  rdf:type       owl:DatatypeProperty;
        rdfs:label           "Runtime";
        rdfs:range           ocsf:string_t;
        dcterms:description  "The backend running the container, such as containerd or cri-o." .

ocsf:chassis  rdf:type       owl:DatatypeProperty;
        rdfs:label           "Chassis";
        rdfs:range           ocsf:string_t;
        dcterms:description  "The chassis type describes the system enclosure or physical form factor. Such as the following examples for Windows <a target='_blank' href='https://docs.microsoft.com/en-us/windows/win32/cimwin32prov/win32-systemenclosure'>Windows Chassis Types</a>" .

ocsf:delivered_to  rdf:type  owl:DatatypeProperty;
        rdfs:label           "Delivered To";
        rdfs:range           ocsf:email_t;
        dcterms:description  "The <strong>Delivered-To</strong> email header field." .

ocsf:employee_uid  rdf:type  owl:DatatypeProperty;
        rdfs:label           "Employee ID";
        rdfs:range           ocsf:string_t;
        dcterms:description  "The employee identifier assigned to the user by the organization." .

ocsf:desktop_display  rdf:type  owl:ObjectProperty;
        rdfs:label           "Desktop Display";
        rdfs:range           ocsf:Display;
        dcterms:description  "The desktop display affiliated with the event" .

ocsf:function_name  rdf:type  owl:DatatypeProperty;
        rdfs:label           "Function Name";
        rdfs:range           ocsf:string_t;
        dcterms:description  "The entry-point function of the module. The system calls the entry-point function whenever a process or thread loads or unloads the module." .

ocsf:interface_name  rdf:type  owl:DatatypeProperty;
        rdfs:label           "Network Interface Name";
        rdfs:range           ocsf:string_t;
        dcterms:description  "The name of the network interface (e.g. eth2)." .

ocsf:OperatingSystemPatchStateEvent
        rdf:type             owl:Class;
        rdfs:label           "Operating System Patch State";
        rdfs:subClassOf      d3f:DigitalEvent;
        rdfs:subClassOf      [ rdf:type            owl:Restriction;
                               owl:onProperty      ocsf:kb_articles;
                               owl:someValuesFrom  ocsf:KBArticle
                             ];
        rdfs:subClassOf      [ rdf:type         owl:Restriction;
                               owl:cardinality  1;
                               owl:onProperty   ocsf:device
                             ];
        dcterms:description  "Operating System Patch State reports the installation of an OS patch.";
        ocsf:constraints     "{\"at_least_one\":[\"device.os.sp_name\",\"device.os.sp_ver\",\"device.os.version\"]}";
        ocsf:name            "patch_state";
        ocsf:profiles        "[\"host\"]";
        ocsf:uid             4 .

ocsf:version  rdf:type       owl:DatatypeProperty;
        rdfs:label           "Version";
        rdfs:range           ocsf:string_t;
        dcterms:description  "The version that pertains to the event or object. See specific usage." .

ocsf:client_hassh  rdf:type  owl:ObjectProperty;
        rdfs:label           "Client HASSH";
        rdfs:range           ocsf:HASSH;
        dcterms:description  "The Client HASSH fingerprinting object." .

ocsf:group_name  rdf:type    owl:DatatypeProperty;
        rdfs:label           "Group Name";
        rdfs:range           ocsf:string_t;
        dcterms:description  "The name of the group that the resource belongs to." .

ocsf:registrar  rdf:type     owl:DatatypeProperty;
        rdfs:label           "Domain Registrar";
        rdfs:range           ocsf:string_t;
        dcterms:description  "The domain registrar." .

ocsf:FindingInformation
        rdf:type             owl:Class;
        rdfs:label           "Finding Information";
        rdfs:subClassOf      ocsf:Object;
        rdfs:subClassOf      [ rdf:type            owl:Restriction;
                               owl:onProperty      ocsf:related_analytics;
                               owl:someValuesFrom  ocsf:Analytic
                             ];
        rdfs:subClassOf      [ rdf:type            owl:Restriction;
                               owl:onProperty      ocsf:related_events;
                               owl:someValuesFrom  ocsf:RelatedEvent
                             ];
        rdfs:subClassOf      [ rdf:type            owl:Restriction;
                               owl:onProperty      ocsf:analytic;
                               owl:someValuesFrom  ocsf:Analytic
                             ];
        rdfs:subClassOf      [ rdf:type            owl:Restriction;
                               owl:onProperty      ocsf:attacks;
                               owl:someValuesFrom  ocsf:MITREATTCK
                             ];
        rdfs:subClassOf      [ rdf:type            owl:Restriction;
                               owl:onProperty      ocsf:kill_chain;
                               owl:someValuesFrom  ocsf:KillChainPhase
                             ];
        dcterms:description  "The Finding Information object describes metadata related to a security finding generated by a security tool or system.";
        ocsf:name            "finding_info" .

ocsf:ja3_hash  rdf:type      owl:ObjectProperty;
        rdfs:label           "JA3 Hash";
        rdfs:range           ocsf:Fingerprint;
        dcterms:description  "The MD5 hash of a JA3 string." .

ocsf:ime  rdf:type           owl:DatatypeProperty;
        rdfs:label           "IME";
        rdfs:range           ocsf:string_t;
        dcterms:description  "The Input Method Editor (IME) file name." .

ocsf:DNS  rdf:type           owl:Class;
        rdfs:label           "DNS";
        rdfs:subClassOf      ocsf:Object;
        dcterms:description  "The Domain Name System (DNS) object represents the shared information associated with the DNS query and answer objects.";
        ocsf:name            "_dns" .

ocsf:api  rdf:type           owl:ObjectProperty;
        rdfs:label           "API Details";
        rdfs:range           ocsf:API;
        dcterms:description  "Describes details about a typical API (Application Programming Interface) call." .

ocsf:sp_ver  rdf:type        owl:DatatypeProperty;
        rdfs:label           "OS Service Pack Version";
        rdfs:range           ocsf:integer_t;
        dcterms:description  "The version number of the latest Service Pack." .

ocsf:phase_id  rdf:type      owl:DatatypeProperty;
        rdfs:label           "Kill Chain Phase ID";
        rdfs:range           ocsf:integer_t;
        dcterms:description  "The cyber kill chain phase identifier.";
        jsonschema:enum      "Command & Control" , "Delivery" , "Unknown" , "Actions on Objectives" , "Reconnaissance" , "Weaponization" , "Installation" , "Other" , "Exploitation" .

ocsf:network_interfaces
        rdf:type             owl:ObjectProperty;
        rdfs:label           "Network Interfaces";
        rdfs:range           ocsf:NetworkInterface;
        dcterms:description  "The network interfaces that are associated with the device, one for each unique MAC address/IP address/hostname/name combination.<p><b>Note:</b> The first element of the array is the network information that pertains to the event.</p>" .

ocsf:Metric  rdf:type        owl:Class;
        rdfs:label           "Metric";
        rdfs:subClassOf      ocsf:Object;
        dcterms:description  "The Metric object defines a simple name/value pair entity for a metric.";
        ocsf:name            "metric" .

ocsf:is_cleartext  rdf:type  owl:DatatypeProperty;
        rdfs:label           "Cleartext Credentials";
        rdfs:range           ocsf:boolean_t;
        dcterms:description  "Indicates whether the credentials were passed in clear text.<p><b>Note:</b> True if the credentials were passed in a clear text protocol such as FTP or TELNET, or if Windows detected that a user's logon password was passed to the authentication package in clear text.</p>" .

ocsf:protocol_ver  rdf:type  owl:DatatypeProperty;
        rdfs:label           "Protocol Version";
        rdfs:range           ocsf:string_t;
        dcterms:description  "The Protocol version, normalized to the caption of the protocol_ver_id value. In the case of 'Other', it is defined by the event source." .

ocsf:Policy  rdf:type        owl:Class;
        rdfs:label           "Policy";
        rdfs:subClassOf      ocsf:Entity;
        rdfs:subClassOf      [ rdf:type            owl:Restriction;
                               owl:onProperty      ocsf:group;
                               owl:someValuesFrom  ocsf:Group
                             ];
        dcterms:description  "The Policy object describes the policies that are applicable. <p>Policy attributes provide traceability to the operational state of the security product at the time that the event was captured, facilitating forensics, troubleshooting, and policy tuning/adjustments.</p>";
        ocsf:name            "policy" .

ocsf:process  rdf:type       owl:ObjectProperty;
        rdfs:label           "Process";
        rdfs:range           ocsf:Process;
        dcterms:description  "The process object." .

ocsf:lang  rdf:type          owl:DatatypeProperty;
        rdfs:label           "Language";
        rdfs:range           ocsf:string_t;
        dcterms:description  "The two letter lower case language codes, as defined by <a target='_blank' href='https://en.wikipedia.org/wiki/ISO_639-1'>ISO 639-1</a>. For example: <code>en</code> (English), <code>de</code> (German), or <code>fr</code> (French)." .

ocsf:user  rdf:type          owl:ObjectProperty;
        rdfs:label           "User";
        rdfs:range           ocsf:User;
        dcterms:description  "The user that pertains to the event or object." .

ocsf:ModuleInfoEvent  rdf:type  owl:Class;
        rdfs:label           "Module Info";
        rdfs:subClassOf      d3f:DigitalEvent;
        rdfs:subClassOf      [ rdf:type         owl:Restriction;
                               owl:cardinality  1;
                               owl:onProperty   ocsf:process
                             ];
        rdfs:subClassOf      [ rdf:type         owl:Restriction;
                               owl:cardinality  1;
                               owl:onProperty   ocsf:module
                             ];
        dcterms:description  "Module Info events report information about loaded modules.";
        ocsf:name            "module_info";
        ocsf:uid             11 .

ocsf:data_sources  rdf:type  owl:DatatypeProperty;
        rdfs:label           "Data Sources";
        rdfs:range           ocsf:string_t;
        dcterms:description  "A list of data sources utilized in generation of the finding." .

ocsf:mac  rdf:type           owl:DatatypeProperty;
        rdfs:label           "MAC Address";
        rdfs:range           ocsf:mac_t;
        dcterms:description  "The Media Access Control (MAC) address that is associated with the network interface." .

ocsf:edition  rdf:type       owl:DatatypeProperty;
        rdfs:label           "OS Edition";
        rdfs:range           ocsf:string_t;
        dcterms:description  "The operating system edition. For example: <code>Professional</code>." .

ocsf:ldap_dn  rdf:type       owl:DatatypeProperty;
        rdfs:label           "LDAP Distinguished Name";
        rdfs:range           ocsf:string_t;
        dcterms:description  "The X.500 Distinguished Name (DN) is a structured string that uniquely identifies an entry, such as a user, in an X.500 directory service For example, <code>cn=John Doe,ou=People,dc=example,dc=com</code>." .

ocsf:vulnerability  rdf:type  owl:ObjectProperty;
        rdfs:label           "Vulnerability";
        rdfs:range           ocsf:VulnerabilityDetails;
        dcterms:description  "The vulnerability object describes details related to the observed vulnerability" .

ocsf:ou_name  rdf:type       owl:DatatypeProperty;
        rdfs:label           "Org Unit Name";
        rdfs:range           ocsf:string_t;
        dcterms:description  "The name of the organizational unit, within an organization.  For example, Finance, IT, R&D" .

ocsf:key_length  rdf:type    owl:DatatypeProperty;
        rdfs:label           "Key Length";
        rdfs:range           ocsf:integer_t;
        dcterms:description  "The length of the encryption key." .

ocsf:original_time  rdf:type  owl:DatatypeProperty;
        rdfs:label           "Original Time";
        rdfs:range           ocsf:string_t;
        dcterms:description  "The original event time as reported by the event source. For example, the time in the original format from system event log such as Syslog on Unix/Linux and the System event file on Windows. Omit if event is generated instead of collected via logs." .

ocsf:standards  rdf:type     owl:DatatypeProperty;
        rdfs:label           "Security Standards";
        rdfs:range           ocsf:string_t;
        dcterms:description  "Security standards are a set of criteria organizations can follow to protect sensitive and confidential information. e.g. <code>NIST SP 800-53, CIS AWS Foundations Benchmark v1.4.0, ISO/IEC 27001</code>" .

ocsf:Session  rdf:type       owl:Class;
        rdfs:label           "Session";
        rdfs:subClassOf      ocsf:Object;
        dcterms:description  "The Session object describes details about an authenticated session. e.g. Session Creation Time, Session Issuer. Defined by D3FEND <a target='_blank' href='https://d3fend.mitre.org/dao/artifact/d3f:Session/'>d3f:Session</a>.";
        ocsf:name            "session" .

ocsf:risk_level_id  rdf:type  owl:DatatypeProperty;
        rdfs:label           "Risk Level ID";
        rdfs:range           ocsf:integer_t;
        dcterms:description  "The normalized risk level id.";
        jsonschema:enum      "Critical" , "High" , "Medium" , "Low" , "Info" .

ocsf:transaction_uid  rdf:type  owl:DatatypeProperty;
        rdfs:label           "Transaction UID";
        rdfs:range           ocsf:string_t;
        dcterms:description  "The unique identifier of the transaction." .

ocsf:comment  rdf:type       owl:DatatypeProperty;
        rdfs:label           "Comment";
        rdfs:range           ocsf:string_t;
        dcterms:description  "The user-provided comment." .

ocsf:entity_result  rdf:type  owl:ObjectProperty;
        rdfs:label           "Entity Result";
        rdfs:range           ocsf:ManagedEntity;
        dcterms:description  "The updated managed entity." .

ocsf:code  rdf:type          owl:DatatypeProperty;
        rdfs:label           "Response Code";
        rdfs:range           ocsf:integer_t;
        dcterms:description  "The numeric response sent to a request." .

ocsf:cipher  rdf:type        owl:DatatypeProperty;
        rdfs:label           "Cipher Suite";
        rdfs:range           ocsf:string_t;
        dcterms:description  "The negotiated cipher suite." .

ocsf:database  rdf:type      owl:ObjectProperty;
        rdfs:label           "Database";
        dcterms:description  "The database object is used for databases which are typically datastore services that contain an organized collection of structured and unstructured data or a types of data." .

ocsf:confidence_id  rdf:type  owl:DatatypeProperty;
        rdfs:label           "Confidence Id";
        rdfs:range           ocsf:integer_t;
        dcterms:description  "The normalized confidence refers to the accuracy of the rule that created the finding. A rule with a low confidence means that the finding scope is wide and may create finding reports that may not be malicious in nature.";
        jsonschema:enum      "Other" , "High" , "Medium" , "Low" , "Unknown" .

ocsf:tag  rdf:type           owl:DatatypeProperty;
        rdfs:label           "Image Tag";
        rdfs:range           ocsf:string_t;
        dcterms:description  "The image tag. For example: <code>1.11-alpine</code>." .

ocsf:entity  rdf:type        owl:ObjectProperty;
        rdfs:label           "Entity";
        rdfs:range           ocsf:ManagedEntity;
        dcterms:description  "The managed entity that is being acted upon." .

ocsf:table  rdf:type         owl:ObjectProperty;
        rdfs:label           "Table";
        dcterms:description  "The table object represents a table within a structured relational database or datastore, which contains columns and rows of data that are able to be create, updated, deleted and queried." .

ocsf:Job  rdf:type           owl:Class;
        rdfs:label           "Job";
        rdfs:subClassOf      ocsf:Object;
        rdfs:subClassOf      [ rdf:type            owl:Restriction;
                               owl:onProperty      ocsf:user;
                               owl:someValuesFrom  ocsf:User
                             ];
        rdfs:subClassOf      [ rdf:type         owl:Restriction;
                               owl:cardinality  1;
                               owl:onProperty   ocsf:file
                             ];
        dcterms:description  "The Job object provides information about a scheduled job or task, including its name, command line, and state. It encompasses attributes that describe the properties and status of the scheduled job.";
        ocsf:name            "job" .

ocsf:priority  rdf:type      owl:DatatypeProperty;
        rdfs:label           "Priority";
        rdfs:range           ocsf:integer_t;
        dcterms:description  "The priority, normalized to the caption of the priority_id value. In the case of 'Other', it is defined by the event source. See specific usage." .

ocsf:sans  rdf:type          owl:ObjectProperty;
        rdfs:label           "Subject Alternative Names";
        rdfs:range           ocsf:SubjectAlternativeName;
        dcterms:description  "The list of subject alternative names that are secured by a specific certificate." .

ocsf:smtp_hello  rdf:type    owl:DatatypeProperty;
        rdfs:label           "SMTP Hello";
        rdfs:range           ocsf:string_t;
        dcterms:description  "The value of the SMTP HELO or EHLO command." .

ocsf:Fingerprint  rdf:type   owl:Class;
        rdfs:label           "Fingerprint";
        rdfs:subClassOf      ocsf:Object;
        dcterms:description  "The Fingerprint object provides detailed information about a digital fingerprint, which is a compact representation of data used to identify a longer piece of information, such as a public key or file content. It contains the algorithm and value of the fingerprint, enabling efficient and reliable identification of the associated data.";
        ocsf:name            "fingerprint";
        ocsf:observable      30 .

ocsf:NetworkInterface
        rdf:type             owl:Class;
        rdfs:label           "Network Interface";
        rdfs:subClassOf      ocsf:Entity;
        dcterms:description  "The Network Interface object describes the type and associated attributes of a network interface.";
        ocsf:constraints     "{\"at_least_one\":[\"ip\",\"mac\",\"name\",\"hostname\"]}";
        ocsf:name            "network_interface" .

ocsf:category_name  rdf:type  owl:DatatypeProperty;
        rdfs:label           "Category";
        rdfs:range           ocsf:string_t;
        dcterms:description  "The event category name, as defined by category_uid value." .

ocsf:Technique  rdf:type     owl:Class;
        rdfs:label           "Technique";
        rdfs:subClassOf      ocsf:Entity;
        dcterms:description  "The Technique object describes the technique ID and/or name associated to an attack, as defined by <a target='_blank' href='https://attack.mitre.org/wiki/ATT&CK_Matrix'>ATT&CK Matrix<sup>TM</sup></a>.";
        ocsf:name            "technique" .

ocsf:cpu_count  rdf:type     owl:DatatypeProperty;
        rdfs:label           "CPU Count";
        rdfs:range           ocsf:integer_t;
        dcterms:description  "The number of physical processors on a system. For example: <code>1</code>." .

ocsf:company_name  rdf:type  owl:DatatypeProperty;
        rdfs:label           "Company Name";
        rdfs:range           ocsf:string_t;
        dcterms:description  "The name of the company that published the file. For example: <code>Microsoft Corporation</code>." .

ocsf:email  rdf:type         owl:ObjectProperty;
        rdfs:label           "Email";
        rdfs:range           ocsf:Email;
        dcterms:description  "The email object." .

ocsf:resources_result
        rdf:type             owl:ObjectProperty;
        rdfs:label           "Resource Results Array";
        rdfs:range           ocsf:ResourceDetails;
        dcterms:description  "Updated resources after an activity/event." .

ocsf:proxy_http_request
        rdf:type             owl:ObjectProperty;
        rdfs:label           "Proxy HTTP Request";
        rdfs:range           ocsf:HTTPRequest;
        dcterms:description  "The HTTP Request from the proxy server to the remote server." .

ocsf:is_renewal  rdf:type    owl:DatatypeProperty;
        rdfs:label           "Renewal";
        rdfs:range           ocsf:boolean_t;
        dcterms:description  "The indication of whether this is a lease/session renewal event." .

ocsf:protocol_num  rdf:type  owl:DatatypeProperty;
        rdfs:label           "Protocol Number";
        rdfs:range           ocsf:integer_t;
        dcterms:description  "The TCP/IP protocol number, as defined by the Internet Assigned Numbers Authority (IANA). Use -1 if the protocol is not defined by IANA. See <a target='_blank' href='https://www.iana.org/assignments/protocol-numbers/protocol-numbers.xhtml'>Protocol Numbers</a>. For example: <code>6</code> for TCP and <code>17</code> for UDP." .

ocsf:attacks  rdf:type       owl:ObjectProperty;
        rdfs:label           "MITRE ATT&CK® Details";
        rdfs:range           ocsf:MITREATTCK;
        dcterms:description  "An array of <a target='_blank' href='https://attack.mitre.org'>MITRE ATT&CK®</a> objects describing the tactics, techniques & sub-techniques identified by a security control or finding." .

ocsf:email_t  rdf:type       rdfs:Datatype;
        rdfs:label           "Email Address";
        rdfs:subClassOf      xsd:string;
        dcterms:description  "Email address. For example: <code>john_doe@example.com</code>.";
        xsd:pattern          "^[a-zA-Z0-9_.+-]+@[a-zA-Z0-9-]+\\.[a-zA-Z0-9-.]+$" .

ocsf:labels  rdf:type        owl:DatatypeProperty;
        rdfs:label           "Labels";
        rdfs:range           ocsf:string_t;
        dcterms:description  "The list of labels attached to an event, object, or attribute." .

ocsf:ComplianceFindingEvent
        rdf:type             owl:Class;
        rdfs:label           "Compliance Finding";
        rdfs:subClassOf      ocsf:Finding , d3f:DigitalEvent;
        rdfs:subClassOf      [ rdf:type            owl:Restriction;
                               owl:onProperty      ocsf:remediation;
                               owl:someValuesFrom  ocsf:Remediation
                             ];
        rdfs:subClassOf      [ rdf:type         owl:Restriction;
                               owl:cardinality  1;
                               owl:onProperty   ocsf:compliance
                             ];
        rdfs:subClassOf      [ rdf:type            owl:Restriction;
                               owl:onProperty      ocsf:resource;
                               owl:someValuesFrom  ocsf:ResourceDetails
                             ];
        dcterms:description  "Compliance Finding events describe results of evaluations performed against resources, to check compliance with various Industry Frameworks or Security Standards such as <code>NIST SP 800-53, CIS AWS Foundations Benchmark v1.4.0, ISO/IEC 27001</code> etc.";
        ocsf:category        "findings";
        ocsf:name            "compliance_finding";
        ocsf:uid             3 .

ocsf:ldap_person  rdf:type   owl:ObjectProperty;
        rdfs:label           "LDAP Person";
        rdfs:range           ocsf:LDAPPerson;
        dcterms:description  "The additonal LDAP attributes that describe a person." .

ocsf:FTPActivityEvent
        rdf:type             owl:Class;
        rdfs:label           "FTP Activity";
        rdfs:subClassOf      d3f:DigitalEvent;
        dcterms:description  "File Transfer Protocol (FTP) Activity events report file transfers between a server and a client as seen on the network.";
        ocsf:name            "ftp_activity";
        ocsf:uid             8 .

ocsf:email_addrs  rdf:type   owl:DatatypeProperty;
        rdfs:label           "Email Addresses";
        rdfs:range           ocsf:email_t;
        dcterms:description  "A list of additional email addresses for the user." .

ocsf:cpu_bits  rdf:type      owl:DatatypeProperty;
        rdfs:label           "CPU Bits";
        rdfs:range           ocsf:integer_t;
        dcterms:description  "The cpu architecture, the number of bits used for addressing in memory. For example: <code>32</code> or <code>64</code>." .

ocsf:extension_list  rdf:type  owl:ObjectProperty;
        rdfs:label           "Extension List";
        rdfs:range           ocsf:TLSExtension;
        dcterms:description  "The list of TLS extensions." .

ocsf:unmapped  rdf:type      owl:ObjectProperty;
        rdfs:label           "Unmapped Data";
        rdfs:range           ocsf:Object;
        dcterms:description  "The attributes that are not mapped to the event schema. The names and values of those attributes are specific to the event source." .

ocsf:is_trusted  rdf:type    owl:DatatypeProperty;
        rdfs:label           "Trusted Device";
        rdfs:range           ocsf:boolean_t;
        dcterms:description  "The event occurred on a trusted device." .

ocsf:FileSystemActivityEvent
        rdf:type             owl:Class;
        rdfs:label           "File System Activity";
        rdfs:subClassOf      d3f:DigitalEvent;
        rdfs:subClassOf      [ rdf:type            owl:Restriction;
                               owl:onProperty      ocsf:file_result;
                               owl:someValuesFrom  ocsf:File
                             ];
        rdfs:subClassOf      [ rdf:type         owl:Restriction;
                               owl:cardinality  1;
                               owl:onProperty   ocsf:file
                             ];
        rdfs:subClassOf      [ rdf:type         owl:Restriction;
                               owl:cardinality  1;
                               owl:onProperty   ocsf:actor
                             ];
        dcterms:description  "File System Activity events report when a process performs an action on a file or folder.";
        ocsf:name            "file_activity";
        ocsf:uid             1 .

ocsf:fingerprints  rdf:type  owl:ObjectProperty;
        rdfs:label           "Fingerprints";
        rdfs:range           ocsf:Fingerprint;
        dcterms:description  "An array of digital fingerprint objects." .

ocsf:epoch  rdf:type         owl:DatatypeProperty;
        rdfs:label           "Epoch";
        rdfs:range           ocsf:integer_t;
        dcterms:description  "The software package epoch. Epoch is a way to define weighted dependencies based on version numbers." .

ocsf:error  rdf:type         owl:DatatypeProperty;
        rdfs:label           "Error Code";
        rdfs:range           ocsf:string_t;
        dcterms:description  "Error Code" .

ocsf:JobInfoEvent  rdf:type  owl:Class;
        rdfs:label           "Job Info";
        rdfs:subClassOf      d3f:DigitalEvent;
        rdfs:subClassOf      [ rdf:type         owl:Restriction;
                               owl:cardinality  1;
                               owl:onProperty   ocsf:job
                             ];
        dcterms:description  "Job Info events report information about scheduled jobs.";
        ocsf:name            "job_info";
        ocsf:uid             10 .

ocsf:ResponseElements
        rdf:type             owl:Class;
        rdfs:label           "Response Elements";
        rdfs:subClassOf      ocsf:Object;
        rdfs:subClassOf      [ rdf:type            owl:Restriction;
                               owl:onProperty      ocsf:containers;
                               owl:someValuesFrom  ocsf:Container
                             ];
        dcterms:description  "The Response Elements object describes characteristics of an API response.";
        ocsf:name            "response" .

ocsf:username_t  rdf:type    rdfs:Datatype;
        rdfs:label           "User Name";
        rdfs:subClassOf      xsd:string;
        dcterms:description  "User name. For example: <code>john_doe</code>." .

ocsf:smtp_to  rdf:type       owl:DatatypeProperty;
        rdfs:label           "SMTP To";
        rdfs:range           ocsf:email_t;
        dcterms:description  "The value of the SMTP envelope RCPT TO command." .

ocsf:base_score  rdf:type    owl:DatatypeProperty;
        rdfs:label           "Base Score";
        rdfs:range           ocsf:float_t;
        dcterms:description  "The base score as reported by the event source. See specific usage." .

ocsf:component  rdf:type     owl:DatatypeProperty;
        rdfs:label           "Component";
        rdfs:range           ocsf:string_t;
        dcterms:description  "<p>The name or relative pathname of a sub-component of the data object, if applicable. </p>For example: <code>attachment.doc</code>, <code>attachment.zip/bad.doc</code>, or <code>part.mime/part.cab/part.uue/part.doc</code>." .

ocsf:driver  rdf:type        owl:ObjectProperty;
        rdfs:label           "Kernel Driver";
        rdfs:range           ocsf:KernelExtension;
        dcterms:description  "The driver that was loaded/unloaded into the kernel" .

ocsf:country  rdf:type       owl:DatatypeProperty;
        rdfs:label           "Country";
        rdfs:range           ocsf:string_t;
        dcterms:description  "The ISO 3166-1 Alpha-2 country code. For the complete list of country codes see <a target='_blank' href='https://www.iso.org/obp/ui/#iso:pub:PUB500001:en' >ISO 3166-1 alpha-2 codes</a>.<p><b>Note:</b> The two letter country code should be capitalized. For example: <code>US</code> or <code>CA</code>.</p>" .

ocsf:created_time  rdf:type  owl:DatatypeProperty;
        rdfs:label           "Created Time";
        rdfs:range           ocsf:timestamp_t;
        dcterms:description  "The time when the object was created. See specific usage." .

ocsf:NetworkProxyEndpoint
        rdf:type             owl:Class;
        rdfs:label           "Network Proxy Endpoint";
        rdfs:subClassOf      ocsf:NetworkEndpoint;
        dcterms:description  "The network proxy endpoint object describes a proxy server, which acts as an intermediary between a client requesting a resource and the server providing that resource.  Defined by D3FEND <a target='_blank' href='https://d3fend.mitre.org/dao/artifact/d3f:ProxyServer/'>d3f:ProxyServer</a>.";
        ocsf:name            "network_proxy" .

ocsf:alert  rdf:type         owl:DatatypeProperty;
        rdfs:label           "Client TLS Alert";
        rdfs:range           ocsf:integer_t;
        dcterms:description  "The integer value of TLS alert if present. The alerts are defined in the TLS specification in <a target='_blank' href='https://datatracker.ietf.org/doc/html/rfc2246'>RFC-2246</a>." .

ocsf:container  rdf:type     owl:ObjectProperty;
        rdfs:label           "Container";
        rdfs:range           ocsf:Container;
        dcterms:description  "The information describing an instance of a container. A container is a prepackaged, portable system image that runs isolated on an existing system using a container runtime like containerd." .

ocsf:DeviceConfigStateEvent
        rdf:type             owl:Class;
        rdfs:label           "Device Config State";
        rdfs:subClassOf      d3f:DigitalEvent;
        rdfs:subClassOf      [ rdf:type         owl:Restriction;
                               owl:cardinality  1;
                               owl:onProperty   ocsf:device
                             ];
        rdfs:subClassOf      [ rdf:type            owl:Restriction;
                               owl:onProperty      ocsf:actor;
                               owl:someValuesFrom  ocsf:Actor
                             ];
        rdfs:subClassOf      [ rdf:type            owl:Restriction;
                               owl:onProperty      ocsf:cis_benchmark_result;
                               owl:someValuesFrom  ocsf:CISBenchmarkResult
                             ];
        dcterms:description  "Device Config State events report device configuration data.";
        ocsf:name            "config_state";
        ocsf:profiles        "[\"host\"]";
        ocsf:uid             2 .

ocsf:is_new_logon  rdf:type  owl:DatatypeProperty;
        rdfs:label           "New Logon";
        rdfs:range           ocsf:boolean_t;
        dcterms:description  "Indicates logon is from a device not seen before or a first time account logon." .

ocsf:disposition  rdf:type   owl:DatatypeProperty;
        rdfs:label           "Disposition";
        rdfs:range           ocsf:string_t;
        dcterms:description  "The disposition name, normalized to the caption of the disposition_id value. In the case of 'Other', it is defined by the event source." .

ocsf:policy  rdf:type        owl:ObjectProperty;
        rdfs:label           "Policy";
        rdfs:range           ocsf:Policy;
        dcterms:description  "Describes details of a policy. See specific usage." .

ocsf:protocol_ver_id  rdf:type  owl:DatatypeProperty;
        rdfs:label           "Protocol Version ID";
        rdfs:range           ocsf:integer_t;
        dcterms:description  "The normalized identifier of the Protocol version." .

ocsf:FolderInfoEvent  rdf:type  owl:Class;
        rdfs:label           "Folder Info";
        rdfs:subClassOf      d3f:DigitalEvent;
        rdfs:subClassOf      [ rdf:type         owl:Restriction;
                               owl:cardinality  1;
                               owl:onProperty   ocsf:folder
                             ];
        dcterms:description  "Folder Info events report information about folders that are present on the system.";
        ocsf:name            "folder_info";
        ocsf:uid             8 .

ocsf:flags  rdf:type         owl:DatatypeProperty;
        rdfs:label           "Flags";
        rdfs:range           ocsf:string_t;
        dcterms:description  "The list of communication flags, normalized to the captions of the flag_ids values. In the case of 'Other', they are defined by the event source." .

ocsf:Email  rdf:type         owl:Class;
        rdfs:label           "Email";
        rdfs:subClassOf      ocsf:Object;
        dcterms:description  "The Email object describes the email metadata such as sender, recipients, and direction. Defined by D3FEND <a target='_blank' href='https://d3fend.mitre.org/dao/artifact/d3f:Email/'>d3f:Email</a>.";
        ocsf:name            "email";
        ocsf:observable      22 .

ocsf:requirements  rdf:type  owl:DatatypeProperty;
        rdfs:label           "Compliance Requirements";
        rdfs:range           ocsf:string_t;
        dcterms:description  "A list of requirements associated to a specific control in an industry or regulatory framework. e.g. <code> NIST.800-53.r5 AU-10 </code>" .

ocsf:float_t  rdf:type       rdfs:Datatype;
        rdfs:label           "Float";
        rdfs:subClassOf      xsd:decimal;
        dcterms:description  "Real floating-point value. For example: <code>3.14</code>." .

ocsf:orchestrator  rdf:type  owl:DatatypeProperty;
        rdfs:label           "Orchestrator";
        rdfs:range           ocsf:string_t;
        dcterms:description  "The orchestrator managing the container, such as ECS, EKS, K8s, or OpenShift." .

ocsf:observables  rdf:type   owl:ObjectProperty;
        rdfs:label           "Observables";
        rdfs:range           ocsf:Observable;
        dcterms:description  "The observables associated with the event or a finding." .

ocsf:instance_uid  rdf:type  owl:DatatypeProperty;
        rdfs:label           "Instance ID";
        rdfs:range           ocsf:string_t;
        dcterms:description  "The unique identifier of a VM instance." .

ocsf:raw_header  rdf:type    owl:DatatypeProperty;
        rdfs:label           "Raw Header";
        rdfs:range           ocsf:string_t;
        dcterms:description  "The email authentication header." .

ocsf:namespace_pid  rdf:type  owl:DatatypeProperty;
        rdfs:label           "Namespace PID";
        rdfs:range           ocsf:integer_t;
        dcterms:description  "If running under a process namespace (such as in a container), the process identifier within that process namespace." .

ocsf:create_mask  rdf:type   owl:DatatypeProperty;
        rdfs:label           "Create Mask";
        rdfs:range           ocsf:string_t;
        dcterms:description  "The original Windows mask that is required to create the object." .

ocsf:types  rdf:type         owl:DatatypeProperty;
        rdfs:label           "Types";
        rdfs:range           ocsf:string_t;
        dcterms:description  "The type/s of an entity. See specific usage." .

ocsf:function_keys  rdf:type  owl:DatatypeProperty;
        rdfs:label           "Function Keys";
        rdfs:range           ocsf:integer_t;
        dcterms:description  "The number of function keys on client keyboard." .

ocsf:Enrichment  rdf:type    owl:Class;
        rdfs:label           "Enrichment";
        rdfs:subClassOf      ocsf:Object;
        dcterms:description  "The Enrichment object provides inline enrichment data for specific attributes of interest within an event. It serves as a mechanism to enhance or supplement the information associated with the event by adding additional relevant details or context.";
        ocsf:name            "enrichment" .

ocsf:args  rdf:type          owl:DatatypeProperty;
        rdfs:label           "HTTP Arguments";
        rdfs:range           ocsf:string_t;
        dcterms:description  "The arguments sent along with the HTTP request." .

ocsf:subnet_uid  rdf:type    owl:DatatypeProperty;
        rdfs:label           "Subnet UID";
        rdfs:range           ocsf:string_t;
        dcterms:description  "The unique identifier of a virtual subnet." .

ocsf:uuid  rdf:type          owl:DatatypeProperty;
        rdfs:label           "UUID";
        rdfs:range           ocsf:uuid_t;
        dcterms:description  "The universally unique identifier. See specific usage." .

ocsf:classification_ids
        rdf:type             owl:DatatypeProperty;
        rdfs:label           "Classification IDs";
        rdfs:range           ocsf:integer_t;
        dcterms:description  "The list of normalized identifiers of the malware classifications. Reference: <a target='_blank' href='https://docs.oasis-open.org/cti/stix/v2.1/os/stix-v2.1-os.html#_oxlc4df65spl'>STIX Malware Types</a> " .

ocsf:class_uid  rdf:type     owl:DatatypeProperty;
        rdfs:label           "Class ID";
        rdfs:range           ocsf:integer_t;
        dcterms:description  "The unique identifier of a class. A Class describes the attributes available in an event." .

ocsf:impact_score  rdf:type  owl:DatatypeProperty;
        rdfs:label           "Impact";
        rdfs:range           ocsf:integer_t;
        dcterms:description  "The impact of the finding, valid range 0-100." .

ocsf:flag_ids  rdf:type      owl:DatatypeProperty;
        rdfs:label           "Communication Flag IDs";
        rdfs:range           ocsf:integer_t;
        dcterms:description  "The list of normalized identifiers of the communication flag IDs." .

ocsf:banner  rdf:type        owl:DatatypeProperty;
        rdfs:label           "SMTP Banner";
        rdfs:range           ocsf:string_t;
        dcterms:description  "The initial SMTP connection response that a messaging server receives after it connects to a email server." .

ocsf:affected_packages
        rdf:type             owl:ObjectProperty;
        rdfs:label           "Affected Software Packages";
        rdfs:range           ocsf:AffectedSoftwarePackage;
        dcterms:description  "List of software packages identified as affected by a vulnerability/vulnerabilities." .

ocsf:connection_uid  rdf:type  owl:DatatypeProperty;
        rdfs:label           "Connection Identifier";
        rdfs:range           ocsf:string_t;
        dcterms:description  "The network connection identifier." .

ocsf:logon_process  rdf:type  owl:ObjectProperty;
        rdfs:label           "Logon Process";
        rdfs:range           ocsf:Process;
        dcterms:description  "The trusted process that validated the authentication credentials." .

ocsf:samesite  rdf:type      owl:DatatypeProperty;
        rdfs:label           "SameSite";
        rdfs:range           ocsf:string_t;
        dcterms:description  "The cookie attribute that lets servers specify whether/when cookies are sent with cross-site requests. Values are: Strict, Lax or None" .

ocsf:answers  rdf:type       owl:ObjectProperty;
        rdfs:label           "DNS Answer";
        rdfs:range           ocsf:DNSAnswer;
        dcterms:description  "The Domain Name System (DNS) answers." .

ocsf:physical_orientation
        rdf:type             owl:DatatypeProperty;
        rdfs:label           "Physical Orientation";
        rdfs:range           ocsf:integer_t;
        dcterms:description  "The numeric physical orientation of display." .

ocsf:product  rdf:type       owl:ObjectProperty;
        rdfs:label           "Product";
        rdfs:range           ocsf:Product;
        dcterms:description  "The product that reported the event." .

ocsf:hypervisor  rdf:type    owl:DatatypeProperty;
        rdfs:label           "Hypervisor";
        rdfs:range           ocsf:string_t;
        dcterms:description  "The name of the hypervisor running on the device. For example, <code>Xen</code>, <code>VMware</code>, <code>Hyper-V</code>, <code>VirtualBox</code>, etc." .

ocsf:SchemaExtension  rdf:type  owl:Class;
        rdfs:label           "Schema Extension";
        rdfs:subClassOf      ocsf:Entity;
        dcterms:description  "The OCSF Schema Extension object provides detailed information about the schema extension used to construct the event. The schema extensions are registered in the <a target='_blank' href='https://github.com/ocsf/ocsf-schema/blob/main/extensions.md'>extensions.md</a> file.";
        ocsf:constraints     "{}";
        ocsf:name            "extension" .

ocsf:share  rdf:type         owl:DatatypeProperty;
        rdfs:label           "Share";
        rdfs:range           ocsf:string_t;
        dcterms:description  "The SMB share name." .

ocsf:VulnerabilityFindingEvent
        rdf:type             owl:Class;
        rdfs:label           "Vulnerability Finding";
        rdfs:subClassOf      d3f:DigitalEvent , ocsf:Finding;
        rdfs:subClassOf      [ rdf:type            owl:Restriction;
                               owl:onProperty      ocsf:device;
                               owl:someValuesFrom  ocsf:Device
                             ];
        rdfs:subClassOf      [ rdf:type         owl:Restriction;
                               owl:cardinality  1;
                               owl:onProperty   ocsf:vulnerabilities
                             ];
        rdfs:subClassOf      [ rdf:type            owl:Restriction;
                               owl:onProperty      ocsf:resource;
                               owl:someValuesFrom  ocsf:ResourceDetails
                             ];
        dcterms:description  "The Vulnerability Finding event is a notification about weakness in an information system, system security procedures, internal controls, or implementation that could be exploited or triggered by a threat source.";
        ocsf:name            "vulnerability_finding";
        ocsf:uid             2 .

ocsf:MITREATTCK  rdf:type    owl:Class;
        rdfs:label           "MITRE ATT&CK®";
        rdfs:subClassOf      ocsf:Object;
        rdfs:subClassOf      [ rdf:type            owl:Restriction;
                               owl:onProperty      ocsf:tactics;
                               owl:someValuesFrom  ocsf:Tactic
                             ];
        rdfs:subClassOf      [ rdf:type            owl:Restriction;
                               owl:onProperty      ocsf:technique;
                               owl:someValuesFrom  ocsf:Technique
                             ];
        rdfs:subClassOf      [ rdf:type            owl:Restriction;
                               owl:onProperty      ocsf:sub_technique;
                               owl:someValuesFrom  ocsf:SubTechnique
                             ];
        rdfs:subClassOf      [ rdf:type            owl:Restriction;
                               owl:onProperty      ocsf:tactic;
                               owl:someValuesFrom  ocsf:Tactic
                             ];
        dcterms:description  "The <a target='_blank' href='https://attack.mitre.org'>MITRE ATT&CK®</a> object describes the tactic, technique & sub-technique associated to an attack as defined in <a target='_blank' href='https://attack.mitre.org/wiki/ATT&CK_Matrix'>ATT&CK Matrix<sup>TM</sup></a>.";
        ocsf:constraints     "{\"at_least_one\":[\"tactic\",\"technique\",\"sub_technique\"]}";
        ocsf:name            "attack" .

ocsf:Analytic  rdf:type      owl:Class;
        rdfs:label           "Analytic";
        rdfs:subClassOf      ocsf:Entity;
        rdfs:subClassOf      [ rdf:type            owl:Restriction;
                               owl:onProperty      ocsf:related_analytics;
                               owl:someValuesFrom  ocsf:Analytic
                             ];
        dcterms:description  "The Analytic object contains details about the analytic technique used to analyze and derive insights from the data or information that led to the creation of a finding or conclusion.";
        ocsf:name            "analytic" .

ocsf:x_originating_ip
        rdf:type             owl:DatatypeProperty;
        rdfs:label           "X-Originating-IP";
        rdfs:range           ocsf:ip_t;
        dcterms:description  "The X-Originating-IP header identifying the emails originating IP address(es)." .

ocsf:EntityManagementEvent
        rdf:type             owl:Class;
        rdfs:label           "Entity Management";
        rdfs:subClassOf      d3f:DigitalEvent;
        rdfs:subClassOf      [ rdf:type            owl:Restriction;
                               owl:onProperty      ocsf:entity_result;
                               owl:someValuesFrom  ocsf:ManagedEntity
                             ];
        rdfs:subClassOf      [ rdf:type         owl:Restriction;
                               owl:cardinality  1;
                               owl:onProperty   ocsf:entity
                             ];
        rdfs:subClassOf      [ rdf:type            owl:Restriction;
                               owl:onProperty      ocsf:actor;
                               owl:someValuesFrom  ocsf:Actor
                             ];
        dcterms:description  "Entity Management events report activity by a managed client, a micro service, or a user at a management console. The activity can be a create, read, update, and delete operation on a managed entity.";
        ocsf:name            "entity_management";
        ocsf:uid             4 .

ocsf:direction  rdf:type     owl:DatatypeProperty;
        rdfs:label           "Direction";
        rdfs:range           ocsf:string_t;
        dcterms:description  "The direction of the initiated connection, traffic, or email, normalized to the caption of the direction_id value. In the case of 'Other', it is defined by the event source." .

ocsf:score  rdf:type         owl:DatatypeProperty;
        rdfs:label           "Reputation Score";
        rdfs:range           ocsf:string_t;
        dcterms:description  "The reputation score, normalized to the caption of the score_id value. In the case of 'Other', it is defined by the event source." .

ocsf:HTTPCookie  rdf:type    owl:Class;
        rdfs:label           "HTTP Cookie";
        rdfs:subClassOf      ocsf:Object;
        dcterms:description  "The HTTP Cookie object, also known as a web cookie or browser cookie, contains details and values pertaining to a small piece of data that a server sends to a user's web browser. This data is then stored by the browser and sent back to the server with subsequent requests, allowing the server to remember and track certain information about the user's browsing session or preferences.";
        ocsf:name            "http_cookie" .

ocsf:mime_type  rdf:type     owl:DatatypeProperty;
        rdfs:label           "MIME type";
        rdfs:range           ocsf:string_t;
        dcterms:description  "The Multipurpose Internet Mail Extensions (MIME) type of the file, if applicable." .

ocsf:serial_number  rdf:type  owl:DatatypeProperty;
        rdfs:label           "Serial Number";
        rdfs:range           ocsf:string_t;
        dcterms:description  "The serial number that pertains to the object. See specific usage." .

ocsf:   rdf:type     owl:Ontology;
        owl:imports  <http://d3fend.mitre.org/ontologies/d3fend.owl> .

ocsf:AuthorizeSessionEvent
        rdf:type             owl:Class;
        rdfs:label           "Authorize Session";
        rdfs:subClassOf      d3f:DigitalEvent;
        rdfs:subClassOf      [ rdf:type            owl:Restriction;
                               owl:onProperty      ocsf:group;
                               owl:someValuesFrom  ocsf:Group
                             ];
        rdfs:subClassOf      [ rdf:type            owl:Restriction;
                               owl:onProperty      ocsf:session;
                               owl:someValuesFrom  ocsf:Session
                             ];
        rdfs:subClassOf      [ rdf:type            owl:Restriction;
                               owl:onProperty      ocsf:dst_endpoint;
                               owl:someValuesFrom  ocsf:NetworkEndpoint
                             ];
        rdfs:subClassOf      [ rdf:type         owl:Restriction;
                               owl:cardinality  1;
                               owl:onProperty   ocsf:user
                             ];
        dcterms:description  "Authorize Session events report privileges or groups assigned to a new user session, usually at login time.";
        ocsf:associations    "{\"session\":[\"user\"],\"user\":[\"session\"]}";
        ocsf:constraints     "{\"just_one\":[\"privileges\",\"group\"]}";
        ocsf:name            "authorize_session";
        ocsf:uid             3 .

ocsf:svc_name  rdf:type      owl:DatatypeProperty;
        rdfs:label           "Service Name";
        rdfs:range           ocsf:string_t;
        dcterms:description  "The service name in service-to-service connections. For example, AWS VPC logs the pkt-src-aws-service and pkt-dst-aws-service fields identify the connection is coming from or going to an AWS service." .

ocsf:x_forwarded_for  rdf:type  owl:DatatypeProperty;
        rdfs:label           "X-Forwarded-For";
        rdfs:range           ocsf:ip_t;
        dcterms:description  "The X-Forwarded-For header identifying the originating IP address(es) of a client connecting to a web server through an HTTP proxy or a load balancer." .

ocsf:resource_type  rdf:type  owl:DatatypeProperty;
        rdfs:label           "Resource Type";
        rdfs:range           ocsf:string_t;
        dcterms:description  "The resource type as defined by the event source." .

ocsf:zone  rdf:type          owl:DatatypeProperty;
        rdfs:label           "Network Zone";
        rdfs:range           ocsf:string_t;
        dcterms:description  "The network zone or LAN segment." .

ocsf:DiscoveryEvent  rdf:type  owl:Class;
        rdfs:label           "Discovery";
        rdfs:subClassOf      d3f:DigitalEvent;
        dcterms:description  "The Discovery event is a generic event that defines a set of attributes available in Discovery category events. As a generic event, it could be used to log events that are not otherwise defined by the Discovery specific event classes.";
        ocsf:category        "discovery";
        ocsf:name            "discovery" .

ocsf:severity_id  rdf:type   owl:DatatypeProperty;
        rdfs:label           "Severity ID";
        rdfs:range           ocsf:integer_t;
        dcterms:description  "<p>The normalized identifier of the event/finding severity.</p>The normalized severity is a measurement the effort and expense required to manage and resolve an event or incident. Smaller numerical values represent lower impact events, and larger numerical values represent higher impact events.";
        jsonschema:enum      "Medium" , "Informational" , "Other" , "Critical" , "Fatal" , "Low" , "Unknown" , "High" .

ocsf:duration  rdf:type      owl:DatatypeProperty;
        rdfs:label           "Duration";
        rdfs:range           ocsf:integer_t;
        dcterms:description  "The event duration or aggregate time, the amount of time the event covers from <code>start_time</code> to <code>end_time</code> in milliseconds." .

ocsf:group  rdf:type         owl:ObjectProperty;
        rdfs:label           "Group";
        rdfs:range           ocsf:Group;
        dcterms:description  "The group object associated with an entity such as user, policy, or rule." .

ocsf:cmd_line  rdf:type      owl:DatatypeProperty;
        rdfs:label           "Command Line";
        rdfs:range           ocsf:string_t;
        dcterms:description  "The full command line used to launch an application, service, process, or job. For example: <code>ssh user@10.0.0.10</code>. If the command line is unavailable or missing, the empty string <code>''</code> is to be used" .

ocsf:DNSActivityEvent
        rdf:type             owl:Class;
        rdfs:label           "DNS Activity";
        rdfs:subClassOf      d3f:DigitalEvent;
        rdfs:subClassOf      [ rdf:type            owl:Restriction;
                               owl:onProperty      ocsf:connection_info;
                               owl:someValuesFrom  ocsf:NetworkConnectionInformation
                             ];
        rdfs:subClassOf      [ rdf:type            owl:Restriction;
                               owl:onProperty      ocsf:traffic;
                               owl:someValuesFrom  ocsf:NetworkTraffic
                             ];
        rdfs:subClassOf      [ rdf:type            owl:Restriction;
                               owl:onProperty      ocsf:answers;
                               owl:someValuesFrom  ocsf:DNSAnswer
                             ];
        rdfs:subClassOf      [ rdf:type            owl:Restriction;
                               owl:onProperty      ocsf:dst_endpoint;
                               owl:someValuesFrom  ocsf:NetworkEndpoint
                             ];
        rdfs:subClassOf      [ rdf:type            owl:Restriction;
                               owl:onProperty      ocsf:query;
                               owl:someValuesFrom  ocsf:DNSQuery
                             ];
        dcterms:description  "DNS Activity events report DNS queries and answers as seen on the network.";
        ocsf:name            "dns_activity";
        ocsf:uid             3 .

ocsf:share_type_id  rdf:type  owl:DatatypeProperty;
        rdfs:label           "Share Type Id";
        rdfs:range           ocsf:integer_t;
        dcterms:description  "The normalized identifier of the SMB share type.";
        jsonschema:enum      "Print" , "Pipe" , "File" , "Unknown" , "Other" .

ocsf:xattributes  rdf:type   owl:ObjectProperty;
        rdfs:label           "Extended Attributes";
        rdfs:range           ocsf:Object;
        dcterms:description  "An unordered collection of zero or more name/value pairs where each pair represents a file or folder extended attribute.</p>For example: Windows alternate data stream attributes (ADS stream name, ADS size, etc.), user-defined or application-defined attributes, ACL, owner, primary group, etc. Examples from DCS: </p><ul><li><strong>ads_name</strong></li><li><strong>ads_size</strong></li><li><strong>dacl</strong></li><li><strong>owner</strong></li><li><strong>primary_group</strong></li><li><strong>link_name</strong> - name of the link associated to the file.</li><li><strong>hard_link_count</strong> - the number of links that are associated to the file.</li></ul>" .

ocsf:KillChainPhase  rdf:type  owl:Class;
        rdfs:label           "Kill Chain Phase";
        rdfs:subClassOf      ocsf:Object;
        dcterms:description  "The Kill Chain Phase object represents a single phase of a cyber attack, including the initial reconnaissance and planning stages up to the final objective of the attacker. It provides a detailed description of each phase and its associated activities within the broader context of a cyber attack. See <a target='_blank' href='https://www.lockheedmartin.com/en-us/capabilities/cyber/cyber-kill-chain.html'>Cyber Kill Chain®</a>.";
        ocsf:name            "kill_chain_phase" .

ocsf:activity_id  rdf:type   owl:DatatypeProperty;
        rdfs:label           "Activity ID";
        rdfs:range           ocsf:integer_t;
        dcterms:description  "The normalized identifier of the activity that triggered the event.";
        jsonschema:enum      "Unknown" , "Other" .

ocsf:priority_id  rdf:type   owl:DatatypeProperty;
        rdfs:label           "Priority ID";
        rdfs:range           ocsf:integer_t;
        dcterms:description  "The normalized priority. See specific usage." .

ocsf:client_ciphers  rdf:type  owl:DatatypeProperty;
        rdfs:label           "Client Cipher Suites";
        rdfs:range           ocsf:string_t;
        dcterms:description  "The client cipher suites that were exchanged during the TLS handshake negotiation." .

ocsf:status_code  rdf:type   owl:DatatypeProperty;
        rdfs:label           "Status Code";
        rdfs:range           ocsf:string_t;
        dcterms:description  "The event status code, as reported by the event source.<br /><br />For example, in a Windows Failed Authentication event, this would be the value of 'Failure Code', e.g. 0x18." .

ocsf:network_driver  rdf:type  owl:DatatypeProperty;
        rdfs:label           "Network Driver";
        rdfs:range           ocsf:string_t;
        dcterms:description  "The network driver used by the container. For example, bridge, overlay, host, none, etc." .

ocsf:UserAccessManagementEvent
        rdf:type             owl:Class;
        rdfs:label           "User Access Management";
        rdfs:subClassOf      d3f:DigitalEvent;
        rdfs:subClassOf      [ rdf:type         owl:Restriction;
                               owl:cardinality  1;
                               owl:onProperty   ocsf:user
                             ];
        rdfs:subClassOf      [ rdf:type            owl:Restriction;
                               owl:onProperty      ocsf:resource;
                               owl:someValuesFrom  ocsf:ResourceDetails
                             ];
        dcterms:description  "User Access Management events report management updates to a user's privileges.";
        ocsf:name            "user_access";
        ocsf:uid             5 .

ocsf:Feature  rdf:type       owl:Class;
        rdfs:label           "Feature";
        rdfs:subClassOf      ocsf:Entity;
        dcterms:description  "The Feature object provides information about the software product feature that generated a specific event. It encompasses details related to the capabilities, components, user interface (UI) design, and performance upgrades associated with the feature.";
        ocsf:name            "feature" .

ocsf:IdentityProvider
        rdf:type             owl:Class;
        rdfs:label           "Identity Provider";
        rdfs:subClassOf      ocsf:Entity;
        dcterms:description  "The Identity Provider object contains detailed information about a provider responsible for creating, maintaining, and managing identity information while offering authentication services to applications. An Identity Provider (IdP) serves as a trusted authority that verifies the identity of users and issues authentication tokens or assertions to enable secure access to applications or services.";
        ocsf:name            "idp" .

ocsf:uid  rdf:type           owl:DatatypeProperty;
        rdfs:label           "Unique ID";
        rdfs:range           ocsf:string_t;
        dcterms:description  "The unique identifier. See specific usage." .

ocsf:FindingEvent  rdf:type  owl:Class;
        rdfs:label           "Finding";
        rdfs:subClassOf      d3f:DigitalEvent;
        rdfs:subClassOf      [ rdf:type         owl:Restriction;
                               owl:cardinality  1;
                               owl:onProperty   ocsf:finding_info
                             ];
        dcterms:description  "The Finding event is a generic event that defines a set of attributes available in the Findings category.";
        ocsf:category        "findings";
        ocsf:name            "finding" .

ocsf:subnet_t  rdf:type      rdfs:Datatype;
        rdfs:label           "Subnet";
        rdfs:subClassOf      xsd:string;
        dcterms:description  "The subnet represented in a CIDR notation, using the format network_address/prefix_length. The network_address can be in either IPv4 or IPv6 format. The prefix length indicates the number of bits used for the network portion, and the remaining bits are available for host addresses within that subnet. <div>For example:<ul><li>192.168.1.0/24</li><li>2001:0db8:85a3:0000::/64</li></ul></div>" .

ocsf:extensions  rdf:type    owl:ObjectProperty;
        rdfs:label           "Schema Extensions";
        rdfs:range           ocsf:SchemaExtension;
        dcterms:description  "The schema extensions used to create the event." .

ocsf:keyboard_type  rdf:type  owl:DatatypeProperty;
        rdfs:label           "Keyboard Type";
        rdfs:range           ocsf:string_t;
        dcterms:description  "The keyboard type (e.g., xt, ico)." .

ocsf:kb_article_list  rdf:type  owl:ObjectProperty;
        rdfs:label           "Knowledgebase Articles";
        rdfs:range           ocsf:KBArticle;
        dcterms:description  "A list of KB articles or patches related to an endpoint." .

ocsf:DCERPC  rdf:type        owl:Class;
        rdfs:label           "DCE/RPC";
        rdfs:subClassOf      ocsf:Object;
        rdfs:subClassOf      [ rdf:type         owl:Restriction;
                               owl:cardinality  1;
                               owl:onProperty   ocsf:rpc_interface
                             ];
        dcterms:description  "The DCE/RPC, or Distributed Computing Environment/Remote Procedure Call, object describes the remote procedure call system for distributed computing environments. Defined by D3FEND <a target='_blank' href='https://d3fend.mitre.org/dao/artifact/d3f:RemoteProcedureCall/'>d3f:RemoteProcedureCall</a>.";
        ocsf:name            "dce_rpc" .

ocsf:count  rdf:type         owl:DatatypeProperty;
        rdfs:label           "Count";
        rdfs:range           ocsf:integer_t;
        dcterms:description  "The number of times that events in the same logical group occurred during the event <strong>Start Time</strong> to <strong>End Time</strong> period." .

ocsf:is_superseded  rdf:type  owl:DatatypeProperty;
        rdfs:label           "The patch is superseded.";
        rdfs:range           ocsf:boolean_t;
        dcterms:description  "The vendor patch has been replaced by another." .

ocsf:dkim_domain  rdf:type   owl:DatatypeProperty;
        rdfs:label           "DKIM Domain";
        rdfs:range           ocsf:string_t;
        dcterms:description  "The DomainKeys Identified Mail (DKIM) signing domain of the email." .

ocsf:RPCInterface  rdf:type  owl:Class;
        rdfs:label           "RPC Interface";
        rdfs:subClassOf      ocsf:Object;
        dcterms:description  "The RPC Interface represents the remote procedure call interface used in the DCE/RPC session.";
        ocsf:name            "rpc_interface" .

ocsf:logged_time  rdf:type   owl:DatatypeProperty;
        rdfs:label           "Logged Time";
        rdfs:range           ocsf:timestamp_t;
        dcterms:description  "<p>The time when the logging system collected and logged the event.</p>This attribute is distinct from the event time in that event time typically contain the time extracted from the original event. Most of the time, these two times will be different." .

ocsf:uid_alt  rdf:type       owl:DatatypeProperty;
        rdfs:label           "Alternate ID";
        rdfs:range           ocsf:string_t;
        dcterms:description  "The alternate unique identifier. See specific usage." .

ocsf:cpu_cores  rdf:type     owl:DatatypeProperty;
        rdfs:label           "CPU Cores";
        rdfs:range           ocsf:integer_t;
        dcterms:description  "The number of processor cores in all installed processors. For Example: <code>42</code>." .

ocsf:load_type  rdf:type     owl:DatatypeProperty;
        rdfs:label           "Load Type";
        rdfs:range           ocsf:string_t;
        dcterms:description  "The load type, normalized to the caption of the load_type_id value. In the case of 'Other', it is defined by the event source. It describes how the module was loaded in memory." .

ocsf:MemoryActivityEvent
        rdf:type             owl:Class;
        rdfs:label           "Memory Activity";
        rdfs:subClassOf      d3f:DigitalEvent;
        rdfs:subClassOf      [ rdf:type         owl:Restriction;
                               owl:cardinality  1;
                               owl:onProperty   ocsf:process
                             ];
        dcterms:description  "Memory Activity events report when a process has memory allocated, read/modified, or other manipulation activities - such as a buffer overflow or turning off data execution protection (DEP).";
        ocsf:name            "memory_activity";
        ocsf:uid             4 .

ocsf:rule  rdf:type          owl:ObjectProperty;
        rdfs:label           "Rule";
        rdfs:range           ocsf:Rule;
        dcterms:description  "The rules that reported the events." .

ocsf:technique  rdf:type     owl:ObjectProperty;
        rdfs:label           "Technique";
        rdfs:range           ocsf:Technique;
        dcterms:description  "The Technique object describes the technique ID and/or name associated to an attack, as defined by <a target='_blank' href='https://attack.mitre.org/wiki/ATT&CK_Matrix'>ATT&CK Matrix<sup>TM</sup></a>." .

ocsf:Group  rdf:type         owl:Class;
        rdfs:label           "Group";
        rdfs:subClassOf      ocsf:Entity;
        dcterms:description  "The Group object represents a collection or association of entities, such as users, policies, or devices. It serves as a logical grouping mechanism to organize and manage entities with similar characteristics or permissions within a system or organization.";
        ocsf:name            "group" .

ocsf:image  rdf:type         owl:ObjectProperty;
        rdfs:label           "Image";
        rdfs:range           ocsf:Image;
        dcterms:description  "The image used as a template to run a container or virtual machine." .

ocsf:finding_info  rdf:type  owl:ObjectProperty;
        rdfs:label           "Finding Information";
        rdfs:range           ocsf:FindingInformation;
        dcterms:description  "Describes the supporting information about a generated finding." .

ocsf:actual_permissions
        rdf:type             owl:DatatypeProperty;
        rdfs:label           "Actual Permissions";
        rdfs:range           ocsf:integer_t;
        dcterms:description  "The permissions that were granted to the in a platform-native format." .

ocsf:vlan_uid  rdf:type      owl:DatatypeProperty;
        rdfs:label           "VLAN";
        rdfs:range           ocsf:string_t;
        dcterms:description  "The Virtual LAN identifier." .

ocsf:LDAPPerson  rdf:type    owl:Class;
        rdfs:label           "LDAP Person";
        rdfs:subClassOf      ocsf:Object;
        rdfs:subClassOf      [ rdf:type            owl:Restriction;
                               owl:onProperty      ocsf:manager;
                               owl:someValuesFrom  ocsf:User
                             ];
        rdfs:subClassOf      [ rdf:type            owl:Restriction;
                               owl:onProperty      ocsf:location;
                               owl:someValuesFrom  ocsf:GeoLocation
                             ];
        dcterms:description  "The additonal LDAP attributes that describe a person.";
        ocsf:name            "ldap_person" .

ocsf:DNSQuery  rdf:type      owl:Class;
        rdfs:label           "DNS Query";
        rdfs:subClassOf      ocsf:DNS;
        dcterms:description  "The DNS query object represents a specific request made to the Domain Name System (DNS) to retrieve information about a domain or perform a DNS operation. This object encapsulates the necessary attributes and methods to construct and send DNS queries, specify the query type (e.g., A, AAAA, MX). Defined by D3FEND <a target='_blank' href='https://d3fend.mitre.org/dao/artifact/d3f:DNSLookup/'>d3f:DNSLookup</a>.";
        ocsf:name            "dns_query" .

ocsf:rcode_id  rdf:type      owl:DatatypeProperty;
        rdfs:label           "Response Code ID";
        rdfs:range           ocsf:integer_t;
        dcterms:description  "The normalized identifier of the server response code. See specific usage.";
        jsonschema:enum      "Unknown" , "Other" .

ocsf:EmailFileActivityEvent
        rdf:type             owl:Class;
        rdfs:label           "Email File Activity";
        rdfs:subClassOf      d3f:DigitalEvent;
        rdfs:subClassOf      [ rdf:type         owl:Restriction;
                               owl:cardinality  1;
                               owl:onProperty   ocsf:file
                             ];
        dcterms:description  "Email File Activity events report files within emails.";
        ocsf:category        "network";
        ocsf:name            "email_file_activity";
        ocsf:profiles        "[\"host\",\"security_control\"]";
        ocsf:uid             11 .

ocsf:confidence_score
        rdf:type             owl:DatatypeProperty;
        rdfs:label           "Confidence Score";
        rdfs:range           ocsf:integer_t;
        dcterms:description  "The confidence score as reported by the event source." .

ocsf:command_responses
        rdf:type             owl:DatatypeProperty;
        rdfs:label           "Command Responses";
        rdfs:range           ocsf:string_t;
        dcterms:description  "The responses to the command." .

ocsf:protocol_name  rdf:type  owl:DatatypeProperty;
        rdfs:label           "Protocol Name";
        rdfs:range           ocsf:string_t;
        dcterms:description  "The TCP/IP protocol name in lowercase, as defined by the Internet Assigned Numbers Authority (IANA). See <a target='_blank' href='https://www.iana.org/assignments/protocol-numbers/protocol-numbers.xhtml'>Protocol Numbers</a>. For example: <code>tcp</code> or <code>udp</code>." .

ocsf:imei  rdf:type          owl:DatatypeProperty;
        rdfs:label           "IMEI";
        rdfs:range           ocsf:string_t;
        dcterms:description  "The International Mobile Station Equipment Identifier that is associated with the device." .

ocsf:open_mask  rdf:type     owl:DatatypeProperty;
        rdfs:label           "Open Mask";
        rdfs:range           ocsf:integer_t;
        dcterms:description  "The Windows options needed to open a registry key." .

ocsf:GroupManagementEvent
        rdf:type             owl:Class;
        rdfs:label           "Group Management";
        rdfs:subClassOf      d3f:DigitalEvent;
        rdfs:subClassOf      [ rdf:type            owl:Restriction;
                               owl:onProperty      ocsf:user;
                               owl:someValuesFrom  ocsf:User
                             ];
        rdfs:subClassOf      [ rdf:type         owl:Restriction;
                               owl:cardinality  1;
                               owl:onProperty   ocsf:group
                             ];
        rdfs:subClassOf      [ rdf:type            owl:Restriction;
                               owl:onProperty      ocsf:resource;
                               owl:someValuesFrom  ocsf:ResourceDetails
                             ];
        dcterms:description  "Group Management events report management updates to a group, including updates to membership and permissions.";
        ocsf:constraints     "{\"at_least_one\":[\"privileges\",\"user\"]}";
        ocsf:name            "group_management";
        ocsf:uid             6 .

ocsf:Object  rdf:type        owl:Class;
        rdfs:label           "Object";
        rdfs:subClassOf      ocsf:CISBenchmarkResult , ocsf:Metadata , ocsf:KillChainPhase , ocsf:UniformResourceLocator , ocsf:HTTPHeader , ocsf:NetworkInterface , ocsf:Endpoint , ocsf:TLSExtension , ocsf:DeviceHardwareInfo , ocsf:PeripheralDevice , ocsf:GeoLocation , ocsf:EPSS , ocsf:Device , ocsf:CVE , ocsf:CISBenchmark , ocsf:Organization , ocsf:Policy , ocsf:HTTPResponse , ocsf:EvidenceArtifacts , ocsf:IdentityProvider , ocsf:Metric , ocsf:User , ocsf:KeyboardInformation , ocsf:MITREATTCK , ocsf:Logger , ocsf:Job , ocsf:NetworkTraffic , ocsf:DNSAnswer , ocsf:API , ocsf:Reputation , ocsf:NetworkEndpoint , ocsf:Analytic , ocsf:KernelExtension , ocsf:Object , ocsf:RequestElements , ocsf:CWE , ocsf:EmailAuthentication , ocsf:DigitalCertificate , ocsf:Remediation , ocsf:CVSSScore , ocsf:VulnerabilityDetails , ocsf:Compliance , ocsf:Observable , ocsf:Resource , ocsf:FindingInformation , ocsf:Rule , ocsf:CISControl , ocsf:File , ocsf:WebResource , ocsf:Session , ocsf:DNS , ocsf:FirewallRule , ocsf:KernelResource , ocsf:Technique , ocsf:KBArticle , ocsf:AffectedCode , ocsf:Malware , ocsf:Display , ocsf:SubTechnique , ocsf:SubjectAlternativeName , ocsf:NetworkConnectionInformation , ocsf:Email , ocsf:Product , ocsf:HTTPCookie , ocsf:Module , ocsf:Image , ocsf:TransportLayerSecurityTLS , ocsf:Process , ocsf:Group , ocsf:RelatedEvent , ocsf:SoftwarePackage , ocsf:ResourceDetails , ocsf:RPCInterface , ocsf:Container , ocsf:OperatingSystemOS , ocsf:DigitalSignature , ocsf:Feature , ocsf:HTTPRequest , ocsf:AuthorizationResult , ocsf:Finding , ocsf:NetworkProxyEndpoint , ocsf:DCERPC , ocsf:Service , ocsf:DNSQuery , ocsf:Fingerprint , ocsf:LDAPPerson , ocsf:Tactic , ocsf:AffectedSoftwarePackage , ocsf:Entity , ocsf:Actor , ocsf:ManagedEntity , ocsf:ResponseElements , ocsf:SchemaExtension , ocsf:Enrichment , ocsf:HASSH , ocsf:Cloud , ocsf:CISCSC , ocsf:Account;
        dcterms:description  "An unordered collection of attributes. It defines a set of attributes available in all objects. It can be also used as a generic object to log objects that are not otherwise defined by the schema.";
        ocsf:name            "object" .

ocsf:url  rdf:type           owl:ObjectProperty;
        rdfs:label           "URL";
        rdfs:range           ocsf:UniformResourceLocator;
        dcterms:description  "The URL object that pertains to the event or object. See specific usage." .

ocsf:cost_center  rdf:type   owl:DatatypeProperty;
        rdfs:label           "Cost Center";
        rdfs:range           ocsf:string_t;
        dcterms:description  "The cost center associated with the user." .

ocsf:port_t  rdf:type        rdfs:Datatype;
        rdfs:label           "Port";
        rdfs:subClassOf      xsd:integer;
        dcterms:description  "The TCP/UDP port number. For example: <code>80</code> or <code>22</code>.";
        xsd:maxInclusive     65535;
        xsd:minInclusive     0 .

ocsf:KBArticle  rdf:type     owl:Class;
        rdfs:label           "KB Article";
        rdfs:subClassOf      ocsf:Object;
        rdfs:subClassOf      [ rdf:type            owl:Restriction;
                               owl:onProperty      ocsf:product;
                               owl:someValuesFrom  ocsf:Product
                             ];
        rdfs:subClassOf      [ rdf:type            owl:Restriction;
                               owl:onProperty      ocsf:os;
                               owl:someValuesFrom  ocsf:OperatingSystemOS
                             ];
        dcterms:description  "The KB Article object contains metadata that describes the patch or update.";
        ocsf:name            "kb_article" .

ocsf:containers  rdf:type    owl:ObjectProperty;
        rdfs:label           "Containers";
        rdfs:range           ocsf:Container;
        dcterms:description  "When working with containerized applications, the set of containers which write to the standard the output of a particular logging driver. For example, this may be the set of containers involved in handling api requests and responses for a containerized application." .

ocsf:requested_permissions
        rdf:type             owl:DatatypeProperty;
        rdfs:label           "Requested Permissions";
        rdfs:range           ocsf:integer_t;
        dcterms:description  "The permissions mask that were requested by the process." .

ocsf:region  rdf:type        owl:DatatypeProperty;
        rdfs:label           "Region";
        rdfs:range           ocsf:string_t;
        dcterms:description  "The name or the code of a region. See specific usage." .

ocsf:ScheduledJobActivityEvent
        rdf:type             owl:Class;
        rdfs:label           "Scheduled Job Activity";
        rdfs:subClassOf      d3f:DigitalEvent;
        rdfs:subClassOf      [ rdf:type         owl:Restriction;
                               owl:cardinality  1;
                               owl:onProperty   ocsf:job
                             ];
        rdfs:subClassOf      [ rdf:type            owl:Restriction;
                               owl:onProperty      ocsf:actor;
                               owl:someValuesFrom  ocsf:Actor
                             ];
        dcterms:description  "Scheduled Job Activity events report activities related to scheduled jobs or tasks.";
        ocsf:name            "scheduled_job_activity";
        ocsf:uid             6 .

ocsf:precision  rdf:type     owl:DatatypeProperty;
        rdfs:label           "Precision";
        rdfs:range           ocsf:integer_t;
        dcterms:description  "The numeric precision. See specific usage." .

ocsf:devices  rdf:type       owl:ObjectProperty;
        rdfs:label           "Devices";
        rdfs:range           ocsf:Device;
        dcterms:description  "The object describes details related to the list of devices." .

ocsf:ttl  rdf:type           owl:DatatypeProperty;
        rdfs:label           "TTL";
        rdfs:range           ocsf:integer_t;
        dcterms:description  "The time interval that the resource record may be cached. Zero value means that the resource record can only be used for the transaction in progress, and should not be cached." .

ocsf:metrics  rdf:type       owl:ObjectProperty;
        rdfs:label           "Metrics";
        rdfs:range           ocsf:Metric;
        dcterms:description  "The general purpose metrics associated with the event. See specific usage." .

ocsf:DNSAnswer  rdf:type     owl:Class;
        rdfs:label           "DNS Answer";
        rdfs:subClassOf      ocsf:DNS;
        dcterms:description  "The DNS Answer object represents a specific response provided by the Domain Name System (DNS) when querying for information about a domain or performing a DNS operation. It encapsulates the relevant details and data returned by the DNS server in response to a query.";
        ocsf:name            "dns_answer" .

ocsf:Image  rdf:type         owl:Class;
        rdfs:label           "Image";
        rdfs:subClassOf      ocsf:Entity;
        dcterms:description  "The Image object provides a description of a specific Virtual Machine (VM) or Container image. Defined by D3FEND <a target='_blank' href='https://d3fend.mitre.org/dao/artifact/d3f:ContainerImage/'>d3f:ContainerImage</a>.";
        ocsf:constraints     "{}";
        ocsf:name            "image" .

ocsf:auth_protocol_id
        rdf:type             owl:DatatypeProperty;
        rdfs:label           "Auth Protocol ID";
        rdfs:range           ocsf:integer_t;
        dcterms:description  "The normalized identifier of the authentication protocol used to create the user session.";
        jsonschema:enum      "Kerberos" , "SAML" , "CHAP" , "RADIUS" , "PAP" , "OpenID" , "OAUTH 2.0" , "EAP" , "NTLM" , "Digest" , "Other" , "Unknown" .

ocsf:SMBActivityEvent
        rdf:type             owl:Class;
        rdfs:label           "SMB Activity";
        rdfs:subClassOf      d3f:DigitalEvent;
        rdfs:subClassOf      [ rdf:type            owl:Restriction;
                               owl:onProperty      ocsf:response;
                               owl:someValuesFrom  ocsf:ResponseElements
                             ];
        rdfs:subClassOf      [ rdf:type            owl:Restriction;
                               owl:onProperty      ocsf:file;
                               owl:someValuesFrom  ocsf:File
                             ];
        rdfs:subClassOf      [ rdf:type            owl:Restriction;
                               owl:onProperty      ocsf:dce_rpc;
                               owl:someValuesFrom  ocsf:DCERPC
                             ];
        dcterms:description  "Server Message Block (SMB) Protocol Activity events report client/server connections sharing resources within the network.";
        ocsf:name            "smb_activity";
        ocsf:uid             6 .

ocsf:digest  rdf:type        owl:ObjectProperty;
        rdfs:label           "Message Digest";
        rdfs:range           ocsf:Fingerprint;
        dcterms:description  "The message digest attribute contains the fixed length message hash representation and the corresponding hashing algorithm information." .

ocsf:connection_info  rdf:type  owl:ObjectProperty;
        rdfs:label           "Connection Info";
        rdfs:range           ocsf:NetworkConnectionInformation;
        dcterms:description  "The network connection information." .

ocsf:bios_date  rdf:type     owl:DatatypeProperty;
        rdfs:label           "BIOS Date";
        rdfs:range           ocsf:string_t;
        dcterms:description  "The BIOS date. For example: <code>03/31/16</code>." .

ocsf:SSHActivityEvent
        rdf:type             owl:Class;
        rdfs:label           "SSH Activity";
        rdfs:subClassOf      d3f:DigitalEvent;
        rdfs:subClassOf      [ rdf:type            owl:Restriction;
                               owl:onProperty      ocsf:server_hassh;
                               owl:someValuesFrom  ocsf:HASSH
                             ];
        rdfs:subClassOf      [ rdf:type            owl:Restriction;
                               owl:onProperty      ocsf:client_hassh;
                               owl:someValuesFrom  ocsf:HASSH
                             ];
        dcterms:description  "SSH Activity events report remote client connections to a server using the Secure Shell (SSH) Protocol.";
        ocsf:name            "ssh_activity";
        ocsf:uid             7 .

ocsf:physical_width  rdf:type  owl:DatatypeProperty;
        rdfs:label           "Physical Width";
        rdfs:range           ocsf:integer_t;
        dcterms:description  "The numeric physical width of display." .

ocsf:hostname_t  rdf:type    rdfs:Datatype;
        rdfs:label           "Hostname";
        rdfs:subClassOf      xsd:string;
        dcterms:description  "Unique name assigned to a device connected to a computer network. A domain name in general is an Internet address that can be resolved through the Domain Name System (DNS). For example: <code>r2-d2.example.com</code>.";
        xsd:pattern          "^(([a-zA-Z0-9]|[a-zA-Z0-9][a-zA-Z0-9\\-]*[a-zA-Z0-9])\\.)*([A-Za-z0-9]|[A-Za-z0-9][A-Za-z0-9\\-]*[A-Za-z0-9])$" .

ocsf:RDPActivityEvent
        rdf:type             owl:Class;
        rdfs:label           "RDP Activity";
        rdfs:subClassOf      d3f:DigitalEvent;
        rdfs:subClassOf      [ rdf:type            owl:Restriction;
                               owl:onProperty      ocsf:device;
                               owl:someValuesFrom  ocsf:Device
                             ];
        rdfs:subClassOf      [ rdf:type            owl:Restriction;
                               owl:onProperty      ocsf:request;
                               owl:someValuesFrom  ocsf:RequestElements
                             ];
        rdfs:subClassOf      [ rdf:type            owl:Restriction;
                               owl:onProperty      ocsf:response;
                               owl:someValuesFrom  ocsf:ResponseElements
                             ];
        rdfs:subClassOf      [ rdf:type            owl:Restriction;
                               owl:onProperty      ocsf:remote_display;
                               owl:someValuesFrom  ocsf:Display
                             ];
        dcterms:description  "Remote Desktop Protocol (RDP) Activity events report remote client connections to a server as seen on the network.";
        ocsf:name            "rdp_activity";
        ocsf:uid             5 .

ocsf:risk_score  rdf:type    owl:DatatypeProperty;
        rdfs:label           "Risk Score";
        rdfs:range           ocsf:integer_t;
        dcterms:description  "The risk score as reported by the event source." .

ocsf:status  rdf:type        owl:DatatypeProperty;
        rdfs:label           "Status";
        rdfs:range           ocsf:string_t;
        dcterms:description  "The event status, normalized to the caption of the status_id value. In the case of 'Other', it is defined by the event source." .

ocsf:developer_uid  rdf:type  owl:DatatypeProperty;
        rdfs:label           "Developer UID";
        rdfs:range           ocsf:string_t;
        dcterms:description  "The developer ID on the certificate that signed the file." .

ocsf:GeoLocation  rdf:type   owl:Class;
        rdfs:label           "Geo Location";
        rdfs:subClassOf      ocsf:Object;
        dcterms:description  "The Geo Location object describes a geographical location, usually associated with an IP address. Defined by D3FEND <a target='_blank' href='https://d3fend.mitre.org/dao/artifact/d3f:PhysicalLocation/'>d3f:PhysicalLocation</a>.";
        ocsf:constraints     "{\"at_least_one\":[\"coordinates\",\"city\",\"country\",\"postal_code\",\"region\"]}";
        ocsf:name            "location";
        ocsf:observable      26 .

ocsf:is_mfa  rdf:type        owl:DatatypeProperty;
        rdfs:label           "Multi Factor Authentication";
        rdfs:range           ocsf:boolean_t;
        dcterms:description  "Indicates whether Multi Factor Authentication was used during authentication." .

ocsf:log_level  rdf:type     owl:DatatypeProperty;
        rdfs:label           "Log Level";
        rdfs:range           ocsf:string_t;
        dcterms:description  "The audit level at which an event was generated." .

ocsf:module  rdf:type        owl:ObjectProperty;
        rdfs:label           "Module";
        rdfs:range           ocsf:Module;
        dcterms:description  "The module that pertains to the event." .

ocsf:ManagedEntity  rdf:type  owl:Class;
        rdfs:label           "Managed Entity";
        rdfs:subClassOf      ocsf:Entity;
        dcterms:description  "The Managed Entity object describes the type and version of an entity, such as a policy or configuration.";
        ocsf:name            "managed_entity" .

ocsf:rdata  rdf:type         owl:DatatypeProperty;
        rdfs:label           "DNS RData";
        rdfs:range           ocsf:string_t;
        dcterms:description  "The data describing the DNS resource. The meaning of this data depends on the type and class of the resource record." .

ocsf:boundary  rdf:type      owl:DatatypeProperty;
        rdfs:label           "Boundary";
        rdfs:range           ocsf:string_t;
        dcterms:description  "The boundary of the connection, normalized to the caption of 'boundary_id'. In the case of 'Other', it is defined by the event source. <p> For cloud connections, this translates to the traffic-boundary(same VPC, through IGW, etc.). For traditional networks, this is described as Local, Internal, or External.</p>" .

ocsf:algorithm_id  rdf:type  owl:DatatypeProperty;
        rdfs:label           "Algorithm ID";
        rdfs:range           ocsf:integer_t;
        dcterms:description  "The identifier of the normalized algorithm. See specific usage.";
        jsonschema:enum      "Unknown" , "Other" .

ocsf:start_time  rdf:type    owl:DatatypeProperty;
        rdfs:label           "Start Time";
        rdfs:range           ocsf:timestamp_t;
        dcterms:description  "The start time of a time period. See specific usage." .

ocsf:service  rdf:type       owl:ObjectProperty;
        rdfs:label           "Service";
        rdfs:range           ocsf:Service;
        dcterms:description  "The service that pertains to the event." .

ocsf:namespace  rdf:type     owl:DatatypeProperty;
        rdfs:label           "Namespace";
        rdfs:range           ocsf:string_t;
        dcterms:description  "The namespace is useful in merger or acquisition situations. For example, when similar entities exist that you need to keep separate." .

ocsf:kill_chain  rdf:type    owl:ObjectProperty;
        rdfs:label           "Kill Chain";
        rdfs:range           ocsf:KillChainPhase;
        dcterms:description  "The <a target='_blank' href='https://www.lockheedmartin.com/en-us/capabilities/cyber/cyber-kill-chain.html'>Cyber Kill Chain®</a> provides a detailed description of each phase and its associated activities within the broader context of a cyber attack." .

ocsf:ack_result  rdf:type    owl:DatatypeProperty;
        rdfs:label           "Acknowledgement Result";
        rdfs:range           ocsf:integer_t;
        dcterms:description  "An integer that denotes the acknowledgment result of the DCE/RPC call." .

ocsf:cwe  rdf:type           owl:ObjectProperty;
        rdfs:label           "CWE";
        rdfs:range           ocsf:CWE;
        dcterms:description  "The CWE object represents a weakness in a software system that can be exploited by a threat actor to perform an attack. The CWE object is based on the <a target='_blank' href='https://cwe.mitre.org/'>Common Weakness Enumeration (CWE)</a> catalog." .

ocsf:relay  rdf:type         owl:ObjectProperty;
        rdfs:label           "Relay";
        rdfs:range           ocsf:NetworkInterface;
        dcterms:description  "The network relay that is associated with the event." .

ocsf:tcp_flags  rdf:type     owl:DatatypeProperty;
        rdfs:label           "TCP Flags";
        rdfs:range           ocsf:integer_t;
        dcterms:description  "The network connection TCP header flags (i.e., control bits)." .

ocsf:File  rdf:type          owl:Class;
        rdfs:label           "File";
        rdfs:subClassOf      ocsf:Entity;
        rdfs:subClassOf      [ rdf:type            owl:Restriction;
                               owl:onProperty      ocsf:product;
                               owl:someValuesFrom  ocsf:Product
                             ];
        rdfs:subClassOf      [ rdf:type            owl:Restriction;
                               owl:onProperty      ocsf:hashes;
                               owl:someValuesFrom  ocsf:Fingerprint
                             ];
        rdfs:subClassOf      [ rdf:type            owl:Restriction;
                               owl:onProperty      ocsf:owner;
                               owl:someValuesFrom  ocsf:User
                             ];
        rdfs:subClassOf      [ rdf:type            owl:Restriction;
                               owl:onProperty      ocsf:signature;
                               owl:someValuesFrom  ocsf:DigitalSignature
                             ];
        rdfs:subClassOf      [ rdf:type            owl:Restriction;
                               owl:onProperty      ocsf:creator;
                               owl:someValuesFrom  ocsf:User
                             ];
        rdfs:subClassOf      [ rdf:type            owl:Restriction;
                               owl:onProperty      ocsf:xattributes;
                               owl:someValuesFrom  ocsf:Object
                             ];
        rdfs:subClassOf      [ rdf:type            owl:Restriction;
                               owl:onProperty      ocsf:accessor;
                               owl:someValuesFrom  ocsf:User
                             ];
        rdfs:subClassOf      [ rdf:type            owl:Restriction;
                               owl:onProperty      ocsf:modifier;
                               owl:someValuesFrom  ocsf:User
                             ];
        dcterms:description  "The File object represents the metadata associated with a file stored in a computer system. It encompasses information about the file itself, including its attributes, properties, and organizational details. Defined by D3FEND <a target='_blank' href='https://next.d3fend.mitre.org/dao/artifact/d3f:File/'>d3f:File</a>.";
        ocsf:constraints     "{}";
        ocsf:name            "file";
        ocsf:observable      24 .

ocsf:end_line  rdf:type      owl:DatatypeProperty;
        rdfs:label           "End Line";
        rdfs:range           ocsf:integer_t;
        dcterms:description  "The line number of the last line of code block identified as vulnerable." .

ocsf:Device  rdf:type        owl:Class;
        rdfs:label           "Device";
        rdfs:subClassOf      ocsf:Endpoint;
        rdfs:subClassOf      [ rdf:type            owl:Restriction;
                               owl:onProperty      ocsf:hw_info;
                               owl:someValuesFrom  ocsf:DeviceHardwareInfo
                             ];
        rdfs:subClassOf      [ rdf:type            owl:Restriction;
                               owl:onProperty      ocsf:os;
                               owl:someValuesFrom  ocsf:OperatingSystemOS
                             ];
        rdfs:subClassOf      [ rdf:type            owl:Restriction;
                               owl:onProperty      ocsf:org;
                               owl:someValuesFrom  ocsf:Organization
                             ];
        rdfs:subClassOf      [ rdf:type            owl:Restriction;
                               owl:onProperty      ocsf:image;
                               owl:someValuesFrom  ocsf:Image
                             ];
        rdfs:subClassOf      [ rdf:type            owl:Restriction;
                               owl:onProperty      ocsf:groups;
                               owl:someValuesFrom  ocsf:Group
                             ];
        rdfs:subClassOf      [ rdf:type            owl:Restriction;
                               owl:onProperty      ocsf:location;
                               owl:someValuesFrom  ocsf:GeoLocation
                             ];
        rdfs:subClassOf      [ rdf:type            owl:Restriction;
                               owl:onProperty      ocsf:network_interfaces;
                               owl:someValuesFrom  ocsf:NetworkInterface
                             ];
        dcterms:description  "The Device object represents an addressable computer system or host, which is typically connected to a computer network and participates in the transmission or processing of data within the computer network. Defined by D3FEND <a target='_blank' href='https://d3fend.mitre.org/dao/artifact/d3f:Host/'>d3f:Host</a>.";
        ocsf:name            "device" .

ocsf:lease_dur  rdf:type     owl:DatatypeProperty;
        rdfs:label           "Lease Duration";
        rdfs:range           ocsf:integer_t;
        dcterms:description  "This represents the length of the DHCP lease in seconds. This is present in DHCP Ack events." .

ocsf:sp_name  rdf:type       owl:DatatypeProperty;
        rdfs:label           "OS Service Pack";
        rdfs:range           ocsf:string_t;
        dcterms:description  "The name of the latest Service Pack." .

ocsf:content_type  rdf:type  owl:DatatypeProperty;
        rdfs:label           "HTTP Content Type";
        rdfs:range           ocsf:string_t;
        dcterms:description  "The request header that identifies the original <a target='_blank' href='https://www.iana.org/assignments/media-types/media-types.xhtml'>media type </a> of the resource (prior to any content encoding applied for sending)." .

ocsf:is_exploit_available
        rdf:type             owl:DatatypeProperty;
        rdfs:label           "Exploit Availability";
        rdfs:range           ocsf:boolean_t;
        dcterms:description  "Indicates if an exploit or a PoC (proof-of-concept) is available for the reported vulnerability." .

ocsf:reply_to  rdf:type      owl:DatatypeProperty;
        rdfs:label           "Reply To";
        rdfs:range           ocsf:email_t;
        dcterms:description  "The email header Reply-To values, as defined by RFC 5322." .

ocsf:open_type  rdf:type     owl:DatatypeProperty;
        rdfs:label           "Open Type";
        rdfs:range           ocsf:string_t;
        dcterms:description  "The file open type." .

ocsf:hash  rdf:type          owl:ObjectProperty;
        rdfs:label           "Hash";
        rdfs:range           ocsf:Fingerprint;
        dcterms:description  "The hash attribute is the value of a digital fingerprint including information about its algorithm." .

ocsf:parent_process  rdf:type  owl:ObjectProperty;
        rdfs:label           "Parent Process";
        rdfs:range           ocsf:Process;
        dcterms:description  "The parent process of this process object. It is recommended to only populate this field for the first process object, to prevent deep nesting." .

ocsf:physical_height  rdf:type  owl:DatatypeProperty;
        rdfs:label           "Physical Height";
        rdfs:range           ocsf:integer_t;
        dcterms:description  "The numeric physical height of display." .

ocsf:terminal  rdf:type      owl:DatatypeProperty;
        rdfs:label           "Terminal";
        rdfs:range           ocsf:string_t;
        dcterms:description  "The Pseudo Terminal. Ex: the tty or pts value." .

ocsf:HASSH  rdf:type         owl:Class;
        rdfs:label           "HASSH";
        rdfs:subClassOf      ocsf:Object;
        rdfs:subClassOf      [ rdf:type         owl:Restriction;
                               owl:cardinality  1;
                               owl:onProperty   ocsf:fingerprint
                             ];
        dcterms:description  "The HASSH object contains SSH network fingerprinting values for specific client/server implementations. It provides a standardized way of identifying and categorizing SSH connections based on their unique characteristics and behavior.";
        ocsf:name            "hassh" .

ocsf:from  rdf:type          owl:DatatypeProperty;
        rdfs:label           "From";
        rdfs:range           ocsf:email_t;
        dcterms:description  "The email header From values, as defined by RFC 5322." .

ocsf:file_hash_t  rdf:type   rdfs:Datatype;
        rdfs:label           "Hash";
        rdfs:subClassOf      xsd:string;
        dcterms:description  "Hash. A unique value that corresponds to the content of the file, image, ja3_hash or hassh found in the schema. For example MD5: <code>3172ac7e2b55cbb81f04a6e65855a628</code>." .

ocsf:tactics  rdf:type       owl:ObjectProperty;
        rdfs:label           "Tactics";
        rdfs:range           ocsf:Tactic;
        dcterms:description  "The Tactic object describes the tactic ID and/or tactic name that are associated with the attack technique, as defined by <a target='_blank' href='https://attack.mitre.org/wiki/ATT&CK_Matrix'>ATT&CK Matrix<sup>TM</sup></a>." .

ocsf:lineage  rdf:type       owl:DatatypeProperty;
        rdfs:label           "Lineage";
        rdfs:range           ocsf:string_t;
        dcterms:description  "The lineage of the process, represented by a list of paths for each ancestor process. For example: <code>['/usr/sbin/sshd', '/usr/bin/bash', '/usr/bin/whoami']</code>." .

ocsf:ram_size  rdf:type      owl:DatatypeProperty;
        rdfs:label           "RAM Size";
        rdfs:range           ocsf:integer_t;
        dcterms:description  "The total amount of installed RAM, in Megabytes. For example: <code>2048</code>." .

ocsf:modified_time  rdf:type  owl:DatatypeProperty;
        rdfs:label           "Modified Time";
        rdfs:range           ocsf:timestamp_t;
        dcterms:description  "The time when the object was last modified. See specific usage." .

ocsf:email_uid  rdf:type     owl:DatatypeProperty;
        rdfs:label           "Email UID";
        rdfs:range           ocsf:string_t;
        dcterms:description  "The unique identifier of the email, used to correlate related email alert and activity events." .

ocsf:referrer  rdf:type      owl:DatatypeProperty;
        rdfs:label           "HTTP Referrer";
        rdfs:range           ocsf:string_t;
        dcterms:description  "The request header that identifies the address of the previous web page, which is linked to the current web page or resource being requested." .

ocsf:customer_uid  rdf:type  owl:DatatypeProperty;
        rdfs:label           "Customer UID";
        rdfs:range           ocsf:string_t;
        dcterms:description  "The unique customer identifier." .

ocsf:smtp_from  rdf:type     owl:DatatypeProperty;
        rdfs:label           "SMTP From";
        rdfs:range           ocsf:email_t;
        dcterms:description  "The value of the SMTP MAIL FROM command." .

ocsf:phones  rdf:type        owl:DatatypeProperty;
        rdfs:label           "Phones";
        rdfs:range           ocsf:string_t;
        dcterms:description  "The phone numbers associated with the user" .

ocsf:continent  rdf:type     owl:DatatypeProperty;
        rdfs:label           "Continent";
        rdfs:range           ocsf:string_t;
        dcterms:description  "The name of the continent." .

ocsf:Finding  rdf:type       owl:Class;
        rdfs:label           "Finding";
        rdfs:subClassOf      ocsf:Object;
        rdfs:subClassOf      [ rdf:type            owl:Restriction;
                               owl:onProperty      ocsf:remediation;
                               owl:someValuesFrom  ocsf:Remediation
                             ];
        rdfs:subClassOf      [ rdf:type            owl:Restriction;
                               owl:onProperty      ocsf:related_events;
                               owl:someValuesFrom  ocsf:RelatedEvent
                             ];
        dcterms:description  "The Finding object describes metadata related to a security finding generated by a security tool or system.";
        ocsf:name            "finding" .

ocsf:proxy_tls  rdf:type     owl:ObjectProperty;
        rdfs:label           "Proxy TLS";
        rdfs:range           ocsf:TransportLayerSecurityTLS;
        dcterms:description  "The TLS protocol negotiated between the proxy server and the remote server." .

ocsf:last_run_time  rdf:type  owl:DatatypeProperty;
        rdfs:label           "Last Run";
        rdfs:range           ocsf:timestamp_t;
        dcterms:description  "The last run time of application or service. See specific usage." .

ocsf:opnum  rdf:type         owl:DatatypeProperty;
        rdfs:label           "Opnum";
        rdfs:range           ocsf:integer_t;
        dcterms:description  "An operation number used to identify a specific remote procedure call (RPC) method or a method in an interface." .

ocsf:long_t  rdf:type        rdfs:Datatype;
        rdfs:label           "Long";
        rdfs:subClassOf      xsd:long;
        dcterms:description  "8-byte long, signed integer value." .

ocsf:cloud_partition  rdf:type  owl:DatatypeProperty;
        rdfs:label           "Cloud Partition";
        rdfs:range           ocsf:string_t;
        dcterms:description  "The canonical cloud partition name to which the region is assigned (e.g. AWS Partitions: aws, aws-cn, aws-us-gov)." .

ocsf:packets  rdf:type       owl:DatatypeProperty;
        rdfs:label           "Total Packets";
        rdfs:range           ocsf:long_t;
        dcterms:description  "The total number of packets (in and out)." .

ocsf:next_run_time  rdf:type  owl:DatatypeProperty;
        rdfs:label           "Next Run";
        rdfs:range           ocsf:timestamp_t;
        dcterms:description  "The next run time. See specific usage." .

ocsf:related_events  rdf:type  owl:ObjectProperty;
        rdfs:label           "Related Events";
        rdfs:range           ocsf:RelatedEvent;
        dcterms:description  "Describes events and/or other findings related to the finding as identified by the security product." .

ocsf:Entity  rdf:type        owl:Class;
        rdfs:label           "Entity";
        rdfs:subClassOf      ocsf:Object;
        dcterms:description  "The Entity object is an unordered collection of attributes, with a name and unique identifier. It serves as a base object that defines a set of attributes and default constraints available in all objects that extend it.";
        ocsf:constraints     "{\"at_least_one\":[\"name\",\"uid\"]}";
        ocsf:name            "_entity" .

ocsf:message_uid  rdf:type   owl:DatatypeProperty;
        rdfs:label           "Message UID";
        rdfs:range           ocsf:string_t;
        dcterms:description  "The email header Message-Id value, as defined by RFC 5322." .

ocsf:match_details  rdf:type  owl:DatatypeProperty;
        rdfs:label           "Match Details";
        rdfs:range           ocsf:string_t;
        dcterms:description  "The data in a request that rule matched. For example: '[\"10\",\"and\",\"1\"]'." .

ocsf:NetworkConnectionInformation
        rdf:type             owl:Class;
        rdfs:label           "Network Connection Information";
        rdfs:subClassOf      ocsf:Object;
        dcterms:description  "The Network Connection Information object describes characteristics of a network connection. Defined by D3FEND <a target='_blank' href='https://d3fend.mitre.org/dao/artifact/d3f:NetworkSession/'>d3f:NetworkSession</a>.";
        ocsf:name            "network_connection_info" .

ocsf:proxy_connection_info
        rdf:type             owl:ObjectProperty;
        rdfs:label           "Proxy Connection Info";
        rdfs:range           ocsf:NetworkConnectionInformation;
        dcterms:description  "The connection information from the proxy server to the remote server." .

ocsf:Compliance  rdf:type    owl:Class;
        rdfs:label           "Compliance";
        rdfs:subClassOf      ocsf:Object;
        dcterms:description  "The Compliance object contains information about Industry and Regulatory Framework standards, controls and requirements.";
        ocsf:name            "compliance" .

ocsf:sandbox  rdf:type       owl:DatatypeProperty;
        rdfs:label           "Sandbox";
        rdfs:range           ocsf:string_t;
        dcterms:description  "The name of the containment jail (i.e., sandbox). For example, hardened_ps, high_security_ps, oracle_ps, netsvcs_ps, or default_ps." .

ocsf:status_id  rdf:type     owl:DatatypeProperty;
        rdfs:label           "Status ID";
        rdfs:range           ocsf:integer_t;
        dcterms:description  "The normalized identifier of the event status.";
        jsonschema:enum      "Failure" , "Success" , "Unknown" , "Other" .

ocsf:given_name  rdf:type    owl:DatatypeProperty;
        rdfs:label           "Given Name";
        rdfs:range           ocsf:string_t;
        dcterms:description  "The given or first name of the user." .

ocsf:name  rdf:type          owl:DatatypeProperty;
        rdfs:label           "Name";
        rdfs:range           ocsf:string_t;
        dcterms:description  "The name of the entity. See specific usage." .

ocsf:DigitalSignature
        rdf:type             owl:Class;
        rdfs:label           "Digital Signature";
        rdfs:subClassOf      ocsf:Object;
        rdfs:subClassOf      [ rdf:type            owl:Restriction;
                               owl:onProperty      ocsf:digest;
                               owl:someValuesFrom  ocsf:Fingerprint
                             ];
        rdfs:subClassOf      [ rdf:type            owl:Restriction;
                               owl:onProperty      ocsf:certificate;
                               owl:someValuesFrom  ocsf:DigitalCertificate
                             ];
        dcterms:description  "The Digital Signature object contains information about the cryptographic mechanism used to verify the authenticity, integrity, and origin of the file or application.";
        ocsf:name            "digital_signature" .

ocsf:access_result  rdf:type  owl:DatatypeProperty;
        rdfs:label           "Access Check Result";
        rdfs:range           ocsf:json_t;
        dcterms:description  "The list of access check results." .

ocsf:opcode_id  rdf:type     owl:DatatypeProperty;
        rdfs:label           "DNS Opcode ID";
        rdfs:range           ocsf:integer_t;
        dcterms:description  "The DNS opcode ID specifies the normalized query message type.";
        jsonschema:enum      "Inverse Query" , "DSO Message" , "Status" , "Notify" , "Query" , "Reserved" , "Update" .

ocsf:email_auth  rdf:type    owl:ObjectProperty;
        rdfs:label           "Email Authentication";
        rdfs:range           ocsf:EmailAuthentication;
        dcterms:description  "The SPF, DKIM and DMARC attributes of an email." .

ocsf:UserInfoEvent  rdf:type  owl:Class;
        rdfs:label           "User Info";
        rdfs:subClassOf      d3f:DigitalEvent;
        rdfs:subClassOf      [ rdf:type         owl:Restriction;
                               owl:cardinality  1;
                               owl:onProperty   ocsf:user
                             ];
        dcterms:description  "User Info events report user data that have been discovered, queried, polled or searched. This event differs from User Inventory as it describes the result of a targeted search by filtering a subset of user attributes.";
        ocsf:name            "user_info";
        ocsf:uid             18 .

ocsf:CVE  rdf:type           owl:Class;
        rdfs:label           "CVE";
        rdfs:subClassOf      ocsf:Object;
        rdfs:subClassOf      [ rdf:type            owl:Restriction;
                               owl:onProperty      ocsf:product;
                               owl:someValuesFrom  ocsf:Product
                             ];
        rdfs:subClassOf      [ rdf:type            owl:Restriction;
                               owl:onProperty      ocsf:epss;
                               owl:someValuesFrom  ocsf:EPSS
                             ];
        rdfs:subClassOf      [ rdf:type            owl:Restriction;
                               owl:onProperty      ocsf:cwe;
                               owl:someValuesFrom  ocsf:CWE
                             ];
        rdfs:subClassOf      [ rdf:type            owl:Restriction;
                               owl:onProperty      ocsf:cvss;
                               owl:someValuesFrom  ocsf:CVSSScore
                             ];
        dcterms:description  "The Common Vulnerabilities and Exposures (CVE) object represents publicly disclosed cybersecurity vulnerabilities defined in CVE Program catalog (<a target='_blank' href='https://cve.mitre.org/'>CVE</a>). There is one CVE Record for each vulnerability in the catalog.";
        ocsf:name            "cve" .

ocsf:stratum  rdf:type       owl:DatatypeProperty;
        rdfs:label           "Stratum";
        rdfs:range           ocsf:string_t;
        dcterms:description  "The stratum level of the NTP server's time source, normalized to the caption of the stratum_id value." .

ocsf:boolean_t  rdf:type     rdfs:Datatype;
        rdfs:label           "Boolean";
        rdfs:subClassOf      xsd:boolean;
        dcterms:description  "Boolean value. One of <code>true</code> or <code>false</code>." .

ocsf:os  rdf:type            owl:ObjectProperty;
        rdfs:label           "OS";
        rdfs:range           ocsf:OperatingSystemOS;
        dcterms:description  "The device operating system." .

ocsf:timestamp_t  rdf:type   rdfs:Datatype;
        rdfs:label           "Timestamp";
        rdfs:subClassOf      xsd:long;
        dcterms:description  "The timestamp format is the number of milliseconds since the Epoch 01/01/1970 00:00:00 UTC. For example <code>1618524549901</code>." .

ocsf:rcode  rdf:type         owl:DatatypeProperty;
        rdfs:label           "Response Code";
        rdfs:range           ocsf:string_t;
        dcterms:description  "The server response code, normalized to the caption of the rcode_id value. In the case of 'Other', it is defined by the event source." .

ocsf:DeviceHardwareInfo
        rdf:type             owl:Class;
        rdfs:label           "Device Hardware Info";
        rdfs:subClassOf      ocsf:Object;
        rdfs:subClassOf      [ rdf:type            owl:Restriction;
                               owl:onProperty      ocsf:keyboard_info;
                               owl:someValuesFrom  ocsf:KeyboardInformation
                             ];
        rdfs:subClassOf      [ rdf:type            owl:Restriction;
                               owl:onProperty      ocsf:desktop_display;
                               owl:someValuesFrom  ocsf:Display
                             ];
        dcterms:description  "The Device Hardware Information object contains details and specifications of the physical components that make up a device. This information provides an overview of the hardware capabilities, configuration, and characteristics of the device.";
        ocsf:name            "device_hw_info" .

ocsf:error_message  rdf:type  owl:DatatypeProperty;
        rdfs:label           "Error Message";
        rdfs:range           ocsf:string_t;
        dcterms:description  "Error Message" .

ocsf:ja3s_hash  rdf:type     owl:ObjectProperty;
        rdfs:label           "JA3S Hash";
        rdfs:range           ocsf:Fingerprint;
        dcterms:description  "The MD5 hash of a JA3S string." .

ocsf:credential_uid  rdf:type  owl:DatatypeProperty;
        rdfs:label           "User Credential ID";
        rdfs:range           ocsf:string_t;
        dcterms:description  "The unique identifier of the user's credential. For example, AWS Access Key ID." .

ocsf:log_version  rdf:type   owl:DatatypeProperty;
        rdfs:label           "Log Version";
        rdfs:range           ocsf:string_t;
        dcterms:description  "The event log schema version that specifies the format of the original event. For example syslog version or Cisco Log Schema Version." .

ocsf:KeyboardInformation
        rdf:type             owl:Class;
        rdfs:label           "Keyboard Information";
        rdfs:subClassOf      ocsf:Object;
        dcterms:description  "The Keyboard Information object contains details and attributes related to a computer or device keyboard. It encompasses information that describes the characteristics, capabilities, and configuration of the keyboard.";
        ocsf:name            "keyboard_info" .

ocsf:is_remote  rdf:type     owl:DatatypeProperty;
        rdfs:label           "Remote";
        rdfs:range           ocsf:boolean_t;
        dcterms:description  "The indication of whether the session is remote." .

ocsf:processed_time  rdf:type  owl:DatatypeProperty;
        rdfs:label           "Processed Time";
        rdfs:range           ocsf:timestamp_t;
        dcterms:description  "The event processed time, such as an ETL operation." .

ocsf:pod_uuid  rdf:type      owl:DatatypeProperty;
        rdfs:label           "Pod UUID";
        rdfs:range           ocsf:uuid_t;
        dcterms:description  "The unique identifier of the pod (or equivalent) that the container is executing on." .

ocsf:condition  rdf:type     owl:DatatypeProperty;
        rdfs:label           "Condition";
        rdfs:range           ocsf:string_t;
        dcterms:description  "The rule trigger condition for the rule. For example: SQL_INJECTION." .

ocsf:affected_code  rdf:type  owl:ObjectProperty;
        rdfs:label           "Affected Code";
        rdfs:range           ocsf:AffectedCode;
        dcterms:description  "List of Affected Code objects that describe details about code blocks identified as vulnerable." .

ocsf:creator  rdf:type       owl:ObjectProperty;
        rdfs:label           "Creator";
        rdfs:range           ocsf:User;
        dcterms:description  "The user that created the object associated with event. See specific usage." .

ocsf:auth_type_id  rdf:type  owl:DatatypeProperty;
        rdfs:label           "Authentication Type ID";
        rdfs:range           ocsf:integer_t;
        dcterms:description  "The normalized identifier of the agreed upon authentication type. See specific usage.";
        jsonschema:enum      "Unknown" , "Other" .

ocsf:reputation  rdf:type    owl:ObjectProperty;
        rdfs:label           "Reputation Scores";
        rdfs:range           ocsf:Reputation;
        dcterms:description  "Contains the original and normalized reputation scores." .

ocsf:is_system  rdf:type     owl:DatatypeProperty;
        rdfs:label           "System";
        rdfs:range           ocsf:boolean_t;
        dcterms:description  "The indication of whether the object is part of the operating system." .

ocsf:app  rdf:type           owl:ObjectProperty;
        rdfs:label           "Application";
        rdfs:range           ocsf:Product;
        dcterms:description  "The application that reported the event." .

ocsf:scale_factor  rdf:type  owl:DatatypeProperty;
        rdfs:label           "Scale Factor";
        rdfs:range           ocsf:integer_t;
        dcterms:description  "The numeric scale factor of display." .

ocsf:KernelExtension  rdf:type  owl:Class;
        rdfs:label           "Kernel Extension";
        rdfs:subClassOf      ocsf:Object;
        rdfs:subClassOf      [ rdf:type         owl:Restriction;
                               owl:cardinality  1;
                               owl:onProperty   ocsf:file
                             ];
        dcterms:description  "The Kernel Extension object describes a kernel driver that has been loaded or unloaded into the operating system (OS) kernel. Defined by D3FEND <a target='_blank' href='https://d3fend.mitre.org/dao/artifact/d3f:KernelModule/'>d3f:KernelModule</a>.";
        ocsf:name            "kernel_driver" .

ocsf:timezone_offset  rdf:type  owl:DatatypeProperty;
        rdfs:label           "Timezone Offset";
        rdfs:range           ocsf:integer_t;
        dcterms:description  "The number of minutes that the reported event <code>time</code> is ahead or behind UTC, in the range -1,080 to +1,080." .

ocsf:certificate  rdf:type   owl:ObjectProperty;
        rdfs:label           "Certificate";
        rdfs:range           ocsf:DigitalCertificate;
        dcterms:description  "The certificate object containing information about the digital certificate." .

ocsf:HTTPRequest  rdf:type   owl:Class;
        rdfs:label           "HTTP Request";
        rdfs:subClassOf      ocsf:Object;
        rdfs:subClassOf      [ rdf:type            owl:Restriction;
                               owl:onProperty      ocsf:url;
                               owl:someValuesFrom  ocsf:UniformResourceLocator
                             ];
        rdfs:subClassOf      [ rdf:type            owl:Restriction;
                               owl:onProperty      ocsf:http_headers;
                               owl:someValuesFrom  ocsf:HTTPHeader
                             ];
        dcterms:description  "The HTTP Request object represents the attributes of a request made to a web server. It encapsulates the details and metadata associated with an HTTP request, including the request method, headers, URL, query parameters, body content, and other relevant information.";
        ocsf:name            "http_request" .

ocsf:WebResourcesActivityEvent
        rdf:type             owl:Class;
        rdfs:label           "Web Resources Activity";
        rdfs:subClassOf      d3f:DigitalEvent;
        rdfs:subClassOf      [ rdf:type            owl:Restriction;
                               owl:onProperty      ocsf:http_request;
                               owl:someValuesFrom  ocsf:HTTPRequest
                             ];
        rdfs:subClassOf      [ rdf:type         owl:Restriction;
                               owl:cardinality  1;
                               owl:onProperty   ocsf:web_resources
                             ];
        rdfs:subClassOf      [ rdf:type            owl:Restriction;
                               owl:onProperty      ocsf:tls;
                               owl:someValuesFrom  ocsf:TransportLayerSecurityTLS
                             ];
        rdfs:subClassOf      [ rdf:type            owl:Restriction;
                               owl:onProperty      ocsf:web_resources_result;
                               owl:someValuesFrom  ocsf:WebResource
                             ];
        rdfs:subClassOf      [ rdf:type            owl:Restriction;
                               owl:onProperty      ocsf:dst_endpoint;
                               owl:someValuesFrom  ocsf:NetworkEndpoint
                             ];
        rdfs:subClassOf      [ rdf:type            owl:Restriction;
                               owl:onProperty      ocsf:http_response;
                               owl:someValuesFrom  ocsf:HTTPResponse
                             ];
        rdfs:subClassOf      [ rdf:type            owl:Restriction;
                               owl:onProperty      ocsf:src_endpoint;
                               owl:someValuesFrom  ocsf:NetworkEndpoint
                             ];
        dcterms:description  "Web Resources Activity events describe actions executed on a set of Web Resources.";
        ocsf:category        "application";
        ocsf:name            "web_resources_activity";
        ocsf:profiles        "[\"host\",\"network_proxy\",\"security_control\"]";
        ocsf:uid             1 .

ocsf:device  rdf:type        owl:ObjectProperty;
        rdfs:label           "Device";
        rdfs:range           ocsf:Device;
        dcterms:description  "An addressable device, computer system or host." .

ocsf:status_detail  rdf:type  owl:DatatypeProperty;
        rdfs:label           "Status Details";
        rdfs:range           ocsf:string_t;
        dcterms:description  "The status details contains additional information about the event/finding outcome." .

ocsf:DeviceInventoryInfoEvent
        rdf:type             owl:Class;
        rdfs:label           "Device Inventory Info";
        rdfs:subClassOf      d3f:DigitalEvent;
        rdfs:subClassOf      [ rdf:type         owl:Restriction;
                               owl:cardinality  1;
                               owl:onProperty   ocsf:device
                             ];
        rdfs:subClassOf      [ rdf:type            owl:Restriction;
                               owl:onProperty      ocsf:actor;
                               owl:someValuesFrom  ocsf:Actor
                             ];
        dcterms:description  "Device Inventory Info events report device inventory data.";
        ocsf:name            "inventory_info";
        ocsf:profiles        "[\"host\"]";
        ocsf:uid             1 .

ocsf:is_personal  rdf:type   owl:DatatypeProperty;
        rdfs:label           "Personal Device";
        rdfs:range           ocsf:boolean_t;
        dcterms:description  "The event occurred on a personal device." .

ocsf:EPSS  rdf:type          owl:Class;
        rdfs:label           "EPSS";
        rdfs:subClassOf      ocsf:Object;
        dcterms:description  "The Exploit Prediction Scoring System (EPSS) object describes the estimated probability a vulnerability will be exploited. EPSS is a community-driven effort to combine descriptive information about vulnerabilities (CVEs) with evidence of actual exploitation in-the-wild. (<a target='_blank' href='https://www.first.org/epss/'>EPSS</a>).";
        ocsf:name            "epss" .

ocsf:color_depth  rdf:type   owl:DatatypeProperty;
        rdfs:label           "Color Depth";
        rdfs:range           ocsf:integer_t;
        dcterms:description  "The numeric color depth." .

ocsf:API  rdf:type           owl:Class;
        rdfs:label           "API";
        rdfs:subClassOf      ocsf:Object;
        rdfs:subClassOf      [ rdf:type            owl:Restriction;
                               owl:onProperty      ocsf:service;
                               owl:someValuesFrom  ocsf:Service
                             ];
        rdfs:subClassOf      [ rdf:type            owl:Restriction;
                               owl:onProperty      ocsf:response;
                               owl:someValuesFrom  ocsf:ResponseElements
                             ];
        rdfs:subClassOf      [ rdf:type            owl:Restriction;
                               owl:onProperty      ocsf:request;
                               owl:someValuesFrom  ocsf:RequestElements
                             ];
        rdfs:subClassOf      [ rdf:type            owl:Restriction;
                               owl:onProperty      ocsf:group;
                               owl:someValuesFrom  ocsf:Group
                             ];
        dcterms:description  "The API, or Application Programming Interface, object represents  information pertaining to an API request and response.";
        ocsf:name            "api" .

ocsf:KernelObjectInfoEvent
        rdf:type             owl:Class;
        rdfs:label           "Kernel Object Info";
        rdfs:subClassOf      d3f:DigitalEvent;
        rdfs:subClassOf      [ rdf:type         owl:Restriction;
                               owl:cardinality  1;
                               owl:onProperty   ocsf:kernel
                             ];
        dcterms:description  "Kernel Object Info events report information about discovered kernel resources.";
        ocsf:name            "kernel_object_info";
        ocsf:uid             6 .

ocsf:ServiceInfoEvent
        rdf:type             owl:Class;
        rdfs:label           "Service Info";
        rdfs:subClassOf      d3f:DigitalEvent;
        rdfs:subClassOf      [ rdf:type         owl:Restriction;
                               owl:cardinality  1;
                               owl:onProperty   ocsf:service
                             ];
        dcterms:description  "Service Info events report information about running services.";
        ocsf:name            "service_info";
        ocsf:uid             16 .

ocsf:tid  rdf:type           owl:DatatypeProperty;
        rdfs:label           "Thread ID";
        rdfs:range           ocsf:integer_t;
        dcterms:description  "The Identifier of the thread associated with the event, as returned by the operating system." .

ocsf:boundary_id  rdf:type   owl:DatatypeProperty;
        rdfs:label           "Boundary ID";
        rdfs:range           ocsf:integer_t;
        dcterms:description  "<p>The normalized identifier of the boundary of the connection. </p><p> For cloud connections, this translates to the traffic-boundary (same VPC, through IGW, etc.). For traditional networks, this is described as Local, Internal, or External.</p>";
        jsonschema:enum      "Other" , "Unknown" , "External" , "Intra-region VPC" , "Inter-region VPC" , "Same VPC" , "Internet/VPC Gateway" , "Local Gateway" , "Gateway VPC" , "Virtual Private Gateway" , "Internet Gateway" , "Internal" , "Localhost" .

ocsf:UserSessionInfoEvent
        rdf:type             owl:Class;
        rdfs:label           "User Session Info";
        rdfs:subClassOf      d3f:DigitalEvent;
        rdfs:subClassOf      [ rdf:type         owl:Restriction;
                               owl:cardinality  1;
                               owl:onProperty   ocsf:session
                             ];
        dcterms:description  "User Session Info events report information about existing user sessions.";
        ocsf:name            "session_info";
        ocsf:uid             17 .

ocsf:is_http_only  rdf:type  owl:DatatypeProperty;
        rdfs:label           "HTTP Only";
        rdfs:range           ocsf:boolean_t;
        dcterms:description  "This attribute prevents the cookie from being accessed via JavaScript." .

ocsf:ModuleActivityEvent
        rdf:type             owl:Class;
        rdfs:label           "Module Activity";
        rdfs:subClassOf      d3f:DigitalEvent;
        rdfs:subClassOf      [ rdf:type         owl:Restriction;
                               owl:cardinality  1;
                               owl:onProperty   ocsf:module
                             ];
        rdfs:subClassOf      [ rdf:type         owl:Restriction;
                               owl:cardinality  1;
                               owl:onProperty   ocsf:actor
                             ];
        dcterms:description  "Module  Activity events report when a process loads or unloads the <code>module</code>.";
        ocsf:name            "module_activity";
        ocsf:uid             5 .

ocsf:session  rdf:type       owl:ObjectProperty;
        rdfs:label           "Session";
        rdfs:range           ocsf:Session;
        dcterms:description  "The authenticated user or service session." .

ocsf:issuer  rdf:type        owl:DatatypeProperty;
        rdfs:label           "Issuer Details";
        rdfs:range           ocsf:string_t;
        dcterms:description  "The identifier of the issuer. See specific usage." .

ocsf:cpe_name  rdf:type      owl:DatatypeProperty;
        rdfs:label           "The product CPE identifier";
        rdfs:range           ocsf:string_t;
        dcterms:description  "The Common Platform Enumeration (CPE) name as described by (<a target='_blank' href='https://nvd.nist.gov/products/cpe'>NIST</a>) For example: <code>cpe:/a:apple:safari:16.2</code>." .

ocsf:User  rdf:type          owl:Class;
        rdfs:label           "User";
        rdfs:subClassOf      ocsf:Entity;
        rdfs:subClassOf      [ rdf:type            owl:Restriction;
                               owl:onProperty      ocsf:account;
                               owl:someValuesFrom  ocsf:Account
                             ];
        rdfs:subClassOf      [ rdf:type            owl:Restriction;
                               owl:onProperty      ocsf:groups;
                               owl:someValuesFrom  ocsf:Group
                             ];
        rdfs:subClassOf      [ rdf:type            owl:Restriction;
                               owl:onProperty      ocsf:org;
                               owl:someValuesFrom  ocsf:Organization
                             ];
        rdfs:subClassOf      [ rdf:type            owl:Restriction;
                               owl:onProperty      ocsf:ldap_person;
                               owl:someValuesFrom  ocsf:LDAPPerson
                             ];
        dcterms:description  "The User object describes the characteristics of a user/person or a security principal. Defined by D3FEND <a target='_blank' href='https://d3fend.mitre.org/dao/artifact/d3f:UserAccount/'>d3f:UserAccount</a>.";
        ocsf:constraints     "{\"at_least_one\":[\"account\",\"name\",\"uid\"]}";
        ocsf:name            "user";
        ocsf:observable      21 .

ocsf:to  rdf:type            owl:DatatypeProperty;
        rdfs:label           "To";
        rdfs:range           ocsf:email_t;
        dcterms:description  "The email header To values, as defined by RFC 5322." .

ocsf:related_vulnerabilities
        rdf:type             owl:DatatypeProperty;
        rdfs:label           "Related Vulnerabilities";
        rdfs:range           ocsf:string_t;
        dcterms:description  "List of vulnerabilities that are related to this vulnerability." .

ocsf:ip_t  rdf:type          rdfs:Datatype;
        rdfs:label           "IP Address";
        rdfs:subClassOf      xsd:string;
        dcterms:description  "Internet Protocol address (IP address), in either IPv4 or IPv6 format. For example, <code>192.168.200.24</code> or <code>2001:0db8:85a3:0000:0000:8a2e:0370:7334</code>.";
        xsd:pattern          "((^\\s*((([0-9]|[1-9][0-9]|1[0-9]{2}|2[0-4][0-9]|25[0-5]).){3}([0-9]|[1-9][0-9]|1[0-9]{2}|2[0-4][0-9]|25[0-5]))\\s*$)|(^\\s*((([0-9A-Fa-f]{1,4}:){7}([0-9A-Fa-f]{1,4}|:))|(([0-9A-Fa-f]{1,4}:){6}(:[0-9A-Fa-f]{1,4}|((25[0-5]|2[0-4]\\d|1\\d\\d|[1-9]?\\d)(.(25[0-5]|2[0-4]\\d|1\\d\\d|[1-9]?\\d)){3})|:))|(([0-9A-Fa-f]{1,4}:){5}(((:[0-9A-Fa-f]{1,4}){1,2})|:((25[0-5]|2[0-4]\\d|1\\d\\d|[1-9]?\\d)(.(25[0-5]|2[0-4]\\d|1\\d\\d|[1-9]?\\d)){3})|:))|(([0-9A-Fa-f]{1,4}:){4}(((:[0-9A-Fa-f]{1,4}){1,3})|((:[0-9A-Fa-f]{1,4})?:((25[0-5]|2[0-4]\\d|1\\d\\d|[1-9]?\\d)(.(25[0-5]|2[0-4]\\d|1\\d\\d|[1-9]?\\d)){3}))|:))|(([0-9A-Fa-f]{1,4}:){3}(((:[0-9A-Fa-f]{1,4}){1,4})|((:[0-9A-Fa-f]{1,4}){0,2}:((25[0-5]|2[0-4]\\d|1\\d\\d|[1-9]?\\d)(.(25[0-5]|2[0-4]\\d|1\\d\\d|[1-9]?\\d)){3}))|:))|(([0-9A-Fa-f]{1,4}:){2}(((:[0-9A-Fa-f]{1,4}){1,5})|((:[0-9A-Fa-f]{1,4}){0,3}:((25[0-5]|2[0-4]\\d|1\\d\\d|[1-9]?\\d)(.(25[0-5]|2[0-4]\\d|1\\d\\d|[1-9]?\\d)){3}))|:))|(([0-9A-Fa-f]{1,4}:){1}(((:[0-9A-Fa-f]{1,4}){1,6})|((:[0-9A-Fa-f]{1,4}){0,4}:((25[0-5]|2[0-4]\\d|1\\d\\d|[1-9]?\\d)(.(25[0-5]|2[0-4]\\d|1\\d\\d|[1-9]?\\d)){3}))|:))|(:(((:[0-9A-Fa-f]{1,4}){1,7})|((:[0-9A-Fa-f]{1,4}){0,5}:((25[0-5]|2[0-4]\\d|1\\d\\d|[1-9]?\\d)(.(25[0-5]|2[0-4]\\d|1\\d\\d|[1-9]?\\d)){3}))|:)))(%.+)?\\s*$))" .

ocsf:depth  rdf:type         owl:DatatypeProperty;
        rdfs:label           "CVSS Depth";
        rdfs:range           ocsf:string_t;
        dcterms:description  "The CVSS depth represents a depth of the equation used to calculate CVSS score.";
        jsonschema:enum      "Temporal" , "Environmental" , "Base" .

ocsf:cis_benchmark  rdf:type  owl:ObjectProperty;
        rdfs:label           "CIS Benchmark";
        rdfs:range           ocsf:CISBenchmark;
        dcterms:description  "The CIS Benchmark describes best practices for securely configuring IT systems, software, networks, and cloud infrastructure as defined by the Center for Internet Security (<a target='_blank' href='https://www.cisecurity.org/cis-benchmarks/'>CIS</a>)." .

ocsf:certificate_chain
        rdf:type             owl:DatatypeProperty;
        rdfs:label           "Certificate Chain";
        rdfs:range           ocsf:string_t;
        dcterms:description  "The Chain of Certificate Serial Numbers field provides a chain of Certificate Issuer Serial Numbers leading to the Root Certificate Issuer." .

ocsf:RelatedEvent  rdf:type  owl:Class;
        rdfs:label           "Related Event";
        rdfs:subClassOf      ocsf:Object;
        rdfs:subClassOf      [ rdf:type            owl:Restriction;
                               owl:onProperty      ocsf:observables;
                               owl:someValuesFrom  ocsf:Observable
                             ];
        rdfs:subClassOf      [ rdf:type            owl:Restriction;
                               owl:onProperty      ocsf:kill_chain;
                               owl:someValuesFrom  ocsf:KillChainPhase
                             ];
        rdfs:subClassOf      [ rdf:type            owl:Restriction;
                               owl:onProperty      ocsf:attacks;
                               owl:someValuesFrom  ocsf:MITREATTCK
                             ];
        dcterms:description  "The Related Event object describes an event related to a finding or detection as identified by the security product.";
        ocsf:name            "related_event" .

ocsf:hw_info  rdf:type       owl:ObjectProperty;
        rdfs:label           "Hardware Info";
        rdfs:range           ocsf:DeviceHardwareInfo;
        dcterms:description  "The device hardware information." .

ocsf:pid  rdf:type           owl:DatatypeProperty;
        rdfs:label           "Process ID";
        rdfs:range           ocsf:integer_t;
        dcterms:description  "The process identifier, as reported by the operating system. Process ID (PID) is a number used by the operating system to uniquely identify an active process." .

ocsf:tree_uid  rdf:type      owl:DatatypeProperty;
        rdfs:label           "Tree UID";
        rdfs:range           ocsf:string_t;
        dcterms:description  "The tree id is a unique SMB identifier which represents an open connection to a share." .

ocsf:control  rdf:type       owl:DatatypeProperty;
        rdfs:label           "Security Control";
        rdfs:range           ocsf:string_t;
        dcterms:description  "A Control is prescriptive, prioritized, and simplified set of best practices that one can use to strengthen their cybersecurity posture. e.g. AWS SecurityHub Controls, CIS Controls." .

ocsf:proxy_traffic  rdf:type  owl:ObjectProperty;
        rdfs:label           "Proxy Traffic";
        rdfs:range           ocsf:NetworkTraffic;
        dcterms:description  "The network traffic refers to the amount of data moving across a network, from proxy to remote server at a given point of time." .

ocsf:keyboard_layout  rdf:type  owl:DatatypeProperty;
        rdfs:label           "Keyboard Layout";
        rdfs:range           ocsf:string_t;
        dcterms:description  "The keyboard locale identifier name (e.g., en-US)." .

ocsf:folder  rdf:type        owl:ObjectProperty;
        rdfs:label           "Folder";
        rdfs:range           ocsf:File;
        dcterms:description  "The folder that pertains to the event." .

ocsf:project_uid  rdf:type   owl:DatatypeProperty;
        rdfs:label           "Project ID";
        rdfs:range           ocsf:string_t;
        dcterms:description  "The unique identifier of a Cloud project." .

ocsf:user_result  rdf:type   owl:ObjectProperty;
        rdfs:label           "User Result";
        rdfs:range           ocsf:User;
        dcterms:description  "The result of the user account change. It should contain the new values of the changed attributes." .

ocsf:subdomain  rdf:type     owl:DatatypeProperty;
        rdfs:label           "Subdomain";
        rdfs:range           ocsf:string_t;
        dcterms:description  "The subdomain portion of the URL. For example: <code>sub</code> in <code>https://sub.example.com</code> or <code>sub2.sub1</code> in <code>https://sub2.sub1.example.com</code>." .

ocsf:resource  rdf:type      owl:ObjectProperty;
        rdfs:label           "Resource";
        rdfs:range           ocsf:ResourceDetails;
        dcterms:description  "The target resource." .

ocsf:Malware  rdf:type       owl:Class;
        rdfs:label           "Malware";
        rdfs:subClassOf      ocsf:Entity;
        rdfs:subClassOf      [ rdf:type            owl:Restriction;
                               owl:onProperty      ocsf:cves;
                               owl:someValuesFrom  ocsf:CVE
                             ];
        dcterms:description  "The Malware object describes the classification of known malicious software, which is intentionally designed to cause damage to a computer, server, client, or computer network.";
        ocsf:name            "malware" .

ocsf:first_seen_time  rdf:type  owl:DatatypeProperty;
        rdfs:label           "First Seen";
        rdfs:range           ocsf:timestamp_t;
        dcterms:description  "The initial detection time of the activity or object. See specific usage" .

ocsf:packets_out  rdf:type   owl:DatatypeProperty;
        rdfs:label           "Packets Out";
        rdfs:range           ocsf:long_t;
        dcterms:description  "The number of packets sent from the source to the destination." .

ocsf:expiration_time  rdf:type  owl:DatatypeProperty;
        rdfs:label           "Expiration Time";
        rdfs:range           ocsf:timestamp_t;
        dcterms:description  "The expiration time. See specific usage." .

ocsf:subnet  rdf:type        owl:DatatypeProperty;
        rdfs:label           "Subnet";
        rdfs:range           ocsf:subnet_t;
        dcterms:description  "The subnet mask." .

ocsf:Account  rdf:type       owl:Class;
        rdfs:label           "Account";
        rdfs:subClassOf      ocsf:Entity;
        dcterms:description  "The Account object contains details about the account that initiated or performed a specific activity within a system or application.";
        ocsf:name            "account" .

ocsf:fix_available  rdf:type  owl:DatatypeProperty;
        rdfs:label           "Fix Availability";
        rdfs:range           ocsf:boolean_t;
        dcterms:description  "Indicates if a fix is available for the reported vulnerability." .

ocsf:ApplicationActivityEvent
        rdf:type         owl:Class;
        rdfs:label       "Application Activity";
        rdfs:subClassOf  d3f:DigitalEvent;
        ocsf:category    "application";
        ocsf:name        "application" .

ocsf:hostname  rdf:type      owl:DatatypeProperty;
        rdfs:label           "Hostname";
        rdfs:range           ocsf:hostname_t;
        dcterms:description  "The hostname of an endpoint or a device." .

ocsf:cpu_speed  rdf:type     owl:DatatypeProperty;
        rdfs:label           "Processor Speed";
        rdfs:range           ocsf:integer_t;
        dcterms:description  "The speed of the processor in Mhz. For Example: <code>4200</code>." .

ocsf:ip  rdf:type            owl:DatatypeProperty;
        rdfs:label           "IP Address";
        rdfs:range           ocsf:ip_t;
        dcterms:description  "The IP address, in either IPv4 or IPv6 format." .

ocsf:Metadata  rdf:type      owl:Class;
        rdfs:label           "Metadata";
        rdfs:subClassOf      ocsf:Object;
        rdfs:subClassOf      [ rdf:type         owl:Restriction;
                               owl:cardinality  1;
                               owl:onProperty   ocsf:product
                             ];
        rdfs:subClassOf      [ rdf:type            owl:Restriction;
                               owl:onProperty      ocsf:loggers;
                               owl:someValuesFrom  ocsf:Logger
                             ];
        rdfs:subClassOf      [ rdf:type            owl:Restriction;
                               owl:onProperty      ocsf:extensions;
                               owl:someValuesFrom  ocsf:SchemaExtension
                             ];
        rdfs:subClassOf      [ rdf:type            owl:Restriction;
                               owl:onProperty      ocsf:extension;
                               owl:someValuesFrom  ocsf:SchemaExtension
                             ];
        dcterms:description  "The Metadata object describes the metadata associated with the event. Defined by D3FEND <a target='_blank' href='https://d3fend.mitre.org/dao/artifact/d3f:Metadata/'>d3f:Metadata</a>.";
        ocsf:name            "metadata" .

ocsf:cves  rdf:type          owl:ObjectProperty;
        rdfs:label           "CVE List";
        rdfs:range           ocsf:CVE;
        dcterms:description  "List of Common Vulnerabilities and Exposures (<a target='_blank' href='https://cve.mitre.org/'>CVE</a>)." .

ocsf:epss  rdf:type          owl:ObjectProperty;
        rdfs:label           "EPSS";
        rdfs:range           ocsf:EPSS;
        dcterms:description  "The Exploit Prediction Scoring System (EPSS) object describes the estimated probability a vulnerability will be exploited. EPSS is a community-driven effort to combine descriptive information about vulnerabilities (CVEs) with evidence of actual exploitation in-the-wild. (<a target='_blank' href='https://www.first.org/epss/'>EPSS</a>)." .

ocsf:proxy_endpoint  rdf:type  owl:ObjectProperty;
        rdfs:label           "Proxy Endpoint";
        rdfs:range           ocsf:NetworkProxyEndpoint;
        dcterms:description  "The proxy (server) in a network connection." .
