@prefix d3f: <http://d3fend.mitre.org/ontologies/d3fend.owl#> .
@prefix dcterms: <http://purl.org/dc/terms/> .
@prefix jsonschema: <https://www.w3.org/2019/wot/json-schema#> .
@prefix ocsf: <https://schema.ocsf.io/1.3.0/ontology/> .
@prefix owl: <http://www.w3.org/2002/07/owl#> .
@prefix rdf: <http://www.w3.org/1999/02/22-rdf-syntax-ns#> .
@prefix rdfs: <http://www.w3.org/2000/01/rdf-schema#> .
@prefix xsd: <http://www.w3.org/2001/XMLSchema#> .

ocsf: a owl:Ontology ;
    owl:imports <http://d3fend.mitre.org/ontologies/d3fend.owl> .

### Object Properties

ocsf:accessor a owl:ObjectProperty ;
    rdfs:label "Accessor" ;
    rdfs:range ocsf:User ;
    dcterms:description "The name of the user who last accessed the object." .

ocsf:account a owl:ObjectProperty ;
    rdfs:label "Account" ;
    rdfs:range ocsf:Account ;
    dcterms:description "The account object describes details about the account that was the source or target of the activity." .

ocsf:actor a owl:ObjectProperty ;
    rdfs:label "Actor" ;
    rdfs:range ocsf:Actor ;
    dcterms:description "The actor object describes details about the user/role/process that was the source of the activity." .

ocsf:affected_code a owl:ObjectProperty ;
    rdfs:label "Affected Code" ;
    rdfs:range ocsf:AffectedCode ;
    dcterms:description "List of Affected Code objects that describe details about code blocks identified as vulnerable." .

ocsf:affected_packages a owl:ObjectProperty ;
    rdfs:label "Affected Software Packages" ;
    rdfs:range ocsf:AffectedSoftwarePackage ;
    dcterms:description "List of software packages identified as affected by a vulnerability/vulnerabilities." .

ocsf:agent a owl:ObjectProperty ;
    rdfs:label "Agent" ;
    rdfs:range ocsf:Agent ;
    dcterms:description "An Agent (also known as a Sensor) is typically installed on an Operating System (OS) and serves as a specialized software component that can be designed to monitor, detect, collect, archive, or take action. These activities and possible actions are defined by the upstream system controlling the Agent and its intended purpose. For instance, an Agent can include Endpoint Detection & Response (EDR) agents, backup/disaster recovery sensors, Application Performance Monitoring or profiling sensors, and similar software." .

ocsf:agent_list a owl:ObjectProperty ;
    rdfs:label "Agent List" ;
    rdfs:range ocsf:Agent ;
    dcterms:description "A list of <code>agent</code> objects associated with a device, endpoint, or resource." .

ocsf:analytic a owl:ObjectProperty ;
    rdfs:label "Analytic" ;
    rdfs:range ocsf:Analytic ;
    dcterms:description "The analytic technique used to analyze and derive insights from the data or information that led to the finding or conclusion." .

ocsf:answers a owl:ObjectProperty ;
    rdfs:label "DNS Answer" ;
    rdfs:range ocsf:DNSAnswer ;
    dcterms:description "The Domain Name System (DNS) answers." .

ocsf:api a owl:ObjectProperty ;
    rdfs:label "API Details" ;
    rdfs:range ocsf:API ;
    dcterms:description "Describes details about a typical API (Application Programming Interface) call." .

ocsf:app a owl:ObjectProperty ;
    rdfs:label "Application" ;
    rdfs:range ocsf:Product ;
    dcterms:description "The application that reported the event." .

ocsf:assignee a owl:ObjectProperty ;
    rdfs:label "Assignee" ;
    rdfs:range ocsf:User ;
    dcterms:description "The details of the user assigned to an Incident." .

ocsf:assignee_group a owl:ObjectProperty ;
    rdfs:label "Assignee Group" ;
    rdfs:range ocsf:Group ;
    dcterms:description "The details of the group assigned to an Incident." .

ocsf:attacks a owl:ObjectProperty ;
    rdfs:label "MITRE ATT&CK® Details" ;
    rdfs:range ocsf:MITREATTCK ;
    dcterms:description "An array of <a target='_blank' href='https://attack.mitre.org'>MITRE ATT&CK®</a> objects describing the tactics, techniques & sub-techniques identified by a security control or finding." .

ocsf:auth_factors a owl:ObjectProperty ;
    rdfs:label "Authentication Factors" ;
    rdfs:range ocsf:AuthenticationFactor ;
    dcterms:description "Describes a category of methods used for identity verification in an authentication attempt." .

ocsf:authorizations a owl:ObjectProperty ;
    rdfs:label "Authorization Information" ;
    rdfs:range ocsf:AuthorizationResult ;
    dcterms:description "Provides details about an authorization, such as authorization outcome, and any associated policies related to the activity/event." .

ocsf:autonomous_system a owl:ObjectProperty ;
    rdfs:label "Autonomous System" ;
    rdfs:range ocsf:AutonomousSystem ;
    dcterms:description "The Autonomous System details associated with an IP address." .

ocsf:avg_timespan a owl:ObjectProperty ;
    rdfs:label "Average Timespan" ;
    rdfs:range ocsf:TimeSpan ;
    dcterms:description "The average time span of an activity." .

ocsf:certificate a owl:ObjectProperty ;
    rdfs:label "Certificate" ;
    rdfs:range ocsf:DigitalCertificate ;
    dcterms:description "The certificate object containing information about the digital certificate." .

ocsf:cis_benchmark a owl:ObjectProperty ;
    rdfs:label "CIS Benchmark" ;
    rdfs:range ocsf:CISBenchmark ;
    dcterms:description "The CIS Benchmark describes best practices for securely configuring IT systems, software, networks, and cloud infrastructure as defined by the Center for Internet Security (<a target='_blank' href='https://www.cisecurity.org/cis-benchmarks/'>CIS</a>)." .

ocsf:cis_benchmark_result a owl:ObjectProperty ;
    rdfs:label "CIS Benchmark Result" ;
    rdfs:range ocsf:CISBenchmarkResult ;
    dcterms:description "The CIS benchmark result." .

ocsf:cis_controls a owl:ObjectProperty ;
    rdfs:label "CIS Controls" ;
    rdfs:range ocsf:CISControl ;
    dcterms:description "The CIS Critical Security Controls is a prioritized set of actions to protect your organization and data from cyber-attack vectors." .

ocsf:cis_csc a owl:ObjectProperty ;
    rdfs:label "CIS CSC" ;
    rdfs:range ocsf:CISCSC ;
    dcterms:description "The CIS Critical Security Controls is a list of top 20 actions and practices an organization’s security team can take on such that cyber attacks or malware, are minimized and prevented." .

ocsf:client_hassh a owl:ObjectProperty ;
    rdfs:label "Client HASSH" ;
    rdfs:range ocsf:HASSH ;
    dcterms:description "The Client HASSH fingerprinting object." .

ocsf:cloud a owl:ObjectProperty ;
    rdfs:label "Cloud" ;
    rdfs:range ocsf:Cloud ;
    dcterms:description "Describes details about the Cloud environment where the event was originally created or logged." .

ocsf:compliance a owl:ObjectProperty ;
    rdfs:label "Compliance" ;
    rdfs:range ocsf:Compliance ;
    dcterms:description "The compliance object provides context to compliance findings (e.g., a check against a specific regulatory or best practice framework such as CIS, NIST etc.) and contains compliance related details." .

ocsf:compliance_references a owl:ObjectProperty ;
    rdfs:label "Complaince References Articles" ;
    rdfs:range ocsf:KBArticle ;
    dcterms:description "A list of sources of information or tools that help organizations understand, interpret, and implement compliance standards. They provide guidance, best practices, and examples." .

ocsf:compliance_standards a owl:ObjectProperty ;
    rdfs:label "Compliance Standards Articles" ;
    rdfs:range ocsf:KBArticle ;
    dcterms:description "A list of established guidelines or criteria that define specific requirements an organization must follow." .

ocsf:connection_info a owl:ObjectProperty ;
    rdfs:label "Connection Info" ;
    rdfs:range ocsf:NetworkConnectionInformation ;
    dcterms:description "The network connection information." .

ocsf:container a owl:ObjectProperty ;
    rdfs:label "Container" ;
    rdfs:range ocsf:Container ;
    dcterms:description "The information describing an instance of a container. A container is a prepackaged, portable system image that runs isolated on an existing system using a container runtime like containerd." .

ocsf:containers a owl:ObjectProperty ;
    rdfs:label "Containers" ;
    rdfs:range ocsf:Container ;
    dcterms:description "When working with containerized applications, the set of containers which write to the standard the output of a particular logging driver. For example, this may be the set of containers involved in handling api requests and responses for a containerized application." .

ocsf:countermeasures a owl:ObjectProperty ;
    rdfs:label "Countermeasures" ;
    rdfs:range ocsf:MITRED3FEND ;
    dcterms:description "The MITRE DEFEND™ Matrix Countermeasures associated with a remediation." .

ocsf:creator a owl:ObjectProperty ;
    rdfs:label "Creator" ;
    rdfs:range ocsf:User ;
    dcterms:description "The user that created the object associated with event. See specific usage." .

ocsf:cve a owl:ObjectProperty ;
    rdfs:label "CVE" ;
    rdfs:range ocsf:CVE ;
    dcterms:description "The Common Vulnerabilities and Exposures (<a target='_blank' href='https://cve.mitre.org/'>CVE</a>)." .

ocsf:cves a owl:ObjectProperty ;
    rdfs:label "CVE List" ;
    rdfs:range ocsf:CVE ;
    dcterms:description "List of Common Vulnerabilities and Exposures (<a target='_blank' href='https://cve.mitre.org/'>CVE</a>)." .

ocsf:cvss a owl:ObjectProperty ;
    rdfs:label "CVSS Score" ;
    rdfs:range ocsf:CVSSScore ;
    dcterms:description "The CVSS object details Common Vulnerability Scoring System (<a target='_blank' href='https://www.first.org/cvss/'>CVSS</a>) scores from the advisory that are related to the vulnerability." .

ocsf:cwe a owl:ObjectProperty ;
    rdfs:label "CWE" ;
    rdfs:range ocsf:CWE ;
    dcterms:description "The CWE object represents a weakness in a software system that can be exploited by a threat actor to perform an attack. The CWE object is based on the <a target='_blank' href='https://cwe.mitre.org/'>Common Weakness Enumeration (CWE)</a> catalog." .

ocsf:d3f_tactic a owl:ObjectProperty ;
    rdfs:label "MITRE DEFEND™ Tactic" ;
    rdfs:range ocsf:MITRED3FENDTactic ;
    dcterms:description "The D3FEND Tactic object describes the defensive tactic name associated with a countermeasure, as defined by <a target='_blank' href='https://d3fend.mitre.org'>D3FEND<sup>TM</sup> Matrix</a>." .

ocsf:d3f_technique a owl:ObjectProperty ;
    rdfs:label "MITRE DEFEND™ Technique" ;
    rdfs:range ocsf:MITREDEFENDTechnique ;
    dcterms:description "The D3FEND Technique object describes the defensive technique ID and/or name associated with a countermeasure, as defined by <a target='_blank' href='https://d3fend.mitre.org'>D3FEND<sup>TM</sup> Matrix</a>." .

ocsf:data_classification a owl:ObjectProperty ;
    rdfs:label "Data Classification" ;
    rdfs:range ocsf:DataClassification ;
    dcterms:description "The Data Classification object includes information about data classification levels and data category types." .

ocsf:data_security a owl:ObjectProperty ;
    rdfs:label "Data Security" ;
    dcterms:description "The Data Security object describes the characteristics, techniques and content of a Data Loss Prevention (DLP), Data Loss Detection (DLD), Data Classification, or similar tools' finding, alert, or detection mechanism(s)." .

ocsf:database a owl:ObjectProperty ;
    rdfs:label "Database" ;
    rdfs:range ocsf:Database ;
    dcterms:description "The database object is used for databases which are typically datastore services that contain an organized collection of structured and unstructured data or a types of data." .

ocsf:databucket a owl:ObjectProperty ;
    rdfs:label "Databucket" ;
    rdfs:range ocsf:Databucket ;
    dcterms:description "The data bucket object is a basic container that holds data, typically organized through the use of data partitions." .

ocsf:dce_rpc a owl:ObjectProperty ;
    rdfs:label "Distributed Computing Environment/Remote Procedure Call (DCE/RPC)" ;
    rdfs:range ocsf:DCERPC ;
    dcterms:description "The DCE/RPC object describes the remote procedure call system for distributed computing environments." .

ocsf:desktop_display a owl:ObjectProperty ;
    rdfs:label "Desktop Display" ;
    rdfs:range ocsf:Display ;
    dcterms:description "The desktop display affiliated with the event" .

ocsf:device a owl:ObjectProperty ;
    rdfs:label "Device" ;
    rdfs:range ocsf:Device ;
    dcterms:description "An addressable device, computer system or host." .

ocsf:devices a owl:ObjectProperty ;
    rdfs:label "Devices" ;
    rdfs:range ocsf:Device ;
    dcterms:description "The object describes details related to the list of devices." .

ocsf:digest a owl:ObjectProperty ;
    rdfs:label "Message Digest" ;
    rdfs:range ocsf:Fingerprint ;
    dcterms:description "The message digest attribute contains the fixed length message hash representation and the corresponding hashing algorithm information." .

ocsf:domain_contact a owl:ObjectProperty ;
    rdfs:label "Domain Contact" ;
    rdfs:range ocsf:DomainContact ;
    dcterms:description "The contact information related to a domain registration, e.g., registrant, administrator, abuse, billing, or technical contact." .

ocsf:domain_contacts a owl:ObjectProperty ;
    rdfs:label "Domain Contacts" ;
    rdfs:range ocsf:DomainContact ;
    dcterms:description "An array of <code>Domain Contact</code> objects." .

ocsf:driver a owl:ObjectProperty ;
    rdfs:label "Kernel Driver" ;
    rdfs:range ocsf:KernelExtension ;
    dcterms:description "The driver that was loaded/unloaded into the kernel" .

ocsf:dst_endpoint a owl:ObjectProperty ;
    rdfs:label "Destination Endpoint" ;
    rdfs:range ocsf:NetworkEndpoint ;
    dcterms:description "The network destination endpoint." .

ocsf:email a owl:ObjectProperty ;
    rdfs:label "Email" ;
    rdfs:range ocsf:Email ;
    dcterms:description "The email object." .

ocsf:email_auth a owl:ObjectProperty ;
    rdfs:label "Email Authentication" ;
    rdfs:range ocsf:EmailAuthentication ;
    dcterms:description "The SPF, DKIM and DMARC attributes of an email." .

ocsf:endpoint_connections a owl:ObjectProperty ;
    rdfs:label "Endpoint Connections" ;
    rdfs:range ocsf:EndpointConnection ;
    dcterms:description "Contains information about network connection attempts. See specific usage." .

ocsf:enrichments a owl:ObjectProperty ;
    rdfs:label "Enrichments" ;
    rdfs:range ocsf:Enrichment ;
    dcterms:description "The additional information from an external data source, which is associated with the event or a finding. For example add location information for the IP address in the DNS answers:</p><code>[{\"name\": \"answers.ip\", \"value\": \"92.24.47.250\", \"type\": \"location\", \"data\": {\"city\": \"Socotra\", \"continent\": \"Asia\", \"coordinates\": [-25.4153, 17.0743], \"country\": \"YE\", \"desc\": \"Yemen\"}}]</code>" .

ocsf:entity a owl:ObjectProperty ;
    rdfs:label "Entity" ;
    rdfs:range ocsf:ManagedEntity ;
    dcterms:description "The managed entity that is being acted upon." .

ocsf:entity_result a owl:ObjectProperty ;
    rdfs:label "Entity Result" ;
    rdfs:range ocsf:ManagedEntity ;
    dcterms:description "The updated managed entity." .

ocsf:epss a owl:ObjectProperty ;
    rdfs:label "EPSS" ;
    rdfs:range ocsf:EPSS ;
    dcterms:description "The Exploit Prediction Scoring System (EPSS) object describes the estimated probability a vulnerability will be exploited. EPSS is a community-driven effort to combine descriptive information about vulnerabilities (CVEs) with evidence of actual exploitation in-the-wild. (<a target='_blank' href='https://www.first.org/epss/'>EPSS</a>)." .

ocsf:evidences a owl:ObjectProperty ;
    rdfs:label "Evidence Artifacts" ;
    rdfs:range ocsf:EvidenceArtifacts ;
    dcterms:description "Describes various evidence artifacts associated to the activity/activities that triggered a security detection." .

ocsf:extension a owl:ObjectProperty ;
    rdfs:label "Schema Extension" ;
    rdfs:range ocsf:SchemaExtension ;
    dcterms:description "The schema extension used to create the event." .

ocsf:extension_list a owl:ObjectProperty ;
    rdfs:label "Extension List" ;
    rdfs:range ocsf:TLSExtension ;
    dcterms:description "The list of TLS extensions." .

ocsf:extensions a owl:ObjectProperty ;
    rdfs:label "Schema Extensions" ;
    rdfs:range ocsf:SchemaExtension ;
    dcterms:description "The schema extensions used to create the event." .

ocsf:feature a owl:ObjectProperty ;
    rdfs:label "Feature" ;
    rdfs:range ocsf:Feature ;
    dcterms:description "The feature that reported the event." .

ocsf:file a owl:ObjectProperty ;
    rdfs:label "File" ;
    rdfs:range ocsf:File ;
    dcterms:description "The file that pertains to the event or object. See specific usage." .

ocsf:file_result a owl:ObjectProperty ;
    rdfs:label "File Result" ;
    rdfs:range ocsf:File ;
    dcterms:description "The result of the file change. It should contain the new values of the changed attributes." .

ocsf:finding a owl:ObjectProperty ;
    rdfs:label "Finding" ;
    rdfs:range ocsf:Finding,
        ocsf:FindingEvent ;
    dcterms:description "The Finding object provides details about a finding/detection generated by a security tool." .

ocsf:finding_info a owl:ObjectProperty ;
    rdfs:label "Finding Information" ;
    rdfs:range ocsf:FindingInformation ;
    dcterms:description "Describes the supporting information about a generated finding." .

ocsf:finding_info_list a owl:ObjectProperty ;
    rdfs:label "Finding Information List" ;
    rdfs:range ocsf:FindingInformation ;
    dcterms:description "A list of <code>finding_info</code> objects associated to an incident." .

ocsf:fingerprint a owl:ObjectProperty ;
    rdfs:label "Fingerprint" ;
    rdfs:range ocsf:Fingerprint ;
    dcterms:description "The digital fingerprint associated with an object." .

ocsf:fingerprints a owl:ObjectProperty ;
    rdfs:label "Fingerprints" ;
    rdfs:range ocsf:Fingerprint ;
    dcterms:description "An array of digital fingerprint objects." .

ocsf:firewall_rule a owl:ObjectProperty ;
    rdfs:label "Firewall Rule" ;
    rdfs:range ocsf:FirewallRule ;
    dcterms:description "The firewall rule that triggered the event." .

ocsf:folder a owl:ObjectProperty ;
    rdfs:label "Folder" ;
    rdfs:range ocsf:File ;
    dcterms:description "The folder that pertains to the event." .

ocsf:group a owl:ObjectProperty ;
    rdfs:label "Group" ;
    rdfs:range ocsf:Group ;
    dcterms:description "The group object associated with an entity such as user, policy, or rule." .

ocsf:groups a owl:ObjectProperty ;
    rdfs:label "Groups" ;
    rdfs:range ocsf:Group ;
    dcterms:description "The groups to which an entity belongs. See specific usage." .

ocsf:hash a owl:ObjectProperty ;
    rdfs:label "Hash" ;
    rdfs:range ocsf:Fingerprint ;
    dcterms:description "The hash attribute is the value of a digital fingerprint including information about its algorithm." .

ocsf:hashes a owl:ObjectProperty ;
    rdfs:label "Hashes" ;
    rdfs:range ocsf:Fingerprint ;
    dcterms:description "An array of hash attributes." .

ocsf:http_cookies a owl:ObjectProperty ;
    rdfs:label "HTTP Cookies" ;
    rdfs:range ocsf:HTTPCookie ;
    dcterms:description "The cookies object describes details about HTTP cookies" .

ocsf:http_headers a owl:ObjectProperty ;
    rdfs:label "HTTP Headers" ;
    rdfs:range ocsf:HTTPHeader ;
    dcterms:description "Additional HTTP headers of an HTTP request or response." .

ocsf:http_request a owl:ObjectProperty ;
    rdfs:label "HTTP Request" ;
    rdfs:range ocsf:HTTPRequest ;
    dcterms:description "The HTTP Request Object documents attributes of a request made to a web server." .

ocsf:http_response a owl:ObjectProperty ;
    rdfs:label "HTTP Response" ;
    rdfs:range ocsf:HTTPResponse ;
    dcterms:description "The HTTP Response from a web server to a requester." .

ocsf:hw_info a owl:ObjectProperty ;
    rdfs:label "Hardware Info" ;
    rdfs:range ocsf:DeviceHardwareInfo ;
    dcterms:description "The endpoint hardware information." .

ocsf:idp a owl:ObjectProperty ;
    rdfs:label "Identity Provider" ;
    rdfs:range ocsf:IdentityProvider ;
    dcterms:description "This object describes details about the Identity Provider used." .

ocsf:image a owl:ObjectProperty ;
    rdfs:label "Image" ;
    rdfs:range ocsf:Image ;
    dcterms:description "The image used as a template to run a container or virtual machine." .

ocsf:ja3_hash a owl:ObjectProperty ;
    rdfs:label "JA3 Hash" ;
    rdfs:range ocsf:Fingerprint ;
    dcterms:description "The MD5 hash of a JA3 string." .

ocsf:ja3s_hash a owl:ObjectProperty ;
    rdfs:label "JA3S Hash" ;
    rdfs:range ocsf:Fingerprint ;
    dcterms:description "The MD5 hash of a JA3S string." .

ocsf:ja4_fingerprint_list a owl:ObjectProperty ;
    rdfs:label "JA4+ Fingerprints" ;
    rdfs:range ocsf:JA4Fingerprint ;
    dcterms:description "A list of the JA4+ network fingerprints." .

ocsf:job a owl:ObjectProperty ;
    rdfs:label "Job" ;
    rdfs:range ocsf:Job ;
    dcterms:description "The job object that pertains to the event." .

ocsf:kb_article_list a owl:ObjectProperty ;
    rdfs:label "Knowledgebase Articles" ;
    rdfs:range ocsf:KBArticle ;
    dcterms:description "A list of KB articles or patches related to an endpoint. A KB Article contains metadata that describes the patch or an update." .

ocsf:kernel a owl:ObjectProperty ;
    rdfs:label "Kernel" ;
    rdfs:range ocsf:KernelResource ;
    dcterms:description "The kernel resource object that pertains to the event." .

ocsf:keyboard_info a owl:ObjectProperty ;
    rdfs:label "Keyboard Information" ;
    rdfs:range ocsf:KeyboardInformation ;
    dcterms:description "The keyboard detailed information." .

ocsf:kill_chain a owl:ObjectProperty ;
    rdfs:label "Kill Chain" ;
    rdfs:range ocsf:KillChainPhase ;
    dcterms:description "The <a target='_blank' href='https://www.lockheedmartin.com/en-us/capabilities/cyber/cyber-kill-chain.html'>Cyber Kill Chain®</a> provides a detailed description of each phase and its associated activities within the broader context of a cyber attack." .

ocsf:ldap_person a owl:ObjectProperty ;
    rdfs:label "LDAP Person" ;
    rdfs:range ocsf:LDAPPerson ;
    dcterms:description "The additional LDAP attributes that describe a person." .

ocsf:load_balancer a owl:ObjectProperty ;
    rdfs:label "Load Balancer" ;
    rdfs:range ocsf:LoadBalancer ;
    dcterms:description "The Load Balancer object contains information related to the device that is distributing incoming traffic to specified destinations." .

ocsf:location a owl:ObjectProperty ;
    rdfs:label "Geo Location" ;
    rdfs:range ocsf:GeoLocation ;
    dcterms:description "The detailed geographical location usually associated with an IP address." .

ocsf:loggers a owl:ObjectProperty ;
    rdfs:label "Loggers" ;
    rdfs:range ocsf:Logger ;
    dcterms:description "An array of Logger objects that describe the devices and logging products between the event source and its eventual destination. Note, this attribute can be used when there is a complex end-to-end path of event flow." .

ocsf:logon_process a owl:ObjectProperty ;
    rdfs:label "Logon Process" ;
    rdfs:range ocsf:Process ;
    dcterms:description "The trusted process that validated the authentication credentials." .

ocsf:malware a owl:ObjectProperty ;
    rdfs:label "Malware" ;
    rdfs:range ocsf:Malware ;
    dcterms:description "A list of Malware objects, describing details about the identified malware." .

ocsf:manager a owl:ObjectProperty ;
    rdfs:label "Manager" ;
    rdfs:range ocsf:User ;
    dcterms:description "The user's manager. This helps in understanding an org hierarchy. This should only ever be populated once in an event. I.e. there should not be a manager's manager in an event." .

ocsf:metadata a owl:ObjectProperty ;
    rdfs:label "Metadata" ;
    rdfs:range ocsf:Metadata ;
    dcterms:description "The metadata associated with the event or a finding." .

ocsf:metrics a owl:ObjectProperty ;
    rdfs:label "Metrics" ;
    rdfs:range ocsf:Metric ;
    dcterms:description "The general purpose metrics associated with the event. See specific usage." .

ocsf:modifier a owl:ObjectProperty ;
    rdfs:label "Modifier" ;
    rdfs:range ocsf:User ;
    dcterms:description "The user that last modified the object associated with the event. See specific usage." .

ocsf:module a owl:ObjectProperty ;
    rdfs:label "Module" ;
    rdfs:range ocsf:Module ;
    dcterms:description "The module that pertains to the event." .

ocsf:network_endpoint a owl:ObjectProperty ;
    rdfs:label "Network Endpoint" ;
    rdfs:range ocsf:NetworkEndpoint ;
    dcterms:description "The Network Endpoint object describes characteristics of a network endpoint. See specific usage." .

ocsf:network_interfaces a owl:ObjectProperty ;
    rdfs:label "Network Interfaces" ;
    rdfs:range ocsf:NetworkInterface ;
    dcterms:description "The network interfaces that are associated with the device, one for each unique MAC address/IP address/hostname/name combination.<p><b>Note:</b> The first element of the array is the network information that pertains to the event.</p>" .

ocsf:observables a owl:ObjectProperty ;
    rdfs:label "Observables" ;
    rdfs:range ocsf:Observable ;
    dcterms:description "The observables associated with the event or a finding." .

ocsf:org a owl:ObjectProperty ;
    rdfs:label "Organization" ;
    rdfs:range ocsf:Organization ;
    dcterms:description "Organization and org unit relevant to the event or object." .

ocsf:os a owl:ObjectProperty ;
    rdfs:label "OS" ;
    rdfs:range ocsf:OperatingSystemOS ;
    dcterms:description "The endpoint operating system." .

ocsf:osint a owl:ObjectProperty ;
    rdfs:label "OSINT" ;
    rdfs:range ocsf:OSINT ;
    dcterms:description "The OSINT (Open Source Intelligence) object contains details related to an indicator such as the indicator itself, related indicators, geolocation, registrar information, subdomains, analyst commentary, and other contextual information. This information can be used to further enrich a detection or finding by providing decisioning support to other analysts and engineers." .

ocsf:owner a owl:ObjectProperty ;
    rdfs:label "Owner" ;
    rdfs:range ocsf:User ;
    dcterms:description "The user that owns the file/object." .

ocsf:package a owl:ObjectProperty ;
    rdfs:label "Software Package" ;
    rdfs:range ocsf:SoftwarePackage ;
    dcterms:description "The Software Package object describes details about a software package. Defined by D3FEND <a target='_blank' href='https://d3fend.mitre.org/dao/artifact/d3f:SoftwarePackage/'>d3f:SoftwarePackage</a>." .

ocsf:packages a owl:ObjectProperty ;
    rdfs:label "Software Packages" ;
    rdfs:range ocsf:SoftwarePackage ;
    dcterms:description "List of vulnerable packages as identified by the security product" .

ocsf:parent_process a owl:ObjectProperty ;
    rdfs:label "Parent Process" ;
    rdfs:range ocsf:Process ;
    dcterms:description "The parent process of this process object. It is recommended to only populate this field for the first process object, to prevent deep nesting." .

ocsf:peripheral_device a owl:ObjectProperty ;
    rdfs:label "Peripheral Device" ;
    rdfs:range ocsf:PeripheralDevice ;
    dcterms:description "The peripheral device that triggered the event." .

ocsf:policies a owl:ObjectProperty ;
    rdfs:label "Policies" ;
    rdfs:range ocsf:Policy ;
    dcterms:description "An array of <code>Policy</code> objects." .

ocsf:policy a owl:ObjectProperty ;
    rdfs:label "Policy" ;
    rdfs:range ocsf:Policy ;
    dcterms:description "Describes details of a policy. See specific usage." .

ocsf:prev_security_states a owl:ObjectProperty ;
    rdfs:label "Previous Security States" ;
    dcterms:description "The previous security states. See specific usage." .

ocsf:process a owl:ObjectProperty ;
    rdfs:label "Process" ;
    rdfs:range ocsf:Process ;
    dcterms:description "The process object." .

ocsf:product a owl:ObjectProperty ;
    rdfs:label "Product" ;
    rdfs:range ocsf:Product ;
    dcterms:description "The product that reported the event." .

ocsf:proxy a owl:ObjectProperty ;
    rdfs:label "Proxy" ;
    rdfs:range ocsf:NetworkProxyEndpoint ;
    dcterms:description "The proxy (server) in a network connection." .

ocsf:proxy_connection_info a owl:ObjectProperty ;
    rdfs:label "Proxy Connection Info" ;
    rdfs:range ocsf:NetworkConnectionInformation ;
    dcterms:description "The connection information from the proxy server to the remote server." .

ocsf:proxy_endpoint a owl:ObjectProperty ;
    rdfs:label "Proxy Endpoint" ;
    rdfs:range ocsf:NetworkProxyEndpoint ;
    dcterms:description "The proxy (server) in a network connection." .

ocsf:proxy_http_request a owl:ObjectProperty ;
    rdfs:label "Proxy HTTP Request" ;
    rdfs:range ocsf:HTTPRequest ;
    dcterms:description "The HTTP Request from the proxy server to the remote server." .

ocsf:proxy_http_response a owl:ObjectProperty ;
    rdfs:label "Proxy HTTP Response" ;
    rdfs:range ocsf:HTTPResponse ;
    dcterms:description "The HTTP Response from the remote server to the proxy server." .

ocsf:proxy_tls a owl:ObjectProperty ;
    rdfs:label "Proxy TLS" ;
    rdfs:range ocsf:TransportLayerSecurityTLS ;
    dcterms:description "The TLS protocol negotiated between the proxy server and the remote server." .

ocsf:proxy_traffic a owl:ObjectProperty ;
    rdfs:label "Proxy Traffic" ;
    rdfs:range ocsf:NetworkTraffic ;
    dcterms:description "The network traffic refers to the amount of data moving across a network, from proxy to remote server at a given point of time." .

ocsf:query a owl:ObjectProperty ;
    rdfs:label "DNS Query" ;
    rdfs:range ocsf:DNSQuery ;
    dcterms:description "The Domain Name System (DNS) query." .

ocsf:query_info a owl:ObjectProperty ;
    rdfs:label "Query Info" ;
    rdfs:range ocsf:QueryInformation ;
    dcterms:description "The query info object holds information related to data access within a datastore. To access, manipulate, delete, or retrieve data from a datastore, a database query must be written using a specific syntax." .

ocsf:related_analytics a owl:ObjectProperty ;
    rdfs:label "Related Analytics" ;
    rdfs:range ocsf:Analytic ;
    dcterms:description "Describes analytics related to the analytic of a finding or detection as identified by the security product." .

ocsf:related_events a owl:ObjectProperty ;
    rdfs:label "Related Events" ;
    rdfs:range ocsf:RelatedEvent ;
    dcterms:description "Describes events and/or other findings related to the finding as identified by the security product." .

ocsf:relay a owl:ObjectProperty ;
    rdfs:label "Relay" ;
    rdfs:range ocsf:NetworkInterface ;
    dcterms:description "The network relay that is associated with the event." .

ocsf:remediation a owl:ObjectProperty ;
    rdfs:label "Remediation Guidance" ;
    rdfs:range ocsf:Remediation ;
    dcterms:description "Describes the recommended remediation steps to address identified issue(s)." .

ocsf:remote_display a owl:ObjectProperty ;
    rdfs:label "Remote Display" ;
    rdfs:range ocsf:Display ;
    dcterms:description "The remote display affiliated with the event" .

ocsf:reputation a owl:ObjectProperty ;
    rdfs:label "Reputation Scores" ;
    rdfs:range ocsf:Reputation ;
    dcterms:description "Contains the original and normalized reputation scores." .

ocsf:request a owl:ObjectProperty ;
    rdfs:label "API Request Details" ;
    rdfs:range ocsf:RequestElements ;
    dcterms:description "General Purpose API Request Object. See specific usage" .

ocsf:resource a owl:ObjectProperty ;
    rdfs:label "Resource" ;
    rdfs:range ocsf:ResourceDetails ;
    dcterms:description "The target resource." .

ocsf:resources a owl:ObjectProperty ;
    rdfs:label "Resources Array" ;
    rdfs:range ocsf:ResourceDetails ;
    dcterms:description "Describes details about resources that were affected by the activity/event." .

ocsf:resources_result a owl:ObjectProperty ;
    rdfs:label "Resource Results Array" ;
    rdfs:range ocsf:ResourceDetails ;
    dcterms:description "Updated resources after an activity/event." .

ocsf:response a owl:ObjectProperty ;
    rdfs:label "API Response Details" ;
    rdfs:range ocsf:ResponseElements ;
    dcterms:description "General Purpose API Response Object. See specific usage." .

ocsf:rpc_interface a owl:ObjectProperty ;
    rdfs:label "Remote Procedure Call Interface" ;
    rdfs:range ocsf:RPCInterface ;
    dcterms:description "The RPC Interface object describes the details pertaining to the remote procedure call interface." .

ocsf:rule a owl:ObjectProperty ;
    rdfs:label "Rule" ;
    rdfs:range ocsf:Rule ;
    dcterms:description "The rules that reported the events." .

ocsf:sans a owl:ObjectProperty ;
    rdfs:label "Subject Alternative Names" ;
    rdfs:range ocsf:SubjectAlternativeName ;
    dcterms:description "The list of subject alternative names that are secured by a specific certificate." .

ocsf:scan a owl:ObjectProperty ;
    rdfs:label "Scan" ;
    rdfs:range ocsf:Scan ;
    dcterms:description "The Scan object describes characteristics of a scan.  See specific usage." .

ocsf:security_states a owl:ObjectProperty ;
    rdfs:label "Security States" ;
    dcterms:description "The current security states. See specific usage." .

ocsf:server_hassh a owl:ObjectProperty ;
    rdfs:label "Server HASSH" ;
    rdfs:range ocsf:HASSH ;
    dcterms:description "The Server HASSH fingerprinting object." .

ocsf:service a owl:ObjectProperty ;
    rdfs:label "Service" ;
    rdfs:range ocsf:Service ;
    dcterms:description "The service that pertains to the event." .

ocsf:session a owl:ObjectProperty ;
    rdfs:label "Session" ;
    rdfs:range ocsf:Session ;
    dcterms:description "The authenticated user or service session." .

ocsf:signature a owl:ObjectProperty ;
    rdfs:label "Digital Signature" ;
    rdfs:range ocsf:DigitalSignature ;
    dcterms:description "The digital signature of the file." .

ocsf:signatures a owl:ObjectProperty ;
    rdfs:label "Digital Signatures" ;
    rdfs:range ocsf:DigitalSignature ;
    dcterms:description "A collection of <code>Digital Signature</code> objects." .

ocsf:src_endpoint a owl:ObjectProperty ;
    rdfs:label "Source Endpoint" ;
    rdfs:range ocsf:NetworkEndpoint ;
    dcterms:description "The network source endpoint." .

ocsf:sub_technique a owl:ObjectProperty ;
    rdfs:label "Sub Technique" ;
    rdfs:range ocsf:MITREATTCKSubTechnique ;
    dcterms:description "The Sub Technique object describes the sub technique ID and/or name associated to an attack, as defined by <a target='_blank' href='https://attack.mitre.org/wiki/ATT&CK_Matrix'>ATT&CK® Matrix</a>." .

ocsf:table a owl:ObjectProperty ;
    rdfs:label "Table" ;
    rdfs:range ocsf:Table ;
    dcterms:description "The table object represents a table within a structured relational database or datastore, which contains columns and rows of data that are able to be create, updated, deleted and queried." .

ocsf:tactic a owl:ObjectProperty ;
    rdfs:label "Tactic" ;
    rdfs:range ocsf:MITREATTCKTactic ;
    dcterms:description "The Tactic object describes the tactic ID and/or name that is associated to an attack, as defined by <a target='_blank' href='https://attack.mitre.org/wiki/ATT&CK_Matrix'>ATT&CK® Matrix</a>." .

ocsf:tactics a owl:ObjectProperty ;
    rdfs:label "Tactics" ;
    rdfs:range ocsf:MITREATTCKTactic ;
    dcterms:description "The Tactic object describes the tactic ID and/or tactic name that are associated with the attack technique, as defined by <a target='_blank' href='https://attack.mitre.org/wiki/ATT&CK_Matrix'>ATT&CK® Matrix</a>." .

ocsf:technique a owl:ObjectProperty ;
    rdfs:label "Technique" ;
    rdfs:range ocsf:MITREATTCKTechnique ;
    dcterms:description "The Technique object describes the technique ID and/or name associated to an attack, as defined by <a target='_blank' href='https://attack.mitre.org/wiki/ATT&CK_Matrix'>ATT&CK® Matrix</a>." .

ocsf:ticket a owl:ObjectProperty ;
    rdfs:label "Ticket" ;
    rdfs:range ocsf:Ticket ;
    dcterms:description "The linked ticket in the ticketing system." .

ocsf:tls a owl:ObjectProperty ;
    rdfs:label "TLS" ;
    rdfs:range ocsf:TransportLayerSecurityTLS ;
    dcterms:description "The Transport Layer Security (TLS) attributes." .

ocsf:tls_extension_list a owl:ObjectProperty ;
    rdfs:label "TLS Extension List" ;
    rdfs:range ocsf:TLSExtension ;
    dcterms:description "The list of TLS extensions." .

ocsf:traffic a owl:ObjectProperty ;
    rdfs:label "Traffic" ;
    rdfs:range ocsf:NetworkTraffic ;
    dcterms:description "The network traffic refers to the amount of data moving across a network at a given point of time. Intended to be used alongside Network Connection." .

ocsf:tunnel_interface a owl:ObjectProperty ;
    rdfs:label "Interface" ;
    rdfs:range ocsf:NetworkInterface ;
    dcterms:description "The information about the tunnel interface. See specific usage." .

ocsf:unmapped a owl:ObjectProperty ;
    rdfs:label "Unmapped Data" ;
    rdfs:range ocsf:Object ;
    dcterms:description "The attributes that are not mapped to the event schema. The names and values of those attributes are specific to the event source." .

ocsf:url a owl:ObjectProperty ;
    rdfs:label "URL" ;
    rdfs:range ocsf:UniformResourceLocator ;
    dcterms:description "The URL object that pertains to the event or object. See specific usage." .

ocsf:user a owl:ObjectProperty ;
    rdfs:label "User" ;
    rdfs:range ocsf:User ;
    dcterms:description "The user that pertains to the event or object." .

ocsf:user_result a owl:ObjectProperty ;
    rdfs:label "User Result" ;
    rdfs:range ocsf:User ;
    dcterms:description "The result of the user account change. It should contain the new values of the changed attributes." .

ocsf:users a owl:ObjectProperty ;
    rdfs:label "Users" ;
    rdfs:range ocsf:User ;
    dcterms:description "The users that pertain to the event or object." .

ocsf:vulnerabilities a owl:ObjectProperty ;
    rdfs:label "Vulnerabilities" ;
    rdfs:range ocsf:VulnerabilityDetails ;
    dcterms:description "This object describes vulnerabilities reported in a security finding." .

ocsf:vulnerability a owl:ObjectProperty ;
    rdfs:label "Vulnerability" ;
    rdfs:range ocsf:VulnerabilityDetails ;
    dcterms:description "The vulnerability object describes details related to the observed vulnerability" .

ocsf:web_resources a owl:ObjectProperty ;
    rdfs:label "Web Resources" ;
    rdfs:range ocsf:WebResource ;
    dcterms:description "Describes details about web resources that were affected by an activity/event." .

ocsf:web_resources_result a owl:ObjectProperty ;
    rdfs:label "Web Resources Result" ;
    rdfs:range ocsf:WebResource ;
    dcterms:description "The results of the activity on web resources. It should contain the new values of the changed attributes of the web resources." .

ocsf:whois a owl:ObjectProperty ;
    rdfs:label "WHOIS" ;
    rdfs:range ocsf:WHOIS ;
    dcterms:description "The resources of a WHOIS record for a given domain. This can include domain names, IP address blocks, autonomous system information, and/or contact and registration information for a domain." .

ocsf:xattributes a owl:ObjectProperty ;
    rdfs:label "Extended Attributes" ;
    rdfs:range ocsf:Object ;
    dcterms:description "An unordered collection of zero or more name/value pairs where each pair represents a file or folder extended attribute.</p>For example: Windows alternate data stream attributes (ADS stream name, ADS size, etc.), user-defined or application-defined attributes, ACL, owner, primary group, etc. Examples from DCS: </p><ul><li><strong>ads_name</strong></li><li><strong>ads_size</strong></li><li><strong>dacl</strong></li><li><strong>owner</strong></li><li><strong>primary_group</strong></li><li><strong>link_name</strong> - name of the link associated to the file.</li><li><strong>hard_link_count</strong> - the number of links that are associated to the file.</li></ul>" .

### Datatypes

ocsf:boolean_t a rdfs:Datatype ;
    rdfs:label "Boolean" ;
    rdfs:subClassOf xsd:boolean ;
    dcterms:description "Boolean value. One of <code>true</code> or <code>false</code>." .

ocsf:bytestring_t a rdfs:Datatype ;
    rdfs:label "Byte String" ;
    rdfs:subClassOf xsd:string ;
    dcterms:description "Base64 encoded immutable byte sequence." .

ocsf:datetime_t a rdfs:Datatype ;
    rdfs:label "Datetime" ;
    rdfs:subClassOf xsd:string ;
    dcterms:description "The Internet Date/Time format as defined in <a target='_blank' href='https://www.rfc-editor.org/rfc/rfc3339.html'>RFC-3339</a>. For example <code>1985-04-12T23:20:50.52Z</code>." ;
    xsd:pattern "^\\d{4}-\\d{2}-\\d{2}T\\d{2}:\\d{2}:\\d{2}(?:\\.\\d+)?(Z|[\\+-]\\d{2}:\\d{2})?$" .

ocsf:email_t a rdfs:Datatype ;
    rdfs:label "Email Address" ;
    rdfs:subClassOf xsd:string ;
    dcterms:description "Email address. For example: <code>john_doe@example.com</code>." ;
    xsd:pattern "^[a-zA-Z0-9!#$%&'*+-/=?^_`{|}~.]+@[a-zA-Z0-9-]+\\.[a-zA-Z0-9-.]+$" .

ocsf:file_hash_t a rdfs:Datatype ;
    rdfs:label "Hash" ;
    rdfs:subClassOf xsd:string ;
    dcterms:description "Hash. A unique value that corresponds to the content of the file, image, ja3_hash or hassh found in the schema. For example MD5: <code>3172ac7e2b55cbb81f04a6e65855a628</code>." .

ocsf:file_name_t a rdfs:Datatype ;
    rdfs:label "File Name" ;
    rdfs:subClassOf xsd:string ;
    dcterms:description "File name. For example: <code>text-file.txt</code>." .

ocsf:float_t a rdfs:Datatype ;
    rdfs:label "Float" ;
    rdfs:subClassOf xsd:decimal ;
    dcterms:description "Real floating-point value. For example: <code>3.14</code>." .

ocsf:hostname_t a rdfs:Datatype ;
    rdfs:label "Hostname" ;
    rdfs:subClassOf xsd:string ;
    dcterms:description "Unique name assigned to a device connected to a computer network. A domain name in general is an Internet address that can be resolved through the Domain Name System (DNS). For example: <code>r2-d2.example.com</code>." ;
    xsd:pattern "^(([a-zA-Z0-9]|[a-zA-Z0-9][a-zA-Z0-9\\-]*[a-zA-Z0-9])\\.)*([A-Za-z0-9]|[A-Za-z0-9][A-Za-z0-9\\-]*[A-Za-z0-9])$" .

ocsf:integer_t a rdfs:Datatype ;
    rdfs:label "Integer" ;
    rdfs:subClassOf xsd:integer ;
    dcterms:description "Signed integer value." .

ocsf:ip_t a rdfs:Datatype ;
    rdfs:label "IP Address" ;
    rdfs:subClassOf xsd:string ;
    dcterms:description "Internet Protocol address (IP address), in either IPv4 or IPv6 format. For example, <code>192.168.200.24</code> or <code>2001:0db8:85a3:0000:0000:8a2e:0370:7334</code>." ;
    xsd:pattern "((^\\s*((([0-9]|[1-9][0-9]|1[0-9]{2}|2[0-4][0-9]|25[0-5]).){3}([0-9]|[1-9][0-9]|1[0-9]{2}|2[0-4][0-9]|25[0-5]))\\s*$)|(^\\s*((([0-9A-Fa-f]{1,4}:){7}([0-9A-Fa-f]{1,4}|:))|(([0-9A-Fa-f]{1,4}:){6}(:[0-9A-Fa-f]{1,4}|((25[0-5]|2[0-4]\\d|1\\d\\d|[1-9]?\\d)(.(25[0-5]|2[0-4]\\d|1\\d\\d|[1-9]?\\d)){3})|:))|(([0-9A-Fa-f]{1,4}:){5}(((:[0-9A-Fa-f]{1,4}){1,2})|:((25[0-5]|2[0-4]\\d|1\\d\\d|[1-9]?\\d)(.(25[0-5]|2[0-4]\\d|1\\d\\d|[1-9]?\\d)){3})|:))|(([0-9A-Fa-f]{1,4}:){4}(((:[0-9A-Fa-f]{1,4}){1,3})|((:[0-9A-Fa-f]{1,4})?:((25[0-5]|2[0-4]\\d|1\\d\\d|[1-9]?\\d)(.(25[0-5]|2[0-4]\\d|1\\d\\d|[1-9]?\\d)){3}))|:))|(([0-9A-Fa-f]{1,4}:){3}(((:[0-9A-Fa-f]{1,4}){1,4})|((:[0-9A-Fa-f]{1,4}){0,2}:((25[0-5]|2[0-4]\\d|1\\d\\d|[1-9]?\\d)(.(25[0-5]|2[0-4]\\d|1\\d\\d|[1-9]?\\d)){3}))|:))|(([0-9A-Fa-f]{1,4}:){2}(((:[0-9A-Fa-f]{1,4}){1,5})|((:[0-9A-Fa-f]{1,4}){0,3}:((25[0-5]|2[0-4]\\d|1\\d\\d|[1-9]?\\d)(.(25[0-5]|2[0-4]\\d|1\\d\\d|[1-9]?\\d)){3}))|:))|(([0-9A-Fa-f]{1,4}:){1}(((:[0-9A-Fa-f]{1,4}){1,6})|((:[0-9A-Fa-f]{1,4}){0,4}:((25[0-5]|2[0-4]\\d|1\\d\\d|[1-9]?\\d)(.(25[0-5]|2[0-4]\\d|1\\d\\d|[1-9]?\\d)){3}))|:))|(:(((:[0-9A-Fa-f]{1,4}){1,7})|((:[0-9A-Fa-f]{1,4}){0,5}:((25[0-5]|2[0-4]\\d|1\\d\\d|[1-9]?\\d)(.(25[0-5]|2[0-4]\\d|1\\d\\d|[1-9]?\\d)){3}))|:)))(%.+)?\\s*$))" .

ocsf:json_t a rdfs:Datatype ;
    rdfs:label "JSON" ;
    rdfs:subClassOf rdf:JSON ;
    dcterms:description "Embedded JSON value. A value can be a string, or a number, or true or false or null, or an object or an array. These structures can be nested. See <a target='_blank' href='https://www.json.org'>www.json.org</a>." .

ocsf:long_t a rdfs:Datatype ;
    rdfs:label "Long" ;
    rdfs:subClassOf xsd:long ;
    dcterms:description "8-byte long, signed integer value." .

ocsf:mac_t a rdfs:Datatype ;
    rdfs:label "MAC Address" ;
    rdfs:subClassOf xsd:string ;
    dcterms:description "Media Access Control (MAC) address. For example: <code>18:36:F3:98:4F:9A</code>." ;
    xsd:pattern "^([0-9A-Fa-f]{2}[:-]){5}([0-9A-Fa-f]{2})$" .

ocsf:port_t a rdfs:Datatype ;
    rdfs:label "Port" ;
    rdfs:subClassOf xsd:integer ;
    dcterms:description "The TCP/UDP port number. For example: <code>80</code> or <code>22</code>." ;
    xsd:maxInclusive 65535 ;
    xsd:minInclusive 0 .

ocsf:process_name_t a rdfs:Datatype ;
    rdfs:label "Process Name" ;
    rdfs:subClassOf xsd:string ;
    dcterms:description "Process name. For example: <code>Notepad</code>." .

ocsf:resource_uid_t a rdfs:Datatype ;
    rdfs:label "Resource UID" ;
    rdfs:subClassOf xsd:string ;
    dcterms:description "Resource unique identifier. For example, S3 Bucket name or EC2 Instance ID." .

ocsf:string_t a rdfs:Datatype ;
    rdfs:label "String" ;
    rdfs:subClassOf xsd:string ;
    dcterms:description "UTF-8 encoded byte sequence." .

ocsf:subnet_t a rdfs:Datatype ;
    rdfs:label "Subnet" ;
    rdfs:subClassOf xsd:string ;
    dcterms:description "The subnet represented in a CIDR notation, using the format network_address/prefix_length. The network_address can be in either IPv4 or IPv6 format. The prefix length indicates the number of bits used for the network portion, and the remaining bits are available for host addresses within that subnet. <div>For example:<ul><li>192.168.1.0/24</li><li>2001:0db8:85a3:0000::/64</li></ul></div>" .

ocsf:timestamp_t a rdfs:Datatype ;
    rdfs:label "Timestamp" ;
    rdfs:subClassOf xsd:long ;
    dcterms:description "The timestamp format is the number of milliseconds since the Epoch 01/01/1970 00:00:00 UTC. For example <code>1618524549901</code>." .

ocsf:url_t a rdfs:Datatype ;
    rdfs:label "URL String" ;
    rdfs:subClassOf xsd:string ;
    dcterms:description "Uniform Resource Locator (URL) string. For example: <code>http://www.example.com/download/trouble.exe</code>." .

ocsf:username_t a rdfs:Datatype ;
    rdfs:label "User Name" ;
    rdfs:subClassOf xsd:string ;
    dcterms:description "User name. For example: <code>john_doe</code>." .

ocsf:uuid_t a rdfs:Datatype ;
    rdfs:label "UUID" ;
    rdfs:subClassOf xsd:string ;
    dcterms:description "128-bit universal unique identifier. For example: <code>123e4567-e89b-12d3-a456-42661417400</code>." ;
    xsd:pattern "[0-9a-fA-F]{8}-[0-9a-fA-F]{4}-[0-9a-fA-F]{4}-[0-9a-fA-F]{4}-[0-9a-fA-F]{12}" .

### Data Properties

ocsf:access_list a owl:DatatypeProperty ;
    rdfs:label "Access List" ;
    rdfs:range ocsf:string_t ;
    dcterms:description "The list of requested access rights." .

ocsf:access_mask a owl:DatatypeProperty ;
    rdfs:label "Access Mask" ;
    rdfs:range ocsf:integer_t ;
    dcterms:description "The access mask in a platform-native format." .

ocsf:access_result a owl:DatatypeProperty ;
    rdfs:label "Access Check Result" ;
    rdfs:range ocsf:json_t ;
    dcterms:description "The list of access check results." .

ocsf:accessed_time a owl:DatatypeProperty ;
    rdfs:label "Accessed Time" ;
    rdfs:range ocsf:timestamp_t ;
    dcterms:description "The time when the file was last accessed." .

ocsf:ack_reason a owl:DatatypeProperty ;
    rdfs:label "Acknowledgement Reason" ;
    rdfs:range ocsf:integer_t ;
    dcterms:description "An integer that provides a reason code or additional information about the acknowledgment result." .

ocsf:ack_result a owl:DatatypeProperty ;
    rdfs:label "Acknowledgement Result" ;
    rdfs:range ocsf:integer_t ;
    dcterms:description "An integer that denotes the acknowledgment result of the DCE/RPC call." .

ocsf:action a owl:DatatypeProperty ;
    rdfs:label "Action" ;
    rdfs:range ocsf:string_t ;
    dcterms:description "The normalized caption of 'action_id' or the source specific action." .

ocsf:action_id a owl:DatatypeProperty ;
    rdfs:label "Action ID" ;
    rdfs:range ocsf:integer_t ;
    dcterms:description "The normalized action taken by a control or other policy-based system leading to an outcome or disposition." ;
    jsonschema:enum "Allowed",
        "Denied",
        "Other",
        "Unknown" .

ocsf:activity_id a owl:DatatypeProperty ;
    rdfs:label "Activity ID" ;
    rdfs:range ocsf:integer_t ;
    dcterms:description "The normalized identifier of the activity that triggered the event." ;
    jsonschema:enum "Other",
        "Unknown" .

ocsf:activity_name a owl:DatatypeProperty ;
    rdfs:label "Activity" ;
    rdfs:range ocsf:string_t ;
    dcterms:description "The event activity name, as defined by the activity_id." .

ocsf:actual_permissions a owl:DatatypeProperty ;
    rdfs:label "Actual Permissions" ;
    rdfs:range ocsf:integer_t ;
    dcterms:description "The permissions that were granted to the in a platform-native format." .

ocsf:alert a owl:DatatypeProperty ;
    rdfs:label "Client TLS Alert" ;
    rdfs:range ocsf:integer_t ;
    dcterms:description "The integer value of TLS alert if present. The alerts are defined in the TLS specification in <a target='_blank' href='https://datatracker.ietf.org/doc/html/rfc2246'>RFC-2246</a>." .

ocsf:algorithm a owl:DatatypeProperty ;
    rdfs:label "Algorithm" ;
    rdfs:range ocsf:string_t ;
    dcterms:description "The applicable algorithm, normalized to the caption of 'algorithm_id'. See specific usage." .

ocsf:algorithm_id a owl:DatatypeProperty ;
    rdfs:label "Algorithm ID" ;
    rdfs:range ocsf:integer_t ;
    dcterms:description "The normalized identifier of the algorithm. See specific usage." ;
    jsonschema:enum "Other",
        "Unknown" .

ocsf:app_name a owl:DatatypeProperty ;
    rdfs:label "Application Name" ;
    rdfs:range ocsf:string_t ;
    dcterms:description "The name of the application associated with the event or object." .

ocsf:app_uid a owl:DatatypeProperty ;
    rdfs:label "Application ID" ;
    rdfs:range ocsf:string_t ;
    dcterms:description "The unique ID of the application associated with the event or object." .

ocsf:architecture a owl:DatatypeProperty ;
    rdfs:label "Architecture" ;
    rdfs:range ocsf:string_t ;
    dcterms:description "Architecture is a shorthand name describing the type of computer hardware the packaged software is meant to run on." .

ocsf:args a owl:DatatypeProperty ;
    rdfs:label "HTTP Arguments" ;
    rdfs:range ocsf:string_t ;
    dcterms:description "The arguments sent along with the HTTP request." .

ocsf:attempt a owl:DatatypeProperty ;
    rdfs:label "Attempt" ;
    rdfs:range ocsf:integer_t ;
    dcterms:description "The delivery attempt." .

ocsf:attributes a owl:DatatypeProperty ;
    rdfs:label "Attributes" ;
    rdfs:range ocsf:integer_t ;
    dcterms:description "The bitmask value that represents the file attributes." .

ocsf:auth_protocol a owl:DatatypeProperty ;
    rdfs:label "Auth Protocol" ;
    rdfs:range ocsf:string_t ;
    dcterms:description "The authentication protocol as defined by the caption of 'auth_protocol_id'. In the case of 'Other', it is defined by the event source." .

ocsf:auth_protocol_id a owl:DatatypeProperty ;
    rdfs:label "Auth Protocol ID" ;
    rdfs:range ocsf:integer_t ;
    dcterms:description "The normalized identifier of the authentication protocol used to create the user session." ;
    jsonschema:enum "CHAP",
        "Digest",
        "EAP",
        "Kerberos",
        "NTLM",
        "OAUTH 2.0",
        "OpenID",
        "Other",
        "PAP",
        "RADIUS",
        "SAML",
        "Unknown" .

ocsf:auth_type a owl:DatatypeProperty ;
    rdfs:label "Authentication Type" ;
    rdfs:range ocsf:string_t ;
    dcterms:description "The agreed upon authentication type, normalized to the caption of 'auth_type_id'. In the case of 'Other', it is defined by the event source." .

ocsf:auth_type_id a owl:DatatypeProperty ;
    rdfs:label "Authentication Type ID" ;
    rdfs:range ocsf:integer_t ;
    dcterms:description "The normalized identifier of the agreed upon authentication type. See specific usage." ;
    jsonschema:enum "Other",
        "Unknown" .

ocsf:autoscale_uid a owl:DatatypeProperty ;
    rdfs:label "Autoscale UID" ;
    rdfs:range ocsf:string_t ;
    dcterms:description "The unique identifier of the cloud autoscale configuration." .

ocsf:banner a owl:DatatypeProperty ;
    rdfs:label "SMTP Banner" ;
    rdfs:range ocsf:string_t ;
    dcterms:description "The initial SMTP connection response that a messaging server receives after it connects to a email server." .

ocsf:base_address a owl:DatatypeProperty ;
    rdfs:label "Base Address" ;
    rdfs:range ocsf:string_t ;
    dcterms:description "The memory address where the module was loaded." .

ocsf:base_score a owl:DatatypeProperty ;
    rdfs:label "Base Score" ;
    rdfs:range ocsf:float_t ;
    dcterms:description "The base score as reported by the event source. See specific usage." .

ocsf:bios_date a owl:DatatypeProperty ;
    rdfs:label "BIOS Date" ;
    rdfs:range ocsf:string_t ;
    dcterms:description "The BIOS date. For example: <code>03/31/16</code>." .

ocsf:bios_manufacturer a owl:DatatypeProperty ;
    rdfs:label "BIOS Manufacturer" ;
    rdfs:range ocsf:string_t ;
    dcterms:description "The BIOS manufacturer. For example: <code>LENOVO</code>." .

ocsf:bios_ver a owl:DatatypeProperty ;
    rdfs:label "BIOS Version" ;
    rdfs:range ocsf:string_t ;
    dcterms:description "The BIOS version. For example: <code>LENOVO G5ETA2WW (2.62)</code>." .

ocsf:boot_time a owl:DatatypeProperty ;
    rdfs:label "Boot Time" ;
    rdfs:range ocsf:timestamp_t ;
    dcterms:description "The time when the system was booted." .

ocsf:boundary a owl:DatatypeProperty ;
    rdfs:label "Boundary" ;
    rdfs:range ocsf:string_t ;
    dcterms:description "The boundary of the connection, normalized to the caption of 'boundary_id'. In the case of 'Other', it is defined by the event source. <p> For cloud connections, this translates to the traffic-boundary(same VPC, through IGW, etc.). For traditional networks, this is described as Local, Internal, or External.</p>" .

ocsf:boundary_id a owl:DatatypeProperty ;
    rdfs:label "Boundary ID" ;
    rdfs:range ocsf:integer_t ;
    dcterms:description "<p>The normalized identifier of the boundary of the connection. </p><p> For cloud connections, this translates to the traffic-boundary (same VPC, through IGW, etc.). For traditional networks, this is described as Local, Internal, or External.</p>" ;
    jsonschema:enum "External",
        "Gateway VPC",
        "Inter-region VPC",
        "Internal",
        "Internet Gateway",
        "Internet/VPC Gateway",
        "Intra-region VPC",
        "Local Gateway",
        "Localhost",
        "Other",
        "Same VPC",
        "Unknown",
        "Virtual Private Gateway" .

ocsf:build a owl:DatatypeProperty ;
    rdfs:label "OS Build" ;
    rdfs:range ocsf:string_t ;
    dcterms:description "The operating system build number." .

ocsf:bulletin a owl:DatatypeProperty ;
    rdfs:label "Patch Bulletin" ;
    rdfs:range ocsf:string_t ;
    dcterms:description "The vendor bulletin identifier." .

ocsf:bytes a owl:DatatypeProperty ;
    rdfs:label "Total Bytes" ;
    rdfs:range ocsf:long_t ;
    dcterms:description "The total number of bytes (in and out)." .

ocsf:bytes_in a owl:DatatypeProperty ;
    rdfs:label "Bytes In" ;
    rdfs:range ocsf:long_t ;
    dcterms:description "The number of bytes sent from the destination to the source." .

ocsf:bytes_out a owl:DatatypeProperty ;
    rdfs:label "Bytes Out" ;
    rdfs:range ocsf:long_t ;
    dcterms:description "The number of bytes sent from the source to the destination." .

ocsf:capabilities a owl:DatatypeProperty ;
    rdfs:label "Capabilities" ;
    rdfs:range ocsf:string_t ;
    dcterms:description "A list of RDP capabilities." .

ocsf:caption a owl:DatatypeProperty ;
    rdfs:label "Caption" ;
    rdfs:range ocsf:string_t ;
    dcterms:description "A short description or caption of the device. For example: <code>Scanner 1</code> or <code>Database Manager</code>." .

ocsf:categories a owl:DatatypeProperty ;
    rdfs:label "Website Categorization" ;
    rdfs:range ocsf:string_t ;
    dcterms:description "The Website categorization names, as defined by <code>category_ids</code> enum values." .

ocsf:category a owl:DatatypeProperty ;
    rdfs:label "Category" ;
    rdfs:range ocsf:string_t ;
    dcterms:description "The object category, normalized to the caption of <code>category_id</code>. See specific usage." .

ocsf:category_id a owl:DatatypeProperty ;
    rdfs:label "Category ID" ;
    rdfs:range ocsf:integer_t ;
    dcterms:description "The normalized identifier of the object category. See specific usage." .

ocsf:category_ids a owl:DatatypeProperty ;
    rdfs:label "Website Categorization IDs" ;
    rdfs:range ocsf:integer_t ;
    dcterms:description "The Website categorization identifiers." ;
    jsonschema:enum "Abortion",
        "Adult/Mature Content",
        "Alcohol",
        "Alternative Spirituality/Belief",
        "Art/Culture",
        "Auctions",
        "Audio/Video Clips",
        "Brokerage/Trading",
        "Business/Economy",
        "Charitable Organizations",
        "Chat (IM)/SMS",
        "Child Pornography",
        "Computer/Information Security",
        "Content Servers",
        "Controlled Substances",
        "Dynamic DNS Host",
        "E-Card/Invitations",
        "Education",
        "Email",
        "Entertainment",
        "Extreme",
        "File Storage/Sharing",
        "Financial Services",
        "For Kids",
        "Gambling",
        "Games",
        "Government/Legal",
        "Hacking",
        "Health",
        "Humor/Jokes",
        "Informational",
        "Internet Connected Devices",
        "Internet Telephony",
        "Intimate Apparel/Swimsuit",
        "Job Search/Careers",
        "Malicious Outbound Data/Botnets",
        "Malicious Sources/Malnets",
        "Marijuana",
        "Media Sharing",
        "Military",
        "Mixed Content/Potentially Adult",
        "News/Media",
        "Newsgroups/Forums",
        "Non-Viewable/Infrastructure",
        "Nudity",
        "Office/Business Applications",
        "Online Meetings",
        "Other",
        "Peer-to-Peer (P2P)",
        "Personal Sites",
        "Personals/Dating",
        "Phishing",
        "Piracy/Copyright Concerns",
        "Placeholders",
        "Political/Social Advocacy",
        "Pornography",
        "Potentially Unwanted Software",
        "Proxy Avoidance",
        "Radio/Audio Streams",
        "Real Estate",
        "Reference",
        "Religion",
        "Remote Access Tools",
        "Restaurants/Dining/Food",
        "Scam/Questionable/Illegal",
        "Search Engines/Portals",
        "Sex Education",
        "Sexual Expression",
        "Shopping",
        "Social Networking",
        "Society/Daily Living",
        "Software Downloads",
        "Spam",
        "Sports/Recreation",
        "Suspicious",
        "Technology/Internet",
        "Tobacco",
        "Translation",
        "Travel",
        "TV/Video Streams",
        "Uncategorized",
        "Unknown",
        "Vehicles",
        "Violence/Hate/Racism",
        "Weapons",
        "Web Ads/Analytics",
        "Web Hosting" .

ocsf:category_name a owl:DatatypeProperty ;
    rdfs:label "Category" ;
    rdfs:range ocsf:string_t ;
    dcterms:description "The event category name, as defined by category_uid value." .

ocsf:category_uid a owl:DatatypeProperty ;
    rdfs:label "Category ID" ;
    rdfs:range ocsf:integer_t ;
    dcterms:description "The category unique identifier of the event." .

ocsf:cc a owl:DatatypeProperty ;
    rdfs:label "Cc" ;
    rdfs:range ocsf:email_t ;
    dcterms:description "The email header Cc values, as defined by RFC 5322." .

ocsf:certificate_chain a owl:DatatypeProperty ;
    rdfs:label "Certificate Chain" ;
    rdfs:range ocsf:string_t ;
    dcterms:description "The Chain of Certificate Serial Numbers field provides a chain of Certificate Issuer Serial Numbers leading to the Root Certificate Issuer." .

ocsf:chassis a owl:DatatypeProperty ;
    rdfs:label "Chassis" ;
    rdfs:range ocsf:string_t ;
    dcterms:description "The chassis type describes the system enclosure or physical form factor. Such as the following examples for Windows <a target='_blank' href='https://docs.microsoft.com/en-us/windows/win32/cimwin32prov/win32-systemenclosure'>Windows Chassis Types</a>" .

ocsf:chunks a owl:DatatypeProperty ;
    rdfs:label "Chunks" ;
    rdfs:range ocsf:long_t ;
    dcterms:description "A unit of information within an SCTP packet, consisting of a chunk header and chunk-specific content. See RFC 4960. This field can be used for the total number of chunks (in and out)." .

ocsf:chunks_in a owl:DatatypeProperty ;
    rdfs:label "Chunks In" ;
    rdfs:range ocsf:long_t ;
    dcterms:description "A unit of information within an SCTP packet, consisting of a chunk header and chunk-specific content. See RFC 4960. This field can be used for the chunks sent from the destination to the source." .

ocsf:chunks_out a owl:DatatypeProperty ;
    rdfs:label "Chunks Out" ;
    rdfs:range ocsf:long_t ;
    dcterms:description "A unit of information within an SCTP packet, consisting of a chunk header and chunk-specific content. See RFC 4960. This field can be used for the chunks sent from the source to the destination." .

ocsf:cipher a owl:DatatypeProperty ;
    rdfs:label "Cipher Suite" ;
    rdfs:range ocsf:string_t ;
    dcterms:description "The negotiated cipher suite." .

ocsf:city a owl:DatatypeProperty ;
    rdfs:label "City" ;
    rdfs:range ocsf:string_t ;
    dcterms:description "The name of the city." .

ocsf:class a owl:DatatypeProperty ;
    rdfs:label "Class" ;
    rdfs:range ocsf:string_t ;
    dcterms:description "The class name of the object. See specific usage." .

ocsf:class_name a owl:DatatypeProperty ;
    rdfs:label "Class" ;
    rdfs:range ocsf:string_t ;
    dcterms:description "The event class name, as defined by class_uid value." .

ocsf:class_uid a owl:DatatypeProperty ;
    rdfs:label "Class ID" ;
    rdfs:range ocsf:integer_t ;
    dcterms:description "The unique identifier of a class. A class describes the attributes available in an event." .

ocsf:classification a owl:DatatypeProperty ;
    rdfs:label "Classification" ;
    rdfs:range ocsf:string_t ;
    dcterms:description "The classification as defined by the vendor." .

ocsf:classification_ids a owl:DatatypeProperty ;
    rdfs:label "Classification IDs" ;
    rdfs:range ocsf:integer_t ;
    dcterms:description "The list of normalized classification identifiers. See specific usage." ;
    jsonschema:enum "Other",
        "Unknown" .

ocsf:classifications a owl:DatatypeProperty ;
    rdfs:label "Classifications" ;
    rdfs:range ocsf:string_t ;
    dcterms:description "The list of malware classifications, normalized to the captions of the classification_id values. In the case of 'Other', they are defined by the event source." .

ocsf:client_ciphers a owl:DatatypeProperty ;
    rdfs:label "Client Cipher Suites" ;
    rdfs:range ocsf:string_t ;
    dcterms:description "The client cipher suites that were exchanged during the TLS handshake negotiation." .

ocsf:client_dialects a owl:DatatypeProperty ;
    rdfs:label "Client Dialects" ;
    rdfs:range ocsf:string_t ;
    dcterms:description "The list of SMB dialects that the client speaks." .

ocsf:cloud_partition a owl:DatatypeProperty ;
    rdfs:label "Cloud Partition" ;
    rdfs:range ocsf:string_t ;
    dcterms:description "The canonical cloud partition name to which the region is assigned (e.g. AWS Partitions: aws, aws-cn, aws-us-gov)." .

ocsf:cmd_line a owl:DatatypeProperty ;
    rdfs:label "Command Line" ;
    rdfs:range ocsf:string_t ;
    dcterms:description "The full command line used to launch an application, service, process, or job. For example: <code>ssh user@10.0.0.10</code>. If the command line is unavailable or missing, the empty string <code>''</code> is to be used." .

ocsf:code a owl:DatatypeProperty ;
    rdfs:label "Response Code" ;
    rdfs:range ocsf:integer_t ;
    dcterms:description "The numeric response sent to a request." .

ocsf:codes a owl:DatatypeProperty ;
    rdfs:label "Response Codes" ;
    rdfs:range ocsf:integer_t ;
    dcterms:description "The list of numeric responses sent to a request." .

ocsf:color_depth a owl:DatatypeProperty ;
    rdfs:label "Color Depth" ;
    rdfs:range ocsf:integer_t ;
    dcterms:description "The numeric color depth." .

ocsf:command a owl:DatatypeProperty ;
    rdfs:label "Command" ;
    rdfs:range ocsf:string_t ;
    dcterms:description "The command name." .

ocsf:command_response a owl:DatatypeProperty ;
    rdfs:label "Command Response" ;
    rdfs:range ocsf:string_t ;
    dcterms:description "The response to the command." .

ocsf:command_responses a owl:DatatypeProperty ;
    rdfs:label "Command Responses" ;
    rdfs:range ocsf:string_t ;
    dcterms:description "The responses to the command." .

ocsf:command_uid a owl:DatatypeProperty ;
    rdfs:label "Command UID" ;
    rdfs:range ocsf:string_t ;
    dcterms:description "The unique command identifier." .

ocsf:comment a owl:DatatypeProperty ;
    rdfs:label "Comment" ;
    rdfs:range ocsf:string_t ;
    dcterms:description "The user-provided comment." .

ocsf:company_name a owl:DatatypeProperty ;
    rdfs:label "Company Name" ;
    rdfs:range ocsf:string_t ;
    dcterms:description "The name of the company that published the file. For example: <code>Microsoft Corporation</code>." .

ocsf:component a owl:DatatypeProperty ;
    rdfs:label "Component" ;
    rdfs:range ocsf:string_t ;
    dcterms:description "The component of a data object. See specific usage." .

ocsf:condition a owl:DatatypeProperty ;
    rdfs:label "Condition" ;
    rdfs:range ocsf:string_t ;
    dcterms:description "The rule trigger condition for the rule. For example: SQL_INJECTION." .

ocsf:confidence a owl:DatatypeProperty ;
    rdfs:label "Confidence" ;
    rdfs:range ocsf:string_t ;
    dcterms:description "The confidence, normalized to the caption of the confidence_id value. In the case of 'Other', it is defined by the event source." .

ocsf:confidence_id a owl:DatatypeProperty ;
    rdfs:label "Confidence Id" ;
    rdfs:range ocsf:integer_t ;
    dcterms:description "The normalized confidence refers to the accuracy of the rule that created the finding. A rule with a low confidence means that the finding scope is wide and may create finding reports that may not be malicious in nature." ;
    jsonschema:enum "High",
        "Low",
        "Medium",
        "Other",
        "Unknown" .

ocsf:confidence_score a owl:DatatypeProperty ;
    rdfs:label "Confidence Score" ;
    rdfs:range ocsf:integer_t ;
    dcterms:description "The confidence score as reported by the event source." .

ocsf:confidentiality a owl:DatatypeProperty ;
    rdfs:label "Confidentiality" ;
    rdfs:range ocsf:string_t ;
    dcterms:description "The file content confidentiality, normalized to the confidentiality_id value. In the case of 'Other', it is defined by the event source." .

ocsf:confidentiality_id a owl:DatatypeProperty ;
    rdfs:label "Confidentiality ID" ;
    rdfs:range ocsf:integer_t ;
    dcterms:description "The normalized identifier of the file content confidentiality indicator." ;
    jsonschema:enum "Confidential",
        "Not Confidential",
        "Other",
        "Private",
        "Restricted",
        "Secret",
        "Top Secret",
        "Unknown" .

ocsf:connection_uid a owl:DatatypeProperty ;
    rdfs:label "Connection Identifier" ;
    rdfs:range ocsf:string_t ;
    dcterms:description "The network connection identifier." .

ocsf:content_type a owl:DatatypeProperty ;
    rdfs:label "HTTP Content Type" ;
    rdfs:range ocsf:string_t ;
    dcterms:description "The request header that identifies the original <a target='_blank' href='https://www.iana.org/assignments/media-types/media-types.xhtml'>media type </a> of the resource (prior to any content encoding applied for sending)." .

ocsf:continent a owl:DatatypeProperty ;
    rdfs:label "Continent" ;
    rdfs:range ocsf:string_t ;
    dcterms:description "The name of the continent." .

ocsf:control a owl:DatatypeProperty ;
    rdfs:label "Security Control" ;
    rdfs:range ocsf:string_t ;
    dcterms:description "A Control is prescriptive, prioritized, and simplified set of best practices that one can use to strengthen their cybersecurity posture. e.g. AWS SecurityHub Controls, CIS Controls." .

ocsf:coordinates a owl:DatatypeProperty ;
    rdfs:label "Coordinates" ;
    rdfs:range ocsf:float_t ;
    dcterms:description "A two-element array, containing a longitude/latitude pair. The format conforms with <a target='_blank' href='https://geojson.org'>GeoJSON</a>. For example: <code>[-73.983, 40.719]</code>." .

ocsf:correlation_uid a owl:DatatypeProperty ;
    rdfs:label "Correlation UID" ;
    rdfs:range ocsf:string_t ;
    dcterms:description "The unique identifier used to correlate events." .

ocsf:cost_center a owl:DatatypeProperty ;
    rdfs:label "Cost Center" ;
    rdfs:range ocsf:string_t ;
    dcterms:description "The cost center associated with the user." .

ocsf:count a owl:DatatypeProperty ;
    rdfs:label "Count" ;
    rdfs:range ocsf:integer_t ;
    dcterms:description "The number of times that events in the same logical group occurred during the event <strong>Start Time</strong> to <strong>End Time</strong> period." .

ocsf:country a owl:DatatypeProperty ;
    rdfs:label "Country" ;
    rdfs:range ocsf:string_t ;
    dcterms:description "The ISO 3166-1 Alpha-2 country code. For the complete list of country codes see <a target='_blank' href='https://www.iso.org/obp/ui/#iso:pub:PUB500001:en' >ISO 3166-1 alpha-2 codes</a>.<p><b>Note:</b> The two letter country code should be capitalized. For example: <code>US</code> or <code>CA</code>.</p>" .

ocsf:cpe_name a owl:DatatypeProperty ;
    rdfs:label "The product CPE identifier" ;
    rdfs:range ocsf:string_t ;
    dcterms:description "The Common Platform Enumeration (CPE) name as described by (<a target='_blank' href='https://nvd.nist.gov/products/cpe'>NIST</a>) For example: <code>cpe:/a:apple:safari:16.2</code>." .

ocsf:cpu_bits a owl:DatatypeProperty ;
    rdfs:label "CPU Bits" ;
    rdfs:range ocsf:integer_t ;
    dcterms:description "The cpu architecture, the number of bits used for addressing in memory. For example: <code>32</code> or <code>64</code>." .

ocsf:cpu_cores a owl:DatatypeProperty ;
    rdfs:label "CPU Cores" ;
    rdfs:range ocsf:integer_t ;
    dcterms:description "The number of processor cores in all installed processors. For Example: <code>42</code>." .

ocsf:cpu_count a owl:DatatypeProperty ;
    rdfs:label "CPU Count" ;
    rdfs:range ocsf:integer_t ;
    dcterms:description "The number of physical processors on a system. For example: <code>1</code>." .

ocsf:cpu_speed a owl:DatatypeProperty ;
    rdfs:label "Processor Speed" ;
    rdfs:range ocsf:integer_t ;
    dcterms:description "The speed of the processor in Mhz. For Example: <code>4200</code>." .

ocsf:cpu_type a owl:DatatypeProperty ;
    rdfs:label "Processor Type" ;
    rdfs:range ocsf:string_t ;
    dcterms:description "The processor type. For example: <code>x86 Family 6 Model 37 Stepping 5</code>." .

ocsf:create_mask a owl:DatatypeProperty ;
    rdfs:label "Create Mask" ;
    rdfs:range ocsf:string_t ;
    dcterms:description "The original Windows mask that is required to create the object." .

ocsf:created_time a owl:DatatypeProperty ;
    rdfs:label "Created Time" ;
    rdfs:range ocsf:timestamp_t ;
    dcterms:description "The time when the object was created. See specific usage." .

ocsf:credential_uid a owl:DatatypeProperty ;
    rdfs:label "User Credential ID" ;
    rdfs:range ocsf:string_t ;
    dcterms:description "The unique identifier of the user's credential. For example, AWS Access Key ID." .

ocsf:criticality a owl:DatatypeProperty ;
    rdfs:label "Criticality" ;
    rdfs:range ocsf:string_t ;
    dcterms:description "Criticality of a resource/object in question" .

ocsf:customer_uid a owl:DatatypeProperty ;
    rdfs:label "Customer UID" ;
    rdfs:range ocsf:string_t ;
    dcterms:description "The unique customer identifier." .

ocsf:cwe_uid a owl:DatatypeProperty ;
    rdfs:label "CWE UID" ;
    rdfs:range ocsf:string_t ;
    dcterms:description "The <a target='_blank' href='https://cwe.mitre.org/'>Common Weakness Enumeration (CWE)</a> unique identifier. For example: <code>CWE-787</code>." .

ocsf:cwe_url a owl:DatatypeProperty ;
    rdfs:label "CWE URL" ;
    rdfs:range ocsf:url_t ;
    dcterms:description "Common Weakness Enumeration (CWE) definition URL. For example: <code>https://cwe.mitre.org/data/definitions/787.html</code>." .

ocsf:data a owl:DatatypeProperty ;
    rdfs:label "Data" ;
    rdfs:range ocsf:json_t ;
    dcterms:description "The additional data that is associated with the event or object. See specific usage." .

ocsf:data_lifecycle_state a owl:DatatypeProperty ;
    rdfs:label "Data Lifecycle State" ;
    rdfs:range ocsf:string_t ;
    dcterms:description "The name of the stage or state that the data was in. E.g., Data-at-Rest, Data-in-Transit, etc." .

ocsf:data_lifecycle_state_id a owl:DatatypeProperty ;
    rdfs:label "Data Lifecycle State ID" ;
    rdfs:range ocsf:integer_t ;
    dcterms:description "The stage or state that the data was in when it was assessed or scanned by a data security tool." ;
    jsonschema:enum "Data at-Rest",
        "Data in-Transit",
        "Data in-Use",
        "Other",
        "Unknown" .

ocsf:data_sources a owl:DatatypeProperty ;
    rdfs:label "Data Sources" ;
    rdfs:range ocsf:string_t ;
    dcterms:description "A list of data sources utilized in generation of the finding." .

ocsf:decision a owl:DatatypeProperty ;
    rdfs:label "Authorization Decision/Outcome" ;
    rdfs:range ocsf:string_t ;
    dcterms:description "Decision/outcome of the authorization mechanism (e.g. Approved, Denied)" .

ocsf:delay a owl:DatatypeProperty ;
    rdfs:label "Root Delay" ;
    rdfs:range ocsf:integer_t ;
    dcterms:description "The total round-trip delay to the reference clock in milliseconds." .

ocsf:deleted_time a owl:DatatypeProperty ;
    rdfs:label "Deleted Time" ;
    rdfs:range ocsf:timestamp_t ;
    dcterms:description "The timestamp when the user was deleted. In Active Directory (AD), when a user is deleted they are moved to a temporary container and then removed after 30 days. So, this field can be populated even after a user is deleted for the next 30 days." .

ocsf:delivered_to a owl:DatatypeProperty ;
    rdfs:label "Delivered To" ;
    rdfs:range ocsf:email_t ;
    dcterms:description "The <strong>Delivered-To</strong> email header field." .

ocsf:depth a owl:DatatypeProperty ;
    rdfs:label "CVSS Depth" ;
    rdfs:range ocsf:string_t ;
    dcterms:description "The CVSS depth represents a depth of the equation used to calculate CVSS score." ;
    jsonschema:enum "Base",
        "Environmental",
        "Temporal" .

ocsf:desc a owl:DatatypeProperty ;
    rdfs:label "Description" ;
    rdfs:range ocsf:string_t ;
    dcterms:description "The description that pertains to the object or event. See specific usage." .

ocsf:details a owl:DatatypeProperty ;
    rdfs:label "Details" ;
    rdfs:range ocsf:string_t ;
    dcterms:description "Details of an entity. See specific usage" .

ocsf:detection_pattern a owl:DatatypeProperty ;
    rdfs:label "Detection Pattern" ;
    rdfs:range ocsf:string_t ;
    dcterms:description "Specific pattern, algorithm, fingerpint, or model used for detection." .

ocsf:detection_system a owl:DatatypeProperty ;
    rdfs:label "Detection System" ;
    rdfs:range ocsf:string_t ;
    dcterms:description "The name of the type of data security tool or system that the finding, detection, or alert originated from. E.g., Endpoint, Secure Email Gateway, etc." .

ocsf:detection_system_id a owl:DatatypeProperty ;
    rdfs:label "Detection System ID" ;
    rdfs:range ocsf:integer_t ;
    dcterms:description "The type of data security tool or system that the finding, detection, or alert originated from." ;
    jsonschema:enum "Application-Level DLP",
        "Cloud Access Security Broker",
        "Data Discovery & Classification",
        "Data Security Posture Management",
        "Database Activity Monitoring",
        "Developer Security",
        "Digital Rights Management",
        "DLP Gateway",
        "Endpoint",
        "Mobile Device Management",
        "Other",
        "Secure Email Gateway",
        "Secure Web Gateway",
        "Unknown" .

ocsf:detection_uid a owl:DatatypeProperty ;
    rdfs:label "Detection UID" ;
    rdfs:range ocsf:string_t ;
    dcterms:description "The associated unique detection event identifier. For example: detection response events include the <b>Detection ID</b> of the original event." .

ocsf:developer_uid a owl:DatatypeProperty ;
    rdfs:label "Developer UID" ;
    rdfs:range ocsf:string_t ;
    dcterms:description "The developer ID on the certificate that signed the file." .

ocsf:dialect a owl:DatatypeProperty ;
    rdfs:label "Dialect" ;
    rdfs:range ocsf:string_t ;
    dcterms:description "The negotiated protocol dialect." .

ocsf:direction a owl:DatatypeProperty ;
    rdfs:label "Direction" ;
    rdfs:range ocsf:string_t ;
    dcterms:description "The direction of the initiated connection, traffic, or email, normalized to the caption of the direction_id value. In the case of 'Other', it is defined by the event source." .

ocsf:direction_id a owl:DatatypeProperty ;
    rdfs:label "Direction ID" ;
    rdfs:range ocsf:integer_t ;
    dcterms:description "The normalized identifier of the direction of the initiated connection, traffic, or email." ;
    jsonschema:enum "Inbound",
        "Lateral",
        "Other",
        "Outbound",
        "Unknown" .

ocsf:dispersion a owl:DatatypeProperty ;
    rdfs:label "Root Dispersion" ;
    rdfs:range ocsf:integer_t ;
    dcterms:description "The dispersion in the NTP protocol is the estimated time error or uncertainty relative to the reference clock in milliseconds." .

ocsf:disposition a owl:DatatypeProperty ;
    rdfs:label "Disposition" ;
    rdfs:range ocsf:string_t ;
    dcterms:description "The disposition name, normalized to the caption of the disposition_id value. In the case of 'Other', it is defined by the event source." .

ocsf:disposition_id a owl:DatatypeProperty ;
    rdfs:label "Disposition ID" ;
    rdfs:range ocsf:integer_t ;
    dcterms:description "Describes the outcome or action taken by a security control, such as access control checks, malware detections or various types of policy violations." ;
    jsonschema:enum "Access Revoked",
        "Alert",
        "Allowed",
        "Approved",
        "Blocked",
        "Captcha",
        "Challenge",
        "Corrected",
        "Count",
        "Custom Action",
        "Delayed",
        "Deleted",
        "Detected",
        "Dropped",
        "Error",
        "Exonerated",
        "Isolated",
        "Logged",
        "No Action",
        "Other",
        "Partially Corrected",
        "Quarantined",
        "Rejected",
        "Reset",
        "Restored",
        "Tagged",
        "Unauthorized",
        "Uncorrected",
        "Unknown" .

ocsf:dkim a owl:DatatypeProperty ;
    rdfs:label "DKIM Status" ;
    rdfs:range ocsf:string_t ;
    dcterms:description "The DomainKeys Identified Mail (DKIM) status of the email." .

ocsf:dkim_domain a owl:DatatypeProperty ;
    rdfs:label "DKIM Domain" ;
    rdfs:range ocsf:string_t ;
    dcterms:description "The DomainKeys Identified Mail (DKIM) signing domain of the email." .

ocsf:dkim_signature a owl:DatatypeProperty ;
    rdfs:label "DKIM Signature" ;
    rdfs:range ocsf:string_t ;
    dcterms:description "The DomainKeys Identified Mail (DKIM) signature used by the sending/receiving system." .

ocsf:dmarc a owl:DatatypeProperty ;
    rdfs:label "DMARC Status" ;
    rdfs:range ocsf:string_t ;
    dcterms:description "The Domain-based Message Authentication, Reporting and Conformance (DMARC) status of the email." .

ocsf:dmarc_override a owl:DatatypeProperty ;
    rdfs:label "DMARC Override" ;
    rdfs:range ocsf:string_t ;
    dcterms:description "The Domain-based Message Authentication, Reporting and Conformance (DMARC) override action." .

ocsf:dmarc_policy a owl:DatatypeProperty ;
    rdfs:label "DMARC Policy" ;
    rdfs:range ocsf:string_t ;
    dcterms:description "The Domain-based Message Authentication, Reporting and Conformance (DMARC) policy status." .

ocsf:dnssec_status a owl:DatatypeProperty ;
    rdfs:label "DNSSEC Status" ;
    rdfs:range ocsf:string_t ;
    dcterms:description "The normalized value of dnssec_status_id." .

ocsf:dnssec_status_id a owl:DatatypeProperty ;
    rdfs:label "DNSSEC Status ID" ;
    rdfs:range ocsf:integer_t ;
    dcterms:description "Describes the normalized status of DNS Security Extensions (DNSSEC) for a domain." ;
    jsonschema:enum "Other",
        "Signed",
        "Unknown",
        "Unsigned" .

ocsf:domain a owl:DatatypeProperty ;
    rdfs:label "Domain" ;
    rdfs:range ocsf:string_t ;
    dcterms:description "The name of the domain." .

ocsf:duration a owl:DatatypeProperty ;
    rdfs:label "Duration Milliseconds" ;
    rdfs:range ocsf:long_t ;
    dcterms:description "This represents the duration of the activity in milliseconds. See specific usage." .

ocsf:duration_days a owl:DatatypeProperty ;
    rdfs:label "Duration Days" ;
    rdfs:range ocsf:integer_t ;
    dcterms:description "Represents the duration of the activity in days. See specific usage." .

ocsf:duration_hours a owl:DatatypeProperty ;
    rdfs:label "Duration Hours" ;
    rdfs:range ocsf:integer_t ;
    dcterms:description "Represents the duration of the activity in hours. See specific usage." .

ocsf:duration_mins a owl:DatatypeProperty ;
    rdfs:label "Duration Minutes" ;
    rdfs:range ocsf:integer_t ;
    dcterms:description "Represents the duration of the activity in minutes. See specific usage." .

ocsf:duration_months a owl:DatatypeProperty ;
    rdfs:label "Duration Months" ;
    rdfs:range ocsf:integer_t ;
    dcterms:description "Represents the duration of the activity in months. See specific usage." .

ocsf:duration_secs a owl:DatatypeProperty ;
    rdfs:label "Duration Seconds" ;
    rdfs:range ocsf:integer_t ;
    dcterms:description "Represents the duration of the activity in seconds. See specific usage." .

ocsf:duration_weeks a owl:DatatypeProperty ;
    rdfs:label "Duration Weeks" ;
    rdfs:range ocsf:integer_t ;
    dcterms:description "Represents the duration of the activity in weeks. See specific usage." .

ocsf:duration_years a owl:DatatypeProperty ;
    rdfs:label "Duration Years" ;
    rdfs:range ocsf:integer_t ;
    dcterms:description "Represents the duration of the activity in years. See specific usage." .

ocsf:edition a owl:DatatypeProperty ;
    rdfs:label "OS Edition" ;
    rdfs:range ocsf:string_t ;
    dcterms:description "The operating system edition. For example: <code>Professional</code>." .

ocsf:email_addr a owl:DatatypeProperty ;
    rdfs:label "Email Address" ;
    rdfs:range ocsf:email_t ;
    dcterms:description "The user's primary email address." .

ocsf:email_addrs a owl:DatatypeProperty ;
    rdfs:label "Email Addresses" ;
    rdfs:range ocsf:email_t ;
    dcterms:description "A list of additional email addresses for the user." .

ocsf:email_uid a owl:DatatypeProperty ;
    rdfs:label "Email UID" ;
    rdfs:range ocsf:string_t ;
    dcterms:description "The unique identifier of the email, used to correlate related email alert and activity events." .

ocsf:employee_uid a owl:DatatypeProperty ;
    rdfs:label "Employee ID" ;
    rdfs:range ocsf:string_t ;
    dcterms:description "The employee identifier assigned to the user by the organization." .

ocsf:end_line a owl:DatatypeProperty ;
    rdfs:label "End Line" ;
    rdfs:range ocsf:integer_t ;
    dcterms:description "The line number of the last line of code block identified as vulnerable." .

ocsf:end_time a owl:DatatypeProperty ;
    rdfs:label "End Time" ;
    rdfs:range ocsf:timestamp_t ;
    dcterms:description "The end time of a time period. See specific usage." .

ocsf:epoch a owl:DatatypeProperty ;
    rdfs:label "Epoch" ;
    rdfs:range ocsf:integer_t ;
    dcterms:description "The software package epoch. Epoch is a way to define weighted dependencies based on version numbers." .

ocsf:error a owl:DatatypeProperty ;
    rdfs:label "Error Code" ;
    rdfs:range ocsf:string_t ;
    dcterms:description "Error Code" .

ocsf:error_message a owl:DatatypeProperty ;
    rdfs:label "Error Message" ;
    rdfs:range ocsf:string_t ;
    dcterms:description "Error Message" .

ocsf:event_code a owl:DatatypeProperty ;
    rdfs:label "Event Code" ;
    rdfs:range ocsf:string_t ;
    dcterms:description "The Event ID or Code that the product uses to describe the event." .

ocsf:evidence a owl:DatatypeProperty ;
    rdfs:label "Evidence" ;
    rdfs:range ocsf:json_t ;
    dcterms:description "The data the finding exposes to the analyst." .

ocsf:exit_code a owl:DatatypeProperty ;
    rdfs:label "Exit Code" ;
    rdfs:range ocsf:integer_t ;
    dcterms:description "The exit code reported by a process when it terminates. The convention is that zero indicates success and any non-zero exit code indicates that some error occurred." .

ocsf:expiration_reason a owl:DatatypeProperty ;
    rdfs:label "Expiration Reason" ;
    rdfs:range ocsf:string_t ;
    dcterms:description "The expiration reason. See specific usage." .

ocsf:expiration_time a owl:DatatypeProperty ;
    rdfs:label "Expiration Time" ;
    rdfs:range ocsf:timestamp_t ;
    dcterms:description "The expiration time. See specific usage." .

ocsf:ext a owl:DatatypeProperty ;
    rdfs:label "Extension" ;
    rdfs:range ocsf:string_t ;
    dcterms:description "The extension. See specific usage." .

ocsf:factor_type a owl:DatatypeProperty ;
    rdfs:label "Factor Type" ;
    rdfs:range ocsf:string_t ;
    dcterms:description "The type of authentication factor used in an authentication attempt." .

ocsf:factor_type_id a owl:DatatypeProperty ;
    rdfs:label "Factor Type ID" ;
    rdfs:range ocsf:integer_t ;
    dcterms:description "The normalized identifier for the authentication factor." ;
    jsonschema:enum "Biometric",
        "Email",
        "Hardware Token",
        "Other",
        "OTP",
        "Password",
        "Phone Call",
        "Push Notification",
        "Security Question",
        "SMS",
        "U2F",
        "Unknown",
        "WebAuthn" .

ocsf:file_diff a owl:DatatypeProperty ;
    rdfs:label "File Diff" ;
    rdfs:range ocsf:string_t ;
    dcterms:description "File content differences used for change detection. For example, a common use case is to identify itemized changes within INI or configuration/property setting values." .

ocsf:first_seen_time a owl:DatatypeProperty ;
    rdfs:label "First Seen" ;
    rdfs:range ocsf:timestamp_t ;
    dcterms:description "The initial detection time of the activity or object. See specific usage" .

ocsf:fix_available a owl:DatatypeProperty ;
    rdfs:label "Fix Availability" ;
    rdfs:range ocsf:boolean_t ;
    dcterms:description "Indicates if a fix is available for the reported vulnerability." .

ocsf:fixed_in_version a owl:DatatypeProperty ;
    rdfs:label "Fixed In Version" ;
    rdfs:range ocsf:string_t ;
    dcterms:description "The software package version in which a reported vulnerability was patched/fixed." .

ocsf:flag_ids a owl:DatatypeProperty ;
    rdfs:label "Communication Flag IDs" ;
    rdfs:range ocsf:integer_t ;
    dcterms:description "The list of normalized identifiers of the communication flag IDs. See specific usage." ;
    jsonschema:enum "Other",
        "Unknown" .

ocsf:flags a owl:DatatypeProperty ;
    rdfs:label "Flags" ;
    rdfs:range ocsf:string_t ;
    dcterms:description "The list of communication flags, normalized to the captions of the flag_ids values. In the case of 'Other', they are defined by the event source." .

ocsf:from a owl:DatatypeProperty ;
    rdfs:label "From" ;
    rdfs:range ocsf:email_t ;
    dcterms:description "The email header From values, as defined by RFC 5322." .

ocsf:full_name a owl:DatatypeProperty ;
    rdfs:label "Full Name" ;
    rdfs:range ocsf:string_t ;
    dcterms:description "The full name of the person, as per the LDAP Common Name attribute (cn)." .

ocsf:function_keys a owl:DatatypeProperty ;
    rdfs:label "Function Keys" ;
    rdfs:range ocsf:integer_t ;
    dcterms:description "The number of function keys on client keyboard." .

ocsf:function_name a owl:DatatypeProperty ;
    rdfs:label "Function Name" ;
    rdfs:range ocsf:string_t ;
    dcterms:description "The entry-point function of the module. The system calls the entry-point function whenever a process or thread loads or unloads the module." .

ocsf:geohash a owl:DatatypeProperty ;
    rdfs:label "Geohash" ;
    rdfs:range ocsf:string_t ;
    dcterms:description "<p>Geohash of the geo-coordinates (latitude and longitude).</p><a target='_blank' href='https://en.wikipedia.org/wiki/Geohash'>Geohashing</a> is a geocoding system used to encode geographic coordinates in decimal degrees, to a single string." .

ocsf:given_name a owl:DatatypeProperty ;
    rdfs:label "Given Name" ;
    rdfs:range ocsf:string_t ;
    dcterms:description "The given or first name of the user." .

ocsf:group_name a owl:DatatypeProperty ;
    rdfs:label "Group Name" ;
    rdfs:range ocsf:string_t ;
    dcterms:description "The name of the group that the resource belongs to." .

ocsf:handshake_dur a owl:DatatypeProperty ;
    rdfs:label "Handshake Duration" ;
    rdfs:range ocsf:integer_t ;
    dcterms:description "The amount of total time for the TLS handshake to complete after the TCP connection is established, including client-side delays, in milliseconds." .

ocsf:hire_time a owl:DatatypeProperty ;
    rdfs:label "Hire Time" ;
    rdfs:range ocsf:timestamp_t ;
    dcterms:description "The timestamp when the user was or will be hired by the organization." .

ocsf:hostname a owl:DatatypeProperty ;
    rdfs:label "Hostname" ;
    rdfs:range ocsf:hostname_t ;
    dcterms:description "The hostname of an endpoint or a device." .

ocsf:http_method a owl:DatatypeProperty ;
    rdfs:label "HTTP Method" ;
    rdfs:range ocsf:string_t ;
    dcterms:description "The HTTP request method indicates the desired action to be performed for a given resource. Expected values: <ul> <li>TRACE</li> <li>CONNECT</li> <li>OPTIONS</li> <li>HEAD</li> <li>DELETE</li> <li>POST</li> <li>PUT</li> <li>GET</li></ul>" .

ocsf:http_only a owl:DatatypeProperty ;
    rdfs:label "HTTP Only" ;
    rdfs:range ocsf:boolean_t ;
    dcterms:description "A cookie attribute to make it inaccessible via JavaScript" .

ocsf:http_status a owl:DatatypeProperty ;
    rdfs:label "HTTP Status" ;
    rdfs:range ocsf:integer_t ;
    dcterms:description "The Hypertext Transfer Protocol (HTTP) <a target='_blank' href='https://www.iana.org/assignments/http-status-codes/http-status-codes.xhtml'>status code</a> returned to the client." .

ocsf:hypervisor a owl:DatatypeProperty ;
    rdfs:label "Hypervisor" ;
    rdfs:range ocsf:string_t ;
    dcterms:description "The name of the hypervisor running on the device. For example, <code>Xen</code>, <code>VMware</code>, <code>Hyper-V</code>, <code>VirtualBox</code>, etc." .

ocsf:identifier_cookie a owl:DatatypeProperty ;
    rdfs:label "Identifier Cookie" ;
    rdfs:range ocsf:string_t ;
    dcterms:description "The client identifier cookie during client/server exchange." .

ocsf:ime a owl:DatatypeProperty ;
    rdfs:label "IME" ;
    rdfs:range ocsf:string_t ;
    dcterms:description "The Input Method Editor (IME) file name." .

ocsf:imei a owl:DatatypeProperty ;
    rdfs:label "IMEI" ;
    rdfs:range ocsf:string_t ;
    dcterms:description "The International Mobile Station Equipment Identifier that is associated with the device." .

ocsf:impact a owl:DatatypeProperty ;
    rdfs:label "Impact" ;
    rdfs:range ocsf:string_t ;
    dcterms:description "The impact , normalized to the caption of the impact_id value. In the case of 'Other', it is defined by the event source." .

ocsf:impact_id a owl:DatatypeProperty ;
    rdfs:label "Impact ID" ;
    rdfs:range ocsf:integer_t ;
    dcterms:description "The normalized impact of the finding." ;
    jsonschema:enum "Critical",
        "High",
        "Low",
        "Medium",
        "Other",
        "Unknown" .

ocsf:impact_score a owl:DatatypeProperty ;
    rdfs:label "Impact" ;
    rdfs:range ocsf:integer_t ;
    dcterms:description "The impact of the finding, valid range 0-100." .

ocsf:injection_type a owl:DatatypeProperty ;
    rdfs:label "Injection Type" ;
    rdfs:range ocsf:string_t ;
    dcterms:description "The process injection method, normalized to the caption of the injection_type_id value. In the case of 'Other', it is defined by the event source." .

ocsf:injection_type_id a owl:DatatypeProperty ;
    rdfs:label "Injection Type ID" ;
    rdfs:range ocsf:integer_t ;
    dcterms:description "The normalized identifier of the process injection method." ;
    jsonschema:enum "Load Library",
        "Other",
        "Queue APC",
        "Remote Thread",
        "Unknown" .

ocsf:install_state a owl:DatatypeProperty ;
    rdfs:label "Install State" ;
    rdfs:range ocsf:string_t ;
    dcterms:description "The install state, normalized to the caption of install_state_id. In the case of 'Other', it is defined by the event source." .

ocsf:install_state_id a owl:DatatypeProperty ;
    rdfs:label "Install State ID" ;
    rdfs:range ocsf:integer_t ;
    dcterms:description "The normalized state of the install." ;
    jsonschema:enum "Installed",
        "Installed Pending Reboot",
        "Not Installed",
        "Other",
        "Unknown" .

ocsf:instance_uid a owl:DatatypeProperty ;
    rdfs:label "Instance ID" ;
    rdfs:range ocsf:string_t ;
    dcterms:description "The unique identifier of a VM instance." .

ocsf:integrity a owl:DatatypeProperty ;
    rdfs:label "Integrity" ;
    rdfs:range ocsf:string_t ;
    dcterms:description "The process integrity level, normalized to the caption of the integrity_id value. In the case of 'Other', it is defined by the event source (Windows only)." .

ocsf:integrity_id a owl:DatatypeProperty ;
    rdfs:label "Integrity Level" ;
    rdfs:range ocsf:integer_t ;
    dcterms:description "The normalized identifier of the process integrity level (Windows only)." ;
    jsonschema:enum "High",
        "Low",
        "Medium",
        "Other",
        "Protected",
        "System",
        "Unknown",
        "Untrusted" .

ocsf:interface_name a owl:DatatypeProperty ;
    rdfs:label "Network Interface Name" ;
    rdfs:range ocsf:string_t ;
    dcterms:description "The name of the network interface (e.g. eth2)." .

ocsf:interface_uid a owl:DatatypeProperty ;
    rdfs:label "Network Interface ID" ;
    rdfs:range ocsf:string_t ;
    dcterms:description "The unique identifier of the network interface." .

ocsf:intermediate_ips a owl:DatatypeProperty ;
    rdfs:label "Intermediate IP Addresses" ;
    rdfs:range ocsf:ip_t ;
    dcterms:description "The intermediate IP Addresses. For example, the IP addresses in the HTTP X-Forwarded-For header." .

ocsf:invoked_by a owl:DatatypeProperty ;
    rdfs:label "Invoked by" ;
    rdfs:range ocsf:string_t ;
    dcterms:description "The name of the service that invoked the activity as described in the event." .

ocsf:ip a owl:DatatypeProperty ;
    rdfs:label "IP Address" ;
    rdfs:range ocsf:ip_t ;
    dcterms:description "The IP address, in either IPv4 or IPv6 format." .

ocsf:is_applied a owl:DatatypeProperty ;
    rdfs:label "Applied" ;
    rdfs:range ocsf:boolean_t ;
    dcterms:description "A determination if a policy, rule, or enforcement action was applied." .

ocsf:is_cleartext a owl:DatatypeProperty ;
    rdfs:label "Cleartext Credentials" ;
    rdfs:range ocsf:boolean_t ;
    dcterms:description "Indicates whether the credentials were passed in clear text.<p><b>Note:</b> True if the credentials were passed in a clear text protocol such as FTP or TELNET, or if Windows detected that a user's logon password was passed to the authentication package in clear text.</p>" .

ocsf:is_compliant a owl:DatatypeProperty ;
    rdfs:label "Compliant Device" ;
    rdfs:range ocsf:boolean_t ;
    dcterms:description "The event occurred on a compliant device." .

ocsf:is_default a owl:DatatypeProperty ;
    rdfs:label "Default Value" ;
    rdfs:range ocsf:boolean_t ;
    dcterms:description "The indication of whether the value is from a default value name. For example, the value name could be missing." .

ocsf:is_exploit_available a owl:DatatypeProperty ;
    rdfs:label "Exploit Availability" ;
    rdfs:range ocsf:boolean_t ;
    dcterms:description "Indicates if an exploit or a PoC (proof-of-concept) is available for the reported vulnerability." .

ocsf:is_fix_available a owl:DatatypeProperty ;
    rdfs:label "Fix Availability" ;
    rdfs:range ocsf:boolean_t ;
    dcterms:description "Indicates if a fix is available for the reported vulnerability." .

ocsf:is_hotp a owl:DatatypeProperty ;
    rdfs:label "HMAC-based One-time Password (HOTP)" ;
    rdfs:range ocsf:boolean_t ;
    dcterms:description "Whether the authentication factor is an HMAC-based One-time Password (HOTP)." .

ocsf:is_http_only a owl:DatatypeProperty ;
    rdfs:label "HTTP Only" ;
    rdfs:range ocsf:boolean_t ;
    dcterms:description "This attribute prevents the cookie from being accessed via JavaScript." .

ocsf:is_managed a owl:DatatypeProperty ;
    rdfs:label "Managed Device" ;
    rdfs:range ocsf:boolean_t ;
    dcterms:description "The event occurred on a managed device." .

ocsf:is_mfa a owl:DatatypeProperty ;
    rdfs:label "Multi Factor Authentication" ;
    rdfs:range ocsf:boolean_t ;
    dcterms:description "Indicates whether Multi Factor Authentication was used during authentication." .

ocsf:is_new_logon a owl:DatatypeProperty ;
    rdfs:label "New Logon" ;
    rdfs:range ocsf:boolean_t ;
    dcterms:description "Indicates logon is from a device not seen before or a first time account logon." .

ocsf:is_on_premises a owl:DatatypeProperty ;
    rdfs:label "On Premises" ;
    rdfs:range ocsf:boolean_t ;
    dcterms:description "The indication of whether the location is on premises." .

ocsf:is_personal a owl:DatatypeProperty ;
    rdfs:label "Personal Device" ;
    rdfs:range ocsf:boolean_t ;
    dcterms:description "The event occurred on a personal device." .

ocsf:is_remote a owl:DatatypeProperty ;
    rdfs:label "Remote" ;
    rdfs:range ocsf:boolean_t ;
    dcterms:description "The indication of whether the session is remote." .

ocsf:is_renewal a owl:DatatypeProperty ;
    rdfs:label "Renewal" ;
    rdfs:range ocsf:boolean_t ;
    dcterms:description "The indication of whether this is a lease/session renewal event." .

ocsf:is_secure a owl:DatatypeProperty ;
    rdfs:label "Secure" ;
    rdfs:range ocsf:boolean_t ;
    dcterms:description "The cookie attribute indicates that cookies are sent to the server only when the request is encrypted using the HTTPS protocol." .

ocsf:is_self_signed a owl:DatatypeProperty ;
    rdfs:label "Certificate Self-Signed" ;
    rdfs:range ocsf:boolean_t ;
    dcterms:description "Denotes whether a digital certificate is self-signed or signed by a known certificate authority (CA)." .

ocsf:is_superseded a owl:DatatypeProperty ;
    rdfs:label "The patch is superseded." ;
    rdfs:range ocsf:boolean_t ;
    dcterms:description "The vendor patch has been replaced by another." .

ocsf:is_suspected_breach a owl:DatatypeProperty ;
    rdfs:label "Suspected Breach" ;
    rdfs:range ocsf:boolean_t ;
    dcterms:description "A determination based on analytics as to whether a potential breach was found." .

ocsf:is_system a owl:DatatypeProperty ;
    rdfs:label "System" ;
    rdfs:range ocsf:boolean_t ;
    dcterms:description "The indication of whether the object is part of the operating system." .

ocsf:is_totp a owl:DatatypeProperty ;
    rdfs:label "Time-based One-time Password (TOTP)" ;
    rdfs:range ocsf:boolean_t ;
    dcterms:description "Whether the authentication factor is a Time-based One-time Password (TOTP)." .

ocsf:is_trusted a owl:DatatypeProperty ;
    rdfs:label "Trusted Device" ;
    rdfs:range ocsf:boolean_t ;
    dcterms:description "The event occurred on a trusted device." .

ocsf:is_vpn a owl:DatatypeProperty ;
    rdfs:label "VPN Session" ;
    rdfs:range ocsf:boolean_t ;
    dcterms:description "The indication of whether the session is a VPN session." .

ocsf:isp a owl:DatatypeProperty ;
    rdfs:label "ISP" ;
    rdfs:range ocsf:string_t ;
    dcterms:description "The name of the Internet Service Provider (ISP)." .

ocsf:issuer a owl:DatatypeProperty ;
    rdfs:label "Issuer Details" ;
    rdfs:range ocsf:string_t ;
    dcterms:description "The identifier of the issuer. See specific usage." .

ocsf:job_title a owl:DatatypeProperty ;
    rdfs:label "Job Title" ;
    rdfs:range ocsf:string_t ;
    dcterms:description "The user's job title." .

ocsf:kb_articles a owl:DatatypeProperty ;
    rdfs:label "Knowledgebase Articles" ;
    rdfs:range ocsf:string_t ;
    dcterms:description "The KB article/s related to the entity. A KB Article contains metadata that describes the patch or an update." .

ocsf:key_length a owl:DatatypeProperty ;
    rdfs:label "Key Length" ;
    rdfs:range ocsf:integer_t ;
    dcterms:description "The length of the encryption key." .

ocsf:keyboard_layout a owl:DatatypeProperty ;
    rdfs:label "Keyboard Layout" ;
    rdfs:range ocsf:string_t ;
    dcterms:description "The keyboard locale identifier name (e.g., en-US)." .

ocsf:keyboard_subtype a owl:DatatypeProperty ;
    rdfs:label "Keyboard Subtype" ;
    rdfs:range ocsf:integer_t ;
    dcterms:description "The keyboard numeric code." .

ocsf:keyboard_type a owl:DatatypeProperty ;
    rdfs:label "Keyboard Type" ;
    rdfs:range ocsf:string_t ;
    dcterms:description "The keyboard type (e.g., xt, ico)." .

ocsf:labels a owl:DatatypeProperty ;
    rdfs:label "Labels" ;
    rdfs:range ocsf:string_t ;
    dcterms:description "The list of labels attached to an event, object, or attribute." .

ocsf:lang a owl:DatatypeProperty ;
    rdfs:label "Language" ;
    rdfs:range ocsf:string_t ;
    dcterms:description "The two letter lower case language codes, as defined by <a target='_blank' href='https://en.wikipedia.org/wiki/ISO_639-1'>ISO 639-1</a>. For example: <code>en</code> (English), <code>de</code> (German), or <code>fr</code> (French)." .

ocsf:last_login_time a owl:DatatypeProperty ;
    rdfs:label "Last Login" ;
    rdfs:range ocsf:timestamp_t ;
    dcterms:description "The last time when the user logged in." .

ocsf:last_run_time a owl:DatatypeProperty ;
    rdfs:label "Last Run" ;
    rdfs:range ocsf:timestamp_t ;
    dcterms:description "The last run time of application or service. See specific usage." .

ocsf:last_seen_time a owl:DatatypeProperty ;
    rdfs:label "Last Seen" ;
    rdfs:range ocsf:timestamp_t ;
    dcterms:description "The most recent detection time of the activity or object. See specific usage." .

ocsf:lat a owl:DatatypeProperty ;
    rdfs:label "Latitude" ;
    rdfs:range ocsf:float_t ;
    dcterms:description "The geographical Latitude coordinate represented in Decimal Degrees (DD). For example: <code>42.361145</code>." .

ocsf:latency a owl:DatatypeProperty ;
    rdfs:label "Latency" ;
    rdfs:range ocsf:integer_t ;
    dcterms:description "The HTTP response latency measured in milliseconds." .

ocsf:ldap_cn a owl:DatatypeProperty ;
    rdfs:label "LDAP Common Name" ;
    rdfs:range ocsf:string_t ;
    dcterms:description "The LDAP and X.500 <code>commonName</code> attribute, typically the full name of the person. For example, <code>John Doe</code>." .

ocsf:ldap_dn a owl:DatatypeProperty ;
    rdfs:label "LDAP Distinguished Name" ;
    rdfs:range ocsf:string_t ;
    dcterms:description "The X.500 Distinguished Name (DN) is a structured string that uniquely identifies an entry, such as a user, in an X.500 directory service For example, <code>cn=John Doe,ou=People,dc=example,dc=com</code>." .

ocsf:lease_dur a owl:DatatypeProperty ;
    rdfs:label "Lease Duration" ;
    rdfs:range ocsf:integer_t ;
    dcterms:description "This represents the length of the DHCP lease in seconds. This is present in DHCP Ack events." .

ocsf:leave_time a owl:DatatypeProperty ;
    rdfs:label "Leave Time" ;
    rdfs:range ocsf:timestamp_t ;
    dcterms:description "The timestamp when the user left or will be leaving the organization." .

ocsf:length a owl:DatatypeProperty ;
    rdfs:label "Response Length" ;
    rdfs:range ocsf:integer_t ;
    dcterms:description "The HTTP response length, in number of bytes." .

ocsf:license a owl:DatatypeProperty ;
    rdfs:label "Software License" ;
    rdfs:range ocsf:string_t ;
    dcterms:description "The name or identifier of the license applied on package or software. See <a target='_blank' href='https://spdx.org/licenses/'>SPDX License List</a>." .

ocsf:lineage a owl:DatatypeProperty ;
    rdfs:label "Lineage" ;
    rdfs:range ocsf:string_t ;
    dcterms:description "The lineage of the process, represented by a list of paths for each ancestor process. For example: <code>['/usr/sbin/sshd', '/usr/bin/bash', '/usr/bin/whoami']</code>." .

ocsf:load_type a owl:DatatypeProperty ;
    rdfs:label "Load Type" ;
    rdfs:range ocsf:string_t ;
    dcterms:description "The load type, normalized to the caption of the load_type_id value. In the case of 'Other', it is defined by the event source." .

ocsf:load_type_id a owl:DatatypeProperty ;
    rdfs:label "Load Type ID" ;
    rdfs:range ocsf:integer_t ;
    dcterms:description "The normalized identifier of the load type. See specific uasge." ;
    jsonschema:enum "Other",
        "Unknown" .

ocsf:loaded_modules a owl:DatatypeProperty ;
    rdfs:label "Loaded Modules" ;
    rdfs:range ocsf:string_t ;
    dcterms:description "The list of loaded module names." .

ocsf:log_level a owl:DatatypeProperty ;
    rdfs:label "Log Level" ;
    rdfs:range ocsf:string_t ;
    dcterms:description "The audit level at which an event was generated." .

ocsf:log_name a owl:DatatypeProperty ;
    rdfs:label "Log Name" ;
    rdfs:range ocsf:string_t ;
    dcterms:description "The event log name. For example, syslog file name or Windows logging subsystem: Security." .

ocsf:log_provider a owl:DatatypeProperty ;
    rdfs:label "Log Provider" ;
    rdfs:range ocsf:string_t ;
    dcterms:description "The logging provider or logging service that logged the event. For example, Microsoft-Windows-Security-Auditing." .

ocsf:log_type a owl:DatatypeProperty ;
    rdfs:label "Log Type" ;
    rdfs:range ocsf:string_t ;
    dcterms:description "The log type, normalized to the caption of the <code>log_type_id</code> value. In the case of 'Other', it is defined by the event source." .

ocsf:log_type_id a owl:DatatypeProperty ;
    rdfs:label "Log Type ID" ;
    rdfs:range ocsf:integer_t ;
    dcterms:description "The normalized log type identifier." ;
    jsonschema:enum "Application",
        "OS",
        "Other",
        "Unknown" .

ocsf:log_version a owl:DatatypeProperty ;
    rdfs:label "Log Version" ;
    rdfs:range ocsf:string_t ;
    dcterms:description "The event log schema version that specifies the format of the original event. For example syslog version or Cisco Log Schema Version." .

ocsf:logged_time a owl:DatatypeProperty ;
    rdfs:label "Logged Time" ;
    rdfs:range ocsf:timestamp_t ;
    dcterms:description "<p>The time when the logging system collected and logged the event.</p>This attribute is distinct from the event time in that event time typically contain the time extracted from the original event. Most of the time, these two times will be different." .

ocsf:logon_type a owl:DatatypeProperty ;
    rdfs:label "Logon Type" ;
    rdfs:range ocsf:string_t ;
    dcterms:description "The logon type, normalized to the caption of the logon_type_id value. In the case of 'Other', it is defined by the event source." .

ocsf:logon_type_id a owl:DatatypeProperty ;
    rdfs:label "Logon Type ID" ;
    rdfs:range ocsf:integer_t ;
    dcterms:description "The normalized logon type identifier." ;
    jsonschema:enum "Batch",
        "Cached Interactive",
        "Cached Remote Interactive",
        "Cached Unlock",
        "Interactive",
        "Network",
        "Network Cleartext",
        "New Credentials",
        "OS Service",
        "Other",
        "Remote Interactive",
        "System",
        "Unknown",
        "Unlock" .

ocsf:long a owl:DatatypeProperty ;
    rdfs:label "Longitude" ;
    rdfs:range ocsf:float_t ;
    dcterms:description "The geographical Longitude coordinate represented in Decimal Degrees (DD). For example: <code>-71.057083</code>." .

ocsf:mac a owl:DatatypeProperty ;
    rdfs:label "MAC Address" ;
    rdfs:range ocsf:mac_t ;
    dcterms:description "The Media Access Control (MAC) address that is associated with the network interface." .

ocsf:match_details a owl:DatatypeProperty ;
    rdfs:label "Match Details" ;
    rdfs:range ocsf:string_t ;
    dcterms:description "The data in a request that rule matched. For example: '[\"10\",\"and\",\"1\"]'." .

ocsf:match_location a owl:DatatypeProperty ;
    rdfs:label "Match Location" ;
    rdfs:range ocsf:string_t ;
    dcterms:description "The location of the matched data in the source which resulted in the triggered firewall rule. For example: HEADER." .

ocsf:message a owl:DatatypeProperty ;
    rdfs:label "Message" ;
    rdfs:range ocsf:string_t ;
    dcterms:description "The description of the event/finding, as defined by the source." .

ocsf:message_uid a owl:DatatypeProperty ;
    rdfs:label "Message UID" ;
    rdfs:range ocsf:string_t ;
    dcterms:description "The email header Message-Id value, as defined by RFC 5322." .

ocsf:mime_type a owl:DatatypeProperty ;
    rdfs:label "MIME type" ;
    rdfs:range ocsf:string_t ;
    dcterms:description "The Multipurpose Internet Mail Extensions (MIME) type of the file, if applicable." .

ocsf:model a owl:DatatypeProperty ;
    rdfs:label "Model" ;
    rdfs:range ocsf:string_t ;
    dcterms:description "The peripheral device model." .

ocsf:modified_time a owl:DatatypeProperty ;
    rdfs:label "Modified Time" ;
    rdfs:range ocsf:timestamp_t ;
    dcterms:description "The time when the object was last modified. See specific usage." .

ocsf:name a owl:DatatypeProperty ;
    rdfs:label "Name" ;
    rdfs:range ocsf:string_t ;
    dcterms:description "The name of the entity. See specific usage." .

ocsf:name_servers a owl:DatatypeProperty ;
    rdfs:label "Name Servers" ;
    rdfs:range ocsf:string_t ;
    dcterms:description "A collection of name servers related to a domain registration or other record." .

ocsf:namespace a owl:DatatypeProperty ;
    rdfs:label "Namespace" ;
    rdfs:range ocsf:string_t ;
    dcterms:description "The namespace is useful in merger or acquisition situations. For example, when similar entities exist that you need to keep separate." .

ocsf:namespace_pid a owl:DatatypeProperty ;
    rdfs:label "Namespace PID" ;
    rdfs:range ocsf:integer_t ;
    dcterms:description "If running under a process namespace (such as in a container), the process identifier within that process namespace." .

ocsf:network_driver a owl:DatatypeProperty ;
    rdfs:label "Network Driver" ;
    rdfs:range ocsf:string_t ;
    dcterms:description "The network driver used by the container. For example, bridge, overlay, host, none, etc." .

ocsf:next_run_time a owl:DatatypeProperty ;
    rdfs:label "Next Run" ;
    rdfs:range ocsf:timestamp_t ;
    dcterms:description "The next run time. See specific usage." .

ocsf:nist a owl:DatatypeProperty ;
    rdfs:label "NIST List" ;
    rdfs:range ocsf:string_t ;
    dcterms:description "The NIST Cybersecurity Framework recommendations for managing the cybersecurity risk." .

ocsf:num_detections a owl:DatatypeProperty ;
    rdfs:label "Detections" ;
    rdfs:range ocsf:integer_t ;
    dcterms:description "The number of detections." .

ocsf:num_files a owl:DatatypeProperty ;
    rdfs:label "Scanned Files" ;
    rdfs:range ocsf:integer_t ;
    dcterms:description "The number of files scanned." .

ocsf:num_folders a owl:DatatypeProperty ;
    rdfs:label "Scanned Folders" ;
    rdfs:range ocsf:integer_t ;
    dcterms:description "The number of folders scanned." .

ocsf:num_network_items a owl:DatatypeProperty ;
    rdfs:label "Scanned Network Items" ;
    rdfs:range ocsf:integer_t ;
    dcterms:description "The number of network items scanned." .

ocsf:num_processes a owl:DatatypeProperty ;
    rdfs:label "Scanned Processes" ;
    rdfs:range ocsf:integer_t ;
    dcterms:description "The number of processes scanned." .

ocsf:num_registry_items a owl:DatatypeProperty ;
    rdfs:label "Scanned Registry Items" ;
    rdfs:range ocsf:integer_t ;
    dcterms:description "The number of registry items scanned." .

ocsf:num_resolutions a owl:DatatypeProperty ;
    rdfs:label "Resolutions" ;
    rdfs:range ocsf:integer_t ;
    dcterms:description "The number of items that were resolved." .

ocsf:num_skipped_items a owl:DatatypeProperty ;
    rdfs:label "Skipped" ;
    rdfs:range ocsf:integer_t ;
    dcterms:description "The number of skipped items." .

ocsf:num_trusted_items a owl:DatatypeProperty ;
    rdfs:label "Trusted" ;
    rdfs:range ocsf:integer_t ;
    dcterms:description "The number of trusted items." .

ocsf:num_violations a owl:DatatypeProperty ;
    rdfs:label "Violations" ;
    rdfs:range ocsf:integer_t ;
    dcterms:description "The number of times the policy or rule was violated." .

ocsf:number a owl:DatatypeProperty ;
    rdfs:label "Number" ;
    rdfs:range ocsf:integer_t ;
    dcterms:description "The number of the entity. See specific usage." .

ocsf:office_location a owl:DatatypeProperty ;
    rdfs:label "Office Location" ;
    rdfs:range ocsf:string_t ;
    dcterms:description "The primary office location associated with the user. This could be any string and isn't a specific address. For example, <code>South East Virtual</code>." .

ocsf:opcode a owl:DatatypeProperty ;
    rdfs:label "DNS Opcode" ;
    rdfs:range ocsf:string_t ;
    dcterms:description "The DNS opcode specifies the type of the query message." .

ocsf:opcode_id a owl:DatatypeProperty ;
    rdfs:label "DNS Opcode ID" ;
    rdfs:range ocsf:integer_t ;
    dcterms:description "The DNS opcode ID specifies the normalized query message type as defined in <a target='_blank' href='https://www.rfc-editor.org/rfc/rfc5395.html'>RFC-5395</a>." ;
    jsonschema:enum "DSO Message",
        "Inverse Query",
        "Notify",
        "Other",
        "Query",
        "Reserved",
        "Status",
        "Update" .

ocsf:open_mask a owl:DatatypeProperty ;
    rdfs:label "Open Mask" ;
    rdfs:range ocsf:integer_t ;
    dcterms:description "The Windows options needed to open a registry key." .

ocsf:open_type a owl:DatatypeProperty ;
    rdfs:label "Open Type" ;
    rdfs:range ocsf:string_t ;
    dcterms:description "The file open type." .

ocsf:operation a owl:DatatypeProperty ;
    rdfs:label "Operation" ;
    rdfs:range ocsf:string_t ;
    dcterms:description "Verb/Operation associated with the request" .

ocsf:opnum a owl:DatatypeProperty ;
    rdfs:label "Opnum" ;
    rdfs:range ocsf:integer_t ;
    dcterms:description "An operation number used to identify a specific remote procedure call (RPC) method or a method in an interface." .

ocsf:orchestrator a owl:DatatypeProperty ;
    rdfs:label "Orchestrator" ;
    rdfs:range ocsf:string_t ;
    dcterms:description "The orchestrator managing the container, such as ECS, EKS, K8s, or OpenShift." .

ocsf:original_time a owl:DatatypeProperty ;
    rdfs:label "Original Time" ;
    rdfs:range ocsf:string_t ;
    dcterms:description "The original event time as reported by the event source. For example, the time in the original format from system event log such as Syslog on Unix/Linux and the System event file on Windows. Omit if event is generated instead of collected via logs." .

ocsf:ou_name a owl:DatatypeProperty ;
    rdfs:label "Org Unit Name" ;
    rdfs:range ocsf:string_t ;
    dcterms:description "The name of the organizational unit, within an organization.  For example, Finance, IT, R&D" .

ocsf:ou_uid a owl:DatatypeProperty ;
    rdfs:label "Org Unit ID" ;
    rdfs:range ocsf:string_t ;
    dcterms:description "The alternate identifier for an entity's unique identifier. For example, its Active Directory OU DN or AWS OU ID." .

ocsf:overall_score a owl:DatatypeProperty ;
    rdfs:label "Overall Score" ;
    rdfs:range ocsf:float_t ;
    dcterms:description "The overall score as reported by the event source. See specific usage." .

ocsf:package_manager a owl:DatatypeProperty ;
    rdfs:label "Package Manager" ;
    rdfs:range ocsf:string_t ;
    dcterms:description "The software packager manager utilized to manage a package on a system, e.g. npm, yum, dpkg etc." .

ocsf:packet_uid a owl:DatatypeProperty ;
    rdfs:label "Packet UID" ;
    rdfs:range ocsf:integer_t ;
    dcterms:description "The packet identifier assigned by the protocol." .

ocsf:packets a owl:DatatypeProperty ;
    rdfs:label "Total Packets" ;
    rdfs:range ocsf:long_t ;
    dcterms:description "The total number of packets (in and out)." .

ocsf:packets_in a owl:DatatypeProperty ;
    rdfs:label "Packets In" ;
    rdfs:range ocsf:long_t ;
    dcterms:description "The number of packets sent from the destination to the source." .

ocsf:packets_out a owl:DatatypeProperty ;
    rdfs:label "Packets Out" ;
    rdfs:range ocsf:long_t ;
    dcterms:description "The number of packets sent from the source to the destination." .

ocsf:parent_folder a owl:DatatypeProperty ;
    rdfs:label "Parent Folder" ;
    rdfs:range ocsf:string_t ;
    dcterms:description "The parent folder in which the file resides. For example: <code>c:\\windows\\system32</code>" .

ocsf:path a owl:DatatypeProperty ;
    rdfs:label "Path" ;
    rdfs:range ocsf:string_t ;
    dcterms:description "The path that pertains to the event or object. See specific usage." .

ocsf:pattern_match a owl:DatatypeProperty ;
    rdfs:label "Pattern Match" ;
    rdfs:range ocsf:string_t ;
    dcterms:description "A text, binary, file name, or datastore that matched against a detection rule." .

ocsf:percentile a owl:DatatypeProperty ;
    rdfs:label "EPSS Percentile" ;
    rdfs:range ocsf:float_t ;
    dcterms:description "The EPSS score's percentile representing relative importance and ranking of the score in the larger EPSS dataset." .

ocsf:permission a owl:DatatypeProperty ;
    rdfs:label "Permission" ;
    rdfs:range ocsf:string_t ;
    dcterms:description "The IAM permission related to an event" .

ocsf:phase a owl:DatatypeProperty ;
    rdfs:label "Kill Chain Phase" ;
    rdfs:range ocsf:string_t ;
    dcterms:description "The cyber kill chain phase." .

ocsf:phase_id a owl:DatatypeProperty ;
    rdfs:label "Kill Chain Phase ID" ;
    rdfs:range ocsf:integer_t ;
    dcterms:description "The cyber kill chain phase identifier." ;
    jsonschema:enum "Actions on Objectives",
        "Command & Control",
        "Delivery",
        "Exploitation",
        "Installation",
        "Other",
        "Reconnaissance",
        "Unknown",
        "Weaponization" .

ocsf:phone_number a owl:DatatypeProperty ;
    rdfs:label "Phone Number" ;
    rdfs:range ocsf:string_t ;
    dcterms:description "The number associated with the phone." .

ocsf:phones a owl:DatatypeProperty ;
    rdfs:label "Phones" ;
    rdfs:range ocsf:string_t ;
    dcterms:description "The phone numbers associated with the user" .

ocsf:physical_height a owl:DatatypeProperty ;
    rdfs:label "Physical Height" ;
    rdfs:range ocsf:integer_t ;
    dcterms:description "The numeric physical height of display." .

ocsf:physical_orientation a owl:DatatypeProperty ;
    rdfs:label "Physical Orientation" ;
    rdfs:range ocsf:integer_t ;
    dcterms:description "The numeric physical orientation of display." .

ocsf:physical_width a owl:DatatypeProperty ;
    rdfs:label "Physical Width" ;
    rdfs:range ocsf:integer_t ;
    dcterms:description "The numeric physical width of display." .

ocsf:pid a owl:DatatypeProperty ;
    rdfs:label "Process ID" ;
    rdfs:range ocsf:integer_t ;
    dcterms:description "The process identifier, as reported by the operating system. Process ID (PID) is a number used by the operating system to uniquely identify an active process." .

ocsf:pod_uuid a owl:DatatypeProperty ;
    rdfs:label "Pod UUID" ;
    rdfs:range ocsf:uuid_t ;
    dcterms:description "The unique identifier of the pod (or equivalent) that the container is executing on." .

ocsf:port a owl:DatatypeProperty ;
    rdfs:label "Port" ;
    rdfs:range ocsf:port_t ;
    dcterms:description "The TCP/UDP port number associated with a connection. See specific usage." .

ocsf:postal_code a owl:DatatypeProperty ;
    rdfs:label "Postal Code" ;
    rdfs:range ocsf:string_t ;
    dcterms:description "The postal code of the location." .

ocsf:precision a owl:DatatypeProperty ;
    rdfs:label "Precision" ;
    rdfs:range ocsf:integer_t ;
    dcterms:description "The numeric precision. See specific usage." .

ocsf:prev_security_level a owl:DatatypeProperty ;
    rdfs:label "Previous Security Level" ;
    rdfs:range ocsf:string_t ;
    dcterms:description "The previous security level of the entity" .

ocsf:prev_security_level_id a owl:DatatypeProperty ;
    rdfs:label "Previous Security Level ID" ;
    rdfs:range ocsf:integer_t ;
    dcterms:description "The previous security level of the entity" ;
    jsonschema:enum "At Risk",
        "Compromised",
        "Other",
        "Secure",
        "Unknown" .

ocsf:priority a owl:DatatypeProperty ;
    rdfs:label "Priority" ;
    rdfs:range ocsf:string_t ;
    dcterms:description "The priority, normalized to the caption of the priority_id value. In the case of 'Other', it is defined by the event source." .

ocsf:priority_id a owl:DatatypeProperty ;
    rdfs:label "Priority ID" ;
    rdfs:range ocsf:integer_t ;
    dcterms:description "The normalized priority. Priority identifies the relative importance of the finding. It is a measurement of urgency." ;
    jsonschema:enum "Critical",
        "High",
        "Low",
        "Medium",
        "Other",
        "Unknown" .

ocsf:privileges a owl:DatatypeProperty ;
    rdfs:label "Privileges" ;
    rdfs:range ocsf:string_t ;
    dcterms:description "The user or group privileges." .

ocsf:processed_time a owl:DatatypeProperty ;
    rdfs:label "Processed Time" ;
    rdfs:range ocsf:timestamp_t ;
    dcterms:description "The event processed time, such as an ETL operation." .

ocsf:product_uid a owl:DatatypeProperty ;
    rdfs:label "Product Identifier" ;
    rdfs:range ocsf:string_t ;
    dcterms:description "Unique Identifier of a product." .

ocsf:profiles a owl:DatatypeProperty ;
    rdfs:label "Profiles" ;
    rdfs:range ocsf:string_t ;
    dcterms:description "The list of profiles used to create the event.  Profiles should be referenced by their <code>name</code> attribute for core profiles, or <code>extension/name</code> for profiles from extensions." .

ocsf:project_uid a owl:DatatypeProperty ;
    rdfs:label "Project ID" ;
    rdfs:range ocsf:string_t ;
    dcterms:description "The unique identifier of a Cloud project." .

ocsf:protocol_name a owl:DatatypeProperty ;
    rdfs:label "Protocol Name" ;
    rdfs:range ocsf:string_t ;
    dcterms:description "The TCP/IP protocol name in lowercase, as defined by the Internet Assigned Numbers Authority (IANA). See <a target='_blank' href='https://www.iana.org/assignments/protocol-numbers/protocol-numbers.xhtml'>Protocol Numbers</a>. For example: <code>tcp</code> or <code>udp</code>." .

ocsf:protocol_num a owl:DatatypeProperty ;
    rdfs:label "Protocol Number" ;
    rdfs:range ocsf:integer_t ;
    dcterms:description "The TCP/IP protocol number, as defined by the Internet Assigned Numbers Authority (IANA). Use -1 if the protocol is not defined by IANA. See <a target='_blank' href='https://www.iana.org/assignments/protocol-numbers/protocol-numbers.xhtml'>Protocol Numbers</a>. For example: <code>6</code> for TCP and <code>17</code> for UDP." .

ocsf:protocol_ver a owl:DatatypeProperty ;
    rdfs:label "Protocol Version" ;
    rdfs:range ocsf:string_t ;
    dcterms:description "The Protocol version, normalized to the caption of the protocol_ver_id value. In the case of 'Other', it is defined by the event source." .

ocsf:protocol_ver_id a owl:DatatypeProperty ;
    rdfs:label "Protocol Version ID" ;
    rdfs:range ocsf:integer_t ;
    dcterms:description "The normalized identifier of the Protocol version. See specific usage." ;
    jsonschema:enum "Other",
        "Unknown" .

ocsf:provider a owl:DatatypeProperty ;
    rdfs:label "Provider" ;
    rdfs:range ocsf:string_t ;
    dcterms:description "The origin of information associated with the event. See specific usage." .

ocsf:purl a owl:DatatypeProperty ;
    rdfs:label "Package URL" ;
    rdfs:range ocsf:string_t ;
    dcterms:description "A purl is a URL string used to identify and locate a software package in a mostly universal and uniform way across programming languages, package managers, packaging conventions, tools, APIs and databases." .

ocsf:query_result a owl:DatatypeProperty ;
    rdfs:label "Query Result" ;
    rdfs:range ocsf:string_t ;
    dcterms:description "The result of the query." .

ocsf:query_result_id a owl:DatatypeProperty ;
    rdfs:label "Query Result ID" ;
    rdfs:range ocsf:integer_t ;
    dcterms:description "The normalized identifier of the query result." ;
    jsonschema:enum "Does not exist",
        "Error",
        "Exists",
        "Other",
        "Partial",
        "Unknown",
        "Unsupported" .

ocsf:query_string a owl:DatatypeProperty ;
    rdfs:label "HTTP Query String" ;
    rdfs:range ocsf:string_t ;
    dcterms:description "The query portion of the URL. For example: the query portion of the URL <code>http://www.example.com/search?q=bad&sort=date</code> is <code>q=bad&sort=date</code>." .

ocsf:query_time a owl:DatatypeProperty ;
    rdfs:label "Query Time" ;
    rdfs:range ocsf:timestamp_t ;
    dcterms:description "The Domain Name System (DNS) query time." .

ocsf:ram_size a owl:DatatypeProperty ;
    rdfs:label "RAM Size" ;
    rdfs:range ocsf:integer_t ;
    dcterms:description "The total amount of installed RAM, in Megabytes. For example: <code>2048</code>." .

ocsf:rate_limit a owl:DatatypeProperty ;
    rdfs:label "Rate Limit" ;
    rdfs:range ocsf:integer_t ;
    dcterms:description "The rate limit for a rate-based rule." .

ocsf:raw_data a owl:DatatypeProperty ;
    rdfs:label "Raw Data" ;
    rdfs:range ocsf:string_t ;
    dcterms:description "The raw event/finding data as received from the source." .

ocsf:raw_header a owl:DatatypeProperty ;
    rdfs:label "Raw Header" ;
    rdfs:range ocsf:string_t ;
    dcterms:description "The email authentication header." .

ocsf:rcode a owl:DatatypeProperty ;
    rdfs:label "Response Code" ;
    rdfs:range ocsf:string_t ;
    dcterms:description "The server response code, normalized to the caption of the rcode_id value. In the case of 'Other', it is defined by the event source." .

ocsf:rcode_id a owl:DatatypeProperty ;
    rdfs:label "Response Code ID" ;
    rdfs:range ocsf:integer_t ;
    dcterms:description "The normalized identifier of the server response code. See specific usage." ;
    jsonschema:enum "Other",
        "Unknown" .

ocsf:rdata a owl:DatatypeProperty ;
    rdfs:label "DNS RData" ;
    rdfs:range ocsf:string_t ;
    dcterms:description "The data describing the DNS resource. The meaning of this data depends on the type and class of the resource record." .

ocsf:references a owl:DatatypeProperty ;
    rdfs:label "References" ;
    rdfs:range ocsf:string_t ;
    dcterms:description "A list of reference URLs supporting the finding/detection." .

ocsf:referrer a owl:DatatypeProperty ;
    rdfs:label "HTTP Referrer" ;
    rdfs:range ocsf:string_t ;
    dcterms:description "The request header that identifies the address of the previous web page, which is linked to the current web page or resource being requested." .

ocsf:region a owl:DatatypeProperty ;
    rdfs:label "Region" ;
    rdfs:range ocsf:string_t ;
    dcterms:description "The name or the code of a region. See specific usage." .

ocsf:registrar a owl:DatatypeProperty ;
    rdfs:label "Domain Registrar" ;
    rdfs:range ocsf:string_t ;
    dcterms:description "The domain registrar." .

ocsf:related_vulnerabilities a owl:DatatypeProperty ;
    rdfs:label "Related Vulnerabilities" ;
    rdfs:range ocsf:string_t ;
    dcterms:description "List of vulnerabilities that are related to this vulnerability." .

ocsf:release a owl:DatatypeProperty ;
    rdfs:label "Software Release Details" ;
    rdfs:range ocsf:string_t ;
    dcterms:description "Release is the number of times a version of the software has been packaged." .

ocsf:reply_to a owl:DatatypeProperty ;
    rdfs:label "Reply To" ;
    rdfs:range ocsf:email_t ;
    dcterms:description "The email header Reply-To values, as defined by RFC 5322." .

ocsf:requested_permissions a owl:DatatypeProperty ;
    rdfs:label "Requested Permissions" ;
    rdfs:range ocsf:integer_t ;
    dcterms:description "The permissions mask that were requested by the process." .

ocsf:requirements a owl:DatatypeProperty ;
    rdfs:label "Compliance Requirements" ;
    rdfs:range ocsf:string_t ;
    dcterms:description "A list of requirements associated to a specific control in an industry or regulatory framework. e.g. <code> NIST.800-53.r5 AU-10 </code>" .

ocsf:resource_type a owl:DatatypeProperty ;
    rdfs:label "Resource Type" ;
    rdfs:range ocsf:string_t ;
    dcterms:description "The resource type as defined by the event source." .

ocsf:response_time a owl:DatatypeProperty ;
    rdfs:label "Response Time" ;
    rdfs:range ocsf:timestamp_t ;
    dcterms:description "The Domain Name System (DNS) response time." .

ocsf:risk_details a owl:DatatypeProperty ;
    rdfs:label "Risk Details" ;
    rdfs:range ocsf:string_t ;
    dcterms:description "Describes the risk associated with the finding." .

ocsf:risk_level a owl:DatatypeProperty ;
    rdfs:label "Risk Level" ;
    rdfs:range ocsf:string_t ;
    dcterms:description "The risk level, normalized to the caption of the risk_level_id value." .

ocsf:risk_level_id a owl:DatatypeProperty ;
    rdfs:label "Risk Level ID" ;
    rdfs:range ocsf:integer_t ;
    dcterms:description "The normalized risk level id." ;
    jsonschema:enum "Critical",
        "High",
        "Info",
        "Low",
        "Medium",
        "Other" .

ocsf:risk_score a owl:DatatypeProperty ;
    rdfs:label "Risk Score" ;
    rdfs:range ocsf:integer_t ;
    dcterms:description "The risk score as reported by the event source." .

ocsf:run_state a owl:DatatypeProperty ;
    rdfs:label "Run State" ;
    rdfs:range ocsf:string_t ;
    dcterms:description "The state of the job or service, normalized to the caption of the run_state_id value. In the case of 'Other', it is defined by the event source. See specific usage." .

ocsf:run_state_id a owl:DatatypeProperty ;
    rdfs:label "Run State ID" ;
    rdfs:range ocsf:integer_t ;
    dcterms:description "The normalized identifier of the state of the job or service. See specific usage." ;
    jsonschema:enum "Other",
        "Unknown" .

ocsf:runtime a owl:DatatypeProperty ;
    rdfs:label "Runtime" ;
    rdfs:range ocsf:string_t ;
    dcterms:description "The backend running the container, such as containerd or cri-o." .

ocsf:samesite a owl:DatatypeProperty ;
    rdfs:label "SameSite" ;
    rdfs:range ocsf:string_t ;
    dcterms:description "The cookie attribute that lets servers specify whether/when cookies are sent with cross-site requests. Values are: Strict, Lax or None" .

ocsf:sandbox a owl:DatatypeProperty ;
    rdfs:label "Sandbox" ;
    rdfs:range ocsf:string_t ;
    dcterms:description "The name of the containment jail (i.e., sandbox). For example, hardened_ps, high_security_ps, oracle_ps, netsvcs_ps, or default_ps." .

ocsf:scale_factor a owl:DatatypeProperty ;
    rdfs:label "Scale Factor" ;
    rdfs:range ocsf:integer_t ;
    dcterms:description "The numeric scale factor of display." .

ocsf:schedule_uid a owl:DatatypeProperty ;
    rdfs:label "Schedule UID" ;
    rdfs:range ocsf:string_t ;
    dcterms:description "The unique identifier of the schedule associated with a scan job." .

ocsf:scheme a owl:DatatypeProperty ;
    rdfs:label "Scheme" ;
    rdfs:range ocsf:string_t ;
    dcterms:description "The scheme portion of the URL. For example: <code>http</code>, <code>https</code>, <code>ftp</code>, or <code>sftp</code>." .

ocsf:score a owl:DatatypeProperty ;
    rdfs:label "Reputation Score" ;
    rdfs:range ocsf:string_t ;
    dcterms:description "The reputation score, normalized to the caption of the score_id value. In the case of 'Other', it is defined by the event source." .

ocsf:score_id a owl:DatatypeProperty ;
    rdfs:label "Reputation Score ID" ;
    rdfs:range ocsf:integer_t ;
    dcterms:description "The normalized reputation score identifier." ;
    jsonschema:enum "Exercise Caution",
        "Leans Safe",
        "Malicious",
        "May not be Safe",
        "Other",
        "Possibly Malicious",
        "Probably Malicious",
        "Probably Safe",
        "Safe",
        "Suspicious/Risky",
        "Unknown",
        "Very Safe" .

ocsf:section_a a owl:DatatypeProperty ;
    rdfs:label "JA4 Section A" ;
    rdfs:range ocsf:string_t ;
    dcterms:description "The 'a' section of the JA4 fingerprint." .

ocsf:section_b a owl:DatatypeProperty ;
    rdfs:label "JA4 Section B" ;
    rdfs:range ocsf:string_t ;
    dcterms:description "The 'b' section of the JA4 fingerprint." .

ocsf:section_c a owl:DatatypeProperty ;
    rdfs:label "JA4 Section C" ;
    rdfs:range ocsf:string_t ;
    dcterms:description "The 'c' section of the JA4 fingerprint." .

ocsf:section_d a owl:DatatypeProperty ;
    rdfs:label "JA4 Section D" ;
    rdfs:range ocsf:string_t ;
    dcterms:description "The 'd' section of the JA4 fingerprint." .

ocsf:secure a owl:DatatypeProperty ;
    rdfs:label "Secure" ;
    rdfs:range ocsf:boolean_t ;
    dcterms:description "The cookie attribute to only send cookies to the server with an encrypted request over the HTTPS protocol." .

ocsf:security_descriptor a owl:DatatypeProperty ;
    rdfs:label "Security Descriptor" ;
    rdfs:range ocsf:string_t ;
    dcterms:description "The object security descriptor." .

ocsf:security_level a owl:DatatypeProperty ;
    rdfs:label "Security Level" ;
    rdfs:range ocsf:string_t ;
    dcterms:description "The current security level of the entity" .

ocsf:security_level_id a owl:DatatypeProperty ;
    rdfs:label "Security Level ID" ;
    rdfs:range ocsf:integer_t ;
    dcterms:description "The current security level of the entity" ;
    jsonschema:enum "At Risk",
        "Compromised",
        "Other",
        "Secure",
        "Unknown" .

ocsf:security_questions a owl:DatatypeProperty ;
    rdfs:label "Security Questions" ;
    rdfs:range ocsf:string_t ;
    dcterms:description "The question(s) provided to user for a question-based authentication factor." .

ocsf:sensitivity a owl:DatatypeProperty ;
    rdfs:label "Sensitivity" ;
    rdfs:range ocsf:string_t ;
    dcterms:description "The sensitivity of the firewall rule in the matched event. For example: HIGH." .

ocsf:sequence a owl:DatatypeProperty ;
    rdfs:label "Sequence Number" ;
    rdfs:range ocsf:integer_t ;
    dcterms:description "Sequence number of the event. The sequence number is a value available in some events, to make the exact ordering of events unambiguous, regardless of the event time precision." .

ocsf:serial_number a owl:DatatypeProperty ;
    rdfs:label "Serial Number" ;
    rdfs:range ocsf:string_t ;
    dcterms:description "The serial number that pertains to the object. See specific usage." .

ocsf:server_ciphers a owl:DatatypeProperty ;
    rdfs:label "Server Cipher Suites" ;
    rdfs:range ocsf:string_t ;
    dcterms:description "The server cipher suites that were exchanged during the TLS handshake negotiation." .

ocsf:severity a owl:DatatypeProperty ;
    rdfs:label "Severity" ;
    rdfs:range ocsf:string_t ;
    dcterms:description "The event/finding severity, normalized to the caption of the severity_id value. In the case of 'Other', it is defined by the source." .

ocsf:severity_id a owl:DatatypeProperty ;
    rdfs:label "Severity ID" ;
    rdfs:range ocsf:integer_t ;
    dcterms:description "<p>The normalized identifier of the event/finding severity.</p>The normalized severity is a measurement the effort and expense required to manage and resolve an event or incident. Smaller numerical values represent lower impact events, and larger numerical values represent higher impact events." ;
    jsonschema:enum "Critical",
        "Fatal",
        "High",
        "Informational",
        "Low",
        "Medium",
        "Other",
        "Unknown" .

ocsf:share a owl:DatatypeProperty ;
    rdfs:label "Share" ;
    rdfs:range ocsf:string_t ;
    dcterms:description "The share name. See specific usage." .

ocsf:share_type a owl:DatatypeProperty ;
    rdfs:label "Share Type" ;
    rdfs:range ocsf:string_t ;
    dcterms:description "The share type, normalized to the caption of the share_type_id value. In the case of 'Other', it is defined by the event source." .

ocsf:share_type_id a owl:DatatypeProperty ;
    rdfs:label "Share Type Id" ;
    rdfs:range ocsf:integer_t ;
    dcterms:description "The normalized identifier of the share type." ;
    jsonschema:enum "File",
        "Other",
        "Pipe",
        "Print",
        "Unknown" .

ocsf:short_desc a owl:DatatypeProperty ;
    rdfs:label "Short Description" ;
    rdfs:range ocsf:string_t ;
    dcterms:description "The short description that pertains to the object or event. See specific usage." .

ocsf:size a owl:DatatypeProperty ;
    rdfs:label "Size" ;
    rdfs:range ocsf:long_t ;
    dcterms:description "The size of data, in bytes." .

ocsf:smtp_from a owl:DatatypeProperty ;
    rdfs:label "SMTP From" ;
    rdfs:range ocsf:email_t ;
    dcterms:description "The value of the SMTP MAIL FROM command." .

ocsf:smtp_hello a owl:DatatypeProperty ;
    rdfs:label "SMTP Hello" ;
    rdfs:range ocsf:string_t ;
    dcterms:description "The value of the SMTP HELO or EHLO command." .

ocsf:smtp_to a owl:DatatypeProperty ;
    rdfs:label "SMTP To" ;
    rdfs:range ocsf:email_t ;
    dcterms:description "The value of the SMTP envelope RCPT TO command." .

ocsf:sni a owl:DatatypeProperty ;
    rdfs:label "Server Name Indication" ;
    rdfs:range ocsf:string_t ;
    dcterms:description " The Server Name Indication (SNI) extension sent by the client." .

ocsf:sp_name a owl:DatatypeProperty ;
    rdfs:label "OS Service Pack" ;
    rdfs:range ocsf:string_t ;
    dcterms:description "The name of the latest Service Pack." .

ocsf:sp_ver a owl:DatatypeProperty ;
    rdfs:label "OS Service Pack Version" ;
    rdfs:range ocsf:integer_t ;
    dcterms:description "The version number of the latest Service Pack." .

ocsf:spf a owl:DatatypeProperty ;
    rdfs:label "SPF Status" ;
    rdfs:range ocsf:string_t ;
    dcterms:description "The Sender Policy Framework (SPF) status of the email." .

ocsf:src_url a owl:DatatypeProperty ;
    rdfs:label "Source URL" ;
    rdfs:range ocsf:url_t ;
    dcterms:description "The URL pointing towards the source of an entity. See specific usage." .

ocsf:standards a owl:DatatypeProperty ;
    rdfs:label "Security Standards" ;
    rdfs:range ocsf:string_t ;
    dcterms:description "Security standards are a set of criteria organizations can follow to protect sensitive and confidential information. e.g. <code>NIST SP 800-53, CIS AWS Foundations Benchmark v1.4.0, ISO/IEC 27001</code>" .

ocsf:start_address a owl:DatatypeProperty ;
    rdfs:label "Start Address" ;
    rdfs:range ocsf:string_t ;
    dcterms:description "The start address of the execution." .

ocsf:start_line a owl:DatatypeProperty ;
    rdfs:label "Start Line" ;
    rdfs:range ocsf:integer_t ;
    dcterms:description "The line number of the first line of code block identified as vulnerable." .

ocsf:start_time a owl:DatatypeProperty ;
    rdfs:label "Start Time" ;
    rdfs:range ocsf:timestamp_t ;
    dcterms:description "The start time of a time period. See specific usage." .

ocsf:state a owl:DatatypeProperty ;
    rdfs:label "State" ;
    rdfs:range ocsf:string_t ;
    dcterms:description "The state of the event or object, normalized to the caption of the state_id value. In the case of 'Other', it is defined by the event source. See specific usage." .

ocsf:state_id a owl:DatatypeProperty ;
    rdfs:label "State ID" ;
    rdfs:range ocsf:integer_t ;
    dcterms:description "The normalized state ID of the event or object. See specific usage." ;
    jsonschema:enum "Other",
        "Unknown" .

ocsf:status a owl:DatatypeProperty ;
    rdfs:label "Status" ;
    rdfs:range ocsf:string_t ;
    dcterms:description "The event status, normalized to the caption of the status_id value. In the case of 'Other', it is defined by the event source." .

ocsf:status_code a owl:DatatypeProperty ;
    rdfs:label "Status Code" ;
    rdfs:range ocsf:string_t ;
    dcterms:description "The event status code, as reported by the event source.<br /><br />For example, in a Windows Failed Authentication event, this would be the value of 'Failure Code', e.g. 0x18." .

ocsf:status_detail a owl:DatatypeProperty ;
    rdfs:label "Status Detail" ;
    rdfs:range ocsf:string_t ;
    dcterms:description "The status detail contains additional information about the event/finding outcome." .

ocsf:status_id a owl:DatatypeProperty ;
    rdfs:label "Status ID" ;
    rdfs:range ocsf:integer_t ;
    dcterms:description "The normalized identifier of the event status." ;
    jsonschema:enum "Failure",
        "Other",
        "Success",
        "Unknown" .

ocsf:stratum a owl:DatatypeProperty ;
    rdfs:label "Stratum" ;
    rdfs:range ocsf:string_t ;
    dcterms:description "The stratum level of the NTP server's time source, normalized to the caption of the stratum_id value." .

ocsf:stratum_id a owl:DatatypeProperty ;
    rdfs:label "Stratum ID" ;
    rdfs:range ocsf:integer_t ;
    dcterms:description "The normalized identifier of the stratum level, as defined in <a target='_blank' href='https://www.rfc-editor.org/rfc/rfc5905.html'>RFC-5905</a>." ;
    jsonschema:enum "Other",
        "Primary Server",
        "Reserved",
        "Secondary Server",
        "Unknown",
        "Unsynchronized" .

ocsf:subdomain a owl:DatatypeProperty ;
    rdfs:label "Subdomain" ;
    rdfs:range ocsf:string_t ;
    dcterms:description "The subdomain portion of the URL. For example: <code>sub</code> in <code>https://sub.example.com</code> or <code>sub2.sub1</code> in <code>https://sub2.sub1.example.com</code>." .

ocsf:subdomains a owl:DatatypeProperty ;
    rdfs:label "Subdomains" ;
    rdfs:range ocsf:string_t ;
    dcterms:description "An array of subdomain strings. Can be used to collect several subdomains such as those from Domain Generation Algorithms (DGAs)." .

ocsf:subject a owl:DatatypeProperty ;
    rdfs:label "Subject Details" ;
    rdfs:range ocsf:string_t ;
    dcterms:description "The identifier of the subject. See specific usage." .

ocsf:subnet a owl:DatatypeProperty ;
    rdfs:label "Subnet" ;
    rdfs:range ocsf:subnet_t ;
    dcterms:description "The subnet mask." .

ocsf:subnet_prefix a owl:DatatypeProperty ;
    rdfs:label "Subnet Prefix Length" ;
    rdfs:range ocsf:integer_t ;
    dcterms:description "The subnet prefix length determines the number of bits used to represent the network part of the IP address. The remaining bits are reserved for identifying individual hosts within that subnet." .

ocsf:subnet_uid a owl:DatatypeProperty ;
    rdfs:label "Subnet UID" ;
    rdfs:range ocsf:string_t ;
    dcterms:description "The unique identifier of a virtual subnet." .

ocsf:supporting_data a owl:DatatypeProperty ;
    rdfs:label "Supporting Data" ;
    rdfs:range ocsf:json_t ;
    dcterms:description "Additional data supporting a finding as provided by security tool" .

ocsf:surname a owl:DatatypeProperty ;
    rdfs:label "Surname" ;
    rdfs:range ocsf:string_t ;
    dcterms:description "The last or family name for the user." .

ocsf:svc_name a owl:DatatypeProperty ;
    rdfs:label "Service Name" ;
    rdfs:range ocsf:string_t ;
    dcterms:description "The service name in service-to-service connections. For example, AWS VPC logs the pkt-src-aws-service and pkt-dst-aws-service fields identify the connection is coming from or going to an AWS service." .

ocsf:system_call a owl:DatatypeProperty ;
    rdfs:label "System Call" ;
    rdfs:range ocsf:string_t ;
    dcterms:description "The system call that was invoked." .

ocsf:tag a owl:DatatypeProperty ;
    rdfs:label "Image Tag" ;
    rdfs:range ocsf:string_t ;
    dcterms:description "The image tag. For example: <code>1.11-alpine</code>." .

ocsf:tcp_flags a owl:DatatypeProperty ;
    rdfs:label "TCP Flags" ;
    rdfs:range ocsf:integer_t ;
    dcterms:description "The network connection TCP header flags (i.e., control bits)." .

ocsf:tenant_uid a owl:DatatypeProperty ;
    rdfs:label "Tenant UID" ;
    rdfs:range ocsf:string_t ;
    dcterms:description "The unique tenant identifier." .

ocsf:terminal a owl:DatatypeProperty ;
    rdfs:label "Terminal" ;
    rdfs:range ocsf:string_t ;
    dcterms:description "The Pseudo Terminal. Ex: the tty or pts value." .

ocsf:terminated_time a owl:DatatypeProperty ;
    rdfs:label "Terminated Time" ;
    rdfs:range ocsf:timestamp_t ;
    dcterms:description "The time when the entity was terminated. See specific usage." .

ocsf:tid a owl:DatatypeProperty ;
    rdfs:label "Thread ID" ;
    rdfs:range ocsf:integer_t ;
    dcterms:description "The Identifier of the thread associated with the event, as returned by the operating system." .

ocsf:time a owl:DatatypeProperty ;
    rdfs:label "Event Time" ;
    rdfs:range ocsf:timestamp_t ;
    dcterms:description "The normalized event occurrence time or the finding creation time." .

ocsf:timezone_offset a owl:DatatypeProperty ;
    rdfs:label "Timezone Offset" ;
    rdfs:range ocsf:integer_t ;
    dcterms:description "The number of minutes that the reported event <code>time</code> is ahead or behind UTC, in the range -1,080 to +1,080." .

ocsf:title a owl:DatatypeProperty ;
    rdfs:label "Title" ;
    rdfs:range ocsf:string_t ;
    dcterms:description "The title of an entity. See specific usage." .

ocsf:tlp a owl:DatatypeProperty ;
    rdfs:label "Traffic Light Protocol" ;
    rdfs:range ocsf:string_t ;
    dcterms:description "The <a target='_blank' href='https://www.first.org/tlp/'>Traffic Light Protocol</a> was created to facilitate greater sharing of potentially sensitive information and more effective collaboration. TLP provides a simple and intuitive schema for indicating with whom potentially sensitive information can be shared." .

ocsf:to a owl:DatatypeProperty ;
    rdfs:label "To" ;
    rdfs:range ocsf:email_t ;
    dcterms:description "The email header To values, as defined by RFC 5322." .

ocsf:total a owl:DatatypeProperty ;
    rdfs:label "Total" ;
    rdfs:range ocsf:integer_t ;
    dcterms:description "The total number of items. See specific usage." .

ocsf:transaction_uid a owl:DatatypeProperty ;
    rdfs:label "Transaction UID" ;
    rdfs:range ocsf:string_t ;
    dcterms:description "The unique identifier of the transaction." .

ocsf:transmit_time a owl:DatatypeProperty ;
    rdfs:label "Transmission Time" ;
    rdfs:range ocsf:timestamp_t ;
    dcterms:description "The event transmission time from one device to another.  See specific usage." .

ocsf:tree_uid a owl:DatatypeProperty ;
    rdfs:label "Tree UID" ;
    rdfs:range ocsf:string_t ;
    dcterms:description "The tree id is a unique SMB identifier which represents an open connection to a share." .

ocsf:ttl a owl:DatatypeProperty ;
    rdfs:label "TTL" ;
    rdfs:range ocsf:integer_t ;
    dcterms:description "The time interval that the resource record may be cached. Zero value means that the resource record can only be used for the transaction in progress, and should not be cached." .

ocsf:tunnel_type a owl:DatatypeProperty ;
    rdfs:label "Type" ;
    rdfs:range ocsf:string_t ;
    dcterms:description "The tunnel type. See specific usage." .

ocsf:tunnel_type_id a owl:DatatypeProperty ;
    rdfs:label "Type" ;
    rdfs:range ocsf:integer_t ;
    dcterms:description "The normalized tunnel type ID." .

ocsf:type a owl:DatatypeProperty ;
    rdfs:label "Type" ;
    rdfs:range ocsf:string_t ;
    dcterms:description "The type of an object or value, normalized to the caption of the type_id value. In the case of 'Other', it is defined by the event source. See specific usage." .

ocsf:type_id a owl:DatatypeProperty ;
    rdfs:label "Type ID" ;
    rdfs:range ocsf:integer_t ;
    dcterms:description "The normalized type identifier of an object. See specific usage." ;
    jsonschema:enum "Other",
        "Unknown" .

ocsf:type_name a owl:DatatypeProperty ;
    rdfs:label "Type Name" ;
    rdfs:range ocsf:string_t ;
    dcterms:description "The event/finding type name, as defined by the type_uid." .

ocsf:type_uid a owl:DatatypeProperty ;
    rdfs:label "Type ID" ;
    rdfs:range ocsf:long_t ;
    dcterms:description "The event/finding type ID. It identifies the event's semantics and structure. The value is calculated by the logging system as: <code>class_uid * 100 + activity_id</code>." .

ocsf:types a owl:DatatypeProperty ;
    rdfs:label "Types" ;
    rdfs:range ocsf:string_t ;
    dcterms:description "The type/s of an entity. See specific usage." .

ocsf:uid a owl:DatatypeProperty ;
    rdfs:label "Unique ID" ;
    rdfs:range ocsf:string_t ;
    dcterms:description "The unique identifier. See specific usage." .

ocsf:uid_alt a owl:DatatypeProperty ;
    rdfs:label "Alternate ID" ;
    rdfs:range ocsf:string_t ;
    dcterms:description "The alternate unique identifier. See specific usage." .

ocsf:url_string a owl:DatatypeProperty ;
    rdfs:label "URL String" ;
    rdfs:range ocsf:url_t ;
    dcterms:description "The URL string. See RFC 1738. For example: <code>http://www.example.com/download/trouble.exe</code>." .

ocsf:user_agent a owl:DatatypeProperty ;
    rdfs:label "HTTP User-Agent" ;
    rdfs:range ocsf:string_t ;
    dcterms:description "The request header that identifies the operating system and web browser." .

ocsf:uuid a owl:DatatypeProperty ;
    rdfs:label "UUID" ;
    rdfs:range ocsf:uuid_t ;
    dcterms:description "The universally unique identifier. See specific usage." .

ocsf:value a owl:DatatypeProperty ;
    rdfs:label "Value" ;
    rdfs:range ocsf:string_t ;
    dcterms:description "The value that pertains to the object. See specific usage." .

ocsf:vector_string a owl:DatatypeProperty ;
    rdfs:label "Vector String" ;
    rdfs:range ocsf:string_t ;
    dcterms:description "The CVSS vector string is a text representation of a set of CVSS metrics. It is commonly used to record or transfer CVSS metric information in a concise form. For example: <code>3.1/AV:L/AC:L/PR:L/UI:N/S:U/C:H/I:N/A:H</code>." .

ocsf:vendor_name a owl:DatatypeProperty ;
    rdfs:label "Vendor Name" ;
    rdfs:range ocsf:string_t ;
    dcterms:description "The name of the vendor. See specific usage." .

ocsf:verdict a owl:DatatypeProperty ;
    rdfs:label "Verdict" ;
    rdfs:range ocsf:string_t ;
    dcterms:description "The verdict assigned to an Incident finding." .

ocsf:verdict_id a owl:DatatypeProperty ;
    rdfs:label "Verdict ID" ;
    rdfs:range ocsf:integer_t ;
    dcterms:description "The normalized verdict of an Incident." ;
    jsonschema:enum "Benign",
        "Disregard",
        "Duplicate",
        "False Positive",
        "Insufficient Data",
        "Managed Externally",
        "Other",
        "Security Risk",
        "Suspicious",
        "Test",
        "True Positive",
        "Unknown" .

ocsf:version a owl:DatatypeProperty ;
    rdfs:label "Version" ;
    rdfs:range ocsf:string_t ;
    dcterms:description "The version that pertains to the event or object. See specific usage." .

ocsf:vlan_uid a owl:DatatypeProperty ;
    rdfs:label "VLAN" ;
    rdfs:range ocsf:string_t ;
    dcterms:description "The Virtual LAN identifier." .

ocsf:vpc_uid a owl:DatatypeProperty ;
    rdfs:label "VPC UID" ;
    rdfs:range ocsf:string_t ;
    dcterms:description "The unique identifier of the Virtual Private Cloud (VPC)." .

ocsf:x_forwarded_for a owl:DatatypeProperty ;
    rdfs:label "X-Forwarded-For" ;
    rdfs:range ocsf:ip_t ;
    dcterms:description "The X-Forwarded-For header identifying the originating IP address(es) of a client connecting to a web server through an HTTP proxy or a load balancer." .

ocsf:x_originating_ip a owl:DatatypeProperty ;
    rdfs:label "X-Originating-IP" ;
    rdfs:range ocsf:ip_t ;
    dcterms:description "The X-Originating-IP header identifying the emails originating IP address(es)." .

ocsf:zone a owl:DatatypeProperty ;
    rdfs:label "Network Zone" ;
    rdfs:range ocsf:string_t ;
    dcterms:description "The network zone or LAN segment." .

### Classes

ocsf:Account a owl:Class ;
    rdfs:label "Account" ;
    rdfs:subClassOf ocsf:Entity,
        [ a owl:Restriction ;
            owl:onProperty ocsf:labels ;
            owl:allValuesFrom ocsf:string_t ],
        [ a owl:Restriction ;
            owl:onProperty ocsf:name ;
            owl:allValuesFrom ocsf:string_t ],
        [ a owl:Restriction ;
            owl:onProperty ocsf:type ;
            owl:allValuesFrom ocsf:string_t ],
        [ a owl:Restriction ;
            owl:onProperty ocsf:type_id ;
            owl:allValuesFrom ocsf:integer_t ],
        [ a owl:Restriction ;
            owl:onProperty ocsf:uid ;
            owl:allValuesFrom ocsf:string_t ] ;
    dcterms:description "The Account object contains details about the account that initiated or performed a specific activity within a system or application." ;
    ocsf:extends "_entity" ;
    ocsf:name "account" .

ocsf:AccountChangeEvent a owl:Class ;
    rdfs:label "Account Change" ;
    rdfs:subClassOf ocsf:IdentityAccessManagementEvent,
        [ a owl:Restriction ;
            owl:onProperty ocsf:activity_id ;
            owl:allValuesFrom ocsf:integer_t ],
        [ a owl:Restriction ;
            owl:onProperty ocsf:actor ;
            owl:allValuesFrom ocsf:Actor ],
        [ a owl:Restriction ;
            owl:onProperty ocsf:policy ;
            owl:allValuesFrom ocsf:Policy ],
        [ a owl:Restriction ;
            owl:onProperty ocsf:user ;
            owl:allValuesFrom ocsf:User ],
        [ a owl:Restriction ;
            owl:onProperty ocsf:user ;
            owl:someValuesFrom ocsf:User ],
        [ a owl:Restriction ;
            owl:onProperty ocsf:user_result ;
            owl:allValuesFrom ocsf:User ] ;
    dcterms:description "Account Change events report when specific user account management tasks are performed, such as a user/role being created, changed, deleted, renamed, disabled, enabled, locked out or unlocked." ;
    ocsf:extends "iam" ;
    ocsf:name "account_change" .

ocsf:Actor a owl:Class ;
    rdfs:label "Actor" ;
    rdfs:subClassOf ocsf:Object,
        [ a owl:Restriction ;
            owl:onProperty ocsf:app_name ;
            owl:allValuesFrom ocsf:string_t ],
        [ a owl:Restriction ;
            owl:onProperty ocsf:app_uid ;
            owl:allValuesFrom ocsf:string_t ],
        [ a owl:Restriction ;
            owl:onProperty ocsf:authorizations ;
            owl:allValuesFrom ocsf:AuthorizationResult ],
        [ a owl:Restriction ;
            owl:onProperty ocsf:idp ;
            owl:allValuesFrom ocsf:IdentityProvider ],
        [ a owl:Restriction ;
            owl:onProperty ocsf:invoked_by ;
            owl:allValuesFrom ocsf:string_t ],
        [ a owl:Restriction ;
            owl:onProperty ocsf:process ;
            owl:allValuesFrom ocsf:Process ],
        [ a owl:Restriction ;
            owl:onProperty ocsf:session ;
            owl:allValuesFrom ocsf:Session ],
        [ a owl:Restriction ;
            owl:onProperty ocsf:user ;
            owl:allValuesFrom ocsf:User ] ;
    dcterms:description "The Actor object contains details about the user, role, application, service, or process that initiated or performed a specific activity." ;
    ocsf:constraints "{\"at_least_one\":[\"process\",\"user\",\"invoked_by\",\"session\",\"app_name\",\"app_uid\"]}" ;
    ocsf:extends "object" ;
    ocsf:name "actor" .

ocsf:AdminGroupQueryEvent a owl:Class ;
    rdfs:label "Admin Group Query" ;
    rdfs:subClassOf ocsf:DiscoveryResultEvent,
        [ a owl:Restriction ;
            owl:onProperty ocsf:group ;
            owl:allValuesFrom ocsf:Group ],
        [ a owl:Restriction ;
            owl:onProperty ocsf:group ;
            owl:someValuesFrom ocsf:Group ],
        [ a owl:Restriction ;
            owl:onProperty ocsf:users ;
            owl:allValuesFrom ocsf:User ] ;
    dcterms:description "Admin Group Query events report information about administrative groups." ;
    ocsf:extends "discovery_result" ;
    ocsf:name "admin_group_query" .

ocsf:AffectedCode a owl:Class ;
    rdfs:label "Affected Code" ;
    rdfs:subClassOf ocsf:Object,
        [ a owl:Restriction ;
            owl:onProperty ocsf:end_line ;
            owl:allValuesFrom ocsf:integer_t ],
        [ a owl:Restriction ;
            owl:onProperty ocsf:file ;
            owl:allValuesFrom ocsf:File ],
        [ a owl:Restriction ;
            owl:onProperty ocsf:file ;
            owl:someValuesFrom ocsf:File ],
        [ a owl:Restriction ;
            owl:onProperty ocsf:owner ;
            owl:allValuesFrom ocsf:User ],
        [ a owl:Restriction ;
            owl:onProperty ocsf:remediation ;
            owl:allValuesFrom ocsf:Remediation ],
        [ a owl:Restriction ;
            owl:onProperty ocsf:start_line ;
            owl:allValuesFrom ocsf:integer_t ] ;
    dcterms:description "The Affected Code object describes details about a code block identified as vulnerable." ;
    ocsf:extends "object" ;
    ocsf:name "affected_code" .

ocsf:AffectedSoftwarePackage a owl:Class ;
    rdfs:label "Affected Software Package" ;
    rdfs:subClassOf ocsf:SoftwarePackage,
        [ a owl:Restriction ;
            owl:onProperty ocsf:fixed_in_version ;
            owl:allValuesFrom ocsf:string_t ],
        [ a owl:Restriction ;
            owl:onProperty ocsf:package_manager ;
            owl:allValuesFrom ocsf:string_t ],
        [ a owl:Restriction ;
            owl:onProperty ocsf:path ;
            owl:allValuesFrom ocsf:string_t ],
        [ a owl:Restriction ;
            owl:onProperty ocsf:remediation ;
            owl:allValuesFrom ocsf:Remediation ] ;
    dcterms:description "The Affected Package object describes details about a software package identified as affected by a vulnerability/vulnerabilities." ;
    ocsf:extends "package" ;
    ocsf:name "affected_package" .

ocsf:Agent a owl:Class ;
    rdfs:label "Agent" ;
    rdfs:subClassOf ocsf:Object,
        [ a owl:Restriction ;
            owl:onProperty ocsf:name ;
            owl:allValuesFrom ocsf:string_t ],
        [ a owl:Restriction ;
            owl:onProperty ocsf:policies ;
            owl:allValuesFrom ocsf:Policy ],
        [ a owl:Restriction ;
            owl:onProperty ocsf:type ;
            owl:allValuesFrom ocsf:string_t ],
        [ a owl:Restriction ;
            owl:onProperty ocsf:type_id ;
            owl:allValuesFrom ocsf:integer_t ],
        [ a owl:Restriction ;
            owl:onProperty ocsf:uid ;
            owl:allValuesFrom ocsf:string_t ],
        [ a owl:Restriction ;
            owl:onProperty ocsf:uid_alt ;
            owl:allValuesFrom ocsf:string_t ],
        [ a owl:Restriction ;
            owl:onProperty ocsf:vendor_name ;
            owl:allValuesFrom ocsf:string_t ],
        [ a owl:Restriction ;
            owl:onProperty ocsf:version ;
            owl:allValuesFrom ocsf:string_t ] ;
    dcterms:description "An Agent (also known as a Sensor) is typically installed on an Operating System (OS) and serves as a specialized software component that can be designed to monitor, detect, collect, archive, or take action. These activities and possible actions are defined by the upstream system controlling the Agent and its intended purpose. For instance, an Agent can include Endpoint Detection & Response (EDR) agents, backup/disaster recovery sensors, Application Performance Monitoring or profiling sensors, and similar software." ;
    ocsf:constraints "{\"at_least_one\":[\"uid\",\"name\"]}" ;
    ocsf:extends "object" ;
    ocsf:name "agent" .

ocsf:Analytic a owl:Class ;
    rdfs:label "Analytic" ;
    rdfs:subClassOf ocsf:Entity,
        [ a owl:Restriction ;
            owl:onProperty ocsf:category ;
            owl:allValuesFrom ocsf:string_t ],
        [ a owl:Restriction ;
            owl:onProperty ocsf:desc ;
            owl:allValuesFrom ocsf:string_t ],
        [ a owl:Restriction ;
            owl:onProperty ocsf:name ;
            owl:allValuesFrom ocsf:string_t ],
        [ a owl:Restriction ;
            owl:onProperty ocsf:related_analytics ;
            owl:allValuesFrom ocsf:Analytic ],
        [ a owl:Restriction ;
            owl:onProperty ocsf:type ;
            owl:allValuesFrom ocsf:string_t ],
        [ a owl:Restriction ;
            owl:onProperty ocsf:type_id ;
            owl:allValuesFrom ocsf:integer_t ],
        [ a owl:Restriction ;
            owl:onProperty ocsf:type_id ;
            owl:cardinality 1 ],
        [ a owl:Restriction ;
            owl:onProperty ocsf:uid ;
            owl:allValuesFrom ocsf:string_t ],
        [ a owl:Restriction ;
            owl:onProperty ocsf:version ;
            owl:allValuesFrom ocsf:string_t ] ;
    dcterms:description "The Analytic object contains details about the analytic technique used to analyze and derive insights from the data or information that led to the creation of a finding or conclusion." ;
    ocsf:extends "_entity" ;
    ocsf:name "analytic" .

ocsf:API a owl:Class ;
    rdfs:label "API" ;
    rdfs:subClassOf ocsf:Object,
        [ a owl:Restriction ;
            owl:onProperty ocsf:group ;
            owl:allValuesFrom ocsf:Group ],
        [ a owl:Restriction ;
            owl:onProperty ocsf:operation ;
            owl:allValuesFrom ocsf:string_t ],
        [ a owl:Restriction ;
            owl:onProperty ocsf:operation ;
            owl:cardinality 1 ],
        [ a owl:Restriction ;
            owl:onProperty ocsf:request ;
            owl:allValuesFrom ocsf:RequestElements ],
        [ a owl:Restriction ;
            owl:onProperty ocsf:response ;
            owl:allValuesFrom ocsf:ResponseElements ],
        [ a owl:Restriction ;
            owl:onProperty ocsf:service ;
            owl:allValuesFrom ocsf:Service ],
        [ a owl:Restriction ;
            owl:onProperty ocsf:version ;
            owl:allValuesFrom ocsf:string_t ] ;
    dcterms:description "The API, or Application Programming Interface, object represents  information pertaining to an API request and response." ;
    ocsf:extends "object" ;
    ocsf:name "api" .

ocsf:APIActivityEvent a owl:Class ;
    rdfs:label "API Activity" ;
    rdfs:subClassOf ocsf:ApplicationActivityEvent,
        [ a owl:Restriction ;
            owl:onProperty ocsf:activity_id ;
            owl:allValuesFrom ocsf:integer_t ],
        [ a owl:Restriction ;
            owl:onProperty ocsf:actor ;
            owl:allValuesFrom ocsf:Actor ],
        [ a owl:Restriction ;
            owl:onProperty ocsf:actor ;
            owl:someValuesFrom ocsf:Actor ],
        [ a owl:Restriction ;
            owl:onProperty ocsf:api ;
            owl:allValuesFrom ocsf:API ],
        [ a owl:Restriction ;
            owl:onProperty ocsf:api ;
            owl:someValuesFrom ocsf:API ],
        [ a owl:Restriction ;
            owl:onProperty ocsf:dst_endpoint ;
            owl:allValuesFrom ocsf:NetworkEndpoint ],
        [ a owl:Restriction ;
            owl:onProperty ocsf:http_request ;
            owl:allValuesFrom ocsf:HTTPRequest ],
        [ a owl:Restriction ;
            owl:onProperty ocsf:resources ;
            owl:allValuesFrom ocsf:ResourceDetails ],
        [ a owl:Restriction ;
            owl:onProperty ocsf:src_endpoint ;
            owl:allValuesFrom ocsf:NetworkEndpoint ],
        [ a owl:Restriction ;
            owl:onProperty ocsf:src_endpoint ;
            owl:someValuesFrom ocsf:NetworkEndpoint ] ;
    dcterms:description "API events describe general CRUD (Create, Read, Update, Delete) API activities, e.g. (AWS Cloudtrail)" ;
    ocsf:extends "application" ;
    ocsf:name "api_activity" .

ocsf:ApplicationActivityEvent a owl:Class ;
    rdfs:label "Application Activity" ;
    rdfs:subClassOf ocsf:BaseEvent ;
    ocsf:category ocsf:ApplicationActivityEvent ;
    ocsf:extends "base_event" ;
    ocsf:name "application" .

ocsf:ApplicationActivityEventCategory a owl:Class ;
    rdfs:label "Application Activity" ;
    rdfs:subClassOf ocsf:EventCategory ;
    d3f:definition "Application Activity events report detailed information about the behavior of applications and services." ;
    ocsf:category_name "application" .

ocsf:ApplicationLifecycleEvent a owl:Class ;
    rdfs:label "Application Lifecycle" ;
    rdfs:subClassOf ocsf:ApplicationActivityEvent,
        [ a owl:Restriction ;
            owl:onProperty ocsf:activity_id ;
            owl:allValuesFrom ocsf:integer_t ],
        [ a owl:Restriction ;
            owl:onProperty ocsf:activity_id ;
            owl:cardinality 1 ],
        [ a owl:Restriction ;
            owl:onProperty ocsf:app ;
            owl:allValuesFrom ocsf:Product ],
        [ a owl:Restriction ;
            owl:onProperty ocsf:app ;
            owl:someValuesFrom ocsf:Product ] ;
    dcterms:description "Application Lifecycle events report installation, removal, start, stop of an application or service." ;
    ocsf:extends "application" ;
    ocsf:name "application_lifecycle" ;
    ocsf:profiles "host" .

ocsf:AuthenticationEvent a owl:Class ;
    rdfs:label "Authentication" ;
    rdfs:subClassOf ocsf:IdentityAccessManagementEvent,
        [ a owl:Restriction ;
            owl:onProperty ocsf:activity_id ;
            owl:allValuesFrom ocsf:integer_t ],
        [ a owl:Restriction ;
            owl:onProperty ocsf:actor ;
            owl:allValuesFrom ocsf:Actor ],
        [ a owl:Restriction ;
            owl:onProperty ocsf:auth_factors ;
            owl:allValuesFrom ocsf:AuthenticationFactor ],
        [ a owl:Restriction ;
            owl:onProperty ocsf:auth_protocol ;
            owl:allValuesFrom ocsf:string_t ],
        [ a owl:Restriction ;
            owl:onProperty ocsf:auth_protocol_id ;
            owl:allValuesFrom ocsf:integer_t ],
        [ a owl:Restriction ;
            owl:onProperty ocsf:certificate ;
            owl:allValuesFrom ocsf:DigitalCertificate ],
        [ a owl:Restriction ;
            owl:onProperty ocsf:dst_endpoint ;
            owl:allValuesFrom ocsf:NetworkEndpoint ],
        [ a owl:Restriction ;
            owl:onProperty ocsf:is_cleartext ;
            owl:allValuesFrom ocsf:boolean_t ],
        [ a owl:Restriction ;
            owl:onProperty ocsf:is_mfa ;
            owl:allValuesFrom ocsf:boolean_t ],
        [ a owl:Restriction ;
            owl:onProperty ocsf:is_new_logon ;
            owl:allValuesFrom ocsf:boolean_t ],
        [ a owl:Restriction ;
            owl:onProperty ocsf:is_remote ;
            owl:allValuesFrom ocsf:boolean_t ],
        [ a owl:Restriction ;
            owl:onProperty ocsf:logon_process ;
            owl:allValuesFrom ocsf:Process ],
        [ a owl:Restriction ;
            owl:onProperty ocsf:logon_type ;
            owl:allValuesFrom ocsf:string_t ],
        [ a owl:Restriction ;
            owl:onProperty ocsf:logon_type_id ;
            owl:allValuesFrom ocsf:integer_t ],
        [ a owl:Restriction ;
            owl:onProperty ocsf:service ;
            owl:allValuesFrom ocsf:Service ],
        [ a owl:Restriction ;
            owl:onProperty ocsf:session ;
            owl:allValuesFrom ocsf:Session ],
        [ a owl:Restriction ;
            owl:onProperty ocsf:status_detail ;
            owl:allValuesFrom ocsf:string_t ],
        [ a owl:Restriction ;
            owl:onProperty ocsf:user ;
            owl:allValuesFrom ocsf:User ],
        [ a owl:Restriction ;
            owl:onProperty ocsf:user ;
            owl:someValuesFrom ocsf:User ] ;
    dcterms:description "Authentication events report authentication session activities such as user attempts a logon or logoff, successfully or otherwise." ;
    ocsf:associations "{\"actor.user\":[\"src_endpoint\"],\"dst_endpoint\":[\"user\"],\"src_endpoint\":[\"actor.user\"],\"user\":[\"dst_endpoint\"]}" ;
    ocsf:constraints "{\"at_least_one\":[\"service\",\"dst_endpoint\"]}" ;
    ocsf:extends "iam" ;
    ocsf:name "authentication" .

ocsf:AuthenticationFactor a owl:Class ;
    rdfs:label "Authentication Factor" ;
    rdfs:subClassOf ocsf:Object,
        [ a owl:Restriction ;
            owl:onProperty ocsf:device ;
            owl:allValuesFrom ocsf:Device ],
        [ a owl:Restriction ;
            owl:onProperty ocsf:email_addr ;
            owl:allValuesFrom ocsf:email_t ],
        [ a owl:Restriction ;
            owl:onProperty ocsf:factor_type ;
            owl:allValuesFrom ocsf:string_t ],
        [ a owl:Restriction ;
            owl:onProperty ocsf:factor_type_id ;
            owl:allValuesFrom ocsf:integer_t ],
        [ a owl:Restriction ;
            owl:onProperty ocsf:factor_type_id ;
            owl:cardinality 1 ],
        [ a owl:Restriction ;
            owl:onProperty ocsf:is_hotp ;
            owl:allValuesFrom ocsf:boolean_t ],
        [ a owl:Restriction ;
            owl:onProperty ocsf:is_totp ;
            owl:allValuesFrom ocsf:boolean_t ],
        [ a owl:Restriction ;
            owl:onProperty ocsf:phone_number ;
            owl:allValuesFrom ocsf:string_t ],
        [ a owl:Restriction ;
            owl:onProperty ocsf:provider ;
            owl:allValuesFrom ocsf:string_t ],
        [ a owl:Restriction ;
            owl:onProperty ocsf:security_questions ;
            owl:allValuesFrom ocsf:string_t ] ;
    dcterms:description "An Authentication Factor object describes a category of methods used for identity verification in an authentication attempt." ;
    ocsf:constraints "{\"just_one\":[\"email_addr\",\"phone_number\",\"security_questions\"]}" ;
    ocsf:extends "object" ;
    ocsf:name "auth_factor" .

ocsf:AuthorizationResult a owl:Class ;
    rdfs:label "Authorization Result" ;
    rdfs:subClassOf ocsf:Object,
        [ a owl:Restriction ;
            owl:onProperty ocsf:decision ;
            owl:allValuesFrom ocsf:string_t ],
        [ a owl:Restriction ;
            owl:onProperty ocsf:policy ;
            owl:allValuesFrom ocsf:Policy ] ;
    dcterms:description "The Authorization Result object provides details about the authorization outcome and associated policies related to activity." ;
    ocsf:extends "object" ;
    ocsf:name "authorization" .

ocsf:AuthorizeSessionEvent a owl:Class ;
    rdfs:label "Authorize Session" ;
    rdfs:subClassOf ocsf:IdentityAccessManagementEvent,
        [ a owl:Restriction ;
            owl:onProperty ocsf:activity_id ;
            owl:allValuesFrom ocsf:integer_t ],
        [ a owl:Restriction ;
            owl:onProperty ocsf:dst_endpoint ;
            owl:allValuesFrom ocsf:NetworkEndpoint ],
        [ a owl:Restriction ;
            owl:onProperty ocsf:group ;
            owl:allValuesFrom ocsf:Group ],
        [ a owl:Restriction ;
            owl:onProperty ocsf:privileges ;
            owl:allValuesFrom ocsf:string_t ],
        [ a owl:Restriction ;
            owl:onProperty ocsf:session ;
            owl:allValuesFrom ocsf:Session ],
        [ a owl:Restriction ;
            owl:onProperty ocsf:user ;
            owl:allValuesFrom ocsf:User ],
        [ a owl:Restriction ;
            owl:onProperty ocsf:user ;
            owl:someValuesFrom ocsf:User ] ;
    dcterms:description "Authorize Session events report privileges or groups assigned to a new user session, usually at login time." ;
    ocsf:associations "{\"session\":[\"user\"],\"user\":[\"session\"]}" ;
    ocsf:constraints "{\"just_one\":[\"privileges\",\"group\"]}" ;
    ocsf:extends "iam" ;
    ocsf:name "authorize_session" .

ocsf:AutonomousSystem a owl:Class ;
    rdfs:label "Autonomous System" ;
    rdfs:subClassOf ocsf:Object,
        [ a owl:Restriction ;
            owl:onProperty ocsf:name ;
            owl:allValuesFrom ocsf:string_t ],
        [ a owl:Restriction ;
            owl:onProperty ocsf:number ;
            owl:allValuesFrom ocsf:integer_t ] ;
    dcterms:description "An autonomous system (AS) is a collection of connected Internet Protocol (IP) routing prefixes under the control of one or more network operators on behalf of a single administrative entity or domain that presents a common, clearly defined routing policy to the internet." ;
    ocsf:constraints "{\"at_least_one\":[\"number\",\"name\"]}" ;
    ocsf:extends "object" ;
    ocsf:name "autonomous_system" .

ocsf:BaseEvent a owl:Class ;
    rdfs:label "Base Event" ;
    rdfs:subClassOf d3f:DigitalEventRecord,
        [ a owl:Restriction ;
            owl:onProperty ocsf:enrichments ;
            owl:allValuesFrom ocsf:Enrichment ],
        [ a owl:Restriction ;
            owl:onProperty ocsf:message ;
            owl:allValuesFrom ocsf:string_t ],
        [ a owl:Restriction ;
            owl:onProperty ocsf:metadata ;
            owl:allValuesFrom ocsf:Metadata ],
        [ a owl:Restriction ;
            owl:onProperty ocsf:metadata ;
            owl:someValuesFrom ocsf:Metadata ],
        [ a owl:Restriction ;
            owl:onProperty ocsf:observables ;
            owl:allValuesFrom ocsf:Observable ],
        [ a owl:Restriction ;
            owl:onProperty ocsf:raw_data ;
            owl:allValuesFrom ocsf:string_t ],
        [ a owl:Restriction ;
            owl:onProperty ocsf:severity ;
            owl:allValuesFrom ocsf:string_t ],
        [ a owl:Restriction ;
            owl:onProperty ocsf:severity_id ;
            owl:allValuesFrom ocsf:integer_t ],
        [ a owl:Restriction ;
            owl:onProperty ocsf:severity_id ;
            owl:cardinality 1 ],
        [ a owl:Restriction ;
            owl:onProperty ocsf:status ;
            owl:allValuesFrom ocsf:string_t ],
        [ a owl:Restriction ;
            owl:onProperty ocsf:status_code ;
            owl:allValuesFrom ocsf:string_t ],
        [ a owl:Restriction ;
            owl:onProperty ocsf:status_detail ;
            owl:allValuesFrom ocsf:string_t ],
        [ a owl:Restriction ;
            owl:onProperty ocsf:status_id ;
            owl:allValuesFrom ocsf:integer_t ],
        [ a owl:Restriction ;
            owl:onProperty ocsf:unmapped ;
            owl:allValuesFrom ocsf:Object ] ;
    dcterms:description "The base event is a generic and concrete event. It also defines a set of attributes available in most event classes. As a generic event that does not belong to any event category, it could be used to log events that are not otherwise defined by the schema." ;
    ocsf:category ocsf:OtherEventCategory ;
    ocsf:name "base_event" ;
    ocsf:profiles "cloud",
        "datetime",
        "osint" .

ocsf:CISBenchmark a owl:Class ;
    rdfs:label "CIS Benchmark" ;
    rdfs:subClassOf ocsf:Object,
        [ a owl:Restriction ;
            owl:onProperty ocsf:cis_controls ;
            owl:allValuesFrom ocsf:CISControl ],
        [ a owl:Restriction ;
            owl:onProperty ocsf:desc ;
            owl:allValuesFrom ocsf:string_t ],
        [ a owl:Restriction ;
            owl:onProperty ocsf:name ;
            owl:allValuesFrom ocsf:string_t ],
        [ a owl:Restriction ;
            owl:onProperty ocsf:name ;
            owl:cardinality 1 ] ;
    dcterms:description "The CIS Benchmark object describes best practices for securely configuring IT systems, software, networks, and cloud infrastructure as defined by the <a target='_blank' href='https://www.cisecurity.org/cis-benchmarks/'>Center for Internet Security</a>. See also <a target='_blank' href='https://www.cisecurity.org/insights/blog/getting-to-know-the-cis-benchmarks'>Getting to Know the CIS Benchmarks</a>." ;
    ocsf:extends "object" ;
    ocsf:name "cis_benchmark" .

ocsf:CISBenchmarkResult a owl:Class ;
    rdfs:label "CIS Benchmark Result" ;
    rdfs:subClassOf ocsf:Object,
        [ a owl:Restriction ;
            owl:onProperty ocsf:desc ;
            owl:allValuesFrom ocsf:string_t ],
        [ a owl:Restriction ;
            owl:onProperty ocsf:name ;
            owl:allValuesFrom ocsf:string_t ],
        [ a owl:Restriction ;
            owl:onProperty ocsf:name ;
            owl:cardinality 1 ],
        [ a owl:Restriction ;
            owl:onProperty ocsf:remediation ;
            owl:allValuesFrom ocsf:Remediation ],
        [ a owl:Restriction ;
            owl:onProperty ocsf:rule ;
            owl:allValuesFrom ocsf:Rule ] ;
    dcterms:description "The CIS Benchmark Result object contains information as defined by the Center for Internet Security (<a target='_blank' href='https://www.cisecurity.org/cis-benchmarks/'>CIS</a>) benchmark result. CIS Benchmarks are a collection of best practices for securely configuring IT systems, software, networks, and cloud infrastructure." ;
    ocsf:extends "object" ;
    ocsf:name "cis_benchmark_result" .

ocsf:CISControl a owl:Class ;
    rdfs:label "CIS Control" ;
    rdfs:subClassOf ocsf:Object,
        [ a owl:Restriction ;
            owl:onProperty ocsf:desc ;
            owl:allValuesFrom ocsf:string_t ],
        [ a owl:Restriction ;
            owl:onProperty ocsf:name ;
            owl:allValuesFrom ocsf:string_t ],
        [ a owl:Restriction ;
            owl:onProperty ocsf:name ;
            owl:cardinality 1 ],
        [ a owl:Restriction ;
            owl:onProperty ocsf:version ;
            owl:allValuesFrom ocsf:string_t ] ;
    dcterms:description "The CIS Control (aka Critical Security Control) object describes a prioritized set of actions to protect your organization and data from cyber-attack vectors. The <a target='_blank' href='https://www.cisecurity.org/controls'>CIS Controls</a> are defined by the Center for Internet Security." ;
    ocsf:extends "object" ;
    ocsf:name "cis_control" .

ocsf:CISCSC a owl:Class ;
    rdfs:label "CIS CSC" ;
    rdfs:subClassOf ocsf:Object,
        [ a owl:Restriction ;
            owl:onProperty ocsf:control ;
            owl:allValuesFrom ocsf:string_t ],
        [ a owl:Restriction ;
            owl:onProperty ocsf:control ;
            owl:cardinality 1 ],
        [ a owl:Restriction ;
            owl:onProperty ocsf:version ;
            owl:allValuesFrom ocsf:string_t ] ;
    dcterms:description "The CIS Critical Security Control (CSC) contains information as defined by the Center for Internet Security Critical Security Control <a target='_blank' href='https://www.cisecurity.org/controls'>(CIS CSC)</a>. Prioritized set of actions to protect your organization and data from cyber-attack vectors." ;
    ocsf:extends "object" ;
    ocsf:name "cis_csc" .

ocsf:Cloud a owl:Class ;
    rdfs:label "Cloud" ;
    rdfs:subClassOf ocsf:Object,
        [ a owl:Restriction ;
            owl:onProperty ocsf:account ;
            owl:allValuesFrom ocsf:Account ],
        [ a owl:Restriction ;
            owl:onProperty ocsf:org ;
            owl:allValuesFrom ocsf:Organization ],
        [ a owl:Restriction ;
            owl:onProperty ocsf:project_uid ;
            owl:allValuesFrom ocsf:string_t ],
        [ a owl:Restriction ;
            owl:onProperty ocsf:provider ;
            owl:allValuesFrom ocsf:string_t ],
        [ a owl:Restriction ;
            owl:onProperty ocsf:provider ;
            owl:cardinality 1 ],
        [ a owl:Restriction ;
            owl:onProperty ocsf:region ;
            owl:allValuesFrom ocsf:string_t ],
        [ a owl:Restriction ;
            owl:onProperty ocsf:zone ;
            owl:allValuesFrom ocsf:string_t ] ;
    dcterms:description "The Cloud object contains information about a cloud account such as AWS Account ID, regions, etc." ;
    ocsf:extends "object" ;
    ocsf:name "cloud" .

ocsf:Compliance a owl:Class ;
    rdfs:label "Compliance" ;
    rdfs:subClassOf ocsf:Object,
        [ a owl:Restriction ;
            owl:onProperty ocsf:compliance_references ;
            owl:allValuesFrom ocsf:KBArticle ],
        [ a owl:Restriction ;
            owl:onProperty ocsf:compliance_standards ;
            owl:allValuesFrom ocsf:KBArticle ],
        [ a owl:Restriction ;
            owl:onProperty ocsf:control ;
            owl:allValuesFrom ocsf:string_t ],
        [ a owl:Restriction ;
            owl:onProperty ocsf:requirements ;
            owl:allValuesFrom ocsf:string_t ],
        [ a owl:Restriction ;
            owl:onProperty ocsf:standards ;
            owl:allValuesFrom ocsf:string_t ],
        [ a owl:Restriction ;
            owl:onProperty ocsf:standards ;
            owl:cardinality 1 ],
        [ a owl:Restriction ;
            owl:onProperty ocsf:status ;
            owl:allValuesFrom ocsf:string_t ],
        [ a owl:Restriction ;
            owl:onProperty ocsf:status_code ;
            owl:allValuesFrom ocsf:string_t ],
        [ a owl:Restriction ;
            owl:onProperty ocsf:status_detail ;
            owl:allValuesFrom ocsf:string_t ],
        [ a owl:Restriction ;
            owl:onProperty ocsf:status_id ;
            owl:allValuesFrom ocsf:integer_t ] ;
    dcterms:description "The Compliance object contains information about Industry and Regulatory Framework standards, controls and requirements." ;
    ocsf:extends "object" ;
    ocsf:name "compliance" .

ocsf:ComplianceFindingEvent a owl:Class ;
    rdfs:label "Compliance Finding" ;
    rdfs:subClassOf ocsf:Finding,
        ocsf:FindingEvent,
        [ a owl:Restriction ;
            owl:onProperty ocsf:compliance ;
            owl:allValuesFrom ocsf:Compliance ],
        [ a owl:Restriction ;
            owl:onProperty ocsf:compliance ;
            owl:someValuesFrom ocsf:Compliance ],
        [ a owl:Restriction ;
            owl:onProperty ocsf:remediation ;
            owl:allValuesFrom ocsf:Remediation ],
        [ a owl:Restriction ;
            owl:onProperty ocsf:resource ;
            owl:allValuesFrom ocsf:ResourceDetails ],
        [ a owl:Restriction ;
            owl:onProperty ocsf:resources ;
            owl:allValuesFrom ocsf:ResourceDetails ] ;
    dcterms:description "Compliance Finding events describe results of evaluations performed against resources, to check compliance with various Industry Frameworks or Security Standards such as <code>NIST SP 800-53, CIS AWS Foundations Benchmark v1.4.0, ISO/IEC 27001</code> etc." ;
    ocsf:extends "finding" ;
    ocsf:name "compliance_finding" .

ocsf:Container a owl:Class ;
    rdfs:label "Container" ;
    rdfs:subClassOf ocsf:Object,
        [ a owl:Restriction ;
            owl:onProperty ocsf:hash ;
            owl:allValuesFrom ocsf:Fingerprint ],
        [ a owl:Restriction ;
            owl:onProperty ocsf:image ;
            owl:allValuesFrom ocsf:Image ],
        [ a owl:Restriction ;
            owl:onProperty ocsf:name ;
            owl:allValuesFrom ocsf:string_t ],
        [ a owl:Restriction ;
            owl:onProperty ocsf:network_driver ;
            owl:allValuesFrom ocsf:string_t ],
        [ a owl:Restriction ;
            owl:onProperty ocsf:orchestrator ;
            owl:allValuesFrom ocsf:string_t ],
        [ a owl:Restriction ;
            owl:onProperty ocsf:pod_uuid ;
            owl:allValuesFrom ocsf:uuid_t ],
        [ a owl:Restriction ;
            owl:onProperty ocsf:runtime ;
            owl:allValuesFrom ocsf:string_t ],
        [ a owl:Restriction ;
            owl:onProperty ocsf:size ;
            owl:allValuesFrom ocsf:long_t ],
        [ a owl:Restriction ;
            owl:onProperty ocsf:tag ;
            owl:allValuesFrom ocsf:string_t ],
        [ a owl:Restriction ;
            owl:onProperty ocsf:uid ;
            owl:allValuesFrom ocsf:string_t ] ;
    dcterms:description "The Container object describes an instance of a specific container. A container is a prepackaged, portable system image that runs isolated on an existing system using a container runtime like containerd." ;
    ocsf:constraints "{\"at_least_one\":[\"uid\",\"name\"]}" ;
    ocsf:extends "object" ;
    ocsf:name "container" .

ocsf:CVE a owl:Class ;
    rdfs:label "CVE" ;
    rdfs:subClassOf ocsf:Object,
        [ a owl:Restriction ;
            owl:onProperty ocsf:created_time ;
            owl:allValuesFrom ocsf:timestamp_t ],
        [ a owl:Restriction ;
            owl:onProperty ocsf:cvss ;
            owl:allValuesFrom ocsf:CVSSScore ],
        [ a owl:Restriction ;
            owl:onProperty ocsf:cwe ;
            owl:allValuesFrom ocsf:CWE ],
        [ a owl:Restriction ;
            owl:onProperty ocsf:cwe_uid ;
            owl:allValuesFrom ocsf:string_t ],
        [ a owl:Restriction ;
            owl:onProperty ocsf:cwe_url ;
            owl:allValuesFrom ocsf:url_t ],
        [ a owl:Restriction ;
            owl:onProperty ocsf:desc ;
            owl:allValuesFrom ocsf:string_t ],
        [ a owl:Restriction ;
            owl:onProperty ocsf:epss ;
            owl:allValuesFrom ocsf:EPSS ],
        [ a owl:Restriction ;
            owl:onProperty ocsf:modified_time ;
            owl:allValuesFrom ocsf:timestamp_t ],
        [ a owl:Restriction ;
            owl:onProperty ocsf:product ;
            owl:allValuesFrom ocsf:Product ],
        [ a owl:Restriction ;
            owl:onProperty ocsf:references ;
            owl:allValuesFrom ocsf:string_t ],
        [ a owl:Restriction ;
            owl:onProperty ocsf:title ;
            owl:allValuesFrom ocsf:string_t ],
        [ a owl:Restriction ;
            owl:onProperty ocsf:type ;
            owl:allValuesFrom ocsf:string_t ],
        [ a owl:Restriction ;
            owl:onProperty ocsf:uid ;
            owl:allValuesFrom ocsf:string_t ],
        [ a owl:Restriction ;
            owl:onProperty ocsf:uid ;
            owl:cardinality 1 ] ;
    dcterms:description "The Common Vulnerabilities and Exposures (CVE) object represents publicly disclosed cybersecurity vulnerabilities defined in CVE Program catalog (<a target='_blank' href='https://cve.mitre.org/'>CVE</a>). There is one CVE Record for each vulnerability in the catalog." ;
    ocsf:extends "object" ;
    ocsf:name "cve" .

ocsf:CVSSScore a owl:Class ;
    rdfs:label "CVSS Score" ;
    rdfs:subClassOf ocsf:Object,
        [ a owl:Restriction ;
            owl:onProperty ocsf:base_score ;
            owl:allValuesFrom ocsf:float_t ],
        [ a owl:Restriction ;
            owl:onProperty ocsf:base_score ;
            owl:cardinality 1 ],
        [ a owl:Restriction ;
            owl:onProperty ocsf:depth ;
            owl:allValuesFrom ocsf:string_t ],
        [ a owl:Restriction ;
            owl:onProperty ocsf:metrics ;
            owl:allValuesFrom ocsf:Metric ],
        [ a owl:Restriction ;
            owl:onProperty ocsf:overall_score ;
            owl:allValuesFrom ocsf:float_t ],
        [ a owl:Restriction ;
            owl:onProperty ocsf:severity ;
            owl:allValuesFrom ocsf:string_t ],
        [ a owl:Restriction ;
            owl:onProperty ocsf:vector_string ;
            owl:allValuesFrom ocsf:string_t ],
        [ a owl:Restriction ;
            owl:onProperty ocsf:version ;
            owl:allValuesFrom ocsf:string_t ],
        [ a owl:Restriction ;
            owl:onProperty ocsf:version ;
            owl:cardinality 1 ] ;
    dcterms:description "The Common Vulnerability Scoring System (<a target='_blank' href='https://www.first.org/cvss/'>CVSS</a>) object provides a way to capture the principal characteristics of a vulnerability and produce a numerical score reflecting its severity." ;
    ocsf:extends "object" ;
    ocsf:name "cvss" .

ocsf:CWE a owl:Class ;
    rdfs:label "CWE" ;
    rdfs:subClassOf ocsf:Object,
        [ a owl:Restriction ;
            owl:onProperty ocsf:caption ;
            owl:allValuesFrom ocsf:string_t ],
        [ a owl:Restriction ;
            owl:onProperty ocsf:src_url ;
            owl:allValuesFrom ocsf:url_t ],
        [ a owl:Restriction ;
            owl:onProperty ocsf:uid ;
            owl:allValuesFrom ocsf:string_t ],
        [ a owl:Restriction ;
            owl:onProperty ocsf:uid ;
            owl:cardinality 1 ] ;
    dcterms:description "The CWE object represents a weakness in a software system that can be exploited by a threat actor to perform an attack. The CWE object is based on the <a target='_blank' href='https://cwe.mitre.org/'>Common Weakness Enumeration (CWE)</a> catalog." ;
    ocsf:extends "object" ;
    ocsf:name "cwe" .

ocsf:Database a owl:Class ;
    rdfs:label "Database" ;
    rdfs:subClassOf ocsf:Entity,
        [ a owl:Restriction ;
            owl:onProperty ocsf:created_time ;
            owl:allValuesFrom ocsf:timestamp_t ],
        [ a owl:Restriction ;
            owl:onProperty ocsf:desc ;
            owl:allValuesFrom ocsf:string_t ],
        [ a owl:Restriction ;
            owl:onProperty ocsf:groups ;
            owl:allValuesFrom ocsf:Group ],
        [ a owl:Restriction ;
            owl:onProperty ocsf:modified_time ;
            owl:allValuesFrom ocsf:timestamp_t ],
        [ a owl:Restriction ;
            owl:onProperty ocsf:name ;
            owl:allValuesFrom ocsf:string_t ],
        [ a owl:Restriction ;
            owl:onProperty ocsf:size ;
            owl:allValuesFrom ocsf:long_t ],
        [ a owl:Restriction ;
            owl:onProperty ocsf:type ;
            owl:allValuesFrom ocsf:string_t ],
        [ a owl:Restriction ;
            owl:onProperty ocsf:type_id ;
            owl:allValuesFrom ocsf:integer_t ],
        [ a owl:Restriction ;
            owl:onProperty ocsf:type_id ;
            owl:cardinality 1 ],
        [ a owl:Restriction ;
            owl:onProperty ocsf:uid ;
            owl:allValuesFrom ocsf:string_t ] ;
    dcterms:description "The database object is used for databases which are typically datastore services that contain an organized collection of structured and unstructured data or a types of data." ;
    ocsf:extends "_entity" ;
    ocsf:name "database" ;
    ocsf:profiles "data_classification" .

ocsf:Databucket a owl:Class ;
    rdfs:label "Databucket" ;
    rdfs:subClassOf ocsf:Entity,
        [ a owl:Restriction ;
            owl:onProperty ocsf:created_time ;
            owl:allValuesFrom ocsf:timestamp_t ],
        [ a owl:Restriction ;
            owl:onProperty ocsf:desc ;
            owl:allValuesFrom ocsf:string_t ],
        [ a owl:Restriction ;
            owl:onProperty ocsf:file ;
            owl:allValuesFrom ocsf:File ],
        [ a owl:Restriction ;
            owl:onProperty ocsf:groups ;
            owl:allValuesFrom ocsf:Group ],
        [ a owl:Restriction ;
            owl:onProperty ocsf:modified_time ;
            owl:allValuesFrom ocsf:timestamp_t ],
        [ a owl:Restriction ;
            owl:onProperty ocsf:name ;
            owl:allValuesFrom ocsf:string_t ],
        [ a owl:Restriction ;
            owl:onProperty ocsf:size ;
            owl:allValuesFrom ocsf:long_t ],
        [ a owl:Restriction ;
            owl:onProperty ocsf:type ;
            owl:allValuesFrom ocsf:string_t ],
        [ a owl:Restriction ;
            owl:onProperty ocsf:type_id ;
            owl:allValuesFrom ocsf:integer_t ],
        [ a owl:Restriction ;
            owl:onProperty ocsf:type_id ;
            owl:cardinality 1 ],
        [ a owl:Restriction ;
            owl:onProperty ocsf:uid ;
            owl:allValuesFrom ocsf:string_t ] ;
    dcterms:description "The databucket object is a basic container that holds data, typically organized through the use of data partitions." ;
    ocsf:extends "_entity" ;
    ocsf:name "databucket" ;
    ocsf:profiles "data_classification" .

ocsf:DataClassification a owl:Class ;
    rdfs:label "Data Classification" ;
    rdfs:subClassOf ocsf:Object,
        [ a owl:Restriction ;
            owl:onProperty ocsf:category ;
            owl:allValuesFrom ocsf:string_t ],
        [ a owl:Restriction ;
            owl:onProperty ocsf:category_id ;
            owl:allValuesFrom ocsf:integer_t ],
        [ a owl:Restriction ;
            owl:onProperty ocsf:confidentiality ;
            owl:allValuesFrom ocsf:string_t ],
        [ a owl:Restriction ;
            owl:onProperty ocsf:confidentiality_id ;
            owl:allValuesFrom ocsf:integer_t ],
        [ a owl:Restriction ;
            owl:onProperty ocsf:policy ;
            owl:allValuesFrom ocsf:Policy ] ;
    dcterms:description "The Data Classification object includes information about data classification levels and data category types." ;
    ocsf:constraints "{\"at_least_one\":[\"category_id\",\"confidentiality_id\"]}" ;
    ocsf:extends "object" ;
    ocsf:name "data_classification" .

ocsf:DataSecurityFindingEvent a owl:Class ;
    rdfs:label "Data Security Finding" ;
    rdfs:subClassOf ocsf:Finding,
        ocsf:FindingEvent,
        [ a owl:Restriction ;
            owl:onProperty ocsf:activity_id ;
            owl:allValuesFrom ocsf:integer_t ],
        [ a owl:Restriction ;
            owl:onProperty ocsf:activity_id ;
            owl:cardinality 1 ],
        [ a owl:Restriction ;
            owl:onProperty ocsf:activity_name ;
            owl:allValuesFrom ocsf:string_t ],
        [ a owl:Restriction ;
            owl:onProperty ocsf:actor ;
            owl:allValuesFrom ocsf:Actor ],
        [ a owl:Restriction ;
            owl:onProperty ocsf:database ;
            owl:allValuesFrom ocsf:Database ],
        [ a owl:Restriction ;
            owl:onProperty ocsf:databucket ;
            owl:allValuesFrom ocsf:Databucket ],
        [ a owl:Restriction ;
            owl:onProperty ocsf:device ;
            owl:allValuesFrom ocsf:Device ],
        [ a owl:Restriction ;
            owl:onProperty ocsf:dst_endpoint ;
            owl:allValuesFrom ocsf:NetworkEndpoint ],
        [ a owl:Restriction ;
            owl:onProperty ocsf:file ;
            owl:allValuesFrom ocsf:File ],
        [ a owl:Restriction ;
            owl:onProperty ocsf:impact ;
            owl:allValuesFrom ocsf:string_t ],
        [ a owl:Restriction ;
            owl:onProperty ocsf:impact_id ;
            owl:allValuesFrom ocsf:integer_t ],
        [ a owl:Restriction ;
            owl:onProperty ocsf:impact_score ;
            owl:allValuesFrom ocsf:integer_t ],
        [ a owl:Restriction ;
            owl:onProperty ocsf:resources ;
            owl:allValuesFrom ocsf:ResourceDetails ],
        [ a owl:Restriction ;
            owl:onProperty ocsf:risk_level ;
            owl:allValuesFrom ocsf:string_t ],
        [ a owl:Restriction ;
            owl:onProperty ocsf:risk_level_id ;
            owl:allValuesFrom ocsf:integer_t ],
        [ a owl:Restriction ;
            owl:onProperty ocsf:risk_score ;
            owl:allValuesFrom ocsf:integer_t ],
        [ a owl:Restriction ;
            owl:onProperty ocsf:src_endpoint ;
            owl:allValuesFrom ocsf:NetworkEndpoint ],
        [ a owl:Restriction ;
            owl:onProperty ocsf:table ;
            owl:allValuesFrom ocsf:Table ] ;
    dcterms:description "A Data Security Finding describes detections or alerts generated by various data security products such as Data Loss Prevention (DLP), Data Classification, Secrets Management, Digital Rights Management (DRM), Data Security Posture Management (DSPM), and similar tools. These detections or alerts can be created using fingerprinting, statistical analysis, machine learning or other methodologies. The finding describes the actors and endpoints who accessed or own the sensitive data, as well as the resources which store the sensitive data." ;
    ocsf:extends "finding" ;
    ocsf:name "data_security_finding" ;
    ocsf:profiles "security_control" .

ocsf:DatastoreActivityEvent a owl:Class ;
    rdfs:label "Datastore Activity" ;
    rdfs:subClassOf ocsf:ApplicationActivityEvent,
        [ a owl:Restriction ;
            owl:onProperty ocsf:activity_id ;
            owl:allValuesFrom ocsf:integer_t ],
        [ a owl:Restriction ;
            owl:onProperty ocsf:actor ;
            owl:allValuesFrom ocsf:Actor ],
        [ a owl:Restriction ;
            owl:onProperty ocsf:actor ;
            owl:someValuesFrom ocsf:Actor ],
        [ a owl:Restriction ;
            owl:onProperty ocsf:database ;
            owl:allValuesFrom ocsf:Database ],
        [ a owl:Restriction ;
            owl:onProperty ocsf:databucket ;
            owl:allValuesFrom ocsf:Databucket ],
        [ a owl:Restriction ;
            owl:onProperty ocsf:dst_endpoint ;
            owl:allValuesFrom ocsf:NetworkEndpoint ],
        [ a owl:Restriction ;
            owl:onProperty ocsf:http_request ;
            owl:allValuesFrom ocsf:HTTPRequest ],
        [ a owl:Restriction ;
            owl:onProperty ocsf:query_info ;
            owl:allValuesFrom ocsf:QueryInformation ],
        [ a owl:Restriction ;
            owl:onProperty ocsf:src_endpoint ;
            owl:allValuesFrom ocsf:NetworkEndpoint ],
        [ a owl:Restriction ;
            owl:onProperty ocsf:src_endpoint ;
            owl:someValuesFrom ocsf:NetworkEndpoint ],
        [ a owl:Restriction ;
            owl:onProperty ocsf:table ;
            owl:allValuesFrom ocsf:Table ],
        [ a owl:Restriction ;
            owl:onProperty ocsf:type ;
            owl:allValuesFrom ocsf:string_t ],
        [ a owl:Restriction ;
            owl:onProperty ocsf:type_id ;
            owl:allValuesFrom ocsf:integer_t ] ;
    dcterms:description "Datastore events describe general activities (Read, Update, Query, Delete, etc.) which affect datastores or data within those datastores, e.g. (AWS RDS, AWS S3)." ;
    ocsf:constraints "{\"at_least_one\":[\"database\",\"databucket\",\"table\"]}" ;
    ocsf:extends "application" ;
    ocsf:name "datastore_activity" ;
    ocsf:profiles "security_control" .

ocsf:DCERPC a owl:Class ;
    rdfs:label "DCE/RPC" ;
    rdfs:subClassOf ocsf:Object,
        [ a owl:Restriction ;
            owl:onProperty ocsf:command ;
            owl:allValuesFrom ocsf:string_t ],
        [ a owl:Restriction ;
            owl:onProperty ocsf:command_response ;
            owl:allValuesFrom ocsf:string_t ],
        [ a owl:Restriction ;
            owl:onProperty ocsf:flags ;
            owl:allValuesFrom ocsf:string_t ],
        [ a owl:Restriction ;
            owl:onProperty ocsf:flags ;
            owl:cardinality 1 ],
        [ a owl:Restriction ;
            owl:onProperty ocsf:opnum ;
            owl:allValuesFrom ocsf:integer_t ],
        [ a owl:Restriction ;
            owl:onProperty ocsf:rpc_interface ;
            owl:allValuesFrom ocsf:RPCInterface ],
        [ a owl:Restriction ;
            owl:onProperty ocsf:rpc_interface ;
            owl:someValuesFrom ocsf:RPCInterface ] ;
    dcterms:description "The DCE/RPC, or Distributed Computing Environment/Remote Procedure Call, object describes the remote procedure call system for distributed computing environments. Defined by D3FEND <a target='_blank' href='https://d3fend.mitre.org/dao/artifact/d3f:RemoteProcedureCall/'>d3f:RemoteProcedureCall</a>." ;
    ocsf:extends "object" ;
    ocsf:name "dce_rpc" .

ocsf:DetectionFindingEvent a owl:Class ;
    rdfs:label "Detection Finding" ;
    rdfs:subClassOf ocsf:Finding,
        ocsf:FindingEvent,
        [ a owl:Restriction ;
            owl:onProperty ocsf:evidences ;
            owl:allValuesFrom ocsf:EvidenceArtifacts ],
        [ a owl:Restriction ;
            owl:onProperty ocsf:impact ;
            owl:allValuesFrom ocsf:string_t ],
        [ a owl:Restriction ;
            owl:onProperty ocsf:impact_id ;
            owl:allValuesFrom ocsf:integer_t ],
        [ a owl:Restriction ;
            owl:onProperty ocsf:impact_score ;
            owl:allValuesFrom ocsf:integer_t ],
        [ a owl:Restriction ;
            owl:onProperty ocsf:remediation ;
            owl:allValuesFrom ocsf:Remediation ],
        [ a owl:Restriction ;
            owl:onProperty ocsf:resources ;
            owl:allValuesFrom ocsf:ResourceDetails ],
        [ a owl:Restriction ;
            owl:onProperty ocsf:risk_details ;
            owl:allValuesFrom ocsf:string_t ],
        [ a owl:Restriction ;
            owl:onProperty ocsf:risk_level ;
            owl:allValuesFrom ocsf:string_t ],
        [ a owl:Restriction ;
            owl:onProperty ocsf:risk_level_id ;
            owl:allValuesFrom ocsf:integer_t ],
        [ a owl:Restriction ;
            owl:onProperty ocsf:risk_score ;
            owl:allValuesFrom ocsf:integer_t ],
        [ a owl:Restriction ;
            owl:onProperty ocsf:vulnerabilities ;
            owl:allValuesFrom ocsf:VulnerabilityDetails ] ;
    dcterms:description "A Detection Finding describes detections or alerts generated by security products using correlation engines, detection engines or other methodologies. Note: if the product is a security control, the <code>security_control</code> profile should be applied and its <code>attacks</code> information should be duplicated into the <code>finding_info</code> object." ;
    ocsf:extends "finding" ;
    ocsf:name "detection_finding" ;
    ocsf:profiles "security_control" .

ocsf:Device a owl:Class ;
    rdfs:label "Device" ;
    rdfs:subClassOf ocsf:Endpoint,
        [ a owl:Restriction ;
            owl:onProperty ocsf:autoscale_uid ;
            owl:allValuesFrom ocsf:string_t ],
        [ a owl:Restriction ;
            owl:onProperty ocsf:boot_time ;
            owl:allValuesFrom ocsf:timestamp_t ],
        [ a owl:Restriction ;
            owl:onProperty ocsf:created_time ;
            owl:allValuesFrom ocsf:timestamp_t ],
        [ a owl:Restriction ;
            owl:onProperty ocsf:desc ;
            owl:allValuesFrom ocsf:string_t ],
        [ a owl:Restriction ;
            owl:onProperty ocsf:domain ;
            owl:allValuesFrom ocsf:string_t ],
        [ a owl:Restriction ;
            owl:onProperty ocsf:first_seen_time ;
            owl:allValuesFrom ocsf:timestamp_t ],
        [ a owl:Restriction ;
            owl:onProperty ocsf:groups ;
            owl:allValuesFrom ocsf:Group ],
        [ a owl:Restriction ;
            owl:onProperty ocsf:hostname ;
            owl:allValuesFrom ocsf:hostname_t ],
        [ a owl:Restriction ;
            owl:onProperty ocsf:hypervisor ;
            owl:allValuesFrom ocsf:string_t ],
        [ a owl:Restriction ;
            owl:onProperty ocsf:image ;
            owl:allValuesFrom ocsf:Image ],
        [ a owl:Restriction ;
            owl:onProperty ocsf:imei ;
            owl:allValuesFrom ocsf:string_t ],
        [ a owl:Restriction ;
            owl:onProperty ocsf:ip ;
            owl:allValuesFrom ocsf:ip_t ],
        [ a owl:Restriction ;
            owl:onProperty ocsf:is_compliant ;
            owl:allValuesFrom ocsf:boolean_t ],
        [ a owl:Restriction ;
            owl:onProperty ocsf:is_managed ;
            owl:allValuesFrom ocsf:boolean_t ],
        [ a owl:Restriction ;
            owl:onProperty ocsf:is_personal ;
            owl:allValuesFrom ocsf:boolean_t ],
        [ a owl:Restriction ;
            owl:onProperty ocsf:is_trusted ;
            owl:allValuesFrom ocsf:boolean_t ],
        [ a owl:Restriction ;
            owl:onProperty ocsf:last_seen_time ;
            owl:allValuesFrom ocsf:timestamp_t ],
        [ a owl:Restriction ;
            owl:onProperty ocsf:location ;
            owl:allValuesFrom ocsf:GeoLocation ],
        [ a owl:Restriction ;
            owl:onProperty ocsf:modified_time ;
            owl:allValuesFrom ocsf:timestamp_t ],
        [ a owl:Restriction ;
            owl:onProperty ocsf:name ;
            owl:allValuesFrom ocsf:string_t ],
        [ a owl:Restriction ;
            owl:onProperty ocsf:network_interfaces ;
            owl:allValuesFrom ocsf:NetworkInterface ],
        [ a owl:Restriction ;
            owl:onProperty ocsf:org ;
            owl:allValuesFrom ocsf:Organization ],
        [ a owl:Restriction ;
            owl:onProperty ocsf:region ;
            owl:allValuesFrom ocsf:string_t ],
        [ a owl:Restriction ;
            owl:onProperty ocsf:risk_level ;
            owl:allValuesFrom ocsf:string_t ],
        [ a owl:Restriction ;
            owl:onProperty ocsf:risk_level_id ;
            owl:allValuesFrom ocsf:integer_t ],
        [ a owl:Restriction ;
            owl:onProperty ocsf:risk_score ;
            owl:allValuesFrom ocsf:integer_t ],
        [ a owl:Restriction ;
            owl:onProperty ocsf:subnet ;
            owl:allValuesFrom ocsf:subnet_t ],
        [ a owl:Restriction ;
            owl:onProperty ocsf:type ;
            owl:allValuesFrom ocsf:string_t ],
        [ a owl:Restriction ;
            owl:onProperty ocsf:type_id ;
            owl:allValuesFrom ocsf:integer_t ],
        [ a owl:Restriction ;
            owl:onProperty ocsf:type_id ;
            owl:cardinality 1 ],
        [ a owl:Restriction ;
            owl:onProperty ocsf:uid ;
            owl:allValuesFrom ocsf:string_t ],
        [ a owl:Restriction ;
            owl:onProperty ocsf:uid_alt ;
            owl:allValuesFrom ocsf:string_t ] ;
    dcterms:description "The Device object represents an addressable computer system or host, which is typically connected to a computer network and participates in the transmission or processing of data within the computer network. Defined by D3FEND <a target='_blank' href='https://d3fend.mitre.org/dao/artifact/d3f:Host/'>d3f:Host</a>." ;
    ocsf:extends "endpoint" ;
    ocsf:name "device" .

ocsf:DeviceConfigStateChangeEvent a owl:Class ;
    rdfs:label "Device Config State Change" ;
    rdfs:subClassOf ocsf:DiscoveryEvent,
        [ a owl:Restriction ;
            owl:onProperty ocsf:actor ;
            owl:allValuesFrom ocsf:Actor ],
        [ a owl:Restriction ;
            owl:onProperty ocsf:device ;
            owl:allValuesFrom ocsf:Device ],
        [ a owl:Restriction ;
            owl:onProperty ocsf:device ;
            owl:someValuesFrom ocsf:Device ],
        [ a owl:Restriction ;
            owl:onProperty ocsf:prev_security_level ;
            owl:allValuesFrom ocsf:string_t ],
        [ a owl:Restriction ;
            owl:onProperty ocsf:prev_security_level_id ;
            owl:allValuesFrom ocsf:integer_t ],
        [ a owl:Restriction ;
            owl:onProperty ocsf:security_level ;
            owl:allValuesFrom ocsf:string_t ],
        [ a owl:Restriction ;
            owl:onProperty ocsf:security_level_id ;
            owl:allValuesFrom ocsf:integer_t ],
        [ a owl:Restriction ;
            owl:onProperty ocsf:state ;
            owl:allValuesFrom ocsf:string_t ],
        [ a owl:Restriction ;
            owl:onProperty ocsf:state_id ;
            owl:allValuesFrom ocsf:integer_t ] ;
    dcterms:description "Device Config State Change events report state changes that impact the security of the device." ;
    ocsf:extends "discovery" ;
    ocsf:name "device_config_state_change" ;
    ocsf:profiles "host" .

ocsf:DeviceConfigStateEvent a owl:Class ;
    rdfs:label "Device Config State" ;
    rdfs:subClassOf ocsf:DiscoveryEvent,
        [ a owl:Restriction ;
            owl:onProperty ocsf:actor ;
            owl:allValuesFrom ocsf:Actor ],
        [ a owl:Restriction ;
            owl:onProperty ocsf:cis_benchmark_result ;
            owl:allValuesFrom ocsf:CISBenchmarkResult ],
        [ a owl:Restriction ;
            owl:onProperty ocsf:device ;
            owl:allValuesFrom ocsf:Device ],
        [ a owl:Restriction ;
            owl:onProperty ocsf:device ;
            owl:someValuesFrom ocsf:Device ] ;
    dcterms:description "Device Config State events report device configuration data and CIS Benchmark results." ;
    ocsf:extends "discovery" ;
    ocsf:name "config_state" ;
    ocsf:profiles "host" .

ocsf:DeviceHardwareInfo a owl:Class ;
    rdfs:label "Device Hardware Info" ;
    rdfs:subClassOf ocsf:Object,
        [ a owl:Restriction ;
            owl:onProperty ocsf:bios_date ;
            owl:allValuesFrom ocsf:string_t ],
        [ a owl:Restriction ;
            owl:onProperty ocsf:bios_manufacturer ;
            owl:allValuesFrom ocsf:string_t ],
        [ a owl:Restriction ;
            owl:onProperty ocsf:bios_ver ;
            owl:allValuesFrom ocsf:string_t ],
        [ a owl:Restriction ;
            owl:onProperty ocsf:chassis ;
            owl:allValuesFrom ocsf:string_t ],
        [ a owl:Restriction ;
            owl:onProperty ocsf:cpu_bits ;
            owl:allValuesFrom ocsf:integer_t ],
        [ a owl:Restriction ;
            owl:onProperty ocsf:cpu_cores ;
            owl:allValuesFrom ocsf:integer_t ],
        [ a owl:Restriction ;
            owl:onProperty ocsf:cpu_count ;
            owl:allValuesFrom ocsf:integer_t ],
        [ a owl:Restriction ;
            owl:onProperty ocsf:cpu_speed ;
            owl:allValuesFrom ocsf:integer_t ],
        [ a owl:Restriction ;
            owl:onProperty ocsf:cpu_type ;
            owl:allValuesFrom ocsf:string_t ],
        [ a owl:Restriction ;
            owl:onProperty ocsf:desktop_display ;
            owl:allValuesFrom ocsf:Display ],
        [ a owl:Restriction ;
            owl:onProperty ocsf:keyboard_info ;
            owl:allValuesFrom ocsf:KeyboardInformation ],
        [ a owl:Restriction ;
            owl:onProperty ocsf:ram_size ;
            owl:allValuesFrom ocsf:integer_t ],
        [ a owl:Restriction ;
            owl:onProperty ocsf:serial_number ;
            owl:allValuesFrom ocsf:string_t ] ;
    dcterms:description "The Device Hardware Information object contains details and specifications of the physical components that make up a device. This information provides an overview of the hardware capabilities, configuration, and characteristics of the device." ;
    ocsf:extends "object" ;
    ocsf:name "device_hw_info" .

ocsf:DeviceInventoryInfoEvent a owl:Class ;
    rdfs:label "Device Inventory Info" ;
    rdfs:subClassOf ocsf:DiscoveryEvent,
        [ a owl:Restriction ;
            owl:onProperty ocsf:actor ;
            owl:allValuesFrom ocsf:Actor ],
        [ a owl:Restriction ;
            owl:onProperty ocsf:device ;
            owl:allValuesFrom ocsf:Device ],
        [ a owl:Restriction ;
            owl:onProperty ocsf:device ;
            owl:someValuesFrom ocsf:Device ] ;
    dcterms:description "Device Inventory Info events report device inventory data that is either logged or proactively collected. For example, when collecting device information from a CMDB or running a network sweep of connected devices." ;
    ocsf:extends "discovery" ;
    ocsf:name "inventory_info" ;
    ocsf:profiles "host" .

ocsf:DHCPActivityEvent a owl:Class ;
    rdfs:label "DHCP Activity" ;
    rdfs:subClassOf ocsf:NetworkEvent,
        [ a owl:Restriction ;
            owl:onProperty ocsf:activity_id ;
            owl:allValuesFrom ocsf:integer_t ],
        [ a owl:Restriction ;
            owl:onProperty ocsf:activity_id ;
            owl:cardinality 1 ],
        [ a owl:Restriction ;
            owl:onProperty ocsf:dst_endpoint ;
            owl:allValuesFrom ocsf:NetworkEndpoint ],
        [ a owl:Restriction ;
            owl:onProperty ocsf:is_renewal ;
            owl:allValuesFrom ocsf:boolean_t ],
        [ a owl:Restriction ;
            owl:onProperty ocsf:lease_dur ;
            owl:allValuesFrom ocsf:integer_t ],
        [ a owl:Restriction ;
            owl:onProperty ocsf:relay ;
            owl:allValuesFrom ocsf:NetworkInterface ],
        [ a owl:Restriction ;
            owl:onProperty ocsf:src_endpoint ;
            owl:allValuesFrom ocsf:NetworkEndpoint ],
        [ a owl:Restriction ;
            owl:onProperty ocsf:transaction_uid ;
            owl:allValuesFrom ocsf:string_t ] ;
    dcterms:description "DHCP Activity events report MAC to IP assignment via DHCP from a client or server." ;
    ocsf:category ocsf:NetworkEvent ;
    ocsf:extends "network" ;
    ocsf:name "dhcp_activity" ;
    ocsf:profiles "host" .

ocsf:DigitalCertificate a owl:Class ;
    rdfs:label "Digital Certificate" ;
    rdfs:subClassOf ocsf:Object,
        [ a owl:Restriction ;
            owl:onProperty ocsf:created_time ;
            owl:allValuesFrom ocsf:timestamp_t ],
        [ a owl:Restriction ;
            owl:onProperty ocsf:expiration_time ;
            owl:allValuesFrom ocsf:timestamp_t ],
        [ a owl:Restriction ;
            owl:onProperty ocsf:fingerprints ;
            owl:allValuesFrom ocsf:Fingerprint ],
        [ a owl:Restriction ;
            owl:onProperty ocsf:fingerprints ;
            owl:someValuesFrom ocsf:Fingerprint ],
        [ a owl:Restriction ;
            owl:onProperty ocsf:is_self_signed ;
            owl:allValuesFrom ocsf:boolean_t ],
        [ a owl:Restriction ;
            owl:onProperty ocsf:issuer ;
            owl:allValuesFrom ocsf:string_t ],
        [ a owl:Restriction ;
            owl:onProperty ocsf:issuer ;
            owl:cardinality 1 ],
        [ a owl:Restriction ;
            owl:onProperty ocsf:serial_number ;
            owl:allValuesFrom ocsf:string_t ],
        [ a owl:Restriction ;
            owl:onProperty ocsf:serial_number ;
            owl:cardinality 1 ],
        [ a owl:Restriction ;
            owl:onProperty ocsf:subject ;
            owl:allValuesFrom ocsf:string_t ],
        [ a owl:Restriction ;
            owl:onProperty ocsf:uid ;
            owl:allValuesFrom ocsf:string_t ],
        [ a owl:Restriction ;
            owl:onProperty ocsf:version ;
            owl:allValuesFrom ocsf:string_t ] ;
    dcterms:description "The Digital Certificate, also known as a Public Key Certificate, object contains information about the ownership and usage of a public key. It serves as a means to establish trust in the authenticity and integrity of the public key and the associated entity. Defined by D3FEND <a target='_blank' href='https://d3fend.mitre.org/dao/artifact/d3f:Certificate/'>d3f:Certificate</a>." ;
    ocsf:extends "object" ;
    ocsf:name "certificate" .

ocsf:DigitalSignature a owl:Class ;
    rdfs:label "Digital Signature" ;
    rdfs:subClassOf ocsf:Object,
        [ a owl:Restriction ;
            owl:onProperty ocsf:algorithm ;
            owl:allValuesFrom ocsf:string_t ],
        [ a owl:Restriction ;
            owl:onProperty ocsf:algorithm_id ;
            owl:allValuesFrom ocsf:integer_t ],
        [ a owl:Restriction ;
            owl:onProperty ocsf:algorithm_id ;
            owl:cardinality 1 ],
        [ a owl:Restriction ;
            owl:onProperty ocsf:certificate ;
            owl:allValuesFrom ocsf:DigitalCertificate ],
        [ a owl:Restriction ;
            owl:onProperty ocsf:created_time ;
            owl:allValuesFrom ocsf:timestamp_t ],
        [ a owl:Restriction ;
            owl:onProperty ocsf:developer_uid ;
            owl:allValuesFrom ocsf:string_t ],
        [ a owl:Restriction ;
            owl:onProperty ocsf:digest ;
            owl:allValuesFrom ocsf:Fingerprint ],
        [ a owl:Restriction ;
            owl:onProperty ocsf:state ;
            owl:allValuesFrom ocsf:string_t ],
        [ a owl:Restriction ;
            owl:onProperty ocsf:state_id ;
            owl:allValuesFrom ocsf:integer_t ] ;
    dcterms:description "The Digital Signature object contains information about the cryptographic mechanism used to verify the authenticity, integrity, and origin of the file or application." ;
    ocsf:extends "object" ;
    ocsf:name "digital_signature" .

ocsf:DiscoveryEvent a owl:Class ;
    rdfs:label "Discovery" ;
    rdfs:subClassOf ocsf:BaseEvent,
        [ a owl:Restriction ;
            owl:onProperty ocsf:activity_id ;
            owl:allValuesFrom ocsf:integer_t ] ;
    dcterms:description "The Discovery event is a generic event that defines a set of attributes available in Discovery category events. As a generic event, it could be used to log events that are not otherwise defined by the Discovery specific event classes." ;
    ocsf:category ocsf:DiscoveryEvent ;
    ocsf:extends "base_event" ;
    ocsf:name "discovery" .

ocsf:DiscoveryEventCategory a owl:Class ;
    rdfs:label "Discovery" ;
    rdfs:subClassOf ocsf:EventCategory ;
    d3f:definition "Discovery events report the existence and state of devices, files, configurations, processes, registry keys, and other objects." ;
    ocsf:category_name "discovery" .

ocsf:DiscoveryResultEvent a owl:Class ;
    rdfs:label "Discovery Result" ;
    rdfs:subClassOf ocsf:BaseEvent,
        [ a owl:Restriction ;
            owl:onProperty ocsf:activity_id ;
            owl:allValuesFrom ocsf:integer_t ],
        [ a owl:Restriction ;
            owl:onProperty ocsf:query_info ;
            owl:allValuesFrom ocsf:QueryInformation ],
        [ a owl:Restriction ;
            owl:onProperty ocsf:query_result ;
            owl:allValuesFrom ocsf:string_t ],
        [ a owl:Restriction ;
            owl:onProperty ocsf:query_result_id ;
            owl:allValuesFrom ocsf:integer_t ],
        [ a owl:Restriction ;
            owl:onProperty ocsf:query_result_id ;
            owl:cardinality 1 ] ;
    dcterms:description "Discovery Result events report the results of a discovery request." ;
    ocsf:category ocsf:DiscoveryEvent ;
    ocsf:extends "base_event" ;
    ocsf:name "discovery_result" ;
    ocsf:profiles "host" .

ocsf:Display a owl:Class ;
    rdfs:label "Display" ;
    rdfs:subClassOf ocsf:Object,
        [ a owl:Restriction ;
            owl:onProperty ocsf:color_depth ;
            owl:allValuesFrom ocsf:integer_t ],
        [ a owl:Restriction ;
            owl:onProperty ocsf:physical_height ;
            owl:allValuesFrom ocsf:integer_t ],
        [ a owl:Restriction ;
            owl:onProperty ocsf:physical_orientation ;
            owl:allValuesFrom ocsf:integer_t ],
        [ a owl:Restriction ;
            owl:onProperty ocsf:physical_width ;
            owl:allValuesFrom ocsf:integer_t ],
        [ a owl:Restriction ;
            owl:onProperty ocsf:scale_factor ;
            owl:allValuesFrom ocsf:integer_t ] ;
    dcterms:description "The Display object contains information about the physical or virtual display connected to a computer system." ;
    ocsf:extends "object" ;
    ocsf:name "display" .

ocsf:DNS a owl:Class ;
    rdfs:label "DNS" ;
    rdfs:subClassOf ocsf:Object,
        [ a owl:Restriction ;
            owl:onProperty ocsf:class ;
            owl:allValuesFrom ocsf:string_t ],
        [ a owl:Restriction ;
            owl:onProperty ocsf:packet_uid ;
            owl:allValuesFrom ocsf:integer_t ],
        [ a owl:Restriction ;
            owl:onProperty ocsf:type ;
            owl:allValuesFrom ocsf:string_t ] ;
    dcterms:description "The Domain Name System (DNS) object represents the shared information associated with the DNS query and answer objects." ;
    ocsf:extends "object" ;
    ocsf:name "_dns" .

ocsf:DNSActivityEvent a owl:Class ;
    rdfs:label "DNS Activity" ;
    rdfs:subClassOf ocsf:NetworkEvent,
        [ a owl:Restriction ;
            owl:onProperty ocsf:activity_id ;
            owl:allValuesFrom ocsf:integer_t ],
        [ a owl:Restriction ;
            owl:onProperty ocsf:answers ;
            owl:allValuesFrom ocsf:DNSAnswer ],
        [ a owl:Restriction ;
            owl:onProperty ocsf:connection_info ;
            owl:allValuesFrom ocsf:NetworkConnectionInformation ],
        [ a owl:Restriction ;
            owl:onProperty ocsf:dst_endpoint ;
            owl:allValuesFrom ocsf:NetworkEndpoint ],
        [ a owl:Restriction ;
            owl:onProperty ocsf:query ;
            owl:allValuesFrom ocsf:DNSQuery ],
        [ a owl:Restriction ;
            owl:onProperty ocsf:query_time ;
            owl:allValuesFrom ocsf:timestamp_t ],
        [ a owl:Restriction ;
            owl:onProperty ocsf:rcode ;
            owl:allValuesFrom ocsf:string_t ],
        [ a owl:Restriction ;
            owl:onProperty ocsf:rcode_id ;
            owl:allValuesFrom ocsf:integer_t ],
        [ a owl:Restriction ;
            owl:onProperty ocsf:response_time ;
            owl:allValuesFrom ocsf:timestamp_t ],
        [ a owl:Restriction ;
            owl:onProperty ocsf:traffic ;
            owl:allValuesFrom ocsf:NetworkTraffic ] ;
    dcterms:description "DNS Activity events report DNS queries and answers as seen on the network." ;
    ocsf:extends "network" ;
    ocsf:name "dns_activity" .

ocsf:DNSAnswer a owl:Class ;
    rdfs:label "DNS Answer" ;
    rdfs:subClassOf ocsf:DNS,
        [ a owl:Restriction ;
            owl:onProperty ocsf:class ;
            owl:allValuesFrom ocsf:string_t ],
        [ a owl:Restriction ;
            owl:onProperty ocsf:flag_ids ;
            owl:allValuesFrom ocsf:integer_t ],
        [ a owl:Restriction ;
            owl:onProperty ocsf:flags ;
            owl:allValuesFrom ocsf:string_t ],
        [ a owl:Restriction ;
            owl:onProperty ocsf:rdata ;
            owl:allValuesFrom ocsf:string_t ],
        [ a owl:Restriction ;
            owl:onProperty ocsf:rdata ;
            owl:cardinality 1 ],
        [ a owl:Restriction ;
            owl:onProperty ocsf:ttl ;
            owl:allValuesFrom ocsf:integer_t ],
        [ a owl:Restriction ;
            owl:onProperty ocsf:type ;
            owl:allValuesFrom ocsf:string_t ] ;
    dcterms:description "The DNS Answer object represents a specific response provided by the Domain Name System (DNS) when querying for information about a domain or performing a DNS operation. It encapsulates the relevant details and data returned by the DNS server in response to a query." ;
    ocsf:extends "_dns" ;
    ocsf:name "dns_answer" .

ocsf:DNSQuery a owl:Class ;
    rdfs:label "DNS Query" ;
    rdfs:subClassOf ocsf:DNS,
        [ a owl:Restriction ;
            owl:onProperty ocsf:hostname ;
            owl:allValuesFrom ocsf:hostname_t ],
        [ a owl:Restriction ;
            owl:onProperty ocsf:hostname ;
            owl:cardinality 1 ],
        [ a owl:Restriction ;
            owl:onProperty ocsf:opcode ;
            owl:allValuesFrom ocsf:string_t ],
        [ a owl:Restriction ;
            owl:onProperty ocsf:opcode_id ;
            owl:allValuesFrom ocsf:integer_t ] ;
    dcterms:description "The DNS query object represents a specific request made to the Domain Name System (DNS) to retrieve information about a domain or perform a DNS operation. This object encapsulates the necessary attributes and methods to construct and send DNS queries, specify the query type (e.g., A, AAAA, MX). Defined by D3FEND <a target='_blank' href='https://d3fend.mitre.org/dao/artifact/d3f:DNSLookup/'>d3f:DNSLookup</a>." ;
    ocsf:extends "_dns" ;
    ocsf:name "dns_query" .

ocsf:DomainContact a owl:Class ;
    rdfs:label "Domain Contact" ;
    rdfs:subClassOf ocsf:Object,
        [ a owl:Restriction ;
            owl:onProperty ocsf:email_addr ;
            owl:allValuesFrom ocsf:email_t ],
        [ a owl:Restriction ;
            owl:onProperty ocsf:location ;
            owl:allValuesFrom ocsf:GeoLocation ],
        [ a owl:Restriction ;
            owl:onProperty ocsf:name ;
            owl:allValuesFrom ocsf:string_t ],
        [ a owl:Restriction ;
            owl:onProperty ocsf:phone_number ;
            owl:allValuesFrom ocsf:string_t ],
        [ a owl:Restriction ;
            owl:onProperty ocsf:type ;
            owl:allValuesFrom ocsf:string_t ],
        [ a owl:Restriction ;
            owl:onProperty ocsf:type_id ;
            owl:allValuesFrom ocsf:integer_t ],
        [ a owl:Restriction ;
            owl:onProperty ocsf:type_id ;
            owl:cardinality 1 ],
        [ a owl:Restriction ;
            owl:onProperty ocsf:uid ;
            owl:allValuesFrom ocsf:string_t ] ;
    dcterms:description "The contact information related to a domain registration, e.g., registrant, administrator, abuse, billing, or technical contact." ;
    ocsf:extends "object" ;
    ocsf:name "domain_contact" .

ocsf:Email a owl:Class ;
    rdfs:label "Email" ;
    rdfs:subClassOf ocsf:Object,
        [ a owl:Restriction ;
            owl:onProperty ocsf:cc ;
            owl:allValuesFrom ocsf:email_t ],
        [ a owl:Restriction ;
            owl:onProperty ocsf:delivered_to ;
            owl:allValuesFrom ocsf:email_t ],
        [ a owl:Restriction ;
            owl:onProperty ocsf:from ;
            owl:allValuesFrom ocsf:email_t ],
        [ a owl:Restriction ;
            owl:onProperty ocsf:from ;
            owl:cardinality 1 ],
        [ a owl:Restriction ;
            owl:onProperty ocsf:message_uid ;
            owl:allValuesFrom ocsf:string_t ],
        [ a owl:Restriction ;
            owl:onProperty ocsf:raw_header ;
            owl:allValuesFrom ocsf:string_t ],
        [ a owl:Restriction ;
            owl:onProperty ocsf:reply_to ;
            owl:allValuesFrom ocsf:email_t ],
        [ a owl:Restriction ;
            owl:onProperty ocsf:size ;
            owl:allValuesFrom ocsf:long_t ],
        [ a owl:Restriction ;
            owl:onProperty ocsf:smtp_from ;
            owl:allValuesFrom ocsf:email_t ],
        [ a owl:Restriction ;
            owl:onProperty ocsf:smtp_to ;
            owl:allValuesFrom ocsf:email_t ],
        [ a owl:Restriction ;
            owl:onProperty ocsf:subject ;
            owl:allValuesFrom ocsf:string_t ],
        [ a owl:Restriction ;
            owl:onProperty ocsf:to ;
            owl:allValuesFrom ocsf:email_t ],
        [ a owl:Restriction ;
            owl:onProperty ocsf:to ;
            owl:cardinality 1 ],
        [ a owl:Restriction ;
            owl:onProperty ocsf:uid ;
            owl:allValuesFrom ocsf:string_t ],
        [ a owl:Restriction ;
            owl:onProperty ocsf:x_originating_ip ;
            owl:allValuesFrom ocsf:ip_t ] ;
    dcterms:description "The Email object describes the email metadata such as sender, recipients, and direction. Defined by D3FEND <a target='_blank' href='https://d3fend.mitre.org/dao/artifact/d3f:Email/'>d3f:Email</a>." ;
    ocsf:extends "object" ;
    ocsf:name "email" ;
    ocsf:profiles "data_classification" .

ocsf:EmailActivityEvent a owl:Class ;
    rdfs:label "Email Activity" ;
    rdfs:subClassOf ocsf:BaseEvent,
        [ a owl:Restriction ;
            owl:onProperty ocsf:activity_id ;
            owl:allValuesFrom ocsf:integer_t ],
        [ a owl:Restriction ;
            owl:onProperty ocsf:attempt ;
            owl:allValuesFrom ocsf:integer_t ],
        [ a owl:Restriction ;
            owl:onProperty ocsf:banner ;
            owl:allValuesFrom ocsf:string_t ],
        [ a owl:Restriction ;
            owl:onProperty ocsf:direction ;
            owl:allValuesFrom ocsf:string_t ],
        [ a owl:Restriction ;
            owl:onProperty ocsf:direction_id ;
            owl:allValuesFrom ocsf:integer_t ],
        [ a owl:Restriction ;
            owl:onProperty ocsf:direction_id ;
            owl:cardinality 1 ],
        [ a owl:Restriction ;
            owl:onProperty ocsf:dst_endpoint ;
            owl:allValuesFrom ocsf:NetworkEndpoint ],
        [ a owl:Restriction ;
            owl:onProperty ocsf:email ;
            owl:allValuesFrom ocsf:Email ],
        [ a owl:Restriction ;
            owl:onProperty ocsf:email ;
            owl:someValuesFrom ocsf:Email ],
        [ a owl:Restriction ;
            owl:onProperty ocsf:email_auth ;
            owl:allValuesFrom ocsf:EmailAuthentication ],
        [ a owl:Restriction ;
            owl:onProperty ocsf:smtp_hello ;
            owl:allValuesFrom ocsf:string_t ],
        [ a owl:Restriction ;
            owl:onProperty ocsf:src_endpoint ;
            owl:allValuesFrom ocsf:NetworkEndpoint ] ;
    dcterms:description "Email events report activities of emails." ;
    ocsf:category ocsf:NetworkEvent ;
    ocsf:extends "base_event" ;
    ocsf:name "email_activity" ;
    ocsf:profiles "host",
        "security_control" .

ocsf:EmailAuthentication a owl:Class ;
    rdfs:label "Email Authentication" ;
    rdfs:subClassOf ocsf:Object,
        [ a owl:Restriction ;
            owl:onProperty ocsf:dkim ;
            owl:allValuesFrom ocsf:string_t ],
        [ a owl:Restriction ;
            owl:onProperty ocsf:dkim_domain ;
            owl:allValuesFrom ocsf:string_t ],
        [ a owl:Restriction ;
            owl:onProperty ocsf:dkim_signature ;
            owl:allValuesFrom ocsf:string_t ],
        [ a owl:Restriction ;
            owl:onProperty ocsf:dmarc ;
            owl:allValuesFrom ocsf:string_t ],
        [ a owl:Restriction ;
            owl:onProperty ocsf:dmarc_override ;
            owl:allValuesFrom ocsf:string_t ],
        [ a owl:Restriction ;
            owl:onProperty ocsf:dmarc_policy ;
            owl:allValuesFrom ocsf:string_t ],
        [ a owl:Restriction ;
            owl:onProperty ocsf:spf ;
            owl:allValuesFrom ocsf:string_t ] ;
    dcterms:description "The Email Authentication object describes the Sender Policy Framework (SPF), DomainKeys Identified Mail (DKIM) and Domain-based Message Authentication, Reporting and Conformance (DMARC) attributes of an email." ;
    ocsf:extends "object" ;
    ocsf:name "email_auth" .

ocsf:EmailFileActivityEvent a owl:Class ;
    rdfs:label "Email File Activity" ;
    rdfs:subClassOf ocsf:BaseEvent,
        [ a owl:Restriction ;
            owl:onProperty ocsf:activity_id ;
            owl:allValuesFrom ocsf:integer_t ],
        [ a owl:Restriction ;
            owl:onProperty ocsf:email_uid ;
            owl:allValuesFrom ocsf:string_t ],
        [ a owl:Restriction ;
            owl:onProperty ocsf:email_uid ;
            owl:cardinality 1 ],
        [ a owl:Restriction ;
            owl:onProperty ocsf:file ;
            owl:allValuesFrom ocsf:File ],
        [ a owl:Restriction ;
            owl:onProperty ocsf:file ;
            owl:someValuesFrom ocsf:File ] ;
    dcterms:description "Email File Activity events report files within emails." ;
    ocsf:category ocsf:NetworkEvent ;
    ocsf:extends "base_event" ;
    ocsf:name "email_file_activity" ;
    ocsf:profiles "host",
        "security_control" .

ocsf:EmailURLActivityEvent a owl:Class ;
    rdfs:label "Email URL Activity" ;
    rdfs:subClassOf ocsf:BaseEvent,
        [ a owl:Restriction ;
            owl:onProperty ocsf:activity_id ;
            owl:allValuesFrom ocsf:integer_t ],
        [ a owl:Restriction ;
            owl:onProperty ocsf:email_uid ;
            owl:allValuesFrom ocsf:string_t ],
        [ a owl:Restriction ;
            owl:onProperty ocsf:email_uid ;
            owl:cardinality 1 ],
        [ a owl:Restriction ;
            owl:onProperty ocsf:url ;
            owl:allValuesFrom ocsf:UniformResourceLocator ],
        [ a owl:Restriction ;
            owl:onProperty ocsf:url ;
            owl:someValuesFrom ocsf:UniformResourceLocator ] ;
    dcterms:description "Email URL Activity events report URLs within an email." ;
    ocsf:category ocsf:NetworkEvent ;
    ocsf:extends "base_event" ;
    ocsf:name "email_url_activity" ;
    ocsf:profiles "host",
        "security_control" .

ocsf:Endpoint a owl:Class ;
    rdfs:label "Endpoint" ;
    rdfs:subClassOf ocsf:Entity,
        [ a owl:Restriction ;
            owl:onProperty ocsf:agent_list ;
            owl:allValuesFrom ocsf:Agent ],
        [ a owl:Restriction ;
            owl:onProperty ocsf:domain ;
            owl:allValuesFrom ocsf:string_t ],
        [ a owl:Restriction ;
            owl:onProperty ocsf:hostname ;
            owl:allValuesFrom ocsf:hostname_t ],
        [ a owl:Restriction ;
            owl:onProperty ocsf:hw_info ;
            owl:allValuesFrom ocsf:DeviceHardwareInfo ],
        [ a owl:Restriction ;
            owl:onProperty ocsf:instance_uid ;
            owl:allValuesFrom ocsf:string_t ],
        [ a owl:Restriction ;
            owl:onProperty ocsf:interface_name ;
            owl:allValuesFrom ocsf:string_t ],
        [ a owl:Restriction ;
            owl:onProperty ocsf:interface_uid ;
            owl:allValuesFrom ocsf:string_t ],
        [ a owl:Restriction ;
            owl:onProperty ocsf:ip ;
            owl:allValuesFrom ocsf:ip_t ],
        [ a owl:Restriction ;
            owl:onProperty ocsf:location ;
            owl:allValuesFrom ocsf:GeoLocation ],
        [ a owl:Restriction ;
            owl:onProperty ocsf:mac ;
            owl:allValuesFrom ocsf:mac_t ],
        [ a owl:Restriction ;
            owl:onProperty ocsf:name ;
            owl:allValuesFrom ocsf:string_t ],
        [ a owl:Restriction ;
            owl:onProperty ocsf:os ;
            owl:allValuesFrom ocsf:OperatingSystemOS ],
        [ a owl:Restriction ;
            owl:onProperty ocsf:owner ;
            owl:allValuesFrom ocsf:User ],
        [ a owl:Restriction ;
            owl:onProperty ocsf:subnet_uid ;
            owl:allValuesFrom ocsf:string_t ],
        [ a owl:Restriction ;
            owl:onProperty ocsf:type ;
            owl:allValuesFrom ocsf:string_t ],
        [ a owl:Restriction ;
            owl:onProperty ocsf:type_id ;
            owl:allValuesFrom ocsf:integer_t ],
        [ a owl:Restriction ;
            owl:onProperty ocsf:uid ;
            owl:allValuesFrom ocsf:string_t ],
        [ a owl:Restriction ;
            owl:onProperty ocsf:vlan_uid ;
            owl:allValuesFrom ocsf:string_t ],
        [ a owl:Restriction ;
            owl:onProperty ocsf:vpc_uid ;
            owl:allValuesFrom ocsf:string_t ],
        [ a owl:Restriction ;
            owl:onProperty ocsf:zone ;
            owl:allValuesFrom ocsf:string_t ] ;
    dcterms:description "The Endpoint object describes a physical or virtual device that connects to and exchanges information with a computer network. Some examples of endpoints are mobile devices, desktop computers, virtual machines, embedded devices, and servers. Internet-of-Things devices—like cameras, lighting, refrigerators, security systems, smart speakers, and thermostats—are also endpoints." ;
    ocsf:constraints "{\"at_least_one\":[\"ip\",\"uid\",\"name\",\"hostname\",\"instance_uid\",\"interface_uid\",\"interface_name\"]}" ;
    ocsf:extends "_entity" ;
    ocsf:name "endpoint" ;
    ocsf:profiles "container" .

ocsf:EndpointConnection a owl:Class ;
    rdfs:label "Endpoint Connection" ;
    rdfs:subClassOf ocsf:Object,
        [ a owl:Restriction ;
            owl:onProperty ocsf:code ;
            owl:allValuesFrom ocsf:integer_t ],
        [ a owl:Restriction ;
            owl:onProperty ocsf:network_endpoint ;
            owl:allValuesFrom ocsf:NetworkEndpoint ] ;
    dcterms:description "The Endpoint Connection object contains information detailing a connection attempt to an endpoint." ;
    ocsf:constraints "{\"at_least_one\":[\"network_endpoint\",\"code\"]}" ;
    ocsf:extends "object" ;
    ocsf:name "endpoint_connection" .

ocsf:Enrichment a owl:Class ;
    rdfs:label "Enrichment" ;
    rdfs:subClassOf ocsf:Object,
        [ a owl:Restriction ;
            owl:onProperty ocsf:created_time ;
            owl:allValuesFrom ocsf:timestamp_t ],
        [ a owl:Restriction ;
            owl:onProperty ocsf:data ;
            owl:allValuesFrom ocsf:json_t ],
        [ a owl:Restriction ;
            owl:onProperty ocsf:data ;
            owl:cardinality 1 ],
        [ a owl:Restriction ;
            owl:onProperty ocsf:desc ;
            owl:allValuesFrom ocsf:string_t ],
        [ a owl:Restriction ;
            owl:onProperty ocsf:name ;
            owl:allValuesFrom ocsf:string_t ],
        [ a owl:Restriction ;
            owl:onProperty ocsf:name ;
            owl:cardinality 1 ],
        [ a owl:Restriction ;
            owl:onProperty ocsf:provider ;
            owl:allValuesFrom ocsf:string_t ],
        [ a owl:Restriction ;
            owl:onProperty ocsf:reputation ;
            owl:allValuesFrom ocsf:Reputation ],
        [ a owl:Restriction ;
            owl:onProperty ocsf:short_desc ;
            owl:allValuesFrom ocsf:string_t ],
        [ a owl:Restriction ;
            owl:onProperty ocsf:src_url ;
            owl:allValuesFrom ocsf:url_t ],
        [ a owl:Restriction ;
            owl:onProperty ocsf:type ;
            owl:allValuesFrom ocsf:string_t ],
        [ a owl:Restriction ;
            owl:onProperty ocsf:value ;
            owl:allValuesFrom ocsf:string_t ],
        [ a owl:Restriction ;
            owl:onProperty ocsf:value ;
            owl:cardinality 1 ] ;
    dcterms:description "The Enrichment object provides inline enrichment data for specific attributes of interest within an event. It serves as a mechanism to enhance or supplement the information associated with the event by adding additional relevant details or context." ;
    ocsf:extends "object" ;
    ocsf:name "enrichment" .

ocsf:Entity a owl:Class ;
    rdfs:label "Entity" ;
    rdfs:subClassOf ocsf:Object,
        [ a owl:Restriction ;
            owl:onProperty ocsf:name ;
            owl:allValuesFrom ocsf:string_t ],
        [ a owl:Restriction ;
            owl:onProperty ocsf:uid ;
            owl:allValuesFrom ocsf:string_t ] ;
    dcterms:description "The Entity object is an unordered collection of attributes, with a name and unique identifier. It serves as a base object that defines a set of attributes and default constraints available in all objects that extend it." ;
    ocsf:constraints "{\"at_least_one\":[\"name\",\"uid\"]}" ;
    ocsf:extends "object" ;
    ocsf:name "_entity" .

ocsf:EntityManagementEvent a owl:Class ;
    rdfs:label "Entity Management" ;
    rdfs:subClassOf ocsf:IdentityAccessManagementEvent,
        [ a owl:Restriction ;
            owl:onProperty ocsf:access_list ;
            owl:allValuesFrom ocsf:string_t ],
        [ a owl:Restriction ;
            owl:onProperty ocsf:access_mask ;
            owl:allValuesFrom ocsf:integer_t ],
        [ a owl:Restriction ;
            owl:onProperty ocsf:activity_id ;
            owl:allValuesFrom ocsf:integer_t ],
        [ a owl:Restriction ;
            owl:onProperty ocsf:actor ;
            owl:allValuesFrom ocsf:Actor ],
        [ a owl:Restriction ;
            owl:onProperty ocsf:comment ;
            owl:allValuesFrom ocsf:string_t ],
        [ a owl:Restriction ;
            owl:onProperty ocsf:entity ;
            owl:allValuesFrom ocsf:ManagedEntity ],
        [ a owl:Restriction ;
            owl:onProperty ocsf:entity ;
            owl:someValuesFrom ocsf:ManagedEntity ],
        [ a owl:Restriction ;
            owl:onProperty ocsf:entity_result ;
            owl:allValuesFrom ocsf:ManagedEntity ] ;
    dcterms:description "Entity Management events report activity by a managed client, a micro service, or a user at a management console. The activity can be a create, read, update, and delete operation on a managed entity." ;
    ocsf:extends "iam" ;
    ocsf:name "entity_management" .

ocsf:EPSS a owl:Class ;
    rdfs:label "EPSS" ;
    rdfs:subClassOf ocsf:Object,
        [ a owl:Restriction ;
            owl:onProperty ocsf:created_time ;
            owl:allValuesFrom ocsf:timestamp_t ],
        [ a owl:Restriction ;
            owl:onProperty ocsf:percentile ;
            owl:allValuesFrom ocsf:float_t ],
        [ a owl:Restriction ;
            owl:onProperty ocsf:score ;
            owl:allValuesFrom ocsf:string_t ],
        [ a owl:Restriction ;
            owl:onProperty ocsf:score ;
            owl:cardinality 1 ],
        [ a owl:Restriction ;
            owl:onProperty ocsf:version ;
            owl:allValuesFrom ocsf:string_t ] ;
    dcterms:description "The Exploit Prediction Scoring System (EPSS) object describes the estimated probability a vulnerability will be exploited. EPSS is a community-driven effort to combine descriptive information about vulnerabilities (CVEs) with evidence of actual exploitation in-the-wild. (<a target='_blank' href='https://www.first.org/epss/'>EPSS</a>)." ;
    ocsf:extends "object" ;
    ocsf:name "epss" .

ocsf:EventCategory a owl:Class ;
    rdfs:label "Event Category" ;
    d3f:definition "An OCSF event category defines a set of event classes, each aligned with a specific domain or area of focus." ;
    dcterms:description "The OCSF categories organize event classes, each aligned with a specific domain or area of focus." .

ocsf:EventLogActivityEvent a owl:Class ;
    rdfs:label "Event Log Activity" ;
    rdfs:subClassOf ocsf:SystemActivityEvent,
        [ a owl:Restriction ;
            owl:onProperty ocsf:activity_id ;
            owl:allValuesFrom ocsf:integer_t ],
        [ a owl:Restriction ;
            owl:onProperty ocsf:actor ;
            owl:allValuesFrom ocsf:Actor ],
        [ a owl:Restriction ;
            owl:onProperty ocsf:device ;
            owl:allValuesFrom ocsf:Device ],
        [ a owl:Restriction ;
            owl:onProperty ocsf:dst_endpoint ;
            owl:allValuesFrom ocsf:NetworkEndpoint ],
        [ a owl:Restriction ;
            owl:onProperty ocsf:file ;
            owl:allValuesFrom ocsf:File ],
        [ a owl:Restriction ;
            owl:onProperty ocsf:log_name ;
            owl:allValuesFrom ocsf:string_t ],
        [ a owl:Restriction ;
            owl:onProperty ocsf:log_provider ;
            owl:allValuesFrom ocsf:string_t ],
        [ a owl:Restriction ;
            owl:onProperty ocsf:log_type ;
            owl:allValuesFrom ocsf:string_t ],
        [ a owl:Restriction ;
            owl:onProperty ocsf:log_type_id ;
            owl:allValuesFrom ocsf:integer_t ],
        [ a owl:Restriction ;
            owl:onProperty ocsf:src_endpoint ;
            owl:allValuesFrom ocsf:NetworkEndpoint ],
        [ a owl:Restriction ;
            owl:onProperty ocsf:status_code ;
            owl:allValuesFrom ocsf:string_t ],
        [ a owl:Restriction ;
            owl:onProperty ocsf:status_detail ;
            owl:allValuesFrom ocsf:string_t ] ;
    dcterms:description "Event Log Activity events report actions pertaining to the system's event logging service(s), such as disabling logging or clearing the log data." ;
    ocsf:constraints "{\"at_least_one\":[\"log_file\",\"log_name\",\"log_provider\",\"log_type\",\"log_type_id\"]}" ;
    ocsf:extends "system" ;
    ocsf:name "event_log" .

ocsf:EvidenceArtifacts a owl:Class ;
    rdfs:label "Evidence Artifacts" ;
    rdfs:subClassOf ocsf:Object,
        [ a owl:Restriction ;
            owl:onProperty ocsf:actor ;
            owl:allValuesFrom ocsf:Actor ],
        [ a owl:Restriction ;
            owl:onProperty ocsf:api ;
            owl:allValuesFrom ocsf:API ],
        [ a owl:Restriction ;
            owl:onProperty ocsf:connection_info ;
            owl:allValuesFrom ocsf:NetworkConnectionInformation ],
        [ a owl:Restriction ;
            owl:onProperty ocsf:container ;
            owl:allValuesFrom ocsf:Container ],
        [ a owl:Restriction ;
            owl:onProperty ocsf:data ;
            owl:allValuesFrom ocsf:json_t ],
        [ a owl:Restriction ;
            owl:onProperty ocsf:database ;
            owl:allValuesFrom ocsf:Database ],
        [ a owl:Restriction ;
            owl:onProperty ocsf:databucket ;
            owl:allValuesFrom ocsf:Databucket ],
        [ a owl:Restriction ;
            owl:onProperty ocsf:device ;
            owl:allValuesFrom ocsf:Device ],
        [ a owl:Restriction ;
            owl:onProperty ocsf:dst_endpoint ;
            owl:allValuesFrom ocsf:NetworkEndpoint ],
        [ a owl:Restriction ;
            owl:onProperty ocsf:email ;
            owl:allValuesFrom ocsf:Email ],
        [ a owl:Restriction ;
            owl:onProperty ocsf:file ;
            owl:allValuesFrom ocsf:File ],
        [ a owl:Restriction ;
            owl:onProperty ocsf:job ;
            owl:allValuesFrom ocsf:Job ],
        [ a owl:Restriction ;
            owl:onProperty ocsf:process ;
            owl:allValuesFrom ocsf:Process ],
        [ a owl:Restriction ;
            owl:onProperty ocsf:query ;
            owl:allValuesFrom ocsf:DNSQuery ],
        [ a owl:Restriction ;
            owl:onProperty ocsf:src_endpoint ;
            owl:allValuesFrom ocsf:NetworkEndpoint ],
        [ a owl:Restriction ;
            owl:onProperty ocsf:url ;
            owl:allValuesFrom ocsf:UniformResourceLocator ],
        [ a owl:Restriction ;
            owl:onProperty ocsf:user ;
            owl:allValuesFrom ocsf:User ] ;
    dcterms:description "A collection of evidence artifacts associated to the activity/activities that triggered a security detection." ;
    ocsf:constraints "{\"at_least_one\":[\"actor\",\"api\",\"connection_info\",\"data\",\"database\",\"databucket\",\"device\",\"dst_endpoint\",\"email\",\"file\",\"process\",\"query\",\"src_endpoint\",\"url\",\"user\",\"job\"]}" ;
    ocsf:extends "object" ;
    ocsf:name "evidences" .

ocsf:Feature a owl:Class ;
    rdfs:label "Feature" ;
    rdfs:subClassOf ocsf:Entity,
        [ a owl:Restriction ;
            owl:onProperty ocsf:name ;
            owl:allValuesFrom ocsf:string_t ],
        [ a owl:Restriction ;
            owl:onProperty ocsf:uid ;
            owl:allValuesFrom ocsf:string_t ],
        [ a owl:Restriction ;
            owl:onProperty ocsf:version ;
            owl:allValuesFrom ocsf:string_t ] ;
    dcterms:description "The Feature object provides information about the software product feature that generated a specific event. It encompasses details related to the capabilities, components, user interface (UI) design, and performance upgrades associated with the feature." ;
    ocsf:extends "_entity" ;
    ocsf:name "feature" .

ocsf:File a owl:Class ;
    rdfs:label "File" ;
    rdfs:subClassOf ocsf:Entity,
        [ a owl:Restriction ;
            owl:onProperty ocsf:accessed_time ;
            owl:allValuesFrom ocsf:timestamp_t ],
        [ a owl:Restriction ;
            owl:onProperty ocsf:accessor ;
            owl:allValuesFrom ocsf:User ],
        [ a owl:Restriction ;
            owl:onProperty ocsf:attributes ;
            owl:allValuesFrom ocsf:integer_t ],
        [ a owl:Restriction ;
            owl:onProperty ocsf:company_name ;
            owl:allValuesFrom ocsf:string_t ],
        [ a owl:Restriction ;
            owl:onProperty ocsf:confidentiality ;
            owl:allValuesFrom ocsf:string_t ],
        [ a owl:Restriction ;
            owl:onProperty ocsf:confidentiality_id ;
            owl:allValuesFrom ocsf:integer_t ],
        [ a owl:Restriction ;
            owl:onProperty ocsf:created_time ;
            owl:allValuesFrom ocsf:timestamp_t ],
        [ a owl:Restriction ;
            owl:onProperty ocsf:creator ;
            owl:allValuesFrom ocsf:User ],
        [ a owl:Restriction ;
            owl:onProperty ocsf:desc ;
            owl:allValuesFrom ocsf:string_t ],
        [ a owl:Restriction ;
            owl:onProperty ocsf:ext ;
            owl:allValuesFrom ocsf:string_t ],
        [ a owl:Restriction ;
            owl:onProperty ocsf:hashes ;
            owl:allValuesFrom ocsf:Fingerprint ],
        [ a owl:Restriction ;
            owl:onProperty ocsf:is_system ;
            owl:allValuesFrom ocsf:boolean_t ],
        [ a owl:Restriction ;
            owl:onProperty ocsf:mime_type ;
            owl:allValuesFrom ocsf:string_t ],
        [ a owl:Restriction ;
            owl:onProperty ocsf:modified_time ;
            owl:allValuesFrom ocsf:timestamp_t ],
        [ a owl:Restriction ;
            owl:onProperty ocsf:modifier ;
            owl:allValuesFrom ocsf:User ],
        [ a owl:Restriction ;
            owl:onProperty ocsf:name ;
            owl:allValuesFrom ocsf:string_t ],
        [ a owl:Restriction ;
            owl:onProperty ocsf:name ;
            owl:cardinality 1 ],
        [ a owl:Restriction ;
            owl:onProperty ocsf:owner ;
            owl:allValuesFrom ocsf:User ],
        [ a owl:Restriction ;
            owl:onProperty ocsf:parent_folder ;
            owl:allValuesFrom ocsf:string_t ],
        [ a owl:Restriction ;
            owl:onProperty ocsf:path ;
            owl:allValuesFrom ocsf:string_t ],
        [ a owl:Restriction ;
            owl:onProperty ocsf:product ;
            owl:allValuesFrom ocsf:Product ],
        [ a owl:Restriction ;
            owl:onProperty ocsf:security_descriptor ;
            owl:allValuesFrom ocsf:string_t ],
        [ a owl:Restriction ;
            owl:onProperty ocsf:signature ;
            owl:allValuesFrom ocsf:DigitalSignature ],
        [ a owl:Restriction ;
            owl:onProperty ocsf:size ;
            owl:allValuesFrom ocsf:long_t ],
        [ a owl:Restriction ;
            owl:onProperty ocsf:type ;
            owl:allValuesFrom ocsf:string_t ],
        [ a owl:Restriction ;
            owl:onProperty ocsf:type_id ;
            owl:allValuesFrom ocsf:integer_t ],
        [ a owl:Restriction ;
            owl:onProperty ocsf:type_id ;
            owl:cardinality 1 ],
        [ a owl:Restriction ;
            owl:onProperty ocsf:uid ;
            owl:allValuesFrom ocsf:string_t ],
        [ a owl:Restriction ;
            owl:onProperty ocsf:version ;
            owl:allValuesFrom ocsf:string_t ],
        [ a owl:Restriction ;
            owl:onProperty ocsf:xattributes ;
            owl:allValuesFrom ocsf:Object ] ;
    dcterms:description "The File object represents the metadata associated with a file stored in a computer system. It encompasses information about the file itself, including its attributes, properties, and organizational details. Defined by D3FEND <a target='_blank' href='https://next.d3fend.mitre.org/dao/artifact/d3f:File/'>d3f:File</a>." ;
    ocsf:constraints "{}" ;
    ocsf:extends "_entity" ;
    ocsf:name "file" ;
    ocsf:profiles "data_classification" .

ocsf:FileHostingActivityEvent a owl:Class ;
    rdfs:label "File Hosting Activity" ;
    rdfs:subClassOf ocsf:ApplicationActivityEvent,
        [ a owl:Restriction ;
            owl:onProperty ocsf:activity_id ;
            owl:allValuesFrom ocsf:integer_t ],
        [ a owl:Restriction ;
            owl:onProperty ocsf:actor ;
            owl:allValuesFrom ocsf:Actor ],
        [ a owl:Restriction ;
            owl:onProperty ocsf:actor ;
            owl:someValuesFrom ocsf:Actor ],
        [ a owl:Restriction ;
            owl:onProperty ocsf:connection_info ;
            owl:allValuesFrom ocsf:NetworkConnectionInformation ],
        [ a owl:Restriction ;
            owl:onProperty ocsf:dst_endpoint ;
            owl:allValuesFrom ocsf:NetworkEndpoint ],
        [ a owl:Restriction ;
            owl:onProperty ocsf:expiration_time ;
            owl:allValuesFrom ocsf:timestamp_t ],
        [ a owl:Restriction ;
            owl:onProperty ocsf:file ;
            owl:allValuesFrom ocsf:File ],
        [ a owl:Restriction ;
            owl:onProperty ocsf:file ;
            owl:someValuesFrom ocsf:File ],
        [ a owl:Restriction ;
            owl:onProperty ocsf:file_result ;
            owl:allValuesFrom ocsf:File ],
        [ a owl:Restriction ;
            owl:onProperty ocsf:src_endpoint ;
            owl:allValuesFrom ocsf:NetworkEndpoint ],
        [ a owl:Restriction ;
            owl:onProperty ocsf:src_endpoint ;
            owl:someValuesFrom ocsf:NetworkEndpoint ] ;
    dcterms:description "File Hosting Activity events report the actions taken by file management applications, including file sharing servers like Sharepoint and services such as Box, MS OneDrive, or Google Drive." ;
    ocsf:category ocsf:ApplicationActivityEvent ;
    ocsf:extends "application" ;
    ocsf:name "file_hosting" .

ocsf:FileQueryEvent a owl:Class ;
    rdfs:label "File Query" ;
    rdfs:subClassOf ocsf:DiscoveryResultEvent,
        [ a owl:Restriction ;
            owl:onProperty ocsf:file ;
            owl:allValuesFrom ocsf:File ],
        [ a owl:Restriction ;
            owl:onProperty ocsf:file ;
            owl:someValuesFrom ocsf:File ] ;
    dcterms:description "File Query events report information about files that are present on the system." ;
    ocsf:extends "discovery_result" ;
    ocsf:name "file_query" .

ocsf:FileRemediationActivityEvent a owl:Class ;
    rdfs:label "File Remediation Activity" ;
    rdfs:subClassOf ocsf:RemediationActivityEvent,
        [ a owl:Restriction ;
            owl:onProperty ocsf:file ;
            owl:allValuesFrom ocsf:File ],
        [ a owl:Restriction ;
            owl:onProperty ocsf:file ;
            owl:someValuesFrom ocsf:File ] ;
    dcterms:description "File Remediation Activity events report on attempts at remediating files. It follows the MITRE countermeasures defined by the D3FEND™ <a target='_blank' href='https://d3fend.mitre.org/'>Matrix</a>. Sub-techniques will include File, such as File Removal or Restore File." ;
    ocsf:extends "remediation_activity" ;
    ocsf:name "file_remediation_activity" .

ocsf:FileSystemActivityEvent a owl:Class ;
    rdfs:label "File System Activity" ;
    rdfs:subClassOf ocsf:SystemActivityEvent,
        [ a owl:Restriction ;
            owl:onProperty ocsf:access_mask ;
            owl:allValuesFrom ocsf:integer_t ],
        [ a owl:Restriction ;
            owl:onProperty ocsf:activity_id ;
            owl:allValuesFrom ocsf:integer_t ],
        [ a owl:Restriction ;
            owl:onProperty ocsf:actor ;
            owl:allValuesFrom ocsf:Actor ],
        [ a owl:Restriction ;
            owl:onProperty ocsf:actor ;
            owl:someValuesFrom ocsf:Actor ],
        [ a owl:Restriction ;
            owl:onProperty ocsf:component ;
            owl:allValuesFrom ocsf:string_t ],
        [ a owl:Restriction ;
            owl:onProperty ocsf:connection_uid ;
            owl:allValuesFrom ocsf:string_t ],
        [ a owl:Restriction ;
            owl:onProperty ocsf:create_mask ;
            owl:allValuesFrom ocsf:string_t ],
        [ a owl:Restriction ;
            owl:onProperty ocsf:file ;
            owl:allValuesFrom ocsf:File ],
        [ a owl:Restriction ;
            owl:onProperty ocsf:file ;
            owl:someValuesFrom ocsf:File ],
        [ a owl:Restriction ;
            owl:onProperty ocsf:file_diff ;
            owl:allValuesFrom ocsf:string_t ],
        [ a owl:Restriction ;
            owl:onProperty ocsf:file_result ;
            owl:allValuesFrom ocsf:File ] ;
    dcterms:description "File System Activity events report when a process performs an action on a file or folder." ;
    ocsf:extends "system" ;
    ocsf:name "file_activity" .

ocsf:Finding a owl:Class ;
    rdfs:label "Finding" ;
    rdfs:subClassOf ocsf:Object,
        [ a owl:Restriction ;
            owl:onProperty ocsf:created_time ;
            owl:allValuesFrom ocsf:timestamp_t ],
        [ a owl:Restriction ;
            owl:onProperty ocsf:desc ;
            owl:allValuesFrom ocsf:string_t ],
        [ a owl:Restriction ;
            owl:onProperty ocsf:first_seen_time ;
            owl:allValuesFrom ocsf:timestamp_t ],
        [ a owl:Restriction ;
            owl:onProperty ocsf:last_seen_time ;
            owl:allValuesFrom ocsf:timestamp_t ],
        [ a owl:Restriction ;
            owl:onProperty ocsf:modified_time ;
            owl:allValuesFrom ocsf:timestamp_t ],
        [ a owl:Restriction ;
            owl:onProperty ocsf:product_uid ;
            owl:allValuesFrom ocsf:string_t ],
        [ a owl:Restriction ;
            owl:onProperty ocsf:related_events ;
            owl:allValuesFrom ocsf:RelatedEvent ],
        [ a owl:Restriction ;
            owl:onProperty ocsf:remediation ;
            owl:allValuesFrom ocsf:Remediation ],
        [ a owl:Restriction ;
            owl:onProperty ocsf:src_url ;
            owl:allValuesFrom ocsf:url_t ],
        [ a owl:Restriction ;
            owl:onProperty ocsf:supporting_data ;
            owl:allValuesFrom ocsf:json_t ],
        [ a owl:Restriction ;
            owl:onProperty ocsf:title ;
            owl:allValuesFrom ocsf:string_t ],
        [ a owl:Restriction ;
            owl:onProperty ocsf:title ;
            owl:cardinality 1 ],
        [ a owl:Restriction ;
            owl:onProperty ocsf:types ;
            owl:allValuesFrom ocsf:string_t ],
        [ a owl:Restriction ;
            owl:onProperty ocsf:uid ;
            owl:allValuesFrom ocsf:string_t ],
        [ a owl:Restriction ;
            owl:onProperty ocsf:uid ;
            owl:cardinality 1 ] ;
    dcterms:description "The Finding object describes metadata related to a security finding generated by a security tool or system." ;
    ocsf:extends "object" ;
    ocsf:name "finding" .

ocsf:FindingEvent a owl:Class ;
    rdfs:label "Finding" ;
    rdfs:subClassOf ocsf:BaseEvent,
        [ a owl:Restriction ;
            owl:onProperty ocsf:activity_id ;
            owl:allValuesFrom ocsf:integer_t ],
        [ a owl:Restriction ;
            owl:onProperty ocsf:activity_name ;
            owl:allValuesFrom ocsf:string_t ],
        [ a owl:Restriction ;
            owl:onProperty ocsf:comment ;
            owl:allValuesFrom ocsf:string_t ],
        [ a owl:Restriction ;
            owl:onProperty ocsf:confidence ;
            owl:allValuesFrom ocsf:string_t ],
        [ a owl:Restriction ;
            owl:onProperty ocsf:confidence_id ;
            owl:allValuesFrom ocsf:integer_t ],
        [ a owl:Restriction ;
            owl:onProperty ocsf:confidence_score ;
            owl:allValuesFrom ocsf:integer_t ],
        [ a owl:Restriction ;
            owl:onProperty ocsf:device ;
            owl:allValuesFrom ocsf:Device ],
        [ a owl:Restriction ;
            owl:onProperty ocsf:end_time ;
            owl:allValuesFrom ocsf:timestamp_t ],
        [ a owl:Restriction ;
            owl:onProperty ocsf:finding_info ;
            owl:allValuesFrom ocsf:FindingInformation ],
        [ a owl:Restriction ;
            owl:onProperty ocsf:finding_info ;
            owl:someValuesFrom ocsf:FindingInformation ],
        [ a owl:Restriction ;
            owl:onProperty ocsf:start_time ;
            owl:allValuesFrom ocsf:timestamp_t ],
        [ a owl:Restriction ;
            owl:onProperty ocsf:status ;
            owl:allValuesFrom ocsf:string_t ],
        [ a owl:Restriction ;
            owl:onProperty ocsf:status_id ;
            owl:allValuesFrom ocsf:integer_t ] ;
    dcterms:description "The Finding event is a generic event that defines a set of attributes available in the Findings category." ;
    ocsf:extends "base_event" ;
    ocsf:name "finding" ;
    ocsf:profiles "host" .

ocsf:FindingInformation a owl:Class ;
    rdfs:label "Finding Information" ;
    rdfs:subClassOf ocsf:Object,
        [ a owl:Restriction ;
            owl:onProperty ocsf:analytic ;
            owl:allValuesFrom ocsf:Analytic ],
        [ a owl:Restriction ;
            owl:onProperty ocsf:attacks ;
            owl:allValuesFrom ocsf:MITREATTCK ],
        [ a owl:Restriction ;
            owl:onProperty ocsf:created_time ;
            owl:allValuesFrom ocsf:timestamp_t ],
        [ a owl:Restriction ;
            owl:onProperty ocsf:data_sources ;
            owl:allValuesFrom ocsf:string_t ],
        [ a owl:Restriction ;
            owl:onProperty ocsf:desc ;
            owl:allValuesFrom ocsf:string_t ],
        [ a owl:Restriction ;
            owl:onProperty ocsf:first_seen_time ;
            owl:allValuesFrom ocsf:timestamp_t ],
        [ a owl:Restriction ;
            owl:onProperty ocsf:kill_chain ;
            owl:allValuesFrom ocsf:KillChainPhase ],
        [ a owl:Restriction ;
            owl:onProperty ocsf:last_seen_time ;
            owl:allValuesFrom ocsf:timestamp_t ],
        [ a owl:Restriction ;
            owl:onProperty ocsf:modified_time ;
            owl:allValuesFrom ocsf:timestamp_t ],
        [ a owl:Restriction ;
            owl:onProperty ocsf:product_uid ;
            owl:allValuesFrom ocsf:string_t ],
        [ a owl:Restriction ;
            owl:onProperty ocsf:related_analytics ;
            owl:allValuesFrom ocsf:Analytic ],
        [ a owl:Restriction ;
            owl:onProperty ocsf:related_events ;
            owl:allValuesFrom ocsf:RelatedEvent ],
        [ a owl:Restriction ;
            owl:onProperty ocsf:src_url ;
            owl:allValuesFrom ocsf:url_t ],
        [ a owl:Restriction ;
            owl:onProperty ocsf:title ;
            owl:allValuesFrom ocsf:string_t ],
        [ a owl:Restriction ;
            owl:onProperty ocsf:title ;
            owl:cardinality 1 ],
        [ a owl:Restriction ;
            owl:onProperty ocsf:types ;
            owl:allValuesFrom ocsf:string_t ],
        [ a owl:Restriction ;
            owl:onProperty ocsf:uid ;
            owl:allValuesFrom ocsf:string_t ],
        [ a owl:Restriction ;
            owl:onProperty ocsf:uid ;
            owl:cardinality 1 ] ;
    dcterms:description "The Finding Information object describes metadata related to a security finding generated by a security tool or system." ;
    ocsf:extends "object" ;
    ocsf:name "finding_info" .

ocsf:FindingsEventCategory a owl:Class ;
    rdfs:label "Findings" ;
    rdfs:subClassOf ocsf:EventCategory ;
    d3f:definition "Findings events report findings, detections, and possible resolutions of malware, anomalies, or other actions performed by security products." ;
    ocsf:category_name "findings" .

ocsf:Fingerprint a owl:Class ;
    rdfs:label "Fingerprint" ;
    rdfs:subClassOf ocsf:Object,
        [ a owl:Restriction ;
            owl:onProperty ocsf:algorithm ;
            owl:allValuesFrom ocsf:string_t ],
        [ a owl:Restriction ;
            owl:onProperty ocsf:algorithm_id ;
            owl:allValuesFrom ocsf:integer_t ],
        [ a owl:Restriction ;
            owl:onProperty ocsf:algorithm_id ;
            owl:cardinality 1 ],
        [ a owl:Restriction ;
            owl:onProperty ocsf:value ;
            owl:allValuesFrom ocsf:string_t ],
        [ a owl:Restriction ;
            owl:onProperty ocsf:value ;
            owl:cardinality 1 ] ;
    dcterms:description "The Fingerprint object provides detailed information about a digital fingerprint, which is a compact representation of data used to identify a longer piece of information, such as a public key or file content. It contains the algorithm and value of the fingerprint, enabling efficient and reliable identification of the associated data." ;
    ocsf:extends "object" ;
    ocsf:name "fingerprint" .

ocsf:FirewallRule a owl:Class ;
    rdfs:label "Firewall Rule" ;
    rdfs:subClassOf ocsf:Rule,
        [ a owl:Restriction ;
            owl:onProperty ocsf:condition ;
            owl:allValuesFrom ocsf:string_t ],
        [ a owl:Restriction ;
            owl:onProperty ocsf:duration ;
            owl:allValuesFrom ocsf:long_t ],
        [ a owl:Restriction ;
            owl:onProperty ocsf:match_details ;
            owl:allValuesFrom ocsf:string_t ],
        [ a owl:Restriction ;
            owl:onProperty ocsf:match_location ;
            owl:allValuesFrom ocsf:string_t ],
        [ a owl:Restriction ;
            owl:onProperty ocsf:rate_limit ;
            owl:allValuesFrom ocsf:integer_t ],
        [ a owl:Restriction ;
            owl:onProperty ocsf:sensitivity ;
            owl:allValuesFrom ocsf:string_t ] ;
    dcterms:description "The Firewall Rule object represents a specific rule within a firewall policy or event. It contains information about a rule's configuration, properties, and associated actions that define how network traffic is handled by the firewall." ;
    ocsf:extends "rule" ;
    ocsf:name "firewall_rule" .

ocsf:FolderQueryEvent a owl:Class ;
    rdfs:label "Folder Query" ;
    rdfs:subClassOf ocsf:DiscoveryResultEvent,
        [ a owl:Restriction ;
            owl:onProperty ocsf:folder ;
            owl:allValuesFrom ocsf:File ],
        [ a owl:Restriction ;
            owl:onProperty ocsf:folder ;
            owl:someValuesFrom ocsf:File ] ;
    dcterms:description "Folder Query events report information about folders that are present on the system." ;
    ocsf:extends "discovery_result" ;
    ocsf:name "folder_query" .

ocsf:FTPActivityEvent a owl:Class ;
    rdfs:label "FTP Activity" ;
    rdfs:subClassOf ocsf:NetworkEvent,
        [ a owl:Restriction ;
            owl:onProperty ocsf:activity_id ;
            owl:allValuesFrom ocsf:integer_t ],
        [ a owl:Restriction ;
            owl:onProperty ocsf:codes ;
            owl:allValuesFrom ocsf:integer_t ],
        [ a owl:Restriction ;
            owl:onProperty ocsf:command ;
            owl:allValuesFrom ocsf:string_t ],
        [ a owl:Restriction ;
            owl:onProperty ocsf:command_responses ;
            owl:allValuesFrom ocsf:string_t ],
        [ a owl:Restriction ;
            owl:onProperty ocsf:file ;
            owl:allValuesFrom ocsf:File ],
        [ a owl:Restriction ;
            owl:onProperty ocsf:name ;
            owl:allValuesFrom ocsf:string_t ],
        [ a owl:Restriction ;
            owl:onProperty ocsf:port ;
            owl:allValuesFrom ocsf:port_t ],
        [ a owl:Restriction ;
            owl:onProperty ocsf:type ;
            owl:allValuesFrom ocsf:string_t ] ;
    dcterms:description "File Transfer Protocol (FTP) Activity events report file transfers between a server and a client as seen on the network." ;
    ocsf:extends "network" ;
    ocsf:name "ftp_activity" .

ocsf:GeoLocation a owl:Class ;
    rdfs:label "Geo Location" ;
    rdfs:subClassOf ocsf:Object,
        [ a owl:Restriction ;
            owl:onProperty ocsf:city ;
            owl:allValuesFrom ocsf:string_t ],
        [ a owl:Restriction ;
            owl:onProperty ocsf:continent ;
            owl:allValuesFrom ocsf:string_t ],
        [ a owl:Restriction ;
            owl:onProperty ocsf:coordinates ;
            owl:allValuesFrom ocsf:float_t ],
        [ a owl:Restriction ;
            owl:onProperty ocsf:country ;
            owl:allValuesFrom ocsf:string_t ],
        [ a owl:Restriction ;
            owl:onProperty ocsf:desc ;
            owl:allValuesFrom ocsf:string_t ],
        [ a owl:Restriction ;
            owl:onProperty ocsf:geohash ;
            owl:allValuesFrom ocsf:string_t ],
        [ a owl:Restriction ;
            owl:onProperty ocsf:is_on_premises ;
            owl:allValuesFrom ocsf:boolean_t ],
        [ a owl:Restriction ;
            owl:onProperty ocsf:isp ;
            owl:allValuesFrom ocsf:string_t ],
        [ a owl:Restriction ;
            owl:onProperty ocsf:lat ;
            owl:allValuesFrom ocsf:float_t ],
        [ a owl:Restriction ;
            owl:onProperty ocsf:long ;
            owl:allValuesFrom ocsf:float_t ],
        [ a owl:Restriction ;
            owl:onProperty ocsf:postal_code ;
            owl:allValuesFrom ocsf:string_t ],
        [ a owl:Restriction ;
            owl:onProperty ocsf:provider ;
            owl:allValuesFrom ocsf:string_t ],
        [ a owl:Restriction ;
            owl:onProperty ocsf:region ;
            owl:allValuesFrom ocsf:string_t ] ;
    dcterms:description "The Geo Location object describes a geographical location, usually associated with an IP address. Defined by D3FEND <a target='_blank' href='https://d3fend.mitre.org/dao/artifact/d3f:PhysicalLocation/'>d3f:PhysicalLocation</a>." ;
    ocsf:constraints "{\"at_least_one\":[\"city\",\"country\",\"postal_code\",\"region\"]}" ;
    ocsf:extends "object" ;
    ocsf:name "location" .

ocsf:Group a owl:Class ;
    rdfs:label "Group" ;
    rdfs:subClassOf ocsf:Entity,
        [ a owl:Restriction ;
            owl:onProperty ocsf:desc ;
            owl:allValuesFrom ocsf:string_t ],
        [ a owl:Restriction ;
            owl:onProperty ocsf:domain ;
            owl:allValuesFrom ocsf:string_t ],
        [ a owl:Restriction ;
            owl:onProperty ocsf:name ;
            owl:allValuesFrom ocsf:string_t ],
        [ a owl:Restriction ;
            owl:onProperty ocsf:privileges ;
            owl:allValuesFrom ocsf:string_t ],
        [ a owl:Restriction ;
            owl:onProperty ocsf:type ;
            owl:allValuesFrom ocsf:string_t ],
        [ a owl:Restriction ;
            owl:onProperty ocsf:uid ;
            owl:allValuesFrom ocsf:string_t ] ;
    dcterms:description "The Group object represents a collection or association of entities, such as users, policies, or devices. It serves as a logical grouping mechanism to organize and manage entities with similar characteristics or permissions within a system or organization." ;
    ocsf:extends "_entity" ;
    ocsf:name "group" .

ocsf:GroupManagementEvent a owl:Class ;
    rdfs:label "Group Management" ;
    rdfs:subClassOf ocsf:IdentityAccessManagementEvent,
        [ a owl:Restriction ;
            owl:onProperty ocsf:activity_id ;
            owl:allValuesFrom ocsf:integer_t ],
        [ a owl:Restriction ;
            owl:onProperty ocsf:group ;
            owl:allValuesFrom ocsf:Group ],
        [ a owl:Restriction ;
            owl:onProperty ocsf:group ;
            owl:someValuesFrom ocsf:Group ],
        [ a owl:Restriction ;
            owl:onProperty ocsf:privileges ;
            owl:allValuesFrom ocsf:string_t ],
        [ a owl:Restriction ;
            owl:onProperty ocsf:resource ;
            owl:allValuesFrom ocsf:ResourceDetails ],
        [ a owl:Restriction ;
            owl:onProperty ocsf:user ;
            owl:allValuesFrom ocsf:User ] ;
    dcterms:description "Group Management events report management updates to a group, including updates to membership and permissions." ;
    ocsf:constraints "{\"at_least_one\":[\"privileges\",\"user\"]}" ;
    ocsf:extends "iam" ;
    ocsf:name "group_management" .

ocsf:HASSH a owl:Class ;
    rdfs:label "HASSH" ;
    rdfs:subClassOf ocsf:Object,
        [ a owl:Restriction ;
            owl:onProperty ocsf:algorithm ;
            owl:allValuesFrom ocsf:string_t ],
        [ a owl:Restriction ;
            owl:onProperty ocsf:fingerprint ;
            owl:allValuesFrom ocsf:Fingerprint ],
        [ a owl:Restriction ;
            owl:onProperty ocsf:fingerprint ;
            owl:someValuesFrom ocsf:Fingerprint ] ;
    dcterms:description "The HASSH object contains SSH network fingerprinting values for specific client/server implementations. It provides a standardized way of identifying and categorizing SSH connections based on their unique characteristics and behavior." ;
    ocsf:extends "object" ;
    ocsf:name "hassh" .

ocsf:HTTPActivityEvent a owl:Class ;
    rdfs:label "HTTP Activity" ;
    rdfs:subClassOf ocsf:NetworkEvent,
        [ a owl:Restriction ;
            owl:onProperty ocsf:activity_id ;
            owl:allValuesFrom ocsf:integer_t ],
        [ a owl:Restriction ;
            owl:onProperty ocsf:file ;
            owl:allValuesFrom ocsf:File ],
        [ a owl:Restriction ;
            owl:onProperty ocsf:http_cookies ;
            owl:allValuesFrom ocsf:HTTPCookie ],
        [ a owl:Restriction ;
            owl:onProperty ocsf:http_request ;
            owl:allValuesFrom ocsf:HTTPRequest ],
        [ a owl:Restriction ;
            owl:onProperty ocsf:http_request ;
            owl:someValuesFrom ocsf:HTTPRequest ],
        [ a owl:Restriction ;
            owl:onProperty ocsf:http_response ;
            owl:allValuesFrom ocsf:HTTPResponse ],
        [ a owl:Restriction ;
            owl:onProperty ocsf:http_response ;
            owl:someValuesFrom ocsf:HTTPResponse ],
        [ a owl:Restriction ;
            owl:onProperty ocsf:http_status ;
            owl:allValuesFrom ocsf:integer_t ] ;
    dcterms:description "HTTP Activity events report HTTP connection and traffic information." ;
    ocsf:category ocsf:NetworkEvent ;
    ocsf:extends "network" ;
    ocsf:name "http_activity" .

ocsf:HTTPCookie a owl:Class ;
    rdfs:label "HTTP Cookie" ;
    rdfs:subClassOf ocsf:Object,
        [ a owl:Restriction ;
            owl:onProperty ocsf:domain ;
            owl:allValuesFrom ocsf:string_t ],
        [ a owl:Restriction ;
            owl:onProperty ocsf:expiration_time ;
            owl:allValuesFrom ocsf:timestamp_t ],
        [ a owl:Restriction ;
            owl:onProperty ocsf:http_only ;
            owl:allValuesFrom ocsf:boolean_t ],
        [ a owl:Restriction ;
            owl:onProperty ocsf:is_http_only ;
            owl:allValuesFrom ocsf:boolean_t ],
        [ a owl:Restriction ;
            owl:onProperty ocsf:is_secure ;
            owl:allValuesFrom ocsf:boolean_t ],
        [ a owl:Restriction ;
            owl:onProperty ocsf:name ;
            owl:allValuesFrom ocsf:string_t ],
        [ a owl:Restriction ;
            owl:onProperty ocsf:name ;
            owl:cardinality 1 ],
        [ a owl:Restriction ;
            owl:onProperty ocsf:path ;
            owl:allValuesFrom ocsf:string_t ],
        [ a owl:Restriction ;
            owl:onProperty ocsf:samesite ;
            owl:allValuesFrom ocsf:string_t ],
        [ a owl:Restriction ;
            owl:onProperty ocsf:secure ;
            owl:allValuesFrom ocsf:boolean_t ],
        [ a owl:Restriction ;
            owl:onProperty ocsf:value ;
            owl:allValuesFrom ocsf:string_t ],
        [ a owl:Restriction ;
            owl:onProperty ocsf:value ;
            owl:cardinality 1 ] ;
    dcterms:description "The HTTP Cookie object, also known as a web cookie or browser cookie, contains details and values pertaining to a small piece of data that a server sends to a user's web browser. This data is then stored by the browser and sent back to the server with subsequent requests, allowing the server to remember and track certain information about the user's browsing session or preferences." ;
    ocsf:extends "object" ;
    ocsf:name "http_cookie" .

ocsf:HTTPHeader a owl:Class ;
    rdfs:label "HTTP Header" ;
    rdfs:subClassOf ocsf:Object,
        [ a owl:Restriction ;
            owl:onProperty ocsf:name ;
            owl:allValuesFrom ocsf:string_t ],
        [ a owl:Restriction ;
            owl:onProperty ocsf:name ;
            owl:cardinality 1 ],
        [ a owl:Restriction ;
            owl:onProperty ocsf:value ;
            owl:allValuesFrom ocsf:string_t ],
        [ a owl:Restriction ;
            owl:onProperty ocsf:value ;
            owl:cardinality 1 ] ;
    dcterms:description "TThe HTTP Header object represents the headers sent in an HTTP request or response. HTTP headers are key-value pairs that convey additional information about the HTTP message, including details about the content, caching, authentication, encoding, and other aspects of the communication." ;
    ocsf:extends "object" ;
    ocsf:name "http_header" .

ocsf:HTTPRequest a owl:Class ;
    rdfs:label "HTTP Request" ;
    rdfs:subClassOf ocsf:Object,
        [ a owl:Restriction ;
            owl:onProperty ocsf:args ;
            owl:allValuesFrom ocsf:string_t ],
        [ a owl:Restriction ;
            owl:onProperty ocsf:http_headers ;
            owl:allValuesFrom ocsf:HTTPHeader ],
        [ a owl:Restriction ;
            owl:onProperty ocsf:http_method ;
            owl:allValuesFrom ocsf:string_t ],
        [ a owl:Restriction ;
            owl:onProperty ocsf:length ;
            owl:allValuesFrom ocsf:integer_t ],
        [ a owl:Restriction ;
            owl:onProperty ocsf:referrer ;
            owl:allValuesFrom ocsf:string_t ],
        [ a owl:Restriction ;
            owl:onProperty ocsf:uid ;
            owl:allValuesFrom ocsf:string_t ],
        [ a owl:Restriction ;
            owl:onProperty ocsf:url ;
            owl:allValuesFrom ocsf:UniformResourceLocator ],
        [ a owl:Restriction ;
            owl:onProperty ocsf:user_agent ;
            owl:allValuesFrom ocsf:string_t ],
        [ a owl:Restriction ;
            owl:onProperty ocsf:version ;
            owl:allValuesFrom ocsf:string_t ],
        [ a owl:Restriction ;
            owl:onProperty ocsf:x_forwarded_for ;
            owl:allValuesFrom ocsf:ip_t ] ;
    dcterms:description "The HTTP Request object represents the attributes of a request made to a web server. It encapsulates the details and metadata associated with an HTTP request, including the request method, headers, URL, query parameters, body content, and other relevant information." ;
    ocsf:extends "object" ;
    ocsf:name "http_request" .

ocsf:HTTPResponse a owl:Class ;
    rdfs:label "HTTP Response" ;
    rdfs:subClassOf ocsf:Object,
        [ a owl:Restriction ;
            owl:onProperty ocsf:code ;
            owl:allValuesFrom ocsf:integer_t ],
        [ a owl:Restriction ;
            owl:onProperty ocsf:code ;
            owl:cardinality 1 ],
        [ a owl:Restriction ;
            owl:onProperty ocsf:content_type ;
            owl:allValuesFrom ocsf:string_t ],
        [ a owl:Restriction ;
            owl:onProperty ocsf:http_headers ;
            owl:allValuesFrom ocsf:HTTPHeader ],
        [ a owl:Restriction ;
            owl:onProperty ocsf:latency ;
            owl:allValuesFrom ocsf:integer_t ],
        [ a owl:Restriction ;
            owl:onProperty ocsf:length ;
            owl:allValuesFrom ocsf:integer_t ],
        [ a owl:Restriction ;
            owl:onProperty ocsf:message ;
            owl:allValuesFrom ocsf:string_t ],
        [ a owl:Restriction ;
            owl:onProperty ocsf:status ;
            owl:allValuesFrom ocsf:string_t ] ;
    dcterms:description "The HTTP Response object contains detailed information about the response sent from a web server to the requester. It encompasses attributes and metadata that describe the response status, headers, body content, and other relevant information." ;
    ocsf:extends "object" ;
    ocsf:name "http_response" .

ocsf:IdentityAccessManagementEvent a owl:Class ;
    rdfs:label "Identity & Access Management" ;
    rdfs:subClassOf ocsf:BaseEvent,
        [ a owl:Restriction ;
            owl:onProperty ocsf:http_request ;
            owl:allValuesFrom ocsf:HTTPRequest ],
        [ a owl:Restriction ;
            owl:onProperty ocsf:src_endpoint ;
            owl:allValuesFrom ocsf:NetworkEndpoint ] ;
    dcterms:description "The Identity & Access Management event is a generic event that defines a set of attributes available in the access control events. As a generic event, it could be used to log events that are not otherwise defined by the IAM category." ;
    ocsf:category ocsf:IdentityAccessManagementEvent ;
    ocsf:extends "base_event" ;
    ocsf:name "iam" ;
    ocsf:profiles "host" .

ocsf:IdentityAccessManagementEventCategory a owl:Class ;
    rdfs:label "Identity & Access Management" ;
    rdfs:subClassOf ocsf:EventCategory ;
    d3f:definition "Identity & Access Management (IAM) events relate to the supervision of the system's authentication and access control model. Examples of such events are the success or failure of authentication, granting of authority, password change, entity change, privileged use etc." ;
    ocsf:category_name "iam" .

ocsf:IdentityProvider a owl:Class ;
    rdfs:label "Identity Provider" ;
    rdfs:subClassOf ocsf:Entity,
        [ a owl:Restriction ;
            owl:onProperty ocsf:name ;
            owl:allValuesFrom ocsf:string_t ],
        [ a owl:Restriction ;
            owl:onProperty ocsf:uid ;
            owl:allValuesFrom ocsf:string_t ] ;
    dcterms:description "The Identity Provider object contains detailed information about a provider responsible for creating, maintaining, and managing identity information while offering authentication services to applications. An Identity Provider (IdP) serves as a trusted authority that verifies the identity of users and issues authentication tokens or assertions to enable secure access to applications or services." ;
    ocsf:extends "_entity" ;
    ocsf:name "idp" .

ocsf:Image a owl:Class ;
    rdfs:label "Image" ;
    rdfs:subClassOf ocsf:Entity,
        [ a owl:Restriction ;
            owl:onProperty ocsf:labels ;
            owl:allValuesFrom ocsf:string_t ],
        [ a owl:Restriction ;
            owl:onProperty ocsf:name ;
            owl:allValuesFrom ocsf:string_t ],
        [ a owl:Restriction ;
            owl:onProperty ocsf:path ;
            owl:allValuesFrom ocsf:string_t ],
        [ a owl:Restriction ;
            owl:onProperty ocsf:tag ;
            owl:allValuesFrom ocsf:string_t ],
        [ a owl:Restriction ;
            owl:onProperty ocsf:uid ;
            owl:allValuesFrom ocsf:string_t ],
        [ a owl:Restriction ;
            owl:onProperty ocsf:uid ;
            owl:cardinality 1 ] ;
    dcterms:description "The Image object provides a description of a specific Virtual Machine (VM) or Container image. Defined by D3FEND <a target='_blank' href='https://d3fend.mitre.org/dao/artifact/d3f:ContainerImage/'>d3f:ContainerImage</a>." ;
    ocsf:constraints "{}" ;
    ocsf:extends "_entity" ;
    ocsf:name "image" .

ocsf:IncidentFindingEvent a owl:Class ;
    rdfs:label "Incident Finding" ;
    rdfs:subClassOf ocsf:BaseEvent,
        [ a owl:Restriction ;
            owl:onProperty ocsf:activity_id ;
            owl:allValuesFrom ocsf:integer_t ],
        [ a owl:Restriction ;
            owl:onProperty ocsf:activity_id ;
            owl:cardinality 1 ],
        [ a owl:Restriction ;
            owl:onProperty ocsf:activity_name ;
            owl:allValuesFrom ocsf:string_t ],
        [ a owl:Restriction ;
            owl:onProperty ocsf:assignee ;
            owl:allValuesFrom ocsf:User ],
        [ a owl:Restriction ;
            owl:onProperty ocsf:assignee_group ;
            owl:allValuesFrom ocsf:Group ],
        [ a owl:Restriction ;
            owl:onProperty ocsf:attacks ;
            owl:allValuesFrom ocsf:MITREATTCK ],
        [ a owl:Restriction ;
            owl:onProperty ocsf:comment ;
            owl:allValuesFrom ocsf:string_t ],
        [ a owl:Restriction ;
            owl:onProperty ocsf:confidence ;
            owl:allValuesFrom ocsf:string_t ],
        [ a owl:Restriction ;
            owl:onProperty ocsf:confidence_id ;
            owl:allValuesFrom ocsf:integer_t ],
        [ a owl:Restriction ;
            owl:onProperty ocsf:confidence_score ;
            owl:allValuesFrom ocsf:integer_t ],
        [ a owl:Restriction ;
            owl:onProperty ocsf:desc ;
            owl:allValuesFrom ocsf:string_t ],
        [ a owl:Restriction ;
            owl:onProperty ocsf:end_time ;
            owl:allValuesFrom ocsf:timestamp_t ],
        [ a owl:Restriction ;
            owl:onProperty ocsf:finding_info_list ;
            owl:allValuesFrom ocsf:FindingInformation ],
        [ a owl:Restriction ;
            owl:onProperty ocsf:finding_info_list ;
            owl:someValuesFrom ocsf:FindingInformation ],
        [ a owl:Restriction ;
            owl:onProperty ocsf:impact ;
            owl:allValuesFrom ocsf:string_t ],
        [ a owl:Restriction ;
            owl:onProperty ocsf:impact_id ;
            owl:allValuesFrom ocsf:integer_t ],
        [ a owl:Restriction ;
            owl:onProperty ocsf:impact_score ;
            owl:allValuesFrom ocsf:integer_t ],
        [ a owl:Restriction ;
            owl:onProperty ocsf:is_suspected_breach ;
            owl:allValuesFrom ocsf:boolean_t ],
        [ a owl:Restriction ;
            owl:onProperty ocsf:priority ;
            owl:allValuesFrom ocsf:string_t ],
        [ a owl:Restriction ;
            owl:onProperty ocsf:priority_id ;
            owl:allValuesFrom ocsf:integer_t ],
        [ a owl:Restriction ;
            owl:onProperty ocsf:src_url ;
            owl:allValuesFrom ocsf:url_t ],
        [ a owl:Restriction ;
            owl:onProperty ocsf:start_time ;
            owl:allValuesFrom ocsf:timestamp_t ],
        [ a owl:Restriction ;
            owl:onProperty ocsf:status ;
            owl:allValuesFrom ocsf:string_t ],
        [ a owl:Restriction ;
            owl:onProperty ocsf:status_id ;
            owl:allValuesFrom ocsf:integer_t ],
        [ a owl:Restriction ;
            owl:onProperty ocsf:status_id ;
            owl:cardinality 1 ],
        [ a owl:Restriction ;
            owl:onProperty ocsf:ticket ;
            owl:allValuesFrom ocsf:Ticket ],
        [ a owl:Restriction ;
            owl:onProperty ocsf:verdict ;
            owl:allValuesFrom ocsf:string_t ],
        [ a owl:Restriction ;
            owl:onProperty ocsf:verdict_id ;
            owl:allValuesFrom ocsf:integer_t ] ;
    dcterms:description "An Incident Finding reports the creation, update, or closure of security incidents as a result of detections and/or analytics." ;
    ocsf:constraints "{\"at_least_one\":[\"assignee\",\"assignee_group\"]}" ;
    ocsf:extends "base_event" ;
    ocsf:name "incident_finding" .

ocsf:JA4Fingerprint a owl:Class ;
    rdfs:label "JA4+ Fingerprint" ;
    rdfs:subClassOf ocsf:Object,
        [ a owl:Restriction ;
            owl:onProperty ocsf:section_a ;
            owl:allValuesFrom ocsf:string_t ],
        [ a owl:Restriction ;
            owl:onProperty ocsf:section_b ;
            owl:allValuesFrom ocsf:string_t ],
        [ a owl:Restriction ;
            owl:onProperty ocsf:section_c ;
            owl:allValuesFrom ocsf:string_t ],
        [ a owl:Restriction ;
            owl:onProperty ocsf:section_d ;
            owl:allValuesFrom ocsf:string_t ],
        [ a owl:Restriction ;
            owl:onProperty ocsf:type ;
            owl:allValuesFrom ocsf:string_t ],
        [ a owl:Restriction ;
            owl:onProperty ocsf:type_id ;
            owl:allValuesFrom ocsf:integer_t ],
        [ a owl:Restriction ;
            owl:onProperty ocsf:type_id ;
            owl:cardinality 1 ],
        [ a owl:Restriction ;
            owl:onProperty ocsf:value ;
            owl:allValuesFrom ocsf:string_t ],
        [ a owl:Restriction ;
            owl:onProperty ocsf:value ;
            owl:cardinality 1 ] ;
    dcterms:description "The JA4+ fingerprint object provides detailed fingerprint information about various aspects of network traffic which is both machine and human readable." ;
    ocsf:extends "object" ;
    ocsf:name "ja4_fingerprint" .

ocsf:Job a owl:Class ;
    rdfs:label "Job" ;
    rdfs:subClassOf ocsf:Object,
        [ a owl:Restriction ;
            owl:onProperty ocsf:cmd_line ;
            owl:allValuesFrom ocsf:string_t ],
        [ a owl:Restriction ;
            owl:onProperty ocsf:created_time ;
            owl:allValuesFrom ocsf:timestamp_t ],
        [ a owl:Restriction ;
            owl:onProperty ocsf:desc ;
            owl:allValuesFrom ocsf:string_t ],
        [ a owl:Restriction ;
            owl:onProperty ocsf:file ;
            owl:allValuesFrom ocsf:File ],
        [ a owl:Restriction ;
            owl:onProperty ocsf:file ;
            owl:someValuesFrom ocsf:File ],
        [ a owl:Restriction ;
            owl:onProperty ocsf:last_run_time ;
            owl:allValuesFrom ocsf:timestamp_t ],
        [ a owl:Restriction ;
            owl:onProperty ocsf:name ;
            owl:allValuesFrom ocsf:string_t ],
        [ a owl:Restriction ;
            owl:onProperty ocsf:name ;
            owl:cardinality 1 ],
        [ a owl:Restriction ;
            owl:onProperty ocsf:next_run_time ;
            owl:allValuesFrom ocsf:timestamp_t ],
        [ a owl:Restriction ;
            owl:onProperty ocsf:run_state ;
            owl:allValuesFrom ocsf:string_t ],
        [ a owl:Restriction ;
            owl:onProperty ocsf:run_state_id ;
            owl:allValuesFrom ocsf:integer_t ],
        [ a owl:Restriction ;
            owl:onProperty ocsf:user ;
            owl:allValuesFrom ocsf:User ] ;
    dcterms:description "The Job object provides information about a scheduled job or task, including its name, command line, and state. It encompasses attributes that describe the properties and status of the scheduled job." ;
    ocsf:extends "object" ;
    ocsf:name "job" .

ocsf:JobQueryEvent a owl:Class ;
    rdfs:label "Job Query" ;
    rdfs:subClassOf ocsf:DiscoveryResultEvent,
        [ a owl:Restriction ;
            owl:onProperty ocsf:job ;
            owl:allValuesFrom ocsf:Job ],
        [ a owl:Restriction ;
            owl:onProperty ocsf:job ;
            owl:someValuesFrom ocsf:Job ] ;
    dcterms:description "Job Query events report information about scheduled jobs." ;
    ocsf:extends "discovery_result" ;
    ocsf:name "job_query" .

ocsf:KBArticle a owl:Class ;
    rdfs:label "KB Article" ;
    rdfs:subClassOf ocsf:Object,
        [ a owl:Restriction ;
            owl:onProperty ocsf:avg_timespan ;
            owl:allValuesFrom ocsf:TimeSpan ],
        [ a owl:Restriction ;
            owl:onProperty ocsf:bulletin ;
            owl:allValuesFrom ocsf:string_t ],
        [ a owl:Restriction ;
            owl:onProperty ocsf:classification ;
            owl:allValuesFrom ocsf:string_t ],
        [ a owl:Restriction ;
            owl:onProperty ocsf:created_time ;
            owl:allValuesFrom ocsf:timestamp_t ],
        [ a owl:Restriction ;
            owl:onProperty ocsf:install_state ;
            owl:allValuesFrom ocsf:string_t ],
        [ a owl:Restriction ;
            owl:onProperty ocsf:install_state_id ;
            owl:allValuesFrom ocsf:integer_t ],
        [ a owl:Restriction ;
            owl:onProperty ocsf:is_superseded ;
            owl:allValuesFrom ocsf:boolean_t ],
        [ a owl:Restriction ;
            owl:onProperty ocsf:os ;
            owl:allValuesFrom ocsf:OperatingSystemOS ],
        [ a owl:Restriction ;
            owl:onProperty ocsf:product ;
            owl:allValuesFrom ocsf:Product ],
        [ a owl:Restriction ;
            owl:onProperty ocsf:severity ;
            owl:allValuesFrom ocsf:string_t ],
        [ a owl:Restriction ;
            owl:onProperty ocsf:size ;
            owl:allValuesFrom ocsf:long_t ],
        [ a owl:Restriction ;
            owl:onProperty ocsf:src_url ;
            owl:allValuesFrom ocsf:url_t ],
        [ a owl:Restriction ;
            owl:onProperty ocsf:title ;
            owl:allValuesFrom ocsf:string_t ],
        [ a owl:Restriction ;
            owl:onProperty ocsf:uid ;
            owl:allValuesFrom ocsf:string_t ],
        [ a owl:Restriction ;
            owl:onProperty ocsf:uid ;
            owl:cardinality 1 ] ;
    dcterms:description "The KB Article object contains metadata that describes the patch or update." ;
    ocsf:extends "object" ;
    ocsf:name "kb_article" .

ocsf:KernelActivityEvent a owl:Class ;
    rdfs:label "Kernel Activity" ;
    rdfs:subClassOf ocsf:SystemActivityEvent,
        [ a owl:Restriction ;
            owl:onProperty ocsf:activity_id ;
            owl:allValuesFrom ocsf:integer_t ],
        [ a owl:Restriction ;
            owl:onProperty ocsf:kernel ;
            owl:allValuesFrom ocsf:KernelResource ],
        [ a owl:Restriction ;
            owl:onProperty ocsf:kernel ;
            owl:someValuesFrom ocsf:KernelResource ] ;
    dcterms:description "Kernel Activity events report when an process creates, reads, or deletes a kernel resource." ;
    ocsf:extends "system" ;
    ocsf:name "kernel_activity" .

ocsf:KernelExtension a owl:Class ;
    rdfs:label "Kernel Extension" ;
    rdfs:subClassOf ocsf:Object,
        [ a owl:Restriction ;
            owl:onProperty ocsf:file ;
            owl:allValuesFrom ocsf:File ],
        [ a owl:Restriction ;
            owl:onProperty ocsf:file ;
            owl:someValuesFrom ocsf:File ] ;
    dcterms:description "The Kernel Extension object describes a kernel driver that has been loaded or unloaded into the operating system (OS) kernel. Defined by D3FEND <a target='_blank' href='https://d3fend.mitre.org/dao/artifact/d3f:KernelModule/'>d3f:KernelModule</a>." ;
    ocsf:extends "object" ;
    ocsf:name "kernel_driver" .

ocsf:KernelExtensionActivityEvent a owl:Class ;
    rdfs:label "Kernel Extension Activity" ;
    rdfs:subClassOf ocsf:SystemActivityEvent,
        [ a owl:Restriction ;
            owl:onProperty ocsf:activity_id ;
            owl:allValuesFrom ocsf:integer_t ],
        [ a owl:Restriction ;
            owl:onProperty ocsf:actor ;
            owl:allValuesFrom ocsf:Actor ],
        [ a owl:Restriction ;
            owl:onProperty ocsf:actor ;
            owl:someValuesFrom ocsf:Actor ],
        [ a owl:Restriction ;
            owl:onProperty ocsf:driver ;
            owl:allValuesFrom ocsf:KernelExtension ],
        [ a owl:Restriction ;
            owl:onProperty ocsf:driver ;
            owl:someValuesFrom ocsf:KernelExtension ] ;
    dcterms:description "Kernel Extension events report when a driver/extension is loaded or unloaded into the kernel" ;
    ocsf:extends "system" ;
    ocsf:name "kernel_extension" .

ocsf:KernelObjectQueryEvent a owl:Class ;
    rdfs:label "Kernel Object Query" ;
    rdfs:subClassOf ocsf:DiscoveryResultEvent,
        [ a owl:Restriction ;
            owl:onProperty ocsf:kernel ;
            owl:allValuesFrom ocsf:KernelResource ],
        [ a owl:Restriction ;
            owl:onProperty ocsf:kernel ;
            owl:someValuesFrom ocsf:KernelResource ] ;
    dcterms:description "Kernel Object Query events report information about discovered kernel resources." ;
    ocsf:extends "discovery_result" ;
    ocsf:name "kernel_object_query" .

ocsf:KernelResource a owl:Class ;
    rdfs:label "Kernel Resource" ;
    rdfs:subClassOf ocsf:Object,
        [ a owl:Restriction ;
            owl:onProperty ocsf:is_system ;
            owl:allValuesFrom ocsf:boolean_t ],
        [ a owl:Restriction ;
            owl:onProperty ocsf:name ;
            owl:allValuesFrom ocsf:string_t ],
        [ a owl:Restriction ;
            owl:onProperty ocsf:name ;
            owl:cardinality 1 ],
        [ a owl:Restriction ;
            owl:onProperty ocsf:path ;
            owl:allValuesFrom ocsf:string_t ],
        [ a owl:Restriction ;
            owl:onProperty ocsf:system_call ;
            owl:allValuesFrom ocsf:string_t ],
        [ a owl:Restriction ;
            owl:onProperty ocsf:type ;
            owl:allValuesFrom ocsf:string_t ],
        [ a owl:Restriction ;
            owl:onProperty ocsf:type_id ;
            owl:allValuesFrom ocsf:integer_t ],
        [ a owl:Restriction ;
            owl:onProperty ocsf:type_id ;
            owl:cardinality 1 ] ;
    dcterms:description "The Kernel Resource object provides information about a specific kernel resource, including its name and type. It describes essential attributes associated with a resource managed by the kernel of an operating system. Defined by D3FEND <a target='_blank' href='https://d3fend.mitre.org/dao/artifact/d3f:Kernel/'>d3f:Kernel</a>." ;
    ocsf:extends "object" ;
    ocsf:name "kernel" .

ocsf:KeyboardInformation a owl:Class ;
    rdfs:label "Keyboard Information" ;
    rdfs:subClassOf ocsf:Object,
        [ a owl:Restriction ;
            owl:onProperty ocsf:function_keys ;
            owl:allValuesFrom ocsf:integer_t ],
        [ a owl:Restriction ;
            owl:onProperty ocsf:ime ;
            owl:allValuesFrom ocsf:string_t ],
        [ a owl:Restriction ;
            owl:onProperty ocsf:keyboard_layout ;
            owl:allValuesFrom ocsf:string_t ],
        [ a owl:Restriction ;
            owl:onProperty ocsf:keyboard_subtype ;
            owl:allValuesFrom ocsf:integer_t ],
        [ a owl:Restriction ;
            owl:onProperty ocsf:keyboard_type ;
            owl:allValuesFrom ocsf:string_t ] ;
    dcterms:description "The Keyboard Information object contains details and attributes related to a computer or device keyboard. It encompasses information that describes the characteristics, capabilities, and configuration of the keyboard." ;
    ocsf:extends "object" ;
    ocsf:name "keyboard_info" .

ocsf:KillChainPhase a owl:Class ;
    rdfs:label "Kill Chain Phase" ;
    rdfs:subClassOf ocsf:Object,
        [ a owl:Restriction ;
            owl:onProperty ocsf:phase ;
            owl:allValuesFrom ocsf:string_t ],
        [ a owl:Restriction ;
            owl:onProperty ocsf:phase_id ;
            owl:allValuesFrom ocsf:integer_t ],
        [ a owl:Restriction ;
            owl:onProperty ocsf:phase_id ;
            owl:cardinality 1 ] ;
    dcterms:description "The Kill Chain Phase object represents a single phase of a cyber attack, including the initial reconnaissance and planning stages up to the final objective of the attacker. It provides a detailed description of each phase and its associated activities within the broader context of a cyber attack. See <a target='_blank' href='https://www.lockheedmartin.com/en-us/capabilities/cyber/cyber-kill-chain.html'>Cyber Kill Chain®</a>." ;
    ocsf:extends "object" ;
    ocsf:name "kill_chain_phase" .

ocsf:LDAPPerson a owl:Class ;
    rdfs:label "LDAP Person" ;
    rdfs:subClassOf ocsf:Object,
        [ a owl:Restriction ;
            owl:onProperty ocsf:cost_center ;
            owl:allValuesFrom ocsf:string_t ],
        [ a owl:Restriction ;
            owl:onProperty ocsf:created_time ;
            owl:allValuesFrom ocsf:timestamp_t ],
        [ a owl:Restriction ;
            owl:onProperty ocsf:deleted_time ;
            owl:allValuesFrom ocsf:timestamp_t ],
        [ a owl:Restriction ;
            owl:onProperty ocsf:email_addrs ;
            owl:allValuesFrom ocsf:email_t ],
        [ a owl:Restriction ;
            owl:onProperty ocsf:employee_uid ;
            owl:allValuesFrom ocsf:string_t ],
        [ a owl:Restriction ;
            owl:onProperty ocsf:given_name ;
            owl:allValuesFrom ocsf:string_t ],
        [ a owl:Restriction ;
            owl:onProperty ocsf:hire_time ;
            owl:allValuesFrom ocsf:timestamp_t ],
        [ a owl:Restriction ;
            owl:onProperty ocsf:job_title ;
            owl:allValuesFrom ocsf:string_t ],
        [ a owl:Restriction ;
            owl:onProperty ocsf:labels ;
            owl:allValuesFrom ocsf:string_t ],
        [ a owl:Restriction ;
            owl:onProperty ocsf:last_login_time ;
            owl:allValuesFrom ocsf:timestamp_t ],
        [ a owl:Restriction ;
            owl:onProperty ocsf:ldap_cn ;
            owl:allValuesFrom ocsf:string_t ],
        [ a owl:Restriction ;
            owl:onProperty ocsf:ldap_dn ;
            owl:allValuesFrom ocsf:string_t ],
        [ a owl:Restriction ;
            owl:onProperty ocsf:leave_time ;
            owl:allValuesFrom ocsf:timestamp_t ],
        [ a owl:Restriction ;
            owl:onProperty ocsf:location ;
            owl:allValuesFrom ocsf:GeoLocation ],
        [ a owl:Restriction ;
            owl:onProperty ocsf:manager ;
            owl:allValuesFrom ocsf:User ],
        [ a owl:Restriction ;
            owl:onProperty ocsf:modified_time ;
            owl:allValuesFrom ocsf:timestamp_t ],
        [ a owl:Restriction ;
            owl:onProperty ocsf:office_location ;
            owl:allValuesFrom ocsf:string_t ],
        [ a owl:Restriction ;
            owl:onProperty ocsf:surname ;
            owl:allValuesFrom ocsf:string_t ] ;
    dcterms:description "The additional LDAP attributes that describe a person." ;
    ocsf:extends "object" ;
    ocsf:name "ldap_person" .

ocsf:LoadBalancer a owl:Class ;
    rdfs:label "Load Balancer" ;
    rdfs:subClassOf ocsf:Entity,
        [ a owl:Restriction ;
            owl:onProperty ocsf:classification ;
            owl:allValuesFrom ocsf:string_t ],
        [ a owl:Restriction ;
            owl:onProperty ocsf:code ;
            owl:allValuesFrom ocsf:integer_t ],
        [ a owl:Restriction ;
            owl:onProperty ocsf:dst_endpoint ;
            owl:allValuesFrom ocsf:NetworkEndpoint ],
        [ a owl:Restriction ;
            owl:onProperty ocsf:endpoint_connections ;
            owl:allValuesFrom ocsf:EndpointConnection ],
        [ a owl:Restriction ;
            owl:onProperty ocsf:error_message ;
            owl:allValuesFrom ocsf:string_t ],
        [ a owl:Restriction ;
            owl:onProperty ocsf:ip ;
            owl:allValuesFrom ocsf:ip_t ],
        [ a owl:Restriction ;
            owl:onProperty ocsf:message ;
            owl:allValuesFrom ocsf:string_t ],
        [ a owl:Restriction ;
            owl:onProperty ocsf:metrics ;
            owl:allValuesFrom ocsf:Metric ],
        [ a owl:Restriction ;
            owl:onProperty ocsf:name ;
            owl:allValuesFrom ocsf:string_t ],
        [ a owl:Restriction ;
            owl:onProperty ocsf:status_detail ;
            owl:allValuesFrom ocsf:string_t ],
        [ a owl:Restriction ;
            owl:onProperty ocsf:uid ;
            owl:allValuesFrom ocsf:string_t ] ;
    dcterms:description "The load balancer object describes the load balancer entity and contains additional information regarding the distribution of traffic across a network." ;
    ocsf:extends "_entity" ;
    ocsf:name "load_balancer" .

ocsf:Logger a owl:Class ;
    rdfs:label "Logger" ;
    rdfs:subClassOf ocsf:Entity,
        [ a owl:Restriction ;
            owl:onProperty ocsf:device ;
            owl:allValuesFrom ocsf:Device ],
        [ a owl:Restriction ;
            owl:onProperty ocsf:log_level ;
            owl:allValuesFrom ocsf:string_t ],
        [ a owl:Restriction ;
            owl:onProperty ocsf:log_name ;
            owl:allValuesFrom ocsf:string_t ],
        [ a owl:Restriction ;
            owl:onProperty ocsf:log_provider ;
            owl:allValuesFrom ocsf:string_t ],
        [ a owl:Restriction ;
            owl:onProperty ocsf:log_version ;
            owl:allValuesFrom ocsf:string_t ],
        [ a owl:Restriction ;
            owl:onProperty ocsf:logged_time ;
            owl:allValuesFrom ocsf:timestamp_t ],
        [ a owl:Restriction ;
            owl:onProperty ocsf:name ;
            owl:allValuesFrom ocsf:string_t ],
        [ a owl:Restriction ;
            owl:onProperty ocsf:product ;
            owl:allValuesFrom ocsf:Product ],
        [ a owl:Restriction ;
            owl:onProperty ocsf:transmit_time ;
            owl:allValuesFrom ocsf:timestamp_t ],
        [ a owl:Restriction ;
            owl:onProperty ocsf:uid ;
            owl:allValuesFrom ocsf:string_t ],
        [ a owl:Restriction ;
            owl:onProperty ocsf:version ;
            owl:allValuesFrom ocsf:string_t ] ;
    dcterms:description "The Logger object represents the device and product where events are stored with times for receipt and transmission.  This may be at the source device where the event occurred, a remote scanning device, intermediate hops, or the ultimate destination." ;
    ocsf:extends "_entity" ;
    ocsf:name "logger" .

ocsf:Malware a owl:Class ;
    rdfs:label "Malware" ;
    rdfs:subClassOf ocsf:Entity,
        [ a owl:Restriction ;
            owl:onProperty ocsf:classification_ids ;
            owl:allValuesFrom ocsf:integer_t ],
        [ a owl:Restriction ;
            owl:onProperty ocsf:classification_ids ;
            owl:cardinality 1 ],
        [ a owl:Restriction ;
            owl:onProperty ocsf:classifications ;
            owl:allValuesFrom ocsf:string_t ],
        [ a owl:Restriction ;
            owl:onProperty ocsf:cves ;
            owl:allValuesFrom ocsf:CVE ],
        [ a owl:Restriction ;
            owl:onProperty ocsf:name ;
            owl:allValuesFrom ocsf:string_t ],
        [ a owl:Restriction ;
            owl:onProperty ocsf:path ;
            owl:allValuesFrom ocsf:string_t ],
        [ a owl:Restriction ;
            owl:onProperty ocsf:provider ;
            owl:allValuesFrom ocsf:string_t ],
        [ a owl:Restriction ;
            owl:onProperty ocsf:uid ;
            owl:allValuesFrom ocsf:string_t ] ;
    dcterms:description "The Malware object describes the classification of known malicious software, which is intentionally designed to cause damage to a computer, server, client, or computer network." ;
    ocsf:extends "_entity" ;
    ocsf:name "malware" .

ocsf:ManagedEntity a owl:Class ;
    rdfs:label "Managed Entity" ;
    rdfs:subClassOf ocsf:Entity,
        [ a owl:Restriction ;
            owl:onProperty ocsf:data ;
            owl:allValuesFrom ocsf:json_t ],
        [ a owl:Restriction ;
            owl:onProperty ocsf:device ;
            owl:allValuesFrom ocsf:Device ],
        [ a owl:Restriction ;
            owl:onProperty ocsf:email ;
            owl:allValuesFrom ocsf:Email ],
        [ a owl:Restriction ;
            owl:onProperty ocsf:group ;
            owl:allValuesFrom ocsf:Group ],
        [ a owl:Restriction ;
            owl:onProperty ocsf:name ;
            owl:allValuesFrom ocsf:string_t ],
        [ a owl:Restriction ;
            owl:onProperty ocsf:org ;
            owl:allValuesFrom ocsf:Organization ],
        [ a owl:Restriction ;
            owl:onProperty ocsf:policy ;
            owl:allValuesFrom ocsf:Policy ],
        [ a owl:Restriction ;
            owl:onProperty ocsf:type ;
            owl:allValuesFrom ocsf:string_t ],
        [ a owl:Restriction ;
            owl:onProperty ocsf:type_id ;
            owl:allValuesFrom ocsf:integer_t ],
        [ a owl:Restriction ;
            owl:onProperty ocsf:uid ;
            owl:allValuesFrom ocsf:string_t ],
        [ a owl:Restriction ;
            owl:onProperty ocsf:user ;
            owl:allValuesFrom ocsf:User ],
        [ a owl:Restriction ;
            owl:onProperty ocsf:version ;
            owl:allValuesFrom ocsf:string_t ] ;
    dcterms:description "The Managed Entity object describes the type and version of an entity, such as a user, device, or policy.  For types in the <code>type_id</code> enum list, an associated attribute should be populated.  If the type of entity is not in the <code>type_id</code> list, information can be put into the <code>data</code> attribute and the <code>type</code> attribute should identify the entity." ;
    ocsf:constraints "{\"at_least_one\":[\"name\",\"uid\",\"device\",\"group\",\"org\",\"policy\",\"user\"]}" ;
    ocsf:extends "_entity" ;
    ocsf:name "managed_entity" .

ocsf:MemoryActivityEvent a owl:Class ;
    rdfs:label "Memory Activity" ;
    rdfs:subClassOf ocsf:SystemActivityEvent,
        [ a owl:Restriction ;
            owl:onProperty ocsf:activity_id ;
            owl:allValuesFrom ocsf:integer_t ],
        [ a owl:Restriction ;
            owl:onProperty ocsf:actual_permissions ;
            owl:allValuesFrom ocsf:integer_t ],
        [ a owl:Restriction ;
            owl:onProperty ocsf:base_address ;
            owl:allValuesFrom ocsf:string_t ],
        [ a owl:Restriction ;
            owl:onProperty ocsf:process ;
            owl:allValuesFrom ocsf:Process ],
        [ a owl:Restriction ;
            owl:onProperty ocsf:process ;
            owl:someValuesFrom ocsf:Process ],
        [ a owl:Restriction ;
            owl:onProperty ocsf:requested_permissions ;
            owl:allValuesFrom ocsf:integer_t ],
        [ a owl:Restriction ;
            owl:onProperty ocsf:size ;
            owl:allValuesFrom ocsf:long_t ] ;
    dcterms:description "Memory Activity events report when a process has memory allocated, read/modified, or other manipulation activities - such as a buffer overflow or turning off data execution protection (DEP)." ;
    ocsf:extends "system" ;
    ocsf:name "memory_activity" .

ocsf:Metadata a owl:Class ;
    rdfs:label "Metadata" ;
    rdfs:subClassOf ocsf:Object,
        [ a owl:Restriction ;
            owl:onProperty ocsf:correlation_uid ;
            owl:allValuesFrom ocsf:string_t ],
        [ a owl:Restriction ;
            owl:onProperty ocsf:event_code ;
            owl:allValuesFrom ocsf:string_t ],
        [ a owl:Restriction ;
            owl:onProperty ocsf:extension ;
            owl:allValuesFrom ocsf:SchemaExtension ],
        [ a owl:Restriction ;
            owl:onProperty ocsf:extensions ;
            owl:allValuesFrom ocsf:SchemaExtension ],
        [ a owl:Restriction ;
            owl:onProperty ocsf:labels ;
            owl:allValuesFrom ocsf:string_t ],
        [ a owl:Restriction ;
            owl:onProperty ocsf:log_level ;
            owl:allValuesFrom ocsf:string_t ],
        [ a owl:Restriction ;
            owl:onProperty ocsf:log_name ;
            owl:allValuesFrom ocsf:string_t ],
        [ a owl:Restriction ;
            owl:onProperty ocsf:log_provider ;
            owl:allValuesFrom ocsf:string_t ],
        [ a owl:Restriction ;
            owl:onProperty ocsf:log_version ;
            owl:allValuesFrom ocsf:string_t ],
        [ a owl:Restriction ;
            owl:onProperty ocsf:logged_time ;
            owl:allValuesFrom ocsf:timestamp_t ],
        [ a owl:Restriction ;
            owl:onProperty ocsf:loggers ;
            owl:allValuesFrom ocsf:Logger ],
        [ a owl:Restriction ;
            owl:onProperty ocsf:modified_time ;
            owl:allValuesFrom ocsf:timestamp_t ],
        [ a owl:Restriction ;
            owl:onProperty ocsf:original_time ;
            owl:allValuesFrom ocsf:string_t ],
        [ a owl:Restriction ;
            owl:onProperty ocsf:processed_time ;
            owl:allValuesFrom ocsf:timestamp_t ],
        [ a owl:Restriction ;
            owl:onProperty ocsf:product ;
            owl:allValuesFrom ocsf:Product ],
        [ a owl:Restriction ;
            owl:onProperty ocsf:product ;
            owl:someValuesFrom ocsf:Product ],
        [ a owl:Restriction ;
            owl:onProperty ocsf:profiles ;
            owl:allValuesFrom ocsf:string_t ],
        [ a owl:Restriction ;
            owl:onProperty ocsf:sequence ;
            owl:allValuesFrom ocsf:integer_t ],
        [ a owl:Restriction ;
            owl:onProperty ocsf:tenant_uid ;
            owl:allValuesFrom ocsf:string_t ],
        [ a owl:Restriction ;
            owl:onProperty ocsf:uid ;
            owl:allValuesFrom ocsf:string_t ],
        [ a owl:Restriction ;
            owl:onProperty ocsf:version ;
            owl:allValuesFrom ocsf:string_t ],
        [ a owl:Restriction ;
            owl:onProperty ocsf:version ;
            owl:cardinality 1 ] ;
    dcterms:description "The Metadata object describes the metadata associated with the event. Defined by D3FEND <a target='_blank' href='https://d3fend.mitre.org/dao/artifact/d3f:Metadata/'>d3f:Metadata</a>." ;
    ocsf:extends "object" ;
    ocsf:name "metadata" ;
    ocsf:profiles "data_classification" .

ocsf:Metric a owl:Class ;
    rdfs:label "Metric" ;
    rdfs:subClassOf ocsf:Object,
        [ a owl:Restriction ;
            owl:onProperty ocsf:name ;
            owl:allValuesFrom ocsf:string_t ],
        [ a owl:Restriction ;
            owl:onProperty ocsf:name ;
            owl:cardinality 1 ],
        [ a owl:Restriction ;
            owl:onProperty ocsf:value ;
            owl:allValuesFrom ocsf:string_t ],
        [ a owl:Restriction ;
            owl:onProperty ocsf:value ;
            owl:cardinality 1 ] ;
    dcterms:description "The Metric object defines a simple name/value pair entity for a metric." ;
    ocsf:extends "object" ;
    ocsf:name "metric" .

ocsf:MITREATTCK a owl:Class ;
    rdfs:label "MITRE ATT&CK®" ;
    rdfs:subClassOf ocsf:Object,
        [ a owl:Restriction ;
            owl:onProperty ocsf:sub_technique ;
            owl:allValuesFrom ocsf:MITREATTCKSubTechnique ],
        [ a owl:Restriction ;
            owl:onProperty ocsf:tactic ;
            owl:allValuesFrom ocsf:MITREATTCKTactic ],
        [ a owl:Restriction ;
            owl:onProperty ocsf:tactics ;
            owl:allValuesFrom ocsf:MITREATTCKTactic ],
        [ a owl:Restriction ;
            owl:onProperty ocsf:technique ;
            owl:allValuesFrom ocsf:MITREATTCKTechnique ],
        [ a owl:Restriction ;
            owl:onProperty ocsf:version ;
            owl:allValuesFrom ocsf:string_t ] ;
    dcterms:description "The <a target='_blank' href='https://attack.mitre.org'>MITRE ATT&CK®</a> object describes the tactic, technique & sub-technique associated to an attack as defined in <a target='_blank' href='https://attack.mitre.org/wiki/ATT&CK_Matrix'>ATT&CK® Matrix</a>." ;
    ocsf:constraints "{\"at_least_one\":[\"tactic\",\"technique\",\"sub_technique\"]}" ;
    ocsf:extends "object" ;
    ocsf:name "attack" .

ocsf:MITREATTCKSubTechnique a owl:Class ;
    rdfs:label "MITRE ATT&CK® Sub Technique" ;
    rdfs:subClassOf ocsf:Entity,
        [ a owl:Restriction ;
            owl:onProperty ocsf:name ;
            owl:allValuesFrom ocsf:string_t ],
        [ a owl:Restriction ;
            owl:onProperty ocsf:src_url ;
            owl:allValuesFrom ocsf:url_t ],
        [ a owl:Restriction ;
            owl:onProperty ocsf:uid ;
            owl:allValuesFrom ocsf:string_t ] ;
    dcterms:description "The MITRE ATT&CK® Sub Technique object describes the sub technique ID and/or name associated to an attack, as defined by <a target='_blank' href='https://attack.mitre.org/wiki/ATT&CK_Matrix'>ATT&CK® Matrix</a>." ;
    ocsf:extends "_entity" ;
    ocsf:name "sub_technique" .

ocsf:MITREATTCKTactic a owl:Class ;
    rdfs:label "MITRE ATT&CK® Tactic" ;
    rdfs:subClassOf ocsf:Entity,
        [ a owl:Restriction ;
            owl:onProperty ocsf:name ;
            owl:allValuesFrom ocsf:string_t ],
        [ a owl:Restriction ;
            owl:onProperty ocsf:src_url ;
            owl:allValuesFrom ocsf:url_t ],
        [ a owl:Restriction ;
            owl:onProperty ocsf:uid ;
            owl:allValuesFrom ocsf:string_t ] ;
    dcterms:description "The MITRE ATT&CK® Tactic object describes the tactic ID and/or name that is associated to an attack, as defined by <a target='_blank' href='https://attack.mitre.org/wiki/ATT&CK_Matrix'>ATT&CK® Matrix</a>." ;
    ocsf:extends "_entity" ;
    ocsf:name "tactic" .

ocsf:MITREATTCKTechnique a owl:Class ;
    rdfs:label "MITRE ATT&CK® Technique" ;
    rdfs:subClassOf ocsf:Entity,
        [ a owl:Restriction ;
            owl:onProperty ocsf:name ;
            owl:allValuesFrom ocsf:string_t ],
        [ a owl:Restriction ;
            owl:onProperty ocsf:src_url ;
            owl:allValuesFrom ocsf:url_t ],
        [ a owl:Restriction ;
            owl:onProperty ocsf:uid ;
            owl:allValuesFrom ocsf:string_t ] ;
    dcterms:description "The MITRE ATT&CK® Technique object describes the technique ID and/or name associated to an attack, as defined by <a target='_blank' href='https://attack.mitre.org/wiki/ATT&CK_Matrix'>ATT&CK® Matrix</a>." ;
    ocsf:extends "_entity" ;
    ocsf:name "technique" .

ocsf:MITRED3FEND a owl:Class ;
    rdfs:label "MITRE D3FEND™" ;
    rdfs:subClassOf ocsf:Object,
        [ a owl:Restriction ;
            owl:onProperty ocsf:d3f_tactic ;
            owl:allValuesFrom ocsf:MITRED3FENDTactic ],
        [ a owl:Restriction ;
            owl:onProperty ocsf:d3f_technique ;
            owl:allValuesFrom ocsf:MITREDEFENDTechnique ],
        [ a owl:Restriction ;
            owl:onProperty ocsf:version ;
            owl:allValuesFrom ocsf:string_t ] ;
    dcterms:description "The <a target='_blank' href='https://d3fend.mitre.org'>MITRE D3FEND™</a> object describes the tactic, technique & sub-technique associated with a countermeasure as defined in <a target='_blank' href='https://d3fend.mitre.org/'>DEFEND Matrix<sup>TM</sup></a>." ;
    ocsf:constraints "{\"at_least_one\":[\"d3f_tactic\",\"d3f_technique\"]}" ;
    ocsf:extends "object" ;
    ocsf:name "d3fend" .

ocsf:MITRED3FENDTactic a owl:Class ;
    rdfs:label "MITRE D3FEND™ Tactic" ;
    rdfs:subClassOf ocsf:Entity,
        [ a owl:Restriction ;
            owl:onProperty ocsf:name ;
            owl:allValuesFrom ocsf:string_t ],
        [ a owl:Restriction ;
            owl:onProperty ocsf:src_url ;
            owl:allValuesFrom ocsf:url_t ] ;
    dcterms:description "The MITRE D3FEND™ Tactic object describes the tactic ID and/or name that is associated to an attack, as defined by <a target='_blank' href='https://d3fend.mitre.org'>D3FEND<sup>TM</sup> Matrix</a>." ;
    ocsf:extends "_entity" ;
    ocsf:name "d3f_tactic" .

ocsf:MITREDEFENDTechnique a owl:Class ;
    rdfs:label "MITRE DEFEND™ Technique" ;
    rdfs:subClassOf ocsf:Entity,
        [ a owl:Restriction ;
            owl:onProperty ocsf:name ;
            owl:allValuesFrom ocsf:string_t ],
        [ a owl:Restriction ;
            owl:onProperty ocsf:src_url ;
            owl:allValuesFrom ocsf:url_t ],
        [ a owl:Restriction ;
            owl:onProperty ocsf:uid ;
            owl:allValuesFrom ocsf:string_t ] ;
    dcterms:description "The MITRE DEFEND™ Technique object describes the leaf defensive technique ID and/or name associated to a countermeasure, as defined by <a target='_blank' href='https://d3fend.mitre.org'>D3FEND<sup>TM</sup> Matrix</a>." ;
    ocsf:extends "_entity" ;
    ocsf:name "d3f_technique" .

ocsf:Module a owl:Class ;
    rdfs:label "Module" ;
    rdfs:subClassOf ocsf:Object,
        [ a owl:Restriction ;
            owl:onProperty ocsf:base_address ;
            owl:allValuesFrom ocsf:string_t ],
        [ a owl:Restriction ;
            owl:onProperty ocsf:file ;
            owl:allValuesFrom ocsf:File ],
        [ a owl:Restriction ;
            owl:onProperty ocsf:function_name ;
            owl:allValuesFrom ocsf:string_t ],
        [ a owl:Restriction ;
            owl:onProperty ocsf:load_type ;
            owl:allValuesFrom ocsf:string_t ],
        [ a owl:Restriction ;
            owl:onProperty ocsf:load_type_id ;
            owl:allValuesFrom ocsf:integer_t ],
        [ a owl:Restriction ;
            owl:onProperty ocsf:load_type_id ;
            owl:cardinality 1 ],
        [ a owl:Restriction ;
            owl:onProperty ocsf:start_address ;
            owl:allValuesFrom ocsf:string_t ],
        [ a owl:Restriction ;
            owl:onProperty ocsf:type ;
            owl:allValuesFrom ocsf:string_t ] ;
    dcterms:description "The Module object describes the load attributes of a module." ;
    ocsf:extends "object" ;
    ocsf:name "module" .

ocsf:ModuleActivityEvent a owl:Class ;
    rdfs:label "Module Activity" ;
    rdfs:subClassOf ocsf:SystemActivityEvent,
        [ a owl:Restriction ;
            owl:onProperty ocsf:activity_id ;
            owl:allValuesFrom ocsf:integer_t ],
        [ a owl:Restriction ;
            owl:onProperty ocsf:actor ;
            owl:allValuesFrom ocsf:Actor ],
        [ a owl:Restriction ;
            owl:onProperty ocsf:actor ;
            owl:someValuesFrom ocsf:Actor ],
        [ a owl:Restriction ;
            owl:onProperty ocsf:module ;
            owl:allValuesFrom ocsf:Module ],
        [ a owl:Restriction ;
            owl:onProperty ocsf:module ;
            owl:someValuesFrom ocsf:Module ] ;
    dcterms:description "Module  Activity events report when a process loads or unloads the <code>module</code>." ;
    ocsf:extends "system" ;
    ocsf:name "module_activity" .

ocsf:ModuleQueryEvent a owl:Class ;
    rdfs:label "Module Query" ;
    rdfs:subClassOf ocsf:DiscoveryResultEvent,
        [ a owl:Restriction ;
            owl:onProperty ocsf:module ;
            owl:allValuesFrom ocsf:Module ],
        [ a owl:Restriction ;
            owl:onProperty ocsf:module ;
            owl:someValuesFrom ocsf:Module ],
        [ a owl:Restriction ;
            owl:onProperty ocsf:process ;
            owl:allValuesFrom ocsf:Process ],
        [ a owl:Restriction ;
            owl:onProperty ocsf:process ;
            owl:someValuesFrom ocsf:Process ] ;
    dcterms:description "Module Query events report information about loaded modules." ;
    ocsf:extends "discovery_result" ;
    ocsf:name "module_query" .

ocsf:NetworkActivityEvent a owl:Class ;
    rdfs:label "Network Activity" ;
    rdfs:subClassOf ocsf:NetworkEvent,
        [ a owl:Restriction ;
            owl:onProperty ocsf:url ;
            owl:allValuesFrom ocsf:UniformResourceLocator ] ;
    dcterms:description "Network Activity events report network connection and traffic activity." ;
    ocsf:category ocsf:NetworkEvent ;
    ocsf:extends "network" ;
    ocsf:name "network_activity" .

ocsf:NetworkActivityEventCategory a owl:Class ;
    rdfs:label "Network Activity" ;
    rdfs:subClassOf ocsf:EventCategory ;
    d3f:definition "Network Activity events." ;
    ocsf:category_name "network" .

ocsf:NetworkConnectionInformation a owl:Class ;
    rdfs:label "Network Connection Information" ;
    rdfs:subClassOf ocsf:Object,
        [ a owl:Restriction ;
            owl:onProperty ocsf:boundary ;
            owl:allValuesFrom ocsf:string_t ],
        [ a owl:Restriction ;
            owl:onProperty ocsf:boundary_id ;
            owl:allValuesFrom ocsf:integer_t ],
        [ a owl:Restriction ;
            owl:onProperty ocsf:direction ;
            owl:allValuesFrom ocsf:string_t ],
        [ a owl:Restriction ;
            owl:onProperty ocsf:direction_id ;
            owl:allValuesFrom ocsf:integer_t ],
        [ a owl:Restriction ;
            owl:onProperty ocsf:direction_id ;
            owl:cardinality 1 ],
        [ a owl:Restriction ;
            owl:onProperty ocsf:protocol_name ;
            owl:allValuesFrom ocsf:string_t ],
        [ a owl:Restriction ;
            owl:onProperty ocsf:protocol_num ;
            owl:allValuesFrom ocsf:integer_t ],
        [ a owl:Restriction ;
            owl:onProperty ocsf:protocol_ver ;
            owl:allValuesFrom ocsf:string_t ],
        [ a owl:Restriction ;
            owl:onProperty ocsf:protocol_ver_id ;
            owl:allValuesFrom ocsf:integer_t ],
        [ a owl:Restriction ;
            owl:onProperty ocsf:session ;
            owl:allValuesFrom ocsf:Session ],
        [ a owl:Restriction ;
            owl:onProperty ocsf:tcp_flags ;
            owl:allValuesFrom ocsf:integer_t ],
        [ a owl:Restriction ;
            owl:onProperty ocsf:uid ;
            owl:allValuesFrom ocsf:string_t ] ;
    dcterms:description "The Network Connection Information object describes characteristics of a network connection. Defined by D3FEND <a target='_blank' href='https://d3fend.mitre.org/dao/artifact/d3f:NetworkSession/'>d3f:NetworkSession</a>." ;
    ocsf:extends "object" ;
    ocsf:name "network_connection_info" .

ocsf:NetworkConnectionQueryEvent a owl:Class ;
    rdfs:label "Network Connection Query" ;
    rdfs:subClassOf ocsf:DiscoveryResultEvent,
        [ a owl:Restriction ;
            owl:onProperty ocsf:connection_info ;
            owl:allValuesFrom ocsf:NetworkConnectionInformation ],
        [ a owl:Restriction ;
            owl:onProperty ocsf:connection_info ;
            owl:someValuesFrom ocsf:NetworkConnectionInformation ],
        [ a owl:Restriction ;
            owl:onProperty ocsf:process ;
            owl:allValuesFrom ocsf:Process ],
        [ a owl:Restriction ;
            owl:onProperty ocsf:process ;
            owl:someValuesFrom ocsf:Process ],
        [ a owl:Restriction ;
            owl:onProperty ocsf:state ;
            owl:allValuesFrom ocsf:string_t ],
        [ a owl:Restriction ;
            owl:onProperty ocsf:state_id ;
            owl:allValuesFrom ocsf:integer_t ],
        [ a owl:Restriction ;
            owl:onProperty ocsf:state_id ;
            owl:cardinality 1 ] ;
    dcterms:description "Network Connection Query events report information about active network connections." ;
    ocsf:extends "discovery_result" ;
    ocsf:name "network_connection_query" .

ocsf:NetworkEndpoint a owl:Class ;
    rdfs:label "Network Endpoint" ;
    rdfs:subClassOf ocsf:Endpoint,
        [ a owl:Restriction ;
            owl:onProperty ocsf:autonomous_system ;
            owl:allValuesFrom ocsf:AutonomousSystem ],
        [ a owl:Restriction ;
            owl:onProperty ocsf:intermediate_ips ;
            owl:allValuesFrom ocsf:ip_t ],
        [ a owl:Restriction ;
            owl:onProperty ocsf:port ;
            owl:allValuesFrom ocsf:port_t ],
        [ a owl:Restriction ;
            owl:onProperty ocsf:proxy_endpoint ;
            owl:allValuesFrom ocsf:NetworkProxyEndpoint ],
        [ a owl:Restriction ;
            owl:onProperty ocsf:svc_name ;
            owl:allValuesFrom ocsf:string_t ],
        [ a owl:Restriction ;
            owl:onProperty ocsf:type ;
            owl:allValuesFrom ocsf:string_t ],
        [ a owl:Restriction ;
            owl:onProperty ocsf:type_id ;
            owl:allValuesFrom ocsf:integer_t ] ;
    dcterms:description "The Network Endpoint object describes characteristics of a network endpoint. These can be a source or destination of a network connection." ;
    ocsf:constraints "{\"at_least_one\":[\"ip\",\"uid\",\"name\",\"hostname\",\"svc_name\",\"instance_uid\",\"interface_uid\",\"interface_name\"]}" ;
    ocsf:extends "endpoint" ;
    ocsf:name "network_endpoint" .

ocsf:NetworkEvent a owl:Class ;
    rdfs:label "Network" ;
    rdfs:subClassOf ocsf:BaseEvent,
        [ a owl:Restriction ;
            owl:onProperty ocsf:app_name ;
            owl:allValuesFrom ocsf:string_t ],
        [ a owl:Restriction ;
            owl:onProperty ocsf:connection_info ;
            owl:allValuesFrom ocsf:NetworkConnectionInformation ],
        [ a owl:Restriction ;
            owl:onProperty ocsf:dst_endpoint ;
            owl:allValuesFrom ocsf:NetworkEndpoint ],
        [ a owl:Restriction ;
            owl:onProperty ocsf:dst_endpoint ;
            owl:someValuesFrom ocsf:NetworkEndpoint ],
        [ a owl:Restriction ;
            owl:onProperty ocsf:ja4_fingerprint_list ;
            owl:allValuesFrom ocsf:JA4Fingerprint ],
        [ a owl:Restriction ;
            owl:onProperty ocsf:proxy ;
            owl:allValuesFrom ocsf:NetworkProxyEndpoint ],
        [ a owl:Restriction ;
            owl:onProperty ocsf:src_endpoint ;
            owl:allValuesFrom ocsf:NetworkEndpoint ],
        [ a owl:Restriction ;
            owl:onProperty ocsf:tls ;
            owl:allValuesFrom ocsf:TransportLayerSecurityTLS ],
        [ a owl:Restriction ;
            owl:onProperty ocsf:traffic ;
            owl:allValuesFrom ocsf:NetworkTraffic ] ;
    dcterms:description "Network event is a generic event that defines a set of attributes available in the Network category." ;
    ocsf:category ocsf:NetworkEvent ;
    ocsf:extends "base_event" ;
    ocsf:name "network" ;
    ocsf:profiles "host",
        "load_balancer",
        "network_proxy",
        "security_control" .

ocsf:NetworkFileActivityEvent a owl:Class ;
    rdfs:label "Network File Activity" ;
    rdfs:subClassOf ocsf:NetworkEvent,
        [ a owl:Restriction ;
            owl:onProperty ocsf:activity_id ;
            owl:allValuesFrom ocsf:integer_t ],
        [ a owl:Restriction ;
            owl:onProperty ocsf:actor ;
            owl:allValuesFrom ocsf:Actor ],
        [ a owl:Restriction ;
            owl:onProperty ocsf:actor ;
            owl:someValuesFrom ocsf:Actor ],
        [ a owl:Restriction ;
            owl:onProperty ocsf:connection_info ;
            owl:allValuesFrom ocsf:NetworkConnectionInformation ],
        [ a owl:Restriction ;
            owl:onProperty ocsf:dst_endpoint ;
            owl:allValuesFrom ocsf:NetworkEndpoint ],
        [ a owl:Restriction ;
            owl:onProperty ocsf:expiration_time ;
            owl:allValuesFrom ocsf:timestamp_t ],
        [ a owl:Restriction ;
            owl:onProperty ocsf:file ;
            owl:allValuesFrom ocsf:File ],
        [ a owl:Restriction ;
            owl:onProperty ocsf:file ;
            owl:someValuesFrom ocsf:File ],
        [ a owl:Restriction ;
            owl:onProperty ocsf:src_endpoint ;
            owl:allValuesFrom ocsf:NetworkEndpoint ],
        [ a owl:Restriction ;
            owl:onProperty ocsf:src_endpoint ;
            owl:someValuesFrom ocsf:NetworkEndpoint ] ;
    dcterms:description "Network File Activity events report file activities traversing the network, including file storage services such as Box, MS OneDrive, or Google Drive." ;
    ocsf:category ocsf:NetworkEvent ;
    ocsf:extends "network" ;
    ocsf:name "network_file_activity" .

ocsf:NetworkInterface a owl:Class ;
    rdfs:label "Network Interface" ;
    rdfs:subClassOf ocsf:Entity,
        [ a owl:Restriction ;
            owl:onProperty ocsf:hostname ;
            owl:allValuesFrom ocsf:hostname_t ],
        [ a owl:Restriction ;
            owl:onProperty ocsf:ip ;
            owl:allValuesFrom ocsf:ip_t ],
        [ a owl:Restriction ;
            owl:onProperty ocsf:mac ;
            owl:allValuesFrom ocsf:mac_t ],
        [ a owl:Restriction ;
            owl:onProperty ocsf:name ;
            owl:allValuesFrom ocsf:string_t ],
        [ a owl:Restriction ;
            owl:onProperty ocsf:namespace ;
            owl:allValuesFrom ocsf:string_t ],
        [ a owl:Restriction ;
            owl:onProperty ocsf:subnet_prefix ;
            owl:allValuesFrom ocsf:integer_t ],
        [ a owl:Restriction ;
            owl:onProperty ocsf:type ;
            owl:allValuesFrom ocsf:string_t ],
        [ a owl:Restriction ;
            owl:onProperty ocsf:type_id ;
            owl:allValuesFrom ocsf:integer_t ],
        [ a owl:Restriction ;
            owl:onProperty ocsf:type_id ;
            owl:cardinality 1 ],
        [ a owl:Restriction ;
            owl:onProperty ocsf:uid ;
            owl:allValuesFrom ocsf:string_t ] ;
    dcterms:description "The Network Interface object describes the type and associated attributes of a network interface." ;
    ocsf:constraints "{\"at_least_one\":[\"ip\",\"mac\",\"name\",\"hostname\"]}" ;
    ocsf:extends "_entity" ;
    ocsf:name "network_interface" .

ocsf:NetworkProxyEndpoint a owl:Class ;
    rdfs:label "Network Proxy Endpoint" ;
    rdfs:subClassOf ocsf:NetworkEndpoint ;
    dcterms:description "The network proxy endpoint object describes a proxy server, which acts as an intermediary between a client requesting a resource and the server providing that resource.  Defined by D3FEND <a target='_blank' href='https://d3fend.mitre.org/dao/artifact/d3f:ProxyServer/'>d3f:ProxyServer</a>." ;
    ocsf:extends "network_endpoint" ;
    ocsf:name "network_proxy" .

ocsf:NetworkRemediationActivityEvent a owl:Class ;
    rdfs:label "Network Remediation Activity" ;
    rdfs:subClassOf ocsf:RemediationActivityEvent,
        [ a owl:Restriction ;
            owl:onProperty ocsf:connection_info ;
            owl:allValuesFrom ocsf:NetworkConnectionInformation ],
        [ a owl:Restriction ;
            owl:onProperty ocsf:connection_info ;
            owl:someValuesFrom ocsf:NetworkConnectionInformation ] ;
    dcterms:description "Network Remediation Activity events report on attempts at remediating computer networks. It follows the MITRE countermeasures defined by the D3FEND™ <a target='_blank' href='https://d3fend.mitre.org/'>Matrix</a>. Techniques and Sub-techniques will include Network, such as Network Isolation or Network Traffic Filtering." ;
    ocsf:extends "remediation_activity" ;
    ocsf:name "network_remediation_activity" .

ocsf:NetworksQueryEvent a owl:Class ;
    rdfs:label "Networks Query" ;
    rdfs:subClassOf ocsf:DiscoveryResultEvent,
        [ a owl:Restriction ;
            owl:onProperty ocsf:network_interfaces ;
            owl:allValuesFrom ocsf:NetworkInterface ],
        [ a owl:Restriction ;
            owl:onProperty ocsf:network_interfaces ;
            owl:someValuesFrom ocsf:NetworkInterface ] ;
    dcterms:description "Networks Query events report information about network adapters." ;
    ocsf:extends "discovery_result" ;
    ocsf:name "networks_query" .

ocsf:NetworkTraffic a owl:Class ;
    rdfs:label "Network Traffic" ;
    rdfs:subClassOf ocsf:Object,
        [ a owl:Restriction ;
            owl:onProperty ocsf:bytes ;
            owl:allValuesFrom ocsf:long_t ],
        [ a owl:Restriction ;
            owl:onProperty ocsf:bytes_in ;
            owl:allValuesFrom ocsf:long_t ],
        [ a owl:Restriction ;
            owl:onProperty ocsf:bytes_out ;
            owl:allValuesFrom ocsf:long_t ],
        [ a owl:Restriction ;
            owl:onProperty ocsf:chunks ;
            owl:allValuesFrom ocsf:long_t ],
        [ a owl:Restriction ;
            owl:onProperty ocsf:chunks_in ;
            owl:allValuesFrom ocsf:long_t ],
        [ a owl:Restriction ;
            owl:onProperty ocsf:chunks_out ;
            owl:allValuesFrom ocsf:long_t ],
        [ a owl:Restriction ;
            owl:onProperty ocsf:packets ;
            owl:allValuesFrom ocsf:long_t ],
        [ a owl:Restriction ;
            owl:onProperty ocsf:packets_in ;
            owl:allValuesFrom ocsf:long_t ],
        [ a owl:Restriction ;
            owl:onProperty ocsf:packets_out ;
            owl:allValuesFrom ocsf:long_t ] ;
    dcterms:description "The Network Traffic object describes characteristics of network traffic. Network traffic refers to data moving across a network at a given point of time. Defined by D3FEND <a target='_blank' href='https://d3fend.mitre.org/dao/artifact/d3f:NetworkTraffic/'>d3f:NetworkTraffic</a>." ;
    ocsf:extends "object" ;
    ocsf:name "network_traffic" .

ocsf:NTPActivityEvent a owl:Class ;
    rdfs:label "NTP Activity" ;
    rdfs:subClassOf ocsf:NetworkEvent,
        [ a owl:Restriction ;
            owl:onProperty ocsf:activity_id ;
            owl:allValuesFrom ocsf:integer_t ],
        [ a owl:Restriction ;
            owl:onProperty ocsf:delay ;
            owl:allValuesFrom ocsf:integer_t ],
        [ a owl:Restriction ;
            owl:onProperty ocsf:dispersion ;
            owl:allValuesFrom ocsf:integer_t ],
        [ a owl:Restriction ;
            owl:onProperty ocsf:precision ;
            owl:allValuesFrom ocsf:integer_t ],
        [ a owl:Restriction ;
            owl:onProperty ocsf:stratum ;
            owl:allValuesFrom ocsf:string_t ],
        [ a owl:Restriction ;
            owl:onProperty ocsf:stratum_id ;
            owl:allValuesFrom ocsf:integer_t ],
        [ a owl:Restriction ;
            owl:onProperty ocsf:version ;
            owl:allValuesFrom ocsf:string_t ],
        [ a owl:Restriction ;
            owl:onProperty ocsf:version ;
            owl:cardinality 1 ] ;
    dcterms:description "The Network Time Protocol (NTP) Activity events report instances of remote clients synchronizing their clocks with an NTP server, as observed on the network." ;
    ocsf:extends "network" ;
    ocsf:name "ntp_activity" .

ocsf:Object a owl:Class ;
    rdfs:label "Object" ;
    rdfs:subClassOf d3f:DigitalArtifact ;
    dcterms:description "An unordered collection of attributes. It defines a set of attributes available in all objects. It can be also used as a generic object to log objects that are not otherwise defined by the schema." ;
    ocsf:name "object" .

ocsf:Observable a owl:Class ;
    rdfs:label "Observable" ;
    rdfs:subClassOf ocsf:Object,
        [ a owl:Restriction ;
            owl:onProperty ocsf:name ;
            owl:allValuesFrom ocsf:string_t ],
        [ a owl:Restriction ;
            owl:onProperty ocsf:name ;
            owl:cardinality 1 ],
        [ a owl:Restriction ;
            owl:onProperty ocsf:reputation ;
            owl:allValuesFrom ocsf:Reputation ],
        [ a owl:Restriction ;
            owl:onProperty ocsf:type ;
            owl:allValuesFrom ocsf:string_t ],
        [ a owl:Restriction ;
            owl:onProperty ocsf:type_id ;
            owl:allValuesFrom ocsf:integer_t ],
        [ a owl:Restriction ;
            owl:onProperty ocsf:type_id ;
            owl:cardinality 1 ],
        [ a owl:Restriction ;
            owl:onProperty ocsf:value ;
            owl:allValuesFrom ocsf:string_t ] ;
    dcterms:description "The observable object is a pivot element that contains related information found in many places in the event." ;
    ocsf:extends "object" ;
    ocsf:name "observable" .

ocsf:OperatingSystemOS a owl:Class ;
    rdfs:label "Operating System (OS)" ;
    rdfs:subClassOf ocsf:Object,
        [ a owl:Restriction ;
            owl:onProperty ocsf:build ;
            owl:allValuesFrom ocsf:string_t ],
        [ a owl:Restriction ;
            owl:onProperty ocsf:country ;
            owl:allValuesFrom ocsf:string_t ],
        [ a owl:Restriction ;
            owl:onProperty ocsf:cpe_name ;
            owl:allValuesFrom ocsf:string_t ],
        [ a owl:Restriction ;
            owl:onProperty ocsf:cpu_bits ;
            owl:allValuesFrom ocsf:integer_t ],
        [ a owl:Restriction ;
            owl:onProperty ocsf:edition ;
            owl:allValuesFrom ocsf:string_t ],
        [ a owl:Restriction ;
            owl:onProperty ocsf:lang ;
            owl:allValuesFrom ocsf:string_t ],
        [ a owl:Restriction ;
            owl:onProperty ocsf:name ;
            owl:allValuesFrom ocsf:string_t ],
        [ a owl:Restriction ;
            owl:onProperty ocsf:name ;
            owl:cardinality 1 ],
        [ a owl:Restriction ;
            owl:onProperty ocsf:sp_name ;
            owl:allValuesFrom ocsf:string_t ],
        [ a owl:Restriction ;
            owl:onProperty ocsf:sp_ver ;
            owl:allValuesFrom ocsf:integer_t ],
        [ a owl:Restriction ;
            owl:onProperty ocsf:type ;
            owl:allValuesFrom ocsf:string_t ],
        [ a owl:Restriction ;
            owl:onProperty ocsf:type_id ;
            owl:allValuesFrom ocsf:integer_t ],
        [ a owl:Restriction ;
            owl:onProperty ocsf:type_id ;
            owl:cardinality 1 ],
        [ a owl:Restriction ;
            owl:onProperty ocsf:version ;
            owl:allValuesFrom ocsf:string_t ] ;
    dcterms:description "The Operating System (OS) object describes characteristics of an OS, such as Linux or Windows. Defined by D3FEND <a target='_blank' href='https://d3fend.mitre.org/dao/artifact/d3f:OperatingSystem/'>d3f:OperatingSystem</a>." ;
    ocsf:extends "object" ;
    ocsf:name "os" .

ocsf:OperatingSystemPatchStateEvent a owl:Class ;
    rdfs:label "Operating System Patch State" ;
    rdfs:subClassOf ocsf:DiscoveryEvent,
        [ a owl:Restriction ;
            owl:onProperty ocsf:device ;
            owl:allValuesFrom ocsf:Device ],
        [ a owl:Restriction ;
            owl:onProperty ocsf:device ;
            owl:someValuesFrom ocsf:Device ],
        [ a owl:Restriction ;
            owl:onProperty ocsf:kb_article_list ;
            owl:allValuesFrom ocsf:KBArticle ] ;
    dcterms:description "Operating System Patch State reports the installation of an OS patch to a device and any associated knowledgebase articles." ;
    ocsf:constraints "{\"at_least_one\":[\"device.os.sp_name\",\"device.os.sp_ver\",\"device.os.version\"]}" ;
    ocsf:extends "discovery" ;
    ocsf:name "patch_state" ;
    ocsf:profiles "host" .

ocsf:Organization a owl:Class ;
    rdfs:label "Organization" ;
    rdfs:subClassOf ocsf:Entity,
        [ a owl:Restriction ;
            owl:onProperty ocsf:name ;
            owl:allValuesFrom ocsf:string_t ],
        [ a owl:Restriction ;
            owl:onProperty ocsf:ou_name ;
            owl:allValuesFrom ocsf:string_t ],
        [ a owl:Restriction ;
            owl:onProperty ocsf:ou_uid ;
            owl:allValuesFrom ocsf:string_t ],
        [ a owl:Restriction ;
            owl:onProperty ocsf:uid ;
            owl:allValuesFrom ocsf:string_t ] ;
    dcterms:description "The Organization object describes characteristics of an organization or company and its division if any." ;
    ocsf:extends "_entity" ;
    ocsf:name "organization" .

ocsf:OSINT a owl:Class ;
    rdfs:label "OSINT" ;
    rdfs:subClassOf ocsf:Entity,
        [ a owl:Restriction ;
            owl:onProperty ocsf:answers ;
            owl:allValuesFrom ocsf:DNSAnswer ],
        [ a owl:Restriction ;
            owl:onProperty ocsf:attacks ;
            owl:allValuesFrom ocsf:MITREATTCK ],
        [ a owl:Restriction ;
            owl:onProperty ocsf:autonomous_system ;
            owl:allValuesFrom ocsf:AutonomousSystem ],
        [ a owl:Restriction ;
            owl:onProperty ocsf:comment ;
            owl:allValuesFrom ocsf:string_t ],
        [ a owl:Restriction ;
            owl:onProperty ocsf:confidence ;
            owl:allValuesFrom ocsf:string_t ],
        [ a owl:Restriction ;
            owl:onProperty ocsf:confidence_id ;
            owl:allValuesFrom ocsf:integer_t ],
        [ a owl:Restriction ;
            owl:onProperty ocsf:email ;
            owl:allValuesFrom ocsf:Email ],
        [ a owl:Restriction ;
            owl:onProperty ocsf:email_auth ;
            owl:allValuesFrom ocsf:EmailAuthentication ],
        [ a owl:Restriction ;
            owl:onProperty ocsf:kill_chain ;
            owl:allValuesFrom ocsf:KillChainPhase ],
        [ a owl:Restriction ;
            owl:onProperty ocsf:location ;
            owl:allValuesFrom ocsf:GeoLocation ],
        [ a owl:Restriction ;
            owl:onProperty ocsf:signatures ;
            owl:allValuesFrom ocsf:DigitalSignature ],
        [ a owl:Restriction ;
            owl:onProperty ocsf:src_url ;
            owl:allValuesFrom ocsf:url_t ],
        [ a owl:Restriction ;
            owl:onProperty ocsf:subdomains ;
            owl:allValuesFrom ocsf:string_t ],
        [ a owl:Restriction ;
            owl:onProperty ocsf:tlp ;
            owl:allValuesFrom ocsf:string_t ],
        [ a owl:Restriction ;
            owl:onProperty ocsf:type ;
            owl:allValuesFrom ocsf:string_t ],
        [ a owl:Restriction ;
            owl:onProperty ocsf:type_id ;
            owl:allValuesFrom ocsf:integer_t ],
        [ a owl:Restriction ;
            owl:onProperty ocsf:type_id ;
            owl:cardinality 1 ],
        [ a owl:Restriction ;
            owl:onProperty ocsf:value ;
            owl:allValuesFrom ocsf:string_t ],
        [ a owl:Restriction ;
            owl:onProperty ocsf:value ;
            owl:cardinality 1 ],
        [ a owl:Restriction ;
            owl:onProperty ocsf:vendor_name ;
            owl:allValuesFrom ocsf:string_t ],
        [ a owl:Restriction ;
            owl:onProperty ocsf:vulnerabilities ;
            owl:allValuesFrom ocsf:VulnerabilityDetails ],
        [ a owl:Restriction ;
            owl:onProperty ocsf:whois ;
            owl:allValuesFrom ocsf:WHOIS ] ;
    dcterms:description "The OSINT (Open Source Intelligence) object contains details related to an indicator such as the indicator itself, related indicators, geolocation, registrar information, subdomains, analyst commentary, and other contextual information. This information can be used to further enrich a detection or finding by providing decisioning support to other analysts and engineers." ;
    ocsf:extends "_entity" ;
    ocsf:name "osint" .

ocsf:OtherEventCategory a owl:Class ;
    rdfs:label "Other Event Category" ;
    rdfs:subClassOf ocsf:EventCategory ;
    dcterms:description "The OCSF category solely for ocsf:BaseEvent." ;
    ocsf:name "other" .

ocsf:PeripheralDevice a owl:Class ;
    rdfs:label "Peripheral Device" ;
    rdfs:subClassOf ocsf:Entity,
        [ a owl:Restriction ;
            owl:onProperty ocsf:class ;
            owl:allValuesFrom ocsf:string_t ],
        [ a owl:Restriction ;
            owl:onProperty ocsf:class ;
            owl:cardinality 1 ],
        [ a owl:Restriction ;
            owl:onProperty ocsf:model ;
            owl:allValuesFrom ocsf:string_t ],
        [ a owl:Restriction ;
            owl:onProperty ocsf:name ;
            owl:allValuesFrom ocsf:string_t ],
        [ a owl:Restriction ;
            owl:onProperty ocsf:name ;
            owl:cardinality 1 ],
        [ a owl:Restriction ;
            owl:onProperty ocsf:serial_number ;
            owl:allValuesFrom ocsf:string_t ],
        [ a owl:Restriction ;
            owl:onProperty ocsf:uid ;
            owl:allValuesFrom ocsf:string_t ],
        [ a owl:Restriction ;
            owl:onProperty ocsf:vendor_name ;
            owl:allValuesFrom ocsf:string_t ] ;
    dcterms:description "The peripheral device object describes the identity, vendor and model of a peripheral device." ;
    ocsf:extends "_entity" ;
    ocsf:name "peripheral_device" .

ocsf:PeripheralDeviceQueryEvent a owl:Class ;
    rdfs:label "Peripheral Device Query" ;
    rdfs:subClassOf ocsf:DiscoveryResultEvent,
        [ a owl:Restriction ;
            owl:onProperty ocsf:peripheral_device ;
            owl:allValuesFrom ocsf:PeripheralDevice ],
        [ a owl:Restriction ;
            owl:onProperty ocsf:peripheral_device ;
            owl:someValuesFrom ocsf:PeripheralDevice ] ;
    dcterms:description "Peripheral Device Query events report information about peripheral devices." ;
    ocsf:extends "discovery_result" ;
    ocsf:name "peripheral_device_query" .

ocsf:Policy a owl:Class ;
    rdfs:label "Policy" ;
    rdfs:subClassOf ocsf:Entity,
        [ a owl:Restriction ;
            owl:onProperty ocsf:desc ;
            owl:allValuesFrom ocsf:string_t ],
        [ a owl:Restriction ;
            owl:onProperty ocsf:group ;
            owl:allValuesFrom ocsf:Group ],
        [ a owl:Restriction ;
            owl:onProperty ocsf:is_applied ;
            owl:allValuesFrom ocsf:boolean_t ],
        [ a owl:Restriction ;
            owl:onProperty ocsf:name ;
            owl:allValuesFrom ocsf:string_t ],
        [ a owl:Restriction ;
            owl:onProperty ocsf:uid ;
            owl:allValuesFrom ocsf:string_t ],
        [ a owl:Restriction ;
            owl:onProperty ocsf:version ;
            owl:allValuesFrom ocsf:string_t ] ;
    dcterms:description "The Policy object describes the policies that are applicable. <p>Policy attributes provide traceability to the operational state of the security product at the time that the event was captured, facilitating forensics, troubleshooting, and policy tuning/adjustments.</p>" ;
    ocsf:extends "_entity" ;
    ocsf:name "policy" .

ocsf:Process a owl:Class ;
    rdfs:label "Process" ;
    rdfs:subClassOf ocsf:Entity,
        [ a owl:Restriction ;
            owl:onProperty ocsf:cmd_line ;
            owl:allValuesFrom ocsf:string_t ],
        [ a owl:Restriction ;
            owl:onProperty ocsf:created_time ;
            owl:allValuesFrom ocsf:timestamp_t ],
        [ a owl:Restriction ;
            owl:onProperty ocsf:file ;
            owl:allValuesFrom ocsf:File ],
        [ a owl:Restriction ;
            owl:onProperty ocsf:integrity ;
            owl:allValuesFrom ocsf:string_t ],
        [ a owl:Restriction ;
            owl:onProperty ocsf:integrity_id ;
            owl:allValuesFrom ocsf:integer_t ],
        [ a owl:Restriction ;
            owl:onProperty ocsf:lineage ;
            owl:allValuesFrom ocsf:string_t ],
        [ a owl:Restriction ;
            owl:onProperty ocsf:loaded_modules ;
            owl:allValuesFrom ocsf:string_t ],
        [ a owl:Restriction ;
            owl:onProperty ocsf:name ;
            owl:allValuesFrom ocsf:string_t ],
        [ a owl:Restriction ;
            owl:onProperty ocsf:parent_process ;
            owl:allValuesFrom ocsf:Process ],
        [ a owl:Restriction ;
            owl:onProperty ocsf:pid ;
            owl:allValuesFrom ocsf:integer_t ],
        [ a owl:Restriction ;
            owl:onProperty ocsf:sandbox ;
            owl:allValuesFrom ocsf:string_t ],
        [ a owl:Restriction ;
            owl:onProperty ocsf:session ;
            owl:allValuesFrom ocsf:Session ],
        [ a owl:Restriction ;
            owl:onProperty ocsf:terminated_time ;
            owl:allValuesFrom ocsf:timestamp_t ],
        [ a owl:Restriction ;
            owl:onProperty ocsf:tid ;
            owl:allValuesFrom ocsf:integer_t ],
        [ a owl:Restriction ;
            owl:onProperty ocsf:uid ;
            owl:allValuesFrom ocsf:string_t ],
        [ a owl:Restriction ;
            owl:onProperty ocsf:user ;
            owl:allValuesFrom ocsf:User ],
        [ a owl:Restriction ;
            owl:onProperty ocsf:xattributes ;
            owl:allValuesFrom ocsf:Object ] ;
    dcterms:description "The Process object describes a running instance of a launched program. Defined by D3FEND <a target='_blank' href='https://d3fend.mitre.org/dao/artifact/d3f:Process/'>d3f:Process</a>." ;
    ocsf:constraints "{\"at_least_one\":[\"pid\",\"uid\"]}" ;
    ocsf:extends "_entity" ;
    ocsf:name "process" ;
    ocsf:profiles "container" .

ocsf:ProcessActivityEvent a owl:Class ;
    rdfs:label "Process Activity" ;
    rdfs:subClassOf ocsf:SystemActivityEvent,
        [ a owl:Restriction ;
            owl:onProperty ocsf:activity_id ;
            owl:allValuesFrom ocsf:integer_t ],
        [ a owl:Restriction ;
            owl:onProperty ocsf:actor ;
            owl:allValuesFrom ocsf:Actor ],
        [ a owl:Restriction ;
            owl:onProperty ocsf:actual_permissions ;
            owl:allValuesFrom ocsf:integer_t ],
        [ a owl:Restriction ;
            owl:onProperty ocsf:exit_code ;
            owl:allValuesFrom ocsf:integer_t ],
        [ a owl:Restriction ;
            owl:onProperty ocsf:injection_type ;
            owl:allValuesFrom ocsf:string_t ],
        [ a owl:Restriction ;
            owl:onProperty ocsf:injection_type_id ;
            owl:allValuesFrom ocsf:integer_t ],
        [ a owl:Restriction ;
            owl:onProperty ocsf:module ;
            owl:allValuesFrom ocsf:Module ],
        [ a owl:Restriction ;
            owl:onProperty ocsf:process ;
            owl:allValuesFrom ocsf:Process ],
        [ a owl:Restriction ;
            owl:onProperty ocsf:process ;
            owl:someValuesFrom ocsf:Process ],
        [ a owl:Restriction ;
            owl:onProperty ocsf:requested_permissions ;
            owl:allValuesFrom ocsf:integer_t ] ;
    dcterms:description "Process Activity events report when a process launches, injects, opens or terminates another process, successful or otherwise." ;
    ocsf:extends "system" ;
    ocsf:name "process_activity" .

ocsf:ProcessQueryEvent a owl:Class ;
    rdfs:label "Process Query" ;
    rdfs:subClassOf ocsf:DiscoveryResultEvent,
        [ a owl:Restriction ;
            owl:onProperty ocsf:process ;
            owl:allValuesFrom ocsf:Process ],
        [ a owl:Restriction ;
            owl:onProperty ocsf:process ;
            owl:someValuesFrom ocsf:Process ] ;
    dcterms:description "Process Query events report information about running processes." ;
    ocsf:extends "discovery_result" ;
    ocsf:name "process_query" .

ocsf:ProcessRemediationActivityEvent a owl:Class ;
    rdfs:label "Process Remediation Activity" ;
    rdfs:subClassOf ocsf:RemediationActivityEvent,
        [ a owl:Restriction ;
            owl:onProperty ocsf:process ;
            owl:allValuesFrom ocsf:Process ],
        [ a owl:Restriction ;
            owl:onProperty ocsf:process ;
            owl:someValuesFrom ocsf:Process ] ;
    dcterms:description "Process Remediation Activity events report on attempts at remediating processes. It follows the MITRE countermeasures defined by the D3FEND™ <a target='_blank' href='https://d3fend.mitre.org/'>Matrix</a>. Sub-techniques will include Process, such as Process Termination or Kernel-based Process Isolation." ;
    ocsf:extends "remediation_activity" ;
    ocsf:name "process_remediation_activity" .

ocsf:Product a owl:Class ;
    rdfs:label "Product" ;
    rdfs:subClassOf ocsf:Entity,
        [ a owl:Restriction ;
            owl:onProperty ocsf:cpe_name ;
            owl:allValuesFrom ocsf:string_t ],
        [ a owl:Restriction ;
            owl:onProperty ocsf:feature ;
            owl:allValuesFrom ocsf:Feature ],
        [ a owl:Restriction ;
            owl:onProperty ocsf:lang ;
            owl:allValuesFrom ocsf:string_t ],
        [ a owl:Restriction ;
            owl:onProperty ocsf:name ;
            owl:allValuesFrom ocsf:string_t ],
        [ a owl:Restriction ;
            owl:onProperty ocsf:path ;
            owl:allValuesFrom ocsf:string_t ],
        [ a owl:Restriction ;
            owl:onProperty ocsf:uid ;
            owl:allValuesFrom ocsf:string_t ],
        [ a owl:Restriction ;
            owl:onProperty ocsf:url_string ;
            owl:allValuesFrom ocsf:url_t ],
        [ a owl:Restriction ;
            owl:onProperty ocsf:vendor_name ;
            owl:allValuesFrom ocsf:string_t ],
        [ a owl:Restriction ;
            owl:onProperty ocsf:vendor_name ;
            owl:cardinality 1 ],
        [ a owl:Restriction ;
            owl:onProperty ocsf:version ;
            owl:allValuesFrom ocsf:string_t ] ;
    dcterms:description "The Product object describes characteristics of a software product." ;
    ocsf:extends "_entity" ;
    ocsf:name "product" ;
    ocsf:profiles "data_classification" .

ocsf:QueryInformation a owl:Class ;
    rdfs:label "Query Information" ;
    rdfs:subClassOf ocsf:Entity,
        [ a owl:Restriction ;
            owl:onProperty ocsf:bytes ;
            owl:allValuesFrom ocsf:long_t ],
        [ a owl:Restriction ;
            owl:onProperty ocsf:data ;
            owl:allValuesFrom ocsf:json_t ],
        [ a owl:Restriction ;
            owl:onProperty ocsf:name ;
            owl:allValuesFrom ocsf:string_t ],
        [ a owl:Restriction ;
            owl:onProperty ocsf:query_string ;
            owl:allValuesFrom ocsf:string_t ],
        [ a owl:Restriction ;
            owl:onProperty ocsf:query_string ;
            owl:cardinality 1 ],
        [ a owl:Restriction ;
            owl:onProperty ocsf:query_time ;
            owl:allValuesFrom ocsf:timestamp_t ],
        [ a owl:Restriction ;
            owl:onProperty ocsf:uid ;
            owl:allValuesFrom ocsf:string_t ] ;
    dcterms:description "The query info object holds information related to data access within a datastore. To access, manipulate, delete, or retrieve data from a datastore, a query must be written using a specific syntax." ;
    ocsf:extends "_entity" ;
    ocsf:name "query_info" .

ocsf:RDPActivityEvent a owl:Class ;
    rdfs:label "RDP Activity" ;
    rdfs:subClassOf ocsf:NetworkEvent,
        [ a owl:Restriction ;
            owl:onProperty ocsf:activity_id ;
            owl:allValuesFrom ocsf:integer_t ],
        [ a owl:Restriction ;
            owl:onProperty ocsf:capabilities ;
            owl:allValuesFrom ocsf:string_t ],
        [ a owl:Restriction ;
            owl:onProperty ocsf:certificate_chain ;
            owl:allValuesFrom ocsf:string_t ],
        [ a owl:Restriction ;
            owl:onProperty ocsf:device ;
            owl:allValuesFrom ocsf:Device ],
        [ a owl:Restriction ;
            owl:onProperty ocsf:file ;
            owl:allValuesFrom ocsf:File ],
        [ a owl:Restriction ;
            owl:onProperty ocsf:identifier_cookie ;
            owl:allValuesFrom ocsf:string_t ],
        [ a owl:Restriction ;
            owl:onProperty ocsf:protocol_ver ;
            owl:allValuesFrom ocsf:string_t ],
        [ a owl:Restriction ;
            owl:onProperty ocsf:remote_display ;
            owl:allValuesFrom ocsf:Display ],
        [ a owl:Restriction ;
            owl:onProperty ocsf:request ;
            owl:allValuesFrom ocsf:RequestElements ],
        [ a owl:Restriction ;
            owl:onProperty ocsf:response ;
            owl:allValuesFrom ocsf:ResponseElements ] ;
    dcterms:description "Remote Desktop Protocol (RDP) Activity events report remote client connections to a server as seen on the network." ;
    ocsf:extends "network" ;
    ocsf:name "rdp_activity" .

ocsf:RelatedEvent a owl:Class ;
    rdfs:label "Related Event" ;
    rdfs:subClassOf ocsf:Object,
        [ a owl:Restriction ;
            owl:onProperty ocsf:attacks ;
            owl:allValuesFrom ocsf:MITREATTCK ],
        [ a owl:Restriction ;
            owl:onProperty ocsf:kill_chain ;
            owl:allValuesFrom ocsf:KillChainPhase ],
        [ a owl:Restriction ;
            owl:onProperty ocsf:observables ;
            owl:allValuesFrom ocsf:Observable ],
        [ a owl:Restriction ;
            owl:onProperty ocsf:product_uid ;
            owl:allValuesFrom ocsf:string_t ],
        [ a owl:Restriction ;
            owl:onProperty ocsf:type ;
            owl:allValuesFrom ocsf:string_t ],
        [ a owl:Restriction ;
            owl:onProperty ocsf:type_name ;
            owl:allValuesFrom ocsf:string_t ],
        [ a owl:Restriction ;
            owl:onProperty ocsf:type_uid ;
            owl:allValuesFrom ocsf:long_t ],
        [ a owl:Restriction ;
            owl:onProperty ocsf:uid ;
            owl:allValuesFrom ocsf:string_t ],
        [ a owl:Restriction ;
            owl:onProperty ocsf:uid ;
            owl:cardinality 1 ] ;
    dcterms:description "The Related Event object describes an OCSF event related to a finding." ;
    ocsf:extends "object" ;
    ocsf:name "related_event" .

ocsf:Remediation a owl:Class ;
    rdfs:label "Remediation" ;
    rdfs:subClassOf ocsf:Object,
        [ a owl:Restriction ;
            owl:onProperty ocsf:desc ;
            owl:allValuesFrom ocsf:string_t ],
        [ a owl:Restriction ;
            owl:onProperty ocsf:desc ;
            owl:cardinality 1 ],
        [ a owl:Restriction ;
            owl:onProperty ocsf:kb_article_list ;
            owl:allValuesFrom ocsf:KBArticle ],
        [ a owl:Restriction ;
            owl:onProperty ocsf:kb_articles ;
            owl:allValuesFrom ocsf:string_t ],
        [ a owl:Restriction ;
            owl:onProperty ocsf:references ;
            owl:allValuesFrom ocsf:string_t ] ;
    dcterms:description "The Remediation object describes the recommended remediation steps to address identified issue(s)." ;
    ocsf:extends "object" ;
    ocsf:name "remediation" .

ocsf:RemediationActivityEvent a owl:Class ;
    rdfs:label "Remediation Activity" ;
    rdfs:subClassOf ocsf:BaseEvent,
        [ a owl:Restriction ;
            owl:onProperty ocsf:activity_id ;
            owl:allValuesFrom ocsf:integer_t ],
        [ a owl:Restriction ;
            owl:onProperty ocsf:command_uid ;
            owl:allValuesFrom ocsf:string_t ],
        [ a owl:Restriction ;
            owl:onProperty ocsf:command_uid ;
            owl:cardinality 1 ],
        [ a owl:Restriction ;
            owl:onProperty ocsf:countermeasures ;
            owl:allValuesFrom ocsf:MITRED3FEND ],
        [ a owl:Restriction ;
            owl:onProperty ocsf:remediation ;
            owl:allValuesFrom ocsf:Remediation ],
        [ a owl:Restriction ;
            owl:onProperty ocsf:scan ;
            owl:allValuesFrom ocsf:Scan ],
        [ a owl:Restriction ;
            owl:onProperty ocsf:status_id ;
            owl:allValuesFrom ocsf:integer_t ] ;
    dcterms:description "Remediation Activity events report on attempts at remediating a compromised device or computer network. It follows the MITRE countermeasures defined by the D3FEND™ <a target='_blank' href='https://d3fend.mitre.org/'>Matrix</a>." ;
    ocsf:category ocsf:Remediation ;
    ocsf:extends "base_event" ;
    ocsf:name "remediation_activity" ;
    ocsf:profiles "host" .

ocsf:RemediationEventCategory a owl:Class ;
    rdfs:label "Remediation" ;
    rdfs:subClassOf ocsf:EventCategory ;
    d3f:definition "Remediation events report the results of remediation commands targeting files, processes, and other objects." ;
    ocsf:category_name "remediation" .

ocsf:Reputation a owl:Class ;
    rdfs:label "Reputation" ;
    rdfs:subClassOf ocsf:Object,
        [ a owl:Restriction ;
            owl:onProperty ocsf:base_score ;
            owl:allValuesFrom ocsf:float_t ],
        [ a owl:Restriction ;
            owl:onProperty ocsf:base_score ;
            owl:cardinality 1 ],
        [ a owl:Restriction ;
            owl:onProperty ocsf:provider ;
            owl:allValuesFrom ocsf:string_t ],
        [ a owl:Restriction ;
            owl:onProperty ocsf:score ;
            owl:allValuesFrom ocsf:string_t ],
        [ a owl:Restriction ;
            owl:onProperty ocsf:score_id ;
            owl:allValuesFrom ocsf:integer_t ],
        [ a owl:Restriction ;
            owl:onProperty ocsf:score_id ;
            owl:cardinality 1 ] ;
    dcterms:description "The Reputation object describes the reputation/risk score of an entity (e.g. device, user, domain)." ;
    ocsf:extends "object" ;
    ocsf:name "reputation" .

ocsf:RequestElements a owl:Class ;
    rdfs:label "Request Elements" ;
    rdfs:subClassOf ocsf:Object,
        [ a owl:Restriction ;
            owl:onProperty ocsf:containers ;
            owl:allValuesFrom ocsf:Container ],
        [ a owl:Restriction ;
            owl:onProperty ocsf:data ;
            owl:allValuesFrom ocsf:json_t ],
        [ a owl:Restriction ;
            owl:onProperty ocsf:flags ;
            owl:allValuesFrom ocsf:string_t ],
        [ a owl:Restriction ;
            owl:onProperty ocsf:uid ;
            owl:allValuesFrom ocsf:string_t ],
        [ a owl:Restriction ;
            owl:onProperty ocsf:uid ;
            owl:cardinality 1 ] ;
    dcterms:description "The Request Elements object describes characteristics of an API request." ;
    ocsf:extends "object" ;
    ocsf:name "request" .

ocsf:Resource a owl:Class ;
    rdfs:label "Resource" ;
    rdfs:subClassOf ocsf:Entity,
        [ a owl:Restriction ;
            owl:onProperty ocsf:data ;
            owl:allValuesFrom ocsf:json_t ],
        [ a owl:Restriction ;
            owl:onProperty ocsf:labels ;
            owl:allValuesFrom ocsf:string_t ],
        [ a owl:Restriction ;
            owl:onProperty ocsf:name ;
            owl:allValuesFrom ocsf:string_t ],
        [ a owl:Restriction ;
            owl:onProperty ocsf:type ;
            owl:allValuesFrom ocsf:string_t ],
        [ a owl:Restriction ;
            owl:onProperty ocsf:uid ;
            owl:allValuesFrom ocsf:string_t ] ;
    dcterms:description "The Resource object contains attributes that provide information about a particular resource. It serves as a base object, offering attributes that help identify and classify the resource effectively." ;
    ocsf:extends "_entity" ;
    ocsf:name "_resource" ;
    ocsf:profiles "data_classification" .

ocsf:ResourceDetails a owl:Class ;
    rdfs:label "Resource Details" ;
    rdfs:subClassOf ocsf:Resource,
        [ a owl:Restriction ;
            owl:onProperty ocsf:agent_list ;
            owl:allValuesFrom ocsf:Agent ],
        [ a owl:Restriction ;
            owl:onProperty ocsf:cloud_partition ;
            owl:allValuesFrom ocsf:string_t ],
        [ a owl:Restriction ;
            owl:onProperty ocsf:criticality ;
            owl:allValuesFrom ocsf:string_t ],
        [ a owl:Restriction ;
            owl:onProperty ocsf:group ;
            owl:allValuesFrom ocsf:Group ],
        [ a owl:Restriction ;
            owl:onProperty ocsf:namespace ;
            owl:allValuesFrom ocsf:string_t ],
        [ a owl:Restriction ;
            owl:onProperty ocsf:owner ;
            owl:allValuesFrom ocsf:User ],
        [ a owl:Restriction ;
            owl:onProperty ocsf:region ;
            owl:allValuesFrom ocsf:string_t ],
        [ a owl:Restriction ;
            owl:onProperty ocsf:version ;
            owl:allValuesFrom ocsf:string_t ] ;
    dcterms:description "The Resource Details object describes details about resources that were affected by the activity/event." ;
    ocsf:extends "_resource" ;
    ocsf:name "resource_details" ;
    ocsf:profiles "cloud" .

ocsf:ResponseElements a owl:Class ;
    rdfs:label "Response Elements" ;
    rdfs:subClassOf ocsf:Object,
        [ a owl:Restriction ;
            owl:onProperty ocsf:code ;
            owl:allValuesFrom ocsf:integer_t ],
        [ a owl:Restriction ;
            owl:onProperty ocsf:containers ;
            owl:allValuesFrom ocsf:Container ],
        [ a owl:Restriction ;
            owl:onProperty ocsf:data ;
            owl:allValuesFrom ocsf:json_t ],
        [ a owl:Restriction ;
            owl:onProperty ocsf:error ;
            owl:allValuesFrom ocsf:string_t ],
        [ a owl:Restriction ;
            owl:onProperty ocsf:error_message ;
            owl:allValuesFrom ocsf:string_t ],
        [ a owl:Restriction ;
            owl:onProperty ocsf:flags ;
            owl:allValuesFrom ocsf:string_t ],
        [ a owl:Restriction ;
            owl:onProperty ocsf:message ;
            owl:allValuesFrom ocsf:string_t ] ;
    dcterms:description "The Response Elements object describes characteristics of an API response." ;
    ocsf:extends "object" ;
    ocsf:name "response" .

ocsf:RPCInterface a owl:Class ;
    rdfs:label "RPC Interface" ;
    rdfs:subClassOf ocsf:Object,
        [ a owl:Restriction ;
            owl:onProperty ocsf:ack_reason ;
            owl:allValuesFrom ocsf:integer_t ],
        [ a owl:Restriction ;
            owl:onProperty ocsf:ack_result ;
            owl:allValuesFrom ocsf:integer_t ],
        [ a owl:Restriction ;
            owl:onProperty ocsf:uuid ;
            owl:allValuesFrom ocsf:uuid_t ],
        [ a owl:Restriction ;
            owl:onProperty ocsf:uuid ;
            owl:cardinality 1 ],
        [ a owl:Restriction ;
            owl:onProperty ocsf:version ;
            owl:allValuesFrom ocsf:string_t ],
        [ a owl:Restriction ;
            owl:onProperty ocsf:version ;
            owl:cardinality 1 ] ;
    dcterms:description "The RPC Interface represents the remote procedure call interface used in the DCE/RPC session." ;
    ocsf:extends "object" ;
    ocsf:name "rpc_interface" .

ocsf:Rule a owl:Class ;
    rdfs:label "Rule" ;
    rdfs:subClassOf ocsf:Entity,
        [ a owl:Restriction ;
            owl:onProperty ocsf:category ;
            owl:allValuesFrom ocsf:string_t ],
        [ a owl:Restriction ;
            owl:onProperty ocsf:desc ;
            owl:allValuesFrom ocsf:string_t ],
        [ a owl:Restriction ;
            owl:onProperty ocsf:name ;
            owl:allValuesFrom ocsf:string_t ],
        [ a owl:Restriction ;
            owl:onProperty ocsf:type ;
            owl:allValuesFrom ocsf:string_t ],
        [ a owl:Restriction ;
            owl:onProperty ocsf:uid ;
            owl:allValuesFrom ocsf:string_t ],
        [ a owl:Restriction ;
            owl:onProperty ocsf:version ;
            owl:allValuesFrom ocsf:string_t ] ;
    dcterms:description "The Rule object describes characteristics of a rule associated with a policy or an event." ;
    ocsf:extends "_entity" ;
    ocsf:name "rule" .

ocsf:Scan a owl:Class ;
    rdfs:label "Scan" ;
    rdfs:subClassOf ocsf:Entity,
        [ a owl:Restriction ;
            owl:onProperty ocsf:name ;
            owl:allValuesFrom ocsf:string_t ],
        [ a owl:Restriction ;
            owl:onProperty ocsf:type ;
            owl:allValuesFrom ocsf:string_t ],
        [ a owl:Restriction ;
            owl:onProperty ocsf:type_id ;
            owl:allValuesFrom ocsf:integer_t ],
        [ a owl:Restriction ;
            owl:onProperty ocsf:type_id ;
            owl:cardinality 1 ],
        [ a owl:Restriction ;
            owl:onProperty ocsf:uid ;
            owl:allValuesFrom ocsf:string_t ] ;
    dcterms:description "The Scan object describes characteristics of a proactive scan." ;
    ocsf:extends "_entity" ;
    ocsf:name "scan" .

ocsf:ScanActivityEvent a owl:Class ;
    rdfs:label "Scan Activity" ;
    rdfs:subClassOf ocsf:BaseEvent,
        [ a owl:Restriction ;
            owl:onProperty ocsf:activity_id ;
            owl:allValuesFrom ocsf:integer_t ],
        [ a owl:Restriction ;
            owl:onProperty ocsf:command_uid ;
            owl:allValuesFrom ocsf:string_t ],
        [ a owl:Restriction ;
            owl:onProperty ocsf:duration ;
            owl:allValuesFrom ocsf:long_t ],
        [ a owl:Restriction ;
            owl:onProperty ocsf:end_time ;
            owl:allValuesFrom ocsf:timestamp_t ],
        [ a owl:Restriction ;
            owl:onProperty ocsf:num_detections ;
            owl:allValuesFrom ocsf:integer_t ],
        [ a owl:Restriction ;
            owl:onProperty ocsf:num_files ;
            owl:allValuesFrom ocsf:integer_t ],
        [ a owl:Restriction ;
            owl:onProperty ocsf:num_folders ;
            owl:allValuesFrom ocsf:integer_t ],
        [ a owl:Restriction ;
            owl:onProperty ocsf:num_network_items ;
            owl:allValuesFrom ocsf:integer_t ],
        [ a owl:Restriction ;
            owl:onProperty ocsf:num_processes ;
            owl:allValuesFrom ocsf:integer_t ],
        [ a owl:Restriction ;
            owl:onProperty ocsf:num_registry_items ;
            owl:allValuesFrom ocsf:integer_t ],
        [ a owl:Restriction ;
            owl:onProperty ocsf:num_resolutions ;
            owl:allValuesFrom ocsf:integer_t ],
        [ a owl:Restriction ;
            owl:onProperty ocsf:num_skipped_items ;
            owl:allValuesFrom ocsf:integer_t ],
        [ a owl:Restriction ;
            owl:onProperty ocsf:num_trusted_items ;
            owl:allValuesFrom ocsf:integer_t ],
        [ a owl:Restriction ;
            owl:onProperty ocsf:policy ;
            owl:allValuesFrom ocsf:Policy ],
        [ a owl:Restriction ;
            owl:onProperty ocsf:scan ;
            owl:allValuesFrom ocsf:Scan ],
        [ a owl:Restriction ;
            owl:onProperty ocsf:scan ;
            owl:someValuesFrom ocsf:Scan ],
        [ a owl:Restriction ;
            owl:onProperty ocsf:schedule_uid ;
            owl:allValuesFrom ocsf:string_t ],
        [ a owl:Restriction ;
            owl:onProperty ocsf:start_time ;
            owl:allValuesFrom ocsf:timestamp_t ],
        [ a owl:Restriction ;
            owl:onProperty ocsf:total ;
            owl:allValuesFrom ocsf:integer_t ] ;
    dcterms:description "Scan events report the start, completion, and results of a scan job. The scan event includes the number of items that were scanned and the number of detections that were resolved." ;
    ocsf:category ocsf:ApplicationActivityEvent ;
    ocsf:extends "base_event" ;
    ocsf:name "scan_activity" ;
    ocsf:profiles "host" .

ocsf:ScheduledJobActivityEvent a owl:Class ;
    rdfs:label "Scheduled Job Activity" ;
    rdfs:subClassOf ocsf:SystemActivityEvent,
        [ a owl:Restriction ;
            owl:onProperty ocsf:activity_id ;
            owl:allValuesFrom ocsf:integer_t ],
        [ a owl:Restriction ;
            owl:onProperty ocsf:actor ;
            owl:allValuesFrom ocsf:Actor ],
        [ a owl:Restriction ;
            owl:onProperty ocsf:job ;
            owl:allValuesFrom ocsf:Job ],
        [ a owl:Restriction ;
            owl:onProperty ocsf:job ;
            owl:someValuesFrom ocsf:Job ] ;
    dcterms:description "Scheduled Job Activity events report activities related to scheduled jobs or tasks." ;
    ocsf:extends "system" ;
    ocsf:name "scheduled_job_activity" .

ocsf:SchemaExtension a owl:Class ;
    rdfs:label "Schema Extension" ;
    rdfs:subClassOf ocsf:Entity,
        [ a owl:Restriction ;
            owl:onProperty ocsf:name ;
            owl:allValuesFrom ocsf:string_t ],
        [ a owl:Restriction ;
            owl:onProperty ocsf:name ;
            owl:cardinality 1 ],
        [ a owl:Restriction ;
            owl:onProperty ocsf:uid ;
            owl:allValuesFrom ocsf:string_t ],
        [ a owl:Restriction ;
            owl:onProperty ocsf:uid ;
            owl:cardinality 1 ],
        [ a owl:Restriction ;
            owl:onProperty ocsf:version ;
            owl:allValuesFrom ocsf:string_t ],
        [ a owl:Restriction ;
            owl:onProperty ocsf:version ;
            owl:cardinality 1 ] ;
    dcterms:description "The OCSF Schema Extension object provides detailed information about the schema extension used to construct the event. The schema extensions are registered in the <a target='_blank' href='https://github.com/ocsf/ocsf-schema/blob/main/extensions.md'>extensions.md</a> file." ;
    ocsf:constraints "{}" ;
    ocsf:extends "_entity" ;
    ocsf:name "extension" .

ocsf:SecurityFindingEvent a owl:Class ;
    rdfs:label "Security Finding" ;
    rdfs:subClassOf ocsf:BaseEvent,
        [ a owl:Restriction ;
            owl:onProperty ocsf:activity_id ;
            owl:allValuesFrom ocsf:integer_t ],
        [ a owl:Restriction ;
            owl:onProperty ocsf:analytic ;
            owl:allValuesFrom ocsf:Analytic ],
        [ a owl:Restriction ;
            owl:onProperty ocsf:attacks ;
            owl:allValuesFrom ocsf:MITREATTCK ],
        [ a owl:Restriction ;
            owl:onProperty ocsf:cis_csc ;
            owl:allValuesFrom ocsf:CISCSC ],
        [ a owl:Restriction ;
            owl:onProperty ocsf:compliance ;
            owl:allValuesFrom ocsf:Compliance ],
        [ a owl:Restriction ;
            owl:onProperty ocsf:confidence ;
            owl:allValuesFrom ocsf:string_t ],
        [ a owl:Restriction ;
            owl:onProperty ocsf:confidence_id ;
            owl:allValuesFrom ocsf:integer_t ],
        [ a owl:Restriction ;
            owl:onProperty ocsf:confidence_score ;
            owl:allValuesFrom ocsf:integer_t ],
        [ a owl:Restriction ;
            owl:onProperty ocsf:data_sources ;
            owl:allValuesFrom ocsf:string_t ],
        [ a owl:Restriction ;
            owl:onProperty ocsf:evidence ;
            owl:allValuesFrom ocsf:json_t ],
        [ a owl:Restriction ;
            owl:onProperty ocsf:finding ;
            owl:allValuesFrom ocsf:Finding ],
        [ a owl:Restriction ;
            owl:onProperty ocsf:finding ;
            owl:allValuesFrom ocsf:FindingEvent ],
        [ a owl:Restriction ;
            owl:onProperty ocsf:finding ;
            owl:someValuesFrom ocsf:Finding ],
        [ a owl:Restriction ;
            owl:onProperty ocsf:finding ;
            owl:someValuesFrom ocsf:FindingEvent ],
        [ a owl:Restriction ;
            owl:onProperty ocsf:impact ;
            owl:allValuesFrom ocsf:string_t ],
        [ a owl:Restriction ;
            owl:onProperty ocsf:impact_id ;
            owl:allValuesFrom ocsf:integer_t ],
        [ a owl:Restriction ;
            owl:onProperty ocsf:impact_score ;
            owl:allValuesFrom ocsf:integer_t ],
        [ a owl:Restriction ;
            owl:onProperty ocsf:kill_chain ;
            owl:allValuesFrom ocsf:KillChainPhase ],
        [ a owl:Restriction ;
            owl:onProperty ocsf:malware ;
            owl:allValuesFrom ocsf:Malware ],
        [ a owl:Restriction ;
            owl:onProperty ocsf:nist ;
            owl:allValuesFrom ocsf:string_t ],
        [ a owl:Restriction ;
            owl:onProperty ocsf:process ;
            owl:allValuesFrom ocsf:Process ],
        [ a owl:Restriction ;
            owl:onProperty ocsf:resources ;
            owl:allValuesFrom ocsf:ResourceDetails ],
        [ a owl:Restriction ;
            owl:onProperty ocsf:risk_level ;
            owl:allValuesFrom ocsf:string_t ],
        [ a owl:Restriction ;
            owl:onProperty ocsf:risk_level_id ;
            owl:allValuesFrom ocsf:integer_t ],
        [ a owl:Restriction ;
            owl:onProperty ocsf:risk_score ;
            owl:allValuesFrom ocsf:integer_t ],
        [ a owl:Restriction ;
            owl:onProperty ocsf:state ;
            owl:allValuesFrom ocsf:string_t ],
        [ a owl:Restriction ;
            owl:onProperty ocsf:state_id ;
            owl:allValuesFrom ocsf:integer_t ],
        [ a owl:Restriction ;
            owl:onProperty ocsf:state_id ;
            owl:cardinality 1 ],
        [ a owl:Restriction ;
            owl:onProperty ocsf:vulnerabilities ;
            owl:allValuesFrom ocsf:VulnerabilityDetails ] ;
    dcterms:description "Security Finding events describe findings, detections, anomalies, alerts and/or actions performed by security products" ;
    ocsf:extends "base_event" ;
    ocsf:name "security_finding" .

ocsf:Service a owl:Class ;
    rdfs:label "Service" ;
    rdfs:subClassOf ocsf:Entity,
        [ a owl:Restriction ;
            owl:onProperty ocsf:labels ;
            owl:allValuesFrom ocsf:string_t ],
        [ a owl:Restriction ;
            owl:onProperty ocsf:name ;
            owl:allValuesFrom ocsf:string_t ],
        [ a owl:Restriction ;
            owl:onProperty ocsf:uid ;
            owl:allValuesFrom ocsf:string_t ],
        [ a owl:Restriction ;
            owl:onProperty ocsf:version ;
            owl:allValuesFrom ocsf:string_t ] ;
    dcterms:description "The Service object describes characteristics of a service, <code> e.g. AWS EC2. </code>" ;
    ocsf:extends "_entity" ;
    ocsf:name "service" .

ocsf:ServiceQueryEvent a owl:Class ;
    rdfs:label "Service Query" ;
    rdfs:subClassOf ocsf:DiscoveryResultEvent,
        [ a owl:Restriction ;
            owl:onProperty ocsf:service ;
            owl:allValuesFrom ocsf:Service ],
        [ a owl:Restriction ;
            owl:onProperty ocsf:service ;
            owl:someValuesFrom ocsf:Service ] ;
    dcterms:description "Service Query events report information about running services." ;
    ocsf:extends "discovery_result" ;
    ocsf:name "service_query" .

ocsf:Session a owl:Class ;
    rdfs:label "Session" ;
    rdfs:subClassOf ocsf:Object,
        [ a owl:Restriction ;
            owl:onProperty ocsf:count ;
            owl:allValuesFrom ocsf:integer_t ],
        [ a owl:Restriction ;
            owl:onProperty ocsf:created_time ;
            owl:allValuesFrom ocsf:timestamp_t ],
        [ a owl:Restriction ;
            owl:onProperty ocsf:credential_uid ;
            owl:allValuesFrom ocsf:string_t ],
        [ a owl:Restriction ;
            owl:onProperty ocsf:expiration_reason ;
            owl:allValuesFrom ocsf:string_t ],
        [ a owl:Restriction ;
            owl:onProperty ocsf:expiration_time ;
            owl:allValuesFrom ocsf:timestamp_t ],
        [ a owl:Restriction ;
            owl:onProperty ocsf:is_mfa ;
            owl:allValuesFrom ocsf:boolean_t ],
        [ a owl:Restriction ;
            owl:onProperty ocsf:is_remote ;
            owl:allValuesFrom ocsf:boolean_t ],
        [ a owl:Restriction ;
            owl:onProperty ocsf:is_vpn ;
            owl:allValuesFrom ocsf:boolean_t ],
        [ a owl:Restriction ;
            owl:onProperty ocsf:issuer ;
            owl:allValuesFrom ocsf:string_t ],
        [ a owl:Restriction ;
            owl:onProperty ocsf:terminal ;
            owl:allValuesFrom ocsf:string_t ],
        [ a owl:Restriction ;
            owl:onProperty ocsf:uid ;
            owl:allValuesFrom ocsf:string_t ],
        [ a owl:Restriction ;
            owl:onProperty ocsf:uid_alt ;
            owl:allValuesFrom ocsf:string_t ],
        [ a owl:Restriction ;
            owl:onProperty ocsf:uuid ;
            owl:allValuesFrom ocsf:uuid_t ] ;
    dcterms:description "The Session object describes details about an authenticated session. e.g. Session Creation Time, Session Issuer. Defined by D3FEND <a target='_blank' href='https://d3fend.mitre.org/dao/artifact/d3f:Session/'>d3f:Session</a>." ;
    ocsf:extends "object" ;
    ocsf:name "session" .

ocsf:SMBActivityEvent a owl:Class ;
    rdfs:label "SMB Activity" ;
    rdfs:subClassOf ocsf:NetworkEvent,
        [ a owl:Restriction ;
            owl:onProperty ocsf:activity_id ;
            owl:allValuesFrom ocsf:integer_t ],
        [ a owl:Restriction ;
            owl:onProperty ocsf:client_dialects ;
            owl:allValuesFrom ocsf:string_t ],
        [ a owl:Restriction ;
            owl:onProperty ocsf:command ;
            owl:allValuesFrom ocsf:string_t ],
        [ a owl:Restriction ;
            owl:onProperty ocsf:dce_rpc ;
            owl:allValuesFrom ocsf:DCERPC ],
        [ a owl:Restriction ;
            owl:onProperty ocsf:dialect ;
            owl:allValuesFrom ocsf:string_t ],
        [ a owl:Restriction ;
            owl:onProperty ocsf:file ;
            owl:allValuesFrom ocsf:File ],
        [ a owl:Restriction ;
            owl:onProperty ocsf:open_type ;
            owl:allValuesFrom ocsf:string_t ],
        [ a owl:Restriction ;
            owl:onProperty ocsf:response ;
            owl:allValuesFrom ocsf:ResponseElements ],
        [ a owl:Restriction ;
            owl:onProperty ocsf:share ;
            owl:allValuesFrom ocsf:string_t ],
        [ a owl:Restriction ;
            owl:onProperty ocsf:share_type ;
            owl:allValuesFrom ocsf:string_t ],
        [ a owl:Restriction ;
            owl:onProperty ocsf:share_type_id ;
            owl:allValuesFrom ocsf:integer_t ],
        [ a owl:Restriction ;
            owl:onProperty ocsf:tree_uid ;
            owl:allValuesFrom ocsf:string_t ] ;
    dcterms:description "Server Message Block (SMB) Protocol Activity events report client/server connections sharing resources within the network." ;
    ocsf:extends "network" ;
    ocsf:name "smb_activity" .

ocsf:SoftwareInventoryInfoEvent a owl:Class ;
    rdfs:label "Software Inventory Info" ;
    rdfs:subClassOf ocsf:DiscoveryEvent,
        [ a owl:Restriction ;
            owl:onProperty ocsf:actor ;
            owl:allValuesFrom ocsf:Actor ],
        [ a owl:Restriction ;
            owl:onProperty ocsf:device ;
            owl:allValuesFrom ocsf:Device ],
        [ a owl:Restriction ;
            owl:onProperty ocsf:device ;
            owl:someValuesFrom ocsf:Device ],
        [ a owl:Restriction ;
            owl:onProperty ocsf:package ;
            owl:allValuesFrom ocsf:SoftwarePackage ],
        [ a owl:Restriction ;
            owl:onProperty ocsf:package ;
            owl:someValuesFrom ocsf:SoftwarePackage ],
        [ a owl:Restriction ;
            owl:onProperty ocsf:product ;
            owl:allValuesFrom ocsf:Product ] ;
    dcterms:description "Software Inventory Info events report device software inventory data that is either logged or proactively collected. For example, when collecting device information from a CMDB or running a network sweep of connected devices." ;
    ocsf:extends "discovery" ;
    ocsf:name "software_info" ;
    ocsf:profiles "host" .

ocsf:SoftwarePackage a owl:Class ;
    rdfs:label "Software Package" ;
    rdfs:subClassOf ocsf:Object,
        [ a owl:Restriction ;
            owl:onProperty ocsf:architecture ;
            owl:allValuesFrom ocsf:string_t ],
        [ a owl:Restriction ;
            owl:onProperty ocsf:cpe_name ;
            owl:allValuesFrom ocsf:string_t ],
        [ a owl:Restriction ;
            owl:onProperty ocsf:epoch ;
            owl:allValuesFrom ocsf:integer_t ],
        [ a owl:Restriction ;
            owl:onProperty ocsf:hash ;
            owl:allValuesFrom ocsf:Fingerprint ],
        [ a owl:Restriction ;
            owl:onProperty ocsf:license ;
            owl:allValuesFrom ocsf:string_t ],
        [ a owl:Restriction ;
            owl:onProperty ocsf:name ;
            owl:allValuesFrom ocsf:string_t ],
        [ a owl:Restriction ;
            owl:onProperty ocsf:name ;
            owl:cardinality 1 ],
        [ a owl:Restriction ;
            owl:onProperty ocsf:purl ;
            owl:allValuesFrom ocsf:string_t ],
        [ a owl:Restriction ;
            owl:onProperty ocsf:release ;
            owl:allValuesFrom ocsf:string_t ],
        [ a owl:Restriction ;
            owl:onProperty ocsf:type ;
            owl:allValuesFrom ocsf:string_t ],
        [ a owl:Restriction ;
            owl:onProperty ocsf:type_id ;
            owl:allValuesFrom ocsf:integer_t ],
        [ a owl:Restriction ;
            owl:onProperty ocsf:vendor_name ;
            owl:allValuesFrom ocsf:string_t ],
        [ a owl:Restriction ;
            owl:onProperty ocsf:version ;
            owl:allValuesFrom ocsf:string_t ],
        [ a owl:Restriction ;
            owl:onProperty ocsf:version ;
            owl:cardinality 1 ] ;
    dcterms:description "The Software Package object describes details about a software package. Defined by D3FEND <a target='_blank' href='https://d3fend.mitre.org/dao/artifact/d3f:SoftwarePackage/'>d3f:SoftwarePackage</a>." ;
    ocsf:extends "object" ;
    ocsf:name "package" .

ocsf:SSHActivityEvent a owl:Class ;
    rdfs:label "SSH Activity" ;
    rdfs:subClassOf ocsf:NetworkEvent,
        [ a owl:Restriction ;
            owl:onProperty ocsf:auth_type ;
            owl:allValuesFrom ocsf:string_t ],
        [ a owl:Restriction ;
            owl:onProperty ocsf:auth_type_id ;
            owl:allValuesFrom ocsf:integer_t ],
        [ a owl:Restriction ;
            owl:onProperty ocsf:client_hassh ;
            owl:allValuesFrom ocsf:HASSH ],
        [ a owl:Restriction ;
            owl:onProperty ocsf:file ;
            owl:allValuesFrom ocsf:File ],
        [ a owl:Restriction ;
            owl:onProperty ocsf:protocol_ver ;
            owl:allValuesFrom ocsf:string_t ],
        [ a owl:Restriction ;
            owl:onProperty ocsf:server_hassh ;
            owl:allValuesFrom ocsf:HASSH ] ;
    dcterms:description "SSH Activity events report remote client connections to a server using the Secure Shell (SSH) Protocol." ;
    ocsf:extends "network" ;
    ocsf:name "ssh_activity" .

ocsf:SubjectAlternativeName a owl:Class ;
    rdfs:label "Subject Alternative Name" ;
    rdfs:subClassOf ocsf:Object,
        [ a owl:Restriction ;
            owl:onProperty ocsf:name ;
            owl:allValuesFrom ocsf:string_t ],
        [ a owl:Restriction ;
            owl:onProperty ocsf:name ;
            owl:cardinality 1 ],
        [ a owl:Restriction ;
            owl:onProperty ocsf:type ;
            owl:allValuesFrom ocsf:string_t ],
        [ a owl:Restriction ;
            owl:onProperty ocsf:type ;
            owl:cardinality 1 ] ;
    dcterms:description "The Subject Alternative name (SAN) object describes a SAN secured by a digital certificate" ;
    ocsf:extends "object" ;
    ocsf:name "san" .

ocsf:SystemActivityEvent a owl:Class ;
    rdfs:label "System Activity" ;
    rdfs:subClassOf ocsf:BaseEvent,
        [ a owl:Restriction ;
            owl:onProperty ocsf:actor ;
            owl:allValuesFrom ocsf:Actor ],
        [ a owl:Restriction ;
            owl:onProperty ocsf:actor ;
            owl:someValuesFrom ocsf:Actor ],
        [ a owl:Restriction ;
            owl:onProperty ocsf:device ;
            owl:allValuesFrom ocsf:Device ],
        [ a owl:Restriction ;
            owl:onProperty ocsf:device ;
            owl:someValuesFrom ocsf:Device ] ;
    dcterms:description "The System Activity event is a generic event that defines a set of attributes available in the system activity events. As a generic event, it could be used to log events that are not otherwise defined by the System Activity category." ;
    ocsf:associations "{\"device\":[\"actor.user\"],\"actor.user\":[\"device\"]}" ;
    ocsf:category ocsf:SystemActivityEvent ;
    ocsf:extends "base_event" ;
    ocsf:name "system" ;
    ocsf:profiles "host",
        "security_control" .

ocsf:SystemActivityEventCategory a owl:Class ;
    rdfs:label "System Activity" ;
    rdfs:subClassOf ocsf:EventCategory ;
    d3f:definition "System Activity events." ;
    ocsf:category_name "system" .

ocsf:Table a owl:Class ;
    rdfs:label "Table" ;
    rdfs:subClassOf ocsf:Entity,
        [ a owl:Restriction ;
            owl:onProperty ocsf:created_time ;
            owl:allValuesFrom ocsf:timestamp_t ],
        [ a owl:Restriction ;
            owl:onProperty ocsf:desc ;
            owl:allValuesFrom ocsf:string_t ],
        [ a owl:Restriction ;
            owl:onProperty ocsf:groups ;
            owl:allValuesFrom ocsf:Group ],
        [ a owl:Restriction ;
            owl:onProperty ocsf:modified_time ;
            owl:allValuesFrom ocsf:timestamp_t ],
        [ a owl:Restriction ;
            owl:onProperty ocsf:name ;
            owl:allValuesFrom ocsf:string_t ],
        [ a owl:Restriction ;
            owl:onProperty ocsf:size ;
            owl:allValuesFrom ocsf:long_t ],
        [ a owl:Restriction ;
            owl:onProperty ocsf:uid ;
            owl:allValuesFrom ocsf:string_t ] ;
    dcterms:description "The table object represents a table within a structured relational database or datastore, which contains columns and rows of data that are able to be create, updated, deleted and queried." ;
    ocsf:extends "_entity" ;
    ocsf:name "table" .

ocsf:Ticket a owl:Class ;
    rdfs:label "Ticket" ;
    rdfs:subClassOf ocsf:Object,
        [ a owl:Restriction ;
            owl:onProperty ocsf:src_url ;
            owl:allValuesFrom ocsf:url_t ],
        [ a owl:Restriction ;
            owl:onProperty ocsf:title ;
            owl:allValuesFrom ocsf:string_t ],
        [ a owl:Restriction ;
            owl:onProperty ocsf:type ;
            owl:allValuesFrom ocsf:string_t ],
        [ a owl:Restriction ;
            owl:onProperty ocsf:type_id ;
            owl:allValuesFrom ocsf:integer_t ],
        [ a owl:Restriction ;
            owl:onProperty ocsf:uid ;
            owl:allValuesFrom ocsf:string_t ] ;
    dcterms:description "The Ticket object represents ticket in the customer's systems like Salesforce, jira etc." ;
    ocsf:constraints "{\"at_least_one\":[\"src_url\",\"uid\"]}" ;
    ocsf:extends "object" ;
    ocsf:name "ticket" .

ocsf:TimeSpan a owl:Class ;
    rdfs:label "Time Span" ;
    rdfs:subClassOf ocsf:Object,
        [ a owl:Restriction ;
            owl:onProperty ocsf:duration ;
            owl:allValuesFrom ocsf:long_t ],
        [ a owl:Restriction ;
            owl:onProperty ocsf:duration_days ;
            owl:allValuesFrom ocsf:integer_t ],
        [ a owl:Restriction ;
            owl:onProperty ocsf:duration_hours ;
            owl:allValuesFrom ocsf:integer_t ],
        [ a owl:Restriction ;
            owl:onProperty ocsf:duration_mins ;
            owl:allValuesFrom ocsf:integer_t ],
        [ a owl:Restriction ;
            owl:onProperty ocsf:duration_months ;
            owl:allValuesFrom ocsf:integer_t ],
        [ a owl:Restriction ;
            owl:onProperty ocsf:duration_secs ;
            owl:allValuesFrom ocsf:integer_t ],
        [ a owl:Restriction ;
            owl:onProperty ocsf:duration_weeks ;
            owl:allValuesFrom ocsf:integer_t ],
        [ a owl:Restriction ;
            owl:onProperty ocsf:duration_years ;
            owl:allValuesFrom ocsf:integer_t ],
        [ a owl:Restriction ;
            owl:onProperty ocsf:type ;
            owl:allValuesFrom ocsf:string_t ],
        [ a owl:Restriction ;
            owl:onProperty ocsf:type_id ;
            owl:allValuesFrom ocsf:integer_t ] ;
    dcterms:description "The Time Span object represents different time period durations. If a timespan is fractional, i.e. crosses one period, e.g. a week and 3 days, more than one may may be populated since each member is of integral type. In that case <code>type_id</code> if present should be set to <code>Other</code>." ;
    ocsf:constraints "{\"at_least_one\":[\"duration\",\"duration_days\",\"duration_hours\",\"duration_mins\",\"duration_months\",\"duration_secs\",\"duration_weeks\",\"duration_years\"]}" ;
    ocsf:extends "object" ;
    ocsf:name "timespan" .

ocsf:TLSExtension a owl:Class ;
    rdfs:label "TLS Extension" ;
    rdfs:subClassOf ocsf:Object,
        [ a owl:Restriction ;
            owl:onProperty ocsf:data ;
            owl:allValuesFrom ocsf:json_t ],
        [ a owl:Restriction ;
            owl:onProperty ocsf:type ;
            owl:allValuesFrom ocsf:string_t ],
        [ a owl:Restriction ;
            owl:onProperty ocsf:type_id ;
            owl:allValuesFrom ocsf:integer_t ],
        [ a owl:Restriction ;
            owl:onProperty ocsf:type_id ;
            owl:cardinality 1 ] ;
    dcterms:description "The TLS Extension object describes additional attributes that extend the base Transport Layer Security (TLS) object." ;
    ocsf:extends "object" ;
    ocsf:name "tls_extension" .

ocsf:TransportLayerSecurityTLS a owl:Class ;
    rdfs:label "Transport Layer Security (TLS)" ;
    rdfs:subClassOf ocsf:Object,
        [ a owl:Restriction ;
            owl:onProperty ocsf:alert ;
            owl:allValuesFrom ocsf:integer_t ],
        [ a owl:Restriction ;
            owl:onProperty ocsf:certificate ;
            owl:allValuesFrom ocsf:DigitalCertificate ],
        [ a owl:Restriction ;
            owl:onProperty ocsf:certificate_chain ;
            owl:allValuesFrom ocsf:string_t ],
        [ a owl:Restriction ;
            owl:onProperty ocsf:cipher ;
            owl:allValuesFrom ocsf:string_t ],
        [ a owl:Restriction ;
            owl:onProperty ocsf:client_ciphers ;
            owl:allValuesFrom ocsf:string_t ],
        [ a owl:Restriction ;
            owl:onProperty ocsf:extension_list ;
            owl:allValuesFrom ocsf:TLSExtension ],
        [ a owl:Restriction ;
            owl:onProperty ocsf:handshake_dur ;
            owl:allValuesFrom ocsf:integer_t ],
        [ a owl:Restriction ;
            owl:onProperty ocsf:ja3_hash ;
            owl:allValuesFrom ocsf:Fingerprint ],
        [ a owl:Restriction ;
            owl:onProperty ocsf:ja3s_hash ;
            owl:allValuesFrom ocsf:Fingerprint ],
        [ a owl:Restriction ;
            owl:onProperty ocsf:key_length ;
            owl:allValuesFrom ocsf:integer_t ],
        [ a owl:Restriction ;
            owl:onProperty ocsf:sans ;
            owl:allValuesFrom ocsf:SubjectAlternativeName ],
        [ a owl:Restriction ;
            owl:onProperty ocsf:server_ciphers ;
            owl:allValuesFrom ocsf:string_t ],
        [ a owl:Restriction ;
            owl:onProperty ocsf:sni ;
            owl:allValuesFrom ocsf:string_t ],
        [ a owl:Restriction ;
            owl:onProperty ocsf:tls_extension_list ;
            owl:allValuesFrom ocsf:TLSExtension ],
        [ a owl:Restriction ;
            owl:onProperty ocsf:version ;
            owl:allValuesFrom ocsf:string_t ],
        [ a owl:Restriction ;
            owl:onProperty ocsf:version ;
            owl:cardinality 1 ] ;
    dcterms:description "The Transport Layer Security (TLS) object describes the negotiated TLS protocol used for secure communications over an establish network connection." ;
    ocsf:extends "object" ;
    ocsf:name "tls" .

ocsf:TunnelActivityEvent a owl:Class ;
    rdfs:label "Tunnel Activity" ;
    rdfs:subClassOf ocsf:NetworkEvent,
        [ a owl:Restriction ;
            owl:onProperty ocsf:activity_id ;
            owl:allValuesFrom ocsf:integer_t ],
        [ a owl:Restriction ;
            owl:onProperty ocsf:activity_id ;
            owl:cardinality 1 ],
        [ a owl:Restriction ;
            owl:onProperty ocsf:connection_info ;
            owl:allValuesFrom ocsf:NetworkConnectionInformation ],
        [ a owl:Restriction ;
            owl:onProperty ocsf:device ;
            owl:allValuesFrom ocsf:Device ],
        [ a owl:Restriction ;
            owl:onProperty ocsf:dst_endpoint ;
            owl:allValuesFrom ocsf:NetworkEndpoint ],
        [ a owl:Restriction ;
            owl:onProperty ocsf:protocol_name ;
            owl:allValuesFrom ocsf:string_t ],
        [ a owl:Restriction ;
            owl:onProperty ocsf:session ;
            owl:allValuesFrom ocsf:Session ],
        [ a owl:Restriction ;
            owl:onProperty ocsf:src_endpoint ;
            owl:allValuesFrom ocsf:NetworkEndpoint ],
        [ a owl:Restriction ;
            owl:onProperty ocsf:traffic ;
            owl:allValuesFrom ocsf:NetworkTraffic ],
        [ a owl:Restriction ;
            owl:onProperty ocsf:tunnel_interface ;
            owl:allValuesFrom ocsf:NetworkInterface ],
        [ a owl:Restriction ;
            owl:onProperty ocsf:tunnel_type ;
            owl:allValuesFrom ocsf:string_t ],
        [ a owl:Restriction ;
            owl:onProperty ocsf:tunnel_type_id ;
            owl:allValuesFrom ocsf:integer_t ],
        [ a owl:Restriction ;
            owl:onProperty ocsf:user ;
            owl:allValuesFrom ocsf:User ] ;
    dcterms:description "Tunnel Activity events report secure tunnel establishment (such as VPN), teardowns, renewals, and other network tunnel specific actions." ;
    ocsf:associations "{\"user\":[\"src_endpoint\"],\"src_endpoint\":[\"user\"]}" ;
    ocsf:category ocsf:NetworkEvent ;
    ocsf:constraints "{\"at_least_one\":[\"connection_info\",\"session\",\"src_endpoint\",\"traffic\",\"tunnel_interface\",\"tunnel_type_id\"]}" ;
    ocsf:extends "network" ;
    ocsf:name "tunnel_activity" .

ocsf:UniformResourceLocator a owl:Class ;
    rdfs:label "Uniform Resource Locator" ;
    rdfs:subClassOf ocsf:Object,
        [ a owl:Restriction ;
            owl:onProperty ocsf:categories ;
            owl:allValuesFrom ocsf:string_t ],
        [ a owl:Restriction ;
            owl:onProperty ocsf:category_ids ;
            owl:allValuesFrom ocsf:integer_t ],
        [ a owl:Restriction ;
            owl:onProperty ocsf:domain ;
            owl:allValuesFrom ocsf:string_t ],
        [ a owl:Restriction ;
            owl:onProperty ocsf:hostname ;
            owl:allValuesFrom ocsf:hostname_t ],
        [ a owl:Restriction ;
            owl:onProperty ocsf:path ;
            owl:allValuesFrom ocsf:string_t ],
        [ a owl:Restriction ;
            owl:onProperty ocsf:port ;
            owl:allValuesFrom ocsf:port_t ],
        [ a owl:Restriction ;
            owl:onProperty ocsf:query_string ;
            owl:allValuesFrom ocsf:string_t ],
        [ a owl:Restriction ;
            owl:onProperty ocsf:resource_type ;
            owl:allValuesFrom ocsf:string_t ],
        [ a owl:Restriction ;
            owl:onProperty ocsf:scheme ;
            owl:allValuesFrom ocsf:string_t ],
        [ a owl:Restriction ;
            owl:onProperty ocsf:subdomain ;
            owl:allValuesFrom ocsf:string_t ],
        [ a owl:Restriction ;
            owl:onProperty ocsf:url_string ;
            owl:allValuesFrom ocsf:url_t ] ;
    dcterms:description "The Uniform Resource Locator(URL) object describes the characteristics of a URL. Defined in <a target='_blank' href='https://datatracker.ietf.org/doc/html/rfc1738'>RFC 1738</a> and by D3FEND <a target='_blank' href='https://d3fend.mitre.org/dao/artifact/d3f:URL/'>d3f:URL</a>." ;
    ocsf:constraints "{\"at_least_one\":[\"url_string\",\"path\"]}" ;
    ocsf:extends "object" ;
    ocsf:name "url" .

ocsf:User a owl:Class ;
    rdfs:label "User" ;
    rdfs:subClassOf ocsf:Entity,
        [ a owl:Restriction ;
            owl:onProperty ocsf:account ;
            owl:allValuesFrom ocsf:Account ],
        [ a owl:Restriction ;
            owl:onProperty ocsf:credential_uid ;
            owl:allValuesFrom ocsf:string_t ],
        [ a owl:Restriction ;
            owl:onProperty ocsf:domain ;
            owl:allValuesFrom ocsf:string_t ],
        [ a owl:Restriction ;
            owl:onProperty ocsf:email_addr ;
            owl:allValuesFrom ocsf:email_t ],
        [ a owl:Restriction ;
            owl:onProperty ocsf:full_name ;
            owl:allValuesFrom ocsf:string_t ],
        [ a owl:Restriction ;
            owl:onProperty ocsf:groups ;
            owl:allValuesFrom ocsf:Group ],
        [ a owl:Restriction ;
            owl:onProperty ocsf:ldap_person ;
            owl:allValuesFrom ocsf:LDAPPerson ],
        [ a owl:Restriction ;
            owl:onProperty ocsf:name ;
            owl:allValuesFrom ocsf:string_t ],
        [ a owl:Restriction ;
            owl:onProperty ocsf:org ;
            owl:allValuesFrom ocsf:Organization ],
        [ a owl:Restriction ;
            owl:onProperty ocsf:risk_level ;
            owl:allValuesFrom ocsf:string_t ],
        [ a owl:Restriction ;
            owl:onProperty ocsf:risk_level_id ;
            owl:allValuesFrom ocsf:integer_t ],
        [ a owl:Restriction ;
            owl:onProperty ocsf:risk_score ;
            owl:allValuesFrom ocsf:integer_t ],
        [ a owl:Restriction ;
            owl:onProperty ocsf:type ;
            owl:allValuesFrom ocsf:string_t ],
        [ a owl:Restriction ;
            owl:onProperty ocsf:type_id ;
            owl:allValuesFrom ocsf:integer_t ],
        [ a owl:Restriction ;
            owl:onProperty ocsf:uid ;
            owl:allValuesFrom ocsf:string_t ],
        [ a owl:Restriction ;
            owl:onProperty ocsf:uid_alt ;
            owl:allValuesFrom ocsf:string_t ] ;
    dcterms:description "The User object describes the characteristics of a user/person or a security principal. Defined by D3FEND <a target='_blank' href='https://d3fend.mitre.org/dao/artifact/d3f:UserAccount/'>d3f:UserAccount</a>." ;
    ocsf:constraints "{\"at_least_one\":[\"account\",\"name\",\"uid\"]}" ;
    ocsf:extends "_entity" ;
    ocsf:name "user" .

ocsf:UserAccessManagementEvent a owl:Class ;
    rdfs:label "User Access Management" ;
    rdfs:subClassOf ocsf:IdentityAccessManagementEvent,
        [ a owl:Restriction ;
            owl:onProperty ocsf:activity_id ;
            owl:allValuesFrom ocsf:integer_t ],
        [ a owl:Restriction ;
            owl:onProperty ocsf:privileges ;
            owl:allValuesFrom ocsf:string_t ],
        [ a owl:Restriction ;
            owl:onProperty ocsf:privileges ;
            owl:cardinality 1 ],
        [ a owl:Restriction ;
            owl:onProperty ocsf:resource ;
            owl:allValuesFrom ocsf:ResourceDetails ],
        [ a owl:Restriction ;
            owl:onProperty ocsf:user ;
            owl:allValuesFrom ocsf:User ],
        [ a owl:Restriction ;
            owl:onProperty ocsf:user ;
            owl:someValuesFrom ocsf:User ] ;
    dcterms:description "User Access Management events report management updates to a user's privileges." ;
    ocsf:extends "iam" ;
    ocsf:name "user_access" .

ocsf:UserInventoryInfoEvent a owl:Class ;
    rdfs:label "User Inventory Info" ;
    rdfs:subClassOf ocsf:DiscoveryEvent,
        [ a owl:Restriction ;
            owl:onProperty ocsf:actor ;
            owl:allValuesFrom ocsf:Actor ],
        [ a owl:Restriction ;
            owl:onProperty ocsf:user ;
            owl:allValuesFrom ocsf:User ],
        [ a owl:Restriction ;
            owl:onProperty ocsf:user ;
            owl:someValuesFrom ocsf:User ] ;
    dcterms:description "User Inventory Info events report user inventory data that is either logged or proactively collected. For example, when collecting user information from Active Directory entries." ;
    ocsf:extends "discovery" ;
    ocsf:name "user_inventory" .

ocsf:UserQueryEvent a owl:Class ;
    rdfs:label "User Query" ;
    rdfs:subClassOf ocsf:DiscoveryResultEvent,
        [ a owl:Restriction ;
            owl:onProperty ocsf:user ;
            owl:allValuesFrom ocsf:User ],
        [ a owl:Restriction ;
            owl:onProperty ocsf:user ;
            owl:someValuesFrom ocsf:User ] ;
    dcterms:description "User Query events report user data that have been discovered, queried, polled or searched. This event differs from User Inventory as it describes the result of a targeted search by filtering a subset of user attributes." ;
    ocsf:extends "discovery_result" ;
    ocsf:name "user_query" .

ocsf:UserSessionQueryEvent a owl:Class ;
    rdfs:label "User Session Query" ;
    rdfs:subClassOf ocsf:DiscoveryResultEvent,
        [ a owl:Restriction ;
            owl:onProperty ocsf:session ;
            owl:allValuesFrom ocsf:Session ],
        [ a owl:Restriction ;
            owl:onProperty ocsf:session ;
            owl:someValuesFrom ocsf:Session ] ;
    dcterms:description "User Session Query events report information about existing user sessions." ;
    ocsf:extends "discovery_result" ;
    ocsf:name "session_query" .

ocsf:VulnerabilityDetails a owl:Class ;
    rdfs:label "Vulnerability Details" ;
    rdfs:subClassOf ocsf:Object,
        [ a owl:Restriction ;
            owl:onProperty ocsf:affected_code ;
            owl:allValuesFrom ocsf:AffectedCode ],
        [ a owl:Restriction ;
            owl:onProperty ocsf:affected_packages ;
            owl:allValuesFrom ocsf:AffectedSoftwarePackage ],
        [ a owl:Restriction ;
            owl:onProperty ocsf:cve ;
            owl:allValuesFrom ocsf:CVE ],
        [ a owl:Restriction ;
            owl:onProperty ocsf:cwe ;
            owl:allValuesFrom ocsf:CWE ],
        [ a owl:Restriction ;
            owl:onProperty ocsf:desc ;
            owl:allValuesFrom ocsf:string_t ],
        [ a owl:Restriction ;
            owl:onProperty ocsf:first_seen_time ;
            owl:allValuesFrom ocsf:timestamp_t ],
        [ a owl:Restriction ;
            owl:onProperty ocsf:fix_available ;
            owl:allValuesFrom ocsf:boolean_t ],
        [ a owl:Restriction ;
            owl:onProperty ocsf:is_exploit_available ;
            owl:allValuesFrom ocsf:boolean_t ],
        [ a owl:Restriction ;
            owl:onProperty ocsf:is_fix_available ;
            owl:allValuesFrom ocsf:boolean_t ],
        [ a owl:Restriction ;
            owl:onProperty ocsf:kb_article_list ;
            owl:allValuesFrom ocsf:KBArticle ],
        [ a owl:Restriction ;
            owl:onProperty ocsf:kb_articles ;
            owl:allValuesFrom ocsf:string_t ],
        [ a owl:Restriction ;
            owl:onProperty ocsf:last_seen_time ;
            owl:allValuesFrom ocsf:timestamp_t ],
        [ a owl:Restriction ;
            owl:onProperty ocsf:packages ;
            owl:allValuesFrom ocsf:SoftwarePackage ],
        [ a owl:Restriction ;
            owl:onProperty ocsf:references ;
            owl:allValuesFrom ocsf:string_t ],
        [ a owl:Restriction ;
            owl:onProperty ocsf:related_vulnerabilities ;
            owl:allValuesFrom ocsf:string_t ],
        [ a owl:Restriction ;
            owl:onProperty ocsf:remediation ;
            owl:allValuesFrom ocsf:Remediation ],
        [ a owl:Restriction ;
            owl:onProperty ocsf:severity ;
            owl:allValuesFrom ocsf:string_t ],
        [ a owl:Restriction ;
            owl:onProperty ocsf:title ;
            owl:allValuesFrom ocsf:string_t ],
        [ a owl:Restriction ;
            owl:onProperty ocsf:vendor_name ;
            owl:allValuesFrom ocsf:string_t ] ;
    dcterms:description "The vulnerability is an unintended characteristic of a computing component or system configuration that multiplies the risk of an adverse event or a loss occurring either due to accidental exposure, deliberate attack, or conflict with new system components." ;
    ocsf:constraints "{\"at_least_one\":[\"cve\",\"cwe\"]}" ;
    ocsf:extends "object" ;
    ocsf:name "vulnerability" .

ocsf:VulnerabilityFindingEvent a owl:Class ;
    rdfs:label "Vulnerability Finding" ;
    rdfs:subClassOf ocsf:Finding,
        ocsf:FindingEvent,
        [ a owl:Restriction ;
            owl:onProperty ocsf:resource ;
            owl:allValuesFrom ocsf:ResourceDetails ],
        [ a owl:Restriction ;
            owl:onProperty ocsf:resources ;
            owl:allValuesFrom ocsf:ResourceDetails ],
        [ a owl:Restriction ;
            owl:onProperty ocsf:vulnerabilities ;
            owl:allValuesFrom ocsf:VulnerabilityDetails ],
        [ a owl:Restriction ;
            owl:onProperty ocsf:vulnerabilities ;
            owl:someValuesFrom ocsf:VulnerabilityDetails ] ;
    dcterms:description "The Vulnerability Finding event is a notification about weakness in an information system, system security procedures, internal controls, or implementation that could be exploited or triggered by a threat source." ;
    ocsf:extends "finding" ;
    ocsf:name "vulnerability_finding" .

ocsf:WebResource a owl:Class ;
    rdfs:label "Web Resource" ;
    rdfs:subClassOf ocsf:Resource,
        [ a owl:Restriction ;
            owl:onProperty ocsf:data ;
            owl:allValuesFrom ocsf:json_t ],
        [ a owl:Restriction ;
            owl:onProperty ocsf:desc ;
            owl:allValuesFrom ocsf:string_t ],
        [ a owl:Restriction ;
            owl:onProperty ocsf:name ;
            owl:allValuesFrom ocsf:string_t ],
        [ a owl:Restriction ;
            owl:onProperty ocsf:type ;
            owl:allValuesFrom ocsf:string_t ],
        [ a owl:Restriction ;
            owl:onProperty ocsf:uid ;
            owl:allValuesFrom ocsf:string_t ],
        [ a owl:Restriction ;
            owl:onProperty ocsf:url_string ;
            owl:allValuesFrom ocsf:url_t ] ;
    dcterms:description "The Web Resource object describes characteristics of a web resource that was affected by the activity/event." ;
    ocsf:extends "_resource" ;
    ocsf:name "web_resource" .

ocsf:WebResourceAccessActivityEvent a owl:Class ;
    rdfs:label "Web Resource Access Activity" ;
    rdfs:subClassOf ocsf:ApplicationActivityEvent,
        [ a owl:Restriction ;
            owl:onProperty ocsf:activity_id ;
            owl:allValuesFrom ocsf:integer_t ],
        [ a owl:Restriction ;
            owl:onProperty ocsf:http_request ;
            owl:allValuesFrom ocsf:HTTPRequest ],
        [ a owl:Restriction ;
            owl:onProperty ocsf:http_request ;
            owl:someValuesFrom ocsf:HTTPRequest ],
        [ a owl:Restriction ;
            owl:onProperty ocsf:http_response ;
            owl:allValuesFrom ocsf:HTTPResponse ],
        [ a owl:Restriction ;
            owl:onProperty ocsf:proxy ;
            owl:allValuesFrom ocsf:NetworkProxyEndpoint ],
        [ a owl:Restriction ;
            owl:onProperty ocsf:src_endpoint ;
            owl:allValuesFrom ocsf:NetworkEndpoint ],
        [ a owl:Restriction ;
            owl:onProperty ocsf:tls ;
            owl:allValuesFrom ocsf:TransportLayerSecurityTLS ],
        [ a owl:Restriction ;
            owl:onProperty ocsf:web_resources ;
            owl:allValuesFrom ocsf:WebResource ],
        [ a owl:Restriction ;
            owl:onProperty ocsf:web_resources ;
            owl:someValuesFrom ocsf:WebResource ] ;
    dcterms:description "Web Resource Access Activity events describe successful/failed attempts to access a web resource over HTTP." ;
    ocsf:category ocsf:ApplicationActivityEvent ;
    ocsf:extends "application" ;
    ocsf:name "web_resource_access_activity" ;
    ocsf:profiles "host",
        "network_proxy" .

ocsf:WebResourcesActivityEvent a owl:Class ;
    rdfs:label "Web Resources Activity" ;
    rdfs:subClassOf ocsf:BaseEvent,
        [ a owl:Restriction ;
            owl:onProperty ocsf:activity_id ;
            owl:allValuesFrom ocsf:integer_t ],
        [ a owl:Restriction ;
            owl:onProperty ocsf:dst_endpoint ;
            owl:allValuesFrom ocsf:NetworkEndpoint ],
        [ a owl:Restriction ;
            owl:onProperty ocsf:http_request ;
            owl:allValuesFrom ocsf:HTTPRequest ],
        [ a owl:Restriction ;
            owl:onProperty ocsf:http_response ;
            owl:allValuesFrom ocsf:HTTPResponse ],
        [ a owl:Restriction ;
            owl:onProperty ocsf:src_endpoint ;
            owl:allValuesFrom ocsf:NetworkEndpoint ],
        [ a owl:Restriction ;
            owl:onProperty ocsf:tls ;
            owl:allValuesFrom ocsf:TransportLayerSecurityTLS ],
        [ a owl:Restriction ;
            owl:onProperty ocsf:web_resources ;
            owl:allValuesFrom ocsf:WebResource ],
        [ a owl:Restriction ;
            owl:onProperty ocsf:web_resources ;
            owl:someValuesFrom ocsf:WebResource ],
        [ a owl:Restriction ;
            owl:onProperty ocsf:web_resources_result ;
            owl:allValuesFrom ocsf:WebResource ] ;
    dcterms:description "Web Resources Activity events describe actions executed on a set of Web Resources." ;
    ocsf:category ocsf:ApplicationActivityEvent ;
    ocsf:extends "base_event" ;
    ocsf:name "web_resources_activity" ;
    ocsf:profiles "host",
        "network_proxy",
        "security_control" .

ocsf:WHOIS a owl:Class ;
    rdfs:label "WHOIS" ;
    rdfs:subClassOf ocsf:Object ;
    dcterms:description "The resources of a WHOIS record for a given domain. This can include domain names, IP address blocks, autonomous system information, and/or contact and registration information for a domain." ;
    ocsf:extends "object" ;
    ocsf:name "whois" .

### Serialized using the ttlser deterministic serializer v1.2.1
